format-version: 1.2
subsetdef: upper_level "upper level ontology"
ontology: ecosim

[Term]
id: ECOSIM:AKSGL
name: aqueous K diffusivity
def: "Aqueous K diffusivity refers to the measure of the rate at which potassium (K) ions migrate or spread through water or an aqueous medium. It represents the ability of K ions to move and mix within a water system. Aqueous K diffusivity is an important parameter in earth systems modeling as it plays a crucial role in understanding nutrient cycling, plant nutrition, and the movement of pollutants in aquatic environments." []
is_a: ECOSIM:CATEGORYHydrology ! category - Hydrology
is_a: ECOSIMCONCEPT:UnclassifiedVariable ! unclassified variable
relationship: attribute ECOSIMCONCEPT:Diffusivity ! Diffusivity
relationship: has_unit ECOSIM:m2h-1 ! m2 h-1
relationship: measured_in ECOSIMCONCEPT:Water ! Water
relationship: measurement_of ECOSIMCONCEPT:Potassium ! Potassium
relationship: qualifier ECOSIMCONCEPT:Aqueous ! Aqueous

[Term]
id: ECOSIM:ALSGL
name: aqueous Al diffusivity
def: "Aqueous Al diffusivity refers to the parameter that quantifies the rate at which aluminum (Al) ions diffuse through water. It is a measure of how quickly Al ions can move from one location to another in an aqueous environment. This parameter is important in Earth system modeling as it affects the transport and distribution of Al in aquatic systems, which in turn can have significant impacts on water quality, nutrient cycling, and the health of aquatic ecosystems." []
is_a: ECOSIM:CATEGORYHydrology ! category - Hydrology
is_a: ECOSIMCONCEPT:UnclassifiedVariable ! unclassified variable
relationship: attribute ECOSIMCONCEPT:Diffusivity ! Diffusivity
relationship: has_unit ECOSIM:m2h-1 ! m2 h-1
relationship: measured_in ECOSIMCONCEPT:Water ! Water
relationship: measurement_of ECOSIMCONCEPT:Aluminium ! Aluminium
relationship: qualifier ECOSIMCONCEPT:Aqueous ! Aqueous

[Term]
id: ECOSIM:ALT
name: altitude of grid cell
def: "The altitude of a grid cell refers to the vertical distance between the surface of the Earth and a specific point within the grid cell. It is a parameter used in earth systems modeling to account for the variation in elevation across different regions. Altitude plays a crucial role in determining temperature, precipitation patterns, atmospheric pressure, and other important climate variables within a grid cell." []
is_a: ECOSIM:CATEGORYAtmosphericConditions ! category - Atmospheric Conditions
relationship: attribute ECOSIMCONCEPT:Altitude ! Altitude
relationship: has_unit ECOSIM:m ! m
relationship: measured_in ECOSIMCONCEPT:GridCell ! GridCell
relationship: measurement_of ECOSIMCONCEPT:Altitude ! Altitude

[Term]
id: ECOSIM:ALTI
name: altitude of landscape
def: "The altitude of a landscape refers to the vertical distance between a specific point on the Earth's surface and a reference point, usually sea level. It is an important parameter in Earth system modeling as it influences a wide range of physical and biological processes, including temperature, precipitation patterns, atmospheric circulation, and distribution of plant and animal species. Altitude is typically measured in meters or feet and is essential for accurately simulating and analyzing the behavior and interactions of Earth's systems." []
is_a: ECOSIM:CATEGORYAtmosphericConditions ! category - Atmospheric Conditions
relationship: attribute ECOSIMCONCEPT:Altitude ! Altitude
relationship: has_unit ECOSIM:m ! m
relationship: measured_in ECOSIMCONCEPT:Landscape ! Landscape

[Term]
id: ECOSIM:ALTZ
name: altitude
def: "Altitude is a parameter that represents the vertical distance of a location above or below a reference point, typically sea level. It is an important parameter in Earth systems modeling as it influences various climatic factors such as temperature, atmospheric pressure, and precipitation. Altitude also impacts the distribution of plants and animals, and is used to define different ecological zones." []
is_a: ECOSIM:CATEGORYAtmosphericConditions ! category - Atmospheric Conditions
relationship: attribute ECOSIMCONCEPT:Altitude ! Altitude
relationship: has_unit ECOSIM:m ! m
relationship: measurement_of ECOSIMCONCEPT:Altitude ! Altitude

[Term]
id: ECOSIM:ANGBR
name: branching angle
def: "Branching angle refers to the angle between the main stem and a branch in a hierarchical tree structure. It is a parameter used in earth systems modeling to describe the architectural characteristics of vegetation, particularly in forest ecosystems. The branching angle affects the distribution of light within the canopy, which in turn influences the photosynthetic capacity and resource allocation of individual plants, as well as the overall structure and function of the ecosystem. Different values of branching angle can result in variations in light interception, crown architecture, and competitive interactions among plants, ultimately influencing ecosystem productivity and carbon cycling." []
is_a: ECOSIM:CATEGORYCanopyStructure ! category - canopy structure
relationship: has_unit ECOSIM:degreefromhorizontal ! degree from horizontal
relationship: measured_in ECOSIMCONCEPT:Plant ! Plant

[Term]
id: ECOSIM:ANGSH
name: sheath angle
def: "The sheath angle refers to the angle between the stem or branch and the leaf sheath in plants. It is an important parameter in earth systems modeling as it affects the canopy structure and influences various processes such as light interception, transpiration, and carbon assimilation. The sheath angle can vary between different plant species and can be influenced by environmental factors such as light availability and competition for resources." []
is_a: ECOSIM:CATEGORYCanopyStructure ! category - canopy structure
relationship: has_unit ECOSIM:degreefromhorizontal ! degree from horizontal
relationship: measured_in ECOSIMCONCEPT:Plant ! Plant
relationship: measurement_of ECOSIMCONCEPT:Sheath ! Sheath

[Term]
id: ECOSIM:ANSGL
name: aqueous Na diffusivity
def: "Aqueous Na diffusivity refers to the measure of the ability of sodium ions (Na+) to move or disperse within an aqueous environment. It quantifies the rate at which these ions can diffuse through the water, indicating how quickly and easily they can spread and mix with other substances or across different compartments of an ecosystem. This parameter is crucial in Earth systems modeling as it influences various processes such as chemical reactions, nutrient transport, and the behavior of Na+ in aquatic environments." []
is_a: ECOSIM:CATEGORYHydrology ! category - Hydrology
is_a: ECOSIMCONCEPT:UnclassifiedVariable ! unclassified variable
relationship: attribute ECOSIMCONCEPT:Diffusivity ! Diffusivity
relationship: has_unit ECOSIM:m2h-1 ! m2 h-1
relationship: measured_in ECOSIMCONCEPT:Water ! Water
relationship: measurement_of ECOSIMCONCEPT:Sodium ! Sodium
relationship: qualifier ECOSIMCONCEPT:Aqueous ! Aqueous

[Term]
id: ECOSIM:ARLF
name: leaf area
def: "Leaf area refers to the total surface area of leaves within a defined ecological system. It is a critical parameter in Earth systems modeling as it directly influences various processes such as photosynthesis, transpiration, and energy exchange between the vegetation and the atmosphere. Leaf area is typically measured in square meters per unit land area and is an important factor for characterizing ecosystem productivity, biodiversity, and carbon cycling." []
is_a: ECOSIM:CATEGORYCanopyStructure ! category - canopy structure
is_a: ECOSIM:CATEGORYPlantPhysiology ! category - plant physiology
relationship: attribute ECOSIMCONCEPT:Area ! Area
relationship: has_unit ECOSIM:m2d-2 ! m2 d-2
relationship: measured_in ECOSIMCONCEPT:Plant ! Plant
relationship: measurement_of ECOSIMCONCEPT:Leaf ! Leaf

[Term]
id: ECOSIM:ARLFX
name: total canopy leaf area
def: "Total canopy leaf area refers to the sum of the surface area of all the leaves within the canopy of a vegetation system. It is a parameter that quantifies the amount of foliage and is an essential characteristic for modeling the exchange of energy, carbon dioxide, and water between the vegetation and the atmosphere." []
is_a: ECOSIM:CATEGORYCanopyStructure ! category - canopy structure
is_a: ECOSIM:CATEGORYPlantPhysiology ! category - plant physiology
relationship: has_unit ECOSIM:m2d-2 ! m2 d-2
relationship: measured_in ECOSIMCONCEPT:Canopy ! Canopy
relationship: measurement_of ECOSIMCONCEPT:LeafArea ! LeafArea

[Term]
id: ECOSIM:ARLFZ
name: branch leaf area
def: "Branch leaf area refers to the total surface area covered by leaves on the branches of a plant or tree. It is an important parameter in earth systems modeling as it influences various processes such as photosynthesis, transpiration, and energy exchange with the atmosphere. The accurate representation of branch leaf area is crucial for accurately simulating carbon and water fluxes at the plant and ecosystem scale." []
is_a: ECOSIM:CATEGORYCanopyStructure ! category - canopy structure
is_a: ECOSIM:CATEGORYPlantPhysiology ! category - plant physiology
relationship: attribute ECOSIMCONCEPT:Area ! Area
relationship: has_unit ECOSIM:m2d-2 ! m2 d-2
relationship: measured_in ECOSIMCONCEPT:Branch ! Branch
relationship: measurement_of ECOSIMCONCEPT:Leaf ! Leaf

[Term]
id: ECOSIM:ARSTX
name: total canopy stem area
def: "Total canopy stem area refers to the combined surface area of all the stems and trunks within the canopy of a vegetation system. It is a parameter used in earth systems modeling to quantify the amount of photosynthetic surface available for biomass production and transpiration within a specific area. Canopy stem area is an important factor that influences energy and water exchange between the terrestrial vegetation and the atmosphere, as well as the overall functioning and productivity of an ecosystem." []
is_a: ECOSIM:CATEGORYCanopyStructure ! category - canopy structure
relationship: attribute ECOSIMCONCEPT:Area ! Area
relationship: has_unit ECOSIM:m2d-2 ! m2 d-2
relationship: measured_in ECOSIMCONCEPT:Canopy ! Canopy
relationship: measurement_of ECOSIMCONCEPT:Stem ! Stem

[Term]
id: ECOSIM:ASP
name: aspect
def: "Aspect refers to the spatial orientation or direction in which a land surface or geographical feature faces. It is typically expressed in terms of compass directions, such as north, south, east, or west. Aspect plays a significant role in various earth system processes, such as solar radiation patterns, temperature distribution, and vegetation growth. It is an important parameter in earth systems modeling as it affects the spatial distribution of climate variables and influences ecosystem dynamics at local and regional scales." []
is_a: ECOSIM:CATEGORYAtmosphericConditions ! category - Atmospheric Conditions
relationship: has_unit ECOSIM:o ! o
relationship: measurement_of ECOSIMCONCEPT:LandSurface ! LandSurface

[Term]
id: ECOSIM:ATCA
name: mean annual air temperature
def: "The mean annual air temperature refers to the average temperature of the atmosphere over a year, calculated by summing the daily temperatures and dividing by the number of days. It is an essential parameter for Earth systems modeling and provides important information about the climate conditions of a region. The mean annual air temperature is influenced by various factors, including solar radiation, land surface characteristics, and atmospheric conditions. It is used in various Earth systems models to understand and predict the behavior of the climate system, such as temperature variations, weather patterns, and climate change." []
is_a: ECOSIM:CATEGORYAtmosphericConditions ! category - Atmospheric Conditions
is_a: ECOSIMCONCEPT:UnclassifiedVariable ! unclassified variable
relationship: attribute ECOSIMCONCEPT:Temperature ! temperature
relationship: has_unit ECOSIM:oC ! oC
relationship: measured_in ECOSIMCONCEPT:Atmosphere ! Atmosphere

[Term]
id: ECOSIM:ATCAI
name: initial mean annual air temperature
def: "The initial mean annual air temperature refers to the average temperature of the atmosphere over a year at the beginning of a simulation or modeling scenario for Earth systems. It represents the starting point for evaluating the impact of various environmental factors on temperature trends and patterns. This parameter is essential for understanding climate change, analyzing atmospheric processes, and studying the broader interactions of Earth's systems. It serves as a crucial input for earth systems models and simulations to simulate and predict future climate conditions." []
is_a: ECOSIM:CATEGORYAtmosphericConditions ! category - Atmospheric Conditions
is_a: ECOSIMCONCEPT:UnclassifiedVariable ! unclassified variable
relationship: attribute ECOSIMCONCEPT:Temperature ! temperature
relationship: has_unit ECOSIM:oC ! oC

[Term]
id: ECOSIM:ATCS
name: mean annual soil temperature
def: "Mean annual soil temperature refers to the average temperature of the soil throughout the year. It is a parameter used in earth systems modeling to understand and simulate the thermal conditions of the soil. The mean annual soil temperature is an important factor that influences various soil processes and dynamics, including nutrient availability, microbial activity, and plant growth. It is typically measured at a certain depth below the surface and is influenced by factors such as climate, vegetation cover, and soil properties." []
is_a: ECOSIM:CATEGORYSoilBiogeochemistry ! category - Soil Biogeochemistry
is_a: ECOSIMCONCEPT:UnclassifiedVariable ! unclassified variable
relationship: attribute ECOSIMCONCEPT:Temperature ! temperature
relationship: has_unit ECOSIM:oC ! oC
relationship: measured_in ECOSIMCONCEPT:Soil ! Soil

[Term]
id: ECOSIM:ATKS
name: mean annual soil temperature
def: "Mean annual soil temperature refers to the average temperature of the soil throughout the year. It is typically measured at a specific depth, such as 10 cm below the surface. Mean annual soil temperature is an important parameter in earth system modeling as it influences the biological activity, nutrient availability, and carbon cycling in the soil. It is influenced by factors such as solar radiation, air temperature, soil moisture, and the thermal properties of the soil." []
is_a: ECOSIM:CATEGORYSoilBiogeochemistry ! category - Soil Biogeochemistry
is_a: ECOSIMCONCEPT:UnclassifiedVariable ! unclassified variable
relationship: attribute ECOSIMCONCEPT:Temperature ! temperature
relationship: has_unit ECOSIM:K ! K
relationship: measurement_of ECOSIMCONCEPT:Soil ! Soil

[Term]
id: ECOSIM:ActiveLayDepth
name: active layer depth
def: "Active layer depth is the thickness of the uppermost layer of soil or permafrost that undergoes seasonal freezing and thawing. It is defined as the vertical distance from the ground surface to the base of the active layer, which is the depth at which freezing and thawing processes no longer occur. The active layer depth is an important parameter in Earth Systems Modeling as it plays a key role in regulating the exchange of heat and moisture between the atmosphere and the underlying soil or permafrost. It is influenced by factors such as air temperature, soil properties, vegetation cover, and snow accumulation." []
is_a: ECOSIMCONCEPT:UnclassifiedVariable ! unclassified variable
relationship: has_unit ECOSIM:m ! m

[Term]
id: ECOSIM:AllPlantRootH2OUptake_vr
name: root water uptake
def: "Root water uptake refers to the process by which plant roots extract water from the soil. It is a vital parameter in earth systems modeling as it influences the distribution and availability of water in terrestrial ecosystems. Root water uptake is influenced by various factors such as soil moisture content, plant root characteristics, and environmental conditions. It is essential for accurately simulating the water cycle and understanding the dynamics of plant-water interactions in ecosystem models." []
is_a: ECOSIM:CATEGORYHydrology ! category - Hydrology
is_a: ECOSIMCONCEPT:UnclassifiedVariable ! unclassified variable
relationship: attribute ECOSIMCONCEPT:Uptake ! Uptake
relationship: has_unit ECOSIM:m2d-2h-1 ! m2 d-2 h-1
relationship: measured_in ECOSIMCONCEPT:Root ! Root
relationship: measurement_of ECOSIMCONCEPT:Water ! Water

[Term]
id: ECOSIM:AveSecndRootLen
name: root layer average length
def: "The term 'root layer average length' refers to the average length of roots within a specific layer of soil. It is a parameter used in earth systems modeling to characterize the size and distribution of roots in the soil profile. This parameter influences various processes such as nutrient uptake, water absorption, and carbon allocation, and can affect the overall productivity and stability of terrestrial ecosystems." []
is_a: ECOSIM:CATEGORYRootPhysiology ! category - root physiology
relationship: has_unit ECOSIM:m ! m

[Term]
id: ECOSIM:BALE
name: plant element balance
def: "Plant element balance refers to the equilibrium between the input and output of essential elements within the plant system. It describes the processes of absorption, translocation, utilization, and accumulation of nutrients such as carbon, oxygen, hydrogen, nitrogen, phosphorus, and potassium by plants. This balance is crucial for the growth, development, and overall health of plants, as it directly impacts their physiological functions and metabolic processes. Understanding and modeling plant element balance is essential for studying plant responses to environmental changes and optimizing agricultural practices and productivity." []
is_a: ECOSIM:CATEGORYPlantPhysiology ! category - plant physiology
is_a: ECOSIMCONCEPT:UnclassifiedVariable ! unclassified variable
relationship: has_unit ECOSIM:gd-2 ! g d-2
relationship: measurement_of ECOSIMCONCEPT:PlantElement ! PlantElement

[Term]
id: ECOSIM:BiomGrowthYieldRoot
name: root growth yield
def: "Root growth yield refers to the productivity of biomass accumulation in the roots of plants, expressed as the amount of new root biomass produced per unit of resource input, such as water, nutrients, or carbon dioxide. It represents the efficiency of plants in utilizing resources for root growth and plays a crucial role in the overall productivity and nutrient cycling within terrestrial ecosystems. Root growth yield is a key parameter in Earth system models as it influences the carbon and nutrient dynamics in soils, water uptake, and the overall functioning of ecosystems." []
is_a: ECOSIM:CATEGORYRootPhysiology ! category - root physiology
relationship: has_unit ECOSIM:gg-1 ! g g-1
relationship: measurement_of ECOSIMCONCEPT:Root ! Root

[Term]
id: ECOSIM:BndlResistAboveCanG
name: isothermal boundary layer resistance
def: "Isothermal boundary layer resistance refers to the measure of resistance that a uniform and constant temperature boundary layer imposes on the exchange of heat and moisture between the surface and the atmosphere in Earth system models. It quantifies the hindrance that the boundary layer presents to the transport and mixing of energy and water vapor, which can significantly influence the surface energy balance and atmospheric processes. This parameter is particularly relevant for simulating and understanding the interactions between the land surface and the lower atmosphere within Earth system models." []
is_a: ECOSIMCONCEPT:UnclassifiedVariable ! unclassified variable
relationship: has_unit ECOSIM:hm-1 ! h m-1

[Term]
id: ECOSIM:BndlResistCanG
name: canopy boundary layer resistance
def: "Canopy boundary layer resistance refers to the hindrance or resistance encountered by the exchange of heat, moisture, and gas between the surface of the Earth and the vegetation canopy. It represents the resistance to the transfer of these variables caused by the layer of still air that exists in the immediate vicinity of the canopy. Canopy boundary layer resistance is an important parameter in earth systems modeling as it influences the exchange rates of energy, water, and gases, such as carbon dioxide and oxygen, between the land and the atmosphere." []
is_a: ECOSIM:CATEGORYPlantPhysiology ! category - plant physiology
relationship: has_unit ECOSIM:mh-1 ! m h-1
relationship: measured_in ECOSIMCONCEPT:Canopy ! Canopy
relationship: measurement_of ECOSIMCONCEPT:BoundaryLayer ! BoundaryLayer

[Term]
id: ECOSIM:C3SGL
name: aqueous CO3 diffusivity
def: "Aqueous CO3 diffusivity refers to the measure of the ability of CO3 molecules to move through a liquid medium, specifically in an aqueous environment. It characterizes the rate at which CO3 molecules can diffuse or spread out from an area of high concentration to an area of low concentration. Aqueous CO3 diffusivity is an important parameter in earth systems modeling as it affects the transport and distribution of CO3 species in aquatic systems, such as lakes, rivers, and oceans. It influences various biogeochemical processes, including carbonate chemistry, pH regulation, and buffering capacity of water bodies." []
is_a: ECOSIM:CATEGORYHydrology ! category - Hydrology
is_a: ECOSIMCONCEPT:UnclassifiedVariable ! unclassified variable
relationship: attribute ECOSIMCONCEPT:Diffusivity ! Diffusivity
relationship: has_unit ECOSIM:m2h-1 ! m2 h-1
relationship: measured_in ECOSIMCONCEPT:Water ! Water
relationship: measurement_of ECOSIMCONCEPT:CO3 ! Carbonate
relationship: qualifier ECOSIMCONCEPT:Aqueous ! Aqueous

[Term]
id: ECOSIM:CAL
name: soil Al content
def: "Soil Al content refers to the concentration or amount of aluminum (Al) present in the soil. This parameter is an important aspect of Earth system modeling as it influences various processes and interactions within the soil-plant system. High levels of soil Al content can negatively affect plant growth, nutrient uptake, and can even be toxic to certain plant species. Therefore, accurately quantifying and representing soil Al content in models is crucial for understanding and predicting various biogeochemical cycles and ecosystem dynamics." []
is_a: ECOSIM:CATEGORYBiogeochemistry ! category - Biogeochemistry
is_a: ECOSIM:CATEGORYSoilBiogeochemistry ! category - Soil Biogeochemistry
is_a: ECOSIM:CATEGORYSoilProperty ! category - soil property
relationship: attribute ECOSIMCONCEPT:Content ! Content
relationship: has_unit ECOSIM:mgkg-1 ! mg kg-1
relationship: measured_in ECOSIMCONCEPT:Soil ! Soil
relationship: measurement_of ECOSIMCONCEPT:Aluminium ! Aluminium

[Term]
id: ECOSIM:CAL1Q
name: surface irrigation AlOH concentration
def: "Surface irrigation AlOH concentration refers to the concentration of AlOH (aluminum hydroxide) in water used for surface irrigation. AlOH is a common mineral compound that can be present in natural water sources or introduced through human activities such as mining and industrial processes. The concentration of AlOH in surface irrigation water can affect plant health and soil properties. Modeling this parameter is important for understanding the potential impacts of AlOH on crop growth, soil fertility, and water quality in agricultural systems." []
is_a: ECOSIMCONCEPT:UnclassifiedVariable ! unclassified variable
relationship: attribute ECOSIMCONCEPT:Concentration ! Concentration
relationship: has_unit ECOSIM:gm-3 ! g m-3
relationship: measured_in ECOSIMCONCEPT:SurfaceIrrigation ! SurfaceIrrigation
relationship: measurement_of ECOSIMCONCEPT:AlOH ! Aluminum hydroxide

[Term]
id: ECOSIM:CAL1R
name: precipitation AlOH concentration
def: "Precipitation AlOH concentration refers to the concentration of aluminum hydroxide (AlOH) in the precipitation, which represents the amount of AlOH particles dissolved in rainwater or snowfall. This parameter is important in earth systems modeling to study the effects of aluminum on various ecological and geochemical processes, such as soil acidity, nutrient availability, and aquatic ecosystem health. The concentration of AlOH in precipitation can be influenced by natural sources, such as atmospheric aerosols and volcanic emissions, as well as anthropogenic activities, such as industrial pollution and agricultural practices." []
is_a: ECOSIM:CATEGORYAtmosphericConditions ! category - Atmospheric Conditions
is_a: ECOSIM:CATEGORYDepositionFlux ! category - deposition flux
relationship: attribute ECOSIMCONCEPT:Concentration ! Concentration
relationship: context ECOSIMCONCEPT:Precipitation ! Precipitation
relationship: has_unit ECOSIM:gm-3 ! g m-3
relationship: measured_in ECOSIMCONCEPT:Water ! Water
relationship: measurement_of ECOSIMCONCEPT:AlOH ! Aluminum hydroxide

[Term]
id: ECOSIM:CAL1U
name: subsurface irrigation AlOH concentration
def: "Subsurface irrigation AlOH concentration refers to the concentration of aluminum hydroxide (AlOH) in the soil water resulting from subsurface irrigation practices. It represents the amount of aluminum hydroxide compound present in the soil water, which can impact the chemical composition and fertility of the soil as well as potentially affect plant growth and health. Monitoring the subsurface irrigation AlOH concentration is important in agricultural and environmental modeling as it helps understand and predict the potential effects of irrigation practices on soil quality and ecosystem functioning." []
is_a: ECOSIMCONCEPT:UnclassifiedVariable ! unclassified variable
relationship: attribute ECOSIMCONCEPT:Concentration ! Concentration
relationship: context ECOSIMCONCEPT:Irrigation ! Irrigation
relationship: has_unit ECOSIM:gm-3 ! g m-3
relationship: measured_in ECOSIMCONCEPT:Subsurface ! Subsurface
relationship: measurement_of ECOSIMCONCEPT:AlOH ! Aluminum hydroxide

[Term]
id: ECOSIM:CAL2Q
name: surface irrigation AlOH2 concentration
def: "Surface irrigation AlOH2 concentration refers to the concentration of AlOH2, which is a compound formed when aluminum reacts with water, in the water used for surface irrigation. Surface irrigation is a method of irrigating crops where water is applied directly to the soil surface and allowed to infiltrate into the root zone. The AlOH2 concentration in surface irrigation water can affect the availability of aluminum for plant uptake and can also have implications for soil health and water quality. This parameter is important to consider in earth systems models as it can influence plant growth, nutrient cycling, and hydrological processes associated with surface irrigation systems." []
is_a: ECOSIMCONCEPT:UnclassifiedVariable ! unclassified variable
relationship: attribute ECOSIMCONCEPT:Concentration ! Concentration
relationship: context ECOSIMCONCEPT:Irrigation ! Irrigation
relationship: has_unit ECOSIM:gm-3 ! g m-3
relationship: measured_in ECOSIMCONCEPT:Surface ! Surface
relationship: measurement_of ECOSIMCONCEPT:AlOH2 ! Aluminum dihydroxide

[Term]
id: ECOSIM:CAL2R
name: precipitation AlOH2 concentration
def: "Precipitation AlOH2 concentration refers to the amount of aluminum hydroxide (AlOH2) in a solution that is formed during or after a precipitation event, such as rain or snowfall. It represents the concentration of AlOH2 particles present in the water as a result of interactions between atmospheric emissions and environmental conditions. This parameter is important in Earth system modeling as it can affect various ecological and biogeochemical processes in aquatic ecosystems, including nutrient cycling, pH regulation, and the bioavailability of other elements." []
is_a: ECOSIM:CATEGORYAtmosphericConditions ! category - Atmospheric Conditions
is_a: ECOSIM:CATEGORYDepositionFlux ! category - deposition flux
relationship: attribute ECOSIMCONCEPT:Concentration ! Concentration
relationship: context ECOSIMCONCEPT:Precipitation ! Precipitation
relationship: has_unit ECOSIM:gm-3 ! g m-3
relationship: measured_in ECOSIMCONCEPT:Water ! Water
relationship: measurement_of ECOSIMCONCEPT:AlOH2 ! Aluminum dihydroxide

[Term]
id: ECOSIM:CAL2U
name: subsurface irrigation AlOH2 concentration
def: "Subsurface irrigation refers to a method of irrigation where water is distributed below the surface of the soil directly to the plant roots. This technique helps minimize water evaporation and allows for more efficient water utilization. AlOH2 concentration refers to the amount of AlOH2 (aluminum hydroxide) present in the soil or water used for subsurface irrigation. Aluminum hydroxide is a common compound found in soils and its concentration can affect various soil properties and plant growth. Monitoring and understanding the AlOH2 concentration is important for assessing the quality of the irrigation water and its potential impacts on soil and plants." []
is_a: ECOSIMCONCEPT:UnclassifiedVariable ! unclassified variable
relationship: attribute ECOSIMCONCEPT:Concentration ! Concentration
relationship: context ECOSIMCONCEPT:Irrigation ! Irrigation
relationship: has_unit ECOSIM:gm-3 ! g m-3
relationship: measured_in ECOSIMCONCEPT:Subsurface ! Subsurface
relationship: measurement_of ECOSIMCONCEPT:AlOH2 ! Aluminum dihydroxide

[Term]
id: ECOSIM:CAL3Q
name: surface irrigation AlOH3 concentration
def: "Surface irrigation AlOH3 concentration refers to the concentration of AlOH3 (aluminum hydroxide) in water used for surface irrigation. Aluminum hydroxide is commonly incorporated into surface water bodies through inputs from surrounding soils, industrial activities, and atmospheric deposition. The concentration of AlOH3 can affect the chemical properties and bioavailability of other elements in the irrigation water, and thus plays a role in nutrient cycling and potential impacts on aquatic ecosystems. Monitoring this parameter is important for understanding the potential risks and impacts of surface irrigation on water quality and ecosystem health." []
is_a: ECOSIMCONCEPT:UnclassifiedVariable ! unclassified variable
relationship: attribute ECOSIMCONCEPT:Concentration ! Concentration
relationship: context ECOSIMCONCEPT:Irrigation ! Irrigation
relationship: has_unit ECOSIM:gm-3 ! g m-3
relationship: measured_in ECOSIMCONCEPT:Surface ! Surface
relationship: measurement_of ECOSIMCONCEPT:AlOH3 ! Aluminum trihydroxide

[Term]
id: ECOSIM:CAL3R
name: precipitation AlOH3 concentration
def: "Precipitation AlOH3 concentration refers to the concentration of AlOH3 (aluminum hydroxide) in the mathematical representation of the Earth system model that simulates the process of precipitation. It is a parameter that determines the amount of aluminum hydroxide present in precipitation events, which affects various aspects of the Earth system, including the chemistry of rainwater, soil composition, and ecosystem dynamics. The concentration of AlOH3 in precipitation is an important factor in studying the impacts of aluminum on various Earth system processes and can be used to investigate the effects of acid rain and pollution on natural systems." []
is_a: ECOSIM:CATEGORYAtmosphericConditions ! category - Atmospheric Conditions
is_a: ECOSIM:CATEGORYDepositionFlux ! category - deposition flux
relationship: attribute ECOSIMCONCEPT:Concentration ! Concentration
relationship: context ECOSIMCONCEPT:Precipitation ! Precipitation
relationship: has_unit ECOSIM:gm-3 ! g m-3
relationship: measurement_of ECOSIMCONCEPT:AlOH3 ! Aluminum trihydroxide

[Term]
id: ECOSIM:CAL3U
name: subsurface irrigation AlOH3 concentration
def: "Subsurface irrigation AlOH3 concentration refers to the level of AlOH3, which is aluminum hydroxide, in the soil water in a subsurface irrigation system. This parameter is used to quantify the amount of aluminum hydroxide present in the irrigation water and is essential for understanding and modeling the potential impact of aluminum toxicity on plant growth and soil health in subsurface irrigation scenarios." []
is_a: ECOSIMCONCEPT:UnclassifiedVariable ! unclassified variable
relationship: attribute ECOSIMCONCEPT:Concentration ! Concentration
relationship: context ECOSIMCONCEPT:Irrigation ! Irrigation
relationship: has_unit ECOSIM:gm-3 ! g m-3
relationship: measured_in ECOSIMCONCEPT:Subsurface ! Subsurface
relationship: measurement_of ECOSIMCONCEPT:AlOH3 ! Aluminum trihydroxide

[Term]
id: ECOSIM:CAL4Q
name: surface irrigation AlOH4 concentration
def: "Surface irrigation AlOH4 concentration refers to the concentration of aluminum hydroxide (AlOH4) in the water used for surface irrigation. It represents the amount of dissolved aluminum hydroxide in the irrigation water, which can have implications for soil health, crop growth, and water quality. Monitoring this parameter is important in earth systems modeling to understand the potential impacts of aluminum toxicity on plant productivity and ecosystem dynamics in areas where surface irrigation is practiced." []
is_a: ECOSIM:CATEGORYDepositionFlux ! category - deposition flux
is_a: ECOSIMCONCEPT:UnclassifiedVariable ! unclassified variable
relationship: attribute ECOSIMCONCEPT:Concentration ! Concentration
relationship: context ECOSIMCONCEPT:SurfaceIrrigation ! SurfaceIrrigation
relationship: has_unit ECOSIM:gm-3 ! g m-3
relationship: measured_in ECOSIMCONCEPT:Water ! Water
relationship: measurement_of ECOSIMCONCEPT:AlOH4 ! Aluminum tetrahydroxide

[Term]
id: ECOSIM:CAL4R
name: precipitation AlOH4 concentration
def: "Precipitation AlOH4 concentration refers to the concentration of aluminum hydroxide (AlOH4) in rainfall or any form of precipitation. This parameter represents the amount of aluminum hydroxide dissolved in water that is deposited onto the Earth's surface through precipitation events. It is an important parameter for studying the transport and deposition of aluminum in terrestrial and aquatic ecosystems, and can have implications for ecosystem health and water quality." []
is_a: ECOSIM:CATEGORYAtmosphericConditions ! category - Atmospheric Conditions
is_a: ECOSIM:CATEGORYDepositionFlux ! category - deposition flux
relationship: attribute ECOSIMCONCEPT:Concentration ! Concentration
relationship: context ECOSIMCONCEPT:Precipitation ! Precipitation
relationship: has_unit ECOSIM:gm-3 ! g m-3
relationship: measured_in ECOSIMCONCEPT:Water ! Water
relationship: measurement_of ECOSIMCONCEPT:AlOH4 ! Aluminum tetrahydroxide

[Term]
id: ECOSIM:CAL4U
name: subsurface irrigation AlOH4 concentration
def: "Subsurface irrigation AlOH4 concentration refers to the level of AlOH4 (aluminum hydroxide) present in the soil profile when using subsurface irrigation techniques. Subsurface irrigation involves the delivery of water and nutrients directly to the root zone of plants through underground pipes or tubing. The concentration of AlOH4 in the irrigation water can affect soil pH and nutrient availability, which can influence plant growth and crop productivity. Monitoring and understanding this parameter is crucial for accurately assessing the impact of subsurface irrigation on soil chemistry and plant health." []
is_a: ECOSIMCONCEPT:UnclassifiedVariable ! unclassified variable
relationship: attribute ECOSIMCONCEPT:Concentration ! Concentration
relationship: context ECOSIMCONCEPT:Irrigation ! Irrigation
relationship: has_unit ECOSIM:gm-3 ! g m-3
relationship: measured_in ECOSIMCONCEPT:Subsurface ! Subsurface
relationship: measurement_of ECOSIMCONCEPT:AlOH4 ! Aluminum tetrahydroxide

[Term]
id: ECOSIM:CALOH
name: soil AlOH3 content
def: "The term 'soil AlOH3 content' refers to the quantity or concentration of aluminum hydroxide (AlOH3) present in the soil. Aluminum hydroxide is a naturally occurring compound in soils and is important for understanding soil properties and processes such as soil pH, nutrient availability, and cation exchange capacity. The soil AlOH3 content parameter provides information about the amount of aluminum hydroxide in the soil, which can influence various biogeochemical processes and ecosystem dynamics, particularly in acidic soils." []
is_a: ECOSIM:CATEGORYBiogeochemistry ! category - Biogeochemistry
is_a: ECOSIM:CATEGORYSoilBiogeochemistry ! category - Soil Biogeochemistry
is_a: ECOSIM:CATEGORYSoilProperty ! category - soil property
relationship: attribute ECOSIMCONCEPT:Content ! Content
relationship: has_unit ECOSIM:mgkg-1 ! mg kg-1
relationship: measured_in ECOSIMCONCEPT:Soil ! Soil
relationship: measurement_of ECOSIMCONCEPT:AlOH3 ! Aluminum trihydroxide

[Term]
id: ECOSIM:CALPO
name: soil AlPO4 content
def: "Soil AlPO4 content refers to the concentration or abundance of aluminum phosphate compound (AlPO4) in soil. It is a parameter used in earth systems modeling to quantify the contribution of this compound to soil composition and fertility. AlPO4 is important for nutrient cycling, as it can bind and release elements such as phosphorus in the soil, affecting the availability of nutrients for plants and other organisms. Soil AlPO4 content is typically measured in units of mass per unit volume of soil (e.g., grams per kilogram)." []
is_a: ECOSIM:CATEGORYBiogeochemistry ! category - Biogeochemistry
is_a: ECOSIM:CATEGORYSoilProperty ! category - soil property
relationship: attribute ECOSIMCONCEPT:Content ! Content
relationship: has_unit ECOSIM:mgkg-1 ! mg kg-1
relationship: measured_in ECOSIMCONCEPT:Soil ! Soil
relationship: measurement_of ECOSIMCONCEPT:AlPO4 ! AlPO4

[Term]
id: ECOSIM:CALQ
name: surface irrigation Al concentration
def: "Surface irrigation Al concentration refers to the concentration of aluminum (Al) in the water used for surface irrigation. Surface irrigation is a method of applying water to crops by allowing water to flow over the soil surface, providing moisture to plant roots. The Al concentration in surface irrigation water can impact soil health, plant growth, and overall agricultural productivity. This parameter is relevant for earth systems modeling to understand the potential effects of aluminum on the water quality, soil chemistry, and plant responses in surface irrigation systems." []
is_a: ECOSIMCONCEPT:UnclassifiedVariable ! unclassified variable
relationship: attribute ECOSIMCONCEPT:Concentration ! Concentration
relationship: context ECOSIMCONCEPT:Irrigation ! Irrigation
relationship: has_unit ECOSIM:gm-3 ! g m-3
relationship: measured_in ECOSIMCONCEPT:Surface ! Surface
relationship: measurement_of ECOSIMCONCEPT:Aluminum ! Aluminum

[Term]
id: ECOSIM:CALR
name: precipitation Al concentration
def: "Precipitation Al (aluminum) concentration refers to the amount of aluminum present in precipitation (rain, snow, etc.) in a specific area or region. It is a parameter that characterizes the level of aluminum pollution in the atmosphere, which can be influenced by natural processes (e.g., weathering of rocks) as well as human activities (e.g., industrial emissions). Monitoring precipitation Al concentration is important for understanding the environmental impact of aluminum on ecosystems and human health and for assessing the effectiveness of pollution control measures." []
is_a: ECOSIM:CATEGORYAtmosphericConditions ! category - Atmospheric Conditions
is_a: ECOSIM:CATEGORYDepositionFlux ! category - deposition flux
relationship: attribute ECOSIMCONCEPT:Concentration ! Concentration
relationship: has_unit ECOSIM:gm-3 ! g m-3
relationship: measured_in ECOSIMCONCEPT:Precipitation ! Precipitation
relationship: measurement_of ECOSIMCONCEPT:Aluminum ! Aluminum

[Term]
id: ECOSIM:CALSQ
name: surface irrigation AlSO4 concentration
def: "Surface irrigation AlSO4 concentration refers to the concentration of aluminum sulfate (AlSO4) in the water used for surface irrigation. This parameter is important in earth systems modeling as it can impact the soil chemistry and plant health in irrigated areas. The concentration of AlSO4 in surface irrigation water can affect the availability and uptake of nutrients by plants, as well as the potential for aluminum toxicity in the soil. Monitoring and understanding the surface irrigation AlSO4 concentration is crucial for accurately simulating the impacts of irrigation practices on agricultural productivity and ecosystem health." []
is_a: ECOSIMCONCEPT:UnclassifiedVariable ! unclassified variable
relationship: attribute ECOSIMCONCEPT:Concentration ! Concentration
relationship: context ECOSIMCONCEPT:Irrigation ! Irrigation
relationship: has_unit ECOSIM:gm-3 ! g m-3
relationship: measured_in ECOSIMCONCEPT:Surface ! Surface
relationship: measurement_of ECOSIMCONCEPT:AlSO4 ! Aluminum sulfate

[Term]
id: ECOSIM:CALSR
name: precipitation AlSO4 concentration
def: "Precipitation AlSO4 concentration refers to the amount of aluminum sulfate (AlSO4) present in precipitation. It is a parameter used in earth system models to represent the concentration of aluminum sulfate in rainwater or snowfall. Aluminum sulfate is often used as a coagulating agent in water treatment processes and can enter the environment through industrial emissions or natural sources. Monitoring and simulating the precipitation AlSO4 concentration is important for understanding the impact of aluminum contamination on ecosystems and water quality." []
is_a: ECOSIM:CATEGORYAtmosphericConditions ! category - Atmospheric Conditions
is_a: ECOSIM:CATEGORYDepositionFlux ! category - deposition flux
relationship: attribute ECOSIMCONCEPT:Concentration ! Concentration
relationship: context ECOSIMCONCEPT:Precipitation ! Precipitation
relationship: has_unit ECOSIM:gm-3 ! g m-3
relationship: measured_in ECOSIMCONCEPT:Water ! Water
relationship: measurement_of ECOSIMCONCEPT:AlSO4 ! Aluminum sulfate

[Term]
id: ECOSIM:CALSU
name: subsurface irrigation AlSO4 concentration
def: "Subsurface irrigation AlSO4 concentration refers to the concentration of aluminum sulfate (AlSO4) in the water used for subsurface irrigation. Subsurface irrigation is a method of watering plants where water is delivered directly to the plant roots through underground pipes or tubes. The concentration of AlSO4 in the irrigation water is an important parameter to monitor, as it can affect the soil pH, nutrient availability, and overall plant health." []
is_a: ECOSIMCONCEPT:UnclassifiedVariable ! unclassified variable
relationship: attribute ECOSIMCONCEPT:Concentration ! Concentration
relationship: context ECOSIMCONCEPT:Irrigation ! Irrigation
relationship: has_unit ECOSIM:gm-3 ! g m-3
relationship: measured_in ECOSIMCONCEPT:Subsurface ! Subsurface
relationship: measurement_of ECOSIMCONCEPT:AlSO4 ! Aluminum sulfate

[Term]
id: ECOSIM:CALU
name: subsurface irrigation Fe concentration
def: "Subsurface irrigation Fe concentration refers to the level of iron (Fe) present in the water used for subsurface irrigation in agricultural systems. It represents a parameter that can be measured or simulated to understand the potential impact of iron concentration on plant growth, nutrient availability, and overall ecosystem dynamics in the soil-water system. This parameter is important for earth systems modeling as it helps in assessing the potential effects of iron concentration on crop yields, water quality, and biogeochemical cycling in agricultural landscapes." []
is_a: ECOSIMCONCEPT:UnclassifiedVariable ! unclassified variable
relationship: attribute ECOSIMCONCEPT:Concentration ! Concentration
relationship: context ECOSIMCONCEPT:Irrigation ! Irrigation
relationship: has_unit ECOSIM:gm-3 ! g m-3
relationship: measured_in ECOSIMCONCEPT:Subsurface ! Subsurface
relationship: measurement_of ECOSIMCONCEPT:Fe ! Iron

[Term]
id: ECOSIM:CARBN
name: total gross CO2 fixation
def: "Total gross CO2 fixation refers to the overall process in which carbon dioxide (CO2) from the atmosphere is converted into organic carbon compounds through photosynthesis by plants and other photosynthetic organisms. It represents the combined rate at which CO2 is being assimilated by the entire ecosystem or a specific region over a given time period, thereby contributing to carbon uptake and storage in terrestrial ecosystems. This parameter is crucial for assessing the capacity of ecosystems to act as carbon sinks and for understanding the global carbon cycle." []
is_a: ECOSIM:CATEGORYPlantPhysiology ! category - plant physiology
is_a: ECOSIMCONCEPT:UnclassifiedVariable ! unclassified variable
relationship: has_unit ECOSIM:gd-2 ! g d-2
relationship: measured_in ECOSIMCONCEPT:Ecosystem ! Ecosystem
relationship: measurement_of ECOSIMCONCEPT:CarbonDioxide ! CarbonDioxide

[Term]
id: ECOSIM:CASGL
name: aqueous Ca diffusivity
def: "Aqueous Ca diffusivity refers to the measure of the ability of calcium ions (Ca) to move through a liquid medium, such as water. It is a parameter used in Earth systems modeling to quantify the rate of diffusion of calcium in aquatic environments. Aqueous Ca diffusivity is influenced by factors such as temperature, salinity, and the concentration gradient of calcium, and it plays a crucial role in processes such as the transport and cycling of calcium in aquatic ecosystems." []
is_a: ECOSIM:CATEGORYHydrology ! category - Hydrology
is_a: ECOSIMCONCEPT:UnclassifiedVariable ! unclassified variable
relationship: attribute ECOSIMCONCEPT:Diffusivity ! Diffusivity
relationship: has_unit ECOSIM:m2h-1 ! m2 h-1
relationship: measured_in ECOSIMCONCEPT:Water ! Water
relationship: measurement_of ECOSIMCONCEPT:Calcium ! Calcium
relationship: qualifier ECOSIMCONCEPT:Aqueous ! Aqueous

[Term]
id: ECOSIM:CATEGORYAtmosphericConditions
name: category - Atmospheric Conditions
def: "Refers to the conditions pertaining to the Earth's atmosphere at a specific time and place, including temperature, humidity, wind velocity, precipitation, and atmospheric pressure conditions." []
is_a: ECOSIMCONCEPT:Variable ! variable

[Term]
id: ECOSIM:CATEGORYBiogeochemistry
name: category - Biogeochemistry
def: "Presents integrated study of the physical, chemical, biological, and geological processes and their interactions in controlling the composition, behavior and distribution of matter in the environment." []
is_a: ECOSIMCONCEPT:Variable ! variable

[Term]
id: ECOSIM:CATEGORYCanopyPhysiology
name: category - Canopy Physiology
def: "A study that deals with plant canopies and their physiological characteristics such as photosynthesis, water use, and nutrient cycling." []
is_a: ECOSIMCONCEPT:Variable ! variable

[Term]
id: ECOSIM:CATEGORYCanopyStructure
name: category - canopy structure
def: "Parameters defining plant canopy architecture, leaf area distribution, organ sizes." []
is_a: ECOSIMCONCEPT:Variable ! variable

[Term]
id: ECOSIM:CATEGORYDepositionFlux
name: category - deposition flux
def: "Atmospheric deposition fluxes of elements to soil and plant surfaces." []
is_a: ECOSIMCONCEPT:Variable ! variable

[Term]
id: ECOSIM:CATEGORYElementFlux
name: category - C and nutrient flux
def: "Fluxes of C, N, P and other elements between soil, plants and atmosphere." []
is_a: ECOSIMCONCEPT:Variable ! variable

[Term]
id: ECOSIM:CATEGORYGasFlux
name: category - Gas Flux
def: "Refers to the rate of gas exchange per unit area between an ecosystem and the atmosphere." []
is_a: ECOSIMCONCEPT:Variable ! variable

[Term]
id: ECOSIM:CATEGORYHydrology
name: category - Hydrology
def: "The scientific study of the movement, distribution, and management of water on Earth and other planets, including the water cycle, water resources and environmental watershed sustainability." []
is_a: ECOSIMCONCEPT:Variable ! variable

[Term]
id: ECOSIM:CATEGORYMicrobialActivity
name: category - microbial activity
def: "Parameters defining soil microbial biomass and its role in OM decomposition." []
is_a: ECOSIMCONCEPT:Variable ! variable

[Term]
id: ECOSIM:CATEGORYNTransformation
name: category - N transformation
def: "Biotic and abiotic processes leading to interconversions between various N species." []
is_a: ECOSIMCONCEPT:Variable ! variable

[Term]
id: ECOSIM:CATEGORYPlantPhysiology
name: category - plant physiology
def: "Parameters related to plant metabolic, photosynthetic, reproductive and phenological processes." []
is_a: ECOSIMCONCEPT:Variable ! variable

[Term]
id: ECOSIM:CATEGORYPlantPopulation
name: category - Plant Population
def: "Pertains to the study of distribution, density, variation, and the number of particular plants in a specified area." []
is_a: ECOSIMCONCEPT:Variable ! variable

[Term]
id: ECOSIM:CATEGORYRootPhysiology
name: category - root physiology
def: "Parameters related to root growth, morphology, resource uptake kinetics." []
is_a: ECOSIMCONCEPT:Variable ! variable

[Term]
id: ECOSIM:CATEGORYSnowpack
name: category - Snowpack
def: "Refers to the total accumulated snow and ice on the ground in mountainous or high altitude regions, that melts gradually and provides water supply." []
is_a: ECOSIMCONCEPT:Variable ! variable

[Term]
id: ECOSIM:CATEGORYSoilBiogeochemistry
name: category - Soil Biogeochemistry
def: "The study of the physical, chemical and biological processes occurring within soils and their interaction, which affect the composition of the natural environment." []
is_a: ECOSIMCONCEPT:Variable ! variable

[Term]
id: ECOSIM:CATEGORYSoilProperty
name: category - soil property
def: "Parameters related to soil chemical and physical characteristics like texture, mineral composition, cation exchange properties." []
is_a: ECOSIMCONCEPT:Variable ! variable

[Term]
id: ECOSIM:CATEGORYSoilSolution
name: category - soil solution
def: "Parameters related to soil pore water composition and properties like ionic strength, electrical conductivity." []
is_a: ECOSIMCONCEPT:Variable ! variable

[Term]
id: ECOSIM:CATEGORYSurfaceEnergyBalance
name: category - Surface Energy Balance
def: "Refers to the balance between incoming energy from the Sun and outgoing long wave (thermal) and reflected (short wave) energy from the Earth's surface." []
is_a: ECOSIMCONCEPT:Variable ! variable

[Term]
id: ECOSIM:CATEGORYTraceGasFlux
name: category - trace gas flux
def: "Production, consumption and emission fluxes of gases like CO2, CH4 between soil, plants and atmosphere." []
is_a: ECOSIMCONCEPT:Variable ! variable

[Term]
id: ECOSIM:CBXN
name: carboxylation efficiency
def: "Carboxylation efficiency refers to the rate at which plants convert carbon dioxide (CO2) into organic compounds through the process of photosynthesis. It represents the ability of plants to utilize CO2 effectively and convert it into carbohydrates, which are necessary for growth and development. Carboxylation efficiency is influenced by various factors such as temperature, light intensity, and the concentration of CO2 in the atmosphere. It is an important parameter in Earth system models as it helps to understand the overall carbon cycle and the response of vegetation to changing environmental conditions." []
is_a: ECOSIM:CATEGORYCanopyPhysiology ! category - Canopy Physiology
is_a: ECOSIM:CATEGORYPlantPhysiology ! category - plant physiology
relationship: has_unit ECOSIM:umolumol-1 ! umol umol-1
relationship: measured_in ECOSIMCONCEPT:Leaf ! Leaf

[Term]
id: ECOSIM:CBXN4
name: C4 carboxylation efficiency
def: "C4 carboxylation efficiency refers to the efficiency of the carbon fixation process in C4 plants, where atmospheric carbon dioxide (CO2) is converted into organic compounds through a series of biochemical reactions. It quantifies the ratio of how much CO2 is taken up by the plant to how much energy is expended during this process. A higher C4 carboxylation efficiency indicates that the plant can more effectively utilize CO2 to produce biomass, resulting in increased productivity and potentially greater resilience to environmental stresses such as drought or high temperatures." []
is_a: ECOSIM:CATEGORYCanopyPhysiology ! category - Canopy Physiology
is_a: ECOSIM:CATEGORYPlantPhysiology ! category - plant physiology
relationship: has_unit ECOSIM:umolumol-1 ! umol umol-1
relationship: measurement_of ECOSIMCONCEPT:C4Carboxylation ! C4 carboxylation

[Term]
id: ECOSIM:CC0PQ
name: surface irrigation CaPO4 concentration
def: "The surface irrigation CaPO4 concentration refers to the concentration of calcium phosphate (CaPO4) in water used for surface irrigation. Surface irrigation is a method of applying water to agricultural fields where it is distributed over the soil surface. The CaPO4 concentration in surface irrigation water is an important parameter to consider in earth systems modeling as it can affect soil fertility, water quality, and nutrient cycling in agricultural systems." []
is_a: ECOSIMCONCEPT:UnclassifiedVariable ! unclassified variable
relationship: attribute ECOSIMCONCEPT:Concentration ! Concentration
relationship: context ECOSIMCONCEPT:Irrigation ! Irrigation
relationship: has_unit ECOSIM:gm-3 ! g m-3
relationship: measured_in ECOSIMCONCEPT:Surface ! Surface
relationship: measurement_of ECOSIMCONCEPT:CaPO4 ! Calcium phosphate

[Term]
id: ECOSIM:CC0PR
name: precipitation CaPO4 concentration
def: "Precipitation CaPO4 concentration refers to the concentration of calcium phosphate (CaPO4) in a body of water that is formed as a result of various precipitation processes. It is a measure of the amount of CaPO4 that has been dissolved and deposited into the water. This parameter is important for studying the biogeochemical cycles of calcium and phosphorus in aquatic ecosystems, as well as for understanding the potential for the formation and dissolution of CaPO4 minerals in the water. The concentration of CaPO4 in precipitation is influenced by factors such as atmospheric inputs, weathering processes, and the biological activity within the ecosystem." []
is_a: ECOSIM:CATEGORYAtmosphericConditions ! category - Atmospheric Conditions
is_a: ECOSIM:CATEGORYDepositionFlux ! category - deposition flux
relationship: attribute ECOSIMCONCEPT:Concentration ! Concentration
relationship: context ECOSIMCONCEPT:Precipitation ! Precipitation
relationship: has_unit ECOSIM:gm-3 ! g m-3
relationship: measured_in ECOSIMCONCEPT:Water ! Water
relationship: measurement_of ECOSIMCONCEPT:CaPO4 ! Calcium phosphate

[Term]
id: ECOSIM:CC0PU
name: subsurface irrigation CaPO4 concentration
def: "Subsurface irrigation CaPO4 concentration refers to the level of calcium phosphate (CaPO4) in the soil water within a subsurface irrigation system. It is a parameter that describes the amount of CaPO4 present in the water used for irrigation in the subsurface, which can impact plant growth and nutrient availability in agricultural systems. The concentration of CaPO4 can vary depending on factors such as the type and quality of irrigation water, soil composition, and management practices. Monitoring and modeling this parameter helps to understand and optimize nutrient management and irrigation practices to ensure sustainable crop production." []
is_a: ECOSIMCONCEPT:UnclassifiedVariable ! unclassified variable
relationship: attribute ECOSIMCONCEPT:Concentration ! Concentration
relationship: context ECOSIMCONCEPT:Irrigation ! Irrigation
relationship: has_unit ECOSIM:gm-3 ! g m-3
relationship: measured_in ECOSIMCONCEPT:Subsurface ! Subsurface
relationship: measurement_of ECOSIMCONCEPT:CaPO4 ! Calcium phosphate

[Term]
id: ECOSIM:CC1PQ
name: surface irrigation CaHPO4 concentration
def: "Surface irrigation refers to a method of watering crops or plants where water is applied to the soil surface and allowed to infiltrate and reach the plant roots. The 'CaHPO4 concentration' parameter refers to the concentration of calcium phosphate (CaHPO4) in the irrigation water used for surface irrigation. CaHPO4 is a compound commonly found in soil and can affect the nutrient content and pH level of the soil. Monitoring and controlling the CaHPO4 concentration in surface irrigation can help optimize plant growth and ensure proper soil health." []
is_a: ECOSIMCONCEPT:UnclassifiedVariable ! unclassified variable
relationship: attribute ECOSIMCONCEPT:Concentration ! Concentration
relationship: context ECOSIMCONCEPT:Irrigation ! Irrigation
relationship: has_unit ECOSIM:gm-3 ! g m-3
relationship: measured_in ECOSIMCONCEPT:Surface ! Surface
relationship: measurement_of ECOSIMCONCEPT:CaHPO4 ! CaHPO4

[Term]
id: ECOSIM:CC1PR
name: precipitation CaHPO4 concentration
def: "Precipitation CaHPO4 concentration refers to the measurement or representation of the amount of calcium hydrogen phosphate (CaHPO4) present in precipitation. This parameter is used to quantify the level of this compound in the water that falls from the atmosphere, which can be important for understanding nutrient cycling and the impact of precipitation on ecosystem health. It is typically expressed in units such as milligrams per liter (mg/L) or parts per million (ppm)." []
is_a: ECOSIM:CATEGORYAtmosphericConditions ! category - Atmospheric Conditions
relationship: attribute ECOSIMCONCEPT:Concentration ! Concentration
relationship: has_unit ECOSIM:gm-3 ! g m-3
relationship: measured_in ECOSIMCONCEPT:Precipitation ! Precipitation
relationship: measurement_of ECOSIMCONCEPT:CaHPO4 ! CaHPO4

[Term]
id: ECOSIM:CC1PU
name: subsurface irrigation CaHPO4 concentration
def: "Subsurface irrigation refers to the practice of applying water and nutrients to crops or plants by delivering them directly to the root zone below the soil surface. It involves the use of specialized irrigation systems that distribute water and nutrients through buried pipes or tubes, allowing for efficient and controlled delivery to plant roots. The 'CaHPO4 concentration' in the context of subsurface irrigation refers to the concentration of calcium hydrogen phosphate (CaHPO4) in the irrigation water or soil solution. CaHPO4 is an important source of calcium and phosphorus, essential nutrients for plant growth. The concentration of CaHPO4 can influence nutrient availability and uptake by plants, as well as plant growth and yield. Monitoring and controlling the CaHPO4 concentration in subsurface irrigation systems is therefore important for optimizing plant health and productivity." []
is_a: ECOSIMCONCEPT:UnclassifiedVariable ! unclassified variable
relationship: attribute ECOSIMCONCEPT:Concentration ! Concentration
relationship: context ECOSIMCONCEPT:Irrigation ! Irrigation
relationship: has_unit ECOSIM:gm-3 ! g m-3
relationship: measured_in ECOSIMCONCEPT:Subsurface ! Subsurface
relationship: measurement_of ECOSIMCONCEPT:CaHPO4 ! CaHPO4

[Term]
id: ECOSIM:CC2PQ
name: surface irrigation CaH2PO4 concentration
def: "Surface irrigation CaH2PO4 concentration refers to the concentration of calcium dihydrogen phosphate (CaH2PO4) in the water used for surface irrigation. It represents the amount of CaH2PO4 dissolved in the irrigation water and can impact soil fertility and nutrient availability for plants. Monitoring and understanding the surface irrigation CaH2PO4 concentration is important for accurately simulating and modeling the nutrient dynamics and water quality in agricultural systems." []
is_a: ECOSIMCONCEPT:UnclassifiedVariable ! unclassified variable
relationship: attribute ECOSIMCONCEPT:Concentration ! Concentration
relationship: context ECOSIMCONCEPT:Irrigation ! Irrigation
relationship: has_unit ECOSIM:gm-3 ! g m-3
relationship: measured_in ECOSIMCONCEPT:Surface ! Surface
relationship: measurement_of ECOSIMCONCEPT:CaH2PO4 ! Calcium dihydrogen phosphate

[Term]
id: ECOSIM:CC2PR
name: precipitation CaH2PO4 concentration
def: "Precipitation CaH2PO4 concentration refers to the concentration of calcium dihydrogen phosphate (CaH2PO4) in precipitation, which is a measure of the amount of this compound present in a given volume of precipitation. This parameter is relevant for understanding the potential nutrient inputs from precipitation to terrestrial ecosystems, as calcium dihydrogen phosphate is a commonly used fertilizer containing essential nutrients for plant growth. Monitoring and modeling precipitation CaH2PO4 concentration can provide insights into nutrient cycling and potential impacts on ecosystem productivity." []
is_a: ECOSIM:CATEGORYAtmosphericConditions ! category - Atmospheric Conditions
is_a: ECOSIM:CATEGORYDepositionFlux ! category - deposition flux
relationship: attribute ECOSIMCONCEPT:Concentration ! Concentration
relationship: has_unit ECOSIM:gm-3 ! g m-3
relationship: measured_in ECOSIMCONCEPT:Precipitation ! Precipitation
relationship: measurement_of ECOSIMCONCEPT:CaH2PO4 ! Calcium dihydrogen phosphate

[Term]
id: ECOSIM:CC2PU
name: subsurface irrigation CaH2PO4 concentration
def: "Subsurface irrigation CaH2PO4 concentration refers to the level or amount of calcium dihydrogen phosphate (CaH2PO4) present in the water used for subsurface irrigation. It represents the concentration of this specific compound, which can be used as a fertilizer or nutrient source, in the irrigation water that is applied below the surface of the soil. This parameter is important in Earth systems modeling as it can affect the availability of essential nutrients for plant growth and can have implications for soil fertility, nutrient cycling, and overall agricultural productivity." []
is_a: ECOSIMCONCEPT:UnclassifiedVariable ! unclassified variable
relationship: attribute ECOSIMCONCEPT:Concentration ! Concentration
relationship: has_unit ECOSIM:gm-3 ! g m-3
relationship: measured_in ECOSIMCONCEPT:SubsurfaceIrrigation ! SubsurfaceIrrigation
relationship: measurement_of ECOSIMCONCEPT:CaH2PO4 ! Calcium dihydrogen phosphate

[Term]
id: ECOSIM:CC3Q
name: surface irrigation CO3 concentration
def: "Surface irrigation CO3 concentration refers to the concentration of carbonate (CO3) ions in the water used for surface irrigation. Surface irrigation is a method of irrigation in which water is applied to the land surface and allowed to flow over the soil surface to irrigate crops. The CO3 concentration parameter is important to monitor as it can impact soil pH, nutrient availability, and the overall health and productivity of the agricultural system." []
is_a: ECOSIMCONCEPT:UnclassifiedVariable ! unclassified variable
relationship: attribute ECOSIMCONCEPT:Concentration ! Concentration
relationship: context ECOSIMCONCEPT:Irrigation ! Irrigation
relationship: has_unit ECOSIM:gm-3 ! g m-3
relationship: measured_in ECOSIMCONCEPT:Surface ! Surface
relationship: measurement_of ECOSIMCONCEPT:CO3 ! Carbonate

[Term]
id: ECOSIM:CC3R
name: precipitation CO3 concentration
def: "Precipitation CO3 concentration refers to the amount of carbonate (CO3) ions present in precipitation, such as rain or snowfall. It is a parameter used in Earth system models to represent the concentration of carbonate in the atmosphere that can be dissolved into precipitation. This parameter is important for studying the carbon cycle and ocean acidification, as carbonate ions play a crucial role in the ocean's ability to absorb and store atmospheric carbon dioxide. By incorporating precipitation CO3 concentration into Earth system models, scientists can better understand the impacts of changing atmospheric CO2 levels on the acidity of precipitation and its subsequent effects on the environment." []
is_a: ECOSIM:CATEGORYAtmosphericConditions ! category - Atmospheric Conditions
is_a: ECOSIM:CATEGORYDepositionFlux ! category - deposition flux
relationship: attribute ECOSIMCONCEPT:Concentration ! Concentration
relationship: context ECOSIMCONCEPT:Precipitation ! Precipitation
relationship: has_unit ECOSIM:gm-3 ! g m-3
relationship: measured_in ECOSIMCONCEPT:Water ! Water
relationship: measurement_of ECOSIMCONCEPT:CO3 ! Carbonate

[Term]
id: ECOSIM:CC3U
name: subsurface irrigation HCO3 concentration
def: "Subsurface irrigation HCO3 concentration refers to the amount of bicarbonate ions (HCO3-) present in the soil water in a subsurface irrigation system. It is a parameter used in earth system modeling to represent the concentration of bicarbonate ions in the water used for irrigation, which can have significant impacts on soil chemistry, nutrient availability, and plant growth." []
is_a: ECOSIMCONCEPT:UnclassifiedVariable ! unclassified variable
relationship: attribute ECOSIMCONCEPT:Concentration ! Concentration
relationship: context ECOSIMCONCEPT:Irrigation ! Irrigation
relationship: has_unit ECOSIM:gm-3 ! g m-3
relationship: measured_in ECOSIMCONCEPT:Subsurface ! Subsurface
relationship: measurement_of ECOSIMCONCEPT:HCO3 ! Bicarbonate

[Term]
id: ECOSIM:CCA
name: soil Ca content
def: "Soil Ca content refers to the concentration or amount of calcium (Ca) present in the soil. It is an important parameter in earth system modeling as it influences various soil processes and properties, such as nutrient availability, pH, and cation exchange capacity. Soil Ca content can vary spatially and temporally and is influenced by factors such as parent material, weathering, leaching, and land management practices. It is typically measured in units of mass per unit volume of soil, such as kilograms per hectare or grams per cubic meter." []
is_a: ECOSIM:CATEGORYBiogeochemistry ! category - Biogeochemistry
is_a: ECOSIM:CATEGORYSoilBiogeochemistry ! category - Soil Biogeochemistry
is_a: ECOSIM:CATEGORYSoilProperty ! category - soil property
relationship: attribute ECOSIMCONCEPT:Content ! Content
relationship: has_unit ECOSIM:mgkg-1 ! mg kg-1
relationship: measured_in ECOSIMCONCEPT:Soil ! Soil
relationship: measurement_of ECOSIMCONCEPT:Calcium ! Calcium

[Term]
id: ECOSIM:CCACO
name: soil CaCO3 content
def: "Soil CaCO3 content refers to the concentration or percentage of calcium carbonate (CaCO3) present in the soil. It is an important parameter in Earth systems modeling as it influences various soil properties and processes, such as soil pH, nutrient availability, water retention capacity, and soil carbon cycling. Soil CaCO3 content can be obtained through laboratory analysis or estimated using models based on soil properties and environmental conditions." []
is_a: ECOSIM:CATEGORYBiogeochemistry ! category - Biogeochemistry
is_a: ECOSIM:CATEGORYSoilBiogeochemistry ! category - Soil Biogeochemistry
is_a: ECOSIM:CATEGORYSoilProperty ! category - soil property
relationship: attribute ECOSIMCONCEPT:Content ! Content
relationship: has_unit ECOSIM:mgkg-1 ! mg kg-1
relationship: measured_in ECOSIMCONCEPT:Soil ! Soil
relationship: measurement_of ECOSIMCONCEPT:CaCO3 ! Calcium carbonate

[Term]
id: ECOSIM:CCACQ
name: surface irrigation CaCO3 concentration
def: "Surface irrigation CaCO3 concentration refers to the amount of calcium carbonate (CaCO3) present in the water used for surface irrigation of agricultural fields. It represents the concentration of this mineral compound, which can influence the water quality and its potential to cause scaling or clogging in irrigation systems. Monitoring and modeling surface irrigation CaCO3 concentration is important for understanding its impact on soil properties, nutrient availability, crop growth, and the overall sustainability of agricultural practices." []
is_a: ECOSIMCONCEPT:UnclassifiedVariable ! unclassified variable
relationship: attribute ECOSIMCONCEPT:Concentration ! Concentration
relationship: context ECOSIMCONCEPT:Irrigation ! Irrigation
relationship: has_unit ECOSIM:gm-3 ! g m-3
relationship: measured_in ECOSIMCONCEPT:Surface ! Surface
relationship: measurement_of ECOSIMCONCEPT:CaCO3 ! Calcium carbonate

[Term]
id: ECOSIM:CCACR
name: precipitation CaCO3 concentration
def: "Precipitation CaCO3 concentration refers to the measurement of the concentration of calcium carbonate (CaCO3) in the water that is formed during the process of precipitation in an Earth system model. It indicates the amount of CaCO3 dissolved in the water, which can have implications for various biogeochemical processes and cycles, including the formation of sedimentary rocks, ocean pH levels, and the carbon cycle. The precipitation CaCO3 concentration parameter helps to understand and model the dynamics of CaCO3 in Earth's systems, particularly in relation to climate change and its effects on the environment." []
is_a: ECOSIM:CATEGORYAtmosphericConditions ! category - Atmospheric Conditions
is_a: ECOSIM:CATEGORYDepositionFlux ! category - deposition flux
relationship: attribute ECOSIMCONCEPT:Concentration ! Concentration
relationship: context ECOSIMCONCEPT:Precipitation ! Precipitation
relationship: has_unit ECOSIM:gm-3 ! g m-3
relationship: measured_in ECOSIMCONCEPT:Water ! Water
relationship: measurement_of ECOSIMCONCEPT:CaCO3 ! Calcium carbonate

[Term]
id: ECOSIM:CCACU
name: subsurface irrigation CaCO3 concentration
def: "Subsurface irrigation CaCO3 concentration refers to the measurement or representation of the concentration of calcium carbonate (CaCO3) in the subsurface irrigation water. It indicates the amount of dissolved calcium carbonate in the water used for subsurface irrigation, which can affect soil fertility and the infiltration and drainage patterns of water in the subsurface. This parameter is important in earth system modeling as it can help understand the potential effects of subsurface irrigation on soil chemistry and water availability for plants." []
is_a: ECOSIMCONCEPT:UnclassifiedVariable ! unclassified variable
relationship: attribute ECOSIMCONCEPT:Concentration ! Concentration
relationship: context ECOSIMCONCEPT:Irrigation ! Irrigation
relationship: has_unit ECOSIM:gm-3 ! g m-3
relationship: measured_in ECOSIMCONCEPT:Subsurface ! Subsurface
relationship: measurement_of ECOSIMCONCEPT:CaCO3 ! Calcium carbonate

[Term]
id: ECOSIM:CCAHQ
name: surface irrigation CaHCO3 concentration
def: "Surface irrigation CaHCO3 concentration refers to the concentration of calcium bicarbonate (CaHCO3) in water used for surface irrigation. Surface irrigation is a method of watering crops where water is distributed over the soil surface and allowed to infiltrate into the root zone. The CaHCO3 concentration in the irrigation water can affect soil pH, nutrient availability, and plant growth. Monitoring this parameter is important for understanding the potential impacts of water quality on agricultural productivity and soil health in surface irrigation systems." []
is_a: ECOSIMCONCEPT:UnclassifiedVariable ! unclassified variable
relationship: attribute ECOSIMCONCEPT:Concentration ! Concentration
relationship: context ECOSIMCONCEPT:Irrigation ! Irrigation
relationship: has_unit ECOSIM:gm-3 ! g m-3
relationship: measured_in ECOSIMCONCEPT:Surface ! Surface
relationship: measurement_of ECOSIMCONCEPT:CaHCO3 ! Calcium bicarbonate

[Term]
id: ECOSIM:CCAHR
name: precipitation CaHCO3 concentration
def: "Precipitation CaHCO3 concentration refers to the concentration of calcium bicarbonate (CaHCO3) in the rainfall or snowfall that is deposited on the Earth's surface. It represents the amount of calcium bicarbonate dissolved in the water present in precipitation events. This parameter is important in earth systems modeling as it affects the chemical composition and pH of soil and water systems, which in turn can impact various ecological processes, nutrient availability, and aquatic ecosystems." []
is_a: ECOSIM:CATEGORYAtmosphericConditions ! category - Atmospheric Conditions
relationship: attribute ECOSIMCONCEPT:Concentration ! Concentration
relationship: has_unit ECOSIM:gm-3 ! g m-3
relationship: measured_in ECOSIMCONCEPT:Precipitation ! Precipitation
relationship: measurement_of ECOSIMCONCEPT:CaHCO3 ! Calcium bicarbonate

[Term]
id: ECOSIM:CCAHU
name: subsurface irrigation CaHCO3 concentration
def: "Subsurface irrigation CaHCO3 concentration refers to the concentration of calcium bicarbonate (CaHCO3) in the irrigation water used for subsurface irrigation. It is a parameter that characterizes the amount of dissolved calcium bicarbonate present in the irrigation water, which can have an impact on the chemical composition of the subsurface soil and the overall hydrological and nutrient dynamics in the irrigated area. This parameter is important to consider in earth systems modeling as it can affect plant growth, soil fertility, and water quality." []
is_a: ECOSIMCONCEPT:UnclassifiedVariable ! unclassified variable
relationship: attribute ECOSIMCONCEPT:Concentration ! Concentration
relationship: context ECOSIMCONCEPT:Irrigation ! Irrigation
relationship: has_unit ECOSIM:gm-3 ! g m-3
relationship: measured_in ECOSIMCONCEPT:Subsurface ! Subsurface
relationship: measurement_of ECOSIMCONCEPT:CaHCO3 ! Calcium bicarbonate

[Term]
id: ECOSIM:CCAOQ
name: surface irrigation CaOH concentration
def: "Surface irrigation CaOH concentration refers to the concentration of calcium hydroxide (CaOH) in the water used for surface irrigation. It is a parameter that affects the quality of the irrigation water and can have an impact on soil pH and nutrient availability for plants. The CaOH concentration is typically measured in units of mass per volume (e.g., mg/L) and is an important parameter to consider when assessing the potential effects of irrigation water on crop growth and soil chemistry." []
is_a: ECOSIMCONCEPT:UnclassifiedVariable ! unclassified variable
relationship: attribute ECOSIMCONCEPT:Concentration ! Concentration
relationship: context ECOSIMCONCEPT:Irrigation ! Irrigation
relationship: has_unit ECOSIM:gm-3 ! g m-3
relationship: measured_in ECOSIMCONCEPT:SurfaceIrrigation ! SurfaceIrrigation
relationship: measurement_of ECOSIMCONCEPT:CaOH ! Calcium hydroxide

[Term]
id: ECOSIM:CCAOR
name: precipitation CaOH concentration
def: "Precipitation CaOH concentration refers to the concentration of calcium hydroxide (CaOH) in precipitation. CaOH is a chemical compound that can be present in precipitation due to anthropogenic or natural sources. The precipitation CaOH concentration is a parameter that can be measured and analyzed to understand the impact of CaOH on various Earth system processes, such as hydrological cycles, water quality, and ecosystem dynamics. It is an important parameter in Earth system modeling as it helps in simulating and predicting the distribution and impact of CaOH in different regions and its interactions with other components of the Earth system." []
is_a: ECOSIM:CATEGORYAtmosphericConditions ! category - Atmospheric Conditions
is_a: ECOSIM:CATEGORYDepositionFlux ! category - deposition flux
relationship: attribute ECOSIMCONCEPT:Concentration ! Concentration
relationship: context ECOSIMCONCEPT:Precipitation ! Precipitation
relationship: has_unit ECOSIM:gm-3 ! g m-3
relationship: measured_in ECOSIMCONCEPT:Water ! Water
relationship: measurement_of ECOSIMCONCEPT:CaOH ! Calcium hydroxide

[Term]
id: ECOSIM:CCAOU
name: subsurface irrigation CaOH concentration
def: "Subsurface irrigation CaOH concentration refers to the concentration of calcium hydroxide (CaOH) in the irrigation water that is applied below the surface of the soil. This parameter is relevant in earth systems modeling as it impacts soil chemistry and nutrient availability to plants. The CaOH concentration can influence soil pH, nutrient uptake by plant roots, and overall plant growth. Tracking and analyzing this parameter can help in understanding and simulating the effects of subsurface irrigation on agricultural systems and water quality." []
is_a: ECOSIMCONCEPT:UnclassifiedVariable ! unclassified variable
relationship: attribute ECOSIMCONCEPT:Concentration ! Concentration
relationship: context ECOSIMCONCEPT:Irrigation ! Irrigation
relationship: has_unit ECOSIM:gm-3 ! g m-3
relationship: measured_in ECOSIMCONCEPT:Subsurface ! Subsurface
relationship: measurement_of ECOSIMCONCEPT:CaOH ! Calcium hydroxide

[Term]
id: ECOSIM:CCAPD
name: soil CaHPO4 content
def: "Soil CaHPO4 content refers to the concentration or amount of calcium hydrogen phosphate (CaHPO4) present in the soil. It is a parameter that is used in earth systems modeling to represent the level of CaHPO4 in the soil, which can influence soil fertility, nutrient availability, and plant growth. The measurement of soil CaHPO4 content helps in understanding the nutrient cycling and dynamics within an ecosystem, and it is essential for accurately simulating and predicting the behavior of earth systems." []
is_a: ECOSIM:CATEGORYBiogeochemistry ! category - Biogeochemistry
is_a: ECOSIM:CATEGORYSoilProperty ! category - soil property
relationship: attribute ECOSIMCONCEPT:Content ! Content
relationship: has_unit ECOSIM:mgkg-1 ! mg kg-1
relationship: measured_in ECOSIMCONCEPT:Soil ! Soil
relationship: measurement_of ECOSIMCONCEPT:CaHPO4 ! CaHPO4

[Term]
id: ECOSIM:CCAPH
name: soil apatite content
def: "Soil apatite content refers to the amount or concentration of apatite minerals found in the soil. Apatite is a group of phosphate minerals that contain phosphorus, calcium, and other elements. It is an important component of many soils and plays a role in the biogeochemical cycling of phosphorus and the availability of this essential nutrient for plant growth. The measurement of soil apatite content is important in earth systems modeling as it provides information about the phosphorus dynamics and availability in the soil, which is crucial for understanding nutrient cycling, ecosystem productivity, and plant growth." []
is_a: ECOSIM:CATEGORYBiogeochemistry ! category - Biogeochemistry
is_a: ECOSIM:CATEGORYSoilBiogeochemistry ! category - Soil Biogeochemistry
is_a: ECOSIM:CATEGORYSoilProperty ! category - soil property
relationship: attribute ECOSIMCONCEPT:Content ! Content
relationship: has_unit ECOSIM:mgkg-1 ! mg kg-1
relationship: measured_in ECOSIMCONCEPT:Soil ! Soil
relationship: measurement_of ECOSIMCONCEPT:Apatite ! Apatite

[Term]
id: ECOSIM:CCAQ
name: surface irrigation Ca concentration
def: "Surface irrigation Ca concentration refers to the concentration of calcium (Ca) in the water used for surface irrigation in agricultural systems. It represents the amount of dissolved calcium ions present in the irrigation water, which can impact the soil chemistry and fertility. The Ca concentration in surface irrigation water is an important parameter to consider in Earth systems modeling, as it can influence soil structure, nutrient availability, and plant growth." []
is_a: ECOSIMCONCEPT:UnclassifiedVariable ! unclassified variable
relationship: attribute ECOSIMCONCEPT:Concentration ! Concentration
relationship: has_unit ECOSIM:gm-3 ! g m-3
relationship: measured_in ECOSIMCONCEPT:SurfaceIrrigation ! SurfaceIrrigation
relationship: measurement_of ECOSIMCONCEPT:Calcium ! Calcium

[Term]
id: ECOSIM:CCAR
name: precipitation Ca concentration
def: "The term 'precipitation Ca concentration' refers to the amount of calcium (Ca) present in precipitation. It represents the concentration of calcium ions in rainfall, snowfall, or any form of atmospheric moisture that reaches the Earth's surface. The precipitation Ca concentration is an important parameter in earth systems modeling as it influences various biogeochemical processes, including nutrient cycling, soil composition, and ecosystem health. It is typically quantified as the mass of calcium per unit volume of precipitation, such as milligrams per liter (mg/L) or parts per million (ppm)." []
is_a: ECOSIM:CATEGORYAtmosphericConditions ! category - Atmospheric Conditions
is_a: ECOSIM:CATEGORYDepositionFlux ! category - deposition flux
relationship: attribute ECOSIMCONCEPT:Concentration ! Concentration
relationship: context ECOSIMCONCEPT:Precipitation ! Precipitation
relationship: has_unit ECOSIM:gm-3 ! g m-3
relationship: measured_in ECOSIMCONCEPT:Water ! Water
relationship: measurement_of ECOSIMCONCEPT:Calcium ! Calcium

[Term]
id: ECOSIM:CCASO
name: soil CaSO4 content
def: "Soil CaSO4 content refers to the concentration of calcium sulfate (CaSO4) in the soil. Calcium sulfate is a common mineral in soils and can play a significant role in soil fertility and nutrient availability. It affects soil structure, water holding capacity, and the balance of essential nutrients for plant growth. The soil CaSO4 content is an important parameter in earth systems modeling as it influences various soil processes and the overall functioning of ecosystems." []
is_a: ECOSIM:CATEGORYBiogeochemistry ! category - Biogeochemistry
is_a: ECOSIM:CATEGORYSoilBiogeochemistry ! category - Soil Biogeochemistry
is_a: ECOSIM:CATEGORYSoilProperty ! category - soil property
relationship: attribute ECOSIMCONCEPT:Content ! Content
relationship: has_unit ECOSIM:mgkg-1 ! mg kg-1
relationship: measured_in ECOSIMCONCEPT:Soil ! Soil
relationship: measurement_of ECOSIMCONCEPT:CaSO4 ! Calcium sulfate

[Term]
id: ECOSIM:CCASQ
name: surface irrigation CaSO4 concentration
def: "Surface irrigation CaSO4 concentration refers to the amount of calcium sulfate (CaSO4) present in the water used for surface irrigation. It represents the concentration of CaSO4 in the irrigation water that is applied to the soil surface to irrigate crops or vegetation. This parameter is important in earth systems modeling as it can affect various processes such as soil salinity, nutrient availability, and crop growth. High concentrations of CaSO4 can lead to increased salinity in the soil, which can negatively impact plant water uptake and overall crop productivity. Monitoring and understanding the surface irrigation CaSO4 concentration can help in predicting and managing the potential effects on agricultural systems and water resources." []
is_a: ECOSIMCONCEPT:UnclassifiedVariable ! unclassified variable
relationship: attribute ECOSIMCONCEPT:Concentration ! Concentration
relationship: context ECOSIMCONCEPT:Irrigation ! Irrigation
relationship: has_unit ECOSIM:gm-3 ! g m-3
relationship: measured_in ECOSIMCONCEPT:Surface ! Surface
relationship: measurement_of ECOSIMCONCEPT:CaSO4 ! Calcium sulfate

[Term]
id: ECOSIM:CCASR
name: precipitation CaSO4 concentration
def: "Precipitation CaSO4 concentration refers to the concentration of calcium sulfate (CaSO4) in the rainwater or snowfall. It represents the amount of CaSO4 present in a given volume of precipitation, usually measured in milligrams per liter (mg/L) or parts per million (ppm). This parameter is important in earth systems modeling as it can impact the quality of water resources, soil chemistry, and ecosystems, especially in regions where calcium sulfate is naturally occurring or where there is anthropogenic deposition of CaSO4 into the atmosphere." []
is_a: ECOSIM:CATEGORYAtmosphericConditions ! category - Atmospheric Conditions
relationship: attribute ECOSIMCONCEPT:Concentration ! Concentration
relationship: has_unit ECOSIM:gm-3 ! g m-3
relationship: measured_in ECOSIMCONCEPT:Precipitation ! Precipitation
relationship: measurement_of ECOSIMCONCEPT:CaSO4 ! Calcium sulfate

[Term]
id: ECOSIM:CCASU
name: subsurface irrigation CaSO4 concentration
def: "Subsurface irrigation CaSO4 concentration refers to the concentration of calcium sulfate (CaSO4) in the water used for subsurface irrigation systems. It represents the amount of calcium sulfate dissolved in the water that is being distributed in underground pipes or channels to deliver water directly to the roots of plants. This parameter is important to monitor and control because it can affect the soil chemistry and fertility, as well as plant health and productivity." []
is_a: ECOSIMCONCEPT:UnclassifiedVariable ! unclassified variable
relationship: attribute ECOSIMCONCEPT:Concentration ! Concentration
relationship: context ECOSIMCONCEPT:Irrigation ! Irrigation
relationship: has_unit ECOSIM:gm-3 ! g m-3
relationship: measured_in ECOSIMCONCEPT:Subsurface ! Subsurface
relationship: measurement_of ECOSIMCONCEPT:CaSO4 ! Calcium sulfate

[Term]
id: ECOSIM:CCAU
name: subsurface irrigation Mg concentration
def: "Subsurface irrigation Mg concentration refers to the measurement of the concentration of Magnesium (Mg) in the soil solution or water used for subsurface irrigation. It is a parameter used in earth systems modeling to understand the distribution and availability of Magnesium in soil and its impact on plant growth and nutrient cycling. The Mg concentration can influence soil fertility, nutrient uptake by plants, and can be used to assess the potential for Mg deficiency or toxicity in agricultural systems utilizing subsurface irrigation." []
is_a: ECOSIMCONCEPT:UnclassifiedVariable ! unclassified variable
relationship: attribute ECOSIMCONCEPT:Concentration ! Concentration
relationship: context ECOSIMCONCEPT:Irrigation ! Irrigation
relationship: has_unit ECOSIM:gm-3 ! g m-3
relationship: measured_in ECOSIMCONCEPT:Subsurface ! Subsurface
relationship: measurement_of ECOSIMCONCEPT:Mg ! Magnesium

[Term]
id: ECOSIM:CCHQ
name: surface irrigation CH4 concentration
def: "Surface irrigation CH4 concentration refers to the measurement of the concentration of methane (CH4) in the atmosphere in a specific area where surface irrigation is being practiced. This parameter is important for earth systems modeling as CH4 is a potent greenhouse gas that significantly contributes to global warming. Monitoring surface irrigation CH4 concentration helps to understand the impact of agricultural practices on CH4 emissions and aids in assessing the overall carbon balance in the atmosphere." []
is_a: ECOSIMCONCEPT:UnclassifiedVariable ! unclassified variable
relationship: attribute ECOSIMCONCEPT:Concentration ! Concentration
relationship: context ECOSIMCONCEPT:Irrigation ! Irrigation
relationship: has_unit ECOSIM:gm-3 ! g m-3
relationship: measured_in ECOSIMCONCEPT:Surface ! Surface
relationship: measurement_of ECOSIMCONCEPT:CH4 ! Methane

[Term]
id: ECOSIM:CCHR
name: precipitation CH4 concentration
def: "Precipitation CH4 concentration refers to the concentration of methane (CH4) in the atmosphere that is influenced by precipitation patterns. This parameter captures the amount of methane dissolved or absorbed in precipitation, which can be deposited on the Earth's surface during rainfall events. It is an essential parameter for Earth system models as methane is a potent greenhouse gas and plays a significant role in climate change." []
is_a: ECOSIM:CATEGORYAtmosphericConditions ! category - Atmospheric Conditions
is_a: ECOSIM:CATEGORYDepositionFlux ! category - deposition flux
relationship: attribute ECOSIMCONCEPT:Concentration ! Concentration
relationship: context ECOSIMCONCEPT:Precipitation ! Precipitation
relationship: has_unit ECOSIM:gm-3 ! g m-3
relationship: measured_in ECOSIMCONCEPT:Atmosphere ! Atmosphere
relationship: measurement_of ECOSIMCONCEPT:CH4 ! Methane

[Term]
id: ECOSIM:CCL
name: soil Cl content
def: "Soil Cl content refers to the concentration or amount of chloride (Cl) present in the soil. It is a parameter that characterizes the level of chloride ions in the soil system. The soil Cl content is an important parameter in earth system modeling as it can influence various processes such as nutrient cycling, plant growth, and soil salinity. Measurement of soil Cl content is typically done through laboratory analysis or remote sensing techniques." []
is_a: ECOSIM:CATEGORYBiogeochemistry ! category - Biogeochemistry
is_a: ECOSIM:CATEGORYSoilProperty ! category - soil property
relationship: attribute ECOSIMCONCEPT:Content ! Content
relationship: has_unit ECOSIM:mgkg-1 ! mg kg-1
relationship: measured_in ECOSIMCONCEPT:Soil ! Soil
relationship: measurement_of ECOSIMCONCEPT:Chloride ! Chloride

[Term]
id: ECOSIM:CCLQ
name: surface irrigation Cl concentration
def: "Surface irrigation Cl concentration refers to the concentration of chloride (Cl) ions in the water used for surface irrigation. It is a parameter that describes the amount of chloride present in the irrigation water, which can have implications for soil fertility and plant health. High levels of Cl in irrigation water can lead to salinity issues, affecting crop growth and soil quality. Monitoring and managing surface irrigation Cl concentration is important for sustainable agriculture practices and efficient water management in earth systems modeling." []
is_a: ECOSIMCONCEPT:UnclassifiedVariable ! unclassified variable
relationship: attribute ECOSIMCONCEPT:Concentration ! Concentration
relationship: has_unit ECOSIM:gm-3 ! g m-3
relationship: measured_in ECOSIMCONCEPT:SurfaceIrrigation ! SurfaceIrrigation
relationship: measurement_of ECOSIMCONCEPT:Chloride ! Chloride

[Term]
id: ECOSIM:CCLR
name: precipitation Cl concentration
def: "Precipitation Cl concentration refers to the amount of chloride (Cl) present in precipitation, which is the water that falls to the Earth's surface in the form of rain, snow, sleet, or hail. This parameter quantifies the concentration of chloride ions in the precipitation, indicating the amount of dissolved chloride in the atmospheric moisture. The Cl concentration in precipitation plays a crucial role in various environmental processes and can affect hydrological cycles, ecosystem health, and the chemistry of soils and water bodies. Monitoring and understanding precipitation Cl concentration is important for assessing the impacts of atmospheric deposition, such as acid rain or the transport of pollutants, on natural and human systems." []
is_a: ECOSIM:CATEGORYAtmosphericConditions ! category - Atmospheric Conditions
is_a: ECOSIM:CATEGORYDepositionFlux ! category - deposition flux
relationship: attribute ECOSIMCONCEPT:Concentration ! Concentration
relationship: has_unit ECOSIM:gm-3 ! g m-3
relationship: measured_in ECOSIMCONCEPT:Percipitation ! Percipitation
relationship: measurement_of ECOSIMCONCEPT:Chloride ! Chloride

[Term]
id: ECOSIM:CCLU
name: subsurface irrigation CO3 concentration
def: "Subsurface irrigation CO3 concentration refers to the level of carbonate ions (CO3) present in the soil water in a subsurface irrigation system. It represents the amount of dissolved carbonate compounds, such as calcium carbonate, in the water that is being used for irrigation purposes. The CO3 concentration can have important implications for soil and plant health, as well as for the efficiency of nutrient uptake by plants. It is a parameter that can be measured and monitored in earth systems models to simulate and understand the impacts of subsurface irrigation on carbonate levels and their influence on agricultural ecosystems." []
is_a: ECOSIMCONCEPT:UnclassifiedVariable ! unclassified variable
relationship: attribute ECOSIMCONCEPT:Concentration ! Concentration
relationship: context ECOSIMCONCEPT:Irrigation ! Irrigation
relationship: has_unit ECOSIM:gm-3 ! g m-3
relationship: measured_in ECOSIMCONCEPT:Subsurface ! Subsurface
relationship: measurement_of ECOSIMCONCEPT:CO3 ! Carbonate

[Term]
id: ECOSIM:CCO2EI
name: initial atmospheric CO2 concentration
def: "The initial atmospheric CO2 concentration refers to the starting concentration of carbon dioxide (CO2) in the Earth's atmosphere at the beginning of a simulation or modeling experiment. It represents the baseline level of CO2 before any external factors (such as human activities) influence its concentration. The initial atmospheric CO2 concentration is an important parameter in earth systems modeling as it affects several processes, including climate change, air quality, and carbon cycle dynamics." []
is_a: ECOSIM:CATEGORYAtmosphericConditions ! category - Atmospheric Conditions
is_a: ECOSIMCONCEPT:UnclassifiedVariable ! unclassified variable
relationship: attribute ECOSIMCONCEPT:Concentration ! Concentration
relationship: has_unit ECOSIM:gCm-3 ! gC m-3
relationship: measured_in ECOSIMCONCEPT:Atmosphere ! Atmosphere
relationship: measurement_of ECOSIMCONCEPT:CO2 ! Carbon dioxide

[Term]
id: ECOSIM:CCOQ
name: surface irrigation CO2 concentration
def: "Surface irrigation CO2 concentration refers to the concentration of carbon dioxide (CO2) in the irrigation water used for surface irrigation methods. Surface irrigation involves the application of water directly onto the soil surface, and the CO2 concentration in the water can influence various biogeochemical processes in the soil and plants. This parameter is important for understanding the potential impacts of elevated CO2 levels on agricultural productivity, water use efficiency, and the soil carbon cycle in surface-irrigated ecosystems." []
is_a: ECOSIMCONCEPT:UnclassifiedVariable ! unclassified variable
relationship: attribute ECOSIMCONCEPT:Concentration ! Concentration
relationship: context ECOSIMCONCEPT:Irrigation ! Irrigation
relationship: has_unit ECOSIM:gm-3 ! g m-3
relationship: measured_in ECOSIMCONCEPT:Surface ! Surface
relationship: measurement_of ECOSIMCONCEPT:CO2 ! Carbon dioxide

[Term]
id: ECOSIM:CCOR
name: precipitation CO2 concentration
def: "Precipitation CO2 concentration refers to the level of carbon dioxide (CO2) present in the atmosphere that influences precipitation patterns. It is a parameter used in earth system models to simulate the impact of changing CO2 concentrations on the hydrological cycle and rainfall. By adjusting the CO2 concentration in the models, researchers can assess how variations in atmospheric CO2 levels affect precipitation and study the potential feedback mechanisms between climate change and the carbon cycle." []
is_a: ECOSIM:CATEGORYAtmosphericConditions ! category - Atmospheric Conditions
is_a: ECOSIM:CATEGORYDepositionFlux ! category - deposition flux
relationship: attribute ECOSIMCONCEPT:Concentration ! Concentration
relationship: has_unit ECOSIM:gm-3 ! g m-3
relationship: measured_in ECOSIMCONCEPT:Precipitation ! Precipitation
relationship: measurement_of ECOSIMCONCEPT:CO2 ! Carbon dioxide

[Term]
id: ECOSIM:CEPOLB
name: branch nonstructural C concentration
def: "Branch nonstructural C concentration refers to the amount of nonstructural carbon (C) present in branches of vegetation. Nonstructural carbon refers to carbon that is not incorporated into structural components such as cellulose, lignin, and other complex molecules. It includes soluble sugars, starches, organic acids, and other compounds that can be rapidly metabolized and used for energy production or growth. The concentration of nonstructural carbon in branches is an important parameter as it affects the overall carbon balance of vegetation and influences various biophysical and biogeochemical processes in the Earth system, such as respiration, photosynthesis, and carbon storage." []
is_a: ECOSIM:CATEGORYPlantPhysiology ! category - plant physiology
is_a: ECOSIMCONCEPT:UnclassifiedVariable ! unclassified variable
relationship: attribute ECOSIMCONCEPT:Concentration ! Concentration
relationship: has_unit ECOSIM:gd-2 ! g d-2
relationship: measured_in ECOSIMCONCEPT:Branch ! Branch
relationship: measurement_of ECOSIMCONCEPT:Carbon ! Carbon

[Term]
id: ECOSIM:CER
name: soil detachment/deposition
def: "Soil detachment/deposition refers to the process of soil particles being eroded (detached) by water or wind and subsequently being transported and deposited in another location. This process plays a significant role in shaping the Earth's surface and impacting the distribution of soil across different regions. Soil detachment may occur through various mechanisms, including raindrop impact, surface runoff, or wind erosion, while deposition can occur in bodies of water, such as rivers or lakes, or on land surfaces, such as floodplains or dunes. Modeling soil detachment/deposition helps in understanding erosion patterns, soil loss rates, and predicting the impacts of land management practices or climate change on soil erosion." []
is_a: ECOSIMCONCEPT:UnclassifiedVariable ! unclassified variable

[Term]
id: ECOSIM:CF1PQ
name: surface irrigation FeHPO4 concentration
def: "Surface irrigation FeHPO4 concentration refers to the concentration of iron phosphate (FeHPO4) in the water used for surface irrigation. Surface irrigation is a method of applying water to crops or vegetation by allowing it to flow over the soil surface. FeHPO4 is a compound containing iron and phosphate, and its concentration in the irrigation water can impact the availability of these nutrients to plants. Monitoring and modeling the FeHPO4 concentration in surface irrigation helps in understanding the potential impact on the nutrient availability and overall health of the agricultural or natural systems." []
is_a: ECOSIMCONCEPT:UnclassifiedVariable ! unclassified variable
relationship: attribute ECOSIMCONCEPT:Concentration ! Concentration
relationship: context ECOSIMCONCEPT:Irrigation ! Irrigation
relationship: has_unit ECOSIM:gm-3 ! g m-3
relationship: measured_in ECOSIMCONCEPT:Surface ! Surface
relationship: measurement_of ECOSIMCONCEPT:FeHPO4 ! Iron hydrogen phosphate

[Term]
id: ECOSIM:CF1PR
name: precipitation FeHPO4 concentration
def: "Precipitation FeHPO4 concentration refers to the amount of iron phosphate (FeHPO4) that is present in the precipitation, which is the process of water droplets falling from the atmosphere to the Earth's surface. FeHPO4 is a type of mineral that can dissolve in water and be carried in precipitation. Monitoring the concentration of FeHPO4 in precipitation is important for studying the biogeochemical cycles of iron and phosphorus, as well as their impacts on ecosystem productivity and water quality." []
is_a: ECOSIM:CATEGORYDepositionFlux ! category - deposition flux
is_a: ECOSIMCONCEPT:UnclassifiedVariable ! unclassified variable
relationship: attribute ECOSIMCONCEPT:Concentration ! Concentration
relationship: context ECOSIMCONCEPT:Precipitation ! Precipitation
relationship: has_unit ECOSIM:gm-3 ! g m-3
relationship: measured_in ECOSIMCONCEPT:Water ! Water
relationship: measurement_of ECOSIMCONCEPT:FeHPO4 ! Iron hydrogen phosphate

[Term]
id: ECOSIM:CF1PU
name: subsurface irrigation FeHPO4 concentration
def: "Subsurface irrigation FeHPO4 concentration refers to the concentration of FeHPO4 (Iron Hydrogen Phosphate) in the soil or water used for subsurface irrigation. It represents the amount of FeHPO4 present in the irrigation system, which can have an impact on the fertility and overall health of the soil and plants. Monitoring this parameter is essential for understanding nutrient cycling and potential effects on plant growth and agricultural practices." []
is_a: ECOSIMCONCEPT:UnclassifiedVariable ! unclassified variable
relationship: attribute ECOSIMCONCEPT:Concentration ! Concentration
relationship: context ECOSIMCONCEPT:Irrigation ! Irrigation
relationship: has_unit ECOSIM:gm-3 ! g m-3
relationship: measured_in ECOSIMCONCEPT:Subsurface ! Subsurface
relationship: measurement_of ECOSIMCONCEPT:FeHPO4 ! Iron hydrogen phosphate

[Term]
id: ECOSIM:CF2PQ
name: surface irrigation FeH2PO4 concentration
def: "Surface irrigation FeH2PO4 concentration refers to the measurement of the concentration of ferrous dihydrogen phosphate (FeH2PO4) in water used for surface irrigation. It represents the amount of FeH2PO4 present in the water that is applied to the land surface for agricultural purposes using various irrigation techniques, such as furrow or flood irrigation. This parameter is crucial in understanding the nutrient content and potential impact on soil and crop health, as FeH2PO4 serves as a source of essential nutrients for plants. Monitoring this concentration helps assess the effectiveness of surface irrigation practices in delivering proper amounts of FeH2PO4 to support plant growth and optimize agricultural productivity." []
is_a: ECOSIMCONCEPT:UnclassifiedVariable ! unclassified variable
relationship: attribute ECOSIMCONCEPT:Concentration ! Concentration
relationship: context ECOSIMCONCEPT:Irrigation ! Irrigation
relationship: has_unit ECOSIM:gm-3 ! g m-3
relationship: measured_in ECOSIMCONCEPT:Surface ! Surface
relationship: measurement_of ECOSIMCONCEPT:FeH2PO4 ! Iron dihydrogen phosphate

[Term]
id: ECOSIM:CF2PR
name: precipitation FeH2PO4 concentration
def: "Precipitation FeH2PO4 concentration refers to the concentration of ferrous phosphate (FeH2PO4) in precipitation, which is the process of water vapor in the atmosphere condensing and falling to the Earth's surface. This parameter is often measured in units of mass per unit volume (e.g., mg/L) and indicates the amount of FeH2PO4 present in the precipitation. The concentration of FeH2PO4 in precipitation can have significant impacts on the biogeochemical cycling of phosphorus in terrestrial and aquatic ecosystems, influencing nutrient availability and primary productivity." []
is_a: ECOSIM:CATEGORYDepositionFlux ! category - deposition flux
is_a: ECOSIMCONCEPT:UnclassifiedVariable ! unclassified variable
relationship: attribute ECOSIMCONCEPT:Concentration ! Concentration
relationship: context ECOSIMCONCEPT:Precipitation ! Precipitation
relationship: has_unit ECOSIM:gm-3 ! g m-3
relationship: measured_in ECOSIMCONCEPT:Water ! Water
relationship: measurement_of ECOSIMCONCEPT:FeH2PO4 ! Iron dihydrogen phosphate

[Term]
id: ECOSIM:CF2PU
name: subsurface irrigation FeH2PO4 concentration
def: "Subsurface irrigation FeH2PO4 concentration refers to the concentration of FeH2PO4, which is iron phosphate, in the soil water below the surface of the soil. It represents the amount of iron phosphate present in the water used for subsurface irrigation, which can be an important parameter for understanding nutrient availability and potential impacts on plant growth and soil health." []
is_a: ECOSIMCONCEPT:UnclassifiedVariable ! unclassified variable
relationship: attribute ECOSIMCONCEPT:Concentration ! Concentration
relationship: context ECOSIMCONCEPT:Irrigation ! Irrigation
relationship: has_unit ECOSIM:gm-3 ! g m-3
relationship: measured_in ECOSIMCONCEPT:Subsurface ! Subsurface
relationship: measurement_of ECOSIMCONCEPT:FeH2PO4 ! Iron dihydrogen phosphate

[Term]
id: ECOSIM:CFE
name: soil Fe content
def: "Soil Fe content refers to the concentration or amount of iron (Fe) present in the soil. It is an important parameter in earth systems modeling, as it influences various soil processes, such as nutrient cycling, organic matter decomposition, and plant growth. The soil Fe content can vary across different soil types and regions, and it is typically measured in units of mass per unit volume (e.g., g/kg or mg/kg). Understanding and accurately representing the soil Fe content is crucial for studying and simulating the interactions between the soil, vegetation, and climate in earth system models." []
is_a: ECOSIM:CATEGORYBiogeochemistry ! category - Biogeochemistry
is_a: ECOSIM:CATEGORYSoilBiogeochemistry ! category - Soil Biogeochemistry
is_a: ECOSIM:CATEGORYSoilProperty ! category - soil property
relationship: attribute ECOSIMCONCEPT:Content ! Content
relationship: has_unit ECOSIM:mgkg-1 ! mg kg-1
relationship: measured_in ECOSIMCONCEPT:Soil ! Soil
relationship: measurement_of ECOSIMCONCEPT:Iron ! Iron

[Term]
id: ECOSIM:CFE1Q
name: surface irrigation FeOH concentration
def: "Surface irrigation FeOH concentration refers to the concentration of ferric hydroxide (FeOH) in surface water used for irrigation purposes. Ferric hydroxide is a common form of iron oxide that precipitates out of water under certain environmental conditions. This parameter is important in earth systems modeling as it influences the availability of iron (Fe) in the soil, which plays a crucial role in plant growth and nutrient uptake. The concentration of FeOH in surface irrigation water can vary depending on factors such as soil characteristics, water quality, and agricultural practices. Monitoring and modeling this parameter can help assess the potential impacts of surface irrigation on soil health and agricultural productivity." []
is_a: ECOSIMCONCEPT:UnclassifiedVariable ! unclassified variable
relationship: attribute ECOSIMCONCEPT:Concentration ! Concentration
relationship: context ECOSIMCONCEPT:Irrigation ! Irrigation
relationship: has_unit ECOSIM:gm-3 ! g m-3
relationship: measured_in ECOSIMCONCEPT:Surface ! Surface
relationship: measurement_of ECOSIMCONCEPT:FeOH ! Iron hydroxide

[Term]
id: ECOSIM:CFE1R
name: precipitation FeOH concentration
def: "Precipitation FeOH concentration refers to the amount of iron hydroxide (FeOH) present in the rain or snowfall. It is a measure of the concentration of iron hydroxide particles that are dissolved or suspended in the liquid or solid precipitation. This parameter is important as FeOH can play a significant role in various earth system processes, including nutrient cycling, carbon sequestration, and atmospheric chemistry. The precipitation FeOH concentration is typically expressed in units of mass per volume of precipitation." []
is_a: ECOSIM:CATEGORYAtmosphericConditions ! category - Atmospheric Conditions
is_a: ECOSIM:CATEGORYDepositionFlux ! category - deposition flux
relationship: attribute ECOSIMCONCEPT:Concentration ! Concentration
relationship: context ECOSIMCONCEPT:Precipitation ! Precipitation
relationship: has_unit ECOSIM:gm-3 ! g m-3
relationship: measured_in ECOSIMCONCEPT:Water ! Water
relationship: measurement_of ECOSIMCONCEPT:FeOH ! Iron hydroxide

[Term]
id: ECOSIM:CFE1U
name: subsurface irrigation FeOH concentration
def: "Subsurface irrigation FeOH concentration refers to the level of iron oxide hydroxide (FeOH) in the soil when subsurface irrigation is used. Subsurface irrigation involves applying water directly to the root zone of plants through buried pipes or tubes, allowing for more efficient water use and reducing water loss through evaporation. The FeOH concentration parameter quantifies the amount of iron oxide hydroxide in the irrigation water or the soil as a result of subsurface irrigation practices. It is an important parameter to consider as it can affect soil fertility, plant growth, and overall ecosystem health." []
is_a: ECOSIMCONCEPT:UnclassifiedVariable ! unclassified variable
relationship: attribute ECOSIMCONCEPT:Concentration ! Concentration
relationship: context ECOSIMCONCEPT:Irrigation ! Irrigation
relationship: has_unit ECOSIM:gm-3 ! g m-3
relationship: measured_in ECOSIMCONCEPT:Subsurface ! Subsurface
relationship: measurement_of ECOSIMCONCEPT:FeOH ! Iron hydroxide

[Term]
id: ECOSIM:CFE2Q
name: surface irrigation FeOH2 concentration
def: "Surface irrigation FeOH2 concentration refers to the concentration of ferrous hydroxide (FeOH2) in water used for surface irrigation. It represents the amount of dissolved ferrous hydroxide present in the irrigation water, which can have implications for plant nutrient uptake, soil fertility, and water quality. The FeOH2 concentration can impact the availability of iron as a micronutrient for crops and influence various chemical reactions occurring in soil and water systems. Monitoring and understanding this parameter is important for accurate modeling of agricultural systems and their interactions with the environment." []
is_a: ECOSIMCONCEPT:UnclassifiedVariable ! unclassified variable
relationship: attribute ECOSIMCONCEPT:Concentration ! Concentration
relationship: context ECOSIMCONCEPT:Irrigation ! Irrigation
relationship: has_unit ECOSIM:gm-3 ! g m-3
relationship: measured_in ECOSIMCONCEPT:Surface ! Surface
relationship: measurement_of ECOSIMCONCEPT:FeOH2 ! Iron dihydroxide

[Term]
id: ECOSIM:CFE2R
name: precipitation FeOH2 concentration
def: "Precipitation FeOH2 concentration refers to the amount of iron hydroxide (FeOH2) present in the precipitation or rainwater. It represents the concentration of dissolved iron hydroxide particles in the rain, which can be an important parameter in earth systems modeling, as iron is a critical micronutrient for many ecosystems and can impact various biogeochemical cycles, such as carbon and nitrogen cycles." []
is_a: ECOSIM:CATEGORYAtmosphericConditions ! category - Atmospheric Conditions
is_a: ECOSIM:CATEGORYDepositionFlux ! category - deposition flux
relationship: attribute ECOSIMCONCEPT:Concentration ! Concentration
relationship: context ECOSIMCONCEPT:Precipitation ! Precipitation
relationship: has_unit ECOSIM:gm-3 ! g m-3
relationship: measured_in ECOSIMCONCEPT:Water ! Water
relationship: measurement_of ECOSIMCONCEPT:FeOH2 ! Iron dihydroxide

[Term]
id: ECOSIM:CFE2U
name: subsurface irrigation FeOH2 concentration
def: "Subsurface irrigation FeOH2 concentration refers to the concentration of ferrous hydroxide (FeOH2) in the subsurface soil layer influenced by irrigation. It represents the amount of ferrous ions (Fe2+) that have reacted with hydroxide ions (OH-) in the soil, forming the FeOH2 compound. This parameter is significant in earth systems modeling, particularly for the assessment of nutrient availability, redox reactions, and biogeochemical cycles in the subsurface environment. It can influence soil fertility, plant nutrient uptake, and overall ecosystem dynamics." []
is_a: ECOSIMCONCEPT:Concentration ! Concentration
is_a: ECOSIMCONCEPT:UnclassifiedVariable ! unclassified variable
relationship: has_unit ECOSIM:gm-3 ! g m-3
relationship: measured_in ECOSIMCONCEPT:SubsurfaceIrrigation ! SubsurfaceIrrigation
relationship: measurement_of ECOSIMCONCEPT:FeOH2 ! Iron dihydroxide

[Term]
id: ECOSIM:CFE3Q
name: surface irrigation FeOH3 concentration
def: "Surface irrigation FeOH3 concentration refers to the concentration of FeOH3 (iron oxyhydroxide) in the water used for surface irrigation. This parameter is relevant for Earth system modeling as it influences the availability of iron in the soil and its subsequent impact on plant growth and nutrient cycling. The concentration of FeOH3 can vary depending on factors such as soil properties, water quality, and agricultural practices." []
is_a: ECOSIMCONCEPT:UnclassifiedVariable ! unclassified variable
relationship: attribute ECOSIMCONCEPT:Concentration ! Concentration
relationship: context ECOSIMCONCEPT:Irrigation ! Irrigation
relationship: has_unit ECOSIM:gm-3 ! g m-3
relationship: measured_in ECOSIMCONCEPT:Surface ! Surface
relationship: measurement_of ECOSIMCONCEPT:FeOH3 ! Iron trihydroxide

[Term]
id: ECOSIM:CFE3R
name: precipitation FeOH3 concentration
def: "Precipitation FeOH3 concentration refers to the amount of FeOH3 (iron hydroxide) dissolved in precipitation, which is a measure of the concentration of iron (Fe) in its oxidized form (Fe(III)) in rainwater. This parameter is important in Earth Systems Modeling as it can influence biogeochemical processes such as nutrient availability, ecosystem productivity, and the formation of iron-rich soils. Precipitation FeOH3 concentration is typically expressed in units of mass per unit volume, such as micrograms per liter (µg/L) or parts per billion (ppb)." []
is_a: ECOSIM:CATEGORYAtmosphericConditions ! category - Atmospheric Conditions
is_a: ECOSIM:CATEGORYDepositionFlux ! category - deposition flux
relationship: attribute ECOSIMCONCEPT:Concentration ! Concentration
relationship: context ECOSIMCONCEPT:Precipitation ! Precipitation
relationship: has_unit ECOSIM:gm-3 ! g m-3
relationship: measured_in ECOSIMCONCEPT:Water ! Water
relationship: measurement_of ECOSIMCONCEPT:FeOH3 ! Iron trihydroxide

[Term]
id: ECOSIM:CFE3U
name: subsurface irrigation FeOH3 concentration
def: "Subsurface irrigation FeOH3 concentration refers to the concentration of Iron (III) hydroxide (FeOH3) in the soil matrix resulting from the application of water or liquid fertilizer through a subsurface irrigation system. It indicates the level of FeOH3 present in the soil, which is essential for understanding the binding and transport of iron in an agricultural or ecosystem model. This parameter plays a crucial role in simulating the biogeochemical processes and nutrient cycling in the soil, as well as evaluating the potential impact of subsurface irrigation on the availability and distribution of iron in the soil profile." []
is_a: ECOSIMCONCEPT:UnclassifiedVariable ! unclassified variable
relationship: attribute ECOSIMCONCEPT:Concentration ! Concentration
relationship: context ECOSIMCONCEPT:Irrigation ! Irrigation
relationship: has_unit ECOSIM:gm-3 ! g m-3
relationship: measured_in ECOSIMCONCEPT:Subsurface ! Subsurface
relationship: measurement_of ECOSIMCONCEPT:FeOH3 ! Iron trihydroxide

[Term]
id: ECOSIM:CFE4Q
name: surface irrigation FeOH4 concentration
def: "Surface irrigation FeOH4 concentration refers to the concentration of iron hydroxide (FeOH4) in the water used for surface irrigation. It represents the amount of FeOH4 suspended in the water and is measured in units of mass per unit volume (e.g., milligrams per liter). FeOH4 concentration is an important parameter in earth systems modeling as it can affect the chemical composition and nutrient availability of the irrigation water, as well as the potential impacts on soil quality and ecosystem health." []
is_a: ECOSIMCONCEPT:UnclassifiedVariable ! unclassified variable
relationship: attribute ECOSIMCONCEPT:Concentration ! Concentration
relationship: context ECOSIMCONCEPT:Irrigation ! Irrigation
relationship: has_unit ECOSIM:gm-3 ! g m-3
relationship: measured_in ECOSIMCONCEPT:Surface ! Surface
relationship: measurement_of ECOSIMCONCEPT:FeOH4 ! Iron tetrahydroxide

[Term]
id: ECOSIM:CFE4R
name: precipitation FeOH4 concentration
def: "Precipitation FeOH4 concentration refers to the amount of iron oxyhydroxide (FeOH4) present in the precipitation (rainfall or snow). It represents the concentration of FeOH4 ions in the liquid phase of the precipitation, indicating the amount of iron dissolved in the water. This parameter is important for understanding the transport and deposition of iron in terrestrial ecosystems, and its availability for biological processes such as nutrient cycling and biological productivity." []
is_a: ECOSIM:CATEGORYAtmosphericConditions ! category - Atmospheric Conditions
is_a: ECOSIM:CATEGORYDepositionFlux ! category - deposition flux
relationship: attribute ECOSIMCONCEPT:Concentration ! Concentration
relationship: has_unit ECOSIM:gm-3 ! g m-3
relationship: measured_in ECOSIMCONCEPT:Precipitation ! Precipitation
relationship: measurement_of ECOSIMCONCEPT:FeOH4 ! Iron tetrahydroxide

[Term]
id: ECOSIM:CFE4U
name: subsurface irrigation FeOH4 concentration
def: "Subsurface irrigation FeOH4 concentration refers to the concentration of FeOH4 (iron hydroxide) in the soil under a subsurface irrigation system. It represents the amount of iron hydroxide present in the soil as a result of the irrigation practices, especially in areas where water with high iron content is used for irrigation. The FeOH4 concentration has implications for the soil's mineral composition, nutrient availability, and overall soil health, and is an important parameter to consider in earth systems modeling related to agricultural practices and soil-water interactions." []
is_a: ECOSIMCONCEPT:UnclassifiedVariable ! unclassified variable
relationship: attribute ECOSIMCONCEPT:Concentration ! Concentration
relationship: context ECOSIMCONCEPT:SubsurfaceIrrigation ! SubsurfaceIrrigation
relationship: has_unit ECOSIM:gm-3 ! g m-3
relationship: measurement_of ECOSIMCONCEPT:FeOH4 ! Iron tetrahydroxide

[Term]
id: ECOSIM:CFEOH
name: soil FeOH3 content
def: "Soil FeOH3 content refers to the concentration of iron (III) hydroxide (FeOH3) in the soil. It represents the amount of this mineral present in the soil system, which can affect various biogeochemical processes such as nutrient cycling, organic matter decomposition, and metal sorption. The soil FeOH3 content is an important parameter in earth systems modeling as it influences the availability and mobility of elements and nutrients in the soil, ultimately affecting ecosystem functioning and productivity." []
is_a: ECOSIM:CATEGORYBiogeochemistry ! category - Biogeochemistry
is_a: ECOSIM:CATEGORYSoilBiogeochemistry ! category - Soil Biogeochemistry
is_a: ECOSIM:CATEGORYSoilProperty ! category - soil property
relationship: attribute ECOSIMCONCEPT:Content ! Content
relationship: has_unit ECOSIM:mgkg-1 ! mg kg-1
relationship: measured_in ECOSIMCONCEPT:Soil ! Soil
relationship: measurement_of ECOSIMCONCEPT:FeOH3 ! Iron trihydroxide

[Term]
id: ECOSIM:CFEPO
name: soil FePO4 content
def: "Soil FePO4 content refers to the concentration or amount of iron phosphate (FePO4) present in the soil. Iron phosphate is an important component of soil minerals, affecting the availability and cycling of phosphorus in terrestrial ecosystems. The measurement of soil FePO4 content is relevant for Earth systems modeling as it can provide insights into nutrient availability, biogeochemical cycles, and ecosystem functioning." []
is_a: ECOSIM:CATEGORYBiogeochemistry ! category - Biogeochemistry
is_a: ECOSIM:CATEGORYSoilBiogeochemistry ! category - Soil Biogeochemistry
is_a: ECOSIM:CATEGORYSoilProperty ! category - soil property
relationship: attribute ECOSIMCONCEPT:Content ! Content
relationship: has_unit ECOSIM:mgkg-1 ! mg kg-1
relationship: measured_in ECOSIMCONCEPT:Soil ! Soil
relationship: measurement_of ECOSIMCONCEPT:FePO4 ! FePO4

[Term]
id: ECOSIM:CFEQ
name: surface irrigation Fe concentration
def: "Surface irrigation Fe concentration refers to the concentration of iron (Fe) in water used for surface irrigation in an earth system modeling context. It represents the amount of dissolved or particulate iron present in the irrigation water, which can have implications for soil fertility, crop growth, and overall ecosystem health. This parameter is important to consider in earth system models as it can affect the biogeochemical cycling of iron, nutrient availability in the soil, and potentially impact downstream water bodies through runoff or leaching." []
is_a: ECOSIMCONCEPT:UnclassifiedVariable ! unclassified variable
relationship: attribute ECOSIMCONCEPT:Concentration ! Concentration
relationship: context ECOSIMCONCEPT:Irrigation ! Irrigation
relationship: has_unit ECOSIM:gm-3 ! g m-3
relationship: measured_in ECOSIMCONCEPT:Surface ! Surface
relationship: measurement_of ECOSIMCONCEPT:Fe ! Iron

[Term]
id: ECOSIM:CFER
name: precipitation Fe concentration
def: "Precipitation Fe concentration refers to the amount of iron (Fe) present in precipitation. It represents the concentration of iron in rainwater, snow, or any other form of precipitation that falls from the atmosphere to the Earth's surface. Iron is an essential micronutrient for plant growth and is also involved in various biogeochemical processes. Monitoring precipitation Fe concentration is important for understanding the input of iron into terrestrial and aquatic systems and its potential impact on ecosystem functioning." []
is_a: ECOSIM:CATEGORYAtmosphericConditions ! category - Atmospheric Conditions
is_a: ECOSIM:CATEGORYDepositionFlux ! category - deposition flux
relationship: attribute ECOSIMCONCEPT:Concentration ! Concentration
relationship: has_unit ECOSIM:gm-3 ! g m-3
relationship: measured_in ECOSIMCONCEPT:Precipitation ! Precipitation
relationship: measurement_of ECOSIMCONCEPT:Iron ! Iron

[Term]
id: ECOSIM:CFESQ
name: surface irrigation FeSO4 concentration
def: "Surface irrigation FeSO4 concentration refers to the concentration of iron sulfate (FeSO4) in the water used for surface irrigation. It is a parameter that quantifies the amount of dissolved iron sulfate present in the irrigation water, which is typically used to supply essential iron nutrients to crops during surface irrigation. The concentration of FeSO4 affects the availability and uptake of iron by plants, influencing their growth, development, and overall productivity." []
is_a: ECOSIMCONCEPT:UnclassifiedVariable ! unclassified variable
relationship: attribute ECOSIMCONCEPT:Concentration ! Concentration
relationship: context ECOSIMCONCEPT:Irrigation ! Irrigation
relationship: has_unit ECOSIM:gm-3 ! g m-3
relationship: measured_in ECOSIMCONCEPT:Surface ! Surface
relationship: measurement_of ECOSIMCONCEPT:FeSO4 ! Iron sulfate

[Term]
id: ECOSIM:CFESR
name: precipitation FeSO4 concentration
def: "Precipitation FeSO4 concentration refers to the amount of dissolved FeSO4 in precipitation, which is the process of transferring atmospheric gases, particles, and other substances to the Earth's surface in the form of rain, snow, or hail. This parameter is important in Earth systems modeling as it affects the chemical composition of soil and water bodies, and can have implications for ecosystem health and nutrient availability." []
is_a: ECOSIM:CATEGORYAtmosphericConditions ! category - Atmospheric Conditions
is_a: ECOSIM:CATEGORYDepositionFlux ! category - deposition flux
relationship: attribute ECOSIMCONCEPT:Concentration ! Concentration
relationship: context ECOSIMCONCEPT:Precipitation ! Precipitation
relationship: has_unit ECOSIM:gm-3 ! g m-3
relationship: measured_in ECOSIMCONCEPT:Water ! Water
relationship: measurement_of ECOSIMCONCEPT:FeSO4 ! Iron sulfate

[Term]
id: ECOSIM:CFESU
name: subsurface irrigation FeSO4 concentration
def: "Subsurface irrigation FeSO4 concentration refers to the concentration of ferrous sulfate (FeSO4) in water used for irrigating plants or crops through a subsurface irrigation system. It is a parameter that affects the availability and uptake of iron by plants, as well as the potential environmental impacts associated with the use of FeSO4 in agricultural practices." []
is_a: ECOSIMCONCEPT:UnclassifiedVariable ! unclassified variable
relationship: attribute ECOSIMCONCEPT:Concentration ! Concentration
relationship: context ECOSIMCONCEPT:Irrigation ! Irrigation
relationship: has_unit ECOSIM:gm-3 ! g m-3
relationship: measured_in ECOSIMCONCEPT:Subsurface ! Subsurface
relationship: measurement_of ECOSIMCONCEPT:FeSO4 ! Iron sulfate

[Term]
id: ECOSIM:CFEU
name: subsurface irrigation H concentration
def: "Subsurface irrigation H concentration refers to the measurement of the concentration of hydrogen ions (H+) in the soil during subsurface irrigation. It is a parameter used in earth systems modeling to understand the pH levels and potential acidity or alkalinity of the soil, which can affect plant growth, nutrient availability, and overall soil health. By monitoring subsurface irrigation H concentration, scientists can assess the suitability of irrigation practices and the potential impacts on water quality and soil fertility." []
is_a: ECOSIMCONCEPT:UnclassifiedVariable ! unclassified variable
relationship: attribute ECOSIMCONCEPT:Concentration ! Concentration
relationship: context ECOSIMCONCEPT:Irrigation ! Irrigation
relationship: has_unit ECOSIM:gm-3 ! g m-3
relationship: measured_in ECOSIMCONCEPT:Subsurface ! Subsurface
relationship: measurement_of ECOSIMCONCEPT:H ! Hydrogen

[Term]
id: ECOSIM:CFOPE
name: litter kinetic fraction
def: "The litter kinetic fraction is a parameter that represents the fraction of litter that undergoes decomposition or decay within a given time period in Earth system models. It is a measure of how quickly organic matter in the litter pool is transformed into soil organic carbon through microbial activity. This parameter is essential for accurately modeling carbon dynamics and cycling in terrestrial ecosystems, as it influences the rates of carbon turnover and the balance between carbon inputs and outputs in the soil system." []
is_a: ECOSIMCONCEPT:UnclassifiedVariable ! unclassified variable
is_a: ECOSIMCONCEPT:Variable ! variable
relationship: measurement_of ECOSIMCONCEPT:Litter ! Litter

[Term]
id: ECOSIM:CH0PQ
name: surface irrigation PO4 concentration
def: "The term 'surface irrigation PO4 concentration' refers to the concentration of phosphate (PO4) in water used for surface irrigation. Surface irrigation is a method of watering crops in which water is applied directly to the soil surface. The PO4 concentration measure allows for the assessment and monitoring of the level of phosphate in the irrigation water, which can have important implications for crop growth, nutrient cycling, and potential water pollution." []
is_a: ECOSIMCONCEPT:UnclassifiedVariable ! unclassified variable
relationship: attribute ECOSIMCONCEPT:Concentration ! Concentration
relationship: has_unit ECOSIM:gm-3 ! g m-3
relationship: measured_in ECOSIMCONCEPT:SurfaceIrrigation ! SurfaceIrrigation
relationship: measurement_of ECOSIMCONCEPT:PO4 ! Phosphate

[Term]
id: ECOSIM:CH0PR
name: precipitation PO4 concentration
def: "Precipitation PO4 concentration refers to the concentration of phosphate (PO4) in precipitation. Phosphate is an essential nutrient for plants and plays a crucial role in various biogeochemical processes, including the growth and productivity of aquatic ecosystems. The concentration of PO4 in precipitation influences the availability of this nutrient for plants and can have significant impacts on ecosystem dynamics and nutrient cycling. Earth system models use this parameter to simulate and study the effects of changing precipitation patterns on phosphate availability and its implications for ecosystem functioning and biogeochemical cycles." []
is_a: ECOSIM:CATEGORYAtmosphericConditions ! category - Atmospheric Conditions
is_a: ECOSIM:CATEGORYDepositionFlux ! category - deposition flux
relationship: attribute ECOSIMCONCEPT:Concentration ! Concentration
relationship: context ECOSIMCONCEPT:Precipitation ! Precipitation
relationship: has_unit ECOSIM:gm-3 ! g m-3
relationship: measured_in ECOSIMCONCEPT:Water ! Water
relationship: measurement_of ECOSIMCONCEPT:PO4 ! Phosphate

[Term]
id: ECOSIM:CH0PU
name: subsurface irrigation PO4 concentration
def: "Subsurface irrigation PO4 concentration refers to the measurement or estimation of the concentration of phosphate (PO4) in the soil water or solution below the ground surface due to the process of subsurface irrigation. This parameter is important in earth systems modeling as it helps assess the availability of phosphorus to plants and understand its dynamics and transport within the subsurface environment. It can be influenced by factors such as fertilizer application, weathering, drainage, and irrigation practices." []
is_a: ECOSIMCONCEPT:UnclassifiedVariable ! unclassified variable
relationship: attribute ECOSIMCONCEPT:Concentration ! Concentration
relationship: context ECOSIMCONCEPT:Irrigation ! Irrigation
relationship: has_unit ECOSIM:gm-3 ! g m-3
relationship: measured_in ECOSIMCONCEPT:Subsurface ! Subsurface
relationship: measurement_of ECOSIMCONCEPT:PO4 ! Phosphate

[Term]
id: ECOSIM:CH1PQ
name: surface irrigation HPO4 concentration
def: "Surface irrigation HPO4 concentration refers to the level of phosphate ions (HPO4) present in water used for surface irrigation. It represents the amount of dissolved phosphate compounds in irrigation water that can potentially affect the nutrient supply to plants and influence their growth and development. Monitoring surface irrigation HPO4 concentration is important in earth systems modeling to understand the dynamics of nutrient cycling, water quality, and the impact of agricultural practices on ecosystem health." []
is_a: ECOSIMCONCEPT:UnclassifiedVariable ! unclassified variable
relationship: attribute ECOSIMCONCEPT:Concentration ! Concentration
relationship: context ECOSIMCONCEPT:Irrigation ! Irrigation
relationship: has_unit ECOSIM:gm-3 ! g m-3
relationship: measured_in ECOSIMCONCEPT:Surface ! Surface
relationship: measurement_of ECOSIMCONCEPT:HPO4 ! Hydrogen phosphate

[Term]
id: ECOSIM:CH1PR
name: precipitation HPO4 concentration
def: "Precipitation HPO4 concentration refers to the concentration of the HPO4 (hydrogen phosphate) ion in rainfall or other forms of atmospheric precipitation. It is a parameter that quantifies the amount of HPO4 present in a given volume or mass of precipitation, typically measured in units of concentration (e.g., milligrams per liter or parts per million). This parameter is relevant in Earth system modeling as it influences the nutrient availability in ecosystems and can impact the cycling of phosphorus, an essential nutrient for plant growth and productivity." []
is_a: ECOSIM:CATEGORYAtmosphericConditions ! category - Atmospheric Conditions
is_a: ECOSIM:CATEGORYDepositionFlux ! category - deposition flux
relationship: attribute ECOSIMCONCEPT:Concentration ! Concentration
relationship: context ECOSIMCONCEPT:Precipitation ! Precipitation
relationship: has_unit ECOSIM:gm-3 ! g m-3
relationship: measured_in ECOSIMCONCEPT:Water ! Water
relationship: measurement_of ECOSIMCONCEPT:HPO4 ! Hydrogen phosphate

[Term]
id: ECOSIM:CH3PQ
name: surface irrigation H3PO4 concentration
def: "The term 'surface irrigation H3PO4 concentration' refers to the concentration of phosphoric acid (H3PO4) in the water used for surface irrigation. Surface irrigation is a method of water delivery where water is distributed over the soil surface through channels or furrows. Monitoring the H3PO4 concentration in surface irrigation water is important for understanding the potential impacts of phosphorus on the soil and plants. Phosphorus is a vital nutrient for plant growth, but excessive levels can lead to water pollution and adversely affect aquatic ecosystems." []
is_a: ECOSIMCONCEPT:UnclassifiedVariable ! unclassified variable
relationship: attribute ECOSIMCONCEPT:Concentration ! Concentration
relationship: context ECOSIMCONCEPT:Irrigation ! Irrigation
relationship: has_unit ECOSIM:gm-3 ! g m-3
relationship: measured_in ECOSIMCONCEPT:Surface ! Surface
relationship: measurement_of ECOSIMCONCEPT:H3PO4 ! Phosphoric acid

[Term]
id: ECOSIM:CH3PR
name: precipitation H3PO4 concentration
def: "Precipitation H3PO4 concentration refers to the amount of phosphoric acid (H3PO4) present in atmospheric precipitation. It quantifies the concentration of phosphoric acid in the form of rain, snow, or other forms of precipitation that fall onto the Earth's surface. This parameter is relevant for Earth systems modeling as it provides insights into the input of phosphorus into ecosystems through rainfall, which plays a crucial role in nutrient cycling and can influence the growth and productivity of plants and aquatic organisms." []
is_a: ECOSIM:CATEGORYAtmosphericConditions ! category - Atmospheric Conditions
is_a: ECOSIM:CATEGORYDepositionFlux ! category - deposition flux
relationship: attribute ECOSIMCONCEPT:Concentration ! Concentration
relationship: has_unit ECOSIM:gm-3 ! g m-3
relationship: measured_in ECOSIMCONCEPT:Precipitation ! Precipitation
relationship: measurement_of ECOSIMCONCEPT:H3PO4 ! Phosphoric acid

[Term]
id: ECOSIM:CH3PU
name: subsurface irrigation H3PO4 concentration
def: "Subsurface irrigation H3PO4 concentration is a parameter that represents the concentration of phosphoric acid (H3PO4) in the water used for subsurface irrigation. It quantifies the amount of phosphoric acid present in the irrigation water that is applied underground to supply moisture and nutrients to plant roots. This parameter is important in earth systems modeling as it can impact the soil fertility, nutrient uptake by plants, and overall plant growth and productivity." []
is_a: ECOSIMCONCEPT:UnclassifiedVariable ! unclassified variable
relationship: attribute ECOSIMCONCEPT:Concentration ! Concentration
relationship: context ECOSIMCONCEPT:Irrigation ! Irrigation
relationship: has_unit ECOSIM:gm-3 ! g m-3
relationship: measured_in ECOSIMCONCEPT:Subsurface ! Subsurface
relationship: measurement_of ECOSIMCONCEPT:H3PO4 ! Phosphoric acid

[Term]
id: ECOSIM:CH4E
name: atmospheric CH4 concentration
def: "Atmospheric CH4 concentration refers to the abundance of methane (CH4) gas in the Earth's atmosphere. It is expressed as the volume of CH4 per unit volume of air (parts per million, ppm) or as a mixing ratio. Methane is an important greenhouse gas and contributes to climate change. Monitoring and understanding changes in atmospheric CH4 concentration is crucial for climate models and Earth system simulations." []
is_a: ECOSIMCONCEPT:UnclassifiedVariable ! unclassified variable
relationship: attribute ECOSIMCONCEPT:Concentration ! Concentration
relationship: has_unit ECOSIM:umolmol-1 ! umol mol-1
relationship: measured_in ECOSIMCONCEPT:Atmosphere ! Atmosphere
relationship: measurement_of ECOSIMCONCEPT:CH4 ! Methane

[Term]
id: ECOSIM:CHCQ
name: surface irrigation HCO3 concentration
def: "Surface irrigation HCO3 concentration refers to the measurement of bicarbonate (HCO3-) concentration in the water used for surface irrigation. It represents the amount of bicarbonate ions dissolved in the irrigation water, which can have an impact on soil chemistry and crop health. The HCO3- concentration is an important parameter to consider in earth system modeling as it can affect nutrient availability, irrigation efficiency, and overall water quality in agricultural systems." []
is_a: ECOSIMCONCEPT:UnclassifiedVariable ! unclassified variable
relationship: attribute ECOSIMCONCEPT:Concentration ! Concentration
relationship: context ECOSIMCONCEPT:Irrigation ! Irrigation
relationship: has_unit ECOSIM:gm-3 ! g m-3
relationship: measured_in ECOSIMCONCEPT:Surface ! Surface
relationship: measurement_of ECOSIMCONCEPT:HCO3 ! Bicarbonate

[Term]
id: ECOSIM:CHCR
name: precipitation HCO3 concentration
def: "Precipitation HCO3 concentration refers to the amount of bicarbonate ions (HCO3-) present in precipitation. Bicarbonate ions are an important component of the carbonate system, which plays a significant role in regulating ocean chemistry and buffering pH levels. Precipitation HCO3 concentration is an important parameter to consider in earth systems modeling as it can have implications for the carbon cycle, ocean acidification, and the overall balance of marine ecosystems." []
is_a: ECOSIM:CATEGORYAtmosphericConditions ! category - Atmospheric Conditions
is_a: ECOSIM:CATEGORYDepositionFlux ! category - deposition flux
relationship: attribute ECOSIMCONCEPT:Concentration ! Concentration
relationship: context ECOSIMCONCEPT:Precipitation ! Precipitation
relationship: has_unit ECOSIM:gm-3 ! g m-3
relationship: measured_in ECOSIMCONCEPT:Water ! Water
relationship: measurement_of ECOSIMCONCEPT:HCO3 ! Bicarbonate

[Term]
id: ECOSIM:CHCU
name: subsurface irrigation CH4 concentration
def: "Subsurface irrigation CH4 concentration refers to the measurement or estimation of the concentration of methane (CH4) within the subsurface soil or water layers during an irrigation process. This parameter is typically used in earth systems modeling to analyze and understand the impact of subsurface irrigation on the emission of methane, a potent greenhouse gas, and its subsequent effects on the environment and climate systems." []
is_a: ECOSIMCONCEPT:UnclassifiedVariable ! unclassified variable
relationship: attribute ECOSIMCONCEPT:Concentration ! Concentration
relationship: context ECOSIMCONCEPT:Irrigation ! Irrigation
relationship: has_unit ECOSIM:gm-3 ! g m-3
relationship: measured_in ECOSIMCONCEPT:Subsurface ! Subsurface
relationship: measurement_of ECOSIMCONCEPT:CH4 ! Methane

[Term]
id: ECOSIM:CHILL
name: chilling effect on CO2 fixation
def: "Chilling effect on CO2 fixation refers to the reduction in the rate of carbon dioxide uptake and conversion into organic compounds through photosynthesis due to low temperatures. It is a parameter that quantifies the impact of low temperatures on the ability of plants and ecosystems to fix carbon dioxide from the atmosphere. Higher values indicate a greater reduction in CO2 fixation under cold conditions, while lower values suggest less sensitivity to temperature changes. This parameter is particularly relevant in Earth system models as it helps capture the response of terrestrial ecosystems to climate change and better predict carbon cycle dynamics under different climate scenarios." []
is_a: ECOSIM:CATEGORYCanopyPhysiology ! category - Canopy Physiology
is_a: ECOSIM:CATEGORYPlantPhysiology ! category - plant physiology
relationship: measured_in ECOSIMCONCEPT:Leaf ! Leaf
relationship: measurement_of ECOSIMCONCEPT:CO2 ! Carbon dioxide

[Term]
id: ECOSIM:CHL
name: leaf C3 chlorophyll content
def: "Leaf C3 chlorophyll content refers to the concentration or amount of chlorophyll present in the leaves of C3 plants. Chlorophyll is the primary pigment responsible for capturing light energy during photosynthesis. This parameter is important in Earth system modeling as it influences the rate of photosynthesis and hence the productivity and carbon uptake of C3 plants. It can be used to estimate plant health, growth, and overall ecosystem functioning. Leaf C3 chlorophyll content is typically measured in units of mass (e.g., milligrams or grams) per unit leaf area (e.g., square meter)." []
is_a: ECOSIM:CATEGORYCanopyPhysiology ! category - Canopy Physiology
is_a: ECOSIM:CATEGORYPlantPhysiology ! category - plant physiology
relationship: attribute ECOSIMCONCEPT:Content ! Content
relationship: has_unit ECOSIM:gg-1 ! g g-1
relationship: measured_in ECOSIMCONCEPT:Leaf ! Leaf
relationship: measurement_of ECOSIMCONCEPT:Chlorophyll ! Chlorophyll

[Term]
id: ECOSIM:CHL4
name: leaf C4 chlorophyll content
def: "The term 'leaf C4 chlorophyll content' refers to the amount of chlorophyll present in the leaves of plants that utilize the C4 photosynthetic pathway. The C4 pathway is a biochemical process that some plants have evolved to optimize carbon fixation in environments with high temperature and low CO2 levels. The chlorophyll content in C4 leaves contributes to their ability to capture and convert sunlight into chemical energy through photosynthesis. Measurement of leaf C4 chlorophyll content is important in earth systems modeling as it helps in estimating plant productivity and the overall carbon cycle in C4 dominated ecosystems." []
is_a: ECOSIM:CATEGORYCanopyPhysiology ! category - Canopy Physiology
is_a: ECOSIM:CATEGORYPlantPhysiology ! category - plant physiology
relationship: attribute ECOSIMCONCEPT:Content ! Content
relationship: has_unit ECOSIM:gg-1 ! g g-1
relationship: measured_in ECOSIMCONCEPT:Leaf ! Leaf
relationship: measurement_of ECOSIMCONCEPT:Chlorophyll ! Chlorophyll

[Term]
id: ECOSIM:CHYQ
name: surface irrigation H concentration
def: "Surface irrigation H concentration refers to the level of hydrogen ions (H+) in the water used for surface irrigation in an earth system model. It represents the acid-base balance of the water, and is typically measured using the pH scale. The H concentration can affect the availability of nutrients in the soil, the soil's ability to retain water, and the overall productivity of the irrigation system. Monitoring and understanding the H concentration in surface irrigation can help in assessing and managing the potential impacts of water acidity on agricultural practices and ecosystems." []
is_a: ECOSIMCONCEPT:UnclassifiedVariable ! unclassified variable
relationship: attribute ECOSIMCONCEPT:Concentration ! Concentration
relationship: context ECOSIMCONCEPT:Irrigation ! Irrigation
relationship: has_unit ECOSIM:gm-3 ! g m-3
relationship: measured_in ECOSIMCONCEPT:Surface ! Surface
relationship: measurement_of ECOSIMCONCEPT:H ! Hydrogen

[Term]
id: ECOSIM:CHYR
name: precipitation H concentration
def: "Precipitation H concentration refers to the amount of hydrogen (H) present in precipitation, which is the collective term for any form of water that falls from the atmosphere to the Earth's surface. It indicates the concentration or abundance of hydrogen ions in the rainwater or other forms of precipitation. The precipitation H concentration plays a crucial role in various earth system processes, including the pH of surface waters, the availability of nutrients for aquatic organisms, and the chemical weathering of rocks and minerals." []
is_a: ECOSIM:CATEGORYAtmosphericConditions ! category - Atmospheric Conditions
is_a: ECOSIM:CATEGORYDepositionFlux ! category - deposition flux
relationship: attribute ECOSIMCONCEPT:Concentration ! Concentration
relationship: context ECOSIMCONCEPT:Precipitation ! Precipitation
relationship: has_unit ECOSIM:gm-3 ! g m-3
relationship: measured_in ECOSIMCONCEPT:Water ! Water
relationship: measurement_of ECOSIMCONCEPT:Hydrogen ! Hydrogen

[Term]
id: ECOSIM:CHYU
name: subsurface irrigation Ca concentration
def: "Subsurface irrigation Ca concentration refers to the measurement of the concentration of calcium (Ca) in the subsurface water used for irrigating agricultural fields. It represents the amount of calcium ions dissolved in the water, which can have significant effects on soil fertility and plant health. Monitoring this parameter is important for understanding the potential impacts of calcium on soil structure, nutrient availability, and crop yield in subsurface irrigation systems." []
is_a: ECOSIMCONCEPT:UnclassifiedVariable ! unclassified variable
relationship: attribute ECOSIMCONCEPT:Concentration ! Concentration
relationship: context ECOSIMCONCEPT:Irrigation ! Irrigation
relationship: has_unit ECOSIM:gm-3 ! g m-3
relationship: measured_in ECOSIMCONCEPT:Subsurface ! Subsurface
relationship: measurement_of ECOSIMCONCEPT:Ca ! Calcium

[Term]
id: ECOSIM:CION
name: solution ion concentratiom
def: "Solution ion concentration refers to the measurement of the amount of ions present in a solution. This parameter is an important aspect of earth systems modeling as it helps in understanding the chemical composition and behavior of various solutions, such as oceans, lakes, and rivers. Solution ion concentration is typically expressed in units of moles per liter (M), and it provides valuable information about the presence and abundance of different ions, which plays a significant role in determining the physical and chemical properties of the solution." []
is_a: ECOSIM:CATEGORYSoilSolution ! category - soil solution
relationship: attribute ECOSIMCONCEPT:Concentration ! Concentration
relationship: has_unit ECOSIM:molm-3 ! mol m-3
relationship: measured_in ECOSIMCONCEPT:Solution ! Solution
relationship: measurement_of ECOSIMCONCEPT:Ions ! Ions

[Term]
id: ECOSIM:CIRRA
name: fraction of FC - WP to which automatic irrigation applied
def: "The fraction of FC (Field Capacity) - WP (Wilting Point) to which automatic irrigation is applied refers to the proportion of water in the soil between field capacity and wilting point that is replenished through automated irrigation systems. Field capacity represents the maximum amount of water that the soil can hold, while the wilting point indicates the point at which plants can no longer extract water from the soil. This parameter is important for Earth systems modeling as it helps to simulate the effects of irrigation on water availability and plant growth in different regions." []
is_a: ECOSIMCONCEPT:Irrigation ! Irrigation
is_a: ECOSIMCONCEPT:UnclassifiedVariable ! unclassified variable
relationship: attribute ECOSIMCONCEPT:Fraction ! Fraction
relationship: measurement_of ECOSIMCONCEPT:FieldCapacityWiltingPoint ! FieldCapacityWiltingPoint

[Term]
id: ECOSIM:CKA
name: soil K content
def: "Soil K content refers to the concentration or amount of potassium (K) present in the soil. It is a parameter in earth systems modeling that represents the availability of potassium to plants and the overall fertility of the soil. The soil K content is influenced by factors such as weathering of parent materials, deposition of potassium from atmospheric sources, and agricultural practices such as fertilizer application." []
is_a: ECOSIM:CATEGORYBiogeochemistry ! category - Biogeochemistry
is_a: ECOSIM:CATEGORYSoilProperty ! category - soil property
relationship: attribute ECOSIMCONCEPT:Content ! Content
relationship: has_unit ECOSIM:mgkg-1 ! mg kg-1
relationship: measured_in ECOSIMCONCEPT:Soil ! Soil
relationship: measurement_of ECOSIMCONCEPT:Potassium ! Potassium

[Term]
id: ECOSIM:CKAQ
name: surface irrigation K concentration
def: "Surface irrigation K concentration refers to the concentration of potassium (K) in water used for surface irrigation of agricultural fields. It is a parameter that affects the availability of potassium in the soil, which in turn influences plant growth and nutrient uptake. The surface irrigation K concentration is typically measured in units of mass per volume (e.g., milligrams per liter) and can vary depending on factors such as soil type, crop requirements, and water quality. Proper management of surface irrigation K concentration is important for maintaining optimal nutrient levels in the soil and maximizing crop productivity." []
is_a: ECOSIMCONCEPT:UnclassifiedVariable ! unclassified variable
relationship: attribute ECOSIMCONCEPT:Concentration ! Concentration
relationship: has_unit ECOSIM:gm-3 ! g m-3
relationship: measured_in ECOSIMCONCEPT:SurfaceIrrigation ! SurfaceIrrigation
relationship: measurement_of ECOSIMCONCEPT:Potassium ! Potassium

[Term]
id: ECOSIM:CKAR
name: precipitation K concentration
def: "The term 'precipitation K concentration' refers to the concentration of potassium (K) in precipitation, which is the amount of K dissolved in liquid or solid form (such as rain or snow) that falls from the atmosphere to the Earth's surface. It is an important parameter in Earth system modeling as it influences nutrient availability for plants and overall ecosystem productivity. Precipitation K concentration can be influenced by factors such as atmospheric conditions and the sources of K emissions." []
is_a: ECOSIM:CATEGORYAtmosphericConditions ! category - Atmospheric Conditions
is_a: ECOSIM:CATEGORYDepositionFlux ! category - deposition flux
relationship: attribute ECOSIMCONCEPT:Concentration ! Concentration
relationship: has_unit ECOSIM:gm-3 ! g m-3
relationship: measured_in ECOSIMCONCEPT:Precipitation ! Precipitation
relationship: measurement_of ECOSIMCONCEPT:Potassium ! Potassium

[Term]
id: ECOSIM:CKASQ
name: surface irrigation K concentration
def: "Surface irrigation K concentration refers to the amount of potassium (K) present in the water used for surface irrigation. It represents the concentration of potassium ions in the irrigation water that is applied to the soil surface for crop irrigation purposes. This parameter is relevant in earth systems modeling as it influences the availability of potassium for plants during irrigation and can impact plant growth, nutrient uptake, and overall agricultural productivity." []
is_a: ECOSIMCONCEPT:UnclassifiedVariable ! unclassified variable
relationship: attribute ECOSIMCONCEPT:Concentration ! Concentration
relationship: context ECOSIMCONCEPT:Irrigation ! Irrigation
relationship: has_unit ECOSIM:gm-3 ! g m-3
relationship: measured_in ECOSIMCONCEPT:Surface ! Surface
relationship: measurement_of ECOSIMCONCEPT:Potassium ! Potassium

[Term]
id: ECOSIM:CKASR
name: precipitation K concentration
def: "Precipitation K concentration refers to the amount of potassium (K) present in rainfall or snowfall. It is a parameter used in Earth system models to represent the concentration of potassium in precipitation, which can affect various biogeochemical processes, such as nutrient cycling, plant growth, and soil fertility. The precipitation K concentration is typically measured in mass per unit volume (e.g., milligrams per liter) and is an important input for modeling studies that aim to understand and simulate the impacts of potassium on ecosystems and the environment." []
is_a: ECOSIM:CATEGORYDepositionFlux ! category - deposition flux
is_a: ECOSIMCONCEPT:UnclassifiedVariable ! unclassified variable
relationship: attribute ECOSIMCONCEPT:Concentration ! Concentration
relationship: has_unit ECOSIM:gm-3 ! g m-3
relationship: measured_in ECOSIMCONCEPT:Precipitation ! Precipitation
relationship: measurement_of ECOSIMCONCEPT:Potassium ! Potassium

[Term]
id: ECOSIM:CKASU
name: subsurface irrigation K concentration
def: "Subsurface irrigation K concentration refers to the measurement of potassium (K) concentration levels in water used for subsurface irrigation. It is a parameter used in earth systems modeling to assess the availability and distribution of potassium in the subsurface irrigation system, which can affect plant growth, nutrient uptake, and soil fertility. This parameter helps to simulate and predict the impact of varying K concentrations on crop productivity, water management, and overall soil health in subsurface irrigation systems." []
is_a: ECOSIMCONCEPT:UnclassifiedVariable ! unclassified variable
relationship: attribute ECOSIMCONCEPT:Concentration ! Concentration
relationship: context ECOSIMCONCEPT:Irrigation ! Irrigation
relationship: has_unit ECOSIM:gm-3 ! g m-3
relationship: measured_in ECOSIMCONCEPT:Subsurface ! Subsurface
relationship: measurement_of ECOSIMCONCEPT:Potassium ! Potassium

[Term]
id: ECOSIM:CKAU
name: subsurface irrigation OH concentration
def: "Subsurface irrigation OH concentration refers to the parameter that quantifies the concentration of hydroxyl radicals (OH) in the subsurface soil environment during irrigation processes. Hydroxyl radicals are highly reactive and play a critical role in various biogeochemical processes, such as organic matter decomposition and nutrient cycling. This parameter helps to assess the potential for chemical reactions and transformations occurring in the subsurface soil due to OH radicals, which can have implications for soil fertility, nutrient availability, and pollutant degradation." []
is_a: ECOSIMCONCEPT:UnclassifiedVariable ! unclassified variable
relationship: attribute ECOSIMCONCEPT:Concentration ! Concentration
relationship: context ECOSIMCONCEPT:Irrigation ! Irrigation
relationship: has_unit ECOSIM:gm-3 ! g m-3
relationship: measured_in ECOSIMCONCEPT:Subsurface ! Subsurface
relationship: measurement_of ECOSIMCONCEPT:OH ! OH

[Term]
id: ECOSIM:CLASS
name: fractionction of leaves in different angle classes
def: "Fraction of leaves in different angle classes refers to the distribution of leaf orientations within a vegetation canopy. It represents the proportion of leaves that fall into different categories based on their angle relative to the vertical axis. This parameter is important for modeling the interception and absorption of solar radiation by vegetation, as it affects the overall canopy structure and the amount of sunlight reaching the underlying surfaces." []
is_a: ECOSIMCONCEPT:UnclassifiedVariable ! unclassified variable
relationship: attribute ECOSIMCONCEPT:Fraction ! Fraction
relationship: measured_in ECOSIMCONCEPT:Canopy ! Canopy
relationship: measurement_of ECOSIMCONCEPT:Leaf ! Leaf

[Term]
id: ECOSIM:CLSXL
name: aqueous Cl diffusivity
def: "Aqueous Cl diffusivity refers to the measure of the ability of chloride ions (Cl-) to diffuse or spread out within a liquid medium, specifically water. It quantifies how easily chloride ions can move through the water, which is important for understanding the transport and distribution of chloride in aquatic systems. Aqueous Cl diffusivity is a parameter used in Earth systems models to simulate and predict the behavior of chloride ions in water bodies and their interactions with other components of the environment." []
is_a: ECOSIM:CATEGORYHydrology ! category - Hydrology
is_a: ECOSIMCONCEPT:UnclassifiedVariable ! unclassified variable
relationship: attribute ECOSIMCONCEPT:Diffusivity ! Diffusivity
relationship: has_unit ECOSIM:m2h-1 ! m2 h-1
relationship: measured_in ECOSIMCONCEPT:Water ! Water
relationship: measurement_of ECOSIMCONCEPT:Chloride ! Chloride
relationship: qualifier ECOSIMCONCEPT:Aqueous ! Aqueous

[Term]
id: ECOSIM:CM1PQ
name: surface irrigation MgHPO4 concentration
def: "The term 'surface irrigation MgHPO4 concentration' refers to the concentration of magnesium dihydrogen phosphate (MgHPO4) in water used for surface irrigation. Surface irrigation is a method of delivering water to crops by allowing it to flow over the soil surface. The MgHPO4 concentration is an important parameter to measure as it can impact plant growth and the overall nutrient balance in agricultural systems." []
is_a: ECOSIMCONCEPT:UnclassifiedVariable ! unclassified variable
relationship: attribute ECOSIMCONCEPT:Concentration ! Concentration
relationship: context ECOSIMCONCEPT:Irrigation ! Irrigation
relationship: has_unit ECOSIM:gm-3 ! g m-3
relationship: measured_in ECOSIMCONCEPT:Surface ! Surface
relationship: measurement_of ECOSIMCONCEPT:MgHPO4 ! Magnesium hydrogen phosphate

[Term]
id: ECOSIM:CM1PR
name: precipitation MgHPO4 concentration
def: "Precipitation MgHPO4 concentration refers to the amount of magnesium hydrophosphate (MgHPO4) present in a unit volume of precipitation. It is a parameter used in earth systems modeling to quantify the concentration of this specific compound in precipitation events, which can have implications for nutrient availability and ecosystem productivity." []
is_a: ECOSIM:CATEGORYAtmosphericConditions ! category - Atmospheric Conditions
is_a: ECOSIM:CATEGORYDepositionFlux ! category - deposition flux
relationship: attribute ECOSIMCONCEPT:Concentration ! Concentration
relationship: context ECOSIMCONCEPT:Precipitation ! Precipitation
relationship: has_unit ECOSIM:gm-3 ! g m-3
relationship: measured_in ECOSIMCONCEPT:Air ! Air
relationship: measurement_of ECOSIMCONCEPT:MgHPO4 ! Magnesium hydrogen phosphate

[Term]
id: ECOSIM:CM1PU
name: subsurface irrigation MgHPO4 concentration
def: "Subsurface irrigation MgHPO4 concentration refers to the level of magnesium hydrogen phosphate (MgHPO4) present in the soil as a result of subsurface irrigation practices. It is a parameter that quantifies the amount of MgHPO4 in the soil and is relevant for earth systems models that simulate the dynamics of subsurface irrigation and its impact on soil chemistry." []
is_a: ECOSIMCONCEPT:UnclassifiedVariable ! unclassified variable
relationship: attribute ECOSIMCONCEPT:Concentration ! Concentration
relationship: context ECOSIMCONCEPT:Irrigation ! Irrigation
relationship: has_unit ECOSIM:gm-3 ! g m-3
relationship: measured_in ECOSIMCONCEPT:Subsurface ! Subsurface
relationship: measurement_of ECOSIMCONCEPT:MgHPO4 ! Magnesium hydrogen phosphate

[Term]
id: ECOSIM:CMG
name: soil Mg content
def: "Soil Mg content refers to the concentration or amount of magnesium (Mg) present in the soil. It is a parameter that is used in Earth systems modeling to represent the level of magnesium in the soil, which plays a crucial role in various soil processes and functions. Soil Mg content is important for understanding nutrient availability, soil fertility, and the overall health and productivity of ecosystems. It can be quantified through laboratory analyses or estimated using remote sensing data or existing soil databases." []
is_a: ECOSIM:CATEGORYBiogeochemistry ! category - Biogeochemistry
is_a: ECOSIM:CATEGORYSoilBiogeochemistry ! category - Soil Biogeochemistry
is_a: ECOSIM:CATEGORYSoilProperty ! category - soil property
relationship: attribute ECOSIMCONCEPT:Content ! Content
relationship: has_unit ECOSIM:mgkg-1 ! mg kg-1
relationship: measured_in ECOSIMCONCEPT:Soil ! Soil
relationship: measurement_of ECOSIMCONCEPT:Magnesium ! Magnesium

[Term]
id: ECOSIM:CMGCQ
name: surface irrigation MgCO3 concentration
def: "The surface irrigation MgCO3 concentration refers to the concentration of magnesium carbonate (MgCO3) in the water used for surface irrigation. It represents the amount of magnesium carbonate dissolved in the irrigation water, typically measured in milligrams per liter (mg/L) or parts per million (ppm). This parameter is important for understanding the potential impacts of irrigation on soil chemistry and the overall nutrient balance in agricultural systems. High levels of magnesium carbonate in irrigation water can affect soil pH and fertility, potentially influencing plant growth and crop yields. Monitoring and managing surface irrigation MgCO3 concentration is therefore crucial for sustainable agricultural practices and effective water resource management." []
is_a: ECOSIMCONCEPT:UnclassifiedVariable ! unclassified variable
relationship: attribute ECOSIMCONCEPT:Concentration ! Concentration
relationship: context ECOSIMCONCEPT:Irrigation ! Irrigation
relationship: has_unit ECOSIM:gm-3 ! g m-3
relationship: measured_in ECOSIMCONCEPT:Surface ! Surface
relationship: measurement_of ECOSIMCONCEPT:MgCO3 ! Magnesium carbonate

[Term]
id: ECOSIM:CMGCR
name: precipitation MgCO3 concentration
def: "Precipitation MgCO3 concentration refers to the level of magnesium carbonate (MgCO3) in the atmospheric precipitation or rainfall. It is a measure of the amount of MgCO3 present in a given volume of precipitation, usually expressed in milligrams per liter (mg/L) or parts per million (ppm). This parameter is important in earth systems modeling as MgCO3 can have various effects on the environment, including determining the pH level of water bodies and influencing the chemistry of soil and aquatic ecosystems." []
is_a: ECOSIM:CATEGORYAtmosphericConditions ! category - Atmospheric Conditions
is_a: ECOSIM:CATEGORYDepositionFlux ! category - deposition flux
relationship: attribute ECOSIMCONCEPT:Concentration ! Concentration
relationship: has_unit ECOSIM:gm-3 ! g m-3
relationship: measured_in ECOSIMCONCEPT:AtmosphericPrecipitation ! AtmosphericPrecipitation
relationship: measurement_of ECOSIMCONCEPT:MgCO3 ! Magnesium carbonate

[Term]
id: ECOSIM:CMGCU
name: subsurface irrigation MgCO3 concentration
def: "Subsurface irrigation MgCO3 concentration refers to the concentration of magnesium carbonate (MgCO3) in water used for irrigating agricultural fields through a subsurface irrigation system. It represents the amount of MgCO3 dissolved in the water and is typically expressed in units of mass per volume (e.g., milligrams per liter). The MgCO3 concentration can have an impact on soil chemistry, nutrient availability, and plant growth, and is an important parameter to consider in earth systems models for simulating the hydrological and biogeochemical processes associated with subsurface irrigation." []
is_a: ECOSIMCONCEPT:UnclassifiedVariable ! unclassified variable
relationship: attribute ECOSIMCONCEPT:Concentration ! Concentration
relationship: context ECOSIMCONCEPT:Irrigation ! Irrigation
relationship: has_unit ECOSIM:gm-3 ! g m-3
relationship: measured_in ECOSIMCONCEPT:Subsurface ! Subsurface
relationship: measurement_of ECOSIMCONCEPT:MgCO3 ! Magnesium carbonate

[Term]
id: ECOSIM:CMGHQ
name: surface irrigation MgHCO3 concentration
def: "Surface irrigation MgHCO3 concentration refers to the concentration of magnesium bicarbonate (MgHCO3) in the water used for surface irrigation. It represents the amount of magnesium and bicarbonate ions dissolved in water, which can have a significant impact on the chemistry and nutrient availability in the soil. The surface irrigation MgHCO3 concentration parameter is important in earth systems modeling as it influences soil fertility, crop productivity, and can contribute to the overall water quality in agricultural systems." []
is_a: ECOSIMCONCEPT:UnclassifiedVariable ! unclassified variable
relationship: attribute ECOSIMCONCEPT:Concentration ! Concentration
relationship: context ECOSIMCONCEPT:Irrigation ! Irrigation
relationship: has_unit ECOSIM:gm-3 ! g m-3
relationship: measured_in ECOSIMCONCEPT:Surface ! Surface
relationship: measurement_of ECOSIMCONCEPT:MgHCO3 ! Magnesium bicarbonate

[Term]
id: ECOSIM:CMGHR
name: precipitation MgHCO3 concentration
def: "Precipitation MgHCO3 concentration refers to the amount of magnesium bicarbonate (MgHCO3) present in precipitation (rainfall and snowfall). It represents the concentration of dissolved MgHCO3 ions in the water that falls from the atmosphere to the Earth's surface as part of the hydrological cycle. This parameter is important in earth system modeling as it affects the chemistry of surface waters and influences various ecological processes in aquatic ecosystems." []
is_a: ECOSIM:CATEGORYDepositionFlux ! category - deposition flux
is_a: ECOSIMCONCEPT:UnclassifiedVariable ! unclassified variable
relationship: attribute ECOSIMCONCEPT:Concentration ! Concentration
relationship: has_unit ECOSIM:gm-3 ! g m-3
relationship: measured_in ECOSIMCONCEPT:Precipitation ! Precipitation
relationship: measurement_of ECOSIMCONCEPT:MgHCO3 ! Magnesium bicarbonate

[Term]
id: ECOSIM:CMGHU
name: subsurface irrigation MgHCO3 concentration
def: "Subsurface irrigation refers to a method of supplying water to plants by delivering it directly to the root zone below the soil surface. The MgHCO3 (magnesium bicarbonate) concentration is a parameter that represents the amount of dissolved magnesium bicarbonate in the irrigation water used in the subsurface irrigation system. This parameter is important to monitor as it can have implications for plant nutrition and soil chemistry." []
is_a: ECOSIMCONCEPT:UnclassifiedVariable ! unclassified variable
relationship: attribute ECOSIMCONCEPT:Concentration ! Concentration
relationship: context ECOSIMCONCEPT:Irrigation ! Irrigation
relationship: has_unit ECOSIM:gm-3 ! g m-3
relationship: measured_in ECOSIMCONCEPT:Subsurface ! Subsurface
relationship: measurement_of ECOSIMCONCEPT:MgHCO3 ! Magnesium bicarbonate

[Term]
id: ECOSIM:CMGOQ
name: surface irrigation MgOH concentration
def: "Surface irrigation MgOH concentration refers to the concentration of magnesium hydroxide (MgOH) in water used for surface irrigation. It is a parameter used in earth systems modeling to quantify the amount of MgOH present in the irrigation water, which has implications for plant health, soil fertility, and water quality. The concentration is typically expressed in units of milligrams per liter (mg/L) or parts per million (ppm)." []
is_a: ECOSIMCONCEPT:UnclassifiedVariable ! unclassified variable
relationship: attribute ECOSIMCONCEPT:Concentration ! Concentration
relationship: context ECOSIMCONCEPT:Irrigation ! Irrigation
relationship: has_unit ECOSIM:gm-3 ! g m-3
relationship: measured_in ECOSIMCONCEPT:Surface ! Surface
relationship: measurement_of ECOSIMCONCEPT:MgOH ! Magnesium hydroxide

[Term]
id: ECOSIM:CMGOR
name: precipitation MgOH concentration
def: "Precipitation MgOH concentration refers to the concentration of magnesium hydroxide (MgOH) in precipitation. It represents the amount of MgOH dissolved in water that falls as rain or snow onto the Earth's surface. This parameter is important for understanding the input of magnesium into ecosystems and its potential impacts on biogeochemical cycles and water quality." []
is_a: ECOSIM:CATEGORYAtmosphericConditions ! category - Atmospheric Conditions
is_a: ECOSIM:CATEGORYDepositionFlux ! category - deposition flux
relationship: attribute ECOSIMCONCEPT:Concentration ! Concentration
relationship: context ECOSIMCONCEPT:Precipitation ! Precipitation
relationship: has_unit ECOSIM:gm-3 ! g m-3
relationship: measured_in ECOSIMCONCEPT:Water ! Water
relationship: measurement_of ECOSIMCONCEPT:MgOH ! Magnesium hydroxide

[Term]
id: ECOSIM:CMGOU
name: subsurface irrigation MgOH concentration
def: "Subsurface irrigation MgOH concentration refers to the measurement and analysis of the concentration of magnesium hydroxide (MgOH) in water used for subsurface irrigation. It provides information about the amount of MgOH present in the irrigation water, which is important for understanding its impact on soil health and plant growth. This parameter is typically used in earth systems modeling to simulate subsurface irrigation practices and evaluate their effects on agricultural systems and water quality." []
is_a: ECOSIMCONCEPT:UnclassifiedVariable ! unclassified variable
relationship: attribute ECOSIMCONCEPT:Concentration ! Concentration
relationship: context ECOSIMCONCEPT:Irrigation ! Irrigation
relationship: has_unit ECOSIM:gm-3 ! g m-3
relationship: measured_in ECOSIMCONCEPT:Subsurface ! Subsurface
relationship: measurement_of ECOSIMCONCEPT:MgOH ! Magnesium hydroxide

[Term]
id: ECOSIM:CMGQ
name: surface irrigation Mg concentration
def: "Surface irrigation Mg concentration refers to the concentration of magnesium (Mg) in the water used for surface irrigation. It represents the amount of magnesium present in the irrigation water that is supplied to the land surface for agricultural purposes. This parameter is important for understanding and modeling the impact of irrigation practices on the soil magnesium levels and subsequent effects on crop growth, nutrient balance, and potential soil degradation." []
is_a: ECOSIMCONCEPT:UnclassifiedVariable ! unclassified variable
relationship: attribute ECOSIMCONCEPT:Concentration ! Concentration
relationship: context ECOSIMCONCEPT:Irrigation ! Irrigation
relationship: has_unit ECOSIM:gm-3 ! g m-3
relationship: measured_in ECOSIMCONCEPT:Surface ! Surface
relationship: measurement_of ECOSIMCONCEPT:Magnesium ! Magnesium

[Term]
id: ECOSIM:CMGR
name: precipitation Mg concentration
def: "Precipitation Mg concentration refers to the amount of magnesium (Mg) present in the water droplets or solid particles that fall from the atmosphere to the Earth's surface as precipitation. It is measured in milligrams (Mg) of magnesium per liter (L) of water. This parameter is important in Earth system modeling as it influences various biogeochemical processes, such as nutrient cycling and water quality in terrestrial and aquatic ecosystems. Changes in precipitation Mg concentration can have significant impacts on the health and productivity of both terrestrial and aquatic organisms." []
is_a: ECOSIM:CATEGORYAtmosphericConditions ! category - Atmospheric Conditions
is_a: ECOSIM:CATEGORYDepositionFlux ! category - deposition flux
relationship: attribute ECOSIMCONCEPT:Concentration ! Concentration
relationship: context ECOSIMCONCEPT:Precipitation ! Precipitation
relationship: has_unit ECOSIM:gm-3 ! g m-3
relationship: measured_in ECOSIMCONCEPT:Water ! Water
relationship: measurement_of ECOSIMCONCEPT:Magnesium ! Magnesium

[Term]
id: ECOSIM:CMGSQ
name: surface irrigation MgSO4 concentration
def: "Surface irrigation MgSO4 concentration refers to the concentration of magnesium sulfate (MgSO4) in the water used for surface irrigation. It is a parameter used in earth systems modeling to quantify the amount of MgSO4 present in irrigation water applied to land surfaces. This parameter is important as it can affect the soil fertility, crop growth, and overall water quality in agricultural systems." []
is_a: ECOSIMCONCEPT:UnclassifiedVariable ! unclassified variable
relationship: attribute ECOSIMCONCEPT:Concentration ! Concentration
relationship: context ECOSIMCONCEPT:SurfaceIrrigation ! SurfaceIrrigation
relationship: has_unit ECOSIM:gm-3 ! g m-3
relationship: measured_in ECOSIMCONCEPT:IrrigationWater ! IrrigationWater
relationship: measurement_of ECOSIMCONCEPT:MgSO4 ! Magnesium sulfate

[Term]
id: ECOSIM:CMGSR
name: precipitation MgSO4 concentration
def: "Precipitation MgSO4 concentration refers to the concentration of magnesium sulfate (MgSO4) in the precipitation, or the amount of MgSO4 dissolved in rainwater or snowfall. It represents the quantity of MgSO4 that is deposited onto the Earth's surface through atmospheric precipitation events. The measurement is typically expressed in milligrams per liter (mg/L) or parts per million (ppm) and is used to study the chemical composition of precipitation and its impacts on ecosystems and water quality." []
is_a: ECOSIMCONCEPT:UnclassifiedVariable ! unclassified variable
relationship: attribute ECOSIMCONCEPT:Concentration ! Concentration
relationship: has_unit ECOSIM:gm-3 ! g m-3
relationship: measured_in ECOSIMCONCEPT:Precipitation ! Precipitation
relationship: measurement_of ECOSIMCONCEPT:MgSO4 ! Magnesium sulfate

[Term]
id: ECOSIM:CMGSU
name: subsurface irrigation MgSO4 concentration
def: "Subsurface irrigation MgSO4 concentration refers to the concentration of magnesium sulfate (MgSO4) in the irrigation water used for subsurface irrigation systems. It is a parameter used in earth systems modeling to study the effects of different concentrations of MgSO4 on soil moisture dynamics, nutrient availability, and plant growth in subsurface irrigation scenarios. This parameter is typically expressed in units of mass of MgSO4 per unit volume of water (e.g., mg/L or g/m3) and is used to simulate and analyze the impacts of different MgSO4 concentrations on groundwater quality, soil salinity, and crop productivity in subsurface irrigated areas." []
is_a: ECOSIMCONCEPT:UnclassifiedVariable ! unclassified variable
relationship: attribute ECOSIMCONCEPT:Concentration ! Concentration
relationship: context ECOSIMCONCEPT:Irrigation ! Irrigation
relationship: has_unit ECOSIM:gm-3 ! g m-3
relationship: measured_in ECOSIMCONCEPT:Subsurface ! Subsurface
relationship: measurement_of ECOSIMCONCEPT:MgSO4 ! Magnesium sulfate

[Term]
id: ECOSIM:CMGU
name: subsurface irrigation Na concentration
def: "Subsurface irrigation Na concentration refers to the level of sodium (Na) concentration in the water used for subsurface irrigation. It represents the amount of sodium present in the irrigation water that is applied below the surface of the ground to the root zone of plants. This parameter is important in earth systems modeling as it can significantly affect the soil salinity, water quality, and plant health. High levels of Na concentration in the irrigation water can lead to the accumulation of salt in the soil, which can negatively impact plant growth and yield. Monitoring and managing subsurface irrigation Na concentration is essential to ensure sustainable agricultural practices and optimal plant performance." []
is_a: ECOSIMCONCEPT:UnclassifiedVariable ! unclassified variable
relationship: attribute ECOSIMCONCEPT:Concentration ! Concentration
relationship: context ECOSIMCONCEPT:Irrigation ! Irrigation
relationship: has_unit ECOSIM:gm-3 ! g m-3
relationship: measured_in ECOSIMCONCEPT:Subsurface ! Subsurface
relationship: measurement_of ECOSIMCONCEPT:Na ! Na

[Term]
id: ECOSIM:CN2Q
name: surface irrigation N2O concentration
def: "Surface irrigation N2O concentration refers to the concentration of nitrous oxide (N2O) in the atmosphere resulting from the surface application of water for agricultural irrigation. Nitrous oxide is a potent greenhouse gas and a significant contributor to climate change. The concentration measurement typically represents the amount of N2O per unit volume of air and is an important parameter for earth systems modeling to understand the impact of agricultural practices on greenhouse gas emissions." []
is_a: ECOSIMCONCEPT:UnclassifiedVariable ! unclassified variable
relationship: attribute ECOSIMCONCEPT:Concentration ! Concentration
relationship: context ECOSIMCONCEPT:Irrigation ! Irrigation
relationship: has_unit ECOSIM:gm-3 ! g m-3
relationship: measured_in ECOSIMCONCEPT:Surface ! Surface
relationship: measurement_of ECOSIMCONCEPT:NitrousOxide ! NitrousOxide

[Term]
id: ECOSIM:CN2R
name: precipitation N2O concentration
def: "Precipitation N2O concentration refers to the concentration of nitrous oxide (N2O) in the atmosphere associated with precipitation events. It represents the amount of N2O present in rain or snowfall, which can be influenced by various factors such as emissions from natural and anthropogenic sources, atmospheric chemical reactions, and deposition processes. Studying precipitation N2O concentration can provide insights into the cycling and distribution of this potent greenhouse gas in the Earth system." []
is_a: ECOSIM:CATEGORYAtmosphericConditions ! category - Atmospheric Conditions
is_a: ECOSIM:CATEGORYDepositionFlux ! category - deposition flux
relationship: attribute ECOSIMCONCEPT:Concentration ! Concentration
relationship: context ECOSIMCONCEPT:Precipitation ! Precipitation
relationship: has_unit ECOSIM:gm-3 ! g m-3
relationship: measured_in ECOSIMCONCEPT:Atmosphere ! Atmosphere
relationship: measurement_of ECOSIMCONCEPT:N2O ! Nitrous oxide

[Term]
id: ECOSIM:CN3
name: CN3
def: "CN3 is a general representation for a specific type of natural chemical compound. The exact identity and properties of this compound may vary depending on the context and the specific system being described." []
is_a: ECOSIM:CATEGORYBiogeochemistry ! category - Biogeochemistry
relationship: measured_in ECOSIMCONCEPT:Soil ! Soil

[Term]
id: ECOSIM:CN3Q
name: surface irrigation NH3 concentration
def: "Surface irrigation NH3 concentration refers to the concentration of ammonia (NH3) in the water used for surface irrigation. It represents the amount of ammonia dissolved in the irrigation water that can potentially interact with the soil and affect various biological and chemical processes within the surface ecosystem. This parameter is often measured in units of mass/volume (e.g., mg/L) and is crucial for understanding and modeling nutrient cycling, water quality, and the overall health and productivity of agricultural and natural systems impacted by surface irrigation practices." []
is_a: ECOSIMCONCEPT:UnclassifiedVariable ! unclassified variable
relationship: attribute ECOSIMCONCEPT:Concentration ! Concentration
relationship: context ECOSIMCONCEPT:Irrigation ! Irrigation
relationship: has_unit ECOSIM:gm-3 ! g m-3
relationship: measured_in ECOSIMCONCEPT:Surface ! Surface
relationship: measurement_of ECOSIMCONCEPT:NH3 ! Ammonia

[Term]
id: ECOSIM:CN3R
name: precipitation NH3 concentration
def: "Precipitation NH3 concentration refers to the level or amount of NH3 (Ammonia) present in the precipitation (rain, snow, sleet, etc.) in a given area or region. It is a parameter used in Earth system modeling to understand and simulate the distribution and impact of atmospheric NH3 deposition on ecosystems, air quality, and overall biogeochemical cycles. The concentration of NH3 in precipitation can be influenced by various sources such as agricultural activities, industrial emissions, and natural processes, and it plays a significant role in the nitrogen cycle and ecosystem dynamics." []
is_a: ECOSIM:CATEGORYAtmosphericConditions ! category - Atmospheric Conditions
is_a: ECOSIM:CATEGORYDepositionFlux ! category - deposition flux
relationship: attribute ECOSIMCONCEPT:Concentration ! Concentration
relationship: has_unit ECOSIM:gm-3 ! g m-3
relationship: measured_in ECOSIMCONCEPT:Precipitation ! Precipitation
relationship: measurement_of ECOSIMCONCEPT:NH3 ! Ammonia

[Term]
id: ECOSIM:CN4
name: CN4
def: "CN4 is a parameter often used in climatology, hydrology, and earth system science to describe the relationship between soil moisture and evapotranspiration." []
is_a: ECOSIM:CATEGORYBiogeochemistry ! category - Biogeochemistry
relationship: measured_in ECOSIMCONCEPT:Soil ! Soil
relationship: measurement_of ECOSIMCONCEPT:Evapotranspiration ! Evapotranspiration
relationship: measurement_of ECOSIMCONCEPT:Moisture ! Moisture

[Term]
id: ECOSIM:CN4Q
name: surface irrigation NH4 concentration
def: "Surface irrigation NH4 concentration refers to the concentration of ammonium (NH4) ions in water used for surface irrigation. Surface irrigation is a method of irrigation where water is directly applied to the soil surface and allowed to infiltrate and move through the crop root zone by gravity. The NH4 concentration in surface irrigation water is an important parameter that affects nutrient availability for plants and can impact soil fertility and water quality. Monitoring and managing NH4 concentration in surface irrigation water is crucial to ensure optimal plant growth and minimize potential environmental impacts." []
is_a: ECOSIMCONCEPT:UnclassifiedVariable ! unclassified variable
relationship: attribute ECOSIMCONCEPT:Concentration ! Concentration
relationship: context ECOSIMCONCEPT:Irrigation ! Irrigation
relationship: has_unit ECOSIM:gm-3 ! g m-3
relationship: measured_in ECOSIMCONCEPT:Surface ! Surface
relationship: measurement_of ECOSIMCONCEPT:NH4 ! Ammonium

[Term]
id: ECOSIM:CN4R
name: precipitation NH4 concentration
def: "Precipitation NH4 concentration refers to the concentration of NH4 (ammonium) ions in precipitation, typically measured in units of mass per volume. It represents the amount of ammonium present in rainwater, snow, or other forms of precipitation, providing insights into the level of nitrogen deposition onto terrestrial ecosystems. This parameter is important for understanding nutrient cycling and assessing the impact of atmospheric deposition on ecosystems, particularly in relation to nitrogen availability and potential effects on vegetation growth and water quality." []
is_a: ECOSIM:CATEGORYAtmosphericConditions ! category - Atmospheric Conditions
is_a: ECOSIM:CATEGORYDepositionFlux ! category - deposition flux
relationship: attribute ECOSIMCONCEPT:Concentration ! Concentration
relationship: has_unit ECOSIM:gm-3 ! g m-3
relationship: measured_in ECOSIMCONCEPT:Precipitation ! Precipitation
relationship: measurement_of ECOSIMCONCEPT:NH4 ! Ammonium

[Term]
id: ECOSIM:CN4RI
name: precipitation initial NH4 concentration
def: "Precipitation initial NH4 concentration refers to the concentration of ammonium (NH4+) ions in the initial state of precipitation, specifically in relation to Earth system modeling. It represents the amount of ammonium present in the atmospheric water vapor or cloud droplets at the beginning of a simulated precipitation event. This parameter is important for understanding the transport, deposition, and cycling of nitrogen in the atmosphere, as ammonium can impact ecosystem productivity and water quality when it is deposited onto land surfaces." []
is_a: ECOSIM:CATEGORYAtmosphericConditions ! category - Atmospheric Conditions
is_a: ECOSIM:CATEGORYDepositionFlux ! category - deposition flux
relationship: attribute ECOSIMCONCEPT:Concentration ! Concentration
relationship: context ECOSIMCONCEPT:Precipitation ! Precipitation
relationship: has_unit ECOSIM:gm-3 ! g m-3
relationship: measured_in ECOSIMCONCEPT:Water ! Water
relationship: measurement_of ECOSIMCONCEPT:NH4 ! Ammonium

[Term]
id: ECOSIM:CNA
name: soil Na content
def: "Soil Na content refers to the amount of sodium (Na) present in the soil. It is a parameter used in earth systems modeling to quantify the concentration of sodium ions in the soil. This parameter is important as it plays a crucial role in soil fertility, nutrient cycling, and plant growth. The soil Na content is typically expressed in units of mass per unit volume (e.g., grams per kilogram of soil)." []
is_a: ECOSIM:CATEGORYBiogeochemistry ! category - Biogeochemistry
is_a: ECOSIM:CATEGORYSoilBiogeochemistry ! category - Soil Biogeochemistry
is_a: ECOSIM:CATEGORYSoilProperty ! category - soil property
relationship: attribute ECOSIMCONCEPT:Content ! Content
relationship: has_unit ECOSIM:mgkg-1 ! mg kg-1
relationship: measured_in ECOSIMCONCEPT:Soil ! Soil
relationship: measurement_of ECOSIMCONCEPT:Na ! Na

[Term]
id: ECOSIM:CNACQ
name: surface irrigation NaCO3 concentration
def: "Surface irrigation NaCO3 concentration refers to the concentration of sodium carbonate (NaCO3) in the water used for surface irrigation. It represents the amount of sodium carbonate present in the irrigation water, which can have an impact on soil properties and vegetation growth. Higher concentrations of NaCO3 can lead to soil alkalinization and have adverse effects on crop growth and yield. Monitoring and managing surface irrigation NaCO3 concentration can help optimize irrigation practices and ensure sustainable agricultural production." []
is_a: ECOSIMCONCEPT:UnclassifiedVariable ! unclassified variable
relationship: attribute ECOSIMCONCEPT:Concentration ! Concentration
relationship: context ECOSIMCONCEPT:Irrigation ! Irrigation
relationship: has_unit ECOSIM:gm-3 ! g m-3
relationship: measured_in ECOSIMCONCEPT:Surface ! Surface
relationship: measurement_of ECOSIMCONCEPT:NaCO3 ! NaCO3

[Term]
id: ECOSIM:CNACR
name: precipitation NaCO3 concentration
def: "Precipitation NaCO3 concentration refers to the amount of sodium carbonate (NaCO3) present in atmospheric precipitation, such as rain or snow. It is a measure of the concentration of sodium carbonate dissolved in water particles within precipitation events. This parameter is important in Earth systems modeling as it can influence various environmental processes, including the pH of water bodies, nutrient availability, and chemical reaction rates in aquatic systems." []
is_a: ECOSIM:CATEGORYDepositionFlux ! category - deposition flux
is_a: ECOSIMCONCEPT:UnclassifiedVariable ! unclassified variable
relationship: attribute ECOSIMCONCEPT:Concentration ! Concentration
relationship: context ECOSIMCONCEPT:Precipitation ! Precipitation
relationship: has_unit ECOSIM:gm-3 ! g m-3
relationship: measured_in ECOSIMCONCEPT:Water ! Water
relationship: measurement_of ECOSIMCONCEPT:NaCO3 ! NaCO3

[Term]
id: ECOSIM:CNACU
name: subsurface irrigation NaCO3 concentration
def: "Subsurface irrigation NaCO3 concentration refers to the level of sodium carbonate (NaCO3) present in the irrigation water used in subsurface irrigation systems. It represents the amount of sodium carbonate dissolved in the water and is an important parameter in understanding the chemical composition and potential impacts of the irrigation water on soil and crops. This parameter helps in assessing the suitability of the water for subsurface irrigation and predicting the long-term effects on soil quality and plant health." []
is_a: ECOSIMCONCEPT:UnclassifiedVariable ! unclassified variable
relationship: attribute ECOSIMCONCEPT:Concentration ! Concentration
relationship: context ECOSIMCONCEPT:Irrigation ! Irrigation
relationship: has_unit ECOSIM:gm-3 ! g m-3
relationship: measured_in ECOSIMCONCEPT:Subsurface ! Subsurface
relationship: measurement_of ECOSIMCONCEPT:NaCO3 ! NaCO3

[Term]
id: ECOSIM:CNAQ
name: surface irrigation Na concentration
def: "Surface irrigation Na concentration refers to the concentration of sodium (Na) in the water used for surface irrigation. It represents the amount of sodium present in the irrigation water that is applied to the soil surface to meet the water demands of crops. This parameter is important in earth systems modeling as it influences soil salinity, affects plant growth and yield, and can have detrimental effects on the overall soil health and fertility. The surface irrigation Na concentration is typically measured in units of milligrams per liter (mg/L) or parts per million (ppm)." []
is_a: ECOSIMCONCEPT:UnclassifiedVariable ! unclassified variable
relationship: attribute ECOSIMCONCEPT:Concentration ! Concentration
relationship: context ECOSIMCONCEPT:Irrigation ! Irrigation
relationship: has_unit ECOSIM:gm-3 ! g m-3
relationship: measured_in ECOSIMCONCEPT:Surface ! Surface
relationship: measurement_of ECOSIMCONCEPT:Na ! Na

[Term]
id: ECOSIM:CNAR
name: precipitation Na concentration
def: "Precipitation Na concentration refers to the level of sodium (Na) present in atmospheric precipitation. It is a parameter used in Earth systems modeling to quantify the amount of sodium deposited from the atmosphere onto the Earth's surface through precipitation events. The concentration of sodium in precipitation can affect various biogeochemical processes, such as soil salinity, nutrient availability, and ecosystem health. Monitoring and understanding precipitation Na concentration is important for assessing the impacts of sodium deposition on the environment and human activities." []
is_a: ECOSIM:CATEGORYAtmosphericConditions ! category - Atmospheric Conditions
is_a: ECOSIM:CATEGORYDepositionFlux ! category - deposition flux
relationship: attribute ECOSIMCONCEPT:Concentration ! Concentration
relationship: has_unit ECOSIM:gm-3 ! g m-3
relationship: measured_in ECOSIMCONCEPT:Precipitation ! Precipitation
relationship: measurement_of ECOSIMCONCEPT:Na ! Na

[Term]
id: ECOSIM:CNASQ
name: surface irrigation NaSO4 concentration
def: "Surface irrigation NaSO4 concentration refers to the concentration of sodium sulfate present in the water used for surface irrigation. It represents the amount of sodium sulfate dissolved in the irrigation water that is applied to the land surface for crop irrigation purposes. The concentration is typically measured in terms of the mass of sodium sulfate per unit volume of water, such as milligrams per liter (mg/L) or parts per million (ppm). This parameter is important in earth systems modeling as it can have implications for soil salinity, water quality, and crop health." []
is_a: ECOSIMCONCEPT:UnclassifiedVariable ! unclassified variable
relationship: attribute ECOSIMCONCEPT:Concentration ! Concentration
relationship: context ECOSIMCONCEPT:Irrigation ! Irrigation
relationship: has_unit ECOSIM:gm-3 ! g m-3
relationship: measured_in ECOSIMCONCEPT:Surface ! Surface
relationship: measurement_of ECOSIMCONCEPT:NaSO4 ! NaSO4

[Term]
id: ECOSIM:CNASR
name: precipitation NaSO4 concentration
def: "Precipitation NaSO4 concentration refers to the amount of sodium sulfate (NaSO4) dissolved in rainwater or snowfall. It represents the concentration of NaSO4 in a given volume of precipitation, usually expressed in units such as milligrams per liter (mg/L) or parts per million (ppm). This parameter is relevant for studying the atmospheric deposition of NaSO4 and its potential impacts on soil, water bodies, and ecosystems." []
is_a: ECOSIM:CATEGORYDepositionFlux ! category - deposition flux
is_a: ECOSIMCONCEPT:UnclassifiedVariable ! unclassified variable
relationship: attribute ECOSIMCONCEPT:Concentration ! Concentration
relationship: context ECOSIMCONCEPT:Precipitation ! Precipitation
relationship: has_unit ECOSIM:gm-3 ! g m-3
relationship: measured_in ECOSIMCONCEPT:Water ! Water
relationship: measurement_of ECOSIMCONCEPT:NaSO4 ! NaSO4

[Term]
id: ECOSIM:CNASU
name: subsurface irrigation NaSO4 concentration
def: "Subsurface irrigation NaSO4 concentration refers to the concentration of sodium sulfate (NaSO4) in water used for subsurface irrigation. Subsurface irrigation involves the application of water directly to the root zone of plants through buried pipes or tubes. The NaSO4 concentration parameter is important because it indicates the amount of sodium sulfate present in the irrigation water, which can have implications for plant growth, soil salinity, and groundwater quality. High levels of NaSO4 concentration in irrigation water can lead to increased soil salinity, affecting plant health and productivity. Monitoring and controlling NaSO4 concentration in subsurface irrigation is crucial for sustainable agriculture and the prevention of adverse environmental impacts." []
is_a: ECOSIMCONCEPT:UnclassifiedVariable ! unclassified variable
relationship: attribute ECOSIMCONCEPT:Concentration ! Concentration
relationship: context ECOSIMCONCEPT:Irrigation ! Irrigation
relationship: has_unit ECOSIM:gm-3 ! g m-3
relationship: measured_in ECOSIMCONCEPT:Subsurface ! Subsurface
relationship: measurement_of ECOSIMCONCEPT:NaSO4 ! NaSO4

[Term]
id: ECOSIM:CNAU
name: subsurface irrigation K concentration
def: "Subsurface irrigation K concentration refers to the concentration of potassium (K) in the water used for subsurface irrigation. It is a parameter that is relevant for earth systems modeling, specifically in studying the effects of irrigation practices on soil fertility and plant nutrition. The K concentration can impact plant growth and productivity, as potassium is an essential nutrient for plants involved in various physiological processes. Monitoring and managing the K concentration in subsurface irrigation water can help optimize agricultural practices and enhance crop performance." []
is_a: ECOSIMCONCEPT:UnclassifiedVariable ! unclassified variable
relationship: attribute ECOSIMCONCEPT:Concentration ! Concentration
relationship: context ECOSIMCONCEPT:Irrigation ! Irrigation
relationship: has_unit ECOSIM:gm-3 ! g m-3
relationship: measured_in ECOSIMCONCEPT:Subsurface ! Subsurface
relationship: measurement_of ECOSIMCONCEPT:Potassium ! Potassium

[Term]
id: ECOSIM:CNEAR
name: ear N:C ratio
def: "The Earth Nitrogen-to-Carbon (N:C) ratio refers to the ratio of nitrogen atoms to carbon atoms in terrestrial ecosystems. It represents the relative abundance of these two elements within the organic matter present in soils, plants, and other components of the ecosystem. The N:C ratio is a crucial parameter in earth systems modeling as it influences nutrient cycling, ecosystem productivity, and the availability of nitrogen for plant growth. It is often used to quantify the nitrogen limitation on primary production and can vary across different ecosystem types and soil conditions." []
is_a: ECOSIM:CATEGORYBiogeochemistry ! category - Biogeochemistry
is_a: ECOSIM:CATEGORYCanopyStructure ! category - canopy structure
relationship: has_unit ECOSIM:gg-1 ! g g-1
relationship: measurement_of ECOSIMCONCEPT:NitrogenCarbonRatio ! NitrogenCarbonRatio

[Term]
id: ECOSIM:CNETX
name: total net canopy CO2 exchange
def: "Total net canopy CO2 exchange refers to the overall balance of carbon dioxide (CO2) uptake and release by vegetation in the Earth's ecosystems. It represents the net difference between the photosynthetic uptake of CO2 by plants during photosynthesis and the CO2 released during respiration and other processes. This parameter is influenced by various factors, including environmental conditions such as temperature, light intensity, and CO2 concentration, as well as the physiological characteristics of the vegetation. Understanding the total net canopy CO2 exchange is crucial for quantifying the carbon cycle and predicting the impact of climate change on terrestrial ecosystems." []
is_a: ECOSIM:CATEGORYPlantPhysiology ! category - plant physiology
is_a: ECOSIMCONCEPT:UnclassifiedVariable ! unclassified variable
relationship: attribute ECOSIMCONCEPT:NetExchange ! Net exchange
relationship: has_unit ECOSIM:gd-2h-1 ! g d-2 h-1
relationship: measured_in ECOSIMCONCEPT:Canopy ! Canopy
relationship: measurement_of ECOSIMCONCEPT:CO2 ! Carbon dioxide

[Term]
id: ECOSIM:CNGR
name: grain N:C ratio
def: "The grain N:C ratio refers to the ratio of nitrogen (N) to carbon (C) in the grain of a plant. It is a parameter used in earth systems modeling to represent the nutritional content and quality of agricultural crops. The grain N:C ratio influences various physiological and ecological processes, such as plant growth, nutrient cycling, and interactions with soil microorganisms. It is an important factor in understanding nutrient dynamics in agricultural systems and predicting the impact of changes in land use and management practices on crop productivity and ecosystem functioning." []
is_a: ECOSIM:CATEGORYCanopyStructure ! category - canopy structure
relationship: has_unit ECOSIM:gg-1 ! g g-1
relationship: measured_in ECOSIMCONCEPT:Grain ! Grain
relationship: measurement_of ECOSIMCONCEPT:NitrogenCarbonRatio ! NitrogenCarbonRatio

[Term]
id: ECOSIM:CNH4
name: soil NH4 content
def: "Soil NH4 content refers to the amount of ammonium (NH4) ions present in the soil. Ammonium is a form of nitrogen essential for plant growth, necessary for the synthesis of amino acids, proteins, and other organic compounds in plants. It plays a crucial role in the nitrogen cycling process and is a parameter of interest in studies related to soil fertility, crop production, environmental health, and global change." []
is_a: ECOSIM:CATEGORYBiogeochemistry ! category - Biogeochemistry
relationship: attribute ECOSIMCONCEPT:Content ! Content
relationship: has_unit ECOSIM:mgkg-1 ! mg kg-1
relationship: measured_in ECOSIMCONCEPT:Soil ! Soil
relationship: measurement_of ECOSIMCONCEPT:NH4 ! Ammonium

[Term]
id: ECOSIM:CNHSK
name: husk N:C ratio
is_a: ECOSIM:CATEGORYCanopyStructure ! category - canopy structure
relationship: has_unit ECOSIM:gg-1 ! g g-1
relationship: measurement_of ECOSIMCONCEPT:NitrogenCarbonRatio ! NitrogenCarbonRatio
relationship: qualifier ECOSIMCONCEPT:Husk ! Husk

[Term]
id: ECOSIM:CNLF
name: maximum leaf N:C ratio
def: "The maximum leaf nitrogen to carbon ratio, often represented as CNLF, refers to the maximum ratio of the amount of nitrogen to the amount of carbon in a leaf. This measure provides critical information about a plant's nutritional status and growth potential. A high nitrogen to carbon ratio in leaves typically indicates a high rate of photosynthesis and growth." []
is_a: ECOSIM:CATEGORYCanopyStructure ! category - canopy structure
is_a: ECOSIM:CATEGORYPlantPhysiology ! category - plant physiology
relationship: has_unit ECOSIM:gg-1 ! g g-1
relationship: measured_in ECOSIMCONCEPT:Leaf ! Leaf
relationship: measurement_of ECOSIMCONCEPT:Carbon ! Carbon
relationship: measurement_of ECOSIMCONCEPT:Nitrogen ! Nitrogen

[Term]
id: ECOSIM:CNND
name: nodule N:C ratio
is_a: ECOSIM:CATEGORYCanopyStructure ! category - canopy structure
relationship: context ECOSIMCONCEPT:NitrogenCarbonRatio ! NitrogenCarbonRatio
relationship: has_unit ECOSIM:gg-1 ! g g-1
relationship: measurement_of ECOSIMCONCEPT:Nodule ! Nodule

[Term]
id: ECOSIM:CNNQ
name: surface irrigation N2 concentration
def: "Surface irrigation N2 concentration refers to the concentration of Nitrogen (N2) in the irrigation water used for surface irrigation. N2 is a crucial nutrient for plant growth and development but excessive concentrations can lead to nutrient pollution, affecting soil and water quality. Monitoring and controlling the N2 concentration in surface irrigation can help optimize plant growth, ensure proper soil health and prevent environmental degradation." []
is_a: ECOSIMCONCEPT:UnclassifiedVariable ! unclassified variable
relationship: attribute ECOSIMCONCEPT:Concentration ! Concentration
relationship: context ECOSIMCONCEPT:Irrigation ! Irrigation
relationship: has_unit ECOSIM:gm-3 ! g m-3
relationship: measured_in ECOSIMCONCEPT:Surface ! Surface
relationship: measurement_of ECOSIMCONCEPT:N2 ! Dinitrogen

[Term]
id: ECOSIM:CNNR
name: precipitation N2 concentration
def: "Precipitation N2 concentration refers to the amount of nitrogen gas (N2) in solution that is formed during or after a precipitation event, such as rain or snowfall. It represents the concentration of N2 particles present in the water as a result of interactions between atmospheric emissions and environmental conditions. This parameter is important in Earth system modeling as it can affect various ecological and biogeochemical processes in aquatic ecosystems, including nutrient cycling, pH regulation, and the bioavailability of other elements." []
is_a: ECOSIM:CATEGORYAtmosphericConditions ! category - Atmospheric Conditions
is_a: ECOSIM:CATEGORYDepositionFlux ! category - deposition flux
relationship: attribute ECOSIMCONCEPT:Concentration ! Concentration
relationship: context ECOSIMCONCEPT:Precipitation ! Precipitation
relationship: has_unit ECOSIM:gm-3 ! g m-3
relationship: measured_in ECOSIMCONCEPT:Water ! Water
relationship: measurement_of ECOSIMCONCEPT:N2 ! Dinitrogen

[Term]
id: ECOSIM:CNO
name: CNO
def: "CNO stands for Carbon, Nitrogen and Oxygen. These elements are essential for life and are considered as primary elements. The carbon, nitrogen, and oxygen cycles are major biogeochemical cycles responsible for the transformation and movement of these elements through the Earth's atmosphere, biosphere, and lithosphere." []
is_a: ECOSIM:CATEGORYBiogeochemistry ! category - Biogeochemistry
is_a: ECOSIMCONCEPT:Element ! Element

[Term]
id: ECOSIM:CNO3
name: soil NO3 content
def: "Soil NO3 Content measures the amount of nitrate (NO3) in the soil. Nitrate is a key nutrient for plant growth which is obtained from fertilisers or organic matter decomposing. It is lost from the soil through the processes of leaching, denitrification and uptake by plants. Excessive amounts of nitrate in the soil can also pose environmental problems and contaminates groundwater. Therefore, monitoring of the NO3 content in soil is important in environmental research." []
is_a: ECOSIM:CATEGORYBiogeochemistry ! category - Biogeochemistry
is_a: ECOSIM:CATEGORYSoilBiogeochemistry ! category - Soil Biogeochemistry
relationship: attribute ECOSIMCONCEPT:Content ! Content
relationship: has_unit ECOSIM:mgkg-1 ! mg kg-1
relationship: measured_in ECOSIMCONCEPT:Soil ! Soil
relationship: measurement_of ECOSIMCONCEPT:NO3 ! Nitrate

[Term]
id: ECOSIM:CNOQ
name: surface irrigation NO3 concentration
def: "Surface irrigation NO3 concentration refers to the concentration of nitrate (NO3) in the irrigation water used for surface irrigation. Surface irrigation involves the application of water to the soil surface to infiltrate and reach the plant roots. The 'NO3 concentration' parameter is crucial because nitrate is a major nutrient required by plants for growth. However, excessive nitrate concentration can lead to various environmental issues such as water pollution and eutrophication." []
is_a: ECOSIMCONCEPT:UnclassifiedVariable ! unclassified variable
relationship: attribute ECOSIMCONCEPT:Concentration ! Concentration
relationship: context ECOSIMCONCEPT:Irrigation ! Irrigation
relationship: has_unit ECOSIM:gm-3 ! g m-3
relationship: measured_in ECOSIMCONCEPT:Surface ! Surface
relationship: measurement_of ECOSIMCONCEPT:NO3 ! Nitrate

[Term]
id: ECOSIM:CNOR
name: precipitation NO3 concentration
def: "Precipitation NO3 concentration refers to the amount of nitrate (NO3) in a solution that is formed during or after a precipitation event, such as rain or snow. It represents the concentration of NO3 particles present in the water as a result of interactions between atmospheric emissions and environmental conditions. This parameter is significant in Earth system modeling as it can impact various ecological and biogeochemical processes in aquatic ecosystems, including nutrient cycling and the bioavailability of other elements." []
is_a: ECOSIM:CATEGORYAtmosphericConditions ! category - Atmospheric Conditions
is_a: ECOSIM:CATEGORYHydrology ! category - Hydrology
relationship: attribute ECOSIMCONCEPT:Concentration ! Concentration
relationship: context ECOSIMCONCEPT:Precipitation ! Precipitation
relationship: has_unit ECOSIM:gm-3 ! g m-3
relationship: measured_in ECOSIMCONCEPT:Water ! Water
relationship: measurement_of ECOSIMCONCEPT:NO3 ! Nitrate

[Term]
id: ECOSIM:CNORI
name: precipitation initial NO3 concentration
def: "Precipitation initial NO3 concentration refers to the initial concentration of nitrate (NO3) present in falling rain or snow. Atmospheric nitrates can be deposited onto the Earth's surface during precipitation events and enter terrestrial and aquatic ecosystems. This measurement is important for understanding the biogeochemical nitrogen cycle, nutrient availability, and potential impacts on environmental and human health from elevated nitrate levels." []
is_a: ECOSIM:CATEGORYAtmosphericConditions ! category - Atmospheric Conditions
is_a: ECOSIM:CATEGORYDepositionFlux ! category - deposition flux
relationship: attribute ECOSIMCONCEPT:Concentration ! Concentration
relationship: context ECOSIMCONCEPT:Precipitation ! Precipitation
relationship: has_unit ECOSIM:gm-3 ! g m-3
relationship: measured_in ECOSIMCONCEPT:Water ! Water
relationship: measurement_of ECOSIMCONCEPT:NO3 ! Nitrate

[Term]
id: ECOSIM:CNRSV
name: reserve N:C ratio
is_a: ECOSIM:CATEGORYCanopyStructure ! category - canopy structure
relationship: has_unit ECOSIM:gg-1 ! g g-1
relationship: measurement_of ECOSIMCONCEPT:NitrogenCarbonRatio ! NitrogenCarbonRatio
relationship: qualifier ECOSIMCONCEPT:Reserve ! Reserve

[Term]
id: ECOSIM:CNRT
name: root N:C ratio
is_a: ECOSIM:CATEGORYRootPhysiology ! category - root physiology
relationship: has_unit ECOSIM:gg-1 ! g g-1
relationship: measurement_of ECOSIMCONCEPT:NitrogenCarbonRatio ! NitrogenCarbonRatio
relationship: qualifier ECOSIMCONCEPT:Root ! Root

[Term]
id: ECOSIM:CNRTS
name: root N:C ratio x root growth yield
def: "Root N:C ratio x root growth yield (CNRTS) is a measure of the relative investment in root nitrogen (N) versus root carbon (C) during root growth. This ratio influences important aspects of plant growth, development, and nutrient use efficiency. In the context of earth systems modeling, CNRTS can play a critical role in simulating plant nutrient dynamics and their influence on broader ecosystem functions." []
is_a: ECOSIM:CATEGORYPlantPhysiology ! category - plant physiology
is_a: ECOSIM:CATEGORYRootPhysiology ! category - root physiology
relationship: measured_in ECOSIMCONCEPT:RootGrowthYield ! RootGrowthYield
relationship: measurement_of ECOSIMCONCEPT:Root ! Root

[Term]
id: ECOSIM:CNSHE
name: sheath N:C ratio
is_a: ECOSIM:CATEGORYCanopyStructure ! category - canopy structure
relationship: has_unit ECOSIM:gg-1 ! g g-1
relationship: measurement_of ECOSIMCONCEPT:CarbonNitrogenRatio ! CarbonNitrogenRatio
relationship: qualifier ECOSIMCONCEPT:Sheath ! Sheath

[Term]
id: ECOSIM:CNSTK
name: stalk N:C ratio
is_a: ECOSIM:CATEGORYCanopyStructure ! category - canopy structure
relationship: has_unit ECOSIM:gg-1 ! g g-1
relationship: measurement_of ECOSIMCONCEPT:NitrogenCarbonRatio ! NitrogenCarbonRatio
relationship: qualifier ECOSIMCONCEPT:Stalk ! Stalk

[Term]
id: ECOSIM:CNWS
name: C:N ratio in remobilizable nonstructural biomass
def: "C:N ratio in remobilizable nonstructural biomass (CNWS) refers to the ratio of carbon to nitrogen in the pool of nonstructural biomass that can be readily remobilized or redistributed within a plant. Nonstructural biomass includes compounds like sugars, amino acids, and lipids that are not incorporated into the plant's structural tissues. These compounds can be remobilized and used as resources during periods of stress or for growth. Understanding the CNWS ratio is important for predicting plant response to environmental changes and for modeling nutrient cycling in ecosystems." []
is_a: ECOSIM:CATEGORYCanopyStructure ! category - canopy structure
is_a: ECOSIM:CATEGORYPlantPhysiology ! category - plant physiology
relationship: measurement_of ECOSIMCONCEPT:CNRatio ! CNRatio

[Term]
id: ECOSIM:CNZU
name: subsurface irrigation Al concentration
def: "Subsurface irrigation refers to the practice of applying water and nutrients to crops or plants by delivering them directly to the root zone below the soil surface. It involves the use of specialized irrigation systems that distribute water and nutrients through buried pipes or tubes, allowing for efficient and controlled delivery to plant roots. The 'Al concentration' in the context of subsurface irrigation refers to the concentration of aluminum in the irrigation water or soil solution. Monitoring and controlling the Al concentration in subsurface irrigation systems is therefore important for optimizing plant health and productivity." []
is_a: ECOSIM:CATEGORYBiogeochemistry ! category - Biogeochemistry
relationship: attribute ECOSIMCONCEPT:Concentration ! Concentration
relationship: context ECOSIMCONCEPT:Irrigation ! Irrigation
relationship: has_unit ECOSIM:gm-3 ! g m-3
relationship: measured_in ECOSIMCONCEPT:Subsurface ! Subsurface
relationship: measurement_of ECOSIMCONCEPT:Al ! Aluminum

[Term]
id: ECOSIM:CO2B
name: bundle sheath nonstructural C3 content in C4 photosynthesis
def: "The bundle sheath nonstructural C3 content in C4 photosynthesis refers to the amount of non-structural carbon compounds in the bundle sheath cells of C4 plants during photosynthesis. Non-structural carbon compounds are essential for plant growth and survival, and play a crucial role in C4 photosynthesis which is a specialized form of photosynthesis that optimizes carbon uptake and water use efficiency." []
is_a: ECOSIM:CATEGORYCanopyPhysiology ! category - Canopy Physiology
is_a: ECOSIM:CATEGORYPlantPhysiology ! category - plant physiology
relationship: context ECOSIMCONCEPT:C4Photosynthesis ! C4Photosynthesis
relationship: has_unit ECOSIM:gd-2 ! g d-2
relationship: measured_in ECOSIMCONCEPT:BundleSheathCell ! BundleSheathCell
relationship: measurement_of ECOSIMCONCEPT:NonstructuralC3Content ! NonstructuralC3Content

[Term]
id: ECOSIM:CO2E
name: atmospheric CO2 concentration
def: "Atmospheric CO2 concentration refers to the amount of carbon dioxide present in the atmosphere. It is an important parameter in earth science and biochemistry. The concentration of CO2 in the atmosphere can affect global warming and climate change, as CO2 is a greenhouse gas that traps heat in the earth's atmosphere." []
is_a: ECOSIM:CATEGORYAtmosphericConditions ! category - Atmospheric Conditions
is_a: ECOSIMCONCEPT:UnclassifiedVariable ! unclassified variable
relationship: attribute ECOSIMCONCEPT:Concentration ! Concentration
relationship: has_unit ECOSIM:umolmol-1 ! umol mol-1
relationship: measured_in ECOSIMCONCEPT:Air ! Air
relationship: measurement_of ECOSIMCONCEPT:CO2 ! Carbon dioxide

[Term]
id: ECOSIM:CO2EI
name: initial atmospheric CO2 concentration
is_a: ECOSIM:CATEGORYAtmosphericConditions ! category - Atmospheric Conditions
is_a: ECOSIMCONCEPT:UnclassifiedVariable ! unclassified variable
relationship: attribute ECOSIMCONCEPT:Concentration ! Concentration
relationship: has_unit ECOSIM:umolmol-1 ! umol mol-1
relationship: measured_in ECOSIMCONCEPT:Atmosphere ! Atmosphere
relationship: measurement_of ECOSIMCONCEPT:CO2 ! Carbon dioxide

[Term]
id: ECOSIM:CO2I
name: leaf gaseous CO2 concentration
is_a: ECOSIM:CATEGORYCanopyPhysiology ! category - Canopy Physiology
is_a: ECOSIM:CATEGORYPlantPhysiology ! category - plant physiology
relationship: attribute ECOSIMCONCEPT:Concentration ! Concentration
relationship: has_unit ECOSIM:umolm-3 ! umol m-3
relationship: measured_in ECOSIMCONCEPT:Leaf ! Leaf
relationship: measurement_of ECOSIMCONCEPT:CO2 ! Carbon dioxide

[Term]
id: ECOSIM:CO2L
name: leaf aqueous CO2 concentration
is_a: ECOSIM:CATEGORYCanopyPhysiology ! category - Canopy Physiology
is_a: ECOSIM:CATEGORYPlantPhysiology ! category - plant physiology
relationship: attribute ECOSIMCONCEPT:Concentration ! Concentration
relationship: has_unit ECOSIM:uM ! uM
relationship: measured_in ECOSIMCONCEPT:Leaf ! Leaf
relationship: measurement_of ECOSIMCONCEPT:CO2 ! Carbon dioxide
relationship: qualifier ECOSIMCONCEPT:Aqueous ! Aqueous

[Term]
id: ECOSIM:CO2NetFix_pft
name: canopy net CO2 exchange
def: "Canopy net CO2 exchange (CO2NetFix_pft) refers to the overall balance between carbon dioxide (CO2) uptake and release by the vegetation canopy of a specific plant functional type (pft) in a given ecosystem. It represents the net amount of CO2 absorbed by the vegetation through photosynthesis minus the amount of CO2 released through respiration and other processes. The CO2NetFix_pft parameter is essential for understanding the carbon cycle and its interaction with the atmosphere, as well as for modeling and simulating ecosystem dynamics and responses to environmental changes." []
is_a: ECOSIM:CATEGORYPlantPhysiology ! category - plant physiology
is_a: ECOSIMCONCEPT:UnclassifiedVariable ! unclassified variable
relationship: attribute ECOSIMCONCEPT:NetExchange ! Net exchange
relationship: has_unit ECOSIM:gd-2h-1 ! g d-2 h-1
relationship: measured_in ECOSIMCONCEPT:Canopy ! Canopy
relationship: measurement_of ECOSIMCONCEPT:CO2 ! Carbon dioxide

[Term]
id: ECOSIM:CO2Q
name: canopy gaesous CO2 concentration
def: "Canopy gaseous CO2 concentration, represented as CO2Q, refers to the concentration of carbon dioxide (CO2) in the gaseous phase within the canopy of vegetation. It is particularly important in studying canopy-atmosphere exchange of CO2 which plays important roles in processes such as photosynthesis, respiration and transpiration." []
is_a: ECOSIM:CATEGORYCanopyPhysiology ! category - Canopy Physiology
is_a: ECOSIM:CATEGORYPlantPhysiology ! category - plant physiology
relationship: attribute ECOSIMCONCEPT:Concentration ! Concentration
relationship: has_unit ECOSIM:umolmol-1 ! umol mol-1
relationship: measured_in ECOSIMCONCEPT:Canopy ! Canopy
relationship: measurement_of ECOSIMCONCEPT:CO2 ! Carbon dioxide

[Term]
id: ECOSIM:COA
name: COA
def: "COA refers to a coenzyme A, a non-protein chemical compound that is required for the biological activity of certain proteins. It plays a central role in the functioning of cellular respiration, lipid metabolism, and many other metabolic pathways." []
is_a: ECOSIM:CATEGORYBiogeochemistry ! category - Biogeochemistry
relationship: measurement_of ECOSIMCONCEPT:MetabolicActivity ! MetabolicActivity

[Term]
id: ECOSIM:COAU
name: subsurface irrigation acetate concentration
def: "Subsurface irrigation refers to the practice of applying water and nutrients to crops or plants by delivering them directly to the root zone below the soil surface. It involves the use of specialized irrigation systems that distribute water and nutrients through buried pipes or tubes, allowing for efficient and controlled delivery to plant roots. The 'acetate concentration' in the context of subsurface irrigation refers to the concentration of acetate ions in the irrigation water or soil solution. Acetate is an important source of carbon for microbial populations in the soil, and its concentration can influence microbial activity, soil health, and plant growth. Monitoring and controlling the acetate concentration in subsurface irrigation systems is therefore important for optimizing soil and plant health." []
is_a: ECOSIMCONCEPT:UnclassifiedVariable ! unclassified variable
relationship: attribute ECOSIMCONCEPT:Concentration ! Concentration
relationship: context ECOSIMCONCEPT:Irrigation ! Irrigation
relationship: has_unit ECOSIM:gm-3 ! g m-3
relationship: measured_in ECOSIMCONCEPT:Subsurface ! Subsurface
relationship: measurement_of ECOSIMCONCEPT:Acetate ! Acetate

[Term]
id: ECOSIM:COC
name: COC
def: "COC (Carbon Organic Compound) refers to any organic compound containing carbon atoms. These can include a wide variety of compounds, such as hydrocarbons, alcohols, sugars, and proteins. COC plays a significant role in the carbon cycle and is an important parameter in earth systems modeling." []
is_a: ECOSIM:CATEGORYBiogeochemistry ! category - Biogeochemistry
relationship: measurement_of ECOSIMCONCEPT:Carbon ! Carbon

[Term]
id: ECOSIM:COCU
name: subsurface irrigation DOC concentration
def: "Subsurface irrigation refers to the practice of applying water and nutrients to crops or plants by delivering them directly to the root zone below the soil surface. It involves the use of specialized irrigation systems that distribute water and nutrients through buried pipes or tubes, allowing for efficient and controlled delivery to plant roots. The 'DOC concentration' in the context of subsurface irrigation refers to the concentration of dissolved organic carbon (DOC) in the irrigation water or soil solution. DOC is an important factor in soil fertility and nutrient cycling, playing key roles in microbial activity, soil aggregation, and the sequestration and transport of nutrients. The concentration of DOC can influence biological and chemical processes in the soil, as well as plant growth and yield. Monitoring and controlling the DOC concentration in subsurface irrigation systems is therefore important for optimizing soil fertility and plant health." []
is_a: ECOSIMCONCEPT:UnclassifiedVariable ! unclassified variable
relationship: attribute ECOSIMCONCEPT:Concentration ! Concentration
relationship: context ECOSIMCONCEPT:Irrigation ! Irrigation
relationship: has_unit ECOSIM:gm-3 ! g m-3
relationship: measured_in ECOSIMCONCEPT:Subsurface ! Subsurface
relationship: measurement_of ECOSIMCONCEPT:DOC ! DOC

[Term]
id: ECOSIM:COHQ
name: surface irrigation OH concentration
def: "Surface irrigation OH concentration refers to the concentration of hydroxide ions (OH-) in the irrigation water used for surface irrigation. Hydroxide ions are an important component of the pH balance in water, with higher concentrations leading to more alkaline conditions. Measuring and controlling the OH- concentration in surface irrigation can help maintain appropriate soil conditions for plant growth." []
is_a: ECOSIMCONCEPT:UnclassifiedVariable ! unclassified variable
relationship: attribute ECOSIMCONCEPT:Concentration ! Concentration
relationship: context ECOSIMCONCEPT:Irrigation ! Irrigation
relationship: has_unit ECOSIM:gm-3 ! g m-3
relationship: measured_in ECOSIMCONCEPT:Surface ! Surface
relationship: measurement_of ECOSIMCONCEPT:OH ! OH

[Term]
id: ECOSIM:COHR
name: precipitation OH concentration
def: "Precipitation OH concentration refers to the amount of hydroxide (OH) in a solution that is formed during or after a precipitation event, such as rain or snowfall. It represents the concentration of OH particles present in the water as a result of interactions between atmospheric emissions and environmental conditions. This parameter is important in Earth system modeling as it can affect various ecological and biogeochemical processes in aquatic ecosystems, including nutrient cycling and pH regulation." []
is_a: ECOSIM:CATEGORYAtmosphericConditions ! category - Atmospheric Conditions
is_a: ECOSIM:CATEGORYDepositionFlux ! category - deposition flux
relationship: attribute ECOSIMCONCEPT:Concentration ! Concentration
relationship: context ECOSIMCONCEPT:Precipitation ! Precipitation
relationship: has_unit ECOSIM:gm-3 ! g m-3
relationship: measured_in ECOSIMCONCEPT:Water ! Water
relationship: measurement_of ECOSIMCONCEPT:Hydroxide ! Hydroxide

[Term]
id: ECOSIM:COHU
name: subsurface irrigation SO4 concentration
def: "Subsurface irrigation refers to the practice of applying water and nutrients to crops or plants by delivering them directly to the root zone below the soil surface. It involves the use of specialized irrigation systems that distribute water and nutrients through buried pipes or tubes, allowing for efficient and controlled delivery to plant roots. The 'SO4 concentration' in the context of subsurface irrigation refers to the concentration of sulfate (SO4) in the irrigation water or soil solution. SO4 is a vital nutrient for plant growth. The concentration of SO4 can impact nutrient availability and uptake by plants, as well as plant growth and yield. Therefore, monitoring and controlling the SO4 concentration in subsurface irrigation systems is critical for optimizing plant health and performance." []
is_a: ECOSIMCONCEPT:UnclassifiedVariable ! unclassified variable
relationship: attribute ECOSIMCONCEPT:Concentration ! Concentration
relationship: context ECOSIMCONCEPT:Irrigation ! Irrigation
relationship: has_unit ECOSIM:gm-3 ! g m-3
relationship: measured_in ECOSIMCONCEPT:Subsurface ! Subsurface
relationship: measurement_of ECOSIMCONCEPT:SO4 ! SO4

[Term]
id: ECOSIM:COMPL
name: CO2 compensation point
def: "CO2 compensation point (COMPL) is the concentration of CO2 in the atmosphere at which the rate of photosynthesis exactly equals the rate of respiration, resulting in no net gas exchange between the plant and the atmosphere. The value is a critical physiological parameter as it influences the carbon balance of plants and ecosystems." []
is_a: ECOSIM:CATEGORYCanopyPhysiology ! category - Canopy Physiology
is_a: ECOSIM:CATEGORYPlantPhysiology ! category - plant physiology
relationship: has_unit ECOSIM:uM ! uM
relationship: measured_in ECOSIMCONCEPT:Plant ! Plant
relationship: measurement_of ECOSIMCONCEPT:CO2Concentration ! CO2Concentration

[Term]
id: ECOSIM:CON
name: CON
def: "Undefined OntologyClass" []
is_a: ECOSIM:CATEGORYBiogeochemistry ! category - Biogeochemistry

[Term]
id: ECOSIM:CONU
name: subsurface irrigation DON concentration
def: "Subsurface irrigation refers to the practice of applying water and nutrients to crops or plants by delivering them directly to the root zone below the soil surface. Dissolved Organic Nitrogen (DON) concentration in the context of subsurface irrigation refers to the concentration of DON in the irrigation water or soil solution. DON is an important source of nitrogen, an essential nutrient for plant growth. The concentration of DON can influence nutrient availability and uptake by plants, as well as plant growth and yield. Monitoring and controlling the DON concentration in subsurface irrigation systems is therefore important for optimizing plant health and productivity." []
is_a: ECOSIMCONCEPT:UnclassifiedVariable ! unclassified variable
relationship: attribute ECOSIMCONCEPT:Concentration ! Concentration
relationship: context ECOSIMCONCEPT:Irrigation ! Irrigation
relationship: has_unit ECOSIM:gm-3 ! g m-3
relationship: measured_in ECOSIMCONCEPT:Subsurface ! Subsurface
relationship: measurement_of ECOSIMCONCEPT:DissolvedOrganicNitrogen ! Dissolved organic nitrogen

[Term]
id: ECOSIM:COPU
name: subsurface irrigation DOP concentration
def: "Subsurface irrigation refers to the practice of applying water and nutrients to crops or plants by delivering them directly to the root zone below the soil surface. It involves the use of specialized irrigation systems that distribute water and nutrients through buried pipes or tubes, allowing for efficient and controlled delivery to plant roots. The 'DOP (Dissolved Organic Phosphorus) concentration' in the context of subsurface irrigation refers to the concentration of dissolved organic phosphorus in the irrigation water or soil solution. This is an important source of phosphorus for plant growth, and its concentration can influence nutrient availability and uptake by plants. Monitoring and controlling the DOP concentration in subsurface irrigation systems is therefore important for optimizing plant productivity." []
is_a: ECOSIMCONCEPT:UnclassifiedVariable ! unclassified variable
relationship: attribute ECOSIMCONCEPT:Concentration ! Concentration
relationship: context ECOSIMCONCEPT:Irrigation ! Irrigation
relationship: has_unit ECOSIM:gm-3 ! g m-3
relationship: measured_in ECOSIMCONCEPT:Subsurface ! Subsurface
relationship: measurement_of ECOSIMCONCEPT:DissolvedOrganicPhosphorus ! DissolvedOrganicPhosphorus

[Term]
id: ECOSIM:COQA
name: acetate concentration
is_a: ECOSIM:CATEGORYMicrobialActivity ! category - microbial activity
relationship: attribute ECOSIMCONCEPT:Concentration ! Concentration
relationship: has_unit ECOSIM:gm-3 ! g m-3
relationship: measured_in ECOSIMCONCEPT:Water ! Water
relationship: measurement_of ECOSIMCONCEPT:Acetate ! Acetate

[Term]
id: ECOSIM:COQC
name: DOC concentration
is_a: ECOSIM:CATEGORYMicrobialActivity ! category - microbial activity
relationship: attribute ECOSIMCONCEPT:Concentration ! Concentration
relationship: has_unit ECOSIM:gm-3 ! g m-3
relationship: measured_in ECOSIMCONCEPT:Water ! Water
relationship: measurement_of ECOSIMCONCEPT:OrganicCarbon ! OrganicCarbon

[Term]
id: ECOSIM:COXQ
name: surface irrigation O2 concentration
def: "Surface irrigation refers to a method of watering crops or plants where water is applied to the soil surface and allowed to infiltrate and reach the plant roots. The 'O2 concentration' parameter refers to the concentration of oxygen (O2) in the irrigation water used for surface irrigation. Oxygen is an essential element for plant growth and development. Monitoring and controlling the O2 concentration in surface irrigation can help optimize plant growth and ensure proper soil health." []
is_a: ECOSIMCONCEPT:UnclassifiedVariable ! unclassified variable
relationship: attribute ECOSIMCONCEPT:Concentration ! Concentration
relationship: context ECOSIMCONCEPT:Irrigation ! Irrigation
relationship: has_unit ECOSIM:gm-3 ! g m-3
relationship: measured_in ECOSIMCONCEPT:Surface ! Surface
relationship: measurement_of ECOSIMCONCEPT:O2 ! Dioxygen

[Term]
id: ECOSIM:COXR
name: precipitation O2 concentration
def: "Precipitation O2 concentration refers to the amount of Oxygen (O2) present in a precipitation event, such as rain or snowfall. This parameter is significant in understanding the oxidation process in aquatic ecosystems and can also provide insights into the atmospheric conditions during the formation of the precipitation." []
is_a: ECOSIM:CATEGORYAtmosphericConditions ! category - Atmospheric Conditions
is_a: ECOSIM:CATEGORYDepositionFlux ! category - deposition flux
relationship: attribute ECOSIMCONCEPT:Concentration ! Concentration
relationship: has_unit ECOSIM:gm-3 ! g m-3
relationship: measured_in ECOSIMCONCEPT:Precipitation ! Precipitation
relationship: measurement_of ECOSIMCONCEPT:O2 ! Dioxygen

[Term]
id: ECOSIM:CPEAR
name: ear P:C ratio
is_a: ECOSIM:CATEGORYCanopyStructure ! category - canopy structure
relationship: has_unit ECOSIM:gg-1 ! g g-1
relationship: measurement_of ECOSIMCONCEPT:PhosphorosCarbonRatio ! PhosphorosCarbonRatio
relationship: qualifier ECOSIMCONCEPT:Ear ! Ear

[Term]
id: ECOSIM:CPGR
name: grain P:C ratio
def: "Grain P:C ratio refers to the ratio of phosphorus to carbon in the grain part of a plant. It is an important parameter in understanding the nutrient balance within plants and can provide insights into plant health and productivity. The P:C ratio can also inform soil fertility management practices as both phosphorus and carbon are crucial nutrients in the soil-plant system." []
is_a: ECOSIM:CATEGORYCanopyStructure ! category - canopy structure
relationship: has_unit ECOSIM:gg-1 ! g g-1
relationship: measured_in ECOSIMCONCEPT:Grain ! Grain
relationship: measurement_of ECOSIMCONCEPT:PCRatio ! PCRatio

[Term]
id: ECOSIM:CPHSK
name: husk P:C ratio
def: "Husk P:C ratio is the ratio of phosphorous to carbon in a plant husk. This quantity reflects the nutrient status of the plant and has important implications for the return of these elements to the soil when the plant dies and decomposes." []
is_a: ECOSIM:CATEGORYCanopyStructure ! category - canopy structure
relationship: has_unit ECOSIM:gg-1 ! g g-1
relationship: measured_in ECOSIMCONCEPT:Husk ! Husk
relationship: measurement_of ECOSIMCONCEPT:PhosphorosCarbonRatio ! PhosphorosCarbonRatio
relationship: qualifier ECOSIMCONCEPT:Husk ! Husk

[Term]
id: ECOSIM:CPLF
name: maximum leaf P:C ratio
def: "The maximum leaf P:C ratio represents the highest ratio of phosphorous (P) to carbon (C) that can be found in a leaf. This metric is critical for understanding the nutrient balance within a plant, as both phosphorous and carbon are vital components of various biological processes." []
is_a: ECOSIM:CATEGORYCanopyStructure ! category - canopy structure
is_a: ECOSIM:CATEGORYPlantPhysiology ! category - plant physiology
relationship: has_unit ECOSIM:gg-1 ! g g-1
relationship: measured_in ECOSIMCONCEPT:Leaf ! Leaf
relationship: measurement_of ECOSIMCONCEPT:PhosphorosCarbonRatio ! PhosphorosCarbonRatio

[Term]
id: ECOSIM:CPND
name: nodule P:C ratio
is_a: ECOSIM:CATEGORYCanopyStructure ! category - canopy structure
relationship: has_unit ECOSIM:gg-1 ! g g-1
relationship: measurement_of ECOSIMCONCEPT:PhosphorosCarbonRatio ! PhosphorosCarbonRatio
relationship: qualifier ECOSIMCONCEPT:Nodule ! Nodule

[Term]
id: ECOSIM:CPO
name: CPO
def: "CPO is a placeholder for a definition." []
is_a: ECOSIM:CATEGORYBiogeochemistry ! category - Biogeochemistry

[Term]
id: ECOSIM:CPO4
name: soil PO4 content
def: "Soil PO4 content refers to the amount of phosphate (PO4) ions present in the soil. Phosphates are a vital nutrient for plant growth and a crucial element of many cell functions in both plants and animals, including energy transfer, photosynthesis, and DNA synthesis. The soil PO4 content can influence the productivity of an ecosystem, and its measure is often used in agricultural practice to determine fertilizer requirements." []
is_a: ECOSIM:CATEGORYBiogeochemistry ! category - Biogeochemistry
relationship: attribute ECOSIMCONCEPT:Content ! Content
relationship: has_unit ECOSIM:mgkg-1 ! mg kg-1
relationship: measured_in ECOSIMCONCEPT:Soil ! Soil
relationship: measurement_of ECOSIMCONCEPT:Phosphate ! Phosphate

[Term]
id: ECOSIM:CPOOL3
name: minimum sink strength for nonstructural C transfer
is_a: ECOSIMCONCEPT:UnclassifiedVariable ! unclassified variable
relationship: has_unit ECOSIM:gd-2 ! g d-2

[Term]
id: ECOSIM:CPOOL4
name: leaf nonstructural C4 content in C4 photosynthesis
def: "Leaf nonstructural C4 content in C4 photosynthesis refers to the amount of nonstructural carbon (C4) present in the leaves of C4 photosynthesizing plants. This can include sugars, starches, and other carbon compounds that are not a part of the plant's structural tissue. It is an important parameter for understanding plant physiology and for modeling photosynthesis and carbon cycling in terrestrial ecosystems." []
is_a: ECOSIM:CATEGORYCanopyPhysiology ! category - Canopy Physiology
is_a: ECOSIM:CATEGORYPlantPhysiology ! category - plant physiology
relationship: attribute ECOSIMCONCEPT:Content ! Content
relationship: context ECOSIMCONCEPT:C4Photosynthesis ! C4Photosynthesis
relationship: has_unit ECOSIM:gd-2 ! g d-2
relationship: measured_in ECOSIMCONCEPT:Leaf ! Leaf
relationship: measurement_of ECOSIMCONCEPT:C4 ! C4

[Term]
id: ECOSIM:CPOQ
name: surface irrigation H2PO4 concentration
def: "Surface irrigation H2PO4 concentration refers to the concentration of the hydrogen phosphate ion (H2PO4-) in the irrigation water used for surface irrigation. H2PO4- is a form of phosphorous available to plants and can affect the nutrient content and pH level of the soil. Monitoring and controlling the H2PO4- concentration in surface irrigation can help optimize plant growth and ensure proper soil health." []
is_a: ECOSIMCONCEPT:UnclassifiedVariable ! unclassified variable
relationship: attribute ECOSIMCONCEPT:Concentration ! Concentration
relationship: context ECOSIMCONCEPT:Irrigation ! Irrigation
relationship: has_unit ECOSIM:gm-3 ! g m-3
relationship: measured_in ECOSIMCONCEPT:Surface ! Surface
relationship: measurement_of ECOSIMCONCEPT:H2PO4 ! Dihydrogen phosphate

[Term]
id: ECOSIM:CPOR
name: precipitation H2PO4 concentration
def: "Precipitation H2PO4 concentration refers to the amount of monohydrogen phosphate (H2PO4-), a type of phosphoric acid, present in a solution resulting from a precipitation event. This can include rain, snow, or any other form of precipitation. This parameter is important to note as it can impact a range of ecological and environmental factors, including soil composition, plant growth, and water quality." []
is_a: ECOSIM:CATEGORYAtmosphericConditions ! category - Atmospheric Conditions
is_a: ECOSIM:CATEGORYDepositionFlux ! category - deposition flux
relationship: attribute ECOSIMCONCEPT:Concentration ! Concentration
relationship: context ECOSIMCONCEPT:Precipitation ! Precipitation
relationship: has_unit ECOSIM:gm-3 ! g m-3
relationship: measured_in ECOSIMCONCEPT:Water ! Water
relationship: measurement_of ECOSIMCONCEPT:H2PO4 ! Dihydrogen phosphate

[Term]
id: ECOSIM:CPRSV
name: reserve P:C ratio
is_a: ECOSIM:CATEGORYCanopyStructure ! category - canopy structure
relationship: has_unit ECOSIM:gg-1 ! g g-1
relationship: measurement_of ECOSIMCONCEPT:PhosphorosCarbonRatio ! PhosphorosCarbonRatio
relationship: qualifier ECOSIMCONCEPT:Reserve ! Reserve

[Term]
id: ECOSIM:CPRT
name: root P:C ratio
is_a: ECOSIM:CATEGORYRootPhysiology ! category - root physiology
relationship: has_unit ECOSIM:gg-1 ! g g-1
relationship: measurement_of ECOSIMCONCEPT:PhosphorosCarbonRatio ! PhosphorosCarbonRatio
relationship: qualifier ECOSIMCONCEPT:Root ! Root

[Term]
id: ECOSIM:CPRTS
name: root P:C ratio x root growth yield
is_a: ECOSIM:CATEGORYRootPhysiology ! category - root physiology
relationship: context ECOSIMCONCEPT:RootGrowthYield ! RootGrowthYield
relationship: measurement_of ECOSIMCONCEPT:PhosphorosCarbonRatio ! PhosphorosCarbonRatio
relationship: qualifier ECOSIMCONCEPT:Root ! Root

[Term]
id: ECOSIM:CPSHE
name: sheath P:C ratio
is_a: ECOSIM:CATEGORYCanopyStructure ! category - canopy structure
relationship: has_unit ECOSIM:gg-1 ! g g-1
relationship: measured_in ECOSIMCONCEPT:Sheath ! Sheath
relationship: measurement_of ECOSIMCONCEPT:PhosphorosCarbonRatio ! PhosphorosCarbonRatio

[Term]
id: ECOSIM:CPSTK
name: stalk P:C ratio
is_a: ECOSIM:CATEGORYCanopyStructure ! category - canopy structure
relationship: has_unit ECOSIM:gg-1 ! g g-1
relationship: measurement_of ECOSIMCONCEPT:PhosphorosCarbonRatio ! PhosphorosCarbonRatio
relationship: qualifier ECOSIMCONCEPT:Stalk ! Stalk

[Term]
id: ECOSIM:CPWS
name: C:P ratio in remobilizable nonstructural biomass
def: "The Carbon to Phosphorus (C:P) ratio in remobilizable non-structural biomass represents the proportion of carbon atoms to phosphorus atoms within the remobilizable non-structural biomass of a plant. This ratio is an important aspect of nutrient cycling within plants and can have implications for plant growth and productivity." []
is_a: ECOSIM:CATEGORYCanopyStructure ! category - canopy structure
relationship: measurement_of ECOSIMCONCEPT:CarbonPhosphorusRatio ! CarbonPhosphorusRatio

[Term]
id: ECOSIM:CSO4
name: soil SO4 content
def: "Soil SO4 content refers to the amount of sulfate (SO4) present in the soil. Sulfate is a form of sulfur, which is a crucial nutrient for plant growth. It plays a key role in protein synthesis and enzyme function in plants. Sulfate is also important for soil health as it contributes to soil fertility." []
is_a: ECOSIM:CATEGORYBiogeochemistry ! category - Biogeochemistry
is_a: ECOSIM:CATEGORYSoilProperty ! category - soil property
relationship: attribute ECOSIMCONCEPT:Content ! Content
relationship: has_unit ECOSIM:mgkg-1 ! mg kg-1
relationship: measured_in ECOSIMCONCEPT:Soil ! Soil
relationship: measurement_of ECOSIMCONCEPT:SO4 ! SO4

[Term]
id: ECOSIM:CSOQ
name: surface irrigation SO4 concentration
def: "Surface irrigation SO4 concentration refers to the concentration of sulfate ions (SO4) in the water used for surface irrigation. Sulfates are a type of sulfur compound that is often present in natural water sources and can affect the pH level and nutrient content of the soil. Monitoring and controlling the SO4 concentration in surface irrigation can help optimize plant growth and ensure proper soil health." []
is_a: ECOSIMCONCEPT:UnclassifiedVariable ! unclassified variable
relationship: attribute ECOSIMCONCEPT:Concentration ! Concentration
relationship: context ECOSIMCONCEPT:Irrigation ! Irrigation
relationship: has_unit ECOSIM:gm-3 ! g m-3
relationship: measured_in ECOSIMCONCEPT:Surface ! Surface
relationship: measurement_of ECOSIMCONCEPT:SO4 ! SO4

[Term]
id: ECOSIM:CSOR
name: precipitation SO4 concentration
def: "Precipitation SO4 concentration refers to the concentration of Sulfate (SO4) in precipitation. Sulfate is a naturally occurring substance that aids in the formation of clouds and increases the reflectivity of the cloud's water droplets, cooling the Earth's surface. This concentration can indicate the presence of air pollution since sulfur dioxide (SO2) is a primary source of SO4 and is released from burning fossil fuels. It can also impact the pH level of soil and water bodies, affecting plant and aquatic life." []
is_a: ECOSIM:CATEGORYAtmosphericConditions ! category - Atmospheric Conditions
is_a: ECOSIM:CATEGORYDepositionFlux ! category - deposition flux
relationship: attribute ECOSIMCONCEPT:Concentration ! Concentration
relationship: context ECOSIMCONCEPT:Precipitation ! Precipitation
relationship: has_unit ECOSIM:gm-3 ! g m-3
relationship: measured_in ECOSIMCONCEPT:Water ! Water
relationship: measurement_of ECOSIMCONCEPT:SO4 ! SO4

[Term]
id: ECOSIM:CSOU
name: subsurface irrigation Cl concentration
is_a: ECOSIMCONCEPT:UnclassifiedVariable ! unclassified variable
relationship: attribute ECOSIMCONCEPT:Concentration ! Concentration
relationship: context ECOSIMCONCEPT:Irrigation ! Irrigation
relationship: has_unit ECOSIM:gm-3 ! g m-3
relationship: measured_in ECOSIMCONCEPT:Subsurface ! Subsurface
relationship: measurement_of ECOSIMCONCEPT:Cl ! Chlorine

[Term]
id: ECOSIM:CSTR
name: solution ion strength
is_a: ECOSIM:CATEGORYSoilSolution ! category - soil solution
relationship: has_unit ECOSIM:molm-3 ! mol m-3
relationship: measured_in ECOSIMCONCEPT:Solution ! Solution
relationship: measurement_of ECOSIMCONCEPT:Ion ! Ion

[Term]
id: ECOSIM:CSTRQ
name: surface irrigation ion strength
def: "Surface irrigation ion strength refers to the strength or concentration of ions in the irrigation water used for surface irrigation. It can impact the nutrient content and pH level of the soil. Monitoring and controlling the ion strength in surface irrigation can help optimize plant growth and ensure proper soil health." []
is_a: ECOSIMCONCEPT:UnclassifiedVariable ! unclassified variable
relationship: context ECOSIMCONCEPT:Irrigation ! Irrigation
relationship: has_unit ECOSIM:gm-3 ! g m-3
relationship: measured_in ECOSIMCONCEPT:Surface ! Surface
relationship: measurement_of ECOSIMCONCEPT:Water ! Water

[Term]
id: ECOSIM:CSTRR
name: surface irrigation ion strength
def: "Surface irrigation ion strength refers to the concentration of dissolved ions in the irrigation water used for surface irrigation. The presence of dissolved ions can influence various soil processes and properties such as soil fertility, structural stability, and water retention capacity. This is a significant parameter for crop nutrition and irrigation water quality." []
is_a: ECOSIMCONCEPT:UnclassifiedVariable ! unclassified variable
relationship: context ECOSIMCONCEPT:Irrigation ! Irrigation
relationship: has_unit ECOSIM:gm-3 ! g m-3
relationship: measured_in ECOSIMCONCEPT:Surface ! Surface
relationship: measurement_of ECOSIMCONCEPT:Ions ! Ions

[Term]
id: ECOSIM:CTC
name: temperature below which seed set is adversely affected
def: "CTC (critical temperature for crop) is the temperature below which the process of seed set in plants is adversely affected, leading to a decreased crop yield. This parameter is critical in agricultural and earth system modeling, as it helps to predict the impacts of climate change on crop productivity." []
is_a: ECOSIM:CATEGORYCanopyPhysiology ! category - Canopy Physiology
is_a: ECOSIM:CATEGORYCanopyStructure ! category - canopy structure
relationship: has_unit ECOSIM:oC ! oC
relationship: measurement_of ECOSIMCONCEPT:Temperature ! temperature

[Term]
id: ECOSIM:CanH2OHeldVg
name: grid canopy held water content
is_a: ECOSIMCONCEPT:UnclassifiedVariable ! unclassified variable
relationship: has_unit ECOSIM:m3d-2 ! m3 d-2

[Term]
id: ECOSIM:CanPBLeafShethC
name: plant branch leaf + sheath C
is_a: ECOSIMCONCEPT:UnclassifiedVariable ! unclassified variable
relationship: has_unit ECOSIM:gd-2 ! g d-2

[Term]
id: ECOSIM:CanPBStalkC
name: branch active stalk C
is_a: ECOSIMCONCEPT:UnclassifiedVariable ! unclassified variable
relationship: has_unit ECOSIM:gd-2 ! g d-2

[Term]
id: ECOSIM:CanPBranchHeight
name: branch height
def: "Branch height refers to the height from the base of the tree to the base of a branch. It provides information about the growth habit of the tree and is used to understand forest structure. It is also important for understanding both aboveground and belowground carbon dynamics." []
is_a: ECOSIM:CATEGORYCanopyStructure ! category - canopy structure
relationship: attribute ECOSIMCONCEPT:Height ! Height
relationship: has_unit ECOSIM:m ! m
relationship: measured_in ECOSIMCONCEPT:Branch ! Branch

[Term]
id: ECOSIM:CanPCi2CaRatio
name: Ci:Ca ratio
is_a: ECOSIMCONCEPT:UnclassifiedVariable ! unclassified variable

[Term]
id: ECOSIM:CanPHeight4WatUptake
name: canopy height
is_a: ECOSIM:CATEGORYCanopyStructure ! category - canopy structure
is_a: ECOSIM:CATEGORYPlantPhysiology ! category - plant physiology
relationship: attribute ECOSIMCONCEPT:Height ! Height
relationship: has_unit ECOSIM:m ! m
relationship: measured_in ECOSIMCONCEPT:Canopy ! Canopy

[Term]
id: ECOSIM:CanPLNBLA
name: layer leaf area
def: "Layer leaf area refers to the total surface area of all the leaves in a specific layer of vegetation or canopy. This parameter helps understand the structure and distribution of leaves in a canopy and also plays a crucial role in processes like photosynthesis, transpiration, and the exchange of gases between the vegetation and the atmosphere." []
is_a: ECOSIM:CATEGORYPlantPhysiology ! category - plant physiology
is_a: ECOSIMCONCEPT:UnclassifiedVariable ! unclassified variable
relationship: attribute ECOSIMCONCEPT:Area ! Area
relationship: has_unit ECOSIM:m2d-2 ! m2 d-2
relationship: measured_in ECOSIMCONCEPT:Layer ! Layer
relationship: measurement_of ECOSIMCONCEPT:Leaf ! Leaf

[Term]
id: ECOSIM:CanPSA
name: plant stem area
def: "Plant Stem Area (CanPSA) represents the total area of a plant's stem. The measurement is helpful in understanding the growth rate, biomass, nutrient uptake and overall health of a plant." []
is_a: ECOSIM:CATEGORYCanopyStructure ! category - canopy structure
relationship: attribute ECOSIMCONCEPT:Area ! Area
relationship: has_unit ECOSIM:m2d-2 ! m2 d-2
relationship: measured_in ECOSIMCONCEPT:Plant ! Plant
relationship: measurement_of ECOSIMCONCEPT:Stem ! Stem

[Term]
id: ECOSIM:CanPSheathHeight
name: sheath height
def: "CanPSheathHeight refers to the height of the sheath in canopy plants. The sheath is the part of the plant that encloses the stem, supporting and protecting it. The sheath height is an important factor in plant development and health, and is often measured in agricultural and ecological studies." []
is_a: ECOSIM:CATEGORYCanopyStructure ! category - canopy structure
is_a: ECOSIM:CATEGORYPlantPhysiology ! category - plant physiology
relationship: attribute ECOSIMCONCEPT:Height ! Height
relationship: has_unit ECOSIM:m ! m
relationship: measured_in ECOSIMCONCEPT:CanopyPlant ! CanopyPlant
relationship: measurement_of ECOSIMCONCEPT:Sheath ! Sheath

[Term]
id: ECOSIM:CanPShootElmMass
name: canopy shoot element
is_a: ECOSIM:CATEGORYPlantPhysiology ! category - plant physiology
is_a: ECOSIMCONCEPT:UnclassifiedVariable ! unclassified variable
relationship: attribute ECOSIMCONCEPT:Mass ! Mass
relationship: has_unit ECOSIM:gd-2 ! g d-2
relationship: measured_in ECOSIMCONCEPT:Canopy ! Canopy
relationship: measurement_of ECOSIMCONCEPT:Shoot ! Shoot

[Term]
id: ECOSIM:CanPStalkC
name: canopy active stalk C
is_a: ECOSIMCONCEPT:UnclassifiedVariable ! unclassified variable
relationship: has_unit ECOSIM:gd-2 ! g d-2

[Term]
id: ECOSIM:CanPStomaResistH2O
name: canopy stomatal resistance
is_a: ECOSIM:CATEGORYPlantPhysiology ! category - plant physiology
relationship: has_unit ECOSIM:hm-1 ! h m-1
relationship: measured_in ECOSIMCONCEPT:Canopy ! Canopy
relationship: measurement_of ECOSIMCONCEPT:Stoma ! Stoma
relationship: qualifier ECOSIMCONCEPT:Water ! Water

[Term]
id: ECOSIM:CanPbndlResist
name: canopy boundary layer resistance
is_a: ECOSIM:CATEGORYPlantPhysiology ! category - plant physiology
is_a: ECOSIMCONCEPT:UnclassifiedVariable ! unclassified variable
relationship: has_unit ECOSIM:hm-1 ! h m-1
relationship: measured_in ECOSIMCONCEPT:Canopy ! Canopy
relationship: measurement_of ECOSIMCONCEPT:BoundaryLayerOfCanopy ! BoundaryLayerOfCanopy

[Term]
id: ECOSIM:CanWatP
name: canopy water content associated with dry matter
is_a: ECOSIMCONCEPT:UnclassifiedVariable ! unclassified variable
relationship: has_unit ECOSIM:m3d-2 ! m3 d-2

[Term]
id: ECOSIM:CanWatg
name: total canopy water content stored in dry matter
def: "Total canopy water content stored in dry matter refers to the total amount of water that can be contained within the dry matter of the canopy of a plant or tree. This measurement is important in studying the water cycle of plants as well as understanding the role of plants in the overall water cycle of the ecosystem." []
is_a: ECOSIM:CATEGORYPlantPhysiology ! category - plant physiology
is_a: ECOSIMCONCEPT:UnclassifiedVariable ! unclassified variable
relationship: attribute ECOSIMCONCEPT:Content ! Content
relationship: has_unit ECOSIM:m3d-2 ! m3 d-2
relationship: measured_in ECOSIMCONCEPT:Canopy ! Canopy
relationship: measurement_of ECOSIMCONCEPT:Water ! Water

[Term]
id: ECOSIM:CanopyArea_pft
name: plant canopy leaf+stem/stalk area
def: "Canopy area (pft) refers to the combined leaf and stem/stalk area of vegetation within a specific plant functional type (pft). It represents the total surface area occupied by the above-ground parts of plants, including the leaves and the supporting structures (such as stems or stalks). Canopy area is an essential parameter in earth systems modeling as it affects various processes including light interception, photosynthesis, evapotranspiration, and carbon uptake by plants." []
is_a: ECOSIM:CATEGORYCanopyStructure ! category - canopy structure
is_a: ECOSIM:CATEGORYPlantPhysiology ! category - plant physiology
relationship: has_unit ECOSIM:m2d-2 ! m2 d-2
relationship: measured_in ECOSIMCONCEPT:Canopy ! Canopy
relationship: measurement_of ECOSIMCONCEPT:Area ! Area

[Term]
id: ECOSIM:CanopyBranchLeafA_pft
name: branch leaf area
def: "The 'branch leaf area' refers to the total surface area of leaves present on the branches of a plant within a specific Plant Functional Type (PFT) in a given ecosystem. It is an important parameter in Earth Systems Models (ESMs) as it is used to estimate the primary productivity, energy exchange, and water fluxes associated with plant growth and photosynthesis. The branch leaf area can vary between different PFTs and is influenced by factors such as vegetation type, climate conditions, and nutrient availability." []
is_a: ECOSIM:CATEGORYCanopyStructure ! category - canopy structure
is_a: ECOSIM:CATEGORYPlantPhysiology ! category - plant physiology
relationship: attribute ECOSIMCONCEPT:Area ! Area
relationship: context ECOSIMCONCEPT:Canopy ! Canopy
relationship: has_unit ECOSIM:m2d-2 ! m2 d-2
relationship: measured_in ECOSIMCONCEPT:Branch ! Branch
relationship: measurement_of ECOSIMCONCEPT:Leaf ! Leaf

[Term]
id: ECOSIM:CanopyBranchStemApft_lyr
name: stem layer area
def: "Stem layer area refers to the total surface area of tree stems within a canopy branch in a specific land ecosystem. It is an important parameter in Earth system models as it provides insights into the energy and carbon exchange processes occurring within the ecosystem." []
is_a: ECOSIM:CATEGORYCanopyStructure ! category - canopy structure
relationship: attribute ECOSIMCONCEPT:Area ! Area
relationship: has_unit ECOSIM:m2d-2 ! m2 d-2
relationship: measured_in ECOSIMCONCEPT:CanopyBranch ! CanopyBranch
relationship: measurement_of ECOSIMCONCEPT:Stem ! Stem

[Term]
id: ECOSIM:CanopyHeight
name: canopy height
is_a: ECOSIM:CATEGORYCanopyStructure ! category - canopy structure
relationship: attribute ECOSIMCONCEPT:Height ! Height
relationship: has_unit ECOSIM:m ! m
relationship: measured_in ECOSIMCONCEPT:Canopy ! Canopy

[Term]
id: ECOSIM:CanopyHeightz
name: canopy layer height
is_a: ECOSIM:CATEGORYCanopyStructure ! category - canopy structure
relationship: attribute ECOSIMCONCEPT:Height ! Height
relationship: has_unit ECOSIM:m ! m
relationship: measured_in ECOSIMCONCEPT:CanopyLayer ! CanopyLayer

[Term]
id: ECOSIM:CanopyLA_grd
name: grid level plant canopy leaf area
def: "CanopyLA_grd refers to the quantity of plant canopy leaf area at the grid level in Earth system models. It represents the total surface area of leaves present in the plant canopy within a specific grid cell. Canopy leaf area is an important parameter for understanding carbon dioxide exchange, water vapor fluxes, and energy balance between the land surface and the atmosphere. It is typically measured in square meters per square meter (m²/m²) and is used to estimate primary productivity, evapotranspiration, and the overall functioning of terrestrial ecosystems." []
is_a: ECOSIM:CATEGORYCanopyStructure ! category - canopy structure
is_a: ECOSIM:CATEGORYPlantPhysiology ! category - plant physiology
relationship: attribute ECOSIMCONCEPT:Area ! Area
relationship: context ECOSIMCONCEPT:Canopy ! Canopy
relationship: has_unit ECOSIM:m2d-2 ! m2 d-2
relationship: measured_in ECOSIMCONCEPT:GridCell ! GridCell
relationship: measurement_of ECOSIMCONCEPT:Leaf ! Leaf

[Term]
id: ECOSIM:CanopyLAgrid_lyr
name: total leaf area
def: "Total leaf area refers to the sum of the areas of all the leaves within a given grid layer of a canopy. It is an important parameter in earth systems modeling as it helps determine the efficiency of photosynthesis, the exchange of gases (such as carbon dioxide and oxygen) between plants and the atmosphere, and the overall energy balance within the ecosystem. The total leaf area is typically quantified using remote sensing techniques or by directly measuring the individual leaf areas and summing them up." []
is_a: ECOSIM:CATEGORYCanopyStructure ! category - canopy structure
is_a: ECOSIM:CATEGORYPlantPhysiology ! category - plant physiology
relationship: attribute ECOSIMCONCEPT:Area ! Area
relationship: has_unit ECOSIM:m2d-2 ! m2 d-2
relationship: measured_in ECOSIMCONCEPT:Canopy ! Canopy
relationship: measured_in ECOSIMCONCEPT:GridLayer ! GridLayer
relationship: measurement_of ECOSIMCONCEPT:Leaf ! Leaf

[Term]
id: ECOSIM:CanopyLeafA_pft
name: plant leaf area
def: "CanopyLeafA_pft refers to the leaf area of plants within a given land cover patch or plant functional type (PFT) in an Earth system model. Leaf area is a measure of the total surface area of leaves per unit ground area. It is an important parameter in modeling processes such as photosynthesis, transpiration, and energy exchange between the vegetation and the atmosphere. The CanopyLeafA_pft parameter is used to represent the spatial distribution and variability of leaf area across different PFTs, which is crucial for accurately simulating land surface processes and their interactions with the climate system." []
is_a: ECOSIM:CATEGORYCanopyStructure ! category - canopy structure
is_a: ECOSIM:CATEGORYPlantPhysiology ! category - plant physiology
relationship: attribute ECOSIMCONCEPT:Area ! Area
relationship: has_unit ECOSIM:m2d-2 ! m2 d-2
relationship: measurement_of ECOSIMCONCEPT:Leaf ! Leaf
relationship: qualifier ECOSIMCONCEPT:Canopy ! Canopy

[Term]
id: ECOSIM:CanopyLeafApft_lyr
name: canopy layer leaf area
def: "Canopy layer leaf area refers to the total surface area covered by leaves within a specific layer of the vegetation canopy. This parameter is important in earth systems modeling as it plays a crucial role in regulating the exchange of energy, water, and carbon dioxide between the vegetation and the atmosphere. The canopy layer leaf area parameter is often used to estimate the overall photosynthetic capacity and productivity of vegetation, as well as to model the interception and absorption of solar radiation within the canopy." []
is_a: ECOSIM:CATEGORYPlantPhysiology ! category - plant physiology
is_a: ECOSIMCONCEPT:UnclassifiedVariable ! unclassified variable
relationship: attribute ECOSIMCONCEPT:Area ! Area
relationship: has_unit ECOSIM:m2d-2 ! m2 d-2
relationship: measured_in ECOSIMCONCEPT:CanopyLayer ! CanopyLayer
relationship: measurement_of ECOSIMCONCEPT:Leaf ! Leaf

[Term]
id: ECOSIM:CanopyLeafCpft_lyr
name: canopy layer leaf C
def: "Canopy layer leaf C (CanopyLeafCpft_lyr) refers to the amount of carbon stored in the leaves of vegetation within a specific layer of the canopy in an Earth System Model. It represents the total mass of carbon in the leaves, including both living and dead biomass. Canopy layer leaf C is an important parameter for calculating the carbon balance and productivity of vegetation in a given ecosystem, and it is influenced by factors such as photosynthesis, respiration, and allocation of carbon to different plant organs." []
is_a: ECOSIM:CATEGORYPlantPhysiology ! category - plant physiology
is_a: ECOSIMCONCEPT:UnclassifiedVariable ! unclassified variable
relationship: attribute ECOSIMCONCEPT:Carbon ! Carbon
relationship: has_unit ECOSIM:gd-2 ! g d-2
relationship: measured_in ECOSIMCONCEPT:Canopy ! Canopy
relationship: measurement_of ECOSIMCONCEPT:Leaf ! Leaf

[Term]
id: ECOSIM:CanopyLeafShethC_pft
name: plant canopy leaf + sheath C
def: "CanopyLeafShethC_pft refers to the parameter that represents the amount of carbon contained in both the leaves and sheaths of plants in a canopy. This parameter is used in Earth system models to simulate the cycling of carbon within vegetation and its impact on the global carbon balance." []
is_a: ECOSIM:CATEGORYPlantPhysiology ! category - plant physiology
is_a: ECOSIMCONCEPT:UnclassifiedVariable ! unclassified variable
relationship: has_unit ECOSIM:gCd-2 ! gC d-2
relationship: measured_in ECOSIMCONCEPT:Canopy ! Canopy
relationship: measured_in ECOSIMCONCEPT:LeafPlusSheath ! LeafPlusSheath
relationship: measurement_of ECOSIMCONCEPT:Carbon ! Carbon

[Term]
id: ECOSIM:CanopyNonstructElementConc_pft
name: canopy nonstructural element concentration
def: "Canopy nonstructural element concentration refers to the amount of nonstructural elements within the canopy of a vegetation patch, expressed as a concentration. Nonstructural elements include compounds such as sugars, starches, and other organic molecules that are stored within plant tissues and are not part of the structural components of the plant. This parameter is important in earth systems modeling as it influences various processes such as carbon allocation, resource utilization, and plant growth." []
is_a: ECOSIMCONCEPT:UnclassifiedVariable ! unclassified variable
relationship: has_unit ECOSIM:gd-2 ! g d-2

[Term]
id: ECOSIM:CanopyNonstructElements_pft
name: canopy nonstructural element
def: "A canopy nonstructural element refers to any component or feature within a vegetation canopy that is not primarily responsible for providing structural support. These nonstructural elements can include various characteristics such as flowers, fruits, leaves, and other reproductive or physiological features of plants. These elements are important for modeling Earth systems as they play a significant role in influencing processes such as carbon assimilation, resource allocation, and overall ecosystem dynamics." []
is_a: ECOSIM:CATEGORYPlantPhysiology ! category - plant physiology
is_a: ECOSIMCONCEPT:UnclassifiedVariable ! unclassified variable
relationship: has_unit ECOSIM:gd-2 ! g d-2
relationship: measured_in ECOSIMCONCEPT:Canopy ! Canopy
relationship: measurement_of ECOSIMCONCEPT:NonStructuralElement ! Non-structural element

[Term]
id: ECOSIM:CanopyPARabsorpty_pft
name: canopy PAR absorptivity
def: "Canopy PAR absorptivity refers to the parameter that quantifies the fraction of photosynthetically active radiation (PAR) incident on the vegetation canopy that is absorbed by the plants. It represents the efficiency of the canopy in absorbing PAR for photosynthesis and is typically expressed as a dimensionless value between 0 and 1. A higher value indicates a higher capacity of the canopy to absorb PAR and convert it into energy for plant growth and development." []
is_a: ECOSIM:CATEGORYPlantPhysiology ! category - plant physiology
relationship: measured_in ECOSIMCONCEPT:Canopy ! Canopy
relationship: measurement_of ECOSIMCONCEPT:PhotosyntheticallyActiveRadiation ! PhotosyntheticallyActiveRadiation

[Term]
id: ECOSIM:CanopyPARalbedo_pft
name: canopy PAR albedo
def: "Canopy PAR albedo (Photosynthetically Active Radiation albedo) of a specific plant functional type (pft) in Earth system modeling refers to the fraction of the incoming PAR that is reflected by the canopy of a vegetation type. It is a parameter that quantifies the amount of light reflected by the canopy, which affects the energy balance and radiation budget of the Earth's surface. Canopy PAR albedo is influenced by various factors such as leaf angle distribution, leaf optical properties, and the presence of other canopy elements like branches and stems." []
is_a: ECOSIM:CATEGORYPlantPhysiology ! category - plant physiology
relationship: measured_in ECOSIMCONCEPT:Canopy ! Canopy
relationship: measurement_of ECOSIMCONCEPT:PhotosyntheticallyActiveRadiation ! PhotosyntheticallyActiveRadiation

[Term]
id: ECOSIM:CanopySWAlbedo_pft
name: canopy shortwave albedo
def: "Canopy shortwave albedo refers to the fraction of shortwave radiation, specifically in the solar spectrum, that is reflected by the vegetation canopy. It is a parameter used in earth system models to quantify the amount of incoming solar radiation that is reflected back to the atmosphere by the vegetation canopy. Canopy shortwave albedo depends on various factors, including the characteristics of the vegetation, such as leaf structure and pigmentation, as well as the solar zenith angle and atmospheric conditions." []
is_a: ECOSIM:CATEGORYPlantPhysiology ! category - plant physiology
is_a: ECOSIMCONCEPT:UnclassifiedVariable ! unclassified variable
relationship: measured_in ECOSIMCONCEPT:Canopy ! Canopy
relationship: measurement_of ECOSIMCONCEPT:ShortwaveRadiation ! ShortwaveRadiation

[Term]
id: ECOSIM:CanopySWabsorpty_pft
name: canopy shortwave absorptivity
def: "Canopy shortwave absorptivity refers to the fraction of shortwave radiation absorbed by the vegetation canopy. It represents the ability of the canopy to capture and convert incoming solar radiation into heat and energy, contributing to the overall energy balance and productivity of the ecosystem. Canopy shortwave absorptivity is an important parameter in earth systems modeling that influences the distribution of energy within the system and can affect processes such as photosynthesis, evapotranspiration, and surface temperature." []
is_a: ECOSIM:CATEGORYPlantPhysiology ! category - plant physiology
relationship: measured_in ECOSIMCONCEPT:Canopy ! Canopy
relationship: measurement_of ECOSIMCONCEPT:ShortwaveRadiation ! ShortwaveRadiation

[Term]
id: ECOSIM:CanopyStemA_lyr
name: total stem area
def: "The term 'total stem area' refers to the combined surface area of all stems and branches within a defined unit area of a forest canopy. It represents the overall area available for photosynthesis, gas exchange, and transpiration by the plants in the canopy. The total stem area is an important parameter in earth systems modeling as it influences various ecosystem processes such as carbon assimilation, water cycle, and energy balance. Additionally, it can be used to estimate important plant properties like biomass and productivity." []
is_a: ECOSIM:CATEGORYCanopyStructure ! category - canopy structure
relationship: has_unit ECOSIM:m2d-2 ! m2 d-2

[Term]
id: ECOSIM:CanopyStemApft_lyr
name: plant canopy layer stem area
def: "Plant canopy layer stem area refers to the total cross-sectional area of plant stems within a specific vertical layer of the canopy. It represents the surface area available for water and nutrient uptake, as well as the mechanical support for the aboveground biomass in that particular layer of the plant canopy." []
is_a: ECOSIMCONCEPT:UnclassifiedVariable ! unclassified variable
relationship: has_unit ECOSIM:m2d-2 ! m2 d-2

[Term]
id: ECOSIM:ClumpFactor
name: clumping factor for self-shading in canopy layer
def: "The clumping factor for self-shading in a canopy layer refers to a variable used in plant canopy models. It measures the degree to which foliage is clumped together rather than being evenly distributed, affecting how much light penetrates the canopy. This in turn can influence photosynthesis rates and other physiological processes." []
is_a: ECOSIM:CATEGORYCanopyStructure ! category - canopy structure
is_a: ECOSIM:CATEGORYPlantPhysiology ! category - plant physiology
relationship: context ECOSIMCONCEPT:Clumping ! Clumping
relationship: measured_in ECOSIMCONCEPT:Canopy ! Canopy
relationship: measurement_of ECOSIMCONCEPT:SelfShading ! SelfShading

[Term]
id: ECOSIM:ClumpFactort
name: clumping factor for self-shading in canopy layer at current LAI
is_a: ECOSIM:CATEGORYCanopyStructure ! category - canopy structure

[Term]
id: ECOSIM:ClumpFactort0
name: initial clumping factor for self-shading in canopy layer
is_a: ECOSIM:CATEGORYCanopyStructure ! category - canopy structure

[Term]
id: ECOSIM:DCO2
name: gaesous CO2 concentration difference across stomates
is_a: ECOSIM:CATEGORYCanopyPhysiology ! category - Canopy Physiology
is_a: ECOSIM:CATEGORYPlantPhysiology ! category - plant physiology
relationship: has_unit ECOSIM:umolm-3 ! umol m-3
relationship: measurement_of ECOSIMCONCEPT:CO2 ! Carbon dioxide

[Term]
id: ECOSIM:DCORP
name: soil mixing fraction with tillage
def: "Soil mixing fraction with tillage refers to the proportion of the soil that is mixed or disturbed during the process of tillage. Tillage is the agricultural process of preparing the soil for planting by mechanical agitation, which can include plowing, turning, stirring, and harrowing. Knowledge of the soil mixing fraction is important for understanding soil structure, nutrient availability, and seedbed preparation." []
is_a: ECOSIMCONCEPT:UnclassifiedVariable ! unclassified variable
relationship: attribute ECOSIMCONCEPT:Fraction ! Fraction
relationship: measured_in ECOSIMCONCEPT:Soil ! Soil

[Term]
id: ECOSIM:DFGS
name: coefficient for dissolution - volatilization
def: "Coefficient for dissolution - volatilization represents the proportional rate at which a soluble compound dissolves into a solvent or volatilizes into the air. The rate can be influenced by temperature, surface area, the nature of the solvent and solute, and other factors. This parameter is used in modeling to understand the fate and transport of chemicals in various environmental compartments." []
is_a: ECOSIMCONCEPT:UnclassifiedVariable ! unclassified variable
relationship: context ECOSIMCONCEPT:Dissolution ! Dissolution
relationship: context ECOSIMCONCEPT:Volatilization ! Volatilization
relationship: measurement_of ECOSIMCONCEPT:Coefficient ! Coefficient

[Term]
id: ECOSIM:DGSTGF
name: gain in normalized node number during reproductive growth stages
def: "The Gain in normalized node number during reproductive growth stages refers to the increase in the relative number of nodes in a plant during its reproductive growth phase. This parameter is essential for understanding plant growth and productivity as nodes are key sites for leaf and flower formation." []
is_a: ECOSIM:CATEGORYCanopyStructure ! category - canopy structure
relationship: has_unit ECOSIM:h-1 ! h-1
relationship: measured_in ECOSIMCONCEPT:Plant ! Plant
relationship: measurement_of ECOSIMCONCEPT:Node ! Node

[Term]
id: ECOSIM:DGSTGI
name: gain in normalized node number during vegetative growth stages
def: "Gain in normalized node number during vegetative growth stages refers to the increase in the number of nodes or branching points in a plant during the vegetative phase of its growth cycle, normalized to standard growth conditions. This is a parameter used in earth systems modeling to understand and simulate plant growth and development." []
is_a: ECOSIM:CATEGORYCanopyStructure ! category - canopy structure
relationship: has_unit ECOSIM:h-1 ! h-1
relationship: measured_in ECOSIMCONCEPT:Plant ! Plant

[Term]
id: ECOSIM:DH
name: number of EW grid cells
def: "Number of EW grid cells is a parameter used to specify the number of grid cells present in east-west (EW) direction in a spatially explicit model or a geographic information system (GIS). It provides information about the spatial resolution of the grid used for the model or the GIS and is useful for understanding the geographical coverage and distribution of the data being used." []
is_a: ECOSIMCONCEPT:UnclassifiedVariable ! unclassified variable
relationship: measurement_of ECOSIMCONCEPT:GridCell ! GridCell

[Term]
id: ECOSIM:DIRRA
name: depth to which automatic irrigation applied
def: "The depth to which automatic irrigation is applied refers to the depth of water that is delivered to the plant's root zone when the automatic irrigation system is triggered. The determination of this depth is crucial to ensure that the sufficient amount of water is supplied to meet the plant's water needs and minimize water wastage." []
is_a: ECOSIMCONCEPT:UnclassifiedVariable ! unclassified variable
relationship: attribute ECOSIMCONCEPT:Depth ! Depth
relationship: has_unit ECOSIM:m ! m
relationship: measured_in ECOSIMCONCEPT:Soil ! Soil

[Term]
id: ECOSIM:DMEAR
name: ear growth yield
def: "Ear growth yield refers to the rate at which the ear size or the ear weight of a crop plant, like maize or corn, increases over time. The rate is typically measured g d-1 (grams per day) or a similar unit. It is a crucial measurement for understanding total crop growth and potential yield." []
is_a: ECOSIM:CATEGORYCanopyStructure ! category - canopy structure
is_a: ECOSIM:CATEGORYPlantPhysiology ! category - plant physiology
is_a: ECOSIM:CATEGORYPlantPopulation ! category - Plant Population
relationship: attribute ECOSIMCONCEPT:Growth ! Growth
relationship: has_unit ECOSIM:gg-1 ! g g-1
relationship: measured_in ECOSIMCONCEPT:Ear ! Ear

[Term]
id: ECOSIM:DMGR
name: grain growth yield
def: "Grain growth yield, represented by the parameter DMGR, refers to the yield of grain growing in a defined area, typically measured in units like kilograms per hectare. It is a key parameter in crop modeling studies focused on understanding agricultural productivity under different climatic and soil conditions. It could be influenced by factors such as irrigation, nutrient availability, pest and disease threats, and variety of the crop." []
is_a: ECOSIM:CATEGORYCanopyStructure ! category - canopy structure
is_a: ECOSIM:CATEGORYPlantPopulation ! category - Plant Population
relationship: has_unit ECOSIM:gg-1 ! g g-1
relationship: measured_in ECOSIMCONCEPT:Field ! Field
relationship: measurement_of ECOSIMCONCEPT:GrainGrowth ! GrainGrowth
relationship: qualifier ECOSIMCONCEPT:Area ! Area

[Term]
id: ECOSIM:DMHSK
name: husk growth yield
is_a: ECOSIM:CATEGORYCanopyStructure ! category - canopy structure
is_a: ECOSIM:CATEGORYPlantPopulation ! category - Plant Population
relationship: context ECOSIMCONCEPT:Husk ! Husk
relationship: has_unit ECOSIM:gg-1 ! g g-1
relationship: measurement_of ECOSIMCONCEPT:Growth ! Growth

[Term]
id: ECOSIM:DMLF
name: leaf growth yield
def: "Leaf growth yield refers to the rate at which new leaves are formed in a plant over a certain period of time. This measurement can help in understanding the plant's growth rate, health, and productivity." []
is_a: ECOSIM:CATEGORYCanopyStructure ! category - canopy structure
is_a: ECOSIM:CATEGORYPlantPopulation ! category - Plant Population
relationship: context ECOSIMCONCEPT:Growth ! Growth
relationship: has_unit ECOSIM:gg-1 ! g g-1
relationship: measured_in ECOSIMCONCEPT:Leaf ! Leaf

[Term]
id: ECOSIM:DMND
name: nodule growth yield
def: "Nodule growth yield refers to the increase in mass or size of a nodule per unit of time. Nodules are formed on the roots of plants, particularly legumes, in a symbiotic relationship with nitrogen-fixing bacteria. Through this symbiotic relationship, these nodules play an essential role in plant nutrition and soil fertility by converting atmospheric nitrogen into a form that can be used by plants. This parameter is crucial in understanding plant growth and productivity, particularly in agricultural systems." []
is_a: ECOSIM:CATEGORYCanopyStructure ! category - canopy structure
is_a: ECOSIM:CATEGORYPlantPhysiology ! category - plant physiology
is_a: ECOSIM:CATEGORYPlantPopulation ! category - Plant Population
relationship: has_unit ECOSIM:gg-1 ! g g-1
relationship: measured_in ECOSIMCONCEPT:Nodule ! Nodule
relationship: measurement_of ECOSIMCONCEPT:Growth ! Growth

[Term]
id: ECOSIM:DMRSV
name: reserve growth yield
is_a: ECOSIM:CATEGORYCanopyStructure ! category - canopy structure
is_a: ECOSIM:CATEGORYPlantPopulation ! category - Plant Population
relationship: context ECOSIMCONCEPT:Reserve ! Reserve
relationship: has_unit ECOSIM:gg-1 ! g g-1
relationship: qualifier ECOSIMCONCEPT:Growth ! Growth

[Term]
id: ECOSIM:DMSHE
name: sheath growth yield
def: "Sheath growth yield refers to the increase in the size or mass of the plant's sheath over a certain period of time. The measure provides useful information about a plant's health, growth rate, and overall productivity." []
is_a: ECOSIM:CATEGORYCanopyStructure ! category - canopy structure
is_a: ECOSIM:CATEGORYPlantPopulation ! category - Plant Population
relationship: has_unit ECOSIM:gg-1 ! g g-1
relationship: measured_in ECOSIMCONCEPT:Sheath ! Sheath
relationship: measurement_of ECOSIMCONCEPT:Growth ! Growth

[Term]
id: ECOSIM:DMSTK
name: stalk growth yield
def: "Stalk growth yield refers to the amount of new plant stalk material (by weight) produced per unit of solar energy captured and used by the plant. It's an important measure in crop modeling that helps to understand the efficiency of energy use in plants." []
is_a: ECOSIM:CATEGORYCanopyStructure ! category - canopy structure
is_a: ECOSIM:CATEGORYPlantPhysiology ! category - plant physiology
is_a: ECOSIM:CATEGORYPlantPopulation ! category - Plant Population
relationship: has_unit ECOSIM:gg-1 ! g g-1
relationship: measured_in ECOSIMCONCEPT:Plants ! Plants

[Term]
id: ECOSIM:DMVL
name: root volume:mass ratio
def: "Root volume:mass ratio (DMVL) is a measure of the volume and mass of plant roots. It provides insights into the root system architecture, root density, and the overall growth and health of plants. This ratio can vary widely among different plant species and can be influenced by various environmental factors such as soil type, nutrient availability, and water content." []
is_a: ECOSIM:CATEGORYPlantPhysiology ! category - plant physiology
is_a: ECOSIM:CATEGORYRootPhysiology ! category - root physiology
relationship: has_unit ECOSIM:m3g-1 ! m3 g-1
relationship: measured_in ECOSIMCONCEPT:Root ! Root

[Term]
id: ECOSIM:DPNH4
name: total depth of NH4 band
def: "Total depth of NH4 band refers to the total depth through which ammonium (NH4) is distributed or contained within a certain band or layer of soil or sediment. This measure provides insight on the vertical distribution of NH4 in soil which is critical in understanding nutrient cycling and availability for plant growth." []
is_a: ECOSIMCONCEPT:UnclassifiedVariable ! unclassified variable
relationship: attribute ECOSIMCONCEPT:Depth ! Depth
relationship: has_unit ECOSIM:m ! m
relationship: measured_in ECOSIMCONCEPT:SoilBand ! SoilBand
relationship: measurement_of ECOSIMCONCEPT:NH4 ! Ammonium

[Term]
id: ECOSIM:DPNHB
name: depth of NH4 band
def: "Depth of NH4 band refers to the depth in the soil at which a band or layer of ammonium (NH4) fertilizer is located. This is an important parameter in agriculture and soil science as it can affect the availability of nutrients to plants." []
is_a: ECOSIMCONCEPT:UnclassifiedVariable ! unclassified variable
relationship: attribute ECOSIMCONCEPT:Depth ! Depth
relationship: context ECOSIMCONCEPT:Band ! Band
relationship: has_unit ECOSIM:m ! m
relationship: measured_in ECOSIMCONCEPT:Soil ! Soil
relationship: measurement_of ECOSIMCONCEPT:NH4 ! Ammonium

[Term]
id: ECOSIM:DPNO3
name: total depth of NO3 band
def: "Total depth of NO3 band refers to the vertical thickness or depth of a layer or band of soil where nitrate (NO3) is concentrated or prominent. This measure can contribute to understanding nutrient cycling, soil fertility, and groundwater quality, as NO3 is a key nutrient but can also be a pollutant when it leaches into water bodies." []
is_a: ECOSIMCONCEPT:UnclassifiedVariable ! unclassified variable
relationship: attribute ECOSIMCONCEPT:Depth ! Depth
relationship: has_unit ECOSIM:m ! m
relationship: measurement_of ECOSIMCONCEPT:Nitrate ! Nitrate

[Term]
id: ECOSIM:DPNOB
name: depth of NO4 band
def: "Depth of NO4 band refers to the vertical distance from the surface of the soil to the band or layer of soil where nitrate (NO4) is concentrated or present in significant amounts. This depth can be important in understanding nutrient availability and movement in soils, as well as potential risks of nutrient leaching and groundwater contamination." []
is_a: ECOSIMCONCEPT:UnclassifiedVariable ! unclassified variable
relationship: attribute ECOSIMCONCEPT:Depth ! Depth
relationship: has_unit ECOSIM:m ! m
relationship: measured_in ECOSIMCONCEPT:Soil ! Soil
relationship: measurement_of ECOSIMCONCEPT:Band ! Band

[Term]
id: ECOSIM:DPPO4
name: total depth of PO4 band
is_a: ECOSIMCONCEPT:UnclassifiedVariable ! unclassified variable
relationship: has_unit ECOSIM:m ! m

[Term]
id: ECOSIM:DPPOB
name: depth of PO4 band
def: "Depth of PO4 band refers to the vertical distance from the surface to a layer in the soil where Phosphate (PO4) is most concentrated. This depth is a crucial parameter for agricultural practices as it helps in understanding the mobility and availability of the nutrient in the soil." []
is_a: ECOSIMCONCEPT:UnclassifiedVariable ! unclassified variable
relationship: context ECOSIMCONCEPT:PO4 ! Phosphate
relationship: has_unit ECOSIM:m ! m
relationship: measured_in ECOSIMCONCEPT:Soil ! Soil
relationship: measurement_of ECOSIMCONCEPT:Depth ! Depth

[Term]
id: ECOSIM:DTBLI
name: external water table depth
is_a: ECOSIM:CATEGORYHydrology ! category - Hydrology
relationship: attribute ECOSIMCONCEPT:Depth ! Depth
relationship: has_unit ECOSIM:m ! m
relationship: measurement_of ECOSIMCONCEPT:WaterTable ! WaterTable

[Term]
id: ECOSIM:DTBLY
name: artificial water table depth
def: "Artificial water table depth refers to the depth at which the water table is artificially maintained through human intervention, often for purposes such as irrigation, drainage, or preventing land subsidence. This is typically done in areas where natural water table levels are unsuitable for the intended land use." []
is_a: ECOSIM:CATEGORYHydrology ! category - Hydrology
relationship: attribute ECOSIMCONCEPT:Depth ! Depth
relationship: has_unit ECOSIM:m ! m
relationship: measurement_of ECOSIMCONCEPT:WaterTable ! WaterTable

[Term]
id: ECOSIM:DTKC
name: change in canopy temperature
def: "Change in canopy temperature refers to the variation in the temperature of the plant canopy over a particular period of time. It is an important metric in agronomy and plant physiology as it directly affects multiple processes such as photosynthesis, respiration, transpiration, and plant microclimate. Factors such as weather conditions, solar radiation, wind speed, and plant water status can significantly impact the canopy temperature." []
is_a: ECOSIM:CATEGORYPlantPhysiology ! category - plant physiology
is_a: ECOSIMCONCEPT:UnclassifiedVariable ! unclassified variable
relationship: has_unit ECOSIM:K ! K
relationship: measured_in ECOSIMCONCEPT:Canopy ! Canopy

[Term]
id: ECOSIM:DV
name: number of EW grid cells
def: "Number of EW grid cells refers to the count of grid cells along the east-west direction in a spatially explicit model or digital representation of a geographic area. This parameter is crucial for defining spatial resolution and mapping variables across a study area. Typically, these cells form the basic units for spatially explicit modeling, simulation, and analysis tasks." []
is_a: ECOSIMCONCEPT:UnclassifiedVariable ! unclassified variable
relationship: measurement_of ECOSIMCONCEPT:GridCell ! GridCell

[Term]
id: ECOSIM:DYLM
name: maximum daylength
def: "Maximum daylength refers to the longest duration of daylight that occurs in a 24-hour period, typically on the summer solstice." []
is_a: ECOSIM:CATEGORYAtmosphericConditions ! category - Atmospheric Conditions
relationship: has_unit ECOSIM:h ! h

[Term]
id: ECOSIM:DYLN
name: daylength
def: "Daylength refers to the duration of time that the sun is above the horizon in a single day. This number varies throughout the year and by geographical location. It has significant effects on the behavior and physiological functions of many organisms, including plants and humans." []
is_a: ECOSIM:CATEGORYAtmosphericConditions ! category - Atmospheric Conditions
relationship: attribute ECOSIMCONCEPT:Duration ! Duration
relationship: has_unit ECOSIM:h ! h
relationship: measurement_of ECOSIMCONCEPT:Day ! Day
relationship: qualifier ECOSIMCONCEPT:Day ! Day

[Term]
id: ECOSIM:DYLX
name: daylength of previous day
is_a: ECOSIM:CATEGORYAtmosphericConditions ! category - Atmospheric Conditions
relationship: has_unit ECOSIM:h ! h
relationship: measured_in ECOSIMCONCEPT:Day ! Day

[Term]
id: ECOSIM:DepthInternalWTBL
name: internal water table depth
is_a: ECOSIMCONCEPT:UnclassifiedVariable ! unclassified variable
relationship: has_unit ECOSIM:m ! m

[Term]
id: ECOSIM:DrySnoFlxBySnowRedistributM
name: runoff snow flux
is_a: ECOSIM:CATEGORYSnowpack ! category - Snowpack
relationship: has_unit ECOSIM:m3d-2t-1 ! m3 d-2 t-1

[Term]
id: ECOSIM:DrysnoBySnowRedistribution
name: snowpack runoff snow
is_a: ECOSIMCONCEPT:UnclassifiedVariable ! unclassified variable
relationship: has_unit ECOSIM:m3d-2h-1 ! m3 d-2 h-1

[Term]
id: ECOSIM:ECND
name: electrical conductivity
def: "Electrical conductivity (ECND) is a measure of a material's ability to conduct an electric current. In the context of soil science, electrical conductivity is used as a proxy for determining the salinity of the soil, which can affect plant growth and productivity." []
is_a: ECOSIM:CATEGORYSoilProperty ! category - soil property
is_a: ECOSIM:CATEGORYSoilSolution ! category - soil solution
relationship: has_unit ECOSIM:dSm-1 ! dS m-1
relationship: measured_in ECOSIMCONCEPT:Soil ! Soil

[Term]
id: ECOSIM:EHUM
name: partitioning coefficient between humus and microbial residue
def: "Partitioning coefficient between humus and microbial residue (EHUM) determines the proportion of carbon matter that is allocated between humus and the residues of microbes. It plays a crucial role in understanding the carbon cycle and its stability in ecosystems, particularly in soils where microbial residues represent a considerable fraction of stable organic matter." []
is_a: ECOSIM:CATEGORYMicrobialActivity ! category - microbial activity
relationship: measurement_of ECOSIMCONCEPT:Humus ! Humus

[Term]
id: ECOSIM:EHVST
name: harvest efficiency
def: "Harvest efficiency refers to the proportion of yield that is successfully harvested from the total available crop. It is a crucial parameter in agricultural systems modelling, influencing yield predictions and management strategies." []
is_a: ECOSIMCONCEPT:UnclassifiedVariable ! unclassified variable
relationship: measurement_of ECOSIMCONCEPT:Harvest ! Harvest

[Term]
id: ECOSIM:ENGYX
name: canopy heat storage from previous time step
def: "Canopy heat storage from previous time step relates to the quantity of heat energy stored in the canopy of a particular plant or vegetation cover from the previous time interval. It is an important parameter to calculate energy balance in the landscape ecosystem." []
is_a: ECOSIMCONCEPT:UnclassifiedVariable ! unclassified variable
relationship: attribute ECOSIMCONCEPT:Energy ! Energy
relationship: has_unit ECOSIM:MJd-2 ! MJ d-2
relationship: measured_in ECOSIMCONCEPT:Canopy ! Canopy
relationship: measurement_of ECOSIMCONCEPT:Heat ! Heat

[Term]
id: ECOSIM:EPOC
name: partitioning coefficient between POC and litter
def: "Partitioning coefficient between Particulate Organic Carbon (POC) and litter refers to the equilibrium ratio of the concentration of a chemical species in POC to the equilibrium concentration of the same species in litter. This coefficient is significant in the process of understanding the distribution and movement of nutrients in different organic matter compartments within an ecosystem." []
is_a: ECOSIM:CATEGORYMicrobialActivity ! category - microbial activity
relationship: attribute ECOSIMCONCEPT:Coefficient ! Coefficient
relationship: context ECOSIMCONCEPT:Litter ! Litter
relationship: measurement_of ECOSIMCONCEPT:Partitioning ! Partitioning

[Term]
id: ECOSIM:EPOLNB
name: branch nodule nonstructural C
def: "Branch nodule nonstructural C refers to the unstructured or non-segregated carbon present in the nodules that grow on the branches of certain legume plants. These nodules are formed due to the symbiotic relationship of plants with nitrogen-fixing bacteria, and play a critical role in nutrient cycling." []
is_a: ECOSIM:CATEGORYPlantPhysiology ! category - plant physiology
is_a: ECOSIMCONCEPT:UnclassifiedVariable ! unclassified variable
relationship: attribute ECOSIMCONCEPT:Carbon ! Carbon
relationship: context ECOSIMCONCEPT:Branch ! Branch
relationship: has_unit ECOSIM:gd-2 ! g d-2
relationship: measurement_of ECOSIMCONCEPT:Nodule ! Nodule

[Term]
id: ECOSIM:EPOLNP
name: canopy nodule nonstructural element
def: "Canopy nodule nonstructural element refers to the amount of nonstructural elements (proteins, sugars, starches, and lipids) in plant nodules within the canopy. This parameter is essential in plant and nitrogen cycle modelling as it determines the amount of nutrients and energy available for plant growth and development." []
is_a: ECOSIM:CATEGORYPlantPhysiology ! category - plant physiology
is_a: ECOSIMCONCEPT:UnclassifiedVariable ! unclassified variable
relationship: has_unit ECOSIM:gd-2 ! g d-2
relationship: measured_in ECOSIMCONCEPT:CanopyNodule ! CanopyNodule
relationship: measurement_of ECOSIMCONCEPT:NonStructuralElement ! Non-structural element

[Term]
id: ECOSIM:EPOOL
name: branch nonstructural element
def: "EPOOL, or Branch Nonstructural Element, refers to elements or compounds that are not part of the structural components of tree branches but play crucial roles in the functioning and growth of the branches. These include nutrients, sugars, and other organic compounds. This measurement is important in understanding tree growth, health, and resilience." []
is_a: ECOSIMCONCEPT:Branch ! Branch
is_a: ECOSIMCONCEPT:UnclassifiedVariable ! unclassified variable
relationship: attribute ECOSIMCONCEPT:Element ! Element
relationship: has_unit ECOSIM:gd-2 ! g d-2

[Term]
id: ECOSIM:EPOOLN
name: root layer nonstructural element
def: "Root layer non-structural element refers to aspects of a plant's root layer that do not contribute to its structural integrity. These may include biomolecules, enzymes, or other compounds that play vital roles in the plant's basic physiological processes. In earth system modeling, these non-structural elements help in understanding the health and function of plant roots and can impact parameters like nutrient uptake, soil interaction, and overall plant vitality." []
is_a: ECOSIM:CATEGORYRootPhysiology ! category - root physiology
relationship: has_unit ECOSIM:gd-2 ! g d-2
relationship: measured_in ECOSIMCONCEPT:RootLayer ! Root layer

[Term]
id: ECOSIM:EPOOLR
name: root layer nonstructural element
def: "Root layer nonstructural element refers to the element in the root layer of plants that is not involved in the physical construction of the plant but plays crucial roles in physiological processes such as nutrient cycling, growth regulation, and stress response. This includes elements like sugars, amino acids, and certain minerals." []
is_a: ECOSIM:CATEGORYRootPhysiology ! category - root physiology
is_a: ECOSIMCONCEPT:UnclassifiedVariable ! unclassified variable
relationship: attribute ECOSIMCONCEPT:Element ! Element
relationship: has_unit ECOSIM:gd-2 ! g d-2
relationship: measured_in ECOSIMCONCEPT:RootLayer ! Root layer

[Term]
id: ECOSIM:ESNC
name: plant litterfall element
def: "ESNC (plant litterfall element) refers to the element, possibly a nutrient like Nitrogen (N), Carbon (C) or others, that falls to the ground from plants - typically as leaves, branches, and other plant debris. This litterfall contributes to the nutrient cycle by slowly decomposing and releasing the elements back into the soil. The term 'ESNC' is used in ecological modeling and can have different specific meanings depending on the context." []
is_a: ECOSIM:CATEGORYPlantPhysiology ! category - plant physiology
is_a: ECOSIMCONCEPT:UnclassifiedVariable ! unclassified variable
relationship: has_unit ECOSIM:gd-2h-1 ! g d-2 h-1
relationship: measured_in ECOSIMCONCEPT:PlantLitterfall ! PlantLitterfall
relationship: measurement_of ECOSIMCONCEPT:Element ! Element

[Term]
id: ECOSIM:ETCanP
name: total transpiration
is_a: ECOSIMCONCEPT:UnclassifiedVariable ! unclassified variable
relationship: has_unit ECOSIM:md-2 ! m d-2
relationship: measured_in ECOSIMCONCEPT:Atmosphere ! Atmosphere
relationship: measurement_of ECOSIMCONCEPT:Water ! Water

[Term]
id: ECOSIM:ETGR4
name: maximum light C4 carboxylation rate under saturating CO2
def: "Maximum light C4 carboxylation rate under saturating CO2 refers to the maximum rate at which the C4 photosynthetic pathway can absorb and convert CO2 into carbohydrates under light conditions when the concentration of CO2 is not limiting. This measurement provides an estimate of the potential efficiency and capacity of the C4 photosynthetic pathway under optimal light conditions." []
is_a: ECOSIM:CATEGORYCanopyPhysiology ! category - Canopy Physiology
is_a: ECOSIM:CATEGORYPlantPhysiology ! category - plant physiology
relationship: attribute ECOSIMCONCEPT:Rate ! Rate
relationship: has_unit ECOSIM:umolm-2s-1 ! umol m-2 s-1
relationship: measured_in ECOSIMCONCEPT:Leaf ! Leaf
relationship: measurement_of ECOSIMCONCEPT:C4Carboxylation ! C4 carboxylation

[Term]
id: ECOSIM:ETGRO
name: maximum light carboxylation rate under saturating CO2
def: "Maximum light carboxylation rate under saturating CO2 refers to the maximum rate at which the function responsible for the absorption and conversion of CO2 into carbohydrates performs during light conditions when CO2 concentration is not limiting. This can help determine the efficiency of the light-dependent reactions in photosynthesis under optimal conditions." []
is_a: ECOSIM:CATEGORYCanopyPhysiology ! category - Canopy Physiology
is_a: ECOSIM:CATEGORYPlantPhysiology ! category - plant physiology
relationship: attribute ECOSIMCONCEPT:Rate ! Rate
relationship: has_unit ECOSIM:umolm-2s-1 ! umol m-2 s-1
relationship: measured_in ECOSIMCONCEPT:Leaf ! Leaf
relationship: measurement_of ECOSIMCONCEPT:Carboxylation ! Carboxylation

[Term]
id: ECOSIM:ETMX
name: cholorophyll activity
is_a: ECOSIM:CATEGORYCanopyPhysiology ! category - Canopy Physiology
is_a: ECOSIM:CATEGORYPlantPhysiology ! category - plant physiology
relationship: attribute ECOSIMCONCEPT:Activity ! Activity
relationship: has_unit ECOSIM:umolg-1h-1at25oC ! umol g-1 h-1 at 25 oC
relationship: measured_in ECOSIMCONCEPT:Leaf ! Leaf
relationship: measurement_of ECOSIMCONCEPT:Chlorophyll ! Chlorophyll

[Term]
id: ECOSIM:EvapTransHeatP
name: canopy latent heat flux
is_a: ECOSIMCONCEPT:UnclassifiedVariable ! unclassified variable
relationship: has_unit ECOSIM:MJd-2h-1 ! MJ d-2 h-1

[Term]
id: ECOSIM:F1PR
name: F1PR
is_a: ECOSIM:CATEGORYAtmosphericConditions ! category - Atmospheric Conditions
relationship: measured_in ECOSIMCONCEPT:Genome ! Genome
relationship: measurement_of ECOSIMCONCEPT:F1PR ! F1PR

[Term]
id: ECOSIM:F2PR
name: F2PR
is_a: ECOSIM:CATEGORYAtmosphericConditions ! category - Atmospheric Conditions

[Term]
id: ECOSIM:FDBK
name: branch down-regulation of CO2 fixation
def: "Branch Down-regulation of CO2 fixation refers to the process that reduces the rate of carbon dioxide fixation in a branch of a plant. This process can occur due to environmental changes or physiological feedback mechanism within the plant." []
is_a: ECOSIM:CATEGORYCanopyPhysiology ! category - Canopy Physiology
is_a: ECOSIM:CATEGORYPlantPhysiology ! category - plant physiology
relationship: measured_in ECOSIMCONCEPT:Branch ! Branch
relationship: measurement_of ECOSIMCONCEPT:CO2Fixation ! CO2Fixation

[Term]
id: ECOSIM:FDBK4
name: down-regulation of C4 photosynthesis
def: "Negative regulation of the carbon fixation pathway, known as C4 photosynthesis, where the reaction is shut down or slowed down." []
is_a: ECOSIM:CATEGORYCanopyPhysiology ! category - Canopy Physiology
is_a: ECOSIM:CATEGORYPlantPhysiology ! category - plant physiology
relationship: measured_in ECOSIMCONCEPT:Leaf ! Leaf
relationship: measurement_of ECOSIMCONCEPT:C4Photosynthesis ! C4Photosynthesis

[Term]
id: ECOSIM:FDBKX
name: down-regulation of C4 photosynthesis
def: "Negative regulation of the carbon fixation pathway, known as C4 photosynthesis, where the reaction is shut down or slowed down." []
is_a: ECOSIM:CATEGORYCanopyPhysiology ! category - Canopy Physiology
is_a: ECOSIM:CATEGORYPlantPhysiology ! category - plant physiology
relationship: measured_in ECOSIMCONCEPT:Leaf ! Leaf
relationship: measurement_of ECOSIMCONCEPT:C4Photosynthesis ! C4Photosynthesis

[Term]
id: ECOSIM:FDPTH
name: depth of fertilizer application
def: "Depth of fertilizer application refers to the distance below the surface of the soil at which fertilizers are applied. Different crops and soils may require different application depths for optimal nutrient absorption and to minimize nutrient losses due to leaching or erosion. It is an important parameter in agricultural modeling and management, directly influencing the effectiveness and environmental impact of fertilization practices." []
is_a: ECOSIMCONCEPT:UnclassifiedVariable ! unclassified variable
relationship: attribute ECOSIMCONCEPT:Depth ! Depth
relationship: has_unit ECOSIM:m ! m
relationship: measured_in ECOSIMCONCEPT:Soil ! Soil
relationship: measurement_of ECOSIMCONCEPT:FertilizerApplication ! FertilizerApplication

[Term]
id: ECOSIM:FERT
name: fertilizer application
def: "Fertilizer application refers to the process of adding supplemental nutrients to the soil to improve plant health and crop yield. The type, amount, timing, and method of application can depend on various factors including the specific crop being grown, the characteristics of the soil, and the overall goals of the agriculture operation." []
is_a: ECOSIMCONCEPT:UnclassifiedVariable ! unclassified variable
relationship: attribute ECOSIMCONCEPT:Process ! process
relationship: context ECOSIMCONCEPT:Fertilizer ! Fertilizer
relationship: has_unit ECOSIM:gm-2 ! g m-2

[Term]
id: ECOSIM:FESGL
name: aqueous Fe diffusivity
is_a: ECOSIM:CATEGORYHydrology ! category - Hydrology
is_a: ECOSIMCONCEPT:UnclassifiedVariable ! unclassified variable
relationship: attribute ECOSIMCONCEPT:Diffusivity ! Diffusivity
relationship: has_unit ECOSIM:m2h-1 ! m2 h-1
relationship: measured_in ECOSIMCONCEPT:Water ! Water
relationship: measurement_of ECOSIMCONCEPT:Iron ! Iron

[Term]
id: ECOSIM:FILM
name: soil water film thickness
def: "Soil water film thickness refers to the thickness of a layer of water that coats soil particles. This water film allows for the movement and availability of nutrients and is crucial for plant absorption and root functions. The thickness can vary depending on soil type, rainfall, and other environmental conditions." []
is_a: ECOSIMCONCEPT:UnclassifiedVariable ! unclassified variable
relationship: has_unit ECOSIM:m ! m
relationship: measured_in ECOSIMCONCEPT:Soil ! Soil

[Term]
id: ECOSIM:FIRRA
name: fraction of FC - WP below which automatic irrigation applied
def: "FIRRA (Fraction of FC - WP below which automatic irrigation applied) is an agriculture modeling concept which refers to the fraction of field capacity (FC) minus wilting point (WP) below which automatic irrigation is applied. FC refers to the amount of water that can be held in the soil after excess water has drained away, and WP is the point at which the soil is so dry that plants can no longer extract water. This parameter helps in determining the optimal irrigation schedule for maximizing crop yield and minimizing water use." []
is_a: ECOSIMCONCEPT:UnclassifiedVariable ! unclassified variable
relationship: attribute ECOSIMCONCEPT:Fraction ! Fraction
relationship: context ECOSIMCONCEPT:Irrigation ! Irrigation
relationship: measurement_of ECOSIMCONCEPT:Water ! Water

[Term]
id: ECOSIM:FLG4
name: flag to detect physiological maturity from grain fill
def: "Flag to detect physiological maturity from grain fill is a parameter in crop models that triggers the simulation of the transition from the grain filling stage to physiological maturity in crops. This might be based on temperature thresholds, day length, or other plant growth parameters. Physiological maturity indicates the stage at which the crop has completed its growth and development and is ready for harvest." []
is_a: ECOSIM:CATEGORYCanopyStructure ! category - canopy structure
relationship: measurement_of ECOSIMCONCEPT:PhysiologicalMaturity ! PhysiologicalMaturity

[Term]
id: ECOSIM:FLGZ
name: counter for mobilizing nonstructural C during autumn leafoff/hardening
def: "Counter for mobilizing nonstructural C during autumn leafoff/hardening indicates the amount or level of nonstructural carbon being mobilised during the process of leaf off or hardening in autumn. This can provide insights into the carbon cycle and plant physiology, especially in relation to adaptations to seasonal changes." []
is_a: ECOSIM:CATEGORYCanopyStructure ! category - canopy structure
relationship: has_unit ECOSIM:h ! h
relationship: measurement_of ECOSIMCONCEPT:NonStructuralC ! Non-structural carbohydrate

[Term]
id: ECOSIM:FLQGI
name: irrifation flux into soil surface
def: "Irrigation flux into soil surface refers to the rate at which water from irrigation enters the soil surface. This is an important factor in agricultural management and water resource planning as it directly influences the amount of water available to crops and its effectiveness in promoting plant growth. Measurements of this parameter can help optimize irrigation strategies and conserve water resources." []
is_a: ECOSIMCONCEPT:UnclassifiedVariable ! unclassified variable
relationship: attribute ECOSIMCONCEPT:Flux ! Flux
relationship: has_unit ECOSIM:m3d-2h-1 ! m3 d-2 h-1
relationship: measured_in ECOSIMCONCEPT:SoilSurface ! Soil surface
relationship: measurement_of ECOSIMCONCEPT:Water ! Water

[Term]
id: ECOSIM:FLQGQ
name: precipitation flux into soil surface
def: "Precipitation flux into soil surface refers to the rate at which water (from rainfall, snow melt, etc.) enters the soil surface per unit area. This parameter is crucial in hydrological studies and modeling, as it impacts soil moisture levels, groundwater recharge, runoff generation and erosion." []
is_a: ECOSIM:CATEGORYHydrology ! category - Hydrology
is_a: ECOSIMCONCEPT:UnclassifiedVariable ! unclassified variable
relationship: attribute ECOSIMCONCEPT:Flux ! Flux
relationship: context ECOSIMCONCEPT:Precipitation ! Precipitation
relationship: has_unit ECOSIM:m3d-2h-1 ! m3 d-2 h-1
relationship: measured_in ECOSIMCONCEPT:SoilSurface ! Soil surface
relationship: measurement_of ECOSIMCONCEPT:Water ! Water

[Term]
id: ECOSIM:FLQRI
name: irrigation flux into surface litter
def: "Irrigation flux into surface litter quantifies the amount of water added to the surface litter layer of the soil through irrigation. Surface litter refers to the organic material, such as dead leaves, twigs, and other plant residues, that covers the soil surface. This process can affect the moisture content and decomposition rates of the surface litter, affecting nutrient cycling and soil fertility." []
is_a: ECOSIM:CATEGORYHydrology ! category - Hydrology
is_a: ECOSIMCONCEPT:UnclassifiedVariable ! unclassified variable
relationship: attribute ECOSIMCONCEPT:Flux ! Flux
relationship: has_unit ECOSIM:m3d-2h-1 ! m3 d-2 h-1
relationship: measured_in ECOSIMCONCEPT:SurfaceLitter ! Surface litter
relationship: measurement_of ECOSIMCONCEPT:IrrigationWater ! IrrigationWater

[Term]
id: ECOSIM:FLQRQ
name: precipitation flux into surface litter
def: "Precipitation flux into surface litter refers to the flow rate of precipitation, such as rain, snowfall, or dew, into the surface litter layer of an ecosystem. Surface litter, which consists of dead plant material such as leaves and twigs, plays a critical role in nutrient cycling and soil formation. Measurement of this precipitation flux is important for understanding the hydrological dynamics of an ecosystem, particularly the processes of infiltration and percolation." []
is_a: ECOSIM:CATEGORYHydrology ! category - Hydrology
is_a: ECOSIMCONCEPT:UnclassifiedVariable ! unclassified variable
relationship: attribute ECOSIMCONCEPT:Flux ! Flux
relationship: has_unit ECOSIM:m3d-2h-1 ! m3 d-2 h-1
relationship: measured_in ECOSIMCONCEPT:SurfaceLitter ! Surface litter
relationship: measurement_of ECOSIMCONCEPT:Precipitation ! Precipitation

[Term]
id: ECOSIM:FMOL
name: total gas concentration
def: "Total gas concentration refers to the overall amount of gas in a specified volume. This parameter can include various types of gases, depending on the context, such as greenhouse gases, pollutants, or atmospheric gases. It is an important parameter in fields such as meteorology, environmental science, and climate modeling." []
is_a: ECOSIM:CATEGORYAtmosphericConditions ! category - Atmospheric Conditions
is_a: ECOSIM:CATEGORYCanopyPhysiology ! category - Canopy Physiology
is_a: ECOSIM:CATEGORYPlantPhysiology ! category - plant physiology
relationship: attribute ECOSIMCONCEPT:Concentration ! Concentration
relationship: has_unit ECOSIM:molm-3 ! mol m-3
relationship: measured_in ECOSIMCONCEPT:Air ! Air
relationship: measurement_of ECOSIMCONCEPT:Gas ! Gas

[Term]
id: ECOSIM:FNOD
name: parameter for allocation of growth to nodes
def: "Parameter for allocation of growth to nodes refers to a factor used in plant growth models that determines how much of the plant's growth is allocated to its nodes. Nodes are the points on a plant stem where leaves or branches are attached. Understanding and accurately estimating this parameter is vital for predicting plant architecture and yield in agricultural systems." []
is_a: ECOSIM:CATEGORYCanopyStructure ! category - canopy structure
is_a: ECOSIM:CATEGORYPlantPhysiology ! category - plant physiology
relationship: measured_in ECOSIMCONCEPT:Plant ! Plant
relationship: measurement_of ECOSIMCONCEPT:Node ! Node
relationship: measurement_of ECOSIMCONCEPT:Nodes ! Nodes

[Term]
id: ECOSIM:FOSRH
name: fraction of total organic C in complex
def: "Fraction of total organic C in complex represents the proportion of the total organic carbon present in complex forms in the soil. Organic carbon in the soil is found in various forms, including simple, complex, soluble, and insoluble forms. Each form plays a unique role in soil processes, including nutrient availability, water retention, and soil structure maintenance. The fraction of total organic carbon in complex forms can help us understand the carbon storage potential of the soil." []
is_a: ECOSIM:CATEGORYMicrobialActivity ! category - microbial activity
is_a: ECOSIM:CATEGORYSoilBiogeochemistry ! category - Soil Biogeochemistry
relationship: measured_in ECOSIMCONCEPT:Soil ! Soil
relationship: measurement_of ECOSIMCONCEPT:Fraction ! Fraction

[Term]
id: ECOSIM:FWatDischarge
name: water discharge
is_a: ECOSIM:CATEGORYHydrology ! category - Hydrology
relationship: has_unit ECOSIM:m3d-2h-1 ! m3 d-2 h-1

[Term]
id: ECOSIM:FWatExMacP2MicPM
name: soil macropore - micropore water transfer
def: "Soil macropore - micropore water transfer refers to the process of movement of water within the soil between the larger pores or cavities (macropores) and the smaller ones (micropores). This is an important aspect of the soil's hydrological behavior, affecting the soil's water-holding capacity, water availability for plant uptake, and the leaching of nutrients and contaminants. The rate of this transfer can be influenced by factors such as soil texture, structure, organic matter content, and external conditions such as precipitation and evaporation." []
is_a: ECOSIM:CATEGORYHydrology ! category - Hydrology
is_a: ECOSIMCONCEPT:UnclassifiedVariable ! unclassified variable
relationship: has_unit ECOSIM:gd-2t-1 ! g d-2 t-1
relationship: measured_in ECOSIMCONCEPT:SoilMacropore ! SoilMacropore
relationship: measured_in ECOSIMCONCEPT:SoilMicropore ! Soil micropore

[Term]
id: ECOSIM:FWatIrrigate2MicP
name: underground irrigation
is_a: ECOSIMCONCEPT:UnclassifiedVariable ! unclassified variable
relationship: has_unit ECOSIM:m3d-2h-1 ! m3 d-2 h-1

[Term]
id: ECOSIM:FracPARByCanP
name: fraction of incoming PAR absorbed by canopy
is_a: ECOSIM:CATEGORYSurfaceEnergyBalance ! category - Surface Energy Balance

[Term]
id: ECOSIM:FracSWRad2Grnd
name: fraction of radiation intercepted by ground surface
is_a: ECOSIMCONCEPT:UnclassifiedVariable ! unclassified variable

[Term]
id: ECOSIM:FracSurfAsBareSoi
name: fraction of exposed soil surface
is_a: ECOSIMCONCEPT:UnclassifiedVariable ! unclassified variable

[Term]
id: ECOSIM:FracSurfByLitR
name: fraction of soil surface covered by surface litter
def: "FracSurfByLitR refers to the proportion of the soil surface that is covered by surface litter. Surface litter refers to the layer of fallen leaves, twigs, bark, and other organic material that covers the soil surface. It plays a crucial role in the nutrient cycling processes in ecosystems, providing a source of nutrients and organic matter to the soil below and offering protection against soil erosion." []
is_a: ECOSIM:CATEGORYSoilBiogeochemistry ! category - Soil Biogeochemistry
is_a: ECOSIMCONCEPT:UnclassifiedVariable ! unclassified variable
relationship: context ECOSIMCONCEPT:SurfaceLitter ! Surface litter
relationship: measured_in ECOSIMCONCEPT:SoilSurface ! Soil surface

[Term]
id: ECOSIM:GAZI
name: azimuth of slope
is_a: ECOSIMCONCEPT:UnclassifiedVariable ! unclassified variable
relationship: measured_in ECOSIMCONCEPT:Slope ! Slope

[Term]
id: ECOSIM:GCOS
name: cosine of slope
is_a: ECOSIMCONCEPT:UnclassifiedVariable ! unclassified variable

[Term]
id: ECOSIM:GFILL
name: maximum rate of fill per grain
def: "Maximum rate of fill per grain denotes the maximum speed at which an individual grain can accumulate matter during the grain filling stage. This parameter has significant implications for the final yield and quality of a crop. The grain filling rate is affected by various factors such as genetic characteristics, environmental conditions, and nutrient availability." []
is_a: ECOSIM:CATEGORYCanopyStructure ! category - canopy structure
relationship: attribute ECOSIMCONCEPT:Rate ! Rate
relationship: has_unit ECOSIM:gh-1 ! g h-1
relationship: measured_in ECOSIMCONCEPT:Grain ! Grain

[Term]
id: ECOSIM:GKC4
name: Ca-NH4 Gapon selectivity coefficient
def: "The Ca-NH4 Gapon selectivity coefficient (GKC4) represents the relative affinity or selectivity between calcium (Ca) and ammonium (NH4) cations being adsorbed onto soil particles. The Gapon selectivity coefficient is a measure used in soil science to explain the ion exchange between different cations in the soil. Cation exchange is an important process in soil fertility and nutrient management in agriculture." []
is_a: ECOSIM:CATEGORYSoilProperty ! category - soil property
relationship: measurement_of ECOSIMCONCEPT:Ca ! Calcium
relationship: measurement_of ECOSIMCONCEPT:NH4 ! Ammonium

[Term]
id: ECOSIM:GKCA
name: Ca-Al Gapon selectivity coefficient
def: "Ca-Al Gapon selectivity coefficient (GKCA) is a parameter used in soil science to quantify the energy of exchange or selectivity between calcium (Ca) and aluminum (Al) ions in the soil. This value is particularly important for understanding nutrient availability in acidic soils, where Al toxicity can limit plant growth. The Gapon selectivity coefficient is calculated based on the ion concentrations and activity coefficients in the soil solution and exchangeable ions on the soil cation exchange complex." []
is_a: ECOSIM:CATEGORYSoilProperty ! category - soil property
relationship: attribute ECOSIMCONCEPT:Coefficient ! Coefficient

[Term]
id: ECOSIM:GKCH
name: Ca-H Gapon selectivity coefficient
def: "The Ca-H Gapon selectivity coefficient refers to a value that represents the ability of a soil to preferentially adsorb calcium ions (Ca) over hydrogen ions (H). This value is derived from the Gapon equation, a model that describes ion-exchange reactions in soils. It is a crucial parameter in soil science and earth system modeling, as it helps in understanding ion exchange processes and nutrient availability in soils." []
is_a: ECOSIM:CATEGORYSoilProperty ! category - soil property
relationship: measured_in ECOSIMCONCEPT:Soil ! Soil
relationship: measurement_of ECOSIMCONCEPT:Calcium ! Calcium
relationship: measurement_of ECOSIMCONCEPT:Hydrogen ! Hydrogen

[Term]
id: ECOSIM:GKCK
name: Ca-K Gapon selectivity coefficient
def: "Ca-K Gapon selectivity coefficient, represented as GK:CK, refers to the quantification of the preferential adsorption of calcium (Ca) and potassium (K) ions by soil particles. It indicates the affinity, or preference, of soil particles for one cation over another. Larger selectivity coefficients for a given cation indicate a stronger affinity for that cation. This parameter is crucial in soil science as it helps in understanding nutrient availability and soil fertility." []
is_a: ECOSIM:CATEGORYSoilProperty ! category - soil property
relationship: context ECOSIMCONCEPT:Calcium ! Calcium
relationship: context ECOSIMCONCEPT:Potassium ! Potassium
relationship: measured_in ECOSIMCONCEPT:Soil ! Soil
relationship: measurement_of ECOSIMCONCEPT:IonSelectivity ! IonSelectivity

[Term]
id: ECOSIM:GKCM
name: Ca-Mg Gapon selectivity coefficient
def: "The Ca-Mg Gapon selectivity coefficient (GKCM) is a measure used in soil chemistry to quantify the preferential adsorption or exchange between calcium (Ca) and magnesium (Mg) cations in the soil. It is used in soil fertility assessments and in modelling the nutrient dynamics in soils." []
is_a: ECOSIM:CATEGORYSoilBiogeochemistry ! category - Soil Biogeochemistry
is_a: ECOSIM:CATEGORYSoilProperty ! category - soil property
relationship: context ECOSIMCONCEPT:Magnesium ! Magnesium
relationship: context ECOSIMCONCEPT:Soil ! Soil
relationship: measurement_of ECOSIMCONCEPT:Calcium ! Calcium
relationship: qualifier ECOSIMCONCEPT:Coefficient ! Coefficient

[Term]
id: ECOSIM:GKCN
name: Ca-Na Gapon selectivity coefficient
def: "The Ca-Na Gapon selectivity coefficient (GKCN) is a measure of the ion exchange selectivity of a soil, which indicates the affinity of a soil's exchange sites for calcium (Ca) in relation to sodium (Na). In situations where excess sodium is present in the soil, a low GKCN value would indicate the soil has a higher ability to retain calcium and prevent the undesirable effects of sodium." []
is_a: ECOSIM:CATEGORYSoilProperty ! category - soil property
relationship: attribute ECOSIMCONCEPT:Calcium ! Calcium
relationship: attribute ECOSIMCONCEPT:Coefficient ! Coefficient
relationship: context ECOSIMCONCEPT:Sodium ! Sodium
relationship: measured_in ECOSIMCONCEPT:Soil ! Soil
relationship: measurement_of ECOSIMCONCEPT:Ca-NaSelection ! Ca-NaSelection

[Term]
id: ECOSIM:GMSGL
name: aqueous Mg diffusivity
def: "Aqueous Mg diffusivity refers to the measure of the rate at which magnesium (Mg) ions move or spread through water or an aqueous medium. It is an important parameter in geochemistry, hydrology, and soil science, as it can impact a range of processes, including nutrient cycling, weathering rates, and water quality." []
is_a: ECOSIMCONCEPT:UnclassifiedVariable ! unclassified variable
relationship: attribute ECOSIMCONCEPT:Diffusivity ! Diffusivity
relationship: has_unit ECOSIM:m2h-1 ! m2 h-1
relationship: measured_in ECOSIMCONCEPT:Water ! Water
relationship: measurement_of ECOSIMCONCEPT:Magnesium ! Magnesium

[Term]
id: ECOSIM:GPP
name: gross primary productivity
def: "Gross Primary Productivity (GPP) is the total amount of energy that plants capture and assimilate in a given period." []
is_a: ECOSIMCONCEPT:UnclassifiedVariable ! unclassified variable
relationship: has_unit ECOSIM:gd-2h-1 ! g d-2 h-1
relationship: measurement_of ECOSIMCONCEPT:Energy ! Energy

[Term]
id: ECOSIM:GRNO
name: canopy grain number
def: "Canopy grain number refers to the total number of grains present in the canopy of a plant or crop. This term is significant in agricultural studies as it affects the yield of crops. It is also important in ecological modeling as it is a key parameter in estimating energy transfer and net primary productivity." []
is_a: ECOSIM:CATEGORYCanopyStructure ! category - canopy structure
is_a: ECOSIM:CATEGORYPlantPhysiology ! category - plant physiology
relationship: has_unit ECOSIM:d-2 ! d-2
relationship: measured_in ECOSIMCONCEPT:Canopy ! Canopy
relationship: measurement_of ECOSIMCONCEPT:Grain ! Grain

[Term]
id: ECOSIM:GRNOB
name: branch grain number
def: "Branch grain number refers to the count of grains present on a branch of a plant. It is a parameter used in agricultural and environmental modelling to understand grain production and yield potential." []
is_a: ECOSIM:CATEGORYCanopyStructure ! category - canopy structure
is_a: ECOSIM:CATEGORYPlantPhysiology ! category - plant physiology
relationship: has_unit ECOSIM:d-2 ! d-2
relationship: measured_in ECOSIMCONCEPT:PlantBranch ! PlantBranch
relationship: measurement_of ECOSIMCONCEPT:Grain ! Grain

[Term]
id: ECOSIM:GRNXB
name: branch potential grain number
def: "Branch potential grain number refers to the number of potential grains that can be developed on a plant branch under ideal conditions. This can vary based on agricultural species or varieties, and their ability to adapt to different environmental conditions." []
is_a: ECOSIM:CATEGORYCanopyStructure ! category - canopy structure
relationship: has_unit ECOSIM:d-2 ! d-2
relationship: measured_in ECOSIMCONCEPT:Branch ! Branch
relationship: measurement_of ECOSIMCONCEPT:GrainNumber ! GrainNumber

[Term]
id: ECOSIM:GROUP
name: plant maturity group
def: "Plant maturity group refers to a classification based on the relative maturity of a plant species. It often used in agriculture to group crops, especially soybeans, based on their adaptability to certain regions and the average dates of their flowering and maturation periods. Knowledge of plant maturity group is crucial for crop management and for predicting yields." []
is_a: ECOSIM:CATEGORYCanopyPhysiology ! category - Canopy Physiology
is_a: ECOSIM:CATEGORYCanopyStructure ! category - canopy structure
is_a: ECOSIM:CATEGORYPlantPhysiology ! category - plant physiology
relationship: measurement_of ECOSIMCONCEPT:Plant ! Plant

[Term]
id: ECOSIM:GROUPI
name: acclimated plant maturity group
def: "Acclimated Plant Maturity Group is a term used to categorize plant varieties or species based on their physiological maturity. This aids in understanding and modeling plant growth and development patterns across different regions. The parameter 'GROUPI' captures this categorization in the context of acclimated plant species, indicating their maturity group in particular environments." []
is_a: ECOSIM:CATEGORYCanopyPhysiology ! category - Canopy Physiology
is_a: ECOSIM:CATEGORYCanopyStructure ! category - canopy structure
is_a: ECOSIM:CATEGORYPlantPhysiology ! category - plant physiology
relationship: measured_in ECOSIMCONCEPT:Plant ! Plant

[Term]
id: ECOSIM:GROUPX
name: initial plant maturity group
def: "Initial plant maturity group refers to the classification of a plant, particularly crops like soybeans, based on their maturity rate at the initial stage of growth. This classification helps to control and manage the harvesting time of the plant, thereby optimizing yield. It's an important parameter in agricultural and earth system modeling, as it impacts the timing of key developmental stages." []
is_a: ECOSIM:CATEGORYCanopyStructure ! category - canopy structure
is_a: ECOSIM:CATEGORYPlantPhysiology ! category - plant physiology
relationship: measured_in ECOSIMCONCEPT:Plant ! Plant
relationship: measurement_of ECOSIMCONCEPT:PlantMaturity ! PlantMaturity

[Term]
id: ECOSIM:GRWTB
name: maximum grain C during grain fill
def: "Maximum grain C during grain fill refers to the maximum amount of carbon (C) allocated to the grain during the grain filling stage of a crop's growth cycle. This is a crucial component of plant growth and development, influencing crop yield and quality. It is an important parameter in crop and ecological modelling, providing insight into plant physiology and nutrient cycling." []
is_a: ECOSIM:CATEGORYPlantPhysiology ! category - plant physiology
is_a: ECOSIMCONCEPT:UnclassifiedVariable ! unclassified variable
relationship: has_unit ECOSIM:gd-2 ! g d-2
relationship: measured_in ECOSIMCONCEPT:Grain ! Grain
relationship: measurement_of ECOSIMCONCEPT:Carbon ! Carbon

[Term]
id: ECOSIM:GSIN
name: sine of slope
def: "The value obtained from the mathematical function of sine applied to the gradient or slope. It is often used in various calculations in earth system sciences, such as those related to hill slopes, flow directions, and solar radiation." []
is_a: ECOSIMCONCEPT:UnclassifiedVariable ! unclassified variable

[Term]
id: ECOSIM:GSTGF
name: normalized node number during reproductive growth stages
def: "Normalized node number during reproductive growth stages refers to the standardization of the node number, which is an important aspect of plant structure, during the reproductive phase of plant growth. This helps in shedding light on the varying developmental processes across different phases of a plant's life cycle." []
is_a: ECOSIM:CATEGORYCanopyStructure ! category - canopy structure
is_a: ECOSIM:CATEGORYPlantPhysiology ! category - plant physiology
relationship: measured_in ECOSIMCONCEPT:Plant ! Plant
relationship: measurement_of ECOSIMCONCEPT:NodeNumber ! NodeNumber

[Term]
id: ECOSIM:GSTGI
name: normalized node number during vegetative growth stages
def: "Normalized node number during vegetative growth stages refers to the number of nodes (joints or points of attachment) on a plant that appear during its vegetative growth period, normalized to account for differences in growth conditions or plant varieties. This measurement is often used in plant physiology and growth modeling to track developmental progression, as the number of nodes can serve as an indicator of a plant's stage in its life cycle." []
is_a: ECOSIM:CATEGORYCanopyStructure ! category - canopy structure
relationship: attribute ECOSIMCONCEPT:Number ! Number
relationship: measured_in ECOSIMCONCEPT:Node ! Node

[Term]
id: ECOSIM:GasSfAtmFlx
name: surface-atmosphere gas exchange flux
def: "The flux of a gas between the Earth's surface and the atmosphere. This can include both emission (gas moving from the surface to the atmosphere) and deposition (gas moving from the atmosphere to the surface)." []
is_a: ECOSIM:CATEGORYGasFlux ! category - Gas Flux
is_a: ECOSIMCONCEPT:UnclassifiedVariable ! unclassified variable
relationship: attribute ECOSIMCONCEPT:Flux ! Flux
relationship: has_unit ECOSIM:gd-2h-1 ! g d-2 h-1
relationship: measured_in ECOSIMCONCEPT:SurfaceAtmosphere ! Surface atmosphere
relationship: measurement_of ECOSIMCONCEPT:Gas ! Gas

[Term]
id: ECOSIM:GridMaxCanopyHeight
name: canopy height
is_a: ECOSIM:CATEGORYCanopyStructure ! category - canopy structure
relationship: attribute ECOSIMCONCEPT:Height ! Height
relationship: has_unit ECOSIM:m ! m
relationship: measured_in ECOSIMCONCEPT:Grid ! Grid

[Term]
id: ECOSIM:GridPlantRootH2OUptake_vr
name: total root water uptake
def: "Total root water uptake refers to the amount of water absorbed by plant roots from the soil in a given area or volume. It represents the sum of water uptake by all plant roots within a specific grid or region in an earth systems model. Root water uptake is a crucial process for plants as it provides them with the necessary water for various physiological functions, including transpiration and photosynthesis." []
is_a: ECOSIM:CATEGORYPlantPhysiology ! category - plant physiology
is_a: ECOSIMCONCEPT:UnclassifiedVariable ! unclassified variable
relationship: attribute ECOSIMCONCEPT:Uptake ! Uptake
relationship: context ECOSIMCONCEPT:Grid ! Grid
relationship: has_unit ECOSIM:m3d-2 ! m3 d-2
relationship: measured_in ECOSIMCONCEPT:Root ! Root
relationship: measurement_of ECOSIMCONCEPT:Water ! Water

[Term]
id: ECOSIM:H2GE
name: atmospheric H2 concentration
def: "Atmospheric H2 concentration refers to the amount of hydrogen gas (H2) in the Earth's atmosphere, expressed typically in parts per million by volume (ppmv). Measuring this concentration is important in understanding the Earth's climate system, as H2 is one of the major constituent gases in the Earth's atmosphere and plays a critical role in various atmospheric processes." []
is_a: ECOSIM:CATEGORYAtmosphericConditions ! category - Atmospheric Conditions
is_a: ECOSIMCONCEPT:UnclassifiedVariable ! unclassified variable
relationship: attribute ECOSIMCONCEPT:Concentration ! Concentration
relationship: has_unit ECOSIM:umolmol-1 ! umol mol-1
relationship: measured_in ECOSIMCONCEPT:Atmosphere ! Atmosphere
relationship: measurement_of ECOSIMCONCEPT:H2 ! Dihydrogen

[Term]
id: ECOSIM:H2OVapDifscSno
name: water vapor diffusivity
def: "Water vapor diffusivity refers to the measure of the rate at which water vapor molecules move or spread through a medium, such as air or soil. It is an important parameter in environmental and earth system modeling, affecting processes like evaporation, condensation, and transpiration." []
is_a: ECOSIM:CATEGORYHydrology ! category - Hydrology
is_a: ECOSIMCONCEPT:UnclassifiedVariable ! unclassified variable
relationship: attribute ECOSIMCONCEPT:Diffusivity ! Diffusivity
relationship: has_unit ECOSIM:m2h-1 ! m2 h-1
relationship: measurement_of ECOSIMCONCEPT:WaterVapor ! Water vapor

[Term]
id: ECOSIM:HCH4G
name: soil CH4 flux
is_a: ECOSIM:CATEGORYBiogeochemistry ! category - Biogeochemistry
is_a: ECOSIM:CATEGORYTraceGasFlux ! category - trace gas flux
relationship: attribute ECOSIMCONCEPT:Flux ! Flux
relationship: has_unit ECOSIM:gd-2h-1 ! g d-2 h-1
relationship: measured_in ECOSIMCONCEPT:Soil ! Soil
relationship: measurement_of ECOSIMCONCEPT:CH4 ! Methane

[Term]
id: ECOSIM:HCO2G
name: soil CO2 flux
is_a: ECOSIM:CATEGORYBiogeochemistry ! category - Biogeochemistry
is_a: ECOSIM:CATEGORYTraceGasFlux ! category - trace gas flux
relationship: attribute ECOSIMCONCEPT:Flux ! Flux
relationship: has_unit ECOSIM:gd-2h-1 ! g d-2 h-1
relationship: measured_in ECOSIMCONCEPT:Soil ! Soil
relationship: measurement_of ECOSIMCONCEPT:CO2 ! Carbon dioxide

[Term]
id: ECOSIM:HCOB
name: bundle sheath nonstructural C3 content in C4 photosynthesis
def: "HCOB refers to the bundle sheath nonstructural C3 content in C4 photosynthesis. In C4 photosynthesis, carbon is fixed in mesophyll cells and then transported to bundle sheath cells in the form of a C4 compound. The C4 compound is then broken down to release C3 compounds, which are eventually fixed by the Calvin cycle. Bundle sheath nonstructural C3 content refers to the amount of these C3 compounds in the bundle sheath that are not structurally incorporated into the plant but can be freely metabolized." []
is_a: ECOSIM:CATEGORYCanopyPhysiology ! category - Canopy Physiology
is_a: ECOSIM:CATEGORYPlantPhysiology ! category - plant physiology
relationship: attribute ECOSIMCONCEPT:Content ! Content
relationship: context ECOSIMCONCEPT:C4Photosynthesis ! C4Photosynthesis
relationship: has_unit ECOSIM:gd-2 ! g d-2
relationship: measured_in ECOSIMCONCEPT:BundleSheathCell ! BundleSheathCell
relationship: measurement_of ECOSIMCONCEPT:C3Compound ! C3Compound

[Term]
id: ECOSIM:HCSGL
name: aqueous HCO3 diffusivity
def: "Aqueous HCO3 diffusivity refers to the measure of the rate at which bicarbonate (HCO3) ions diffuse or move through an aqueous medium. It is an important parameter in environmental and biomedical research, as it can impact various physiological processes such as pH regulation and respiration." []
is_a: ECOSIMCONCEPT:UnclassifiedVariable ! unclassified variable
relationship: attribute ECOSIMCONCEPT:Diffusivity ! Diffusivity
relationship: has_unit ECOSIM:m2h-1 ! m2 h-1
relationship: measured_in ECOSIMCONCEPT:Water ! Water
relationship: measurement_of ECOSIMCONCEPT:Bicarbonate ! Bicarbonate

[Term]
id: ECOSIM:HESNC
name: plant element litterfall
def: "Plant element litterfall refers to the organic material, including leaves, twigs, other plant parts, and animal feces, that falls to the ground and contributes to the organic matter found in the soil or on the forest floor. Litterfall is an important component of nutrient cycling in terrestrial ecosystems, as it represents a primary source of nutrient return to the soil." []
is_a: ECOSIMCONCEPT:UnclassifiedVariable ! unclassified variable
relationship: attribute ECOSIMCONCEPT:Litterfall ! Litterfall
relationship: has_unit ECOSIM:gd-2h-1 ! g d-2 h-1
relationship: measured_in ECOSIMCONCEPT:PlantElement ! PlantElement
relationship: measurement_of ECOSIMCONCEPT:Nutrient ! Nutrient

[Term]
id: ECOSIM:HEUPTK
name: net root element uptake (+ve) - exudation (-ve)
def: "Net root element uptake (+ve) - exudation (-ve) refers to the net amount of nutrient elements taken up by the roots of a plant, minus the amount lost through exudation. Exudation is the process whereby roots release organic substances into the surrounding soil. This parameter is essential in agricultural and ecological modeling as it helps in understanding nutrient cycling in soils and the nutrient utilization efficiency of plants." []
is_a: ECOSIM:CATEGORYRootPhysiology ! category - root physiology
is_a: ECOSIMCONCEPT:UnclassifiedVariable ! unclassified variable
relationship: attribute ECOSIMCONCEPT:Uptake ! Uptake
relationship: has_unit ECOSIM:gd-2h-1 ! g d-2 h-1
relationship: measured_in ECOSIMCONCEPT:Root ! Root
relationship: measurement_of ECOSIMCONCEPT:Element ! Element

[Term]
id: ECOSIM:HGSGL
name: gaseous H2 diffusivity
def: "Gaseous H2 diffusivity refers to the motion and spread of hydrogen gas (H2) molecules resulting from their kinetic energy. This property impacts how rapidly gases can spread through a medium (air, water, etc.)" []
is_a: ECOSIM:CATEGORYAtmosphericConditions ! category - Atmospheric Conditions
is_a: ECOSIMCONCEPT:UnclassifiedVariable ! unclassified variable
relationship: attribute ECOSIMCONCEPT:Diffusivity ! Diffusivity
relationship: has_unit ECOSIM:m2h-1 ! m2 h-1
relationship: measured_in ECOSIMCONCEPT:Air ! Air
relationship: measurement_of ECOSIMCONCEPT:HydrogenGas ! HydrogenGas

[Term]
id: ECOSIM:HLSGL
name: aqueous H2 diffusivity
def: "Aqueous H2 diffusivity refers to the measure of the rate at which hydrogen (H2) molecules move or spread through water or an aqueous medium. It is an important parameter in environmental and earth system modeling, as it can impact a range of processes including reactions in which hydrogen acts as a reductant, isotope fractionation, and the transfer of nutrients and pollutants." []
is_a: ECOSIM:CATEGORYHydrology ! category - Hydrology
is_a: ECOSIMCONCEPT:UnclassifiedVariable ! unclassified variable
relationship: attribute ECOSIMCONCEPT:Diffusivity ! Diffusivity
relationship: has_unit ECOSIM:m2h-1 ! m2 h-1
relationship: measured_in ECOSIMCONCEPT:Water ! Water
relationship: measurement_of ECOSIMCONCEPT:Hydrogen ! Hydrogen

[Term]
id: ECOSIM:HN2GG
name: soil N2 flux
is_a: ECOSIM:CATEGORYBiogeochemistry ! category - Biogeochemistry
is_a: ECOSIM:CATEGORYTraceGasFlux ! category - trace gas flux
relationship: attribute ECOSIMCONCEPT:Flux ! Flux
relationship: has_unit ECOSIM:gd-2h-1 ! g d-2 h-1
relationship: measured_in ECOSIMCONCEPT:Soil ! Soil
relationship: measurement_of ECOSIMCONCEPT:N2 ! Dinitrogen

[Term]
id: ECOSIM:HN2OG
name: soil N2O flux
is_a: ECOSIM:CATEGORYBiogeochemistry ! category - Biogeochemistry
is_a: ECOSIM:CATEGORYTraceGasFlux ! category - trace gas flux
relationship: attribute ECOSIMCONCEPT:Flux ! Flux
relationship: has_unit ECOSIM:gd-2h-1 ! g d-2 h-1
relationship: measured_in ECOSIMCONCEPT:Soil ! Soil
relationship: measurement_of ECOSIMCONCEPT:N2O ! Nitrous oxide

[Term]
id: ECOSIM:HNH3G
name: soil NH3 flux
is_a: ECOSIM:CATEGORYBiogeochemistry ! category - Biogeochemistry
is_a: ECOSIM:CATEGORYTraceGasFlux ! category - trace gas flux
relationship: attribute ECOSIMCONCEPT:Flux ! Flux
relationship: has_unit ECOSIM:gd-2h-1 ! g d-2 h-1
relationship: measured_in ECOSIMCONCEPT:Soil ! Soil
relationship: measurement_of ECOSIMCONCEPT:NH3 ! Ammonia

[Term]
id: ECOSIM:HOXYG
name: soil O2 flux
is_a: ECOSIM:CATEGORYBiogeochemistry ! category - Biogeochemistry
is_a: ECOSIM:CATEGORYTraceGasFlux ! category - trace gas flux
relationship: attribute ECOSIMCONCEPT:Flux ! Flux
relationship: has_unit ECOSIM:gd-2h-1 ! g d-2 h-1
relationship: measured_in ECOSIMCONCEPT:Soil ! Soil
relationship: measurement_of ECOSIMCONCEPT:O2 ! Dioxygen

[Term]
id: ECOSIM:HTC
name: temperature above which seed set is adversely affected
def: "HTC, or High Temperature Cutoff, is the temperature above which seed set is adversely affected. As temperature rises beyond this point, the process of seed set is disrupted, potentially leading to lower yield. This is an important parameter in agricultural and earth systems modeling, particularly in the context of climate change and global warming." []
is_a: ECOSIM:CATEGORYCanopyPhysiology ! category - Canopy Physiology
is_a: ECOSIM:CATEGORYCanopyStructure ! category - canopy structure
is_a: ECOSIM:CATEGORYPlantPhysiology ! category - plant physiology
relationship: has_unit ECOSIM:oC ! oC
relationship: measured_in ECOSIMCONCEPT:Temperature ! temperature
relationship: measurement_of ECOSIMCONCEPT:SeedSet ! SeedSet

[Term]
id: ECOSIM:HTNODE
name: internode height
def: "Height of the internode, which is the part of the plant stem between two nodes - the points where leaves attach" []
is_a: ECOSIM:CATEGORYCanopyStructure ! category - canopy structure
relationship: attribute ECOSIMCONCEPT:Height ! Height
relationship: has_unit ECOSIM:m ! m
relationship: measured_in ECOSIMCONCEPT:Internode ! Internode

[Term]
id: ECOSIM:HTNODX
name: internode height
is_a: ECOSIM:CATEGORYCanopyStructure ! category - canopy structure
relationship: attribute ECOSIMCONCEPT:Height ! Height
relationship: has_unit ECOSIM:m ! m
relationship: measured_in ECOSIMCONCEPT:Internode ! Internode

[Term]
id: ECOSIM:HUDN
name: daily minimum vapor pressure
is_a: ECOSIM:CATEGORYAtmosphericConditions ! category - Atmospheric Conditions
relationship: attribute ECOSIMCONCEPT:Pressure ! Pressure
relationship: has_unit ECOSIM:kPa ! kPa
relationship: measurement_of ECOSIMCONCEPT:Vapor ! Vapor

[Term]
id: ECOSIM:HUDX
name: daily maximum vapor pressure
is_a: ECOSIM:CATEGORYAtmosphericConditions ! category - Atmospheric Conditions
relationship: attribute ECOSIMCONCEPT:Pressure ! Pressure
relationship: has_unit ECOSIM:kPa ! kPa
relationship: measurement_of ECOSIMCONCEPT:Vapor ! Vapor

[Term]
id: ECOSIM:HVST
name: harvest cutting height (+ve) or fractional LAI removal (-ve)
def: "Harvest cutting height or fractional Leaf Area Index (LAI) removal refers to the parameter used in agricultural and ecosystem modelling to denote the height at which crops are cut during harvesting or the fraction of LAI that is removed. When positive, it represents the cutting height in harvesting, and when negative, it represents the fractional removal of LAI. This is used to estimate the biomass yield and the impact of the harvest on the remaining crop and soil nutrient balance." []
is_a: ECOSIMCONCEPT:UnclassifiedVariable ! unclassified variable
relationship: attribute ECOSIMCONCEPT:Height ! Height
relationship: has_unit ECOSIM:mor- ! m or -
relationship: measured_in ECOSIMCONCEPT:Harvest ! Harvest
relationship: measurement_of ECOSIMCONCEPT:LAI ! LAI

[Term]
id: ECOSIM:HVSTE
name: plant element harvest
def: "Plant element harvest refers to the process of gathering mature plant elements during a particular season. These plant elements can include grains, fruits, vegetables, or other plant parts that are typically used for food, fuel, medicinal plants, and other uses. It's an important parameter in agricultural practices and earth system modeling as it affects crop yield and sustainability." []
is_a: ECOSIMCONCEPT:UnclassifiedVariable ! unclassified variable
relationship: has_unit ECOSIM:gd-2 ! g d-2
relationship: measurement_of ECOSIMCONCEPT:PlantElement ! PlantElement

[Term]
id: ECOSIM:HYSGL
name: aqueous H diffusivity
def: "Aqueous H diffusivity refers to the measure of the rate at which hydrogen (H) ions migrate or spread through water or an aqueous medium. It represents the ability of H ions to move and mix within a water system. Aqueous H diffusivity is an important parameter in earth systems modeling as it plays a crucial role in understanding nutrient cycling, acid-base reactions, and the movement of pollutants in aquatic environments." []
is_a: ECOSIM:CATEGORYHydrology ! category - Hydrology
is_a: ECOSIMCONCEPT:UnclassifiedVariable ! unclassified variable
relationship: attribute ECOSIMCONCEPT:Diffusivity ! Diffusivity
relationship: has_unit ECOSIM:m2h-1 ! m2 h-1
relationship: measured_in ECOSIMCONCEPT:Water ! Water
relationship: measurement_of ECOSIMCONCEPT:Hydrogen ! Hydrogen
relationship: qualifier ECOSIMCONCEPT:Aqueous ! Aqueous

[Term]
id: ECOSIM:Heat2GridBySurfRunoff
name: soil surface runoff heat
is_a: ECOSIMCONCEPT:UnclassifiedVariable ! unclassified variable
relationship: has_unit ECOSIM:MJd-2h-1 ! MJ d-2 h-1

[Term]
id: ECOSIM:HeatByRadiation
name: total net radiation at ground surface
is_a: ECOSIM:CATEGORYSurfaceEnergyBalance ! category - Surface Energy Balance
relationship: has_unit ECOSIM:MJd-2t-1 ! MJ d-2 t-1

[Term]
id: ECOSIM:HeatBySnowRedistribution
name: snowpack runoff heat
is_a: ECOSIM:CATEGORYSnowpack ! category - Snowpack
relationship: has_unit ECOSIM:MJd-2h-1 ! MJ d-2 h-1

[Term]
id: ECOSIM:HeatEvapAir2Surf
name: total latent heat flux at ground surface
is_a: ECOSIM:CATEGORYSurfaceEnergyBalance ! category - Surface Energy Balance
relationship: has_unit ECOSIM:MJd-2t-1 ! MJ d-2 t-1

[Term]
id: ECOSIM:HeatFLo2LitrByWat
name: net heat transfer to surface litter
is_a: ECOSIMCONCEPT:UnclassifiedVariable ! unclassified variable
relationship: has_unit ECOSIM:MJd-2t-1 ! MJ d-2 t-1

[Term]
id: ECOSIM:HeatFlow2Soil
name: convective heat flux micropore
is_a: ECOSIMCONCEPT:UnclassifiedVariable ! unclassified variable
relationship: has_unit ECOSIM:MJd-2h-1 ! MJ d-2 h-1

[Term]
id: ECOSIM:HeatIrrigation
name: convective heat of underground irrigation
is_a: ECOSIMCONCEPT:UnclassifiedVariable ! unclassified variable
relationship: has_unit ECOSIM:MJd-2h-1 ! MJ d-2 h-1

[Term]
id: ECOSIM:HeatNet2Surf
name: total ground heat flux at ground surface
def: "Total ground heat flux at ground surface, often expressed in watts per square meter (W/m²), refers to the rate at which heat energy is transferred to the ground surface. It is an important component of the Earth's surface energy balance and can have significant impacts on climate, weather patterns, and physical processes in the Earth's surface and subsurface." []
is_a: ECOSIM:CATEGORYSurfaceEnergyBalance ! category - Surface Energy Balance
relationship: attribute ECOSIMCONCEPT:Flux ! Flux
relationship: context ECOSIMCONCEPT:GroundSurface ! Ground surface
relationship: has_unit ECOSIM:MJd-2t-1 ! MJ d-2 t-1
relationship: measured_in ECOSIMCONCEPT:GroundSurface ! Ground surface
relationship: measurement_of ECOSIMCONCEPT:Heat ! Heat

[Term]
id: ECOSIM:HeatSensAir2Surf
name: total sensible heat flux at ground surface
def: "Total sensible heat flux at ground surface refers to the total amount of energy, in Joules (J), transferred from the ground surface to the atmosphere as a result of differences in temperature. This process is one of the main ways energy is exchanged between the surface and the atmosphere, impacting climate and weather patterns." []
is_a: ECOSIM:CATEGORYSurfaceEnergyBalance ! category - Surface Energy Balance
relationship: has_unit ECOSIM:MJd-2t-1 ! MJ d-2 t-1
relationship: measured_in ECOSIMCONCEPT:GroundSurface ! Ground surface
relationship: measurement_of ECOSIMCONCEPT:Energy ! Energy

[Term]
id: ECOSIM:HeatSensVapAir2Surf
name: total convective heat flux at ground surface
def: "Total convective heat flux at ground surface refers to the total amount of heat transferred by convection from the air to the ground surface. This parameter is important in meteorology and climate science as it influences local air temperatures, weather patterns, and the overall energy balance of the Earth's surface. It is usually expressed in watts per square meter (W/m²)." []
is_a: ECOSIM:CATEGORYSurfaceEnergyBalance ! category - Surface Energy Balance
is_a: ECOSIMCONCEPT:GroundSurface ! Ground surface
relationship: attribute ECOSIMCONCEPT:Flux ! Flux
relationship: has_unit ECOSIM:MJd-2t-1 ! MJ d-2 t-1
relationship: measured_in ECOSIMCONCEPT:Air ! Air
relationship: measured_in ECOSIMCONCEPT:GroundSurface ! Ground surface
relationship: measurement_of ECOSIMCONCEPT:Heat ! Heat

[Term]
id: ECOSIM:HeatStorCanP
name: canopy storage heat flux
def: "Canopy storage heat flux, or 'heat stored in the canopy', refers to the amount of heat that is absorbed and stored in a vegetation canopy. This heat is later released back into the atmosphere, affecting the local microclimate. The heat flux contributes to the overall energy balance of an ecosystem, influencing processes like evapotranspiration and photosynthesis." []
is_a: ECOSIMCONCEPT:UnclassifiedVariable ! unclassified variable
relationship: has_unit ECOSIM:MJd-2h-1 ! MJ d-2 h-1
relationship: measured_in ECOSIMCONCEPT:Canopy ! Canopy

[Term]
id: ECOSIM:HeatXAir2PCan
name: air to canopy sensible heat flux
def: "Air to Canopy Sensible Heat Flux refers to the rate of heat transfer from the air to the vegetation canopy due to the difference in temperature between the two media. This process plays a significant role in the energy balance of landscapes and is a key parameter in Earth system modeling. Factors that can influence this flux include air and canopy temperature, wind speed, and canopy structure." []
is_a: ECOSIMCONCEPT:UnclassifiedVariable ! unclassified variable
relationship: has_unit ECOSIM:MJd-2h-1 ! MJ d-2 h-1
relationship: measured_in ECOSIMCONCEPT:Air ! Air
relationship: measured_in ECOSIMCONCEPT:Canopy ! Canopy

[Term]
id: ECOSIM:HourCounter4LeafOut_brch
name: counter for mobilizing nonstructural C during spring leafout/dehardening
def: "A parameter that represents the counter for mobilizing nonstructural carbon (C) during the process of spring leafout and dehardening in vegetation. Spring leafout refers to the sprouting and growth of new leaves in plants during the spring season, while dehardening refers to the process by which plants transition from a dormant, hardened state to an active, growing state. The mobilization of nonstructural carbon refers to the utilization and movement of stored carbon reserves within the vegetation for the purpose of new growth and development during this period. This parameter tracks the accumulation and release of nonstructural carbon during leafout and dehardening, providing information on the timing and intensity of this process in Earth system models." []
is_a: ECOSIM:CATEGORYCanopyStructure ! category - canopy structure
relationship: has_unit ECOSIM:h ! h

[Term]
id: ECOSIM:HydroCondMacP
name: macropore hydraulic conductivity
def: "Macropore hydraulic conductivity (HydroCondMacP) refers to the ability of the soil's macropores (pores that are greater than 0.08mm in diameter) to transmit water under the influence of a hydraulic gradient. It plays a crucial role in determining the rate and direction of water movement in the soil, and thus impacts soil water availability and nutrient mobility." []
is_a: ECOSIM:CATEGORYHydrology ! category - Hydrology
relationship: context ECOSIMCONCEPT:Soil ! Soil
relationship: has_unit ECOSIM:mMPa-1h-1 ! m MPa-1 h-1
relationship: measured_in ECOSIMCONCEPT:Macropore ! Macropore

[Term]
id: ECOSIM:HypoctoylHeight
name: cotyledon height
is_a: ECOSIM:CATEGORYCanopyStructure ! category - canopy structure
relationship: attribute ECOSIMCONCEPT:Height ! Height
relationship: has_unit ECOSIM:m ! m
relationship: measured_in ECOSIMCONCEPT:Plant ! Plant
relationship: measurement_of ECOSIMCONCEPT:Cotyledon ! Cotyledon

[Term]
id: ECOSIM:IceBySnowRedistribution
name: snowpack runoff ice
def: "Snowpack runoff ice refers to the portion of a snowpack that has melted, flowed over the snow surface, and then re-frozen into ice. In colder climate regions, this can be a significant component of spring flood volumes, as ice can block channels and store water on the landscape, which then melts at a later time contributing to flood flow. Understanding and measuring this phenomenon is important for forecasting and managing flood risks in these regions." []
is_a: ECOSIM:CATEGORYSnowpack ! category - Snowpack
is_a: ECOSIMCONCEPT:Snowpack ! Snowpack
relationship: attribute ECOSIMCONCEPT:Ice ! Ice
relationship: has_unit ECOSIM:m3d-2h-1 ! m3 d-2 h-1

[Term]
id: ECOSIM:IrrigSubsurf
name: underground irrigation
def: "Underground irrigation, also known as subsurface irrigation, refers to a method of irrigation where water is applied directly to the root zone of plants, bypassing the surface of the soil. This can be achieved by the use of drip lines or pipes that deliver water to the roots of plants. Underground irrigation is highly efficient as it reduces evaporation losses and runoff, thereby conserving water. It can also minimize the spread of some plant diseases that are waterborne." []
is_a: ECOSIMCONCEPT:UnclassifiedVariable ! unclassified variable
is_a: ECOSIMCONCEPT:Variable ! variable
relationship: context ECOSIMCONCEPT:Irrigation ! Irrigation
relationship: has_unit ECOSIM:m3d-2h-1 ! m3 d-2 h-1

[Term]
id: ECOSIM:IrrigSurface
name: surface irrigation
is_a: ECOSIMCONCEPT:UnclassifiedVariable ! unclassified variable
relationship: has_unit ECOSIM:m3d-2h-1 ! m3 d-2 h-1

[Term]
id: ECOSIM:K
name: K
def: "K refers to the chemical symbol for potassium. As one of the most abundant elements in the Earth's crust, potassium is essential for plant growth and is one of the three primary nutrients, along with nitrogen (N) and phosphorus (P). In ecosystems, the dynamics of potassium can affect soil fertility, plant health, and overall ecosystem productivity." []
is_a: ECOSIMCONCEPT:Element ! Element
is_a: ECOSIMCONCEPT:Unit ! unit

[Term]
id: ECOSIM:KASR
name: KASR
def: "The definition of KASR is not provided." []
is_a: ECOSIM:CATEGORYAtmosphericConditions ! category - Atmospheric Conditions

[Term]
id: ECOSIM:LWRadBySurf
name: longwave radiation emitted from ground surface
is_a: ECOSIMCONCEPT:UnclassifiedVariable ! unclassified variable
relationship: has_unit ECOSIM:MJd-2t-1 ! MJ d-2 t-1

[Term]
id: ECOSIM:LWRadCanG
name: total canopy LW emission
is_a: ECOSIM:CATEGORYSurfaceEnergyBalance ! category - Surface Energy Balance
relationship: attribute ECOSIMCONCEPT:Emission ! Emission
relationship: has_unit ECOSIM:MJd-2h-1 ! MJ d-2 h-1
relationship: measured_in ECOSIMCONCEPT:Canopy ! Canopy
relationship: measurement_of ECOSIMCONCEPT:LWRad ! LWRad

[Term]
id: ECOSIM:LWRadCanGPrev
name: longwave radiation emitted by canopy
def: "Longwave radiation emitted by the canopy, also known as thermal infrared radiation, is a type of electromagnetic radiation, which is emitted by the canopy layer of trees or other types of vegetation when they absorb and then re-emit part of the solar radiation they receive. This plays a critical role in the energy balance of the earth's surface and is essential in climate modelling and the study of global warming." []
is_a: ECOSIM:CATEGORYSurfaceEnergyBalance ! category - Surface Energy Balance
relationship: attribute ECOSIMCONCEPT:Emission ! Emission
relationship: has_unit ECOSIM:MJm-2h-1 ! MJ m-2 h-1
relationship: measured_in ECOSIMCONCEPT:Canopy ! Canopy
relationship: measurement_of ECOSIMCONCEPT:LongwaveRadiation ! LongwaveRadiation

[Term]
id: ECOSIM:LWRadCanP
name: canopy longwave radiation
def: "Canopy longwave radiation refers to the longwave radiation that is either absorbed, emitted or transmitted by the canopy." []
is_a: ECOSIM:CATEGORYSurfaceEnergyBalance ! category - Surface Energy Balance
relationship: has_unit ECOSIM:MJd-2h-1 ! MJ d-2 h-1
relationship: measured_in ECOSIMCONCEPT:Canopy ! Canopy
relationship: measurement_of ECOSIMCONCEPT:LongwaveRadiation ! LongwaveRadiation

[Term]
id: ECOSIM:LWRadGrnd
name: longwave radiation emitted by ground surface
is_a: ECOSIM:CATEGORYSurfaceEnergyBalance ! category - Surface Energy Balance
relationship: has_unit ECOSIM:MJm-2h-1 ! MJ m-2 h-1

[Term]
id: ECOSIM:LWRadSky
name: sky longwave radiation
def: "Sky longwave radiation refers to the part of the electromagnetic spectrum that is radiated from the sky in the form of thermal radiation, or heat. This is a key component of the earth's energy balance, affecting both climatic and biological processes." []
is_a: ECOSIM:CATEGORYAtmosphericConditions ! category - Atmospheric Conditions
relationship: attribute ECOSIMCONCEPT:Radiation ! Radiation
relationship: has_unit ECOSIM:MJd-2h-1 ! MJ d-2 h-1

[Term]
id: ECOSIM:LeafAUnshaded_seclyrnodbrpft
name: leaf irradiated surface area
def: "The leaf irradiated surface area is a parameter that refers to the surface area of a leaf that is exposed to direct sunlight. It quantifies the amount of leaf surface that receives solar radiation and is an important parameter for modeling the energy balance and photosynthetic processes of vegetation in Earth system models." []
is_a: ECOSIMCONCEPT:UnclassifiedVariable ! unclassified variable
relationship: has_unit ECOSIM:m2d-2 ! m2 d-2

[Term]
id: ECOSIM:LeafA_lyrnodbrchpft
name: leaf surface area
def: "Leaf surface area refers to the total area of all the leaves in a plant or vegetation community. It is a key parameter in ecosystem modeling as it influences the exchange of gases (such as carbon dioxide and oxygen) and water vapor between the leaves and the atmosphere. Leaf surface area is typically measured in square meters and can vary depending on factors such as leaf size, shape, and density. It is an important parameter for estimating photosynthesis, transpiration, and other physiological processes in plants." []
is_a: ECOSIMCONCEPT:UnclassifiedVariable ! unclassified variable
relationship: has_unit ECOSIM:m2d-2 ! m2 d-2

[Term]
id: ECOSIM:LitrfalChemElemnts_vr
name: total litterfall C
def: "Total litterfall C refers to the amount of carbon that is shed from vegetation and accumulated on the forest floor as litter. It includes both aboveground and belowground litter, such as leaves, branches, and roots, that have fallen or been shed by plants. Total litterfall C is an important parameter in earth systems modeling as it represents a major pathway for carbon cycling in forests, impacting ecosystem productivity, nutrient cycling, and carbon sequestration." []
is_a: ECOSIMCONCEPT:UnclassifiedVariable ! unclassified variable
relationship: has_unit ECOSIM:gd-2h-1 ! g d-2 h-1

[Term]
id: ECOSIM:MGHR
name: MGHR
def: "This is the class representing MGHR. Details about this class are currently not available." []
is_a: ECOSIM:CATEGORYAtmosphericConditions ! category - Atmospheric Conditions

[Term]
id: ECOSIM:MGSR
name: MGSR
def: "MGSR refers to the abbreviation of Magnesium Sulphate Reaction. This is a soil test used to predict the lime requirement of acid soils. It's a measure of soil acidity or alkalinity status and an essential determinant of soil's suitability for plant growth." []
is_a: ECOSIM:CATEGORYAtmosphericConditions ! category - Atmospheric Conditions
relationship: measured_in ECOSIMCONCEPT:Soil ! Soil

[Term]
id: ECOSIM:MJd-1
name: MJ d-1
is_a: ECOSIMCONCEPT:Unit ! unit

[Term]
id: ECOSIM:MJd-2
name: MJ d-2
is_a: ECOSIMCONCEPT:Unit ! unit

[Term]
id: ECOSIM:MJd-2K-1
name: MJ d-2 K-1
is_a: ECOSIMCONCEPT:Unit ! unit

[Term]
id: ECOSIM:MJd-2h-1
name: MJ d-2 h-1
is_a: ECOSIMCONCEPT:Unit ! unit

[Term]
id: ECOSIM:MJd-2t-1
name: MJ d-2 t-1
is_a: ECOSIMCONCEPT:Unit ! unit

[Term]
id: ECOSIM:MJm-1
name: MJ m-1
is_a: ECOSIMCONCEPT:Unit ! unit

[Term]
id: ECOSIM:MJm-2h-1
name: MJ m-2 h-1
is_a: ECOSIMCONCEPT:Unit ! unit

[Term]
id: ECOSIM:MJm-3K-1
name: MJ m-3 K-1
is_a: ECOSIMCONCEPT:Unit ! unit

[Term]
id: ECOSIM:MPa
name: MPa
is_a: ECOSIMCONCEPT:Unit ! unit

[Term]
id: ECOSIM:MPahm-2
name: MPa h m-2
is_a: ECOSIMCONCEPT:Unit ! unit

[Term]
id: ECOSIM:MPahm-4
name: MPa h m-4
is_a: ECOSIMCONCEPT:Unit ! unit

[Term]
id: ECOSIM:MaxCanPStomaResistH2O
name: maximum stomatal resistance to vapor
is_a: ECOSIM:CATEGORYPlantPhysiology ! category - plant physiology
relationship: has_unit ECOSIM:sh-1 ! s h-1
relationship: measured_in ECOSIMCONCEPT:Canopy ! Canopy
relationship: measurement_of ECOSIMCONCEPT:Stoma ! Stoma
relationship: qualifier ECOSIMCONCEPT:Vapor ! Vapor

[Term]
id: ECOSIM:MaxPrimRootRadius
name: maximum radius of primary roots
is_a: ECOSIM:CATEGORYRootPhysiology ! category - root physiology
relationship: has_unit ECOSIM:m ! m

[Term]
id: ECOSIM:MaxPrimRootRadius1
name: root diameter primary axes
is_a: ECOSIM:CATEGORYRootPhysiology ! category - root physiology
relationship: has_unit ECOSIM:m ! m

[Term]
id: ECOSIM:MaxSecndRootRadius
name: maximum radius of secondary roots
is_a: ECOSIM:CATEGORYRootPhysiology ! category - root physiology
relationship: has_unit ECOSIM:m ! m

[Term]
id: ECOSIM:MaxSecndRootRadius1
name: root diameter secondary axes
def: "Root diameter refers to the thickness of the root and root diameter secondary axes refers to the thickness of the secondary (or lateral) roots. Different species of plants have different types of roots systems and different root thicknesses. This thickness can play a significant role in the plant's ability to take up water and nutrients from the soil." []
is_a: ECOSIM:CATEGORYRootPhysiology ! category - root physiology
relationship: context ECOSIMCONCEPT:SecondaryAxes ! SecondaryAxes
relationship: has_unit ECOSIM:m ! m
relationship: measured_in ECOSIMCONCEPT:Root ! Root

[Term]
id: ECOSIM:MaxSeedCMass
name: maximum grain size
is_a: ECOSIM:CATEGORYCanopyStructure ! category - canopy structure
relationship: has_unit ECOSIM:g ! g

[Term]
id: ECOSIM:Mgd-2
name: Mg d-2
is_a: ECOSIMCONCEPT:Unit ! unit

[Term]
id: ECOSIM:Mgd-2h-1
name: Mg d-2 h-1
is_a: ECOSIMCONCEPT:Unit ! unit

[Term]
id: ECOSIM:Mgm-3
name: Mg m-3
is_a: ECOSIMCONCEPT:Unit ! unit

[Term]
id: ECOSIM:MinCanPStomaResistH2O
name: canopy minimum stomatal resistance
is_a: ECOSIM:CATEGORYPlantPhysiology ! category - plant physiology
relationship: has_unit ECOSIM:sm-1 ! s m-1
relationship: measured_in ECOSIMCONCEPT:Canopy ! Canopy
relationship: measurement_of ECOSIMCONCEPT:Stoma ! Stoma

[Term]
id: ECOSIM:Mpa
name: Mpa
is_a: ECOSIMCONCEPT:Unit ! unit

[Term]
id: ECOSIM:NACR
name: NACR
def: "NACR refers to a specific conceptual entity or class within an ontology system. The exact definition and characteristics of this class could vary depending on the context and the specific ontology being used." []
is_a: ECOSIM:CATEGORYAtmosphericConditions ! category - Atmospheric Conditions

[Term]
id: ECOSIM:NASR
name: NASR
def: "NASR (Net Aboveground Stand Respiration) represents the total respiration of all aboveground portion of trees in a forest stand. It is a key parameter in forest ecosystem modelling, specifically in carbon cycling and budgeting." []
is_a: ECOSIM:CATEGORYAtmosphericConditions ! category - Atmospheric Conditions

[Term]
id: ECOSIM:NewSnowDens
name: new snowpack density
is_a: ECOSIM:CATEGORYSnowpack ! category - Snowpack
relationship: has_unit ECOSIM:Mgm-3 ! Mg m-3

[Term]
id: ECOSIM:NoduleNonstructCconc_pft
name: nodule nonstructural C
def: "Nodule nonstructural C (carbon) refers to the concentration or amount of carbon that is stored in the nodules of a plant without being in a structural form. Nodules are specialized structures found in certain plant species, particularly legumes, that house symbiotic bacteria capable of fixing atmospheric nitrogen. The nonstructural carbon stored in these nodules can be used by the plant for various metabolic processes and for supporting nitrogen fixation. The concentration of nodule nonstructural C can be an important parameter in earth systems models as it can influence plant growth, nitrogen fixation rates, and carbon cycling in terrestrial ecosystems." []
is_a: ECOSIMCONCEPT:UnclassifiedVariable ! unclassified variable
relationship: has_unit ECOSIM:gd-2 ! g d-2

[Term]
id: ECOSIM:O2I
name: leaf gaseous O2 concentration
is_a: ECOSIM:CATEGORYCanopyPhysiology ! category - Canopy Physiology
is_a: ECOSIM:CATEGORYPlantPhysiology ! category - plant physiology
relationship: attribute ECOSIMCONCEPT:Concentration ! Concentration
relationship: has_unit ECOSIM:umolm-3 ! umol m-3
relationship: measured_in ECOSIMCONCEPT:Leaf ! Leaf
relationship: measurement_of ECOSIMCONCEPT:O2 ! Dioxygen

[Term]
id: ECOSIM:O2L
name: leaf aqueous O2 concentration
is_a: ECOSIM:CATEGORYCanopyPhysiology ! category - Canopy Physiology
is_a: ECOSIM:CATEGORYPlantPhysiology ! category - plant physiology
relationship: attribute ECOSIMCONCEPT:Concentration ! Concentration
relationship: has_unit ECOSIM:uM ! uM
relationship: measured_in ECOSIMCONCEPT:Leaf ! Leaf
relationship: measurement_of ECOSIMCONCEPT:O2 ! Dioxygen
relationship: qualifier ECOSIMCONCEPT:Aqueous ! Aqueous

[Term]
id: ECOSIM:OASGL
name: aqueous acetate diffusivity
is_a: ECOSIMCONCEPT:UnclassifiedVariable ! unclassified variable
relationship: has_unit ECOSIM:m2h-1 ! m2 h-1

[Term]
id: ECOSIM:OCSGL
name: aqueous DOC diffusivity
is_a: ECOSIMCONCEPT:UnclassifiedVariable ! unclassified variable
relationship: has_unit ECOSIM:m2h-1 ! m2 h-1

[Term]
id: ECOSIM:OFFSET
name: offset for calculating temperature in Arrhenius curves
def: "Offset for calculating temperature in Arrhenius curves refers to a constant adjustment applied when calculating the temperature in Arrhenius equations. It is used to shift the calculated temperature value by a certain amount to achieve better fit or representation in earth systems modeling." []
is_a: ECOSIM:CATEGORYAtmosphericConditions ! category - Atmospheric Conditions
relationship: has_unit ECOSIM:oC ! oC
relationship: measurement_of ECOSIMCONCEPT:Temperature ! temperature

[Term]
id: ECOSIM:OFFST
name: adjustment of Arhhenius curves for plant thermal acclimation
def: "OFFST refers to the adjustment of Arrhenius curves for plant thermal acclimation. It's a factor applied to adjust the response of physiological processes to temperature changes in the context of plant thermal acclimation. It's an important parameter in vegetation and Earth system modeling." []
is_a: ECOSIM:CATEGORYCanopyStructure ! category - canopy structure
is_a: ECOSIM:CATEGORYPlantPhysiology ! category - plant physiology
is_a: ECOSIM:CATEGORYPlantPopulation ! category - Plant Population
relationship: has_unit ECOSIM:oC ! oC

[Term]
id: ECOSIM:OHAER
name: adsorbed acetate erosion
is_a: ECOSIMCONCEPT:UnclassifiedVariable ! unclassified variable
relationship: has_unit ECOSIM:gd-2h-1 ! g d-2 h-1

[Term]
id: ECOSIM:OHCER
name: adsorbed C erosion
is_a: ECOSIMCONCEPT:UnclassifiedVariable ! unclassified variable
relationship: has_unit ECOSIM:gd-2h-1 ! g d-2 h-1

[Term]
id: ECOSIM:OHNER
name: adsorbed N erosion
is_a: ECOSIMCONCEPT:UnclassifiedVariable ! unclassified variable
relationship: has_unit ECOSIM:gd-2h-1 ! g d-2 h-1

[Term]
id: ECOSIM:OHPER
name: adsorbed P erosion
is_a: ECOSIMCONCEPT:UnclassifiedVariable ! unclassified variable
relationship: has_unit ECOSIM:gd-2h-1 ! g d-2 h-1

[Term]
id: ECOSIM:OHSGL
name: aqueous OH diffusivity
is_a: ECOSIMCONCEPT:UnclassifiedVariable ! unclassified variable
relationship: has_unit ECOSIM:m2h-1 ! m2 h-1

[Term]
id: ECOSIM:OMEGAG
name: sine of solar beam on leaf surface
is_a: ECOSIMCONCEPT:UnclassifiedVariable ! unclassified variable

[Term]
id: ECOSIM:ONSGL
name: aqueous DON diffusivity
is_a: ECOSIMCONCEPT:UnclassifiedVariable ! unclassified variable
relationship: has_unit ECOSIM:m2h-1 ! m2 h-1

[Term]
id: ECOSIM:OPSGL
name: aqueous DOP diffusivity
is_a: ECOSIMCONCEPT:UnclassifiedVariable ! unclassified variable
relationship: has_unit ECOSIM:m2h-1 ! m2 h-1

[Term]
id: ECOSIM:ORCER
name: microbial residue C erosion
is_a: ECOSIMCONCEPT:UnclassifiedVariable ! unclassified variable
relationship: has_unit ECOSIM:gd-2h-1 ! g d-2 h-1

[Term]
id: ECOSIM:ORNER
name: microbial residue N erosion
is_a: ECOSIMCONCEPT:UnclassifiedVariable ! unclassified variable
relationship: has_unit ECOSIM:gd-2h-1 ! g d-2 h-1

[Term]
id: ECOSIM:ORPER
name: microbial residue P erosion
is_a: ECOSIMCONCEPT:UnclassifiedVariable ! unclassified variable
relationship: has_unit ECOSIM:gd-2h-1 ! g d-2 h-1

[Term]
id: ECOSIM:OSAER
name: colonized humus C erosion
is_a: ECOSIMCONCEPT:UnclassifiedVariable ! unclassified variable
relationship: has_unit ECOSIM:gd-2h-1 ! g d-2 h-1

[Term]
id: ECOSIM:OSCER
name: humus C erosion
is_a: ECOSIMCONCEPT:UnclassifiedVariable ! unclassified variable
relationship: has_unit ECOSIM:gd-2h-1 ! g d-2 h-1

[Term]
id: ECOSIM:OSMO
name: canopy osmotic potential when canopy water potential = 0 MPa
def: "Canopy osmotic potential when canopy water potential = 0 MPa refers to the osmotic potential of the canopy at which the canopy water potential equals zero. Osmotic potential is the potential of water molecules to move from a hypotonic solution (low solute concentration) to a hypertonic solution (high solute concentration) across a semipermeable membrane. In Earth system modeling, canopy osmotic potential is an important parameter representing the water status of plants and can affect their growth and survival." []
is_a: ECOSIM:CATEGORYCanopyStructure ! category - canopy structure
is_a: ECOSIM:CATEGORYPlantPhysiology ! category - plant physiology
relationship: has_unit ECOSIM:MPa ! MPa
relationship: measured_in ECOSIMCONCEPT:Canopy ! Canopy

[Term]
id: ECOSIM:OSNER
name: humus N erosion
is_a: ECOSIMCONCEPT:UnclassifiedVariable ! unclassified variable
relationship: has_unit ECOSIM:gd-2h-1 ! g d-2 h-1

[Term]
id: ECOSIM:OSPER
name: humus P erosion
is_a: ECOSIMCONCEPT:UnclassifiedVariable ! unclassified variable
relationship: has_unit ECOSIM:gd-2h-1 ! g d-2 h-1

[Term]
id: ECOSIM:OXYE
name: atmospheric O2 concentration
is_a: ECOSIMCONCEPT:UnclassifiedVariable ! unclassified variable
relationship: has_unit ECOSIM:umolmol-1 ! umol mol-1

[Term]
id: ECOSIM:PAR
name: direct incoming PAR
is_a: ECOSIMCONCEPT:UnclassifiedVariable ! unclassified variable
relationship: has_unit ECOSIM:umolm-2s-1 ! umol m-2 s-1

[Term]
id: ECOSIM:PARByCanP
name: canopy absorbed PAR
is_a: ECOSIM:CATEGORYSurfaceEnergyBalance ! category - Surface Energy Balance
relationship: has_unit ECOSIM:umolm-2s-1 ! umol m-2 s-1

[Term]
id: ECOSIM:PARDIF
name: diffuse incoming PAR
is_a: ECOSIMCONCEPT:UnclassifiedVariable ! unclassified variable
relationship: has_unit ECOSIM:umolm-2s-1 ! umol m-2 s-1

[Term]
id: ECOSIM:PARG
name: soil surface boundary layer conductance
def: "Soil surface boundary layer conductance refers to the ease with which moisture is transported from the soil surface to the atmosphere. It is an important parameter in hydrological and climate models as it can help in understanding and simulating evaporation processes, soil moisture dynamics, and heat transfer in the soil. Its value can be influenced by factors such as soil texture, moisture content, and air movement." []
is_a: ECOSIM:CATEGORYSurfaceEnergyBalance ! category - Surface Energy Balance
relationship: has_unit ECOSIM:mt-1 ! m t-1
relationship: measured_in ECOSIMCONCEPT:SoilSurface ! Soil surface
relationship: measurement_of ECOSIMCONCEPT:BoundaryLayer ! BoundaryLayer

[Term]
id: ECOSIM:PARR
name: surface litter boundary layer conductance
def: "Surface litter boundary layer conductance refers to the rate of energy or mass transfer from the litter layer on the surface of the soil to the atmosphere. This is largely dependent on factors such as litter type, structure, and moisture content, along with atmospheric conditions such as wind speed, temperature, and humidity." []
is_a: ECOSIM:CATEGORYHydrology ! category - Hydrology
relationship: context ECOSIMCONCEPT:BoundaryLayer ! BoundaryLayer
relationship: has_unit ECOSIM:mt-1 ! m t-1
relationship: measured_in ECOSIMCONCEPT:GroundSurface ! Ground surface

[Term]
id: ECOSIM:PB
name: branch nonstructural C content required for new branch
def: "The nonstructural carbon content required for a new branch in a plant. This refers to the carbon that is not part of the plant's physical structure, such as sugars and other compounds that can be used for energy." []
is_a: ECOSIM:CATEGORYCanopyStructure ! category - canopy structure
is_a: ECOSIM:CATEGORYPlantPhysiology ! category - plant physiology
relationship: attribute ECOSIMCONCEPT:Content ! Content
relationship: has_unit ECOSIM:gg-1 ! g g-1
relationship: qualifier ECOSIMCONCEPT:Branch ! Branch

[Term]
id: ECOSIM:PDRAIN
name: total P drainage below root zone
is_a: ECOSIM:CATEGORYTraceGasFlux ! category - trace gas flux
relationship: has_unit ECOSIM:gd-2 ! g d-2

[Term]
id: ECOSIM:PEPC
name: leaf PEP carboxylase content
def: "Leaf PEP carboxylase content refers to the amount of phosphoenolpyruvate (PEP) carboxylase, an enzyme widely distributed in plants and bacteria involved in many biochemical pathways including carbon fixation and amino acid metabolism, present in the leaf. This measure is key in the modelling of plant photosynthesis and primary productivity, and influences the responses of plant growth to environmental factors such as light, temperature, and CO2 concentrations." []
is_a: ECOSIM:CATEGORYCanopyPhysiology ! category - Canopy Physiology
is_a: ECOSIM:CATEGORYPlantPhysiology ! category - plant physiology
relationship: attribute ECOSIMCONCEPT:Content ! Content
relationship: has_unit ECOSIM:gg-1 ! g g-1
relationship: measured_in ECOSIMCONCEPT:Leaf ! Leaf
relationship: measurement_of ECOSIMCONCEPT:PEPCarboxylase ! Phosphoenolpyruvate carboxylase

[Term]
id: ECOSIM:PHQ
name: surface irrigation pH
is_a: ECOSIMCONCEPT:UnclassifiedVariable ! unclassified variable

[Term]
id: ECOSIM:PHR
name: precipitation pH
def: "Precipitation pH refers to the acidity or alkalinity of a precipitation event such as raing or snowfall. This measure is important in understanding the environmental impact of atmospheric pollution, as it can indicate the presence of acid rain. Acid rain is primarily caused by emissions of sulfur dioxide and nitrogen oxide, which react with the water molecules in the atmosphere to produce acids." []
is_a: ECOSIM:CATEGORYAtmosphericConditions ! category - Atmospheric Conditions
relationship: measured_in ECOSIMCONCEPT:Precipitation ! Precipitation

[Term]
id: ECOSIM:POSGL
name: aqueous PO4 diffusivity
is_a: ECOSIMCONCEPT:UnclassifiedVariable ! unclassified variable
relationship: has_unit ECOSIM:m2h-1 ! m2 h-1

[Term]
id: ECOSIM:PPI
name: initial plant population
def: "Initial plant population refers to the original number of plants present in a specific area or plot at the start of a growing season. This statistic is often used in agricultural contexts to track the growth and progress of a crop over time." []
is_a: ECOSIM:CATEGORYCanopyStructure ! category - canopy structure
is_a: ECOSIM:CATEGORYPlantPopulation ! category - Plant Population
relationship: has_unit ECOSIM:m-2 ! m-2

[Term]
id: ECOSIM:PPT
name: total plant population
def: "The total plant population refers to the total number of plants inhabiting a specific area. This measure is useful in ecological studies for understanding the distribution and density of plant life, as well as for modeling plant life cycles and assessing the health of an ecosystem." []
is_a: ECOSIM:CATEGORYCanopyStructure ! category - canopy structure
is_a: ECOSIM:CATEGORYPlantPopulation ! category - Plant Population
relationship: has_unit ECOSIM:d-2 ! d-2

[Term]
id: ECOSIM:PPX
name: plant population
def: "Refers to the total number of individual plants in a particular area or population." []
is_a: ECOSIM:CATEGORYCanopyStructure ! category - canopy structure
is_a: ECOSIM:CATEGORYPlantPopulation ! category - Plant Population
relationship: has_unit ECOSIM:m-2 ! m-2

[Term]
id: ECOSIM:PPZ
name: plant population at seeding
def: "Plant population at seeding, also known as PPZ, refers to the total number of seeds of a specific plant species that are sown or planted in a particular area. It is an important parameter in agricultural and earth systems modeling, influencing the modeling of plant growth, biomass production, and yield estimates." []
is_a: ECOSIM:CATEGORYCanopyStructure ! category - canopy structure
is_a: ECOSIM:CATEGORYPlantPopulation ! category - Plant Population
relationship: context ECOSIMCONCEPT:Seed ! Seed
relationship: has_unit ECOSIM:m-2 ! m-2
relationship: measurement_of ECOSIMCONCEPT:Plant ! Plant

[Term]
id: ECOSIM:PR
name: threshold root nonstructural C content for initiating new root axis
def: "Threshold root nonstructural C content for initiating new root axis is a plant physiological parameter that indicates the minimum concentration of nonstructural carbon (C) in a plant's root that is required for the initiation of a new root axis. It plays a critical role in plant root development and further plant growth." []
is_a: ECOSIM:CATEGORYRootPhysiology ! category - root physiology
relationship: has_unit ECOSIM:gg-1 ! g g-1
relationship: measured_in ECOSIMCONCEPT:Plant ! Plant
relationship: measurement_of ECOSIMCONCEPT:Carbon ! Carbon
relationship: measurement_of ECOSIMCONCEPT:Root ! Root

[Term]
id: ECOSIM:PRECB
name: precipitation at ground surface used to calculate soil erosion
is_a: ECOSIMCONCEPT:UnclassifiedVariable ! unclassified variable
relationship: has_unit ECOSIM:mh-1 ! m h-1

[Term]
id: ECOSIM:PRECD
name: precipitation at ground surface used to calculate soil erosion
is_a: ECOSIMCONCEPT:UnclassifiedVariable ! unclassified variable
relationship: has_unit ECOSIM:mh-1 ! m h-1

[Term]
id: ECOSIM:PSIAtFldCapacity
name: water potentials at field capacity
is_a: ECOSIMCONCEPT:UnclassifiedVariable ! unclassified variable
relationship: has_unit ECOSIM:MPa ! MPa

[Term]
id: ECOSIM:PSICanP
name: plant canopy total water potential
is_a: ECOSIMCONCEPT:UnclassifiedVariable ! unclassified variable
relationship: has_unit ECOSIM:Mpa ! Mpa

[Term]
id: ECOSIM:PSICanPDailyMin
name: minimum daily canopy water potential
is_a: ECOSIM:CATEGORYCanopyStructure ! category - canopy structure
is_a: ECOSIM:CATEGORYPlantPhysiology ! category - plant physiology
relationship: has_unit ECOSIM:MPa ! MPa
relationship: measured_in ECOSIMCONCEPT:Canopy ! Canopy
relationship: measurement_of ECOSIMCONCEPT:Water ! Water

[Term]
id: ECOSIM:PSICanPOsmo
name: platn canopy osmotic water potential
is_a: ECOSIMCONCEPT:UnclassifiedVariable ! unclassified variable
relationship: has_unit ECOSIM:Mpa ! Mpa

[Term]
id: ECOSIM:PSICanPTurg
name: plant canopy turgor water potential
is_a: ECOSIMCONCEPT:UnclassifiedVariable ! unclassified variable
relationship: has_unit ECOSIM:Mpa ! Mpa

[Term]
id: ECOSIM:PSIGrav
name: gravimetric soil water potential
is_a: ECOSIMCONCEPT:UnclassifiedVariable ! unclassified variable
relationship: has_unit ECOSIM:Mpa ! Mpa

[Term]
id: ECOSIM:PSIRoot
name: root total water potential
is_a: ECOSIMCONCEPT:UnclassifiedVariable ! unclassified variable
relationship: has_unit ECOSIM:Mpa ! Mpa

[Term]
id: ECOSIM:PSIRootOSMO
name: root osmotic water potential
is_a: ECOSIMCONCEPT:UnclassifiedVariable ! unclassified variable
relationship: has_unit ECOSIM:Mpa ! Mpa

[Term]
id: ECOSIM:PSIRootTurg
name: root turgor water potential
is_a: ECOSIMCONCEPT:UnclassifiedVariable ! unclassified variable
relationship: has_unit ECOSIM:Mpa ! Mpa

[Term]
id: ECOSIM:PSISE
name: soil water potential at saturation
is_a: ECOSIMCONCEPT:UnclassifiedVariable ! unclassified variable
relationship: has_unit ECOSIM:Mpa ! Mpa

[Term]
id: ECOSIM:PSISoilAirEntry
name: soil water potential at air entry
is_a: ECOSIMCONCEPT:UnclassifiedVariable ! unclassified variable
relationship: has_unit ECOSIM:Mpa ! Mpa

[Term]
id: ECOSIM:PSISoilOsmotic
name: osmotic soil water potential
is_a: ECOSIMCONCEPT:UnclassifiedVariable ! unclassified variable
relationship: has_unit ECOSIM:Mpa ! Mpa

[Term]
id: ECOSIM:PSTG
name: node number
def: "Node number refers to the count of nodes or joints in a plant stem or branch. This parameter is essential in plant phenotypic characterization and developmental studies." []
is_a: ECOSIM:CATEGORYCanopyStructure ! category - canopy structure
is_a: ECOSIM:CATEGORYPlantPhysiology ! category - plant physiology
relationship: measured_in ECOSIMCONCEPT:Plant ! Plant
relationship: measurement_of ECOSIMCONCEPT:Node ! Node

[Term]
id: ECOSIM:PSTGF
name: node number at anthesis
def: "Node number at anthesis refers to the number of nodes on the plant at the time of anthesis, i.e., when the flower is fully open and functional. This is an important measure in agriculture and botany as it can provide information about the plant's growth and development, and it can be influenced by various factors such as genetics, environmental conditions, and agricultural practices." []
is_a: ECOSIM:CATEGORYCanopyStructure ! category - canopy structure
is_a: ECOSIM:CATEGORYPlantPhysiology ! category - plant physiology
relationship: measured_in ECOSIMCONCEPT:Plant ! Plant
relationship: measurement_of ECOSIMCONCEPT:Node ! Node

[Term]
id: ECOSIM:PSTGI
name: node number at floral initiation
def: "Node number at floral initiation represents the number of nodes on the plant stem at the time when the plant begins to produce flowers. This parameter is important for plant growth modeling and agronomy, as it is a significant determinant of the plant's reproductive capacity." []
is_a: ECOSIM:CATEGORYCanopyStructure ! category - canopy structure
is_a: ECOSIM:CATEGORYPlantPhysiology ! category - plant physiology
relationship: attribute ECOSIMCONCEPT:Number ! Number
relationship: measured_in ECOSIMCONCEPT:Plant ! Plant
relationship: measurement_of ECOSIMCONCEPT:Node ! Node

[Term]
id: ECOSIM:PTSHT
name: shoot-root rate constant for nonstructural C exchange
def: "Shoot-root rate constant for nonstructural C exchange refers to the rate at which carbon is exchanged between the shoot and root of a plant, specifically in relation to nonstructural carbon compounds. This value can impact a range of plant processes, including growth, resource allocation, and response to environmental stress." []
is_a: ECOSIM:CATEGORYRootPhysiology ! category - root physiology
relationship: attribute ECOSIMCONCEPT:Rate ! Rate
relationship: context ECOSIMCONCEPT:Root ! Root
relationship: context ECOSIMCONCEPT:Shoot ! Shoot
relationship: has_unit ECOSIM:h-1 ! h-1

[Term]
id: ECOSIM:PTrans
name: canopy transpiration
is_a: ECOSIMCONCEPT:UnclassifiedVariable ! unclassified variable
relationship: has_unit ECOSIM:m2d-2h-1 ! m2 d-2 h-1

[Term]
id: ECOSIM:PlantO2Stress
name: plant O2 stress indicator
def: "Plant O2 stress indicator is a measure of the stress response in plants due to low or high levels of oxygen (O2). It is an important parameter in plant physiology and crop modeling, as oxygen stress can have significant impacts on plant growth and productivity." []
is_a: ECOSIM:CATEGORYCanopyStructure ! category - canopy structure
relationship: context ECOSIMCONCEPT:Oxygen ! Oxygen
relationship: context ECOSIMCONCEPT:Plant ! Plant

[Term]
id: ECOSIM:PlantinDepth
name: planting depth
def: "Planting depth refers to the depth at which a seed is placed in the soil during planting. The appropriate planting depth varies by the type of seed and is vital for the successful establishment and growth of the plant. It highly influences the emergence, growth rate and development of the plant. Planting depth is a crucial factor in agricultural and horticultural practices." []
is_a: ECOSIM:CATEGORYCanopyStructure ! category - canopy structure
is_a: ECOSIM:CATEGORYPlantPopulation ! category - Plant Population
relationship: attribute ECOSIMCONCEPT:Depth ! Depth
relationship: has_unit ECOSIM:m ! m
relationship: measured_in ECOSIMCONCEPT:Soil ! Soil
relationship: measurement_of ECOSIMCONCEPT:Plant ! Plant

[Term]
id: ECOSIM:PopPlantRootC_vr
name: root layer C
def: "Root layer C refers to the amount of carbon present in the soil layer where plant roots predominantly reside. It is a parameter used in earth systems modeling to simulate and understand the carbon dynamics and cycling within terrestrial ecosystems. The root layer C can vary across different plant types, soil conditions, and land management practices, and plays a crucial role in influencing soil carbon stocks, nutrient availability, and overall ecosystem productivity." []
is_a: ECOSIMCONCEPT:UnclassifiedVariable ! unclassified variable
relationship: has_unit ECOSIM:gd-2 ! g d-2

[Term]
id: ECOSIM:PrecAtm
name: rainfall + snowfall
def: "The sum of rainfall and snowfall that a particular region receives over a period of time. This value is often used in meteorology to monitor and predict weather patterns and to analyze the climate patterns of a particular region." []
is_a: ECOSIM:CATEGORYAtmosphericConditions ! category - Atmospheric Conditions
relationship: has_unit ECOSIM:m3d-2h-1 ! m3 d-2 h-1

[Term]
id: ECOSIM:PrecIntcptByCanG
name: grid net precipitation water interception to canopy
is_a: ECOSIMCONCEPT:UnclassifiedVariable ! unclassified variable
relationship: has_unit ECOSIM:MJd-2t-1 ! MJ d-2 t-1

[Term]
id: ECOSIM:PrecIntcptByCanP
name: water flux into plant canopy
is_a: ECOSIMCONCEPT:UnclassifiedVariable ! unclassified variable
relationship: has_unit ECOSIM:m3d-2h-1 ! m3 d-2 h-1

[Term]
id: ECOSIM:PrecRainAndSurfirrig
name: rainfall + irrigation
is_a: ECOSIMCONCEPT:UnclassifiedVariable ! unclassified variable
relationship: has_unit ECOSIM:m3d-2h-1 ! m3 d-2 h-1

[Term]
id: ECOSIM:PrimRootDepth
name: root layer depth
is_a: ECOSIM:CATEGORYRootPhysiology ! category - root physiology
relationship: has_unit ECOSIM:m ! m

[Term]
id: ECOSIM:PrimRootLen
name: root layer length primary axes
def: "Root layer length of primary axes refers to the length of the primary roots in the layer of soil. It provides information on the depth distribution of roots within the soil profile." []
is_a: ECOSIM:CATEGORYRootPhysiology ! category - root physiology
relationship: has_unit ECOSIM:md-2 ! m d-2
relationship: measured_in ECOSIMCONCEPT:RootLayer ! Root layer
relationship: measurement_of ECOSIMCONCEPT:Root ! Root

[Term]
id: ECOSIM:PrimRootRadius
name: root layer diameter primary axes
is_a: ECOSIM:CATEGORYRootPhysiology ! category - root physiology
relationship: has_unit ECOSIM:m ! m

[Term]
id: ECOSIM:PrimRootSpecLen
name: specific root length primary axes
is_a: ECOSIM:CATEGORYRootPhysiology ! category - root physiology
relationship: has_unit ECOSIM:mg-1 ! m g-1

[Term]
id: ECOSIM:PrimRootXNumL
name: root layer number primary axes
def: "Root layer number primary axes refers to the count of primary root axes in a specific layer of root system. The primary root axis is the main root from which smaller lateral roots grow. Different root layers can have different densities and organization of primary root axes, affecting nutrient uptake and anchorage of the plant. This count aids in understanding root architecture and its effects on plant growth." []
is_a: ECOSIM:CATEGORYRootPhysiology ! category - root physiology
relationship: attribute ECOSIMCONCEPT:Number ! Number
relationship: context ECOSIMCONCEPT:RootLayer ! Root layer
relationship: has_unit ECOSIM:d-2 ! d-2

[Term]
id: ECOSIM:PrimRootXSecArea
name: root cross-sectional area primary axes
def: "The cross-sectional area of the primary root axes refers to the area of a section cut through the primary root axis perpendicular to its length. This is an important parameter in understanding the root architecture, water and nutrient uptake, as well as overall plant growth." []
is_a: ECOSIM:CATEGORYRootPhysiology ! category - root physiology
relationship: attribute ECOSIMCONCEPT:Area ! Area
relationship: has_unit ECOSIM:m2 ! m2
relationship: measured_in ECOSIMCONCEPT:Root ! Root

[Term]
id: ECOSIM:R3GasADTFlx
name: 3D gaseous fluxes
is_a: ECOSIMCONCEPT:UnclassifiedVariable ! unclassified variable
relationship: has_unit ECOSIM:gd-2h-1 ! g d-2 h-1

[Term]
id: ECOSIM:RAD
name: shortwave radiation in solar beam
is_a: ECOSIMCONCEPT:UnclassifiedVariable ! unclassified variable
relationship: has_unit ECOSIM:MJm-2h-1 ! MJ m-2 h-1

[Term]
id: ECOSIM:RADS
name: direct shortwave radiation
is_a: ECOSIMCONCEPT:UnclassifiedVariable ! unclassified variable
relationship: has_unit ECOSIM:Wm-2 ! W m-2

[Term]
id: ECOSIM:RADY
name: diffuse shortwave radiation
is_a: ECOSIMCONCEPT:UnclassifiedVariable ! unclassified variable
relationship: has_unit ECOSIM:Wm-2 ! W m-2

[Term]
id: ECOSIM:RAP
name: PAR radiation in solar beam
is_a: ECOSIMCONCEPT:UnclassifiedVariable ! unclassified variable
relationship: has_unit ECOSIM:umolm-2s-1 ! umol m-2 s-1

[Term]
id: ECOSIM:RAPS
name: direct PAR
is_a: ECOSIMCONCEPT:UnclassifiedVariable ! unclassified variable
relationship: has_unit ECOSIM:umolm-2s-1 ! umol m-2 s-1

[Term]
id: ECOSIM:RAPY
name: diffuse PAR
is_a: ECOSIMCONCEPT:UnclassifiedVariable ! unclassified variable
relationship: has_unit ECOSIM:umolm-2s-1 ! umol m-2 s-1

[Term]
id: ECOSIM:RAZ
name: canopy roughness height
def: "Canopy roughness height refers to the height of unevenness or irregularity on the surface of a plant canopy. It is a parameter used in earth system modeling to understand the movement of wind over and through the canopy. The roughness height can influence the speed of the wind, the transport of gases and aerosols, and the exchange of energy and momentum between the canopy and the atmosphere." []
is_a: ECOSIM:CATEGORYCanopyStructure ! category - canopy structure
relationship: attribute ECOSIMCONCEPT:Height ! Height
relationship: has_unit ECOSIM:m ! m
relationship: measured_in ECOSIMCONCEPT:Canopy ! Canopy

[Term]
id: ECOSIM:RCELX
name: element translocated from leaf during senescence
def: "Element translocated from leaf during senescence, often represented as RCELX, refers to the movement of certain nutrients or elements from the leaf to other parts of the plant during the process of senescence, which is the aging process in the plant where the leaf cellular structure degrades, often leading to leaf fall. This translocation typically happens to reuse or relocate valuable elements within the plant for normative growth or survival purposes." []
is_a: ECOSIM:CATEGORYRootPhysiology ! category - root physiology
relationship: has_unit ECOSIM:gd-2h-1 ! g d-2 h-1
relationship: measured_in ECOSIMCONCEPT:Leaf ! Leaf

[Term]
id: ECOSIM:RCESX
name: element translocated from sheath during senescence
def: "Element translocated from sheath during senescence refers to the process of nutrients being moved away from the sheath during plant senescence. Senescence is the last phase of development in a plant's lifecycle, characterized by degradation of cell structures, protein catabolism, and nutrient mobilization." []
is_a: ECOSIM:CATEGORYRootPhysiology ! category - root physiology
relationship: has_unit ECOSIM:gd-2h-1 ! g d-2 h-1
relationship: measured_in ECOSIMCONCEPT:Plant ! Plant

[Term]
id: ECOSIM:RCH4F
name: net gaseous CH4 flux
is_a: ECOSIMCONCEPT:UnclassifiedVariable ! unclassified variable
relationship: has_unit ECOSIM:gd-2h-1 ! g d-2 h-1

[Term]
id: ECOSIM:RCH4L
name: net aqueous CH4 flux
is_a: ECOSIMCONCEPT:UnclassifiedVariable ! unclassified variable
relationship: has_unit ECOSIM:gd-2h-1 ! g d-2 h-1

[Term]
id: ECOSIM:RCH4O
name: microbial net CH4 exchange
is_a: ECOSIM:CATEGORYMicrobialActivity ! category - microbial activity
is_a: ECOSIM:CATEGORYNTransformation ! category - N transformation
is_a: ECOSIM:CATEGORYSoilBiogeochemistry ! category - Soil Biogeochemistry
relationship: attribute ECOSIMCONCEPT:Exchange ! Exchange
relationship: has_unit ECOSIM:gd-2h-1 ! g d-2 h-1
relationship: measurement_of ECOSIMCONCEPT:CH4 ! Methane

[Term]
id: ECOSIM:RCH4S
name: RCH4S
is_a: ECOSIM:CATEGORYHydrology ! category - Hydrology
is_a: ECOSIM:CATEGORYSoilBiogeochemistry ! category - Soil Biogeochemistry
relationship: attribute ECOSIMCONCEPT:Rate ! Rate

[Term]
id: ECOSIM:RCHGD
name: lower subsurface boundary water flux
def: "Lower subsurface boundary water flux is the movement or flow of water across the lower boundary of the subsurface layer of the soil. It represents the quantity of water that moves from the subsurface soil layer to deeper layer, which may include groundwater reservoir or deeper layers of the soil profile. This flux can occur through processes such as deep percolation and groundwater recharge." []
is_a: ECOSIM:CATEGORYHydrology ! category - Hydrology
relationship: attribute ECOSIMCONCEPT:Flux ! Flux
relationship: measurement_of ECOSIMCONCEPT:Water ! Water

[Term]
id: ECOSIM:RCMX
name: maximum stomatal resistance to CO2
def: "Maximum stomatal resistance to CO2, also known as RCMX, refers to the maximum level of resistance that occurs in the stomata, microscopic openings in the plant leaf, to the exchange of carbon dioxide (CO2) during photosynthesis. It plays a critical role in determining the efficiency of a plant's photosynthetic process and can vary significantly among different plant species as well as under different environmental conditions." []
is_a: ECOSIM:CATEGORYCanopyPhysiology ! category - Canopy Physiology
is_a: ECOSIM:CATEGORYPlantPhysiology ! category - plant physiology
relationship: has_unit ECOSIM:sh-1 ! s h-1
relationship: measured_in ECOSIMCONCEPT:Stoma ! Stoma
relationship: measurement_of ECOSIMCONCEPT:CO2 ! Carbon dioxide

[Term]
id: ECOSIM:RCO2A
name: root respiration constrained by O2
is_a: ECOSIMCONCEPT:UnclassifiedVariable ! unclassified variable
relationship: has_unit ECOSIM:gd-2h-1 ! g d-2 h-1

[Term]
id: ECOSIM:RCO2F
name: net gaseous CO2 flux
is_a: ECOSIMCONCEPT:UnclassifiedVariable ! unclassified variable
relationship: has_unit ECOSIM:gd-2h-1 ! g d-2 h-1

[Term]
id: ECOSIM:RCO2M
name: root respiration unconstrained by O2
is_a: ECOSIMCONCEPT:UnclassifiedVariable ! unclassified variable
relationship: has_unit ECOSIM:gd-2h-1 ! g d-2 h-1

[Term]
id: ECOSIM:RCO2N
name: root CO2 efflux unconstrained by root nonstructural C
is_a: ECOSIMCONCEPT:UnclassifiedVariable ! unclassified variable
relationship: has_unit ECOSIM:gd-2h-1 ! g d-2 h-1

[Term]
id: ECOSIM:RCO2O
name: microbial net CO2 exchange
def: "Microbial net CO2 exchange refers to the overall balance between carbon dioxide (CO2) uptake and release by microbial communities in an ecosystem. It includes CO2 absorbed by microbes during photosynthesis and CO2 released during respiration and decomposition. This parameter is important in understanding the role of microbes in the carbon cycle and their impact on ecosystem health and function." []
is_a: ECOSIM:CATEGORYNTransformation ! category - N transformation
is_a: ECOSIM:CATEGORYSoilBiogeochemistry ! category - Soil Biogeochemistry
relationship: attribute ECOSIMCONCEPT:NetExchange ! Net exchange
relationship: has_unit ECOSIM:gd-2h-1 ! g d-2 h-1
relationship: measurement_of ECOSIMCONCEPT:CO2 ! Carbon dioxide

[Term]
id: ECOSIM:RCO2P
name: aqueous CO2 flux from roots to root water
is_a: ECOSIMCONCEPT:UnclassifiedVariable ! unclassified variable
relationship: has_unit ECOSIM:gd-2h-1 ! g d-2 h-1

[Term]
id: ECOSIM:RCO2S
name: aqueous CO2 flux from roots to soil water
is_a: ECOSIM:CATEGORYHydrology ! category - Hydrology
is_a: ECOSIM:CATEGORYSoilBiogeochemistry ! category - Soil Biogeochemistry
relationship: attribute ECOSIMCONCEPT:Flux ! Flux
relationship: has_unit ECOSIM:gd-2h-1 ! g d-2 h-1
relationship: measured_in ECOSIMCONCEPT:Root ! Root
relationship: measured_in ECOSIMCONCEPT:SoilWater ! Soil water
relationship: measurement_of ECOSIMCONCEPT:CO2 ! Carbon dioxide

[Term]
id: ECOSIM:RCPSX
name: P translocated from sheath during senescence
is_a: ECOSIMCONCEPT:UnclassifiedVariable ! unclassified variable
relationship: has_unit ECOSIM:gd-2h-1 ! g d-2 h-1

[Term]
id: ECOSIM:RCS
name: shape parameter for calculating stomatal resistance from turgor pressure
def: "Shape parameter for calculating stomatal resistance from turgor pressure refers to a specific parameter values used in mathematical or computational models to quantify the effect of turgor pressure on stomatal resistance. The stomatal resistance is a measure of how open or closed stomata are in plant leaves, influencing the rate of evapotranspiration and photosynthesis. Turgor pressure in plant cells plays a vital role in controlling stomatal movement and hence stomatal resistance." []
is_a: ECOSIM:CATEGORYCanopyPhysiology ! category - Canopy Physiology
is_a: ECOSIM:CATEGORYPlantPhysiology ! category - plant physiology
relationship: measured_in ECOSIMCONCEPT:Stoma ! Stoma

[Term]
id: ECOSIM:RCZSX
name: N translocated from sheath during senescence
is_a: ECOSIMCONCEPT:UnclassifiedVariable ! unclassified variable
relationship: has_unit ECOSIM:gd-2h-1 ! g d-2 h-1

[Term]
id: ECOSIM:RDFOME
name: root uptake (+ve) - exudation (-ve) of DOC
def: "RDFOME refers to the Root uptake which is positive or exudation which is negative of Dissolved Organic Carbon (DOC). This term helps in understanding the process by which roots extract or exude DOC from or into the soil environment. It is an important parameter in earth systems modeling as it plays a crucial role in carbon cycling and soil organic matter dynamics." []
is_a: ECOSIM:CATEGORYRootPhysiology ! category - root physiology
relationship: attribute ECOSIMCONCEPT:UptakeExudation ! Uptake exudation
relationship: has_unit ECOSIM:gd-2h-1 ! g d-2 h-1
relationship: measured_in ECOSIMCONCEPT:Root ! Root
relationship: measurement_of ECOSIMCONCEPT:DOC ! DOC

[Term]
id: ECOSIM:RECO
name: ecosystem respiration
is_a: ECOSIMCONCEPT:UnclassifiedVariable ! unclassified variable
relationship: has_unit ECOSIM:gd-2h-1 ! g d-2 h-1

[Term]
id: ECOSIM:RH2GO
name: microbial net H2 exchange
def: "Microbial net H2 exchange refers to the balance of the production and use of molecular hydrogen (H2) by microorganisms in an ecosystem. This can be influenced by various factors, such as microbial community composition, environmental conditions, and availability of substrates. It plays a key role in biogeochemical cycles, including the global carbon cycle." []
is_a: ECOSIM:CATEGORYMicrobialActivity ! category - microbial activity
is_a: ECOSIM:CATEGORYNTransformation ! category - N transformation
is_a: ECOSIM:CATEGORYSoilBiogeochemistry ! category - Soil Biogeochemistry
relationship: attribute ECOSIMCONCEPT:Exchange ! Exchange
relationship: has_unit ECOSIM:gd-2h-1 ! g d-2 h-1
relationship: measurement_of ECOSIMCONCEPT:H2 ! Dihydrogen

[Term]
id: ECOSIM:RH2GS
name: RH2GS
is_a: ECOSIM:CATEGORYSoilBiogeochemistry ! category - Soil Biogeochemistry

[Term]
id: ECOSIM:RH2GZ
name: gaseous H2 flux fron root disturbance
is_a: ECOSIMCONCEPT:UnclassifiedVariable ! unclassified variable
relationship: has_unit ECOSIM:gd-2h-1 ! g d-2 h-1

[Term]
id: ECOSIM:RIB
name: Richardson number for calculating boundary layer resistance
is_a: ECOSIMCONCEPT:UnclassifiedVariable ! unclassified variable

[Term]
id: ECOSIM:RN2BX
name: total root + microbial NO2 uptake band
is_a: ECOSIMCONCEPT:UnclassifiedVariable ! unclassified variable
relationship: has_unit ECOSIM:gd-2h-1 ! g d-2 h-1

[Term]
id: ECOSIM:RN2BY
name: total root + microbial NO2 uptake band
is_a: ECOSIMCONCEPT:UnclassifiedVariable ! unclassified variable
relationship: has_unit ECOSIM:gd-2h-1 ! g d-2 h-1

[Term]
id: ECOSIM:RN2G
name: microbial net N2 exchange
is_a: ECOSIM:CATEGORYNTransformation ! category - N transformation
is_a: ECOSIM:CATEGORYSoilBiogeochemistry ! category - Soil Biogeochemistry
relationship: attribute ECOSIMCONCEPT:Exchange ! Exchange
relationship: has_unit ECOSIM:gd-2h-1 ! g d-2 h-1
relationship: measurement_of ECOSIMCONCEPT:N2 ! Dinitrogen

[Term]
id: ECOSIM:RN2O
name: microbial net N2O exchange
is_a: ECOSIM:CATEGORYNTransformation ! category - N transformation
is_a: ECOSIM:CATEGORYSoilBiogeochemistry ! category - Soil Biogeochemistry
relationship: attribute ECOSIMCONCEPT:NetExchange ! Net exchange
relationship: has_unit ECOSIM:gd-2h-1 ! g d-2 h-1
relationship: measurement_of ECOSIMCONCEPT:N2O ! Nitrous oxide

[Term]
id: ECOSIM:RN2OX
name: total root + microbial N2O uptake
is_a: ECOSIMCONCEPT:UnclassifiedVariable ! unclassified variable
relationship: has_unit ECOSIM:gd-2h-1 ! g d-2 h-1

[Term]
id: ECOSIM:RN2OY
name: total root + microbial N2O uptake
is_a: ECOSIMCONCEPT:UnclassifiedVariable ! unclassified variable
relationship: has_unit ECOSIM:gd-2h-1 ! g d-2 h-1

[Term]
id: ECOSIM:RN2S
name: RN2S
is_a: ECOSIM:CATEGORYSoilBiogeochemistry ! category - Soil Biogeochemistry

[Term]
id: ECOSIM:RN3BX
name: total root + microbial NO3 uptake band
is_a: ECOSIMCONCEPT:UnclassifiedVariable ! unclassified variable
relationship: has_unit ECOSIM:gd-2h-1 ! g d-2 h-1

[Term]
id: ECOSIM:RN3BY
name: total root + microbial NO3 uptake band
is_a: ECOSIMCONCEPT:UnclassifiedVariable ! unclassified variable
relationship: has_unit ECOSIM:gd-2h-1 ! g d-2 h-1

[Term]
id: ECOSIM:RNH3B
name: gaseous NH3 flux fron root disturbance band
is_a: ECOSIMCONCEPT:UnclassifiedVariable ! unclassified variable
relationship: has_unit ECOSIM:gd-2h-1 ! g d-2 h-1

[Term]
id: ECOSIM:RNH3C
name: canopy NH3 flux
is_a: ECOSIMCONCEPT:UnclassifiedVariable ! unclassified variable
relationship: has_unit ECOSIM:gd-2h-1 ! g d-2 h-1

[Term]
id: ECOSIM:RNH3Z
name: gaseous NH3 flux fron root disturbance non-band
is_a: ECOSIMCONCEPT:UnclassifiedVariable ! unclassified variable
relationship: has_unit ECOSIM:gd-2h-1 ! g d-2 h-1

[Term]
id: ECOSIM:RNH4X
name: total root + microbial NH4 uptake non-band
is_a: ECOSIMCONCEPT:UnclassifiedVariable ! unclassified variable
relationship: has_unit ECOSIM:gd-2h-1 ! g d-2 h-1

[Term]
id: ECOSIM:RNH4Y
name: total root + microbial NH4 uptake non-band
is_a: ECOSIMCONCEPT:UnclassifiedVariable ! unclassified variable
relationship: has_unit ECOSIM:gd-2h-1 ! g d-2 h-1

[Term]
id: ECOSIM:RNHBX
name: total root + microbial NH4 uptake band
is_a: ECOSIMCONCEPT:UnclassifiedVariable ! unclassified variable
relationship: has_unit ECOSIM:gd-2h-1 ! g d-2 h-1

[Term]
id: ECOSIM:RNHBY
name: total root + microbial NH4 uptake band
is_a: ECOSIMCONCEPT:UnclassifiedVariable ! unclassified variable
relationship: has_unit ECOSIM:gd-2h-1 ! g d-2 h-1

[Term]
id: ECOSIM:RNO2X
name: total root + microbial NO2 uptake non-band
is_a: ECOSIMCONCEPT:UnclassifiedVariable ! unclassified variable
relationship: has_unit ECOSIM:gd-2h-1 ! g d-2 h-1

[Term]
id: ECOSIM:RNO2Y
name: total root + microbial NO2 uptake non-band
is_a: ECOSIMCONCEPT:UnclassifiedVariable ! unclassified variable
relationship: has_unit ECOSIM:gd-2h-1 ! g d-2 h-1

[Term]
id: ECOSIM:RNO3X
name: total root + microbial NO3 uptake non-band
is_a: ECOSIMCONCEPT:UnclassifiedVariable ! unclassified variable
relationship: has_unit ECOSIM:gd-2h-1 ! g d-2 h-1

[Term]
id: ECOSIM:RNO3Y
name: total root + microbial NO3 uptake non-band
is_a: ECOSIMCONCEPT:UnclassifiedVariable ! unclassified variable
relationship: has_unit ECOSIM:gd-2h-1 ! g d-2 h-1

[Term]
id: ECOSIM:ROQAX
name: total root + microbial acetate uptake
is_a: ECOSIMCONCEPT:UnclassifiedVariable ! unclassified variable
relationship: has_unit ECOSIM:gd-2h-1 ! g d-2 h-1

[Term]
id: ECOSIM:ROQAY
name: total root + microbial acetate uptake
is_a: ECOSIMCONCEPT:UnclassifiedVariable ! unclassified variable
relationship: has_unit ECOSIM:gd-2h-1 ! g d-2 h-1

[Term]
id: ECOSIM:ROQCX
name: total root + microbial DOC uptake
is_a: ECOSIMCONCEPT:UnclassifiedVariable ! unclassified variable
relationship: has_unit ECOSIM:gd-2h-1 ! g d-2 h-1

[Term]
id: ECOSIM:ROQCY
name: total root + microbial DOC uptake
is_a: ECOSIMCONCEPT:UnclassifiedVariable ! unclassified variable
relationship: has_unit ECOSIM:gd-2h-1 ! g d-2 h-1

[Term]
id: ECOSIM:ROWI
name: row spacing of fertilizer band
is_a: ECOSIMCONCEPT:UnclassifiedVariable ! unclassified variable
relationship: has_unit ECOSIM:m ! m

[Term]
id: ECOSIM:ROWN
name: row spacing of NH4 fertilizer band
is_a: ECOSIMCONCEPT:UnclassifiedVariable ! unclassified variable
relationship: has_unit ECOSIM:m ! m

[Term]
id: ECOSIM:ROWO
name: row spacing of NO3 fertilizer band
is_a: ECOSIMCONCEPT:UnclassifiedVariable ! unclassified variable
relationship: has_unit ECOSIM:m ! m

[Term]
id: ECOSIM:ROWP
name: row spacing of PO4 fertilizer band
is_a: ECOSIMCONCEPT:UnclassifiedVariable ! unclassified variable
relationship: has_unit ECOSIM:m ! m

[Term]
id: ECOSIM:ROXSK
name: total O2 sink
def: "Total O2 sink refers to the total quantity or capacity of a system to absorb or consume O2 (Oxygen). This can vary based on factors such as environmental conditions and the presence of certain organisms or substances." []
is_a: ECOSIM:CATEGORYBiogeochemistry ! category - Biogeochemistry
is_a: ECOSIM:CATEGORYTraceGasFlux ! category - trace gas flux
relationship: has_unit ECOSIM:gd-2t-1 ! g d-2 t-1
relationship: measurement_of ECOSIMCONCEPT:O2 ! Dioxygen

[Term]
id: ECOSIM:ROXYF
name: net gaseous O2 flux
is_a: ECOSIMCONCEPT:UnclassifiedVariable ! unclassified variable
relationship: has_unit ECOSIM:gd-2h-1 ! g d-2 h-1

[Term]
id: ECOSIM:ROXYL
name: net aqueous O2 flux
is_a: ECOSIMCONCEPT:UnclassifiedVariable ! unclassified variable
relationship: has_unit ECOSIM:gd-2h-1 ! g d-2 h-1

[Term]
id: ECOSIM:ROXYP
name: root O2 demand from respiration
is_a: ECOSIMCONCEPT:UnclassifiedVariable ! unclassified variable
relationship: has_unit ECOSIM:gd-2h-1 ! g d-2 h-1

[Term]
id: ECOSIM:ROXYX
name: total root + microbial O2 uptake
is_a: ECOSIMCONCEPT:UnclassifiedVariable ! unclassified variable
relationship: has_unit ECOSIM:gd-2h-1 ! g d-2 h-1

[Term]
id: ECOSIM:ROXYY
name: total root + microbial O2 uptake
is_a: ECOSIMCONCEPT:UnclassifiedVariable ! unclassified variable
relationship: has_unit ECOSIM:gd-2h-1 ! g d-2 h-1

[Term]
id: ECOSIM:RPO4X
name: total root + microbial PO4 uptake non-band
is_a: ECOSIMCONCEPT:UnclassifiedVariable ! unclassified variable
relationship: has_unit ECOSIM:gd-2h-1 ! g d-2 h-1

[Term]
id: ECOSIM:RPO4Y
name: total root + microbial PO4 uptake non-band
is_a: ECOSIMCONCEPT:UnclassifiedVariable ! unclassified variable
relationship: has_unit ECOSIM:gd-2h-1 ! g d-2 h-1

[Term]
id: ECOSIM:RPOBX
name: total root + microbial PO4 uptake band
is_a: ECOSIMCONCEPT:UnclassifiedVariable ! unclassified variable
relationship: has_unit ECOSIM:gd-2h-1 ! g d-2 h-1

[Term]
id: ECOSIM:RPOBY
name: total root + microbial PO4 uptake band
is_a: ECOSIMCONCEPT:UnclassifiedVariable ! unclassified variable
relationship: has_unit ECOSIM:gd-2h-1 ! g d-2 h-1

[Term]
id: ECOSIM:RRADP
name: root internal radius
def: "Root internal radius refers to the inner radius of a plant's root. It is an important factor in plant growth and development, affecting the plant's ability to absorb water and nutrients from the soil." []
is_a: ECOSIM:CATEGORYRootPhysiology ! category - root physiology
relationship: has_unit ECOSIM:m ! m
relationship: measured_in ECOSIMCONCEPT:Root ! Root

[Term]
id: ECOSIM:RRIG
name: irrigation application
is_a: ECOSIMCONCEPT:UnclassifiedVariable ! unclassified variable
relationship: has_unit ECOSIM:mmh-1 ! mm h-1

[Term]
id: ECOSIM:RSETE
name: effect of canopy element status on seed set
is_a: ECOSIMCONCEPT:UnclassifiedVariable ! unclassified variable

[Term]
id: ECOSIM:RSMX
name: maximum stomatal resistance to vapor
def: "Maximum stomatal resistance to vapor refers to the maximum resistance, or opposition, that stomata of plants provide to the passage of water vapor. It is a key parameter in plant physiology, having implications for processes like photosynthesis, respiration, and plant water use efficiency." []
is_a: ECOSIM:CATEGORYCanopyPhysiology ! category - Canopy Physiology
is_a: ECOSIM:CATEGORYPlantPhysiology ! category - plant physiology
relationship: has_unit ECOSIM:sm-1 ! s m-1
relationship: measured_in ECOSIMCONCEPT:Stoma ! Stoma
relationship: measurement_of ECOSIMCONCEPT:Vapor ! Vapor

[Term]
id: ECOSIM:RSRA
name: root axial resistivity
def: "Root axial resistivity (RSRA) is a measure of the ability of a plant's root system to resist the flow of electric current along its length. It is an important parameter in the study of plant physiology and root system architecture, as it can provide insights into the structure and function of the root system. The RSRA value can be influenced by various factors, including the species and age of the plant, soil conditions, and environmental factors." []
is_a: ECOSIM:CATEGORYRootPhysiology ! category - root physiology
relationship: has_unit ECOSIM:MPahm-4 ! MPa h m-4
relationship: measured_in ECOSIMCONCEPT:Root ! Root

[Term]
id: ECOSIM:RSRR
name: root radial resistivity
def: "Root radial resistivity refers to the resistance offered by the root system of a plant to the radial flow of water and nutrients. It is an important factor affecting the uptake of water and nutrients from soil." []
is_a: ECOSIM:CATEGORYRootPhysiology ! category - root physiology
relationship: has_unit ECOSIM:MPahm-2 ! MPa h m-2
relationship: measurement_of ECOSIMCONCEPT:Root ! Root

[Term]
id: ECOSIM:RTARP
name: root layer area per plant
def: "Root layer area per plant refers to the total area covered by the roots of a single plant. It is a parameter used in ecological and earth system modeling to understand root development, nutrient uptake, and the overall growth of plants. This information is also important for understanding soil-plant interactions and nutrient cycling." []
is_a: ECOSIM:CATEGORYPlantPhysiology ! category - plant physiology
is_a: ECOSIM:CATEGORYRootPhysiology ! category - root physiology
relationship: has_unit ECOSIM:mp-1 ! m p-1
relationship: measured_in ECOSIMCONCEPT:RootLayer ! Root layer
relationship: measurement_of ECOSIMCONCEPT:Area ! Area

[Term]
id: ECOSIM:RTDNT
name: total root length density
is_a: ECOSIMCONCEPT:UnclassifiedVariable ! unclassified variable
relationship: has_unit ECOSIM:mm-3 ! m m-3

[Term]
id: ECOSIM:RTFQ
name: root brancing frequency
def: "Root branching frequency refers to the number of root branches per unit length of root. This is an important attribute of root system architecture and can significantly influence root function, including nutrient and water uptake." []
is_a: ECOSIM:CATEGORYRootPhysiology ! category - root physiology
relationship: has_unit ECOSIM:m-1 ! m-1
relationship: measured_in ECOSIMCONCEPT:Root ! Root

[Term]
id: ECOSIM:RTN2
name: root layer number secondary axes
def: "Root layer number secondary axes refer to the number of secondary roots emerging from the primary roots in the root layer of plants. This measure is critical in understanding the complexity and efficiency of the root system of plants, influencing nutrient and water uptake, plant stability, and interactions with the soil microorganisms." []
is_a: ECOSIM:CATEGORYRootPhysiology ! category - root physiology
relationship: attribute ECOSIMCONCEPT:Number ! Number
relationship: has_unit ECOSIM:d-2 ! d-2
relationship: measured_in ECOSIMCONCEPT:RootLayer ! Root layer

[Term]
id: ECOSIM:RTVLP
name: root layer volume air
def: "Root layer volume air refers to the amount of air space present within the root layer of soil. This space is critical for plant growth as it allows for the exchange of gases between the roots and the atmosphere, facilitates the movement of water and nutrients to the roots, and prevents the soil from becoming overly compacted. It is a vital parameter in understanding plant physiology and soil-plant interactions, and can be influenced by factors such as soil type, compaction, moisture content, and root growth." []
is_a: ECOSIM:CATEGORYRootPhysiology ! category - root physiology
relationship: attribute ECOSIMCONCEPT:Volume ! Volume
relationship: has_unit ECOSIM:m2d-2 ! m2 d-2
relationship: measured_in ECOSIMCONCEPT:RootLayer ! Root layer
relationship: measurement_of ECOSIMCONCEPT:Air ! Air

[Term]
id: ECOSIM:RTVLW
name: root layer volume water
def: "Root layer volume water refers to the volume of water present within the root layer of soil. This measurement is crucial in understanding plant water uptake, soil water retention, and the hydrological balance within the soil profile. It is measured in volume units (e.g., cubic meters) per soil layer depth (e.g., meters) and can significantly vary based on soil characteristics, environmental conditions, and plant root systems." []
is_a: ECOSIM:CATEGORYPlantPhysiology ! category - plant physiology
is_a: ECOSIM:CATEGORYRootPhysiology ! category - root physiology
relationship: attribute ECOSIMCONCEPT:Volume ! Volume
relationship: has_unit ECOSIM:m2d-2 ! m2 d-2
relationship: measured_in ECOSIMCONCEPT:RootLayer ! Root layer
relationship: measurement_of ECOSIMCONCEPT:Water ! Water

[Term]
id: ECOSIM:RTWT1E
name: root C primary axes
is_a: ECOSIMCONCEPT:UnclassifiedVariable ! unclassified variable
relationship: has_unit ECOSIM:gd-2 ! g d-2

[Term]
id: ECOSIM:RUBP
name: leaf rubisco content
is_a: ECOSIM:CATEGORYCanopyPhysiology ! category - Canopy Physiology
is_a: ECOSIM:CATEGORYPlantPhysiology ! category - plant physiology
relationship: has_unit ECOSIM:gg-1 ! g g-1
relationship: measured_in ECOSIMCONCEPT:Leaf ! Leaf

[Term]
id: ECOSIM:RUCH2B
name: root uptake of PO4 band unconstrained by root nonstructural C
is_a: ECOSIMCONCEPT:UnclassifiedVariable ! unclassified variable
relationship: has_unit ECOSIM:gd-2h-1 ! g d-2 h-1

[Term]
id: ECOSIM:RUCH2P
name: root uptake of PO4 non-band unconstrained by root nonstructural C
is_a: ECOSIMCONCEPT:UnclassifiedVariable ! unclassified variable
relationship: has_unit ECOSIM:gd-2h-1 ! g d-2 h-1

[Term]
id: ECOSIM:RUCNH4
name: root uptake of NH4 non-band unconstrained by root nonstructural C
is_a: ECOSIMCONCEPT:UnclassifiedVariable ! unclassified variable
relationship: has_unit ECOSIM:gd-2h-1 ! g d-2 h-1

[Term]
id: ECOSIM:RUCNHB
name: root uptake of NH4 band unconstrained by root nonstructural C
is_a: ECOSIMCONCEPT:UnclassifiedVariable ! unclassified variable
relationship: has_unit ECOSIM:gd-2h-1 ! g d-2 h-1

[Term]
id: ECOSIM:RUCNO3
name: root uptake of NO3 non-band unconstrained by root nonstructural C
is_a: ECOSIMCONCEPT:UnclassifiedVariable ! unclassified variable
relationship: has_unit ECOSIM:gd-2h-1 ! g d-2 h-1

[Term]
id: ECOSIM:RUCNOB
name: root uptake of NO3 band unconstrained by root nonstructural C
is_a: ECOSIMCONCEPT:UnclassifiedVariable ! unclassified variable
relationship: has_unit ECOSIM:gd-2h-1 ! g d-2 h-1

[Term]
id: ECOSIM:RUNNBP
name: root uptake of NO3 band unconstrained by NO3
is_a: ECOSIMCONCEPT:UnclassifiedVariable ! unclassified variable
relationship: has_unit ECOSIM:gd-2h-1 ! g d-2 h-1

[Term]
id: ECOSIM:RUNNHP
name: root uptake of NH4 non-band unconstrained by NH4
is_a: ECOSIMCONCEPT:UnclassifiedVariable ! unclassified variable
relationship: has_unit ECOSIM:gd-2h-1 ! g d-2 h-1

[Term]
id: ECOSIM:RUNNOP
name: root uptake of NH4 band unconstrained by NH4
is_a: ECOSIMCONCEPT:UnclassifiedVariable ! unclassified variable
relationship: has_unit ECOSIM:gd-2h-1 ! g d-2 h-1

[Term]
id: ECOSIM:RUNNXP
name: root uptake of NO3 non-band unconstrained by NO3
is_a: ECOSIMCONCEPT:UnclassifiedVariable ! unclassified variable
relationship: has_unit ECOSIM:gd-2h-1 ! g d-2 h-1

[Term]
id: ECOSIM:RUOH2B
name: root uptake of PO4 band unconstrained by O2
is_a: ECOSIMCONCEPT:UnclassifiedVariable ! unclassified variable
relationship: has_unit ECOSIM:gd-2h-1 ! g d-2 h-1

[Term]
id: ECOSIM:RUOH2P
name: root uptake of PO4 non-band unconstrained by O2
is_a: ECOSIMCONCEPT:UnclassifiedVariable ! unclassified variable
relationship: has_unit ECOSIM:gd-2h-1 ! g d-2 h-1

[Term]
id: ECOSIM:RUONH4
name: root uptake of NH4 non-band unconstrained by O2
is_a: ECOSIMCONCEPT:UnclassifiedVariable ! unclassified variable
relationship: has_unit ECOSIM:gd-2h-1 ! g d-2 h-1

[Term]
id: ECOSIM:RUONHB
name: root uptake of NH4 band unconstrained by O2
is_a: ECOSIMCONCEPT:UnclassifiedVariable ! unclassified variable
relationship: has_unit ECOSIM:gd-2h-1 ! g d-2 h-1

[Term]
id: ECOSIM:RUONO3
name: root uptake of NO3 non-band unconstrained by O2
is_a: ECOSIMCONCEPT:UnclassifiedVariable ! unclassified variable
relationship: has_unit ECOSIM:gd-2h-1 ! g d-2 h-1

[Term]
id: ECOSIM:RUONOB
name: root uptake of NO3 band unconstrained by O2
is_a: ECOSIMCONCEPT:UnclassifiedVariable ! unclassified variable
relationship: has_unit ECOSIM:gd-2h-1 ! g d-2 h-1

[Term]
id: ECOSIM:RUPCHS
name: aqueous CH4 flux from roots to soil water
is_a: ECOSIMCONCEPT:UnclassifiedVariable ! unclassified variable
relationship: has_unit ECOSIM:gd-2h-1 ! g d-2 h-1

[Term]
id: ECOSIM:RUPH2B
name: root uptake of PO4 band
is_a: ECOSIMCONCEPT:UnclassifiedVariable ! unclassified variable
relationship: has_unit ECOSIM:gd-2h-1 ! g d-2 h-1

[Term]
id: ECOSIM:RUPH2P
name: root uptake of PO4 non-band
is_a: ECOSIMCONCEPT:UnclassifiedVariable ! unclassified variable
relationship: has_unit ECOSIM:gd-2h-1 ! g d-2 h-1

[Term]
id: ECOSIM:RUPHGS
name: aqueous H2 flux from roots to soil water
is_a: ECOSIMCONCEPT:UnclassifiedVariable ! unclassified variable
relationship: has_unit ECOSIM:gd-2h-1 ! g d-2 h-1

[Term]
id: ECOSIM:RUPN2S
name: aqueous N2O flux from roots to soil water
is_a: ECOSIMCONCEPT:UnclassifiedVariable ! unclassified variable
relationship: has_unit ECOSIM:gd-2h-1 ! g d-2 h-1

[Term]
id: ECOSIM:RUPN3B
name: aqueous NH3 flux from roots to soil water band
is_a: ECOSIMCONCEPT:UnclassifiedVariable ! unclassified variable
relationship: has_unit ECOSIM:gd-2h-1 ! g d-2 h-1

[Term]
id: ECOSIM:RUPN3S
name: aqueous NH3 flux from roots to soil water non-band
is_a: ECOSIMCONCEPT:UnclassifiedVariable ! unclassified variable
relationship: has_unit ECOSIM:gd-2h-1 ! g d-2 h-1

[Term]
id: ECOSIM:RUPNF
name: root N2 fixation
is_a: ECOSIMCONCEPT:UnclassifiedVariable ! unclassified variable
relationship: has_unit ECOSIM:gd-2h-1 ! g d-2 h-1

[Term]
id: ECOSIM:RUPNH4
name: root uptake of NH4 non-band
is_a: ECOSIMCONCEPT:UnclassifiedVariable ! unclassified variable
relationship: has_unit ECOSIM:gd-2h-1 ! g d-2 h-1

[Term]
id: ECOSIM:RUPNHB
name: root uptake of NH4 band
is_a: ECOSIMCONCEPT:UnclassifiedVariable ! unclassified variable
relationship: has_unit ECOSIM:gd-2h-1 ! g d-2 h-1

[Term]
id: ECOSIM:RUPNO3
name: root uptake of NO3 non-band
is_a: ECOSIMCONCEPT:UnclassifiedVariable ! unclassified variable
relationship: has_unit ECOSIM:gd-2h-1 ! g d-2 h-1

[Term]
id: ECOSIM:RUPNOB
name: root uptake of NO3 band
is_a: ECOSIMCONCEPT:UnclassifiedVariable ! unclassified variable
relationship: has_unit ECOSIM:gd-2h-1 ! g d-2 h-1

[Term]
id: ECOSIM:RUPOXO
name: microbial O2 uptake
def: "Microbial O2 uptake refers to the process by which microbes in an ecosystem consume oxygen (O2). This process is crucial in many biological and ecological functions, including decomposition of organic matter, nutrient cycling, and maintenance of soil and water quality. Microbial O2 uptake is an important parameter in Earth system modeling as it provides insights into microbial respiration, soil health, and the biogeochemical cycling of elements." []
is_a: ECOSIM:CATEGORYNTransformation ! category - N transformation
is_a: ECOSIM:CATEGORYSoilBiogeochemistry ! category - Soil Biogeochemistry
relationship: attribute ECOSIMCONCEPT:Uptake ! Uptake
relationship: has_unit ECOSIM:gd-2h-1 ! g d-2 h-1
relationship: measurement_of ECOSIMCONCEPT:O2 ! Dioxygen

[Term]
id: ECOSIM:RUPOXP
name: aqueous O2 flux from roots to root water
is_a: ECOSIMCONCEPT:UnclassifiedVariable ! unclassified variable
relationship: has_unit ECOSIM:gd-2h-1 ! g d-2 h-1

[Term]
id: ECOSIM:RUPOXS
name: aqueous O2 flux from roots to soil water
def: "Aqueous O2 flux from roots to soil water refers to the movement of oxygen from plant roots to the surrounding water in the soil. This process can be an essential part of soil ecosystem dynamics, influencing the availability of oxygen for aerobic microorganisms in the soil and potentially affecting nutrient cycling." []
is_a: ECOSIM:CATEGORYHydrology ! category - Hydrology
is_a: ECOSIM:CATEGORYSoilBiogeochemistry ! category - Soil Biogeochemistry
relationship: attribute ECOSIMCONCEPT:Flux ! Flux
relationship: context ECOSIMCONCEPT:Root ! Root
relationship: context ECOSIMCONCEPT:Water ! Water
relationship: has_unit ECOSIM:gd-2h-1 ! g d-2 h-1
relationship: measured_in ECOSIMCONCEPT:Soil ! Soil
relationship: measurement_of ECOSIMCONCEPT:Oxygen ! Oxygen

[Term]
id: ECOSIM:RVMBC
name: total chemodenitrification N2O uptake band unconstrained by N2O
is_a: ECOSIMCONCEPT:UnclassifiedVariable ! unclassified variable
relationship: has_unit ECOSIM:gd-2h-1 ! g d-2 h-1

[Term]
id: ECOSIM:RVMXC
name: total chemodenitrification N2O uptake non-band unconstrained by N2O
is_a: ECOSIMCONCEPT:UnclassifiedVariable ! unclassified variable
relationship: has_unit ECOSIM:gd-2h-1 ! g d-2 h-1

[Term]
id: ECOSIM:RadNet2CanP
name: canopy net radiation
def: "Canopy net radiation (RadNet2CanP) refers to the difference between the total incident solar radiation and the outgoing radiation at the canopy surface of a specific plant functional type (pft). It is an important parameter in earth systems modeling as it drives the energy budget of the canopy and affects various physiological processes such as photosynthesis and transpiration." []
is_a: ECOSIM:CATEGORYCanopyPhysiology ! category - Canopy Physiology
is_a: ECOSIM:CATEGORYSurfaceEnergyBalance ! category - Surface Energy Balance
relationship: has_unit ECOSIM:MJd-2h-1 ! MJ d-2 h-1
relationship: measured_in ECOSIMCONCEPT:Canopy ! Canopy
relationship: measurement_of ECOSIMCONCEPT:Radiation ! Radiation

[Term]
id: ECOSIM:RainFalPrec
name: rainfall
is_a: ECOSIM:CATEGORYAtmosphericConditions ! category - Atmospheric Conditions
relationship: has_unit ECOSIM:m3d-2h-1 ! m3 d-2 h-1

[Term]
id: ECOSIM:RechargEastSubSurf
name: eastern subsurface boundary water flux
is_a: ECOSIMCONCEPT:UnclassifiedVariable ! unclassified variable

[Term]
id: ECOSIM:RechargEastSurf
name: eastern surface boundary water flux
is_a: ECOSIMCONCEPT:UnclassifiedVariable ! unclassified variable

[Term]
id: ECOSIM:RechargNorthSubSurf
name: northern subsurface boundary water flux
is_a: ECOSIMCONCEPT:UnclassifiedVariable ! unclassified variable

[Term]
id: ECOSIM:RechargNorthSurf
name: northern surface boundary water flux
is_a: ECOSIMCONCEPT:UnclassifiedVariable ! unclassified variable

[Term]
id: ECOSIM:RechargRateEastWTBL
name: eastern subsurface boundary water flux rate constant
is_a: ECOSIMCONCEPT:UnclassifiedVariable ! unclassified variable
relationship: has_unit ECOSIM:h-1 ! h-1

[Term]
id: ECOSIM:RechargRateNorthWTBL
name: northern subsurface boundary water flux rate constant
is_a: ECOSIMCONCEPT:UnclassifiedVariable ! unclassified variable
relationship: has_unit ECOSIM:h-1 ! h-1

[Term]
id: ECOSIM:RechargRateSouthWTBL
name: southern subsurface boundary water flux rate constant
is_a: ECOSIMCONCEPT:UnclassifiedVariable ! unclassified variable
relationship: has_unit ECOSIM:h-1 ! h-1

[Term]
id: ECOSIM:RechargRateWestWTBL
name: western subsurface boundary water flux rate constant
is_a: ECOSIMCONCEPT:UnclassifiedVariable ! unclassified variable
relationship: has_unit ECOSIM:h-1 ! h-1

[Term]
id: ECOSIM:RechargSouthSubSurf
name: southern subsurface boundary water flux
is_a: ECOSIMCONCEPT:UnclassifiedVariable ! unclassified variable

[Term]
id: ECOSIM:RechargSouthSurf
name: southern surface boundary water flux
is_a: ECOSIMCONCEPT:UnclassifiedVariable ! unclassified variable

[Term]
id: ECOSIM:RechargWestSubSurf
name: western subsurface boundary water flux
is_a: ECOSIMCONCEPT:UnclassifiedVariable ! unclassified variable

[Term]
id: ECOSIM:RechargWestSurf
name: western surface boundary water flux
is_a: ECOSIMCONCEPT:UnclassifiedVariable ! unclassified variable

[Term]
id: ECOSIM:ReductVLsoiAirPM
name: change in soil air volume for layer from last to current iteration
is_a: ECOSIMCONCEPT:UnclassifiedVariable ! unclassified variable
relationship: has_unit ECOSIM:gd-2t-1 ! g d-2 t-1

[Term]
id: ECOSIM:RootFracRemobilizableBiom
name: fraction of remobilizable nonstructural biomass in root
is_a: ECOSIM:CATEGORYRootPhysiology ! category - root physiology

[Term]
id: ECOSIM:RootLenDensNLP
name: root length density in soil layers
is_a: ECOSIM:CATEGORYRootPhysiology ! category - root physiology
relationship: has_unit ECOSIM:mm-3 ! m m-3

[Term]
id: ECOSIM:RootLenPerP
name: root layer length per plant
is_a: ECOSIM:CATEGORYRootPhysiology ! category - root physiology
relationship: has_unit ECOSIM:mp-1 ! m p-1

[Term]
id: ECOSIM:RootNonstructElementConcpft_vr
name: root layer nonstructural element concentration
def: "Root layer nonstructural element concentration refers to the concentration of nonstructural elements, such as carbohydrates and sugars, within the root layer of a terrestrial ecosystem. Nonstructural elements are organic compounds that are not part of the plant's structural tissues but are important for energy storage and metabolism. The concentration of these elements in the root layer can influence various processes, including nutrient uptake, plant growth, and carbon cycling within the ecosystem. This parameter is relevant for earth system modeling as it provides insights into the carbon dynamics and functioning of terrestrial ecosystems." []
is_a: ECOSIMCONCEPT:UnclassifiedVariable ! unclassified variable
relationship: has_unit ECOSIM:gg-1 ! g g-1

[Term]
id: ECOSIM:RootPoreTortu4Gas
name: power function of root porosity used to calculate root gaseous diffusivity
def: "Power function of root porosity used to calculate root gaseous diffusivity. This value is used in modeling to adjust for the deviation of gas diffusion in roots from the ideal linear relationship due to the complex structure and tortuosity of root pores." []
is_a: ECOSIM:CATEGORYRootPhysiology ! category - root physiology

[Term]
id: ECOSIM:RootPorosity
name: root porosity
def: "Root porosity refers to the percentage of the total root volume that is not occupied by plant cells or materials. This includes air spaces and intercellular spaces within the root structure. Root porosity is an important factor in determining a plant's ability to uptake water and nutrients from the soil, and can be influenced by factors such as root architecture, soil conditions, and water availability." []
is_a: ECOSIM:CATEGORYPlantPhysiology ! category - plant physiology
is_a: ECOSIM:CATEGORYRootPhysiology ! category - root physiology
relationship: has_unit ECOSIM:m3m-3 ! m3 m-3
relationship: measured_in ECOSIMCONCEPT:Root ! Root

[Term]
id: ECOSIM:RootProteinConc_pftvr
name: root layer protein C concentration
def: "Root layer protein C concentration refers to the concentration of organic carbon in the root layer of the soil. It represents the amount of carbon contained in proteins found in the roots of plants within a given area of soil. This parameter is important in earth systems modeling as it influences nutrient uptake, soil carbon dynamics, and soil microbial activity." []
is_a: ECOSIMCONCEPT:UnclassifiedVariable ! unclassified variable
relationship: has_unit ECOSIM:gg-1 ! g g-1

[Term]
id: ECOSIM:RoughHeight
name: canopy surface roughness height
is_a: ECOSIMCONCEPT:UnclassifiedVariable ! unclassified variable
relationship: has_unit ECOSIM:m ! m

[Term]
id: ECOSIM:RunoffVelocity
name: runoff velocity
is_a: ECOSIMCONCEPT:UnclassifiedVariable ! unclassified variable
relationship: has_unit ECOSIM:mt-1 ! m t-1

[Term]
id: ECOSIM:SCO2
name: leaf CO2 solubility
def: "Leaf CO2 solubility refers to the degree to which carbon dioxide (CO2) is dissolvable or soluble in the leaves of a plant. It is an important parameter in plant physiology and earth system modeling, as it directly affects the rate of photosynthesis, plant growth, and carbon cycling." []
is_a: ECOSIM:CATEGORYCanopyPhysiology ! category - Canopy Physiology
is_a: ECOSIM:CATEGORYPlantPhysiology ! category - plant physiology
relationship: has_unit ECOSIM:uM/umolmol-1 ! uM /umol mol-1
relationship: measured_in ECOSIMCONCEPT:Leaf ! Leaf
relationship: measurement_of ECOSIMCONCEPT:CO2 ! Carbon dioxide

[Term]
id: ECOSIM:SDMX
name: maximum grain number per node
is_a: ECOSIM:CATEGORYCanopyStructure ! category - canopy structure
is_a: ECOSIM:CATEGORYPlantPhysiology ! category - plant physiology
relationship: attribute ECOSIMCONCEPT:GrainNumber ! GrainNumber
relationship: attribute ECOSIMCONCEPT:Number ! Number
relationship: measured_in ECOSIMCONCEPT:Node ! Node
relationship: measurement_of ECOSIMCONCEPT:Grain ! Grain

[Term]
id: ECOSIM:SED
name: sediment transport
is_a: ECOSIMCONCEPT:UnclassifiedVariable ! unclassified variable
relationship: has_unit ECOSIM:Mgd-2h-1 ! Mg d-2 h-1

[Term]
id: ECOSIM:SL
name: slope
is_a: ECOSIMCONCEPT:UnclassifiedVariable ! unclassified variable
relationship: has_unit ECOSIM:o ! o

[Term]
id: ECOSIM:SLA1
name: leaf area:mass during growth
def: "Leaf area:mass during growth refers to the ratio of the surface area of a leaf to its mass during the plant's growth phase. It is often used as an indicator of plant growth and health, as well as a measure of the plant's photosynthetic capacity." []
is_a: ECOSIM:CATEGORYCanopyPhysiology ! category - Canopy Physiology
is_a: ECOSIM:CATEGORYCanopyStructure ! category - canopy structure
is_a: ECOSIM:CATEGORYPlantPhysiology ! category - plant physiology
relationship: context ECOSIMCONCEPT:Growth ! Growth
relationship: has_unit ECOSIM:m2g-1 ! m2 g-1
relationship: measured_in ECOSIMCONCEPT:Leaf ! Leaf
relationship: measurement_of ECOSIMCONCEPT:Area ! Area
relationship: measurement_of ECOSIMCONCEPT:Mass ! Mass

[Term]
id: ECOSIM:SNL1
name: internode length:mass during growth
def: "Internode length:mass during growth refers to the ratio of internode length to mass during the growth phase of a plant. This measure can provide insights into the growth patterns and overall health of the plant." []
is_a: ECOSIM:CATEGORYCanopyStructure ! category - canopy structure
relationship: attribute ECOSIMCONCEPT:Mass ! Mass
relationship: context ECOSIMCONCEPT:Growth ! Growth
relationship: has_unit ECOSIM:mg-1 ! m g-1
relationship: measured_in ECOSIMCONCEPT:Internode ! Internode

[Term]
id: ECOSIM:SO2
name: leaf O2 solubility
def: "Leaf O2 solubility refers to the measurement of the amount of oxygen (O2) that can be dissolved in the leaf tissue at a particular temperature and pressure. It is an essential parameter in earth system and plant physiology modeling as it affects the process of photosynthesis, respiration, and transpiration." []
is_a: ECOSIM:CATEGORYCanopyPhysiology ! category - Canopy Physiology
is_a: ECOSIM:CATEGORYPlantPhysiology ! category - plant physiology
relationship: has_unit ECOSIM:uM/umolmol-1 ! uM /umol mol-1
relationship: measured_in ECOSIMCONCEPT:Leaf ! Leaf
relationship: measurement_of ECOSIMCONCEPT:Oxygen ! Oxygen

[Term]
id: ECOSIM:SOSGL
name: aqueous SO4 diffusivity
is_a: ECOSIMCONCEPT:UnclassifiedVariable ! unclassified variable
relationship: has_unit ECOSIM:m2h-1 ! m2 h-1

[Term]
id: ECOSIM:SSIN
name: sine of solar angle
is_a: ECOSIMCONCEPT:UnclassifiedVariable ! unclassified variable

[Term]
id: ECOSIM:SSINN
name: sine of solar angle next hour
is_a: ECOSIMCONCEPT:UnclassifiedVariable ! unclassified variable

[Term]
id: ECOSIM:SSL1
name: petiole length:mass during growth
is_a: ECOSIM:CATEGORYCanopyStructure ! category - canopy structure
is_a: ECOSIM:CATEGORYPlantPhysiology ! category - plant physiology
relationship: attribute ECOSIMCONCEPT:Mass ! Mass
relationship: has_unit ECOSIM:mg-1 ! m g-1
relationship: measured_in ECOSIMCONCEPT:Growth ! Growth

[Term]
id: ECOSIM:STMX
name: maximum grain node number per branch
def: "Maximum grain node number per branch refers to the maximum number of grain nodes that can be present on a single branch of the plant. This measurement is crucial for understanding the productivity potential of crop varieties, as the number of grain nodes directly impact the yield." []
is_a: ECOSIM:CATEGORYCanopyStructure ! category - canopy structure
relationship: attribute ECOSIMCONCEPT:Number ! Number
relationship: measured_in ECOSIMCONCEPT:Branch ! Branch

[Term]
id: ECOSIM:SWRadByCanP
name: canopy absorbed shortwave radiation
def: "Canopy absorbed shortwave radiation generally refers to the amount of incoming shortwave solar radiation that is absorbed by the leaves of the plant canopy. It is a key component of the overall energy balance of terrestrial ecosystems, influencing processes such as temperature regulation, photosynthesis, and evapotranspiration. Measurement of this factor is essential for understanding and modeling ecosystem energy dynamics." []
is_a: ECOSIM:CATEGORYPlantPhysiology ! category - plant physiology
is_a: ECOSIM:CATEGORYSurfaceEnergyBalance ! category - Surface Energy Balance
relationship: has_unit ECOSIM:MJd-2h-1 ! MJ d-2 h-1
relationship: measured_in ECOSIMCONCEPT:Canopy ! Canopy
relationship: measurement_of ECOSIMCONCEPT:ShortwaveRadiation ! ShortwaveRadiation

[Term]
id: ECOSIM:SWRadOnGrnd
name: radiation intercepted by ground surface
is_a: ECOSIMCONCEPT:UnclassifiedVariable ! unclassified variable
relationship: has_unit ECOSIM:MJm-2h-1 ! MJ m-2 h-1

[Term]
id: ECOSIM:SatHydroCondHrzn
name: soil horizontal saturated hydraulic conductivity
is_a: ECOSIMCONCEPT:UnclassifiedVariable ! unclassified variable
relationship: has_unit ECOSIM:mmh-1 ! mm h-1

[Term]
id: ECOSIM:SecndRootLen
name: root layer length secondary axes
def: "Secondary root length refers to the length of the secondary, or lateral, roots in a plant's root system. Secondary roots develop from the primary root and enhance the root system's ability to anchor the plant and absorb water and nutrients from the soil. This measure can vary greatly depending on plant species, age, and environmental conditions." []
is_a: ECOSIM:CATEGORYRootPhysiology ! category - root physiology
relationship: has_unit ECOSIM:md-2 ! m d-2
relationship: measured_in ECOSIMCONCEPT:Root ! Root
relationship: measured_in ECOSIMCONCEPT:RootLayer ! Root layer

[Term]
id: ECOSIM:SecndRootRadius
name: root layer diameter secondary axes
is_a: ECOSIM:CATEGORYRootPhysiology ! category - root physiology
relationship: has_unit ECOSIM:m ! m

[Term]
id: ECOSIM:SecndRootSpecLen
name: specific root length secondary axes
is_a: ECOSIM:CATEGORYRootPhysiology ! category - root physiology
relationship: has_unit ECOSIM:mg-1 ! m g-1

[Term]
id: ECOSIM:SecndRootXNumL
name: root layer number axes
is_a: ECOSIM:CATEGORYRootPhysiology ! category - root physiology
relationship: has_unit ECOSIM:d-2 ! d-2

[Term]
id: ECOSIM:SecndRootXSecArea
name: root cross-sectional area secondary axes
is_a: ECOSIM:CATEGORYRootPhysiology ! category - root physiology
relationship: has_unit ECOSIM:m2 ! m2

[Term]
id: ECOSIM:SeedArea
name: seed surface area
def: "Seed surface area refers to the measurement of the total exterior surface of a given seed. This measurement can provide insights into seed physiology, dispersal potential, and growth rate, among other things. It is an important parameter in ecology and plant biology research." []
is_a: ECOSIM:CATEGORYCanopyStructure ! category - canopy structure
is_a: ECOSIM:CATEGORYPlantPhysiology ! category - plant physiology
relationship: attribute ECOSIMCONCEPT:Area ! Area
relationship: has_unit ECOSIM:m2 ! m2
relationship: measured_in ECOSIMCONCEPT:Seed ! Seed
relationship: measurement_of ECOSIMCONCEPT:Seed ! Seed

[Term]
id: ECOSIM:SeedCMass
name: grain size at seeding
is_a: ECOSIM:CATEGORYCanopyStructure ! category - canopy structure
relationship: has_unit ECOSIM:g ! g

[Term]
id: ECOSIM:SeedLength
name: seed length
def: "Seed length is the measurement of the longest dimension of a seed. This measurement can be important for classification and identification of plant species, as well as determining the maturity and viability of seeds for sowing." []
is_a: ECOSIM:CATEGORYCanopyStructure ! category - canopy structure
relationship: has_unit ECOSIM:m ! m
relationship: measurement_of ECOSIMCONCEPT:Seed ! Seed

[Term]
id: ECOSIM:SeedVolume
name: seed volume
is_a: ECOSIM:CATEGORYCanopyStructure ! category - canopy structure
relationship: has_unit ECOSIM:m3 ! m3

[Term]
id: ECOSIM:SeedinDepth
name: seeding depth
def: "Seeding depth refers to the depth at which seeds are planted in the soil. It is a critical factor for successful germination and establishment of plants as it can affect the ability of the seed to obtain necessary moisture, oxygen, and light (if light is required for germination)." []
is_a: ECOSIM:CATEGORYCanopyStructure ! category - canopy structure
relationship: context ECOSIMCONCEPT:Seed ! Seed
relationship: has_unit ECOSIM:m ! m
relationship: measured_in ECOSIMCONCEPT:Soil ! Soil
relationship: measurement_of ECOSIMCONCEPT:Depth ! Depth

[Term]
id: ECOSIM:SnoDensL
name: snowpack density
def: "Snowpack density refers to the mass of snow contained in a given volume of snowpack. It is an essential parameter in understanding the characteristics of a snowpack and its water equivalence. A higher snow density indicates that the snowpack has a higher water content." []
is_a: ECOSIM:CATEGORYSnowpack ! category - Snowpack
is_a: ECOSIMCONCEPT:Snowpack ! Snowpack
relationship: has_unit ECOSIM:Mgm-3 ! Mg m-3
relationship: measurement_of ECOSIMCONCEPT:Snowpack ! Snowpack

[Term]
id: ECOSIM:SnoFalPrec
name: snowfall
def: "Snowfall refers to the amount of snow that falls in a specific area in a certain time period. It is usually measured in millimeters or inches of water equivalent. Snowfall is an important aspect in climate and weather studies, as it affects factors such as surface albedo, soil moisture levels, hydrology, and ecosystem dynamics." []
is_a: ECOSIM:CATEGORYAtmosphericConditions ! category - Atmospheric Conditions
relationship: attribute ECOSIMCONCEPT:Precipitation ! Precipitation
relationship: has_unit ECOSIM:m3d-2h-1 ! m3 d-2 h-1
relationship: measured_in ECOSIMCONCEPT:Air ! Air

[Term]
id: ECOSIM:SnowDepth
name: snowpack depth
def: "Snowpack depth refers to the total depth of snow and ice on the ground in mountainous or high altitude regions. This depth can vary greatly due to factors such as precipitation, temperature, and wind. Measuring this depth helps in understanding the water resource availability in such regions, as this snow will melt and provide water supply." []
is_a: ECOSIM:CATEGORYSnowpack ! category - Snowpack
relationship: attribute ECOSIMCONCEPT:Depth ! Depth
relationship: has_unit ECOSIM:m ! m
relationship: measured_in ECOSIMCONCEPT:Snowpack ! Snowpack

[Term]
id: ECOSIM:SoiBulkDensity
name: soil bulk density
is_a: ECOSIMCONCEPT:UnclassifiedVariable ! unclassified variable
relationship: has_unit ECOSIM:Mgm-3 ! Mg m-3

[Term]
id: ECOSIM:SoiSurfRoughness
name: soil surface roughness height for calculating runoff velocity
is_a: ECOSIMCONCEPT:UnclassifiedVariable ! unclassified variable
relationship: has_unit ECOSIM:m ! m

[Term]
id: ECOSIM:SoiSurfRoughnesst0
name: initial soil surface roughness height
is_a: ECOSIMCONCEPT:UnclassifiedVariable ! unclassified variable
relationship: has_unit ECOSIM:m ! m

[Term]
id: ECOSIM:SoilDetachability4Erosion1
name: soil detachment
is_a: ECOSIMCONCEPT:UnclassifiedVariable ! unclassified variable

[Term]
id: ECOSIM:SoilHeatSrcDepth
name: depth of soil heat sink/source
is_a: ECOSIMCONCEPT:UnclassifiedVariable ! unclassified variable
relationship: has_unit ECOSIM:m ! m

[Term]
id: ECOSIM:SoilResit4RootPentration
name: soil hydraulic resistance
is_a: ECOSIMCONCEPT:UnclassifiedVariable ! unclassified variable
relationship: has_unit ECOSIM:MPahm-2 ! MPa h m-2

[Term]
id: ECOSIM:StemA_lyrnodbrchpft
name: stem surface area
def: "Stem surface area refers to the total external surface area of the stems (trunk and branches) of plants within a specified area. It is an important parameter in earth systems modeling as it influences several ecological processes, including water uptake by plants, gas exchange with the atmosphere, and energy balance within ecosystems. Stem surface area can vary depending on the growth form and architecture of different plant species, as well as their age and environmental conditions." []
is_a: ECOSIMCONCEPT:UnclassifiedVariable ! unclassified variable
relationship: has_unit ECOSIM:m2d-2 ! m2 d-2

[Term]
id: ECOSIM:StemAreag
name: total canopy stem area
is_a: ECOSIM:CATEGORYCanopyStructure ! category - canopy structure
relationship: has_unit ECOSIM:m2d-2 ! m2 d-2

[Term]
id: ECOSIM:TAMN
name: daily minimum air temperature
def: "Daily minimum air temperature refers to the lowest temperature recorded at a specific location in a 24-hour period. It is an important variable in climate studies, agriculture, and weather forecasting. Measuring daily temperatures, including the minimum, can help to understand the local climate and its variability, as well as provide data for climate modeling and weather forecasting." []
is_a: ECOSIM:CATEGORYAtmosphericConditions ! category - Atmospheric Conditions
relationship: attribute ECOSIMCONCEPT:Temperature ! temperature
relationship: has_unit ECOSIM:oC ! oC
relationship: measured_in ECOSIMCONCEPT:Air ! Air
relationship: measurement_of ECOSIMCONCEPT:Air ! Air

[Term]
id: ECOSIM:TAMX
name: daily maximum air temperature
is_a: ECOSIM:CATEGORYAtmosphericConditions ! category - Atmospheric Conditions
relationship: attribute ECOSIMCONCEPT:Temperature ! temperature
relationship: has_unit ECOSIM:oC ! oC
relationship: measured_in ECOSIMCONCEPT:Air ! Air
relationship: measurement_of ECOSIMCONCEPT:Air ! Air

[Term]
id: ECOSIM:TAU0
name: fraction of radiation transmitted by canopy layer
is_a: ECOSIM:CATEGORYAtmosphericConditions ! category - Atmospheric Conditions
is_a: ECOSIM:CATEGORYPlantPhysiology ! category - plant physiology
is_a: ECOSIM:CATEGORYSurfaceEnergyBalance ! category - Surface Energy Balance
relationship: attribute ECOSIMCONCEPT:Fraction ! Fraction
relationship: measured_in ECOSIMCONCEPT:Canopy ! Canopy
relationship: measured_in ECOSIMCONCEPT:CanopyLayer ! CanopyLayer
relationship: measurement_of ECOSIMCONCEPT:Radiation ! Radiation
relationship: qualifier ECOSIMCONCEPT:Fraction ! Fraction

[Term]
id: ECOSIM:TAUP
name: canopy PAR transmissivity
def: "Canopy PAR transmissivity (TAUP) refers to the fraction of incident Photosynthetic Active Radiation (PAR) that is transmitted through the canopy without being absorbed or reflected. It depends on factors such as leaf area, leaf angle distribution, and radiation conditions. TAUP is a key parameter in modeling light distribution and photosynthetic activity in plant canopies." []
is_a: ECOSIM:CATEGORYPlantPhysiology ! category - plant physiology
relationship: measured_in ECOSIMCONCEPT:Canopy ! Canopy
relationship: measurement_of ECOSIMCONCEPT:PhotosyntheticallyActiveRadiation ! PhotosyntheticallyActiveRadiation

[Term]
id: ECOSIM:TAUR
name: canopy shortwave transmissivity
is_a: ECOSIMCONCEPT:UnclassifiedVariable ! unclassified variable

[Term]
id: ECOSIM:TAUS
name: fraction of radiation intercepted by canopy layer
def: "Fraction of radiation intercepted by canopy layer (TAUS) refers to the proportion of the incident solar radiation that is intercepted or absorbed by a specified canopy layer in an ecosystem. TAUS is an important parameter in biophysical and ecological modeling because it influences processes such as photosynthesis, energy balance, and microclimate conditions within the canopy. It is determined by factors including leaf area index (LAI), leaf angle distribution, canopy architecture, and optical properties of leaves." []
is_a: ECOSIM:CATEGORYPlantPhysiology ! category - plant physiology
is_a: ECOSIM:CATEGORYSurfaceEnergyBalance ! category - Surface Energy Balance
relationship: attribute ECOSIMCONCEPT:Fraction ! Fraction
relationship: measured_in ECOSIMCONCEPT:CanopyLayer ! CanopyLayer

[Term]
id: ECOSIM:TBCO2
name: total solute CO2 transformation boundary
is_a: ECOSIMCONCEPT:UnclassifiedVariable ! unclassified variable
relationship: has_unit ECOSIM:mold-2h-1 ! mol d-2 h-1

[Term]
id: ECOSIM:TBION
name: total solute ion transformation boundary
is_a: ECOSIMCONCEPT:UnclassifiedVariable ! unclassified variable
relationship: has_unit ECOSIM:mold-2h-1 ! mol d-2 h-1

[Term]
id: ECOSIM:TCA
name: air temperature
is_a: ECOSIMCONCEPT:UnclassifiedVariable ! unclassified variable
relationship: has_unit ECOSIM:oC ! oC

[Term]
id: ECOSIM:TCC
name: canopy temperature
is_a: ECOSIMCONCEPT:UnclassifiedVariable ! unclassified variable
relationship: has_unit ECOSIM:oC ! oC

[Term]
id: ECOSIM:TCG
name: canopy growth temperature
def: "Canopy growth temperature refers to the temperature conditions under which plant canopy grows. It can refer to both the actual temperature experienced by the plants and the optimal temperature for the growth of the canopy. Canopy growth temperature influences photosynthesis, respiration, and several other physiological processes. It is crucial for modeling and predicting plant growth and development in response to changing climate conditions." []
is_a: ECOSIM:CATEGORYCanopyStructure ! category - canopy structure
is_a: ECOSIM:CATEGORYPlantPhysiology ! category - plant physiology
is_a: ECOSIM:CATEGORYPlantPopulation ! category - Plant Population
relationship: attribute ECOSIMCONCEPT:Growth ! Growth
relationship: context ECOSIMCONCEPT:Growth ! Growth
relationship: has_unit ECOSIM:oC ! oC
relationship: measured_in ECOSIMCONCEPT:Canopy ! Canopy
relationship: measurement_of ECOSIMCONCEPT:Temperature ! temperature

[Term]
id: ECOSIM:TCNET
name: total canopy net CO2 exchange
is_a: ECOSIMCONCEPT:UnclassifiedVariable ! unclassified variable
relationship: has_unit ECOSIM:gd-2h-1 ! g d-2 h-1

[Term]
id: ECOSIM:TCO2A
name: total autotrophic respiration
is_a: ECOSIMCONCEPT:UnclassifiedVariable ! unclassified variable
relationship: has_unit ECOSIM:gd-2 ! g d-2

[Term]
id: ECOSIM:TCO2P
name: total root CO2 flux
is_a: ECOSIMCONCEPT:UnclassifiedVariable ! unclassified variable
relationship: has_unit ECOSIM:gd-2h-1 ! g d-2 h-1

[Term]
id: ECOSIM:TCO2S
name: total root-soil CO2 flux
is_a: ECOSIMCONCEPT:UnclassifiedVariable ! unclassified variable
relationship: has_unit ECOSIM:gd-2h-1 ! g d-2 h-1

[Term]
id: ECOSIM:TCO2T
name: total plant respiration
is_a: ECOSIMCONCEPT:UnclassifiedVariable ! unclassified variable
relationship: has_unit ECOSIM:gd-2 ! g d-2

[Term]
id: ECOSIM:TCSnow
name: snow temperature
def: "Snow temperature (TCSnow) refers to the temperature of the snowpack. This parameter is typically expressed in degrees Celsius and can vary significantly within the snowpack, affecting various processes such as snow melting, sublimation, compaction, and metamorphosis. Snow temperature is crucial for understanding and predicting various snow-related phenomena and has important implications for ecosystem dynamics, climate change studies, and water resource management." []
is_a: ECOSIM:CATEGORYSnowpack ! category - Snowpack
relationship: attribute ECOSIMCONCEPT:Temperature ! temperature
relationship: has_unit ECOSIM:oC ! oC
relationship: measured_in ECOSIMCONCEPT:Snow ! Snow

[Term]
id: ECOSIM:TCX
name: threshold temperature for autumn leafoff/hardening
def: "The threshold temperature for autumn leafoff/hardening is the estimated temperature at which plants begin to prepare for winter. This involves processes such as leaf drop (leafoff) in deciduous trees and hardening (development of resistance to freezing) in many types of plants." []
is_a: ECOSIM:CATEGORYCanopyPhysiology ! category - Canopy Physiology
is_a: ECOSIM:CATEGORYCanopyStructure ! category - canopy structure
is_a: ECOSIM:CATEGORYPlantPhysiology ! category - plant physiology
relationship: has_unit ECOSIM:oC ! oC
relationship: measured_in ECOSIMCONCEPT:Plant ! Plant
relationship: measurement_of ECOSIMCONCEPT:Temperature ! temperature

[Term]
id: ECOSIM:TCZ
name: threshold temperature for spring leafout/dehardening
def: "The threshold temperature for spring leafout/dehardening, often abbreviated as TCZ, refers to the specific temperature at which plants begin to deharden or soften their tissue and produce new leaves in spring. It is a critical parameter in plant phenology and earth systems modeling, indicating the response of plants to changing seasonal temperatures." []
is_a: ECOSIM:CATEGORYCanopyPhysiology ! category - Canopy Physiology
is_a: ECOSIM:CATEGORYCanopyStructure ! category - canopy structure
is_a: ECOSIM:CATEGORYPlantPhysiology ! category - plant physiology
relationship: attribute ECOSIMCONCEPT:Temperature ! temperature
relationship: context ECOSIMCONCEPT:Dehardening ! Dehardening
relationship: context ECOSIMCONCEPT:SpringLeafout ! Spring leaf out
relationship: has_unit ECOSIM:oC ! oC
relationship: measurement_of ECOSIMCONCEPT:Dehardening ! Dehardening
relationship: measurement_of ECOSIMCONCEPT:Leafout ! Leaf out

[Term]
id: ECOSIM:TDCN4
name: accumulated change for NH4 in precipitation
is_a: ECOSIMCONCEPT:UnclassifiedVariable ! unclassified variable

[Term]
id: ECOSIM:TDCNO
name: accumulated change for NO3 in precipitation
is_a: ECOSIMCONCEPT:UnclassifiedVariable ! unclassified variable

[Term]
id: ECOSIM:TDCO2
name: accumulated change for atmospheric CO2 concentration
is_a: ECOSIMCONCEPT:UnclassifiedVariable ! unclassified variable

[Term]
id: ECOSIM:TDFOME
name: total root element exchange
is_a: ECOSIMCONCEPT:UnclassifiedVariable ! unclassified variable
relationship: has_unit ECOSIM:gd-2h-1 ! g d-2 h-1

[Term]
id: ECOSIM:TDHUM
name: accumulated change for humidity
is_a: ECOSIMCONCEPT:UnclassifiedVariable ! unclassified variable

[Term]
id: ECOSIM:TDIRI
name: accumulated change for irrigation
is_a: ECOSIMCONCEPT:UnclassifiedVariable ! unclassified variable

[Term]
id: ECOSIM:TDPRC
name: accumulated change for precipitation
is_a: ECOSIMCONCEPT:UnclassifiedVariable ! unclassified variable

[Term]
id: ECOSIM:TDRAD
name: accumulated change for radiation
is_a: ECOSIMCONCEPT:UnclassifiedVariable ! unclassified variable

[Term]
id: ECOSIM:TDTPN
name: accumulated change for minimum temperature
is_a: ECOSIMCONCEPT:UnclassifiedVariable ! unclassified variable

[Term]
id: ECOSIM:TDWND
name: accumulated change for wind speed
is_a: ECOSIMCONCEPT:UnclassifiedVariable ! unclassified variable

[Term]
id: ECOSIM:TENGYC
name: total canopy heat content
is_a: ECOSIMCONCEPT:UnclassifiedVariable ! unclassified variable
relationship: has_unit ECOSIM:MJd-2 ! MJ d-2

[Term]
id: ECOSIM:TESN0
name: total surface litterfall element
is_a: ECOSIMCONCEPT:UnclassifiedVariable ! unclassified variable
relationship: has_unit ECOSIM:gd-2 ! g d-2

[Term]
id: ECOSIM:TESNC
name: total plant element litterfall
is_a: ECOSIMCONCEPT:UnclassifiedVariable ! unclassified variable
relationship: has_unit ECOSIM:gd-2 ! g d-2

[Term]
id: ECOSIM:TEUPTK
name: total net root element uptake (+ve) - exudation (-ve)
is_a: ECOSIMCONCEPT:UnclassifiedVariable ! unclassified variable
relationship: has_unit ECOSIM:gd-2 ! g d-2

[Term]
id: ECOSIM:TEVAPP
name: total canopy evaporation + transpiration
is_a: ECOSIMCONCEPT:UnclassifiedVariable ! unclassified variable
relationship: has_unit ECOSIM:m3d-2 ! m3 d-2

[Term]
id: ECOSIM:TFLWCI
name: net ice transfer to canopy
is_a: ECOSIMCONCEPT:UnclassifiedVariable ! unclassified variable
relationship: has_unit ECOSIM:MJd-2t-1 ! MJ d-2 t-1

[Term]
id: ECOSIM:TFNQ
name: constraints of temperature and water potential on microbial activity
def: "Constraints of temperature and water potential on microbial activity refers to how factors such as temperature and water potential can limit the activity of microorganisms in an environmental setting. In particular, temperature can affect microbial metabolism while water potential affects the availability of water for microbial processes." []
is_a: ECOSIM:CATEGORYNTransformation ! category - N transformation
relationship: attribute ECOSIMCONCEPT:Constraint ! Constraint
relationship: attribute ECOSIMCONCEPT:Temperature ! temperature
relationship: measurement_of ECOSIMCONCEPT:Constraint ! Constraint

[Term]
id: ECOSIM:TGH
name: ecosystem storage heat flux
is_a: ECOSIMCONCEPT:UnclassifiedVariable ! unclassified variable
relationship: has_unit ECOSIM:MJd-2h-1 ! MJ d-2 h-1

[Term]
id: ECOSIM:TGPP
name: ecosystem GPP
is_a: ECOSIMCONCEPT:UnclassifiedVariable ! unclassified variable
relationship: has_unit ECOSIM:gd-2h-1 ! g d-2 h-1

[Term]
id: ECOSIM:TGSTGF
name: normalized node number during reproductive growth stages
def: "Normalized node number during reproductive growth stages refers to the average number of nodes (junction points from where leaves, branches or flowers grow) a plant produces during its reproductive growth phase, normalized under some standard conditions. It helps plant physiologists to understand plant architecture and growth dynamics during reproductive phase." []
is_a: ECOSIM:CATEGORYCanopyStructure ! category - canopy structure
is_a: ECOSIM:CATEGORYPlantPhysiology ! category - plant physiology
relationship: attribute ECOSIMCONCEPT:Number ! Number
relationship: measurement_of ECOSIMCONCEPT:Node ! Node
relationship: measurement_of ECOSIMCONCEPT:NodeNumber ! NodeNumber

[Term]
id: ECOSIM:TGSTGI
name: normalized node number during vegetative growth stages
def: "Normalized node number during vegetative growth stages is a measure used to describe the progress of a plant through its developmental stages. It is calculated by dividing the current node number by the total node number at maturity, giving a relative measure of growth progress." []
is_a: ECOSIM:CATEGORYCanopyStructure ! category - canopy structure
is_a: ECOSIM:CATEGORYPlantPhysiology ! category - plant physiology
relationship: attribute ECOSIMCONCEPT:NodeNumber ! NodeNumber
relationship: measured_in ECOSIMCONCEPT:Plant ! Plant
relationship: measurement_of ECOSIMCONCEPT:NodeNumber ! NodeNumber

[Term]
id: ECOSIM:TH2GZ
name: total root H2 flux
is_a: ECOSIMCONCEPT:UnclassifiedVariable ! unclassified variable
relationship: has_unit ECOSIM:gd-2 ! g d-2

[Term]
id: ECOSIM:THETPM
name: soil air-filled porosity
is_a: ECOSIMCONCEPT:UnclassifiedVariable ! unclassified variable
relationship: has_unit ECOSIM:m3m-3 ! m3 m-3

[Term]
id: ECOSIM:THETY
name: air-dry water content
is_a: ECOSIMCONCEPT:UnclassifiedVariable ! unclassified variable
relationship: has_unit ECOSIM:m3m-3 ! m3 m-3

[Term]
id: ECOSIM:THFLXC
name: total canopy heat flux
is_a: ECOSIMCONCEPT:UnclassifiedVariable ! unclassified variable
relationship: has_unit ECOSIM:MJd-2 ! MJ d-2

[Term]
id: ECOSIM:THIN_pft
name: thinning of plant population
def: "Thinning of plant population refers to the process of reducing the density or abundance of plants within a given area. It involves selectively removing certain individuals or groups of plants to create more space and resources for the remaining plants to grow and thrive. Thinning can be done manually or through natural processes such as competition, predation, or disease. The purpose of thinning plant populations in earth systems modeling is to simulate realistic vegetation dynamics, including changes in species composition, productivity, and ecosystem functioning." []
is_a: ECOSIMCONCEPT:UnclassifiedVariable ! unclassified variable

[Term]
id: ECOSIM:THRE
name: ecosystem heterotrophic respiration
is_a: ECOSIMCONCEPT:UnclassifiedVariable ! unclassified variable
relationship: has_unit ECOSIM:gd-2h-1 ! g d-2 h-1

[Term]
id: ECOSIM:THSX
name: sky longwave radiation
def: "Sky longwave radiation refers to the energy emitted by the Earth's atmosphere in the form of longwave (also known as infrared) radiation. This type of radiation is primarily due to the greenhouse effect, where greenhouse gases in the atmosphere absorb radiation from the Earth's surface and re-emit it back to the surface and space. Longwave radiation plays a crucial role in the Earth's energy balance and in determining the temperature of the Earth's surface and atmosphere." []
is_a: ECOSIM:CATEGORYAtmosphericConditions ! category - Atmospheric Conditions
relationship: attribute ECOSIMCONCEPT:Radiation ! Radiation
relationship: has_unit ECOSIM:MJm-2h-1 ! MJ m-2 h-1
relationship: measured_in ECOSIMCONCEPT:Atmosphere ! Atmosphere
relationship: measurement_of ECOSIMCONCEPT:LongwaveRadiation ! LongwaveRadiation

[Term]
id: ECOSIM:THVSTE
name: total plant harvest
is_a: ECOSIMCONCEPT:UnclassifiedVariable ! unclassified variable
relationship: has_unit ECOSIM:gd-2 ! g d-2

[Term]
id: ECOSIM:THeatRootUptake
name: total root heat uptake
is_a: ECOSIMCONCEPT:UnclassifiedVariable ! unclassified variable
relationship: has_unit ECOSIM:MJd-2 ! MJ d-2

[Term]
id: ECOSIM:TKC
name: canopy temperature
is_a: ECOSIMCONCEPT:UnclassifiedVariable ! unclassified variable
relationship: has_unit ECOSIM:K ! K

[Term]
id: ECOSIM:TKCZ
name: canopy temperature
is_a: ECOSIMCONCEPT:UnclassifiedVariable ! unclassified variable
relationship: has_unit ECOSIM:K ! K

[Term]
id: ECOSIM:TKG
name: canopy growth temperature
def: "Canopy growth temperature or TKG refers to the temperature at which the growth of a plant canopy is optimal. It can also refer to the average or mean temperature recorded at the canopy level of a plant or in a forested area. The measurement of TKG is important as it impacts various physiological processes of plants including photosynthesis, respiration, and transpiration." []
is_a: ECOSIM:CATEGORYCanopyStructure ! category - canopy structure
is_a: ECOSIM:CATEGORYPlantPhysiology ! category - plant physiology
relationship: attribute ECOSIMCONCEPT:Temperature ! temperature
relationship: context ECOSIMCONCEPT:Growth ! Growth
relationship: has_unit ECOSIM:K ! K
relationship: measured_in ECOSIMCONCEPT:Canopy ! Canopy

[Term]
id: ECOSIM:TKSD
name: temperature of soil heat sink/source
is_a: ECOSIMCONCEPT:UnclassifiedVariable ! unclassified variable
relationship: has_unit ECOSIM:oC ! oC

[Term]
id: ECOSIM:TKSnow
name: snow temperature
def: "Snow temperature, also referred to as TKSnow, refers to the average temperature of a snowpack. Monitoring snow temperature is important for various reasons. It can help predict avalanches, determine the speed of snowmelt, and understand the insulation value of snowpack. Data regarding snow temperature can be used in climate models to accurately simulate snow-covered regions." []
is_a: ECOSIM:CATEGORYSnowpack ! category - Snowpack
relationship: attribute ECOSIMCONCEPT:Temperature ! temperature
relationship: has_unit ECOSIM:K ! K
relationship: measured_in ECOSIMCONCEPT:Snow ! Snow
relationship: measured_in ECOSIMCONCEPT:Snowpack ! Snowpack

[Term]
id: ECOSIM:TLE
name: ecosystem latent heat flux
is_a: ECOSIMCONCEPT:UnclassifiedVariable ! unclassified variable
relationship: has_unit ECOSIM:MJd-2h-1 ! MJ d-2 h-1

[Term]
id: ECOSIM:TLEC
name: total latent heat flux x boundary layer resistance
is_a: ECOSIMCONCEPT:UnclassifiedVariable ! unclassified variable
relationship: has_unit ECOSIM:MJm-1 ! MJ m-1

[Term]
id: ECOSIM:TLEX
name: total latent heat flux x boundary layer resistance
is_a: ECOSIMCONCEPT:UnclassifiedVariable ! unclassified variable
relationship: has_unit ECOSIM:MJm-1 ! MJ m-1

[Term]
id: ECOSIM:TLitrIceFlxThaw
name: water from ice thaw in surface litter
is_a: ECOSIMCONCEPT:UnclassifiedVariable ! unclassified variable
relationship: has_unit ECOSIM:m3d-2h-1 ! m3 d-2 h-1

[Term]
id: ECOSIM:TLitrIceHeatFlxFrez
name: latent heat released from water freeze in surface litter
is_a: ECOSIMCONCEPT:UnclassifiedVariable ! unclassified variable
relationship: has_unit ECOSIM:MJd-2h-1 ! MJ d-2 h-1

[Term]
id: ECOSIM:TNBP
name: total NBP
is_a: ECOSIMCONCEPT:UnclassifiedVariable ! unclassified variable
relationship: has_unit ECOSIM:gd-2 ! g d-2

[Term]
id: ECOSIM:TNH3C
name: total canopy NH3 flux
is_a: ECOSIMCONCEPT:UnclassifiedVariable ! unclassified variable
relationship: has_unit ECOSIM:gd-2 ! g d-2

[Term]
id: ECOSIM:TNPP
name: ecosystem NPP
is_a: ECOSIMCONCEPT:UnclassifiedVariable ! unclassified variable
relationship: has_unit ECOSIM:gd-2h-1 ! g d-2 h-1

[Term]
id: ECOSIM:TOMT
name: total micriobial C
def: "Total microbial C refers to the sum of all carbon stored in microbial biomass in a given soil sample. Microbial biomass plays a key role in the cycling of nutrients, including carbon, in soil ecosystems. It is an important component of soil organic matter and contributes to soil fertility. Measurements of total microbial C can be useful in assessing soil health and productivity." []
is_a: ECOSIM:CATEGORYMicrobialActivity ! category - microbial activity
relationship: has_unit ECOSIM:gd-2 ! g d-2
relationship: measured_in ECOSIMCONCEPT:MicrobialBiomass ! MicrobialBiomass
relationship: measurement_of ECOSIMCONCEPT:Carbon ! Carbon

[Term]
id: ECOSIM:TONT
name: total micriobial N
def: "Total microbial N refers to the total amount of nitrogen (N) present in microbial biomass. The microbial community in the soil plays a crucial role in decomposing organic matter and recycling nutrients such as nitrogen. This is an essential parameter in soil biosphere studies, as it helps understand nutrient cycling and the roles of microbes in soil fertility." []
is_a: ECOSIM:CATEGORYMicrobialActivity ! category - microbial activity
relationship: has_unit ECOSIM:gd-2 ! g d-2
relationship: measurement_of ECOSIMCONCEPT:Nitrogen ! Nitrogen

[Term]
id: ECOSIM:TOPT
name: total micriobial P
is_a: ECOSIM:CATEGORYMicrobialActivity ! category - microbial activity
relationship: has_unit ECOSIM:gd-2 ! g d-2

[Term]
id: ECOSIM:TRAD
name: total daily solar radiation
def: "Total daily solar radiation (TRAD) refers to the accumulated solar radiation received in a certain location over a day. This solar radiation includes not only the direct radiation from the sun, but also includes diffuse solar radiation that is scattered in the atmosphere. The value of daily solar radiation can be used in a variety of scientific fields, such as climatology, ecology, solar energy, and agriculture, to interpret and predict different environmental phenomena." []
is_a: ECOSIM:CATEGORYAtmosphericConditions ! category - Atmospheric Conditions
relationship: has_unit ECOSIM:MJd-1 ! MJ d-1
relationship: measured_in ECOSIMCONCEPT:Day ! Day

[Term]
id: ECOSIM:TRAI
name: total daily precipitation
def: "Total daily precipitation refers to the total amount of rain, snow, or other forms of moisture that falls from clouds in the sky into a specific area over a 24-hour period. It typically includes drizzle, rain, sleet, snow, graupel and hail. It is a key measurement for meteorological, hydrological and climatological considerations." []
is_a: ECOSIM:CATEGORYAtmosphericConditions ! category - Atmospheric Conditions
is_a: ECOSIMCONCEPT:Precipitation ! Precipitation
relationship: has_unit ECOSIM:md-1 ! m d-1
relationship: measured_in ECOSIMCONCEPT:Atmosphere ! Atmosphere

[Term]
id: ECOSIM:TRAU
name: ecosystem autotrophic respiration
is_a: ECOSIMCONCEPT:UnclassifiedVariable ! unclassified variable
relationship: has_unit ECOSIM:gd-2h-1 ! g d-2 h-1

[Term]
id: ECOSIM:TRCO2
name: total solute CO2 transformation
def: "Total solute CO2 transformation refers to the total alteration or conversion of solute CO2, which indicates CO2 dissolved in a solvent, in a particular system or environment over time. It's a key parameter in understanding the carbon cycle and the impact of CO2 fluxes." []
is_a: ECOSIM:CATEGORYBiogeochemistry ! category - Biogeochemistry
is_a: ECOSIM:CATEGORYElementFlux ! category - C and nutrient flux
relationship: context ECOSIMCONCEPT:Solute ! Solute
relationship: has_unit ECOSIM:mold-2h-1 ! mol d-2 h-1
relationship: measurement_of ECOSIMCONCEPT:CO2 ! Carbon dioxide

[Term]
id: ECOSIM:TRFE3
name: total solute FeOH3 transformation
def: "Total solute FeOH3 transformation refers to the total changes or conversions that the iron trihydroxide (FeOH3) solute undergoes in a given system. These transformations can include processes such as precipitation, dissolution, oxidation, reduction, sorption, desorption, or biological uptake and release. The parameter 'TRFE3' is valuable in earth systems and geochemical modeling as it influences nutrient cycling, soil formation, and the mobility and bioavailability of nutrients and contaminants." []
is_a: ECOSIM:CATEGORYElementFlux ! category - C and nutrient flux
relationship: context ECOSIMCONCEPT:Solute ! Solute
relationship: has_unit ECOSIM:mold-2h-1 ! mol d-2 h-1
relationship: measurement_of ECOSIMCONCEPT:FeOH3 ! Iron trihydroxide

[Term]
id: ECOSIM:TRH1B
name: total solute HPO4 transformation band
def: "Total solute HPO4 transformation band, referred to as TRH1B, represents the total amount of HPO4 ions that are transformed in a particular band or section of land. These transformations can include processes such as absorption, formation of complexes, precipitation, and biotransformation. This parameter is critical in understanding the biogeochemical cycling of phosphorus." []
is_a: ECOSIM:CATEGORYElementFlux ! category - C and nutrient flux
is_a: ECOSIMCONCEPT:Variable ! variable
relationship: has_unit ECOSIM:mold-2h-1 ! mol d-2 h-1
relationship: measurement_of ECOSIMCONCEPT:HPO4 ! Hydrogen phosphate

[Term]
id: ECOSIM:TRH1P
name: total solute HPO4 transformation non-band
def: "Total solute HPO4 transformation non-band refers to the total conversion of the solute HPO4 (Phosphate) that is not associated with a specific band. This could refer to conversions due to various chemical, biological, or physical processes in the soil or water. Monitoring this total conversion is important to understand nutrient dynamics in the ecosystem and can help optimize the management of soil fertility." []
is_a: ECOSIM:CATEGORYElementFlux ! category - C and nutrient flux
is_a: ECOSIM:CATEGORYSoilBiogeochemistry ! category - Soil Biogeochemistry
relationship: context ECOSIMCONCEPT:Solute ! Solute
relationship: has_unit ECOSIM:mold-2h-1 ! mol d-2 h-1
relationship: measurement_of ECOSIMCONCEPT:HPO4 ! Hydrogen phosphate

[Term]
id: ECOSIM:TRH2B
name: total solute H2PO4 transformation band
def: "Total solute H2PO4 transformation band refers to the total amount of dihydrogen phosphate (H2PO4) solute that undergoes transformation within a defined band or zone in a system. This could involve processes such as precipitation, dissolution, advection, diffusion, or biological uptake which change the form, state or location of the H2PO4 solute in the system. The parameter 'TRH2B' is important in environmental and earth system modeling as it helps in understanding phosphorus cycling and the implications for nutrient availability and water quality." []
is_a: ECOSIM:CATEGORYElementFlux ! category - C and nutrient flux
relationship: context ECOSIMCONCEPT:Solute ! Solute
relationship: has_unit ECOSIM:mold-2h-1 ! mol d-2 h-1
relationship: measured_in ECOSIMCONCEPT:Band ! Band
relationship: measurement_of ECOSIMCONCEPT:H2PO4 ! Dihydrogen phosphate

[Term]
id: ECOSIM:TRH2O
name: total solute H2O transformation
def: "Total solute H2O transformation refers to the total change in the form, structure, or composition of dissolved substances in water (H2O). It is a comprehensive measure that includes all the processes that can transform solutes in water, including biological activity (e.g., microbial degradation, plant uptake), chemical reactions (e.g., oxidation, reduction), and physical processes (e.g., sorption, volatilization). This parameter is crucial in earth systems modeling, as it determines the fate and transport of solutes in aquatic environments." []
is_a: ECOSIM:CATEGORYElementFlux ! category - C and nutrient flux
is_a: ECOSIM:CATEGORYHydrology ! category - Hydrology
relationship: has_unit ECOSIM:mold-2h-1 ! mol d-2 h-1
relationship: measured_in ECOSIMCONCEPT:Water ! Water
relationship: measurement_of ECOSIMCONCEPT:Solute ! Solute

[Term]
id: ECOSIM:TRH2P
name: total solute H2PO4 transformation non-band
def: "Total solute H2PO4 transformation non-band refers to the total conversion or chemical change of the solute dihydrogen phosphate (H2PO4-) in a non-band area, which is not restricted to a specific band or section of land. This is a vital process for the availability of phosphorus in soils and plays a significant role in plant nutrition and growth." []
is_a: ECOSIM:CATEGORYElementFlux ! category - C and nutrient flux
relationship: context ECOSIMCONCEPT:Solute ! Solute
relationship: has_unit ECOSIM:mold-2h-1 ! mol d-2 h-1
relationship: measurement_of ECOSIMCONCEPT:H2PO4 ! Dihydrogen phosphate

[Term]
id: ECOSIM:TRHCO
name: total solute HCO3 transformation
def: "Total solute HCO3 transformation refers to the total transformation of bicarbonate (HCO3) solute in a given system. This transformation can occur through various processes, such as dissolution, precipitation, or biological uptake. Understanding this transformation is crucial as HCO3 plays a significant role in maintaining pH balance in aquatic environments, influencing the ability of water bodies to buffer against acidity." []
is_a: ECOSIM:CATEGORYElementFlux ! category - C and nutrient flux
is_a: ECOSIM:CATEGORYHydrology ! category - Hydrology
relationship: context ECOSIMCONCEPT:Solute ! Solute
relationship: has_unit ECOSIM:mold-2h-1 ! mol d-2 h-1
relationship: measurement_of ECOSIMCONCEPT:HCO3 ! Bicarbonate

[Term]
id: ECOSIM:TRKAS
name: total solute KSO4 transformation
def: "Total solute KSO4 transformation refers to the total amount of transformation of solute potassium sulfate (KSO4) in the soil solution. This includes the processes of dissolution, precipitation, adsorption, desorption, and biological uptake, all of which modulate the potassium supply to plants and determine the fertility of the soil. Monitoring the transformation of KSO4 in soil solution can help understand nutrient cycling and soil fertility." []
is_a: ECOSIM:CATEGORYElementFlux ! category - C and nutrient flux
is_a: ECOSIM:CATEGORYSoilBiogeochemistry ! category - Soil Biogeochemistry
relationship: has_unit ECOSIM:mold-2h-1 ! mol d-2 h-1
relationship: measurement_of ECOSIMCONCEPT:KSO4 ! Potassium sulfate

[Term]
id: ECOSIM:TRN
name: ecosystem net radiation
is_a: ECOSIMCONCEPT:UnclassifiedVariable ! unclassified variable
relationship: has_unit ECOSIM:MJd-2h-1 ! MJ d-2 h-1

[Term]
id: ECOSIM:TRN2B
name: total solute NO2 transformation band
is_a: ECOSIMCONCEPT:UnclassifiedVariable ! unclassified variable
relationship: has_unit ECOSIM:mold-2h-1 ! mol d-2 h-1

[Term]
id: ECOSIM:TRN3B
name: total solute NH3 transformation band
def: "Total solute NH3 transformation band refers to the total amount of ammonium (NH3) in a specific soil band or layer that is transformed into other forms or compounds through various processes. These processes may include microbial activities or chemical reactions in the soil. The transformation of NH3 in soil is an important part of nitrogen cycling in ecosystems and agricultural systems and can greatly affect nutrient availability to plants." []
is_a: ECOSIM:CATEGORYElementFlux ! category - C and nutrient flux
is_a: ECOSIM:CATEGORYNTransformation ! category - N transformation
relationship: has_unit ECOSIM:mold-2h-1 ! mol d-2 h-1
relationship: measured_in ECOSIMCONCEPT:Solute ! Solute
relationship: measurement_of ECOSIMCONCEPT:NH3 ! Ammonia

[Term]
id: ECOSIM:TRN3G
name: total gaseous NH3 transformation
is_a: ECOSIMCONCEPT:UnclassifiedVariable ! unclassified variable
relationship: has_unit ECOSIM:mold-2h-1 ! mol d-2 h-1

[Term]
id: ECOSIM:TRN3S
name: total solute NH3 transformation non-band
def: "Total solute NH3 transformation (non-band) refers to the total change in the form or properties of ammonium (NH3) dissolved in a solution, not limited to a specific band or section of land. This includes processes like mineralization (conversion to mineral form), nitrification (conversion to nitrate), and immobilization (conversion to organic nitrogen compounds). The measurement helps in understanding nitrogen cycling in ecosystems." []
is_a: ECOSIM:CATEGORYElementFlux ! category - C and nutrient flux
relationship: has_unit ECOSIM:mold-2h-1 ! mol d-2 h-1
relationship: measured_in ECOSIMCONCEPT:Solution ! Solution
relationship: measurement_of ECOSIMCONCEPT:NH3 ! Ammonia

[Term]
id: ECOSIM:TRN4B
name: total solute NH4 transformation band
def: "Total solute NH4 transformation band refers to the combined total of all changes in the state, form, or properties of the ammonium ion (NH4) in the solute, within a specified band or section. It includes any process that alters the concentration or distribution of NH4, such as diffusion, reaction, dilution or loss of NH4 to the environment. The TRN4B parameter is important in understanding and modeling cycles and fluxes of nutrients and pollutants in ecosystems." []
is_a: ECOSIM:CATEGORYElementFlux ! category - C and nutrient flux
relationship: context ECOSIMCONCEPT:Solute ! Solute
relationship: has_unit ECOSIM:mold-2h-1 ! mol d-2 h-1
relationship: measured_in ECOSIMCONCEPT:Band ! Band
relationship: measurement_of ECOSIMCONCEPT:NH4 ! Ammonium

[Term]
id: ECOSIM:TRN4S
name: total solute NH4 transformation non-band
def: "Total solute NH4 transformation non-band refers to the total amount of transformation of ammonium (NH4) solute in a non-banded or uniform manner across a particular environment or medium. This typically includes processes like nitrification, volatilization, immobilization, mineralization, uptake by crops, and leaching. These processes are driven by multiple factors including temperature, soil moisture, and the presence of microorganisms." []
is_a: ECOSIM:CATEGORYElementFlux ! category - C and nutrient flux
relationship: context ECOSIMCONCEPT:Solute ! Solute
relationship: has_unit ECOSIM:mold-2h-1 ! mol d-2 h-1
relationship: measurement_of ECOSIMCONCEPT:NH4 ! Ammonium

[Term]
id: ECOSIM:TRNO2
name: total solute NO2 transformation non-band
is_a: ECOSIMCONCEPT:UnclassifiedVariable ! unclassified variable
relationship: has_unit ECOSIM:mold-2h-1 ! mol d-2 h-1

[Term]
id: ECOSIM:TRNO3
name: total solute NO3 transformation non-band
def: "Total solute NO3 transformation non-band refers to the total transformation of nitrate (NO3) solutes in a soil environment outside a specified band or area. This process often involves the conversion of NO3 into different forms, influenced by microorganisms in the soil. Such transformations are pivotal for nutrient cycling and availability in ecosystems." []
is_a: ECOSIM:CATEGORYElementFlux ! category - C and nutrient flux
relationship: context ECOSIMCONCEPT:Solute ! Solute
relationship: has_unit ECOSIM:mold-2h-1 ! mol d-2 h-1
relationship: measurement_of ECOSIMCONCEPT:NO3 ! Nitrate

[Term]
id: ECOSIM:TRNOB
name: total solute NO3 transformation band
def: "Total solute NO3 transformation band refers to the total amount of nitrate (NO3) solute that is transformed or altered in a specific band or section of land or soil. This transformation can occur due to various biotic and abiotic processes, including microbial activity, chemical reactions, and environmental factors. Measuring the total solute NO3 transformation band can provide insights into the nitrogen cycling in an ecosystem, which is crucial for understanding soil fertility and crop productivity." []
is_a: ECOSIM:CATEGORYElementFlux ! category - C and nutrient flux
relationship: context ECOSIMCONCEPT:Band ! Band
relationship: has_unit ECOSIM:mold-2h-1 ! mol d-2 h-1

[Term]
id: ECOSIM:TRXAL
name: total adsorbed Al transformation
def: "Total adsorbed Al transformation refers to the process of transforming aluminum in the soil by adsorption. This is a key process in the soil and plays a critical role in soil structure stabilization, nutrient cation supply, and buffering soil solution pH." []
is_a: ECOSIM:CATEGORYElementFlux ! category - C and nutrient flux
relationship: has_unit ECOSIM:mold-2h-1 ! mol d-2 h-1
relationship: measured_in ECOSIMCONCEPT:Soil ! Soil
relationship: measurement_of ECOSIMCONCEPT:Aluminum ! Aluminum

[Term]
id: ECOSIM:TRXAL2
name: total adsorbed AlOH2 transformation
def: "Total adsorbed AlOH2 transformation refers to the total change in the quantity of adsorbed AlOH2 (Aluminum Hydroxide) in a certain period of time. This transformation can occur as a result of various biogeochemical processes such as adsorption, desorption, chemical reactions, and biological activity. The transformation rate of adsorbed AlOH2 is an important parameter in environmental and earth system modeling as it influences water quality, soil fertility, and nutrient availability." []
is_a: ECOSIM:CATEGORYElementFlux ! category - C and nutrient flux
is_a: ECOSIM:CATEGORYNTransformation ! category - N transformation
relationship: has_unit ECOSIM:mold-2h-1 ! mol d-2 h-1

[Term]
id: ECOSIM:TRXCA
name: total adsorbed Ca transformation
def: "Total adsorbed Ca transformation refers to the total change or conversion of calcium (Ca) ions that are adsorbed or attached to the surface of a material, such as soil particles. This process plays a crucial role in the nutrient cycle in soils, influencing nutrient availability to plants and soil pH balance." []
is_a: ECOSIM:CATEGORYElementFlux ! category - C and nutrient flux
relationship: has_unit ECOSIM:mold-2h-1 ! mol d-2 h-1

[Term]
id: ECOSIM:TRXHC
name: total adsorbed COOH transformation
def: "Total adsorbed COOH transformation refers to the total change or conversion of adsorbed carboxyl groups (COOH) in a system. These groups often attach to surfaces and contribute to important processes in various environmental systems, including soil chemistry, water treatment, and atmospheric chemistry." []
is_a: ECOSIM:CATEGORYElementFlux ! category - C and nutrient flux
relationship: has_unit ECOSIM:mold-2h-1 ! mol d-2 h-1

[Term]
id: ECOSIM:TRXHY
name: total adsorbed H transformation
def: "Total adsorbed H transformation refers to the total amount of hydrogen (H) that undergoes transformation while being adsorbed on the surface of a material. In environmental science, this process plays a crucial role in various processes such as nutrient adsorption, contaminant removal, and catalyst activity." []
is_a: ECOSIM:CATEGORYElementFlux ! category - C and nutrient flux
relationship: has_unit ECOSIM:mold-2h-1 ! mol d-2 h-1
relationship: measurement_of ECOSIMCONCEPT:Hydrogen ! Hydrogen

[Term]
id: ECOSIM:TRXKA
name: total adsorbed K transformation
def: "Total adsorbed K transformation refers to the total change in the amount of potassium (K) that is adsorbed onto the surfaces of solid particles, such as soil or sediments, over a certain period of time. This is an important aspect of nutrient cycling in terrestrial and aquatic environments." []
is_a: ECOSIM:CATEGORYElementFlux ! category - C and nutrient flux
relationship: has_unit ECOSIM:mold-2h-1 ! mol d-2 h-1

[Term]
id: ECOSIM:TRXMG
name: total adsorbed Mg transformation
def: "Total adsorbed Mg transformation refers to the total amount of magnesium that is adsorbed by the soil and is subsequently transformed, usually by microorganisms. It is an important parameter in soil chemistry and nutrient cycling as it could affect the availability of Magnesium, a key nutrient, for plant uptake." []
is_a: ECOSIM:CATEGORYElementFlux ! category - C and nutrient flux
relationship: has_unit ECOSIM:mold-2h-1 ! mol d-2 h-1
relationship: measured_in ECOSIMCONCEPT:Soil ! Soil
relationship: measurement_of ECOSIMCONCEPT:Magnesium ! Magnesium

[Term]
id: ECOSIM:TRXNA
name: total adsorbed Na transformation
def: "Total adsorbed Na transformation refers to the total transformation or changes in the adsorbed Sodium (Na) in the soil. Adsorbed sodium refers to Sodium ions that are attached to the surfaces of soil particles. This parameter is significant for understanding the sodium cycling and its availability in the soils." []
is_a: ECOSIM:CATEGORYElementFlux ! category - C and nutrient flux
is_a: ECOSIM:CATEGORYSoilBiogeochemistry ! category - Soil Biogeochemistry
relationship: has_unit ECOSIM:mold-2h-1 ! mol d-2 h-1
relationship: measured_in ECOSIMCONCEPT:Soil ! Soil
relationship: measurement_of ECOSIMCONCEPT:Sodium ! Sodium

[Term]
id: ECOSIM:TRootGasLoss_disturb
name: total root gas content
def: "The parameter 'total root gas content' refers to the amount of gas stored in the root system of a plant. It represents the total volume of gases, such as oxygen and carbon dioxide, that are present in the root zone. This parameter can be influenced by disturbances, such as deforestation or land use change, which can lead to changes in the root system and subsequently impact the amount of gas stored in the roots." []
is_a: ECOSIMCONCEPT:UnclassifiedVariable ! unclassified variable
relationship: has_unit ECOSIM:gd-2 ! g d-2

[Term]
id: ECOSIM:TSH
name: ecosystem sensible heat flux
is_a: ECOSIMCONCEPT:UnclassifiedVariable ! unclassified variable
relationship: has_unit ECOSIM:MJd-2h-1 ! MJ d-2 h-1

[Term]
id: ECOSIM:TSHC
name: total sensible heat flux x boundary layer resistance
is_a: ECOSIMCONCEPT:UnclassifiedVariable ! unclassified variable
relationship: has_unit ECOSIM:MJm-1 ! MJ m-1

[Term]
id: ECOSIM:TSHX
name: total sensible heat flux x boundary layer resistance
is_a: ECOSIMCONCEPT:UnclassifiedVariable ! unclassified variable
relationship: has_unit ECOSIM:MJm-1 ! MJ m-1

[Term]
id: ECOSIM:TUPCHS
name: total root-soil CH4 flux
is_a: ECOSIMCONCEPT:UnclassifiedVariable ! unclassified variable
relationship: has_unit ECOSIM:gd-2h-1 ! g d-2 h-1

[Term]
id: ECOSIM:TUPH2B
name: total root-soil PO4 flux band
is_a: ECOSIMCONCEPT:UnclassifiedVariable ! unclassified variable
relationship: has_unit ECOSIM:gd-2h-1 ! g d-2 h-1

[Term]
id: ECOSIM:TUPH2P
name: total root-soil PO4 flux non-band
is_a: ECOSIMCONCEPT:UnclassifiedVariable ! unclassified variable
relationship: has_unit ECOSIM:gd-2h-1 ! g d-2 h-1

[Term]
id: ECOSIM:TUPHGS
name: total root-soil H2 flux
is_a: ECOSIMCONCEPT:UnclassifiedVariable ! unclassified variable
relationship: has_unit ECOSIM:gd-2h-1 ! g d-2 h-1

[Term]
id: ECOSIM:TUPN2S
name: total root-soil N2O flux
is_a: ECOSIMCONCEPT:UnclassifiedVariable ! unclassified variable
relationship: has_unit ECOSIM:gd-2h-1 ! g d-2 h-1

[Term]
id: ECOSIM:TUPN3B
name: total root-soil NH3 flux band
is_a: ECOSIMCONCEPT:UnclassifiedVariable ! unclassified variable
relationship: has_unit ECOSIM:gd-2h-1 ! g d-2 h-1

[Term]
id: ECOSIM:TUPN3S
name: total root-soil NH3 flux non-band
is_a: ECOSIMCONCEPT:UnclassifiedVariable ! unclassified variable
relationship: has_unit ECOSIM:gd-2h-1 ! g d-2 h-1

[Term]
id: ECOSIM:TUPNF
name: total root N2 fixation
is_a: ECOSIMCONCEPT:UnclassifiedVariable ! unclassified variable
relationship: has_unit ECOSIM:gd-2h-1 ! g d-2 h-1

[Term]
id: ECOSIM:TUPNH4
name: total root-soil NH4 flux non-band
is_a: ECOSIMCONCEPT:UnclassifiedVariable ! unclassified variable
relationship: has_unit ECOSIM:gd-2h-1 ! g d-2 h-1

[Term]
id: ECOSIM:TUPNHB
name: total root-soil NH4 flux band
is_a: ECOSIMCONCEPT:UnclassifiedVariable ! unclassified variable
relationship: has_unit ECOSIM:gd-2h-1 ! g d-2 h-1

[Term]
id: ECOSIM:TUPNO3
name: total root-soil NO3 flux non-band
is_a: ECOSIMCONCEPT:UnclassifiedVariable ! unclassified variable
relationship: has_unit ECOSIM:gd-2h-1 ! g d-2 h-1

[Term]
id: ECOSIM:TUPNOB
name: total root-soil NO3 flux band
is_a: ECOSIMCONCEPT:UnclassifiedVariable ! unclassified variable
relationship: has_unit ECOSIM:gd-2h-1 ! g d-2 h-1

[Term]
id: ECOSIM:TUPOXP
name: total root internal O2 flux
is_a: ECOSIMCONCEPT:UnclassifiedVariable ! unclassified variable
relationship: has_unit ECOSIM:gd-2h-1 ! g d-2 h-1

[Term]
id: ECOSIM:TUPOXS
name: total root-soil O2 flux
is_a: ECOSIMCONCEPT:UnclassifiedVariable ! unclassified variable
relationship: has_unit ECOSIM:gd-2h-1 ! g d-2 h-1

[Term]
id: ECOSIM:TWIND
name: total daily wind travel
def: "Total daily wind travel is the total distance covered by the wind in a single day. This measure can be important in various studies, such as those related to weather patterns, climate modelling, and even the spread of airborne particles or pollutants." []
is_a: ECOSIM:CATEGORYAtmosphericConditions ! category - Atmospheric Conditions
relationship: attribute ECOSIMCONCEPT:Wind ! Wind
relationship: has_unit ECOSIM:md-1 ! m d-1

[Term]
id: ECOSIM:TZUPFX
name: total plant N2 fixation
is_a: ECOSIMCONCEPT:UnclassifiedVariable ! unclassified variable
relationship: has_unit ECOSIM:gd-2 ! g d-2

[Term]
id: ECOSIM:TairK
name: air temperature
is_a: ECOSIM:CATEGORYAtmosphericConditions ! category - Atmospheric Conditions
relationship: has_unit ECOSIM:K ! K

[Term]
id: ECOSIM:TairKClimMean
name: mean annual air temperature
is_a: ECOSIM:CATEGORYAtmosphericConditions ! category - Atmospheric Conditions
relationship: has_unit ECOSIM:K ! K

[Term]
id: ECOSIM:TortMacPM
name: macropore tortuosity
is_a: ECOSIMCONCEPT:UnclassifiedVariable ! unclassified variable

[Term]
id: ECOSIM:TortMicPM
name: soil tortuosity
is_a: ECOSIMCONCEPT:UnclassifiedVariable ! unclassified variable

[Term]
id: ECOSIM:UCH4F
name: total CH4 flux from fire
is_a: ECOSIMCONCEPT:UnclassifiedVariable ! unclassified variable
relationship: has_unit ECOSIM:gd-2 ! g d-2

[Term]
id: ECOSIM:UCH4G
name: total soil CH4 flux
def: "Total soil CH4 flux refers to the total amount of methane (CH4) gas that is released or absorbed by the soil over a specified time period. Methane is a potent greenhouse gas, and understanding its flux in and out of the soil can provide important insights into the carbon cycle and the overall health of an ecosystem." []
is_a: ECOSIM:CATEGORYBiogeochemistry ! category - Biogeochemistry
is_a: ECOSIM:CATEGORYTraceGasFlux ! category - trace gas flux
is_a: ECOSIMCONCEPT:Flux ! Flux
relationship: has_unit ECOSIM:gd-2 ! g d-2
relationship: measured_in ECOSIMCONCEPT:Soil ! Soil
relationship: measurement_of ECOSIMCONCEPT:CH4 ! Methane

[Term]
id: ECOSIM:UCO2F
name: total CO2 flux from fire
is_a: ECOSIMCONCEPT:UnclassifiedVariable ! unclassified variable
relationship: has_unit ECOSIM:gd-2 ! g d-2

[Term]
id: ECOSIM:UCO2G
name: total soil CO2 flux
is_a: ECOSIM:CATEGORYBiogeochemistry ! category - Biogeochemistry
is_a: ECOSIM:CATEGORYTraceGasFlux ! category - trace gas flux
relationship: attribute ECOSIMCONCEPT:Flux ! Flux
relationship: has_unit ECOSIM:gd-2 ! g d-2
relationship: measured_in ECOSIMCONCEPT:Soil ! Soil
relationship: measurement_of ECOSIMCONCEPT:CO2 ! Carbon dioxide

[Term]
id: ECOSIM:UCO2S
name: total soil DIC
def: "Total soil DIC refers to the total amount of Dissolved Inorganic Carbon in the soil. DIC in soil can originate from various sources such as decay of organic material, root respiration, carbonate dissolution, or atmospheric CO2 dissolution in water. It plays a crucial role in the carbon cycle of ecosystems, contributing to both carbon sequestration and greenhouse gas emissions." []
is_a: ECOSIM:CATEGORYMicrobialActivity ! category - microbial activity
is_a: ECOSIM:CATEGORYSoilBiogeochemistry ! category - Soil Biogeochemistry
relationship: has_unit ECOSIM:gd-2 ! g d-2
relationship: measured_in ECOSIMCONCEPT:Soil ! Soil

[Term]
id: ECOSIM:UCOP
name: total soil autotrophic respiration
def: "Total soil autotrophic respiration refers to the total amount of carbon dioxide (CO2) released by the metabolic activity of autotrophic organisms in the soil. Autotrophic organisms, which include plants and some types of microorganisms, produce energy through photosynthesis and release CO2 as a byproduct. Autotrophic respiration contributes significantly to the overall soil respiration and is a key component of the carbon cycle. It is influenced by various factors such as temperature, moisture, and nutrient availability." []
is_a: ECOSIM:CATEGORYSoilBiogeochemistry ! category - Soil Biogeochemistry
is_a: ECOSIM:CATEGORYTraceGasFlux ! category - trace gas flux
relationship: has_unit ECOSIM:gd-2 ! g d-2
relationship: measured_in ECOSIMCONCEPT:Soil ! Soil
relationship: measurement_of ECOSIMCONCEPT:CO2 ! Carbon dioxide

[Term]
id: ECOSIM:UDICD
name: total subsurface DIC flux
def: "Total subsurface DIC flux refers to the total amount of Dissolved Inorganic Carbon (DIC) that moves within the subsurface layers of an ecosystem. This includes movements through soil water, groundwater, and other subsurface flows. DIC in aquatic ecosystems includes gases, such as CO2 and CH4, and bicarbonates and carbonates. The measurement of this flux is important for understanding the carbon cycle within an ecosystem, particularly in the context of climate change and ocean acidification." []
is_a: ECOSIM:CATEGORYTraceGasFlux ! category - trace gas flux
relationship: attribute ECOSIMCONCEPT:Flux ! Flux
relationship: has_unit ECOSIM:gd-2 ! g d-2
relationship: measured_in ECOSIMCONCEPT:Subsurface ! Subsurface

[Term]
id: ECOSIM:UDICQ
name: total surface DIC flux
def: "Total surface DIC flux refers to the total amount of dissolved inorganic carbon (DIC) that moves across the Earth's surface over a specified period of time. In the context of Earth system modeling, this is an important parameter that helps to understand and quantify the biogeochemical cycling of carbon at the global scale. It includes the natural fluxes of DIC to and from oceans, rivers, lakes, and other surface bodies of water, as well as anthropogenic (human-caused) DIC fluxes, such as those resulting from fossil fuel combustion and land use change." []
is_a: ECOSIM:CATEGORYTraceGasFlux ! category - trace gas flux
relationship: has_unit ECOSIM:gd-2 ! g d-2
relationship: measured_in ECOSIMCONCEPT:Surface ! Surface
relationship: measurement_of ECOSIMCONCEPT:DIC ! Dissolved inorganic carbon

[Term]
id: ECOSIM:UDIND
name: total subsurface DIN flux
def: "The term 'total subsurface DIN flux' refers to the total amount of dissolved inorganic nitrogen (DIN) that moves through the subsurface layer of an ecosystem over a particular period of time. This flux describes the rate of DIN transfer from one location to another, typically due to the process of leaching. DIN flux is an important component of the nitrogen cycle in an ecosystem, influencing soil fertility, plant growth, and water quality." []
is_a: ECOSIM:CATEGORYTraceGasFlux ! category - trace gas flux
relationship: attribute ECOSIMCONCEPT:Flux ! Flux
relationship: has_unit ECOSIM:gd-2 ! g d-2
relationship: measured_in ECOSIMCONCEPT:Subsurface ! Subsurface
relationship: measurement_of ECOSIMCONCEPT:DissolvedInorganicNitrogen ! Dissolved inorganic nitrogen

[Term]
id: ECOSIM:UDINQ
name: total surface DIN flux
def: "The total surface dissolved inorganic nitrogen (DIN) flux refers to the total amount of DIN (comprising nitrate, nitrite, and ammonium) that moves across the surface of a given area over a certain period of time. This can include fluxes from atmospheric deposition, biological activity, and hydrological processes. Measuring the total surface DIN flux is important for understanding nitrogen cycling and nutrient availability in ecosystems." []
is_a: ECOSIM:CATEGORYTraceGasFlux ! category - trace gas flux
relationship: has_unit ECOSIM:gd-2 ! g d-2
relationship: measurement_of ECOSIMCONCEPT:DissolvedInorganicNitrogen ! Dissolved inorganic nitrogen

[Term]
id: ECOSIM:UDIPD
name: total subsurface DIP flux
is_a: ECOSIM:CATEGORYTraceGasFlux ! category - trace gas flux
relationship: has_unit ECOSIM:gd-2 ! g d-2
relationship: measured_in ECOSIMCONCEPT:Subsurface ! Subsurface
relationship: measurement_of ECOSIMCONCEPT:DIP ! Dissolved inorganic phosphorus

[Term]
id: ECOSIM:UDIPQ
name: total surface DIP flux
def: "Total surface DIP (Dissolvable Inorganic Phosphorus) flux refers to the total amount of DIP that is transferred from the surface of the Earth (land and water bodies) to the atmosphere. The DIP flux is an important part of the phosphorus cycle and plays a crucial role in marine and terrestrial ecosystems. It influences productivity, food web dynamics, and the concentrations of greenhouse gases." []
is_a: ECOSIM:CATEGORYTraceGasFlux ! category - trace gas flux
relationship: attribute ECOSIMCONCEPT:Flux ! Flux
relationship: has_unit ECOSIM:gd-2 ! g d-2
relationship: measured_in ECOSIMCONCEPT:Surface ! Surface
relationship: measurement_of ECOSIMCONCEPT:DIP ! Dissolved inorganic phosphorus

[Term]
id: ECOSIM:UDOCD
name: total subsurface DOC flux
def: "Total subsurface DOC flux refers to the total amount of dissolved organic carbon (DOC) that moves or flows below the surface of the earth. DOC is a key component of the global carbon cycle and is involved in numerous biogeochemical processes, including the nutrition and metabolism of soil microbiota and the transport of pollutants, such as heavy metals. Monitoring and quantifying the flux of DOC in subsurface environments is crucial for understanding carbon dynamics and the transfer of carbon between the soil, groundwater, and atmosphere." []
is_a: ECOSIM:CATEGORYBiogeochemistry ! category - Biogeochemistry
is_a: ECOSIM:CATEGORYSoilBiogeochemistry ! category - Soil Biogeochemistry
is_a: ECOSIM:CATEGORYTraceGasFlux ! category - trace gas flux
relationship: context ECOSIMCONCEPT:Flux ! Flux
relationship: has_unit ECOSIM:gd-2 ! g d-2
relationship: measured_in ECOSIMCONCEPT:Subsurface ! Subsurface
relationship: measurement_of ECOSIMCONCEPT:DissolvedOrganicCarbon ! Dissolved organic carbon

[Term]
id: ECOSIM:UDOCQ
name: total surface DOC flux
def: "Total Surface Dissolved Organic Carbon (DOC) flux refers to the total amount or concentration of Dissolved Organic Carbon transported on the surface of a particular ecosystem, such as a lake, river or ocean, over a certain period. It is a comprehensive measure that encompasses all horizontal and vertical DOC fluxes occurring at the air-water interface." []
is_a: ECOSIM:CATEGORYBiogeochemistry ! category - Biogeochemistry
is_a: ECOSIM:CATEGORYTraceGasFlux ! category - trace gas flux
relationship: attribute ECOSIMCONCEPT:Flux ! Flux
relationship: has_unit ECOSIM:gd-2 ! g d-2
relationship: measured_in ECOSIMCONCEPT:Surface ! Surface
relationship: measurement_of ECOSIMCONCEPT:DissolvedOrganicCarbon ! Dissolved organic carbon

[Term]
id: ECOSIM:UDOND
name: total subsurface DON flux
def: "Total Subsurface DON Flux refers to the total flow or movement of Dissolved Organic Nitrogen (DON) below the Earth's surface. It is a part of the nitrogen cycle that involves the breakdown and distribution of nitrogenous compounds in the soil, which can affect the health of ecosystems and the quality of groundwater." []
is_a: ECOSIM:CATEGORYBiogeochemistry ! category - Biogeochemistry
is_a: ECOSIM:CATEGORYHydrology ! category - Hydrology
is_a: ECOSIM:CATEGORYTraceGasFlux ! category - trace gas flux
relationship: attribute ECOSIMCONCEPT:Flux ! Flux
relationship: has_unit ECOSIM:gd-2 ! g d-2
relationship: measured_in ECOSIMCONCEPT:Subsurface ! Subsurface
relationship: measurement_of ECOSIMCONCEPT:DissolvedOrganicNitrogen ! Dissolved organic nitrogen

[Term]
id: ECOSIM:UDONQ
name: total surface DON flux
def: "Total surface DON flux refers to the total amount of dissolved organic nitrogen (DON) that is transported across the surface through various processes, such as runoff, leaching, and atmospheric deposition. It is a key parameter in studying and modeling the global nitrogen cycle. High levels of DON flux can contribute to nutrient pollution and influence the health of aquatic and terrestrial ecosystems." []
is_a: ECOSIM:CATEGORYBiogeochemistry ! category - Biogeochemistry
is_a: ECOSIM:CATEGORYTraceGasFlux ! category - trace gas flux
relationship: attribute ECOSIMCONCEPT:Flux ! Flux
relationship: has_unit ECOSIM:gd-2 ! g d-2
relationship: measured_in ECOSIMCONCEPT:Surface ! Surface
relationship: measurement_of ECOSIMCONCEPT:DissolvedOrganicNitrogen ! Dissolved organic nitrogen

[Term]
id: ECOSIM:UDOPD
name: total subsurface DOP flux
def: "Total subsurface DOP flux refers to the total flow of dissolved organic phosphorus (DOP) from higher to lower concentrations in a specified subsurface area, usually measured in units of mass per time per area. DOP is a subset of total phosphorus that includes any organic compounds containing phosphorus, such as phospholipids and nucleic acids. Being able to quantify DOP fluxes is key to understanding nutrient cycling in ecosystems and crucial for constructing ecosystem and land surface models." []
is_a: ECOSIM:CATEGORYBiogeochemistry ! category - Biogeochemistry
is_a: ECOSIM:CATEGORYTraceGasFlux ! category - trace gas flux
relationship: has_unit ECOSIM:gd-2 ! g d-2
relationship: measured_in ECOSIMCONCEPT:Subsurface ! Subsurface
relationship: measurement_of ECOSIMCONCEPT:DOP ! Dissolved organic phosphorus

[Term]
id: ECOSIM:UDOPQ
name: total surface DOP flux
def: "Total surface DOP Flux refers to the total quantity of Dissolved Organic Phosphorus (DOP) that is transferred from one place to another on the earth's surface over a specific time period. It is a critical component of the phosphate cycle and is primarily produced through the breakdown of organic compound. This measure plays a critical role in the uptake of phosphorus and its availability in the environment." []
is_a: ECOSIM:CATEGORYBiogeochemistry ! category - Biogeochemistry
is_a: ECOSIM:CATEGORYTraceGasFlux ! category - trace gas flux
relationship: attribute ECOSIMCONCEPT:Flux ! Flux
relationship: has_unit ECOSIM:gd-2 ! g d-2
relationship: measured_in ECOSIMCONCEPT:Surface ! Surface
relationship: measurement_of ECOSIMCONCEPT:DOP ! Dissolved organic phosphorus

[Term]
id: ECOSIM:UDRAIN
name: total water drainage below root zone
def: "Total water drainage below root zone, also known as deep percolation, is the process by which water moves down through the soil profile, below the root zone, and eventually reaches the groundwater system. This parameter is important in assessing water loss from the soil and its availability for plant use, as well as for estimating groundwater recharge and understanding nutrient leaching." []
is_a: ECOSIM:CATEGORYHydrology ! category - Hydrology
relationship: attribute ECOSIMCONCEPT:Drainage ! Drainage
relationship: has_unit ECOSIM:m3d-2 ! m3 d-2
relationship: measured_in ECOSIMCONCEPT:RootZone ! Root zone
relationship: measurement_of ECOSIMCONCEPT:Water ! Water

[Term]
id: ECOSIM:UEVAP
name: total evaporation
def: "Total evaporation, or evapotranspiration, is the sum of evaporation and plant transpiration from the Earth's land and ocean surface to the atmosphere. It is an important part of the water cycle, and affects micro and macro climate." []
is_a: ECOSIM:CATEGORYHydrology ! category - Hydrology
relationship: attribute ECOSIMCONCEPT:Evaporation ! Evaporation
relationship: has_unit ECOSIM:m3d-2 ! m3 d-2
relationship: measurement_of ECOSIMCONCEPT:Water ! Water

[Term]
id: ECOSIM:UFERTN
name: total fertilizer N amendment
def: "Total fertilizer nitrogen (N) amendment refers to the total amount of nitrogen added to a soil or system through the application of fertilizers. It represents an input of nitrogen into the system. This is an important parameter in agricultural and earth system modeling, affecting nutrient cycling, plant growth, and greenhouse gas emissions." []
is_a: ECOSIM:CATEGORYBiogeochemistry ! category - Biogeochemistry
is_a: ECOSIM:CATEGORYTraceGasFlux ! category - trace gas flux
relationship: has_unit ECOSIM:gd-2 ! g d-2
relationship: measurement_of ECOSIMCONCEPT:Nitrogen ! Nitrogen

[Term]
id: ECOSIM:UFERTP
name: total fertilizer P amendment
def: "Total fertilizer P amendment refers to the total amount of phosphorus (P) introduced into soil or a particular ecosystem through the application of fertilizers. It is a key parameter in agronomic and environmental research, as it has significant implications for crop productivity and soil fertility, as well as environmental impacts such as water quality and eutrophication. The amount, timing, and method of P fertilization can significantly affect P availability to crops, P losses to the environment, and overall ecosystem dynamics." []
is_a: ECOSIM:CATEGORYBiogeochemistry ! category - Biogeochemistry
is_a: ECOSIM:CATEGORYSoilBiogeochemistry ! category - Soil Biogeochemistry
is_a: ECOSIM:CATEGORYTraceGasFlux ! category - trace gas flux
relationship: context ECOSIMCONCEPT:Fertilizer ! Fertilizer
relationship: has_unit ECOSIM:gd-2 ! g d-2
relationship: measurement_of ECOSIMCONCEPT:Phosphorus ! Phosphorus

[Term]
id: ECOSIM:UH2GG
name: total H2 flux
def: "Refers to the total amount of hydrogen gas (H2) that is released or absorbed in an environment or ecosystem over a specific period of time. This flux can occur through various processes such as fermentation, respiration, and photosynthesis and can have significant impacts on atmospheric chemistry and climate regulation." []
is_a: ECOSIM:CATEGORYBiogeochemistry ! category - Biogeochemistry
is_a: ECOSIM:CATEGORYGasFlux ! category - Gas Flux
is_a: ECOSIM:CATEGORYTraceGasFlux ! category - trace gas flux
relationship: measurement_of ECOSIMCONCEPT:H2 ! Dihydrogen

[Term]
id: ECOSIM:UION
name: total soil ion content
def: "Total soil ion content refers to the sum of all the ion concentrations in a soil sample. It is an aggregate measure of the total quantity of ions present, which could include essential plant nutrients like nitrogen (N), phosphorous (P), and potassium (K), as well as other elements. This measurement is useful in determining soil fertility and nutrient availability for plant growth." []
is_a: ECOSIM:CATEGORYSoilBiogeochemistry ! category - Soil Biogeochemistry
is_a: ECOSIM:CATEGORYTraceGasFlux ! category - trace gas flux
relationship: attribute ECOSIMCONCEPT:Content ! Content
relationship: has_unit ECOSIM:mold-2 ! mol d-2
relationship: measured_in ECOSIMCONCEPT:Soil ! Soil
relationship: measurement_of ECOSIMCONCEPT:Ions ! Ions

[Term]
id: ECOSIM:UIONOU
name: total subsurface ion flux
def: "Total subsurface ion flux refers to the total movement of ions, or charged particles, within the subsurface or subsurface waters. This includes both the downward movement of ions through the soil profile (leaching) and the upward movement of ions from the subsurface to the surface (capillary rise or upward diffusion). It is a crucial factor in nutrient cycling, soil chemistry, and water quality." []
is_a: ECOSIM:CATEGORYHydrology ! category - Hydrology
is_a: ECOSIM:CATEGORYTraceGasFlux ! category - trace gas flux
relationship: has_unit ECOSIM:mold-2 ! mol d-2
relationship: measured_in ECOSIMCONCEPT:Subsurface ! Subsurface
relationship: measurement_of ECOSIMCONCEPT:Ion ! Ion

[Term]
id: ECOSIM:UN2GG
name: total soil N2 flux
def: "Total soil N2 flux refers to the overall movement of nitrogen in the form of N2 from the soil to the atmosphere. This encompasses all processes that result in the release of N2 from the soil surface, including microbial (denitrification) and non-microbial (volatilization) processes. This parameter is essential in understanding the nitrogen cycle and its interaction with other biogeochemical cycles. It also aids in modeling and simulation of soil dynamics and nutrient balance in ecosystems." []
is_a: ECOSIM:CATEGORYBiogeochemistry ! category - Biogeochemistry
is_a: ECOSIM:CATEGORYTraceGasFlux ! category - trace gas flux
relationship: attribute ECOSIMCONCEPT:Flux ! Flux
relationship: has_unit ECOSIM:gd-2 ! g d-2
relationship: measured_in ECOSIMCONCEPT:Soil ! Soil
relationship: measurement_of ECOSIMCONCEPT:N2 ! Dinitrogen

[Term]
id: ECOSIM:UN2GS
name: total N2 fixation
def: "Total N2 fixation refers to the total amount of nitrogen (N2) in the atmosphere that is converted into a form that plants and other organisms can use for growth. This is primarily done by certain bacteria in a process called nitrogen fixation. This parameter is important in the Earth system modeling as it plays a crucial role in the global nitrogen cycle and directly influences primary productivity." []
is_a: ECOSIM:CATEGORYBiogeochemistry ! category - Biogeochemistry
is_a: ECOSIM:CATEGORYTraceGasFlux ! category - trace gas flux
relationship: has_unit ECOSIM:gd-2 ! g d-2
relationship: measured_in ECOSIMCONCEPT:Atmosphere ! Atmosphere
relationship: measurement_of ECOSIMCONCEPT:NitrogenFixation ! Nitrogen fixation

[Term]
id: ECOSIM:UN2OF
name: total N2O flux from fire
def: "Total N2O flux from fire refers to the total amount of nitrous oxide (N2O) that is released into the atmosphere as a result of burning processes. Fires, including forest and grassland fires, can produce N2O as a byproduct of combustion. This parameter is significant in Earth system modeling as N2O is a potent greenhouse gas that can contribute to global warming and climate change." []
is_a: ECOSIM:CATEGORYGasFlux ! category - Gas Flux
is_a: ECOSIMCONCEPT:UnclassifiedVariable ! unclassified variable
relationship: context ECOSIMCONCEPT:Fire ! Fire
relationship: has_unit ECOSIM:gd-2 ! g d-2
relationship: measurement_of ECOSIMCONCEPT:N2O ! Nitrous oxide

[Term]
id: ECOSIM:UN2OG
name: total soil N2O flux
def: "Total soil N2O flux refers to the total amount of nitrous oxide (N2O) gas that is emitted from the soil into the atmosphere. N2O is a potent greenhouse gas and its emissions are primarily due to microbial processes in the soil, including nitrification and denitrification. The total soil N2O flux is an important parameter in earth systems modeling as it contributes to global warming and climate change." []
is_a: ECOSIM:CATEGORYBiogeochemistry ! category - Biogeochemistry
is_a: ECOSIM:CATEGORYGasFlux ! category - Gas Flux
is_a: ECOSIM:CATEGORYTraceGasFlux ! category - trace gas flux
relationship: attribute ECOSIMCONCEPT:Flux ! Flux
relationship: has_unit ECOSIM:gd-2 ! g d-2
relationship: measured_in ECOSIMCONCEPT:Soil ! Soil
relationship: measurement_of ECOSIMCONCEPT:N2O ! Nitrous oxide

[Term]
id: ECOSIM:UNH3F
name: total NH3 flux from fire
is_a: ECOSIMCONCEPT:UnclassifiedVariable ! unclassified variable
relationship: attribute ECOSIMCONCEPT:Flux ! Flux
relationship: has_unit ECOSIM:gd-2 ! g d-2
relationship: measurement_of ECOSIMCONCEPT:NH3 ! Ammonia

[Term]
id: ECOSIM:UNH3G
name: total soil NH3 flux
def: "Total soil NH3 flux refers to the total amount of ammonia (NH3) that is released from or absorbed by the soil. This can happen through processes such as nitrification and denitrification, which are carried out by microorganisms in the soil. The rate of NH3 flux depends on several environmental factors including soil type, temperature, pH, and moisture levels." []
is_a: ECOSIM:CATEGORYBiogeochemistry ! category - Biogeochemistry
is_a: ECOSIM:CATEGORYGasFlux ! category - Gas Flux
is_a: ECOSIM:CATEGORYTraceGasFlux ! category - trace gas flux
relationship: attribute ECOSIMCONCEPT:Flux ! Flux
relationship: has_unit ECOSIM:gd-2 ! g d-2
relationship: measured_in ECOSIMCONCEPT:Soil ! Soil
relationship: measurement_of ECOSIMCONCEPT:NH3 ! Ammonia

[Term]
id: ECOSIM:UNH4
name: total soil NH4 + NH3 content
def: "Total soil NH4 + NH3 content refers to the total amount of ammonium ions (NH4+) and ammonia (NH3) present in the soil. This is a significant measure in studies related to soil fertility, biogeochemical cycling of nitrogen, and environmental pollution." []
is_a: ECOSIM:CATEGORYMicrobialActivity ! category - microbial activity
relationship: attribute ECOSIMCONCEPT:Content ! Content
relationship: has_unit ECOSIM:gd-2 ! g d-2
relationship: measured_in ECOSIMCONCEPT:Soil ! Soil
relationship: measurement_of ECOSIMCONCEPT:NH4NH3 ! Ammonium/Ammonia

[Term]
id: ECOSIM:UNO3
name: total soil NO3 + NO2 content
def: "Total soil NO3 + NO2 content refers to the sum of the amounts of nitrate (NO3) and nitrite (NO2), which are forms of inorganic nitrogen, in the soil. This measurement is vital for understanding the nitrogen cycle and assessing soil fertility as both NO3 and NO2 are key nutrients for plant growth. Moreover, high levels of these compounds can indicate soil acidification and potential contaminants in groundwater." []
is_a: ECOSIM:CATEGORYMicrobialActivity ! category - microbial activity
is_a: ECOSIM:CATEGORYSoilBiogeochemistry ! category - Soil Biogeochemistry
relationship: has_unit ECOSIM:gd-2 ! g d-2
relationship: measured_in ECOSIMCONCEPT:Soil ! Soil
relationship: measurement_of ECOSIMCONCEPT:NO2 ! Nitrogen dioxide
relationship: measurement_of ECOSIMCONCEPT:NO3 ! Nitrate

[Term]
id: ECOSIM:UORGC
name: total humus C
def: "Total humus C refers to the total amount of carbon contained in the humus in the soil. Humus, the organic component of soil, is formed by the decomposition of leaves and other plant material by soil microorganisms. It is an essential element in the fertility of the soil, contributing to the retention of moisture, and is a source of nutrients for plants. The total humus C parameter is important in the modelling of carbon cycling in ecosystems, as it is an indicator of the amount of carbon stored in the soil." []
is_a: ECOSIM:CATEGORYMicrobialActivity ! category - microbial activity
is_a: ECOSIM:CATEGORYSoilBiogeochemistry ! category - Soil Biogeochemistry
relationship: context ECOSIMCONCEPT:Humus ! Humus
relationship: has_unit ECOSIM:gd-2 ! g d-2
relationship: measured_in ECOSIMCONCEPT:Soil ! Soil
relationship: measurement_of ECOSIMCONCEPT:Carbon ! Carbon

[Term]
id: ECOSIM:UORGF
name: total C amendment
def: "Refers to the total amount of carbon added to a system or an area as an amendment. This could be in the form of organic matter or other carbon-rich materials added to the soil to improve its fertility and functionality." []
is_a: ECOSIM:CATEGORYBiogeochemistry ! category - Biogeochemistry
is_a: ECOSIM:CATEGORYSoilBiogeochemistry ! category - Soil Biogeochemistry
is_a: ECOSIM:CATEGORYTraceGasFlux ! category - trace gas flux
relationship: attribute ECOSIMCONCEPT:Carbon ! Carbon
relationship: has_unit ECOSIM:gd-2 ! g d-2
relationship: measured_in ECOSIMCONCEPT:Soil ! Soil

[Term]
id: ECOSIM:UORGN
name: total humus N
is_a: ECOSIM:CATEGORYMicrobialActivity ! category - microbial activity
relationship: attribute ECOSIMCONCEPT:Nitrogen ! Nitrogen
relationship: has_unit ECOSIM:gd-2 ! g d-2
relationship: measured_in ECOSIMCONCEPT:Humus ! Humus

[Term]
id: ECOSIM:UORGP
name: total humus P
def: "Total humus P refers to the total phosphorous content in the humus component of soil. Humus, the organic component of soil, is rich in nutrients including phosphorous. This plays a key role in plant nutrition and overall soil fertility. Therefore, total humus P is an important factor in earth system modelling and ecological studies." []
is_a: ECOSIM:CATEGORYMicrobialActivity ! category - microbial activity
relationship: has_unit ECOSIM:gd-2 ! g d-2
relationship: measured_in ECOSIMCONCEPT:SoilHumus ! Soil humus
relationship: measurement_of ECOSIMCONCEPT:Phosphorus ! Phosphorus

[Term]
id: ECOSIM:UOXYF
name: total O2 flux from fire
def: "Total O2 flux from fire refers to the total amount of oxygen that is released or absorbed during a fire. This measure includes the oxygen used for combustion as well as the oxygen produced during the burning process. It is a critical component in understanding the impact of fire on the atmosphere and the role it plays in the earth's carbon cycle." []
is_a: ECOSIMCONCEPT:UnclassifiedVariable ! unclassified variable
relationship: attribute ECOSIMCONCEPT:Flux ! Flux
relationship: context ECOSIMCONCEPT:Fire ! Fire
relationship: has_unit ECOSIM:gd-2 ! g d-2
relationship: measured_in ECOSIMCONCEPT:Air ! Air
relationship: measurement_of ECOSIMCONCEPT:Oxygen ! Oxygen

[Term]
id: ECOSIM:UOXYG
name: total soil O2 flux
def: "Total soil O2 flux refers to the total amount of oxygen (O2) exchanged between the soil and the atmosphere through absorption and emission. It is a parameter used in Earth system modeling to understand and simulate the gas exchange between the soil and the atmosphere. This measure plays an important role in the understanding of soil respiration and microbial activity." []
is_a: ECOSIM:CATEGORYBiogeochemistry ! category - Biogeochemistry
is_a: ECOSIM:CATEGORYGasFlux ! category - Gas Flux
is_a: ECOSIM:CATEGORYTraceGasFlux ! category - trace gas flux
relationship: attribute ECOSIMCONCEPT:Flux ! Flux
relationship: has_unit ECOSIM:gd-2 ! g d-2
relationship: measured_in ECOSIMCONCEPT:Soil ! Soil
relationship: measurement_of ECOSIMCONCEPT:O2 ! Dioxygen

[Term]
id: ECOSIM:UPH1P
name: total root uptake of HPO4
is_a: ECOSIMCONCEPT:UnclassifiedVariable ! unclassified variable
relationship: has_unit ECOSIM:gd-2h-1 ! g d-2 h-1
relationship: measured_in ECOSIMCONCEPT:Root ! Root
relationship: measurement_of ECOSIMCONCEPT:HPO4 ! Hydrogen phosphate

[Term]
id: ECOSIM:UPH2P
name: total root uptake of PO4
def: "Total root uptake of PO4 refers to the amount of phosphates, PO4, a plant absorbs from the soil through its roots. This phosphorus uptake is vital for plant growth and development as phosphorus is a key element that plays several roles in plant physiology including energy transfer and storage, photosynthesis, respiration, and synthesis of nucleic acids. This parameter is often measured in Earth system modeling to understand nutrient cycling in ecosystems." []
is_a: ECOSIM:CATEGORYPlantPhysiology ! category - plant physiology
is_a: ECOSIMCONCEPT:UnclassifiedVariable ! unclassified variable
relationship: has_unit ECOSIM:gd-2h-1 ! g d-2 h-1
relationship: measured_in ECOSIMCONCEPT:Root ! Root
relationship: measurement_of ECOSIMCONCEPT:Phosphates ! Phosphates

[Term]
id: ECOSIM:UPKMPO
name: Km for root PO4 uptake
def: "Km for root PO4 uptake refers to the half-maximal velocity constant (Km) of phosphate (PO4) uptake by plant roots. It is a parameter that characterizes the efficiency and capacity of root systems to absorb phosphate from the soil. A lower Km value indicates higher efficiency of phosphate uptake, while a higher Km value indicates lower efficiency. This parameter is important in understanding nutrient dynamics, plant growth and productivity, and strategies for optimizing nutrient use efficiency." []
is_a: ECOSIM:CATEGORYRootPhysiology ! category - root physiology
relationship: attribute ECOSIMCONCEPT:UptakeVelocity ! Uptake velocity
relationship: has_unit ECOSIM:gm-3 ! g m-3
relationship: measured_in ECOSIMCONCEPT:Root ! Root
relationship: measurement_of ECOSIMCONCEPT:PO4 ! Phosphate

[Term]
id: ECOSIM:UPKMZH
name: Km for root NH4 uptake
def: "Km for root NH4 uptake refers to the half-saturation constant for the uptake of ammonium (NH4) by plant roots. It is a parameter used in modeling to describe the nutrient uptake kinetics of plants. A lower Km value indicates a higher affinity of the plant for NH4, meaning that the plant can uptake NH4 efficiently even at low soil NH4 concentrations. Conversely, a higher Km value indicates a lower affinity of the plant for NH4, meaning that the plant needs higher soil NH4 concentrations to uptake NH4 efficiently. The Km for root NH4 uptake is an important factor that influences nutrient cycling, plant nutrition, and productivity." []
is_a: ECOSIM:CATEGORYRootPhysiology ! category - root physiology
relationship: attribute ECOSIMCONCEPT:HalfSaturationConstant ! Half saturation constant
relationship: has_unit ECOSIM:gm-3 ! g m-3
relationship: measured_in ECOSIMCONCEPT:Root ! Root
relationship: measurement_of ECOSIMCONCEPT:AmmoniumUptake ! Ammonium uptake

[Term]
id: ECOSIM:UPKMZO
name: Km for root NO3 uptake
is_a: ECOSIM:CATEGORYPlantPhysiology ! category - plant physiology
is_a: ECOSIM:CATEGORYRootPhysiology ! category - root physiology
relationship: attribute ECOSIMCONCEPT:UptakeKinetics ! Uptake kinetics
relationship: has_unit ECOSIM:gm-3 ! g m-3
relationship: measured_in ECOSIMCONCEPT:Root ! Root
relationship: measurement_of ECOSIMCONCEPT:NO3 ! Nitrate

[Term]
id: ECOSIM:UPMNPO
name: minimum PO4 concentration for root NH4 uptake
def: "Minimum PO4 concentration for root NH4 uptake refers to the minimum concentration of phosphate (PO4) in the soil solution that allows roots of plants to absorb or take up ammonium (NH4). Ammonium is a form of nitrogen that is absorbed by plant roots from the soil and used as a nutrient. The absorption of ammonium by plant roots is often dependent on the concentration of other nutrients in the soil solution, including phosphate. By defining the minimum PO4 concentration for root NH4 uptake, it becomes possible to better understand and model nutrient dynamics and plant nutrition in soil ecosystems." []
is_a: ECOSIM:CATEGORYRootPhysiology ! category - root physiology
relationship: has_unit ECOSIM:gm-3 ! g m-3
relationship: measured_in ECOSIMCONCEPT:Root ! Root
relationship: measurement_of ECOSIMCONCEPT:Phosphate ! Phosphate

[Term]
id: ECOSIM:UPMNZH
name: minimum NH4 concentration for root NH4 uptake
is_a: ECOSIM:CATEGORYRootPhysiology ! category - root physiology
relationship: has_unit ECOSIM:gm-3 ! g m-3
relationship: measured_in ECOSIMCONCEPT:Root ! Root

[Term]
id: ECOSIM:UPMNZO
name: minimum NO3 concentration for root NH4 uptake
def: "The minimum concentration of nitrate (NO3) required in root zone for root ammonium (NH4) uptake" []
is_a: ECOSIM:CATEGORYPlantPhysiology ! category - plant physiology
is_a: ECOSIM:CATEGORYRootPhysiology ! category - root physiology
relationship: has_unit ECOSIM:gm-3 ! g m-3
relationship: measured_in ECOSIMCONCEPT:RootZone ! Root zone

[Term]
id: ECOSIM:UPMXPO
name: maximum root PO4 uptake rate
is_a: ECOSIM:CATEGORYPlantPhysiology ! category - plant physiology
is_a: ECOSIM:CATEGORYRootPhysiology ! category - root physiology
relationship: attribute ECOSIMCONCEPT:UptakeRate ! UptakeRate
relationship: context ECOSIMCONCEPT:Root ! Root
relationship: has_unit ECOSIM:gm-2h-1 ! g m-2 h-1
relationship: measurement_of ECOSIMCONCEPT:PO4 ! Phosphate

[Term]
id: ECOSIM:UPMXZH
name: maximum root NH4 uptake rate
def: "The maximum rate at which roots can take up ammonium (NH4) from the soil. This rate can depend on various factors, such as the concentration of NH4 in the soil, the root characteristics, temperature, and soil moisture." []
is_a: ECOSIM:CATEGORYRootPhysiology ! category - root physiology
relationship: has_unit ECOSIM:gm-2h-1 ! g m-2 h-1
relationship: measured_in ECOSIMCONCEPT:Root ! Root
relationship: measurement_of ECOSIMCONCEPT:AmmoniumUptakeRate ! Ammonium uptake rate

[Term]
id: ECOSIM:UPMXZO
name: maximum root NO3 uptake rate
is_a: ECOSIM:CATEGORYPlantPhysiology ! category - plant physiology
is_a: ECOSIM:CATEGORYRootPhysiology ! category - root physiology
relationship: has_unit ECOSIM:gm-2h-1 ! g m-2 h-1
relationship: measured_in ECOSIMCONCEPT:Root ! Root
relationship: measurement_of ECOSIMCONCEPT:NO3 ! Nitrate
relationship: measurement_of ECOSIMCONCEPT:UptakeRate ! UptakeRate

[Term]
id: ECOSIM:UPNF
name: total root N2 fixation
def: "Total root N2 fixation refers to the total amount of nitrogen that is fixed by the root system of a plant through the process of nitrogen fixation. Nitrogen fixation is the process by which nitrogen in the air is converted into a form that can be used by plants for growth. This is an essential process in the nitrogen cycle and is particularly important in agricultural systems." []
is_a: ECOSIM:CATEGORYPlantPhysiology ! category - plant physiology
is_a: ECOSIMCONCEPT:UnclassifiedVariable ! unclassified variable
relationship: has_unit ECOSIM:gd-2h-1 ! g d-2 h-1
relationship: measured_in ECOSIMCONCEPT:Root ! Root
relationship: measurement_of ECOSIMCONCEPT:NitrogenFixation ! Nitrogen fixation

[Term]
id: ECOSIM:UPNH4
name: total root uptake of NH4
def: "Total root uptake of NH4 refers to the process whereby plant roots absorb ammonium (NH4) from the surrounding soil. This process is important for plant growth, as NH4 is a key form of nitrogen, a critical nutrient for plants. Ammonium uptake is influenced by various factors including soil properties, environmental conditions, and plant species characteristics." []
is_a: ECOSIM:CATEGORYRootPhysiology ! category - root physiology
is_a: ECOSIMCONCEPT:UnclassifiedVariable ! unclassified variable
relationship: attribute ECOSIMCONCEPT:Uptake ! Uptake
relationship: has_unit ECOSIM:gd-2h-1 ! g d-2 h-1
relationship: measured_in ECOSIMCONCEPT:Root ! Root
relationship: measurement_of ECOSIMCONCEPT:Ammonium ! Ammonium

[Term]
id: ECOSIM:UPNO3
name: total root uptake of NO3
is_a: ECOSIMCONCEPT:UnclassifiedVariable ! unclassified variable
relationship: attribute ECOSIMCONCEPT:Uptake ! Uptake
relationship: has_unit ECOSIM:gd-2h-1 ! g d-2 h-1
relationship: measured_in ECOSIMCONCEPT:Root ! Root
relationship: measurement_of ECOSIMCONCEPT:NO3 ! Nitrate

[Term]
id: ECOSIM:UPO4
name: total soil PO4 content
def: "Total soil PO4 content refers to the collective amount of phosphate (PO4) ions held within the soil. Phosphate is a form of phosphorus which is considered an essential nutrient for plant life. It is necessary for various biological processes including energy metabolism and the synthesis of nucleic acids. The total soil PO4 content can influence nutrient availability and uptake by plants, as well as overall soil fertility. Assessing the total soil PO4 content is important for agricultural practices and soil management strategies." []
is_a: ECOSIM:CATEGORYMicrobialActivity ! category - microbial activity
is_a: ECOSIM:CATEGORYSoilBiogeochemistry ! category - Soil Biogeochemistry
relationship: has_unit ECOSIM:gd-2 ! g d-2
relationship: measured_in ECOSIMCONCEPT:Soil ! Soil
relationship: measurement_of ECOSIMCONCEPT:PO4 ! Phosphate

[Term]
id: ECOSIM:UPO4F
name: total PO4 flux from fire
def: "Total PO4 flux from fire refers to the quantity of phosphate, an essential plant nutrient, that is expelled into the environment as a result of combustion processes. Fire events cause the release of nutrients, including phosphate, which are usually bound in plant biomass and soil organic matter. These nutrients can then be transported through smoke, ash, or post-fire run-off. Understanding the flux of these nutrients helps in assessing the impacts of fires on nutrient cycling and ecosystem productivity." []
is_a: ECOSIMCONCEPT:UnclassifiedVariable ! unclassified variable
relationship: attribute ECOSIMCONCEPT:Flux ! Flux
relationship: has_unit ECOSIM:gd-2 ! g d-2
relationship: measurement_of ECOSIMCONCEPT:PO4 ! Phosphate

[Term]
id: ECOSIM:UPOME
name: total root uptake (+ve) - exudation (-ve) of dissovled element
def: "Total root uptake refers to the positive value of the amount of a specific dissolved element absorbed by the roots from the soil solution. Exudation refers to the negative value of the amount of that element released by the roots back to the soil. This parameter plays a vital role in soil-plant nutrient cycling and can help provide insights into the nutrient acquisition strategies of plants in different soil conditions." []
is_a: ECOSIM:CATEGORYRootPhysiology ! category - root physiology
is_a: ECOSIMCONCEPT:UnclassifiedVariable ! unclassified variable
relationship: has_unit ECOSIM:gd-2h-1 ! g d-2 h-1
relationship: measured_in ECOSIMCONCEPT:Root ! Root

[Term]
id: ECOSIM:UPP4
name: total soil precipited P
def: "Total soil precipitated P refers to the total amount of phosphorus (P) in the soil that is in a precipitated form. It is an important measure of the nutrient status of the soil, as phosphorus is a vital nutrient for plant growth. This parameter is often used in Earth system modeling to understand and simulate nutrient cycling and soil fertility." []
is_a: ECOSIM:CATEGORYBiogeochemistry ! category - Biogeochemistry
is_a: ECOSIM:CATEGORYTraceGasFlux ! category - trace gas flux
relationship: has_unit ECOSIM:gd-2 ! g d-2
relationship: measured_in ECOSIMCONCEPT:Soil ! Soil
relationship: measurement_of ECOSIMCONCEPT:Phosphorus ! Phosphorus

[Term]
id: ECOSIM:URAIN
name: total precipitation
def: "Total precipitation refers to the sum of all forms of precipitation, including rain, snow, sleet, and hail, over a certain period. It is a crucial element of the Earth’s water cycle, and its measurement is critical for meteorology, hydrology, and climatology. Notably, total precipitation enables the quantification of water resources and facilitates the understanding of weather patterns and climate change." []
is_a: ECOSIM:CATEGORYHydrology ! category - Hydrology
relationship: has_unit ECOSIM:m3d-2 ! m3 d-2
relationship: measured_in ECOSIMCONCEPT:Atmosphere ! Atmosphere
relationship: measurement_of ECOSIMCONCEPT:Water ! Water

[Term]
id: ECOSIM:URSDC
name: total litter C
def: "Total litter carbon (URSDC) refers to the total amount of carbon in organic material and debris, such as leaves, twigs, and other dead plant parts, present on the soil surface. This parameter is used in earth system models to understand and simulate the cycling of carbon and nutrients in terrestrial ecosystems. The decomposition of litter plays a crucial role in providing nutrients for plant growth and in sequestering carbon." []
is_a: ECOSIM:CATEGORYMicrobialActivity ! category - microbial activity
is_a: ECOSIMCONCEPT:Litter ! Litter
relationship: has_unit ECOSIM:gd-2 ! g d-2
relationship: measurement_of ECOSIMCONCEPT:Carbon ! Carbon

[Term]
id: ECOSIM:URSDN
name: total litter N
def: "Total litter N refers to the total amount of nitrogen contained in the layer of dead organic material (leaves, branches, etc.) that covers the soil in forest ecosystems. It is an important element of the nutrient cycle as the litter decomposition releases the nutrients making it available for plants." []
is_a: ECOSIM:CATEGORYMicrobialActivity ! category - microbial activity
relationship: has_unit ECOSIM:gd-2 ! g d-2
relationship: measured_in ECOSIMCONCEPT:Litter ! Litter
relationship: measurement_of ECOSIMCONCEPT:Nitrogen ! Nitrogen

[Term]
id: ECOSIM:URSDP
name: total litter P
is_a: ECOSIM:CATEGORYMicrobialActivity ! category - microbial activity
relationship: has_unit ECOSIM:gd-2 ! g d-2
relationship: measurement_of ECOSIMCONCEPT:Litter ! Litter

[Term]
id: ECOSIM:URUN
name: total surface runoff
def: "Total surface runoff, commonly referred to as 'runoff', is the part of the water cycle that flows over land as surface water instead of being absorbed into the ground or evaporating into the air. It is a major component of the water cycle, and it is responsible for transporting water from the land to the ocean. Runoff can originate from rain, snowmelt, and other forms of precipitation, and it is major source of water pollution, carrying surface pollutants through the environment. In Earth systems modeling, total surface runoff is a key variable which helps us understand and simulate the water flow within a catchment area." []
is_a: ECOSIM:CATEGORYHydrology ! category - Hydrology
relationship: has_unit ECOSIM:m3d-2 ! m3 d-2
relationship: measured_in ECOSIMCONCEPT:Runoff ! Runoff
relationship: measurement_of ECOSIMCONCEPT:Water ! Water

[Term]
id: ECOSIM:USEDOU
name: total sediment subsurface flux
def: "Total sediment subsurface flux refers to the total amount of sediment that is transported below the surface level due to natural processes such as soil erosion, landslide, and others. It is an important measure in the study of land degradation, soil conservation, and sediment transport." []
is_a: ECOSIM:CATEGORYTraceGasFlux ! category - trace gas flux
relationship: attribute ECOSIMCONCEPT:Flux ! Flux
relationship: has_unit ECOSIM:Mgd-2 ! Mg d-2
relationship: measured_in ECOSIMCONCEPT:Subsurface ! Subsurface
relationship: measurement_of ECOSIMCONCEPT:Sediment ! Sediment

[Term]
id: ECOSIM:UVLWatMicP
name: total soil water content
def: "Total soil water content refers to the volume of water contained within a soil sample, usually expressed as a percentage of the total volume of the soil. It is an important parameter in the study of soil and environmental sciences because it affects various physical, chemical, and biological properties of the soil such as its permeability, nutrient cycling, and microbial activity. Soil water content is also a critical factor for plant growth as it affects the availability of water for plant uptake." []
is_a: ECOSIMCONCEPT:UnclassifiedVariable ! unclassified variable
relationship: attribute ECOSIMCONCEPT:WaterContent ! Water content
relationship: has_unit ECOSIM:m3d-2 ! m3 d-2
relationship: measured_in ECOSIMCONCEPT:Soil ! Soil

[Term]
id: ECOSIM:UVOLO
name: total subsurface water flux
def: "Total subsurface water flux refers to the collective movement of water below the surface of the Earth, including through soil, substrates, and aquifers. It represents the sum of various flux-related processes such as infiltration, percolation, groundwater flow, and capillary rise. This parameter plays a crucial role in hydrology and Earth system modeling, influencing various processes like nutrient cycling, crop production, and ecosystem functioning, as well as human activities such as water supply and irrigation practices." []
is_a: ECOSIM:CATEGORYHydrology ! category - Hydrology
relationship: attribute ECOSIMCONCEPT:WaterFlux ! WaterFlux
relationship: has_unit ECOSIM:m3d-2 ! m3 d-2
relationship: measured_in ECOSIMCONCEPT:Subsurface ! Subsurface

[Term]
id: ECOSIM:UXCSN
name: total litterfall C
def: "Total litterfall carbon refers to the total amount of carbon contained in plant material (leaves, branches, etc.) that falls to the ground in a given time period. It's an important variable in carbon cycle modeling as it is a major source of carbon input to the soil through decomposition." []
is_a: ECOSIM:CATEGORYTraceGasFlux ! category - trace gas flux
relationship: has_unit ECOSIM:gd-2 ! g d-2
relationship: measured_in ECOSIMCONCEPT:Litter ! Litter
relationship: measurement_of ECOSIMCONCEPT:Carbon ! Carbon

[Term]
id: ECOSIM:UXPSN
name: total litterfall P
def: "Total Litterfall P pertains to the total annual Phosphorus (P) content as measured in litterfall." []
is_a: ECOSIM:CATEGORYTraceGasFlux ! category - trace gas flux
is_a: ECOSIMCONCEPT:Litterfall ! Litterfall
relationship: has_unit ECOSIM:gd-2 ! g d-2
relationship: measured_in ECOSIMCONCEPT:Litterfall ! Litterfall

[Term]
id: ECOSIM:UXZSN
name: total litterfall N
is_a: ECOSIM:CATEGORYTraceGasFlux ! category - trace gas flux
relationship: has_unit ECOSIM:gd-2 ! g d-2
relationship: measured_in ECOSIMCONCEPT:Litterfall ! Litterfall
relationship: measurement_of ECOSIMCONCEPT:Nitrogen ! Nitrogen

[Term]
id: ECOSIM:VCGR4
name: maximum dark C4 carboxylation rate under saturating CO2
def: "VCGR4 refers to the maximum rate of C4 carboxylation in the dark under  saturating CO2 which represents a key physiological parameter in C4 photosynthesis. This rate is indicative of the plant's metabolic capacity to convert CO2 into energy-rich molecules in the absence of sunlight." []
is_a: ECOSIM:CATEGORYCanopyPhysiology ! category - Canopy Physiology
is_a: ECOSIM:CATEGORYPlantPhysiology ! category - plant physiology
relationship: attribute ECOSIMCONCEPT:MetabolicRate ! Metabolic rate
relationship: has_unit ECOSIM:umolm-2s-1 ! umol m-2 s-1
relationship: measured_in ECOSIMCONCEPT:Leaf ! Leaf
relationship: measurement_of ECOSIMCONCEPT:C4Carboxylation ! C4 carboxylation

[Term]
id: ECOSIM:VCGRO
name: maximum dark carboxylation rate under saturating CO2
is_a: ECOSIM:CATEGORYCanopyPhysiology ! category - Canopy Physiology
is_a: ECOSIM:CATEGORYPlantPhysiology ! category - plant physiology
relationship: has_unit ECOSIM:umolm-2s-1 ! umol m-2 s-1
relationship: measurement_of ECOSIMCONCEPT:CO2CarboxylationRate ! Carbon dioxide carboxylation rate

[Term]
id: ECOSIM:VCH4F
name: plant CH4 emission from fire
def: "Refers to the emission of methane (CH4), a powerful greenhouse gas, from plants during a fire event." []
is_a: ECOSIMCONCEPT:UnclassifiedVariable ! unclassified variable
relationship: attribute ECOSIMCONCEPT:Plant ! Plant
relationship: has_unit ECOSIM:gd-2 ! g d-2
relationship: measured_in ECOSIMCONCEPT:Fire ! Fire
relationship: measurement_of ECOSIMCONCEPT:Ch4Emission ! Methane emission

[Term]
id: ECOSIM:VCMX
name: rubisco carboxylase activity
def: "The maximum carboxylation rate of the enzyme Rubisco. It is an important parameter in plant physiology and biochemistry, as it determines the maximum rate at which plants can assimilate carbon dioxide during photosynthesis." []
is_a: ECOSIM:CATEGORYPlantPhysiology ! category - plant physiology
is_a: ECOSIMCONCEPT:UnclassifiedVariable ! unclassified variable
relationship: attribute ECOSIMCONCEPT:Activity ! Activity
relationship: has_unit ECOSIM:umolg-1h-1at25oC ! umol g-1 h-1 at 25 oC
relationship: measured_in ECOSIMCONCEPT:Leaf ! Leaf
relationship: measurement_of ECOSIMCONCEPT:RubiscoActivity ! Rubisco activity

[Term]
id: ECOSIM:VCMX4
name: PEP carboxylase activity
is_a: ECOSIM:CATEGORYPlantPhysiology ! category - plant physiology
is_a: ECOSIMCONCEPT:UnclassifiedVariable ! unclassified variable
relationship: attribute ECOSIMCONCEPT:Activity ! Activity
relationship: has_unit ECOSIM:umolg-1h-1at25oC ! umol g-1 h-1 at 25 oC
relationship: measured_in ECOSIMCONCEPT:Leaf ! Leaf
relationship: measurement_of ECOSIMCONCEPT:PEPCarboxylase ! Phosphoenolpyruvate carboxylase

[Term]
id: ECOSIM:VCO2F
name: plant CO2 emission from fire
def: "VCO2F refers to the volume of CO2 emitted due to combustion of plant biomass during wildfires. Wildfires return substantial amounts of carbon that was sequestered by plants back into the atmosphere. This parameter is essential to capture the full carbon cycle including influence of fire disturbances in Earth system models." []
is_a: ECOSIM:CATEGORYBiogeochemistry ! category - Biogeochemistry
is_a: ECOSIMCONCEPT:UnclassifiedVariable ! unclassified variable
relationship: attribute ECOSIMCONCEPT:Emission ! Emission
relationship: context ECOSIMCONCEPT:Fire ! Fire
relationship: has_unit ECOSIM:gd-2 ! g d-2
relationship: measured_in ECOSIMCONCEPT:Plant ! Plant
relationship: measurement_of ECOSIMCONCEPT:CO2 ! Carbon dioxide

[Term]
id: ECOSIM:VGRO
name: carboxylation rate
def: "Carboxylation rate refers to the rate at which carbon dioxide (CO2) is incorporated into organic compounds in the photosynthetic process in plants. It is a key parameter in plant physiology and growth studies, and can be influenced by various factors such as light intensity, temperature, water availability, and CO2 concentration in the atmosphere." []
is_a: ECOSIM:CATEGORYCanopyPhysiology ! category - Canopy Physiology
is_a: ECOSIM:CATEGORYPlantPhysiology ! category - plant physiology
relationship: attribute ECOSIMCONCEPT:Rate ! Rate
relationship: has_unit ECOSIM:umolm-2s-1 ! umol m-2 s-1
relationship: measured_in ECOSIMCONCEPT:Leaf ! Leaf
relationship: measurement_of ECOSIMCONCEPT:CO2 ! Carbon dioxide

[Term]
id: ECOSIM:VGRO4
name: C4 carboxylation rate
def: "C4 carboxylation rate is a measure of the speed at which a plant is able to convert carbon dioxide into a four carbon compound during the process of photosynthesis. This is an important factor in determining a plant's overall efficiency in converting sunlight into energy." []
is_a: ECOSIM:CATEGORYCanopyPhysiology ! category - Canopy Physiology
is_a: ECOSIM:CATEGORYPlantPhysiology ! category - plant physiology
relationship: attribute ECOSIMCONCEPT:Activity ! Activity
relationship: has_unit ECOSIM:umolm-2s-1 ! umol m-2 s-1
relationship: measured_in ECOSIMCONCEPT:Leaf ! Leaf
relationship: measurement_of ECOSIMCONCEPT:C4CarboxylationRate ! C4 carboxylation rate

[Term]
id: ECOSIM:VHeatCapCanP
name: canopy heat capacity
is_a: ECOSIM:CATEGORYPlantPhysiology ! category - plant physiology
is_a: ECOSIMCONCEPT:UnclassifiedVariable ! unclassified variable
relationship: has_unit ECOSIM:MJd-2K-1 ! MJ d-2 K-1
relationship: measured_in ECOSIMCONCEPT:Canopy ! Canopy
relationship: measurement_of ECOSIMCONCEPT:VHeatCap ! VHeatCap

[Term]
id: ECOSIM:VHeatCapLitR
name: threshold surface litter heat capacity
def: "Threshold surface litter heat capacity refers to the minimum amount of heat energy required to change the temperature of a given amount of surface litter by a certain degree. It is an important parameter in the modelling of fire dynamics and the effects of wildfires on ecosystems, as it helps to determine the susceptiblity of surface litter to ignition and combustion." []
is_a: ECOSIMCONCEPT:UnclassifiedVariable ! unclassified variable
relationship: attribute ECOSIMCONCEPT:HeatCapacity ! Heat capacity
relationship: has_unit ECOSIM:MJd-2K-1 ! MJ d-2 K-1
relationship: measured_in ECOSIMCONCEPT:SurfaceLitter ! Surface litter

[Term]
id: ECOSIM:VLHeatCapSnow
name: snowpack heat capacity
def: "Snowpack heat capacity refers to the amount of heat energy required to raise the temperature of a given amount of snow by a certain degree. It is a critical parameter for understanding the thermal properties of the snowpack, predicting snowmelt rates and timing, and modeling the impacts of snow on local and regional climate." []
is_a: ECOSIM:CATEGORYSnowpack ! category - Snowpack
relationship: attribute ECOSIMCONCEPT:HeatCapacity ! Heat capacity
relationship: has_unit ECOSIM:MJm-3K-1 ! MJ m-3 K-1
relationship: measured_in ECOSIMCONCEPT:Snow ! Snow

[Term]
id: ECOSIM:VLNHB
name: NH4 band volume fracrion
def: "NH4 band volume fraction refers to the volume percentage of the ammonium ion (NH4+) in a given band or section in a medium. It represents the distribution of NH4+ ions within the band, often used in studies related to earth system modeling, cloud process simulation, or aerosol chemistry. This parameter helps understand the dispersion, interactions, and transformations of NH4+ in the environment, which can influence processes like nutrient cycling and atmospheric chemistry." []
is_a: ECOSIMCONCEPT:UnclassifiedVariable ! unclassified variable
relationship: attribute ECOSIMCONCEPT:VolumeFraction ! Volume fraction
relationship: measured_in ECOSIMCONCEPT:Band ! Band
relationship: measurement_of ECOSIMCONCEPT:NH4 ! Ammonium

[Term]
id: ECOSIM:VLNOB
name: NO3 band volume fracrion
def: "NO3 band volume fraction refers to the fraction of volume that nitrate (NO3) occupies in a particular band. It is a fraction by volume of the NO3 band to the total volume. This parameter is important for earth system modeling to understand the dispersion and distribution of nitrate in different layers of the earth's system." []
is_a: ECOSIMCONCEPT:UnclassifiedVariable ! unclassified variable
relationship: attribute ECOSIMCONCEPT:Fraction ! Fraction
relationship: measured_in ECOSIMCONCEPT:Volume ! Volume

[Term]
id: ECOSIM:VLPO4
name: PO4 non-band volume fracrion
def: "PO4 non-band volume fraction refers to the fraction of a sample's total volume that is not occupied by the phosphate (PO4) band. This parameter is an important indicator in spectrophotometric measurements and can be used to determine the concentration of phosphate in a sample." []
is_a: ECOSIMCONCEPT:UnclassifiedVariable ! unclassified variable
relationship: attribute ECOSIMCONCEPT:VolumeFraction ! Volume fraction
relationship: measurement_of ECOSIMCONCEPT:PO4 ! Phosphate

[Term]
id: ECOSIM:VLPOB
name: PO4 band volume fracrion
is_a: ECOSIMCONCEPT:UnclassifiedVariable ! unclassified variable
relationship: attribute ECOSIMCONCEPT:VolumeFraction ! Volume fraction
relationship: measurement_of ECOSIMCONCEPT:PO4band ! Phosphate band

[Term]
id: ECOSIM:VLSnowt0
name: Initial snowpack volume
is_a: ECOSIM:CATEGORYSnowpack ! category - Snowpack
relationship: attribute ECOSIMCONCEPT:Volume ! Volume
relationship: has_unit ECOSIM:m3d-2 ! m3 d-2
relationship: measured_in ECOSIMCONCEPT:Snow ! Snow

[Term]
id: ECOSIM:VLWatMacPM
name: macropore water flux
def: "Macropore water flux refers to the rate at which water moves through the large pores within the soil structure. Macropores, typically greater than 0.05mm in diameter, play a crucial role in soil hydrology, influencing water infiltration, storage, and redistribution within the soil. The macropore water flux can be influenced by factors such as soil type, texture, structure, and organic matter content, as well as external conditions such as precipitation, temperature, and evaporation rates." []
is_a: ECOSIM:CATEGORYHydrology ! category - Hydrology
is_a: ECOSIMCONCEPT:UnclassifiedVariable ! unclassified variable
relationship: attribute ECOSIMCONCEPT:Flux ! Flux
relationship: has_unit ECOSIM:m3d-2 ! m3 d-2
relationship: measured_in ECOSIMCONCEPT:SoilMacropore ! SoilMacropore
relationship: measurement_of ECOSIMCONCEPT:Water ! Water

[Term]
id: ECOSIM:VLWatMicPM
name: micropore water flux
def: "The micropore water flux is the volume of water moving through the micropores in the soil per unit time. This can be influenced by various factors, including soil type, texture, precipitation, and evaporation rates among others." []
is_a: ECOSIM:CATEGORYHydrology ! category - Hydrology
is_a: ECOSIMCONCEPT:UnclassifiedVariable ! unclassified variable
relationship: has_unit ECOSIM:m3d-2 ! m3 d-2
relationship: measured_in ECOSIMCONCEPT:SoilMicropore ! Soil micropore
relationship: measurement_of ECOSIMCONCEPT:Water ! Water

[Term]
id: ECOSIM:VLitR
name: surface litter volume
is_a: ECOSIMCONCEPT:UnclassifiedVariable ! unclassified variable
relationship: attribute ECOSIMCONCEPT:Volume ! Volume
relationship: has_unit ECOSIM:m3d-2 ! m3 d-2
relationship: measured_in ECOSIMCONCEPT:SurfaceLitter ! Surface litter

[Term]
id: ECOSIM:VLsoiAirPM
name: soil air content
def: "Soil air content refers to the volume or percentage of air space in a soil sample. It determines the amount of oxygen available to roots and soil organisms. Proper soil aeration is essential for the health of soil ecosystems, as it affects root growth, nutrient uptake by plants, and the activity of soil microorganisms. It is considered a key factor in soil health, productivity, and sustainability. Typically, a soil with an air content of about 50% is considered ideal for plant growth. More compacted soils have less air space and can become waterlogged, while lighter, sandy soils may have higher air space but less water and nutrient retention." []
is_a: ECOSIM:CATEGORYSoilProperty ! category - soil property
is_a: ECOSIMCONCEPT:UnclassifiedVariable ! unclassified variable
relationship: has_unit ECOSIM:m3d-2 ! m3 d-2
relationship: measured_in ECOSIMCONCEPT:Soil ! Soil

[Term]
id: ECOSIM:VN2OF
name: plant N2O emission from fire
def: "Plant N2O emission from fire refers to the amount of nitrous oxide (N2O) released by plants during a fire event. It represents the contribution of vegetation to N2O emissions under burning conditions. This parameter is important in Earth system modeling as it helps understand the role of wildfires in altering greenhouse gas dynamics and contributing to climate change. It is influenced by the type and quantity of the biomass burned, fire intensity, and environmental conditions." []
is_a: ECOSIM:CATEGORYNTransformation ! category - N transformation
is_a: ECOSIMCONCEPT:UnclassifiedVariable ! unclassified variable
relationship: attribute ECOSIMCONCEPT:Emission ! Emission
relationship: context ECOSIMCONCEPT:Fire ! Fire
relationship: has_unit ECOSIM:gd-2 ! g d-2
relationship: measured_in ECOSIMCONCEPT:Plant ! Plant
relationship: measurement_of ECOSIMCONCEPT:N2O ! Nitrous oxide

[Term]
id: ECOSIM:VNH3F
name: plant NH3 emission from fire
def: "The amount of Ammonia (NH3) released into the atmosphere as a result of fire or burning in vegetation area." []
is_a: ECOSIMCONCEPT:UnclassifiedVariable ! unclassified variable
relationship: has_unit ECOSIM:gd-2 ! g d-2
relationship: measurement_of ECOSIMCONCEPT:NH3 ! Ammonia

[Term]
id: ECOSIM:VOLQ
name: soil water volume occupied by microial biomass
def: "Soil water volume occupied by microbial biomass refers to the portion of the total soil water volume that is occupied by the biomass of microorganisms present in the soil, including bacteria, fungi, and other microbes. This metric provides information about the microbial activity and the nutrient cycling capacity of the soil. Microbial biomass plays a significant role in various soil processes, including organic matter decomposition, nutrient cycling, and the formation of soil structure, and can serve as an indicator of soil health and fertility." []
is_a: ECOSIM:CATEGORYNTransformation ! category - N transformation
is_a: ECOSIM:CATEGORYSoilBiogeochemistry ! category - Soil Biogeochemistry
relationship: attribute ECOSIMCONCEPT:Volume ! Volume
relationship: has_unit ECOSIM:m3m-3 ! m3 m-3
relationship: measured_in ECOSIMCONCEPT:SoilWater ! Soil water
relationship: measurement_of ECOSIMCONCEPT:MicrobialBiomass ! MicrobialBiomass

[Term]
id: ECOSIM:VOMX
name: rubisco oxygenase activity
def: "Rubisco oxygenase activity refers to the rate or extent of the reaction catalyzed by the enzyme Rubisco (Ribulose-1,5-bisphosphate carboxylase/oxygenase) that involves the incorporation of oxygen (O2) into RuBP (ribulose-1,5-bisphosphate). This reaction is part of the photorespiratory pathway, which is a side reaction of photosynthesis in plants and cyanobacteria. Understanding Rubisco oxygenase activity is important for studying and modeling plant physiology and responses to environmental changes, as well as for crop improvement and climate change research." []
is_a: ECOSIM:CATEGORYPlantPhysiology ! category - plant physiology
is_a: ECOSIMCONCEPT:UnclassifiedVariable ! unclassified variable
relationship: attribute ECOSIMCONCEPT:Activity ! Activity
relationship: has_unit ECOSIM:umolg-1h-1at25oC ! umol g-1 h-1 at 25 oC
relationship: measured_in ECOSIMCONCEPT:Leaf ! Leaf
relationship: measurement_of ECOSIMCONCEPT:RubiscoOxygenase ! Rubisco oxygenase

[Term]
id: ECOSIM:VOXYF
name: plant O2 uptake from fire
def: "VOXYF refers to the concept of plant oxygen uptake from fire. It means how much oxygen plants consume during a fire event." []
is_a: ECOSIMCONCEPT:UnclassifiedVariable ! unclassified variable
relationship: context ECOSIMCONCEPT:Fire ! Fire
relationship: has_unit ECOSIM:gd-2 ! g d-2
relationship: measured_in ECOSIMCONCEPT:Plant ! Plant
relationship: measurement_of ECOSIMCONCEPT:Oxygen ! Oxygen

[Term]
id: ECOSIM:VPA
name: vapor concentration
def: "Vapor concentration refers to the amount of a substance present in the air in the form of gas or vapor. It is usually expressed in terms of mass or volume of the substance per unit volume of air. Vapor concentration is an important parameter in atmospheric sciences and environmental studies as it can affect air quality, climate and weather patterns, and the health and wellbeing of organisms." []
is_a: ECOSIM:CATEGORYAtmosphericConditions ! category - Atmospheric Conditions
relationship: attribute ECOSIMCONCEPT:Concentration ! Concentration
relationship: has_unit ECOSIM:m3m-3 ! m3 m-3
relationship: measurement_of ECOSIMCONCEPT:Vapor ! Vapor

[Term]
id: ECOSIM:VPK
name: vapor pressure
def: "Vapor pressure refers to the pressure exerted by a vapor in thermodynamic equilibrium with its condensed phases at a given temperature in a closed system. It is indicative of a liquid's or solid's evaporation rate." []
is_a: ECOSIM:CATEGORYAtmosphericConditions ! category - Atmospheric Conditions
relationship: attribute ECOSIMCONCEPT:Pressure ! Pressure
relationship: has_unit ECOSIM:kPa ! kPa

[Term]
id: ECOSIM:VPO4F
name: plant PO4 emission from fire
def: "Release of phosphate or PO4 from plant material during a fire event. It's a specific form of nutrient release during biomass burning and plays a role in biogeochemical cycles." []
is_a: ECOSIM:CATEGORYBiogeochemistry ! category - Biogeochemistry
is_a: ECOSIMCONCEPT:Emission ! Emission
is_a: ECOSIMCONCEPT:UnclassifiedVariable ! unclassified variable
relationship: context ECOSIMCONCEPT:Fire ! Fire
relationship: has_unit ECOSIM:gd-2 ! g d-2
relationship: measurement_of ECOSIMCONCEPT:PO4 ! Phosphate

[Term]
id: ECOSIM:VRNF
name: cold requirement for autumn leafoff/hardening
def: "Cold requirement for autumn leafoff/hardening (VRNF) refers to the amount of cold exposure (in terms of temperature and duration) required by certain plant species to trigger their transition to autumn or winter mode, which typically involves shedding leaves (leafoff) and/or undergoing physiological changes to harden or prepare for the harsh winter conditions. This cold requirement is typically expressed as a specific number of chill hours (hours of exposure to temperatures below a certain threshold). Understanding this requirement is important for predicting the seasonal behaviour and geographic distribution of plants, as well as simulating ecosystem responses to changes in climate." []
is_a: ECOSIM:CATEGORYCanopyStructure ! category - canopy structure
relationship: attribute ECOSIMCONCEPT:ColdRequirement ! Cold requirement
relationship: has_unit ECOSIM:h ! h
relationship: measured_in ECOSIMCONCEPT:Plant ! Plant

[Term]
id: ECOSIM:VRNL
name: hours above threshold temperature required for spring leafout/dehardening
def: "The total number of hours that the temperature stays above a certain threshold, which is typically required for spring leafout or dehardening processes in plants. This is an important parameter for understanding plant phenology and growth dynamics." []
is_a: ECOSIM:CATEGORYCanopyPhysiology ! category - Canopy Physiology
is_a: ECOSIM:CATEGORYCanopyStructure ! category - canopy structure
relationship: attribute ECOSIMCONCEPT:Temperature ! temperature

[Term]
id: ECOSIM:VRNS
name: heat requirement for spring leafout/dehardening
def: "Heat requirement for spring leafout/dehardening represents the quantity of accumulated heat (typically measured in degree days) a plant or tree species requires before its buds burst and leaves unfold (leafout) or lose their frost resistance (dehardening) in the spring. This parameter is important for understanding and predicting plant phenology and its responses to climate change." []
is_a: ECOSIM:CATEGORYCanopyStructure ! category - canopy structure
is_a: ECOSIM:CATEGORYPlantPhysiology ! category - plant physiology
relationship: has_unit ECOSIM:h ! h
relationship: measurement_of ECOSIMCONCEPT:Dehardening ! Dehardening
relationship: measurement_of ECOSIMCONCEPT:HeatRequirement ! HeatRequirement
relationship: measurement_of ECOSIMCONCEPT:SpringLeafout ! Spring leaf out

[Term]
id: ECOSIM:VRNX
name: number of hours below set temperature required for autumn leafoff/hardening
def: "Number of hours below set temperature required for autumn leafoff/hardening refers to the cumulative time that a plant species has been exposed to temperatures below a certain critical point. This is usually required for a plant to enter a dormant state (leaf off and hardening) in preparation for winter. It is a parameter used in plant phenology models to simulate the timing of seasonal events in plants, such as leaf fall in autumn." []
is_a: ECOSIM:CATEGORYCanopyStructure ! category - canopy structure
relationship: attribute ECOSIMCONCEPT:Temperature ! temperature

[Term]
id: ECOSIM:VRNY
name: initial heat requirement for spring leafout/dehardening
def: "The initial heat requirement for spring leafout/dehardening refers to the accumulated heat units (degree days) required by a plant to switch from winter dormancy to active growth in spring. This is an important parameter in plant phenology models and understanding the timing of spring leafout in relation to climate change." []
is_a: ECOSIM:CATEGORYCanopyStructure ! category - canopy structure
relationship: has_unit ECOSIM:h ! h
relationship: measured_in ECOSIMCONCEPT:Plants ! Plants
relationship: measurement_of ECOSIMCONCEPT:Leafout ! Leaf out

[Term]
id: ECOSIM:VRNZ
name: initial cold requirement for autumn leafoff/hardening
def: "VRNZ is a parameter in plant physiology representing the initial cold requirement for autumn leaf off or hardening. It refers to the amount of cold a plant needs to start the process of hardening or preparing for winter dormancy. This usually involves changes such as leaf drop, growth cessation, and alterations in biochemistry and physiology to increase cold tolerance. Hardening can be triggered by a combination of falling temperatures and shortening day length." []
is_a: ECOSIM:CATEGORYCanopyStructure ! category - canopy structure
is_a: ECOSIM:CATEGORYPlantPhysiology ! category - plant physiology
relationship: attribute ECOSIMCONCEPT:ColdRequirement ! Cold requirement
relationship: has_unit ECOSIM:h ! h
relationship: measured_in ECOSIMCONCEPT:Plant ! Plant

[Term]
id: ECOSIM:VSTG
name: leaf number
def: "Refer to the number of leaves in a plant or crop, which is a useful measurement for crop growth and development analysis." []
is_a: ECOSIM:CATEGORYCanopyStructure ! category - canopy structure
relationship: attribute ECOSIMCONCEPT:Number ! Number
relationship: measured_in ECOSIMCONCEPT:Plant ! Plant
relationship: measurement_of ECOSIMCONCEPT:LeafNumber ! LeafNumber

[Term]
id: ECOSIM:VSTGX
name: leaf number at floral initiation
def: "Number of leaves present on the plant at the time of floral initiation." []
is_a: ECOSIM:CATEGORYCanopyStructure ! category - canopy structure
is_a: ECOSIM:CATEGORYPlantPhysiology ! category - plant physiology
relationship: measured_in ECOSIMCONCEPT:Plant ! Plant
relationship: measurement_of ECOSIMCONCEPT:Leaf ! Leaf
relationship: measurement_of ECOSIMCONCEPT:LeafNumber ! LeafNumber

[Term]
id: ECOSIM:VWatLitRHoldCapcity
name: surface litter water holding capacity
is_a: ECOSIMCONCEPT:UnclassifiedVariable ! unclassified variable
relationship: has_unit ECOSIM:m3d-2 ! m3 d-2

[Term]
id: ECOSIM:VWatStoreCapSurf
name: surface water storage capacity
is_a: ECOSIMCONCEPT:UnclassifiedVariable ! unclassified variable
relationship: has_unit ECOSIM:m3d-2 ! m3 d-2

[Term]
id: ECOSIM:VapXAir2CanG
name: total canopy evaporation
def: "Total canopy evaporation (VapXAir2CanG) is the sum of all forms of evaporation from the canopy, including wet canopy evaporation (evaporation of intercept rainfall), cuticular transpiration (water vapor loss through plant leaf cuticle), and lenticular transpiration (evaporation from leaf surface through stomata or pores). It is a key element in the water cycle and influences the energy balance and climate of a region. Canopy evaporation can be influenced by factors like the type of vegetation, leaf surface characteristics, environmental conditions (temperature, humidity), and regional rainfall patterns." []
is_a: ECOSIMCONCEPT:UnclassifiedVariable ! unclassified variable
relationship: attribute ECOSIMCONCEPT:Evaporation ! Evaporation
relationship: has_unit ECOSIM:m3d-2 ! m3 d-2
relationship: measured_in ECOSIMCONCEPT:Canopy ! Canopy

[Term]
id: ECOSIM:VapXAir2GSurf
name: negative of total evaporation at ground surface
def: "Negative of total evaporation at ground surface refers to the negative amount of the total water evaporated from the ground surface, including water bodies, soil surface and plant surfaces. This value indicates the rate or speed at which water changes from a liquid to a gas or vapor state. This evaporation can occur due to solar radiation, wind, temperature, air pressure, and other environmental conditions." []
is_a: ECOSIM:CATEGORYHydrology ! category - Hydrology
is_a: ECOSIM:CATEGORYSurfaceEnergyBalance ! category - Surface Energy Balance
relationship: has_unit ECOSIM:m3d-2t-1 ! m3 d-2 t-1
relationship: measured_in ECOSIMCONCEPT:GroundSurface ! Ground surface
relationship: measurement_of ECOSIMCONCEPT:TotalEvaporation ! TotalEvaporation

[Term]
id: ECOSIM:VapXAir2PCan
name: negative of canopy evaporation
def: "Negative of canopy evaporation refers to the moisture loss from the aerial parts of the plants (leaves, stem, flowers, etc.), including the evaporation of water through stomata, a process known as transpiration, as well as evaporation from wet surfaces. It is a negative value because moisture is being lost from the system, reducing the overall water content." []
is_a: ECOSIMCONCEPT:UnclassifiedVariable ! unclassified variable
relationship: attribute ECOSIMCONCEPT:Evaporation ! Evaporation
relationship: has_unit ECOSIM:m2d-2h-1 ! m2 d-2 h-1
relationship: measured_in ECOSIMCONCEPT:Canopy ! Canopy

[Term]
id: ECOSIM:VaporDiffusivityLitR
name: water vapor diffusivity
def: "Water vapor diffusivity refers to the measure of the rate at which water vapor (the gaseous state of water) spreads or migrates in the atmosphere. It represents the ability of water vapor to mix and move within the air. Water vapor diffusivity is an important parameter in earth systems modeling as it plays a crucial role in understanding weather patterns, climate change, and the hydrological cycle." []
is_a: ECOSIMCONCEPT:UnclassifiedVariable ! unclassified variable
relationship: attribute ECOSIMCONCEPT:Diffusivity ! Diffusivity
relationship: has_unit ECOSIM:m2h-1 ! m2 h-1
relationship: measured_in ECOSIMCONCEPT:Atmosphere ! Atmosphere
relationship: measurement_of ECOSIMCONCEPT:WaterVapor ! Water vapor

[Term]
id: ECOSIM:VcumDrySnoWE
name: snow volume in snowpack (water equivalent)
def: "Snow volume in snowpack (water equivalent) refers to the volume of water that would result from melting a given volume of accumulated snow in a snowpack. It is commonly used in hydrology and climate studies to estimate available water resources and understand climate variability and trends. This measurement is typically expressed in millimeters (mm) of water equivalent and it reflects the density, depth and water content of the snowpack." []
is_a: ECOSIM:CATEGORYSnowpack ! category - Snowpack
relationship: attribute ECOSIMCONCEPT:Volume ! Volume
relationship: has_unit ECOSIM:m3d-2 ! m3 d-2
relationship: measured_in ECOSIMCONCEPT:Snowpack ! Snowpack
relationship: measurement_of ECOSIMCONCEPT:Water ! Water

[Term]
id: ECOSIM:VcumIceSnow
name: ice volume in snowpack
def: "Ice volume in snowpack refers to the total volume of ice present in a snowpack area. This can vary greatly due to factors such as temperature, precipitation, and the nature of the snowpack itself. Measuring this volume helps in understanding the water resource availability in high altitude regions, as this ice will eventually melt and provide water supply." []
is_a: ECOSIM:CATEGORYSnowpack ! category - Snowpack
is_a: ECOSIMCONCEPT:Snowpack ! Snowpack
relationship: attribute ECOSIMCONCEPT:Volume ! Volume
relationship: has_unit ECOSIM:m3d-2 ! m3 d-2
relationship: measured_in ECOSIMCONCEPT:Snowpack ! Snowpack

[Term]
id: ECOSIM:VcumSnoDWI
name: snowpack volume
def: "Snowpack volume refers to the total volume of water that would be released if all the snow in a given area was melted instantaneously. It represents a significant source of freshwater in many regions and plays a crucial role in the hydrological cycle. This parameter is typically expressed in units of water depth and is essential for monitoring and predicting changes in water resources." []
is_a: ECOSIM:CATEGORYSnowpack ! category - Snowpack
relationship: attribute ECOSIMCONCEPT:Volume ! Volume
relationship: has_unit ECOSIM:m3d-2 ! m3 d-2
relationship: measured_in ECOSIMCONCEPT:Area ! Area
relationship: measurement_of ECOSIMCONCEPT:Snow ! Snow

[Term]
id: ECOSIM:VcumWatSnow
name: water volume in snowpack
def: "The volume of water present in the snowpack, including both liquid water and ice." []
is_a: ECOSIM:CATEGORYSnowpack ! category - Snowpack
relationship: attribute ECOSIMCONCEPT:Volume ! Volume
relationship: has_unit ECOSIM:m3d-2 ! m3 d-2
relationship: measured_in ECOSIMCONCEPT:Snowpack ! Snowpack
relationship: measurement_of ECOSIMCONCEPT:Water ! Water

[Term]
id: ECOSIM:WDLF
name: leaf length:width ratio
def: "The leaf length to width ratio, often represented as WDLF, refers to the ratio of the length of a leaf to its width. It is an important measure in plant morphology helping to describe the shape of leaves, and can influence factors such as the leaf's exposure to light and its rate of water loss through transpiration." []
is_a: ECOSIM:CATEGORYCanopyPhysiology ! category - Canopy Physiology
is_a: ECOSIM:CATEGORYCanopyStructure ! category - canopy structure
is_a: ECOSIM:CATEGORYPlantPhysiology ! category - plant physiology
relationship: measurement_of ECOSIMCONCEPT:Leaf ! Leaf

[Term]
id: ECOSIM:WDNHB
name: width of NH4 band
def: "Width of NH4 band refers to the spatial extent or breadth of the distribution of ammonium (NH4) in a particular area or medium. It is a parameter often measured in soil or water systems to understand the dispersion and concentration of NH4. This information is important in various ecological or environmental contexts, including nutrient cycling, pollution monitoring, and the modeling of biogeochemical processes." []
is_a: ECOSIM:CATEGORYSoilBiogeochemistry ! category - Soil Biogeochemistry
is_a: ECOSIMCONCEPT:UnclassifiedVariable ! unclassified variable
relationship: attribute ECOSIMCONCEPT:Width ! Width
relationship: has_unit ECOSIM:m ! m
relationship: measured_in ECOSIMCONCEPT:Soil ! Soil
relationship: measurement_of ECOSIMCONCEPT:Ammonium ! Ammonium

[Term]
id: ECOSIM:WDNOB
name: width of NO3 band
is_a: ECOSIMCONCEPT:UnclassifiedVariable ! unclassified variable
relationship: attribute ECOSIMCONCEPT:Width ! Width
relationship: context ECOSIMCONCEPT:NO3 ! Nitrate
relationship: has_unit ECOSIM:m ! m
relationship: measured_in ECOSIMCONCEPT:Soil ! Soil

[Term]
id: ECOSIM:WDPOB
name: width of PO4 band
is_a: ECOSIMCONCEPT:UnclassifiedVariable ! unclassified variable
relationship: attribute ECOSIMCONCEPT:Width ! Width
relationship: has_unit ECOSIM:m ! m
relationship: measurement_of ECOSIMCONCEPT:PO4Band ! Phosphate band

[Term]
id: ECOSIM:WDPTH
name: depth of irrigation application
def: "Depth of irrigation application refers to the depth to which water is applied during irrigation. This is an important parameter in irrigation management, as it can influence the distribution of water and nutrients in the soil, crop water use efficiency, and ultimately, crop yield and quality. The depth of irrigation application can vary depending on factors such as the type of irrigation system used, crop type and growth stage, soil type, and weather conditions." []
is_a: ECOSIMCONCEPT:UnclassifiedVariable ! unclassified variable
relationship: attribute ECOSIMCONCEPT:Depth ! Depth
relationship: has_unit ECOSIM:m ! m
relationship: measured_in ECOSIMCONCEPT:Irrigation ! Irrigation

[Term]
id: ECOSIM:WDPTHD
name: real(r8),target,allocatable :: TDTPX(:,:,:)
is_a: ECOSIM:CATEGORYHydrology ! category - Hydrology
is_a: ECOSIMCONCEPT:UnclassifiedVariable ! unclassified variable
relationship: attribute ECOSIMCONCEPT:Duration ! Duration
relationship: measured_in ECOSIMCONCEPT:Water ! Water
relationship: measurement_of ECOSIMCONCEPT:Soil ! Soil

[Term]
id: ECOSIM:WFR
name: O2 constraint to root respiration
def: "The constraint of oxygen concentration to root respiration. This might be the case in waterlogged soils where oxygen availability can limit the respiration process." []
is_a: ECOSIM:CATEGORYPlantPhysiology ! category - plant physiology
is_a: ECOSIMCONCEPT:UnclassifiedVariable ! unclassified variable
relationship: attribute ECOSIMCONCEPT:Constraint ! Constraint
relationship: measured_in ECOSIMCONCEPT:Root ! Root
relationship: measurement_of ECOSIMCONCEPT:O2 ! Dioxygen

[Term]
id: ECOSIM:WGLFE
name: leaf element
def: "WGLFE refers to the weighted average of leaf element. It represents the average concentration of a particular element in the leaves of a plant, taking into account the relative proportion of each leaf. This is an important parameter in ecology and plant physiology, affecting plant nutrition, photosynthesis and growth." []
is_a: ECOSIM:CATEGORYPlantPhysiology ! category - plant physiology
is_a: ECOSIMCONCEPT:UnclassifiedVariable ! unclassified variable
relationship: has_unit ECOSIM:gd-2 ! g d-2
relationship: measurement_of ECOSIMCONCEPT:LeafElement ! Leaf element

[Term]
id: ECOSIM:WGLFEX
name: branch leaf structural element
is_a: ECOSIM:CATEGORYPlantPhysiology ! category - plant physiology
is_a: ECOSIMCONCEPT:UnclassifiedVariable ! unclassified variable
relationship: has_unit ECOSIM:gd-2 ! g d-2
relationship: measured_in ECOSIMCONCEPT:Branch ! Branch
relationship: measurement_of ECOSIMCONCEPT:LeafStructuralElement ! LeafStructuralElement

[Term]
id: ECOSIM:WGLFLE
name: layer leaf element
is_a: ECOSIMCONCEPT:UnclassifiedVariable ! unclassified variable
relationship: attribute ECOSIMCONCEPT:Element ! Element
relationship: has_unit ECOSIM:gd-2 ! g d-2
relationship: measured_in ECOSIMCONCEPT:Leaf ! Leaf
relationship: qualifier ECOSIMCONCEPT:Layer ! Layer

[Term]
id: ECOSIM:WGLFT
name: total leaf mass
def: "Total leaf mass refers to the cumulative mass of all leaves of a plant or vegetation system. It is an essential characteristic for studying the energy balance, carbon cycling and water cycle in vegetation ecosystems." []
is_a: ECOSIM:CATEGORYPlantPhysiology ! category - plant physiology
is_a: ECOSIMCONCEPT:UnclassifiedVariable ! unclassified variable
relationship: attribute ECOSIMCONCEPT:Mass ! Mass
relationship: has_unit ECOSIM:gd-2 ! g d-2
relationship: measured_in ECOSIMCONCEPT:Leaf ! Leaf

[Term]
id: ECOSIM:WGNODE
name: internode element
is_a: ECOSIMCONCEPT:UnclassifiedVariable ! unclassified variable
relationship: has_unit ECOSIM:gd-2 ! g d-2

[Term]
id: ECOSIM:WGSGA
name: water vapor diffusivity
def: "Water vapor diffusivity refers to the rate or speed at which water vapor molecules spread due to random motion. Higher diffusivity implies that the substance spreads out more quickly. It is important in understanding and modelling how moisture moves through the atmosphere, particularly in relation to weather patterns and climate models." []
is_a: ECOSIMCONCEPT:UnclassifiedVariable ! unclassified variable
relationship: attribute ECOSIMCONCEPT:Diffusivity ! Diffusivity
relationship: has_unit ECOSIM:m2h-1 ! m2 h-1
relationship: measured_in ECOSIMCONCEPT:Air ! Air
relationship: measurement_of ECOSIMCONCEPT:WaterVapor ! Water vapor

[Term]
id: ECOSIM:WGSGL
name: water vapor diffusivity
def: "Water vapor diffusivity refers to the measure of the rate at which water vapor migrates or spreads in a given medium. It represents the ability of water vapor to move and mix. This characteristic is important in atmospheric science as it can affect humidity, cloud formation, and other weather patterns." []
is_a: ECOSIMCONCEPT:UnclassifiedVariable ! unclassified variable
relationship: attribute ECOSIMCONCEPT:Diffusivity ! Diffusivity
relationship: has_unit ECOSIM:m2h-1 ! m2 h-1
relationship: measured_in ECOSIMCONCEPT:Air ! Air
relationship: measurement_of ECOSIMCONCEPT:WaterVapor ! Water vapor

[Term]
id: ECOSIM:WGSHE
name: sheath element
is_a: ECOSIMCONCEPT:UnclassifiedVariable ! unclassified variable
relationship: attribute ECOSIMCONCEPT:Element ! Element
relationship: has_unit ECOSIM:gd-2 ! g d-2
relationship: measured_in ECOSIMCONCEPT:Sheath ! Sheath

[Term]
id: ECOSIM:WGSHEXE
name: branch sheath structural element
is_a: ECOSIM:CATEGORYPlantPhysiology ! category - plant physiology
is_a: ECOSIMCONCEPT:UnclassifiedVariable ! unclassified variable
relationship: has_unit ECOSIM:gd-2 ! g d-2
relationship: measured_in ECOSIMCONCEPT:Branch ! Branch
relationship: measurement_of ECOSIMCONCEPT:Sheath ! Sheath

[Term]
id: ECOSIM:WQRH
name: runoff from surface water
def: "Runoff from surface water refers to the water that flows off the surface of the land - including fields, forest floors, city streets, and lawns, etc. - without sinking into the ground. It's a key component in the hydrological cycle, contributing significantly to the overall water resources in an area. Monitoring runoff is crucial for various environmental assessments and management practices, including flood forecasting, water supply planning, and water quality management." []
is_a: ECOSIM:CATEGORYHydrology ! category - Hydrology
relationship: attribute ECOSIMCONCEPT:Runoff ! Runoff
relationship: has_unit ECOSIM:m3d-2h-1 ! m3 d-2 h-1
relationship: measured_in ECOSIMCONCEPT:SurfaceWater ! Surface water

[Term]
id: ECOSIM:WSLF
name: layer leaf protein C
def: "Layer leaf protein C refers to the part of a plant leaf structure that contains the protein carbon. It is usually a parameter in biology and earth sciences to measure the amount of carbon in the protein of leaves in specific layers. This could give an insight into the photosynthesis rate and other plant physiological processes." []
is_a: ECOSIMCONCEPT:UnclassifiedVariable ! unclassified variable
relationship: has_unit ECOSIM:gd-2 ! g d-2
relationship: measurement_of ECOSIMCONCEPT:ProteinCarbon ! ProteinCarbon

[Term]
id: ECOSIM:WSRTL
name: root layer protein C
is_a: ECOSIM:CATEGORYRootPhysiology ! category - root physiology
is_a: ECOSIMCONCEPT:UnclassifiedVariable ! unclassified variable
relationship: has_unit ECOSIM:gd-2 ! g d-2
relationship: measured_in ECOSIMCONCEPT:RootLayer ! Root layer
relationship: measurement_of ECOSIMCONCEPT:Carbon ! Carbon

[Term]
id: ECOSIM:WSSHE
name: layer sheath protein C
def: "Layer sheath protein C refers to a type of sheath protein found in the outer layer of specific types of bacteria. It is involved in the formation of the bacterial sheath, which is an extracellular matrix that protects the bacteria and aids in adhesion to surfaces. The concentration of layer sheath protein C can be a measure of bacterial activity and health." []
is_a: ECOSIMCONCEPT:UnclassifiedVariable ! unclassified variable
relationship: attribute ECOSIMCONCEPT:Concentration ! Concentration
relationship: has_unit ECOSIM:gd-2 ! g d-2
relationship: measured_in ECOSIMCONCEPT:Bacteria ! Bacteria
relationship: measurement_of ECOSIMCONCEPT:SheathProteinC ! Sheath protein carbon

[Term]
id: ECOSIM:WSTR
name: canopy plant water stress indicator, number of hours PSILT < PSILY
def: "An indicator of water stress in the canopy of a plant, measured by the number of hours that the PSILT (plant's soil moisture level) is less than the PSILY (plant's leaf water potential)" []
is_a: ECOSIM:CATEGORYCanopyStructure ! category - canopy structure
is_a: ECOSIM:CATEGORYPlantPhysiology ! category - plant physiology
is_a: ECOSIM:CATEGORYPlantPopulation ! category - Plant Population
relationship: attribute ECOSIMCONCEPT:StressIndicator ! Stress indicator
relationship: measurement_of ECOSIMCONCEPT:PlantWaterStress ! PlantWaterStress

[Term]
id: ECOSIM:WTEARBE
name: branch ear element
def: "Branch ear element refers to a conceptual model parameter used to represent the concentration or amount of a specific element, such as carbon or nitrogen, in the ear of a branched plant structure. This parameter can be instrumental in plant growth modelling, where it is used to simulate nutrient uptake and allocation in various plant parts." []
is_a: ECOSIM:CATEGORYPlantPhysiology ! category - plant physiology
is_a: ECOSIMCONCEPT:UnclassifiedVariable ! unclassified variable
relationship: has_unit ECOSIM:gd-2 ! g d-2
relationship: measured_in ECOSIMCONCEPT:Ear ! Ear
relationship: measurement_of ECOSIMCONCEPT:Element ! Element

[Term]
id: ECOSIM:WTEARE
name: canopy ear element
is_a: ECOSIM:CATEGORYPlantPhysiology ! category - plant physiology
is_a: ECOSIMCONCEPT:UnclassifiedVariable ! unclassified variable
relationship: attribute ECOSIMCONCEPT:Element ! Element
relationship: has_unit ECOSIM:gd-2 ! g d-2
relationship: measured_in ECOSIMCONCEPT:Canopy ! Canopy
relationship: measurement_of ECOSIMCONCEPT:Ear ! Ear

[Term]
id: ECOSIM:WTGRBE
name: branch grain element
def: "The weight of a grain element on a branch is used in models that simulate the growth and development of grains on a plant." []
is_a: ECOSIM:CATEGORYPlantPhysiology ! category - plant physiology
is_a: ECOSIMCONCEPT:UnclassifiedVariable ! unclassified variable
relationship: has_unit ECOSIM:gd-2 ! g d-2
relationship: measured_in ECOSIMCONCEPT:Branch ! Branch
relationship: measured_in ECOSIMCONCEPT:GrainElement ! GrainElement
relationship: measurement_of ECOSIMCONCEPT:Grain ! Grain

[Term]
id: ECOSIM:WTGRE
name: canopy grain element
def: "Canopy grain element refers to a specific portion or element of the grain produced by crops in the plant canopy. This concept is used in earth system modeling to understand the growth, development and productivity of crops." []
is_a: ECOSIM:CATEGORYPlantPhysiology ! category - plant physiology
is_a: ECOSIMCONCEPT:UnclassifiedVariable ! unclassified variable
relationship: attribute ECOSIMCONCEPT:GrainElement ! GrainElement
relationship: has_unit ECOSIM:gd-2 ! g d-2
relationship: measured_in ECOSIMCONCEPT:Canopy ! Canopy

[Term]
id: ECOSIM:WTHSKBE
name: branch husk element
def: "WTHSKBE represents the weight of husk elements in branches in a selected area. It is critical for understanding ecological cycles like carbon and nutrient cycling, as different components of a plant have distinct decomposition rates and nutrient contents." []
is_a: ECOSIMCONCEPT:UnclassifiedVariable ! unclassified variable
relationship: has_unit ECOSIM:gd-2 ! g d-2
relationship: measured_in ECOSIMCONCEPT:Branch ! Branch
relationship: measurement_of ECOSIMCONCEPT:HuskElement ! HuskElement

[Term]
id: ECOSIM:WTHSKE
name: canopy husk element
def: "This parameter represents the amount of elemental content in husk components of the plant canopy." []
is_a: ECOSIM:CATEGORYPlantPhysiology ! category - plant physiology
is_a: ECOSIMCONCEPT:UnclassifiedVariable ! unclassified variable
relationship: attribute ECOSIMCONCEPT:Element ! Element
relationship: has_unit ECOSIM:gd-2 ! g d-2
relationship: measured_in ECOSIMCONCEPT:Canopy ! Canopy
relationship: measurement_of ECOSIMCONCEPT:Husk ! Husk

[Term]
id: ECOSIM:WTLFBE
name: branch leaf element
def: "Branch leaf element refers to the elemental components (such as carbon, nitrogen, etc.) present in the leaves on a tree's branches. This is an important aspect of understanding a tree's chemical composition and its role in the ecosystem, as these elements are part of various biogeochemical processes." []
is_a: ECOSIM:CATEGORYPlantPhysiology ! category - plant physiology
is_a: ECOSIMCONCEPT:UnclassifiedVariable ! unclassified variable
relationship: attribute ECOSIMCONCEPT:Element ! Element
relationship: has_unit ECOSIM:gd-2 ! g d-2
relationship: measured_in ECOSIMCONCEPT:BranchLeaf ! BranchLeaf

[Term]
id: ECOSIM:WTLFE
name: canopy leaf element
is_a: ECOSIM:CATEGORYPlantPhysiology ! category - plant physiology
is_a: ECOSIMCONCEPT:UnclassifiedVariable ! unclassified variable
relationship: attribute ECOSIMCONCEPT:Element ! Element
relationship: has_unit ECOSIM:gd-2 ! g d-2
relationship: measured_in ECOSIMCONCEPT:Canopy ! Canopy
relationship: measurement_of ECOSIMCONCEPT:Leaf ! Leaf

[Term]
id: ECOSIM:WTNDBE
name: branch nodule element
def: "Branch nodule element refers to a specific part or component of a branch nodule. A branch nodule is a small swelling or growth that develops on a branch. These nodules can fulfill various functions, depending on the plant species, including storing nutrients, housing symbiotic microorganisms, or as dormant buds ready for sprouting. These elements can be used to assess the health and nutrient content of the plant." []
is_a: ECOSIMCONCEPT:UnclassifiedVariable ! unclassified variable
relationship: has_unit ECOSIM:gd-2 ! g d-2

[Term]
id: ECOSIM:WTNDE
name: root total nodule mass
def: "Root total nodule mass refers to the total mass of the nodules that are present in the roots of a plant. Nodules contain bacteria that convert nitrogen in the air into a form that can be used by the plant, a process known as nitrogen fixation. Thus, the total nodule mass can indicate the capacity of a plant to fix nitrogen." []
is_a: ECOSIM:CATEGORYPlantPhysiology ! category - plant physiology
is_a: ECOSIMCONCEPT:UnclassifiedVariable ! unclassified variable
relationship: attribute ECOSIMCONCEPT:Mass ! Mass
relationship: has_unit ECOSIM:gd-2 ! g d-2
relationship: measured_in ECOSIMCONCEPT:Root ! Root
relationship: measurement_of ECOSIMCONCEPT:Nodule ! Nodule

[Term]
id: ECOSIM:WTNDLE
name: root layer nodule element
def: "Root layer nodule element refers to the mineral content in the root nodules of plants. These nodules, which are formed in a mutualistic relationship between certain plants and bacteria, play an essential role in the nitrogen cycle by housing bacteria that can convert atmospheric nitrogen into a form that can be used by plants." []
is_a: ECOSIM:CATEGORYRootPhysiology ! category - root physiology
is_a: ECOSIMCONCEPT:UnclassifiedVariable ! unclassified variable
relationship: attribute ECOSIMCONCEPT:Element ! Element
relationship: has_unit ECOSIM:gd-2 ! g d-2
relationship: measured_in ECOSIMCONCEPT:RootLayer ! Root layer
relationship: measured_in ECOSIMCONCEPT:RootNodule ! Root nodule

[Term]
id: ECOSIM:WTRSVBE
name: branch reserve element
is_a: ECOSIMCONCEPT:UnclassifiedVariable ! unclassified variable
relationship: attribute ECOSIMCONCEPT:Reserve ! Reserve
relationship: has_unit ECOSIM:gd-2 ! g d-2
relationship: measured_in ECOSIMCONCEPT:Branch ! Branch
relationship: measurement_of ECOSIMCONCEPT:Element ! Element

[Term]
id: ECOSIM:WTRSVE
name: canopy reserve element
is_a: ECOSIM:CATEGORYPlantPhysiology ! category - plant physiology
is_a: ECOSIMCONCEPT:UnclassifiedVariable ! unclassified variable
relationship: has_unit ECOSIM:gd-2 ! g d-2
relationship: measured_in ECOSIMCONCEPT:Canopy ! Canopy
relationship: measurement_of ECOSIMCONCEPT:ReserveElement ! Reserve element

[Term]
id: ECOSIM:WTRT1E
name: root layer element primary axes
def: "Root layer element primary axes refers to the main or principal axes of elements (parts or sections) within the root layer." []
is_a: ECOSIM:CATEGORYRootPhysiology ! category - root physiology
is_a: ECOSIMCONCEPT:UnclassifiedVariable ! unclassified variable
relationship: has_unit ECOSIM:gd-2 ! g d-2
relationship: measured_in ECOSIMCONCEPT:RootLayer ! Root layer

[Term]
id: ECOSIM:WTRT2E
name: root layer element secondary axes
def: "The secondary axes of an element in the root layer." []
is_a: ECOSIM:CATEGORYRootPhysiology ! category - root physiology
is_a: ECOSIMCONCEPT:UnclassifiedVariable ! unclassified variable
relationship: has_unit ECOSIM:gd-2 ! g d-2
relationship: measured_in ECOSIMCONCEPT:RootLayer ! Root layer
relationship: measurement_of ECOSIMCONCEPT:SecondaryAxes ! SecondaryAxes

[Term]
id: ECOSIM:WTRTA
name: root C per plant
is_a: ECOSIMCONCEPT:UnclassifiedVariable ! unclassified variable
relationship: has_unit ECOSIM:gp-1 ! g p-1
relationship: measured_in ECOSIMCONCEPT:Plant ! Plant
relationship: measured_in ECOSIMCONCEPT:Root ! Root
relationship: measurement_of ECOSIMCONCEPT:Carbon ! Carbon

[Term]
id: ECOSIM:WTRTE
name: plant root element
def: "Plant root element refers to any chemical element found in the roots of a plant. These elements play a crucial role in plant growth and nutrition, as well as in soil fertility and the wider ecosystem." []
is_a: ECOSIM:CATEGORYRootPhysiology ! category - root physiology
is_a: ECOSIMCONCEPT:UnclassifiedVariable ! unclassified variable
relationship: attribute ECOSIMCONCEPT:Element ! Element
relationship: has_unit ECOSIM:gd-2 ! g d-2
relationship: measured_in ECOSIMCONCEPT:Root ! Root

[Term]
id: ECOSIM:WTRTL
name: root layer structural C
def: "Root layer structural C is the amount of carbon found in the structural components of the root layer of plants. The structural components of the plants are responsible for the growth and development of the plant. Understanding the amount of structural carbon in roots can provide insights into the plant's health and productivity." []
is_a: ECOSIM:CATEGORYRootPhysiology ! category - root physiology
is_a: ECOSIMCONCEPT:UnclassifiedVariable ! unclassified variable
relationship: attribute ECOSIMCONCEPT:Structure ! Structure
relationship: has_unit ECOSIM:gd-2 ! g d-2
relationship: measured_in ECOSIMCONCEPT:RootLayer ! Root layer

[Term]
id: ECOSIM:WTRTSE
name: plant root structural element
def: "Plant root structural element refers to the features that comprise the structure of a plant's roots, including the root hairs, root tip, and root cap. These elements are crucial for nutrient absorption, water uptake, and structural support." []
is_a: ECOSIM:CATEGORYRootPhysiology ! category - root physiology
is_a: ECOSIMCONCEPT:UnclassifiedVariable ! unclassified variable
relationship: has_unit ECOSIM:gd-2 ! g d-2
relationship: measured_in ECOSIMCONCEPT:Root ! Root

[Term]
id: ECOSIM:WTRVE
name: plant stored nonstructural element
def: "Stored nonstructural element refers to elements stored in various parts of plants that do not form a part of the primary structure of the plant. These include elements found in starch, sugars, and fats, and are stored in roots, stems, leaves, seeds, and fruits. These stored elements provide energy for plant growth and metabolic activities." []
is_a: ECOSIM:CATEGORYPlantPhysiology ! category - plant physiology
is_a: ECOSIMCONCEPT:UnclassifiedVariable ! unclassified variable
relationship: has_unit ECOSIM:gd-2 ! g d-2
relationship: measured_in ECOSIMCONCEPT:Plant ! Plant
relationship: measurement_of ECOSIMCONCEPT:Element ! Element

[Term]
id: ECOSIM:WTRVX
name: plant stored nonstructural C at planting
def: "Plant stored nonstructural C at planting refers to the amount of nonstructural carbohydrates, especially in the form of carbon, that a plant has stored at the time of planting. These stored carbohydrates are crucial for the early growth and development of the plant, providing it with a source of energy until it is able to produce its own food through photosynthesis." []
is_a: ECOSIM:CATEGORYPlantPhysiology ! category - plant physiology
is_a: ECOSIMCONCEPT:UnclassifiedVariable ! unclassified variable
relationship: has_unit ECOSIM:gd-2 ! g d-2
relationship: measured_in ECOSIMCONCEPT:Plant ! Plant
relationship: measurement_of ECOSIMCONCEPT:NonstructuralOrganicCompounds ! NonstructuralOrganicCompounds

[Term]
id: ECOSIM:WTSHEBE
name: branch sheath element
def: "Branch sheath element refers to a particular element or component of the sheath that surrounds a branch in a plant. This could be a reference to a specific chemical or cellular component, or a characteristic trait of the sheath. In a broader framework, this parameter can be related to various aspects of plant morphology and physiology, as well as biogeochemical cycling in ecosystems." []
is_a: ECOSIM:CATEGORYPlantPhysiology ! category - plant physiology
is_a: ECOSIMCONCEPT:UnclassifiedVariable ! unclassified variable
relationship: attribute ECOSIMCONCEPT:Element ! Element
relationship: has_unit ECOSIM:gd-2 ! g d-2
relationship: measured_in ECOSIMCONCEPT:BranchSheath ! BranchSheath

[Term]
id: ECOSIM:WTSHEE
name: canopy sheath element
is_a: ECOSIM:CATEGORYPlantPhysiology ! category - plant physiology
is_a: ECOSIMCONCEPT:UnclassifiedVariable ! unclassified variable
relationship: attribute ECOSIMCONCEPT:Element ! Element
relationship: has_unit ECOSIM:gd-2 ! g d-2
relationship: measured_in ECOSIMCONCEPT:Canopy ! Canopy
relationship: measurement_of ECOSIMCONCEPT:Sheath ! Sheath

[Term]
id: ECOSIM:WTSHTA
name: landscape average canopy shoot C
def: "The landscape average canopy shoot C refers to the average amount of carbon contained in the shoots of plants across a certain landscape. This is influenced by factors such as plant species, growth stage, and environmental conditions, and is a key parameter for understanding the carbon cycle in terrestrial ecosystems." []
is_a: ECOSIMCONCEPT:UnclassifiedVariable ! unclassified variable
relationship: context ECOSIMCONCEPT:Landscape ! Landscape
relationship: has_unit ECOSIM:gd-2 ! g d-2
relationship: measured_in ECOSIMCONCEPT:CanopyShoot ! CanopyShoot
relationship: measurement_of ECOSIMCONCEPT:Carbon ! Carbon

[Term]
id: ECOSIM:WTSHTBE
name: branch shoot C
def: "Branch shoot C refers to the amount of carbon stored in the branches and shoots of a plant or tree. This is an important measure in studies of carbon sequestration and the carbon cycle, as plants and trees play a vital role in absorbing CO2 from the atmosphere." []
is_a: ECOSIMCONCEPT:UnclassifiedVariable ! unclassified variable
relationship: has_unit ECOSIM:gd-2 ! g d-2
relationship: measured_in ECOSIMCONCEPT:BranchShoot ! Branch shoot
relationship: measurement_of ECOSIMCONCEPT:Carbon ! Carbon

[Term]
id: ECOSIM:WTSTDE
name: standing dead element fraction
is_a: ECOSIM:CATEGORYPlantPhysiology ! category - plant physiology
is_a: ECOSIMCONCEPT:UnclassifiedVariable ! unclassified variable
relationship: attribute ECOSIMCONCEPT:Fraction ! Fraction
relationship: has_unit ECOSIM:gd-2 ! g d-2
relationship: measured_in ECOSIMCONCEPT:StandingDead ! Standing dead
relationship: measurement_of ECOSIMCONCEPT:Element ! Element

[Term]
id: ECOSIM:WTSTDI
name: initial standing dead C
def: "Initial standing dead C refers to the initial amount of carbon contained in dead standing trees in a particular area at the commencement of observation or a study period. This is an important initial condition for earth systems modeling and helps in tracking changes in carbon pools in forest ecosystems over time." []
is_a: ECOSIM:CATEGORYCanopyStructure ! category - canopy structure
relationship: has_unit ECOSIM:gCm-2 ! g C m-2
relationship: measured_in ECOSIMCONCEPT:DeadStandingTree ! DeadStandingTree
relationship: measurement_of ECOSIMCONCEPT:Carbon ! Carbon

[Term]
id: ECOSIM:WTSTGE
name: standing dead element
def: "Standing dead element refers to the elements present in dead standing trees. These elements can range from carbon, nitrogen and other nutrients. The standing dead element contributes to nutrient cycling and carbon storage in forest ecosystems." []
is_a: ECOSIMCONCEPT:UnclassifiedVariable ! unclassified variable
relationship: has_unit ECOSIM:gd-2 ! g d-2
relationship: measured_in ECOSIMCONCEPT:DeadStandingTree ! DeadStandingTree

[Term]
id: ECOSIM:WTSTGET
name: total standing dead C
def: "Total standing dead C refers to the total amount of carbon contained in dead standing trees in a particular area. This can vary based on factors such as forest type, tree species, and disturbance history. It represents a significant pool of carbon in forest ecosystems, and is important for understanding the carbon cycle and the role of forests in climate change." []
is_a: ECOSIM:CATEGORYTraceGasFlux ! category - trace gas flux
relationship: has_unit ECOSIM:gd-2 ! g d-2
relationship: measured_in ECOSIMCONCEPT:DeadStandingTree ! DeadStandingTree
relationship: measurement_of ECOSIMCONCEPT:Carbon ! Carbon

[Term]
id: ECOSIM:WTSTKBE
name: branch stalk element
def: "Branch stalk element refers to the amount of a specific chemical element contained in branch stalks of a plant. The exact element and its amount can vary greatly depending on factors such as the plant species, growth conditions, and the nature of the soil in which the plant is grown. Studying the elemental composition of plants can help in understanding the nutrient cycling within ecosystems, and can assist in the development of strategies for sustainable agriculture." []
is_a: ECOSIMCONCEPT:UnclassifiedVariable ! unclassified variable
relationship: has_unit ECOSIM:gd-2 ! g d-2
relationship: measured_in ECOSIMCONCEPT:BranchStalk ! BranchStalk
relationship: measurement_of ECOSIMCONCEPT:SpecificChemicalElement ! SpecificChemicalElement

[Term]
id: ECOSIM:WTSTKE
name: canopy stalk element
is_a: ECOSIM:CATEGORYPlantPhysiology ! category - plant physiology
is_a: ECOSIMCONCEPT:UnclassifiedVariable ! unclassified variable
relationship: attribute ECOSIMCONCEPT:Element ! Element
relationship: has_unit ECOSIM:gd-2 ! g d-2
relationship: measured_in ECOSIMCONCEPT:Canopy ! Canopy
relationship: measurement_of ECOSIMCONCEPT:Stalk ! Stalk

[Term]
id: ECOSIM:WTSTXBE
name: branch stalk structural C
def: "Branch stalk structural C refers to the amount of structural carbon in the branch stalk of plants. Structural carbon forms the basic structural components of plant tissues such as cellulose and lignin. It is crucial for the strength and rigidity of plant structures including the branch stalk. It is an important parameter for understanding plant physiology and contributions to the carbon cycle." []
is_a: ECOSIM:CATEGORYPlantPhysiology ! category - plant physiology
is_a: ECOSIMCONCEPT:UnclassifiedVariable ! unclassified variable
relationship: has_unit ECOSIM:gd-2 ! g d-2
relationship: measured_in ECOSIMCONCEPT:BranchStalk ! BranchStalk
relationship: measurement_of ECOSIMCONCEPT:StructuralCarbon ! StructuralCarbon

[Term]
id: ECOSIM:Wat2GridBySurfRunoff
name: soil surface runoff water
is_a: ECOSIMCONCEPT:UnclassifiedVariable ! unclassified variable
relationship: has_unit ECOSIM:m3d-2h-1 ! m3 d-2 h-1

[Term]
id: ECOSIM:WatByPCan
name: canopy held water content
def: "Canopy held water content refers to the amount of water that is intercepted by the canopy of trees and plants. This water is typically held on the surface of leaves, branches, and other plant structures. Canopy held water content is a key component of the hydrological cycle because it has direct impacts on processes such as evaporation, transpiration, and runoff." []
is_a: ECOSIM:CATEGORYHydrology ! category - Hydrology
is_a: ECOSIMCONCEPT:UnclassifiedVariable ! unclassified variable
relationship: attribute ECOSIMCONCEPT:Content ! Content
relationship: has_unit ECOSIM:m3d-2 ! m3 d-2
relationship: measured_in ECOSIMCONCEPT:Canopy ! Canopy
relationship: measurement_of ECOSIMCONCEPT:Water ! Water

[Term]
id: ECOSIM:WatBySnowRedistribution
name: snowpack runoff water
is_a: ECOSIM:CATEGORYSnowpack ! category - Snowpack
relationship: has_unit ECOSIM:m3d-2h-1 ! m3 d-2 h-1

[Term]
id: ECOSIM:WatFLo2Litr
name: net water transfer to surface litter
def: "Net water transfer to surface litter refers to the total amount of water that is transferred to the surface litter layer of an ecosystem from other parts of the ecosystem, over a given period of time. The surface litter layer, which is made up of decomposing organic matter such as dead leaves, grasses, and other plant materials, plays a crucial role in the hydrological cycle of the ecosystem. This process is an essential aspect of water cycle in ecosystems, influencing soil moisture levels, nutrient cycling, and the overall health and functioning of the ecosystem." []
is_a: ECOSIM:CATEGORYHydrology ! category - Hydrology
is_a: ECOSIMCONCEPT:UnclassifiedVariable ! unclassified variable
relationship: has_unit ECOSIM:MJd-2t-1 ! MJ d-2 t-1
relationship: measured_in ECOSIMCONCEPT:Litter ! Litter
relationship: measurement_of ECOSIMCONCEPT:Water ! Water
relationship: qualifier ECOSIMCONCEPT:Surface ! Surface

[Term]
id: ECOSIM:WatFLo2LitrM
name: water transfer between soil surface and surface litter
def: "Water transfer between soil surface and surface litter this variable represents the movement of water between the soil surface and the surface litter, or organic material, that covers the soil. This exchange of water can occur through various processes, including direct contact, capillary action, and gravitational movement. The amount and rate of water transfer can vary depending on factors such as soil properties, litter characteristics, and environmental conditions. Understanding this water exchange is important for modeling and simulating soil hydrology, soil moisture dynamics, and overall ecosystem functioning." []
is_a: ECOSIM:CATEGORYHydrology ! category - Hydrology
is_a: ECOSIMCONCEPT:UnclassifiedVariable ! unclassified variable
relationship: has_unit ECOSIM:gd-2t-1 ! g d-2 t-1
relationship: measured_in ECOSIMCONCEPT:SoilSurface ! Soil surface
relationship: measured_in ECOSIMCONCEPT:SurfaceLitter ! Surface litter
relationship: measurement_of ECOSIMCONCEPT:Water ! Water

[Term]
id: ECOSIM:WatFlowSno2LitRM
name: meltwater flux into surface litter
is_a: ECOSIMCONCEPT:UnclassifiedVariable ! unclassified variable
relationship: has_unit ECOSIM:m3d-2h-1 ! m3 d-2 h-1

[Term]
id: ECOSIM:WatFlux4ErosionM
name: runoff water flux
def: "WatFlux4ErosionM, or runoff water flux, is the volume of water available for soil erosion due to the force of raindrop impact and the flow of surface water. This measure is crucial in understanding soil erosion rates, soil stability, and landscape evolution and informs our ability to develop successful soil conservation strategies." []
is_a: ECOSIM:CATEGORYHydrology ! category - Hydrology
is_a: ECOSIMCONCEPT:UnclassifiedVariable ! unclassified variable
relationship: attribute ECOSIMCONCEPT:Flux ! Flux
relationship: context ECOSIMCONCEPT:Runoff ! Runoff
relationship: has_unit ECOSIM:m3d-2t-1 ! m3 d-2 t-1
relationship: measurement_of ECOSIMCONCEPT:Water ! Water

[Term]
id: ECOSIM:WaterFlow2MacPM
name: macropore water flux
is_a: ECOSIMCONCEPT:UnclassifiedVariable ! unclassified variable
relationship: has_unit ECOSIM:m3d-2t-1 ! m3 d-2 t-1

[Term]
id: ECOSIM:WaterFlow2MicPM
name: micropore water flux
is_a: ECOSIMCONCEPT:UnclassifiedVariable ! unclassified variable
relationship: has_unit ECOSIM:m3d-2t-1 ! m3 d-2 t-1

[Term]
id: ECOSIM:WaterFlowMacP
name: water flux macropore
is_a: ECOSIMCONCEPT:UnclassifiedVariable ! unclassified variable
relationship: has_unit ECOSIM:m3d-2h-1 ! m3 d-2 h-1

[Term]
id: ECOSIM:WaterFlowSoiMicP
name: water flux micropore
def: "The flow of water through the micropores in the soil. This is one of the main processes through which water moves downwards from the surface to deeper levels in the soil, besides macropore flow. Micropores typically have a diameter less than 0.08 mm and are responsible for the soil's water holding capacity and the flow of water and nutrients towards plant roots. They can be found between clay particles and organic matter, and their presence improves soil structure and fertility." []
is_a: ECOSIM:CATEGORYHydrology ! category - Hydrology
is_a: ECOSIMCONCEPT:UnclassifiedVariable ! unclassified variable
relationship: attribute ECOSIMCONCEPT:Micropore ! Micropore
relationship: has_unit ECOSIM:m3d-2h-1 ! m3 d-2 h-1
relationship: measured_in ECOSIMCONCEPT:Soil ! Soil
relationship: measurement_of ECOSIMCONCEPT:Water ! Water

[Term]
id: ECOSIM:WaterFlowSoiMicPX
name: unsaturated water flux
def: "Unsaturated water flux refers to the movement of water through the unsaturated zone of the soil, which is the layer above the water table where some spaces within the soil structure are filled with air rather than water. It is an important process in hydrology and soil science as it influences soil moisture dynamics, nutrient transport, and groundwater recharge." []
is_a: ECOSIM:CATEGORYHydrology ! category - Hydrology
is_a: ECOSIMCONCEPT:UnclassifiedVariable ! unclassified variable
relationship: attribute ECOSIMCONCEPT:Flux ! Flux
relationship: has_unit ECOSIM:m3d-2h-1 ! m3 d-2 h-1
relationship: measured_in ECOSIMCONCEPT:Soil ! Soil

[Term]
id: ECOSIM:WaterTBLSlope
name: slope of water table relative to surface slope
def: "WaterTBLSlope refers to the angle of the water table in relation to the surface slope. It is an important measurement in hydrology as it can significantly impact the flow of groundwater, the saturation of soils, and ultimately the distribution of water in a landscape." []
is_a: ECOSIM:CATEGORYHydrology ! category - Hydrology
is_a: ECOSIMCONCEPT:UnclassifiedVariable ! unclassified variable
relationship: attribute ECOSIMCONCEPT:Slope ! Slope
relationship: context ECOSIMCONCEPT:Surface ! Surface
relationship: measured_in ECOSIMCONCEPT:WaterTable ! WaterTable

[Term]
id: ECOSIM:WindMesHeight
name: wind speed measurement height
is_a: ECOSIMCONCEPT:UnclassifiedVariable ! unclassified variable
relationship: has_unit ECOSIM:m ! m

[Term]
id: ECOSIM:WindSpeedAtm
name: wind speed
def: "Wind speed is a fundamental atmospheric quantity. It is the speed at which air is moving horizontally relative to the surface of the earth. Wind speed is measured in various units of speed, such as meters per second or kilometers per hour. It is an essential parameter in understanding atmospheric dynamics, weather forecasting, and in many environmental and engineering applications." []
is_a: ECOSIM:CATEGORYAtmosphericConditions ! category - Atmospheric Conditions
relationship: attribute ECOSIMCONCEPT:Speed ! Speed
relationship: has_unit ECOSIM:mh-1 ! m h-1
relationship: measurement_of ECOSIMCONCEPT:Wind ! Wind

[Term]
id: ECOSIM:Wm-2
name: W m-2
def: "Watt per square meter (W/m²) is a unit of power flux density, representing energy transfer rate per unit area in the International System of Units (SI). It is commonly used in meteorology, to denote the intensity of solar radiation, infrared radiation or luminous flux." []
is_a: ECOSIMCONCEPT:Unit ! unit
relationship: attribute ECOSIMCONCEPT:PowerFluxDensity ! Power flux density

[Term]
id: ECOSIM:XAL1BS
name: wet deposition of AlOH
def: "A process in which AlOH (aluminium hydroxide) from the atmosphere is dissolved into precipitation, such as rain or snow, then carried to the Earth's surface. It plays a significant role in the Earth's chemical balance." []
is_a: ECOSIM:CATEGORYDepositionFlux ! category - deposition flux
relationship: has_unit ECOSIM:gd-2h-1 ! g d-2 h-1
relationship: measurement_of ECOSIMCONCEPT:AlOH ! Aluminum hydroxide

[Term]
id: ECOSIM:XAL2BS
name: wet deposition of AlOH2
def: "Wet deposition of AlOH2 refers to the process by which aluminum hydroxide (AlOH2) particles present in the atmosphere are carried to the Earth's surface with precipitation, such as rain or snow. The quantity of AlOH2 deposited can be influenced by various factors including precipitation intensity, wind speed, particle size, and atmospheric concentration of AlOH2. It is an important parameter in Earth system modeling as it affects the chemistry of the boundary layer and can influence various ecological processes in terrestrial and aquatic ecosystems." []
is_a: ECOSIM:CATEGORYDepositionFlux ! category - deposition flux
relationship: attribute ECOSIMCONCEPT:Deposition ! Deposition
relationship: context ECOSIMCONCEPT:Precipitation ! Precipitation
relationship: has_unit ECOSIM:gd-2h-1 ! g d-2 h-1
relationship: measurement_of ECOSIMCONCEPT:AlOH2 ! Aluminum dihydroxide

[Term]
id: ECOSIM:XAL3BS
name: wet deposition of AlOH3
def: "A process in which AlOH3 (Aluminium hydroxide) from the atmosphere is dissolved into precipitation, such as rain or snow, then carried to the Earth's surface. It is an important process in the Earth's aluminium cycle." []
is_a: ECOSIM:CATEGORYDepositionFlux ! category - deposition flux
relationship: has_unit ECOSIM:gd-2h-1 ! g d-2 h-1
relationship: measurement_of ECOSIMCONCEPT:AlOH3 ! Aluminum trihydroxide

[Term]
id: ECOSIM:XAL4BS
name: wet deposition of AlOH4
def: "The process in which Aluminum hydroxide ions (AlOH4) from the atmosphere are dissolved into precipitation, such as rain or snowmelt, then carried to the Earth's surface. It is an important process in understanding hydrogeochemical cycling and deposition." []
is_a: ECOSIM:CATEGORYDepositionFlux ! category - deposition flux
relationship: has_unit ECOSIM:gd-2h-1 ! g d-2 h-1
relationship: measurement_of ECOSIMCONCEPT:AlOH4 ! Aluminum tetrahydroxide

[Term]
id: ECOSIM:XALBLS
name: wet deposition of Al
def: "The process of deposition of aluminum (Al) from the atmosphere onto the earth's surface during precipitation events such as rain or snowfall. It is an important part of the hydrological cycle and can impact the pH of soils and water bodies." []
is_a: ECOSIM:CATEGORYDepositionFlux ! category - deposition flux
relationship: attribute ECOSIMCONCEPT:Deposition ! Deposition
relationship: has_unit ECOSIM:gd-2h-1 ! g d-2 h-1
relationship: measurement_of ECOSIMCONCEPT:Aluminium ! Aluminium

[Term]
id: ECOSIM:XALSBS
name: wet deposition of AlSO4
def: "Wet deposition of AlSO4 refers to the process where sulfuric acid (SO4) combined with aluminum (Al) is removed from the atmosphere through precipitation events such as rain, sleet, or snow. This process plays a significant role in the biogeochemical cycling of sulfur and aluminum through various terrestrial and aquatic ecosystems, and can impact soil chemistry, plant health and water quality." []
is_a: ECOSIM:CATEGORYDepositionFlux ! category - deposition flux
relationship: has_unit ECOSIM:gd-2h-1 ! g d-2 h-1
relationship: measurement_of ECOSIMCONCEPT:AlSO4 ! Aluminum sulfate

[Term]
id: ECOSIM:XC0PBS
name: wet deposition of CaPO4
def: "A process in which CaPO4 (calcium phosphate) from the atmosphere is dissolved into precipitation, such as rain or snow, then carried to the Earth's surface. This process plays an important role in the geochemical cycling of calcium and phosphorous, with implications for soil fertility and plant nutrition." []
is_a: ECOSIM:CATEGORYDepositionFlux ! category - deposition flux
relationship: has_unit ECOSIM:gd-2h-1 ! g d-2 h-1
relationship: measurement_of ECOSIMCONCEPT:CaPO4 ! Calcium phosphate

[Term]
id: ECOSIM:XC1PBS
name: wet deposition of CHPO4
def: "A process in which calcium hydrogen phosphate (CHPO4) from the atmosphere is dissolved into precipitation, such as rain or snow, then carried to the Earth's surface. It plays a crucial role in various biogeochemical cycles." []
is_a: ECOSIM:CATEGORYDepositionFlux ! category - deposition flux
relationship: has_unit ECOSIM:gd-2h-1 ! g d-2 h-1
relationship: measurement_of ECOSIMCONCEPT:CHPO4 ! Calcium hydrogen phosphate

[Term]
id: ECOSIM:XC2PBS
name: wet deposition of CaH2PO4
def: "A process in which CaH2PO4 (calcium dihydrogen phosphate) from the atmosphere is dissolved into precipitation, such as rain or snow, then carried to the Earth's surface. It is an important process in the Earth's phosphorous cycle." []
is_a: ECOSIM:CATEGORYDepositionFlux ! category - deposition flux
relationship: has_unit ECOSIM:gd-2h-1 ! g d-2 h-1
relationship: measurement_of ECOSIMCONCEPT:CaH2PO4 ! Calcium dihydrogen phosphate

[Term]
id: ECOSIM:XC3BLS
name: wet deposition of CO3
def: "A process in which CO3 (carbon trioxide) from the atmosphere is dissolved into precipitation, such as rain or snow, then carried to the Earth's surface. It is an important process in the Earth's carbon cycle." []
is_a: ECOSIM:CATEGORYDepositionFlux ! category - deposition flux
relationship: has_unit ECOSIM:gd-2h-1 ! g d-2 h-1
relationship: measurement_of ECOSIMCONCEPT:CO3 ! Carbonate

[Term]
id: ECOSIM:XCABLS
name: wet deposition of Ca
def: "Wet deposition of Calcium is a process where calcium from the atmosphere dissolves into precipitation, such as rain or snow, and then is carried to the Earth's surface. It plays a key role in maintaining the balance of calcium in the environment." []
is_a: ECOSIM:CATEGORYDepositionFlux ! category - deposition flux
relationship: has_unit ECOSIM:gd-2h-1 ! g d-2 h-1
relationship: measurement_of ECOSIMCONCEPT:Ca ! Calcium

[Term]
id: ECOSIM:XCACBS
name: wet deposition of CaCO3
def: "Wet deposition of CaCO3 refers to the process by which calcium carbonate (CaCO3) particles in the atmosphere are captured by precipitation, such as rain or snow, and then deposited onto the Earth's surface. This can occur through various atmospheric processes, such as cloud capture and scavenging. Wet deposition of CaCO3 is an important part of the Earth's carbon and calcium cycles, and can influence soil chemistry, aquatic ecosystems, and climate." []
is_a: ECOSIM:CATEGORYDepositionFlux ! category - deposition flux
relationship: has_unit ECOSIM:gd-2h-1 ! g d-2 h-1
relationship: measurement_of ECOSIMCONCEPT:CaCO3 ! Calcium carbonate

[Term]
id: ECOSIM:XCAHBS
name: wet deposition of CaHCO3
def: "Wet deposition of CaHCO3 refers to the process in which calcium bicarbonate (CaHCO3), which is dissolved in the atmosphere, is carried down to the Earth's surface by precipitation, such as rain or snow. This factor plays a significant role in the Earth's carbon cycle and can affect various ecological processes, such as soil acidity and nutrient cycling." []
is_a: ECOSIM:CATEGORYDepositionFlux ! category - deposition flux
relationship: attribute ECOSIMCONCEPT:Deposition ! Deposition
relationship: has_unit ECOSIM:gd-2h-1 ! g d-2 h-1
relationship: measured_in ECOSIMCONCEPT:Water ! Water
relationship: measurement_of ECOSIMCONCEPT:CaHCO3 ! Calcium bicarbonate

[Term]
id: ECOSIM:XCAOBS
name: wet deposition of CaOH
def: "Wet deposition of CaOH refers to the process in which calcium hydroxide (CaOH) particles in the atmosphere dissolve in precipitation and are carried to the Earth's surface. This process plays an important role in the redistribution of calcium in terrestrial ecosystems and can affect soil pH, nutrient cycling, and plant health. The rate of wet deposition of CaOH can vary depending on atmospheric and environmental conditions, and therefore, it's an important parameter in Earth system modeling." []
is_a: ECOSIM:CATEGORYDepositionFlux ! category - deposition flux
relationship: attribute ECOSIMCONCEPT:Deposition ! Deposition
relationship: has_unit ECOSIM:gd-2h-1 ! g d-2 h-1
relationship: measurement_of ECOSIMCONCEPT:CaOH ! Calcium hydroxide

[Term]
id: ECOSIM:XCASBS
name: wet deposition of CaSO4
def: "This is the process in which the compound Calcium Sulphate (CaSO4) is captured by atmospheric precipitations and deposited into the earth's surface. The main natural sources of atmospheric gasous sulphur are volcanic emissions. Wet deposition of CaSO4 is critical in the biogeochemical cycling of sulphur." []
is_a: ECOSIM:CATEGORYDepositionFlux ! category - deposition flux
relationship: has_unit ECOSIM:gd-2h-1 ! g d-2 h-1
relationship: measurement_of ECOSIMCONCEPT:CaSO4 ! Calcium sulfate

[Term]
id: ECOSIM:XCHBLS
name: wet deposition of CH4
def: "A process in which CH4 (methane) from the atmosphere is dissolved into precipitation, such as rain or snow, then carried to the Earth's surface. It is an important process in the Earth's carbon cycle." []
is_a: ECOSIM:CATEGORYDepositionFlux ! category - deposition flux
relationship: has_unit ECOSIM:gd-2h-1 ! g d-2 h-1
relationship: measurement_of ECOSIMCONCEPT:CH4 ! Methane

[Term]
id: ECOSIM:XCHDFG
name: soil CH4 dissolution (+ve) - volatilization (-ve)
def: "This metric refers to the soil methane dissolution which is captured by the positive value, and the volatilization of the same which is captured by its negative value. Methane dissolution refers to the process by which methane, a potent greenhouse gas produced by biological processes in the soil, dissolves into soil water or infiltrating rainwater. Volatilization, on the other hand, refers to the process of methane being released from the soil into the atmosphere." []
is_a: ECOSIM:CATEGORYGasFlux ! category - Gas Flux
is_a: ECOSIM:CATEGORYSoilBiogeochemistry ! category - Soil Biogeochemistry
relationship: attribute ECOSIMCONCEPT:Dissolution ! Dissolution
relationship: attribute ECOSIMCONCEPT:Volatilization ! Volatilization
relationship: has_unit ECOSIM:gd-2h-1 ! g d-2 h-1
relationship: measurement_of ECOSIMCONCEPT:CH4 ! Methane

[Term]
id: ECOSIM:XCHDFS
name: surface - atmosphere CH4 dissolution (+ve) - volatilization (-ve)
def: "Surface - atmosphere CH4 dissolution (+ve) - volatilization (-ve) refers to the exchange of methane (CH4) between a surface (such as a lake, river, ocean, or soil surface) and the atmosphere. A positive value denotes dissolution (uptake) of CH4 from the atmosphere by the surface, while a negative value denotes volatilization (release) of CH4 from the surface to the atmosphere. This is an important parameter in earth system modeling and for understanding the global methane cycle." []
is_a: ECOSIM:CATEGORYGasFlux ! category - Gas Flux
relationship: attribute ECOSIMCONCEPT:DissolutionVolatilization ! Dissolution volatilization
relationship: has_unit ECOSIM:gd-2h-1 ! g d-2 h-1

[Term]
id: ECOSIM:XCHQSS
name: snowpack runoff CH4 flux
def: "Snowpack runoff CH4 flux refers to the amount of methane (CH4) that is released or transported from the snowpack into downstream water systems or into the atmosphere. This can occur when methane that is trapped within the snowpack is released as the snow melts and runs off. The measurement of this flux can provide insights into the contribution of snowpacks to methane emissions, which is an important aspect of global greenhouse gas balance." []
is_a: ECOSIM:CATEGORYHydrology ! category - Hydrology
is_a: ECOSIM:CATEGORYSnowpack ! category - Snowpack
relationship: context ECOSIMCONCEPT:Runoff ! Runoff
relationship: has_unit ECOSIM:gd-2h-1 ! g d-2 h-1
relationship: measured_in ECOSIMCONCEPT:Snowpack ! Snowpack
relationship: measurement_of ECOSIMCONCEPT:CH4 ! Methane
relationship: measurement_of ECOSIMCONCEPT:Flux ! Flux

[Term]
id: ECOSIM:XCLAER
name: total clay erosion
def: "Total clay erosion refers to the cumulative loss of clay particles from soil surface due to various factors such as water flow (surface runoff and soil erosion), wind (wind erosion), and human activities (tillage, deforestation, etc.). These actions can displace the clay particles and transport them away from the area, resulting in lost nutrients and degradation of soil structure. The measurement of total clay erosion is important in studying soil conservation, water quality, and ecosystem services." []
is_a: ECOSIM:CATEGORYSoilProperty ! category - soil property
is_a: ECOSIMCONCEPT:UnclassifiedVariable ! unclassified variable
relationship: attribute ECOSIMCONCEPT:Erosion ! Erosion
relationship: has_unit ECOSIM:Mgd-2h-1 ! Mg d-2 h-1
relationship: measured_in ECOSIMCONCEPT:Clay ! Clay

[Term]
id: ECOSIM:XCLBLS
name: wet deposition of Cl
def: "Wet deposition of Cl refers to the process in which chloride ions (Cl-) from the atmosphere are dissolved into precipitation, such as rain or snow, then carried to the Earth's surface. This process is part of the global chloride cycle and plays a crucial role in maintaining the salinity of the oceans and influencing terrestrial ecosystems." []
is_a: ECOSIM:CATEGORYDepositionFlux ! category - deposition flux
relationship: has_unit ECOSIM:gd-2h-1 ! g d-2 h-1
relationship: measurement_of ECOSIMCONCEPT:Cl ! Chlorine

[Term]
id: ECOSIM:XCOBLS
name: wet deposition of CO2
def: "A process in which CO2 (carbon dioxide) from the atmosphere is dissolved into precipitation, such as rain or snow, then carried to the Earth's surface. It is an important process in the Earth's carbon cycle." []
is_a: ECOSIM:CATEGORYDepositionFlux ! category - deposition flux
relationship: has_unit ECOSIM:gd-2h-1 ! g d-2 h-1
relationship: measurement_of ECOSIMCONCEPT:CO2 ! Carbon dioxide

[Term]
id: ECOSIM:XCODFG
name: soil CO2 dissolution (+ve) - volatilization (-ve)
def: "Soil CO2 dissolution (+ve) - volatilization (-ve) refers to the process where carbon dioxide (CO2) gets dissolved into the soil (positive process), and the contrasting process where CO2 gets volatilized or liberated from the soil to the atmosphere (negative process). These processes are part of the soil-atmosphere carbon exchange and play crucial roles in the global carbon cycle impacting the levels of greenhouse gases." []
is_a: ECOSIM:CATEGORYGasFlux ! category - Gas Flux
is_a: ECOSIM:CATEGORYSoilBiogeochemistry ! category - Soil Biogeochemistry
relationship: attribute ECOSIMCONCEPT:Dissolution ! Dissolution
relationship: attribute ECOSIMCONCEPT:Volatilization ! Volatilization
relationship: has_unit ECOSIM:gd-2h-1 ! g d-2 h-1
relationship: measured_in ECOSIMCONCEPT:Soil ! Soil
relationship: measurement_of ECOSIMCONCEPT:CO2 ! Carbon dioxide

[Term]
id: ECOSIM:XCODFS
name: surface - atmosphere CO2 dissolution (+ve) - volatilization (-ve)
def: "Surface - Atmosphere CO2 Dissolution (+ve) - Volatilization (-ve) represents the two-way movement of carbon dioxide (CO2) between the atmosphere and the surface, including both dissolution (positive) and volatilization (negative). Dissolution refers to the process by which CO2 is absorbed by the surface (for example, by bodies of water), while volatilization refers to the release of CO2 back into the atmosphere." []
is_a: ECOSIM:CATEGORYBiogeochemistry ! category - Biogeochemistry
is_a: ECOSIM:CATEGORYGasFlux ! category - Gas Flux
relationship: has_unit ECOSIM:gd-2h-1 ! g d-2 h-1
relationship: measured_in ECOSIMCONCEPT:Atmosphere ! Atmosphere
relationship: measured_in ECOSIMCONCEPT:Surface ! Surface
relationship: measurement_of ECOSIMCONCEPT:CO2 ! Carbon dioxide
relationship: qualifier ECOSIMCONCEPT:Dissolution ! Dissolution
relationship: qualifier ECOSIMCONCEPT:Volatilization ! Volatilization

[Term]
id: ECOSIM:XCOQSS
name: snowpack runoff CO2 flux
def: "Snowpack runoff CO2 flux refers to the amount of CO2 that is transferred from the snowpack to other Earth's components such as soil, air and rivers during snowmelt. This process of carbon transfer plays an essential role in Earth's carbon cycle." []
is_a: ECOSIM:CATEGORYSnowpack ! category - Snowpack
is_a: ECOSIM:CATEGORYTraceGasFlux ! category - trace gas flux
relationship: attribute ECOSIMCONCEPT:Flux ! Flux
relationship: context ECOSIMCONCEPT:Snowpack ! Snowpack
relationship: has_unit ECOSIM:gd-2h-1 ! g d-2 h-1
relationship: measurement_of ECOSIMCONCEPT:CO2 ! Carbon dioxide
relationship: qualifier ECOSIMCONCEPT:Runoff ! Runoff

[Term]
id: ECOSIM:XDL
name: critical daylength for phenological progress
def: "Critical daylength for phenological progress refers to the amount of daylight necessary for a plant to transition from one stage of development to another. It is a critical factor in determining the timing of development and maturity in many plant species." []
is_a: ECOSIM:CATEGORYCanopyPhysiology ! category - Canopy Physiology
is_a: ECOSIM:CATEGORYCanopyStructure ! category - canopy structure
is_a: ECOSIM:CATEGORYPlantPhysiology ! category - plant physiology
relationship: has_unit ECOSIM:h ! h
relationship: measurement_of ECOSIMCONCEPT:PhenologicalProgress ! PhenologicalProgress
relationship: qualifier ECOSIMCONCEPT:Critical ! Critical

[Term]
id: ECOSIM:XER
name: soil detachment/deposition
def: "Soil detachment or deposition refers to the process by which soil particles are removed from their original location and deposited in another area. This can result from various factors, including water and wind erosion, human activities, and changes in the landscape." []
is_a: ECOSIMCONCEPT:UnclassifiedVariable ! unclassified variable
relationship: measured_in ECOSIMCONCEPT:Soil ! Soil

[Term]
id: ECOSIM:XF1PBS
name: wet deposition of FeHPO4
def: "Wet deposition of FeHPO4 refers to the process in which iron phosphate (FeHPO4) from the atmosphere is dissolved into precipitation, such as rain or snow, then carried to the Earth's surface. This process plays a crucial role in the Earth's phosphorus and iron cycle, as it contributes to the re-distribution of these nutrients in the environment. Furthermore, it can significantly impact various biological and ecological processes in terrestrial and aquatic ecosystems." []
is_a: ECOSIM:CATEGORYDepositionFlux ! category - deposition flux
relationship: has_unit ECOSIM:gd-2h-1 ! g d-2 h-1
relationship: measurement_of ECOSIMCONCEPT:FeHPO4 ! Iron hydrogen phosphate

[Term]
id: ECOSIM:XF2PBS
name: wet deposition of FeH2PO4
def: "A process in which FeH2PO4 (iron(II) phosphate) from the atmosphere is dissolved into precipitation, such as rain or snow, then carried to the Earth's surface. It is an important process in the Earth's phosphorus and iron cycle." []
is_a: ECOSIM:CATEGORYDepositionFlux ! category - deposition flux
relationship: has_unit ECOSIM:gd-2h-1 ! g d-2 h-1
relationship: measurement_of ECOSIMCONCEPT:FeH2PO4 ! Iron dihydrogen phosphate

[Term]
id: ECOSIM:XFE1BS
name: wet deposition of FeOH
def: "Wet deposition of FeOH refers to the process by which iron hydroxide (FeOH) is removed from the air and deposited onto surfaces, primarily through the action of rain, snow, and other forms of precipitation. This process plays a key role in the global cycling of iron, which is an essential nutrient for many forms of life, and can have significant impacts on terrestrial and aquatic ecosystems." []
is_a: ECOSIM:CATEGORYDepositionFlux ! category - deposition flux
relationship: attribute ECOSIMCONCEPT:Deposition ! Deposition
relationship: has_unit ECOSIM:gd-2h-1 ! g d-2 h-1
relationship: measured_in ECOSIMCONCEPT:Water ! Water
relationship: measurement_of ECOSIMCONCEPT:FeOH ! Iron hydroxide

[Term]
id: ECOSIM:XFE2BS
name: wet deposition of FeOH2
def: "Wet deposition of FeOH2 refers to the process where airborne particles of iron hydroxide (FeOH2) are washed out of the atmosphere by rain, sleet, snow, or fog. It's an important pathway by which FeOH2 is removed from the atmosphere and deposited onto the earth's surface. This process has implications for nutrient composition of terrestrial and aquatic ecosystems." []
is_a: ECOSIM:CATEGORYDepositionFlux ! category - deposition flux
relationship: has_unit ECOSIM:gd-2h-1 ! g d-2 h-1
relationship: measured_in ECOSIMCONCEPT:Atmosphere ! Atmosphere
relationship: measurement_of ECOSIMCONCEPT:FeOH2 ! Iron dihydroxide

[Term]
id: ECOSIM:XFE3BS
name: wet deposition of FeOH3
def: "A process in which FeOH3 (iron(III) hydroxide) from the atmosphere is dissolved into precipitation, such as rain or snow, then carried to the Earth's surface. It is an important process in the Earth's iron cycle, affecting soil fertility and plant growth." []
is_a: ECOSIM:CATEGORYDepositionFlux ! category - deposition flux
relationship: has_unit ECOSIM:gd-2h-1 ! g d-2 h-1
relationship: measurement_of ECOSIMCONCEPT:FeOH3 ! Iron trihydroxide

[Term]
id: ECOSIM:XFE4BS
name: wet deposition of FeOH4
def: "Wet deposition of FeOH4 refers to the process where iron hydroxide (FeOH4) in the atmosphere is dissolved in precipitation and transported to the surface. It is an important mechanism for the removal of pollutants from the atmosphere and can impact nutrient availability in ecosystems." []
is_a: ECOSIM:CATEGORYDepositionFlux ! category - deposition flux
relationship: has_unit ECOSIM:gd-2h-1 ! g d-2 h-1
relationship: measurement_of ECOSIMCONCEPT:FeOH4 ! Iron tetrahydroxide

[Term]
id: ECOSIM:XFEBLS
name: wet deposition of Fe
def: "Wet deposition of Fe refers to the process by which iron (Fe) from the atmosphere is dissolved into precipitation, such as rain or snow, and then carried to the Earth's surface. This process is an important aspect of the nutrient cycle, contributing to the distribution and availability of iron in the soil." []
is_a: ECOSIM:CATEGORYDepositionFlux ! category - deposition flux
relationship: has_unit ECOSIM:gd-2h-1 ! g d-2 h-1
relationship: measurement_of ECOSIMCONCEPT:Fe ! Iron

[Term]
id: ECOSIM:XFESBS
name: wet deposition of FeSO4
def: "A process in which FeSO4 (Iron(II) sulfate) from the atmosphere is dissolved into precipitation, such as rain or snow, then carried to the Earth's surface. This process plays a significant role in the bioavailability of iron in terrestrial and aquatic systems. The availability of iron in these environments, which is governed in part by its deposition from the atmosphere in forms like FeSO4, affects the health and productivity of ecosystems." []
is_a: ECOSIM:CATEGORYDepositionFlux ! category - deposition flux
relationship: attribute ECOSIMCONCEPT:Deposition ! Deposition
relationship: has_unit ECOSIM:gd-2h-1 ! g d-2 h-1
relationship: measurement_of ECOSIMCONCEPT:FeSO4 ! Iron sulfate

[Term]
id: ECOSIM:XH0PBS
name: wet deposition of PO4
def: "Wet deposition of PO4 refers to the process where PO4 (phosphate) particles from the atmosphere are dissolved into precipitation, such as rain or snow, then carried to the Earth's surface. This is an important process in the nutrient cycle of ecosystems." []
is_a: ECOSIM:CATEGORYDepositionFlux ! category - deposition flux
relationship: has_unit ECOSIM:gd-2h-1 ! g d-2 h-1
relationship: measurement_of ECOSIMCONCEPT:PO4 ! Phosphate

[Term]
id: ECOSIM:XH1BS
name: net microbial HPO4 exchange band
is_a: ECOSIM:CATEGORYNTransformation ! category - N transformation
relationship: attribute ECOSIMCONCEPT:Exchange ! Exchange
relationship: has_unit ECOSIM:gd-2h-1 ! g d-2 h-1
relationship: measurement_of ECOSIMCONCEPT:HPO4 ! Hydrogen phosphate
relationship: qualifier ECOSIMCONCEPT:Band ! Band

[Term]
id: ECOSIM:XH1PBS
name: wet deposition of HPO4
def: "A process in which HPO4 (hydrogen phosphate) from the atmosphere is dissolved into precipitation, such as rain or snow, then carried to the Earth's surface. It is an important process in the Earth's phosphate cycle." []
is_a: ECOSIM:CATEGORYDepositionFlux ! category - deposition flux
relationship: has_unit ECOSIM:gd-2h-1 ! g d-2 h-1
relationship: measurement_of ECOSIMCONCEPT:HPO4 ! Hydrogen phosphate

[Term]
id: ECOSIM:XH1PS
name: net microibal HPO4 exchange non-band
is_a: ECOSIM:CATEGORYNTransformation ! category - N transformation
relationship: attribute ECOSIMCONCEPT:Exchange ! Exchange
relationship: has_unit ECOSIM:gd-2h-1 ! g d-2 h-1
relationship: measurement_of ECOSIMCONCEPT:HPO4 ! Hydrogen phosphate

[Term]
id: ECOSIM:XH2BS
name: net microbial PO4 exchange band
is_a: ECOSIM:CATEGORYNTransformation ! category - N transformation
relationship: attribute ECOSIMCONCEPT:Exchange ! Exchange
relationship: has_unit ECOSIM:gd-2h-1 ! g d-2 h-1
relationship: measurement_of ECOSIMCONCEPT:PO4 ! Phosphate

[Term]
id: ECOSIM:XH2PBS
name: wet deposition of H2PO4
def: "Wet deposition of H2PO4 refers to a process in which H2PO4 (dihydrogen phosphate) from the atmosphere is dissolved into water droplets in the form of precipitation (such as rain or snow) and then carried to the Earth's surface. This is an important process in the Earth's phosphorus cycle, contributing to the natural fertilization of terrestrial and aquatic ecosystems." []
is_a: ECOSIM:CATEGORYDepositionFlux ! category - deposition flux
relationship: has_unit ECOSIM:gd-2h-1 ! g d-2 h-1
relationship: measurement_of ECOSIMCONCEPT:H2PO4 ! Dihydrogen phosphate

[Term]
id: ECOSIM:XH2PS
name: net microbial PO4 exchange nonband
is_a: ECOSIM:CATEGORYNTransformation ! category - N transformation
relationship: attribute ECOSIMCONCEPT:Exchange ! Exchange
relationship: has_unit ECOSIM:gd-2h-1 ! g d-2 h-1
relationship: measurement_of ECOSIMCONCEPT:PO4 ! Phosphate

[Term]
id: ECOSIM:XH3PBS
name: wet deposition of H3PO4
def: "The wet deposition of phosphoric acid (H3PO4) is a process where the chemical compound H3PO4 is absorbed from the atmosphere by precipitation and then depicts onto the Earth's surface. This process is critical in the phosphorous cycle, influencing the productivity of ecosystems." []
is_a: ECOSIM:CATEGORYDepositionFlux ! category - deposition flux
relationship: has_unit ECOSIM:gd-2h-1 ! g d-2 h-1
relationship: measurement_of ECOSIMCONCEPT:H3PO4 ! Phosphoric acid

[Term]
id: ECOSIM:XHCBLS
name: wet deposition of HCO3
def: "Wet deposition of HCO3 refers to the process where bicarbonate (HCO3-) ions are carried from the atmosphere to the Earth's surface through precipitation. This includes processes like rain, snow, sleet, or hail. The bicarbonate ions can originate from several sources including pollution, and natural atmospheric processes. Wet deposition is important in the natural buffering of environmental acidity. It is also an important process in the global carbon cycle, contributing to the transfer of carbon between different reservoirs." []
is_a: ECOSIM:CATEGORYDepositionFlux ! category - deposition flux
relationship: has_unit ECOSIM:gd-2h-1 ! g d-2 h-1
relationship: measurement_of ECOSIMCONCEPT:HCO3 ! Bicarbonate

[Term]
id: ECOSIM:XHGBLS
name: wet deposition of H2
def: "A process in which H2 (hydrogen gas) from the atmosphere is dissolved into precipitation, such as rain or snow, then carried to the Earth's surface. It is an important process in the Earth's hydrogen cycle." []
is_a: ECOSIM:CATEGORYDepositionFlux ! category - deposition flux
relationship: has_unit ECOSIM:gd-2h-1 ! g d-2 h-1
relationship: measurement_of ECOSIMCONCEPT:H2 ! Dihydrogen

[Term]
id: ECOSIM:XHGDFG
name: soil H2 dissolution (+ve) - volatilization (-ve)
def: "Soil H2 dissolution (+ve) - volatilization (-ve) indicates the rate at which hydrogen gas (H2) dissolves into the soil or volatilizes (turns into gas and released) from it. A positive value indicates the gas is being absorbed into the soil (dissolution) while a negative value suggests the gas is being released from the soil (volatilization). This parameter plays a crucial role in the soil's biogeochemical cycling and can influence microbial activity, nutrient availability, and other soil properties." []
is_a: ECOSIM:CATEGORYGasFlux ! category - Gas Flux
is_a: ECOSIM:CATEGORYSoilBiogeochemistry ! category - Soil Biogeochemistry
relationship: attribute ECOSIMCONCEPT:Dissolution ! Dissolution
relationship: attribute ECOSIMCONCEPT:Volatilization ! Volatilization
relationship: has_unit ECOSIM:gd-2h-1 ! g d-2 h-1
relationship: measured_in ECOSIMCONCEPT:Soil ! Soil
relationship: measurement_of ECOSIMCONCEPT:Hydrogen ! Hydrogen

[Term]
id: ECOSIM:XHGDFS
name: surface - atmosphere H2 dissolution (+ve) - volatilization (-ve)
def: "Surface - Atmosphere H2 dissolution (+ve) - volatilization (-ve) refers to the process of hydrogen gas (H2) moving into (dissolution, positive) and out of (volatilization, negative) the atmosphere from the earth's surface. In other words, it describes the transfer of H2 between the atmosphere and the earth's surface. This process is influenced by various factors including temperature, pressure, humidity, and the concentration of H2 in both the atmosphere and the surface." []
is_a: ECOSIM:CATEGORYGasFlux ! category - Gas Flux
relationship: attribute ECOSIMCONCEPT:Exchange ! Exchange
relationship: context ECOSIMCONCEPT:Atmosphere ! Atmosphere
relationship: context ECOSIMCONCEPT:Surface ! Surface
relationship: has_unit ECOSIM:gd-2h-1 ! g d-2 h-1
relationship: measurement_of ECOSIMCONCEPT:H2 ! Dihydrogen
relationship: qualifier ECOSIMCONCEPT:Dissolution ! Dissolution
relationship: qualifier ECOSIMCONCEPT:Volatilization ! Volatilization

[Term]
id: ECOSIM:XHVSTE
name: ecosystem harvest
def: "Ecosystem harvest refers to the removal of biological products (like timber, fodder, firewood, biofuels, and non-timber forest products) from an ecosystem. It is a form of ecosystem service and is critical to many human livelihoods and economies worldwide. In the context of an earth system model, ecosystem harvest is important to consider as it can significantly impact biodiversity, vegetation structure, and biogeochemical cycles." []
is_a: ECOSIMCONCEPT:UnclassifiedVariable ! unclassified variable
relationship: attribute ECOSIMCONCEPT:Harvest ! Harvest
relationship: has_unit ECOSIM:gd-2 ! g d-2

[Term]
id: ECOSIM:XHYBLS
name: wet deposition of H
def: "Wet deposition of H refers to the process wherein hydrogen (H) from the atmosphere is dissolved into the precipitation, such as rain or snow. It then gets transported to the Earth's surface. It symbolizes an important part of the biological-chemical cycling of substances in the ecosystem and plays a significant role in keeping the acid-base balance in check." []
is_a: ECOSIM:CATEGORYDepositionFlux ! category - deposition flux
relationship: has_unit ECOSIM:gd-2h-1 ! g d-2 h-1
relationship: measurement_of ECOSIMCONCEPT:H ! Hydrogen

[Term]
id: ECOSIM:XKABLS
name: wet deposition of K
def: "The process by which potassium (K) in the atmosphere is dissolved into precipitation, such as rain or snow, then transported to the Earth's surface. This plays a crucial role in replenishing soil potassium levels and influences nutrient cycling in ecosystems." []
is_a: ECOSIM:CATEGORYDepositionFlux ! category - deposition flux
relationship: has_unit ECOSIM:gd-2h-1 ! g d-2 h-1
relationship: measurement_of ECOSIMCONCEPT:K ! Potassium

[Term]
id: ECOSIM:XKASBS
name: wet deposition of KSO4
def: "A process in which KSO4 (potassium sulfate) from the atmosphere is dissolved into precipitation, such as rain or snow, then carried to the Earth's surface. This process is an important way in which nutrients, such as potassium, are transferred from the atmosphere to the soil." []
is_a: ECOSIM:CATEGORYDepositionFlux ! category - deposition flux
relationship: has_unit ECOSIM:gd-2h-1 ! g d-2 h-1
relationship: measurement_of ECOSIMCONCEPT:KSO4 ! Potassium sulfate

[Term]
id: ECOSIM:XKCO2
name: Km for rubisco carboxylase activity
def: "Km for rubisco carboxylase activity is the Michaelis-Menten constant for the enzyme ribulose-1,5-bisphosphate carboxylase/oxygenase (rubisco) during its carboxylation reaction. It represents the concentration of CO2 at which the reaction rate is half of its maximum. This parameter is crucial in understanding and modelling the process of photosynthesis because rubisco is the key enzyme that catalyzes the first step of carbon fixation." []
is_a: ECOSIM:CATEGORYPlantPhysiology ! category - plant physiology
is_a: ECOSIMCONCEPT:UnclassifiedVariable ! unclassified variable
relationship: has_unit ECOSIM:uM ! uM
relationship: measurement_of ECOSIMCONCEPT:RubiscoCarboxylaseActivity ! RubiscoCarboxylaseActivity

[Term]
id: ECOSIM:XKCO24
name: Km for PEP carboxylase activity
def: "Km for PEP carboxylase activity refers to the substrate concentration at which the reaction rate is half of the maximum rate for the PEP carboxylase enzyme. It is an important measure in plant physiology, indicating the enzyme's affinity for its substrate under specific conditions." []
is_a: ECOSIM:CATEGORYPlantPhysiology ! category - plant physiology
is_a: ECOSIMCONCEPT:UnclassifiedVariable ! unclassified variable
relationship: has_unit ECOSIM:uM ! uM
relationship: measured_in ECOSIMCONCEPT:Plant ! Plant
relationship: measurement_of ECOSIMCONCEPT:PEPCarboxylase ! Phosphoenolpyruvate carboxylase

[Term]
id: ECOSIM:XKCO2L
name: leaf aqueous CO2 Km no O2
is_a: ECOSIM:CATEGORYCanopyPhysiology ! category - Canopy Physiology
is_a: ECOSIM:CATEGORYPlantPhysiology ! category - plant physiology
relationship: attribute ECOSIMCONCEPT:Concentration ! Concentration
relationship: has_unit ECOSIM:uM ! uM
relationship: measured_in ECOSIMCONCEPT:Leaf ! Leaf
relationship: measurement_of ECOSIMCONCEPT:CO2 ! Carbon dioxide
relationship: qualifier ECOSIMCONCEPT:Aqueous ! Aqueous

[Term]
id: ECOSIM:XKCO2O
name: leaf aqueous CO2 Km ambient O2
is_a: ECOSIM:CATEGORYCanopyPhysiology ! category - Canopy Physiology
is_a: ECOSIM:CATEGORYPlantPhysiology ! category - plant physiology
relationship: context ECOSIMCONCEPT:O2 ! Dioxygen
relationship: has_unit ECOSIM:uM ! uM
relationship: measured_in ECOSIMCONCEPT:Leaf ! Leaf
relationship: measurement_of ECOSIMCONCEPT:CO2 ! Carbon dioxide

[Term]
id: ECOSIM:XKO2
name: Km for rubisco oxygenase activity
def: "Km for Rubisco oxygenase activity refers to the concentration of O2 at which the carbon fixation by Rubisco (ribulose-1,5-bisphosphate carboxylase/oxygenase, the enzyme responsible for photosynthesis) is half of the maximum rate. This gives an indication of the affinity of Rubisco for O2 and its role in photorespiration, a process that decreases the efficiency of photosynthesis." []
is_a: ECOSIM:CATEGORYPlantPhysiology ! category - plant physiology
is_a: ECOSIMCONCEPT:UnclassifiedVariable ! unclassified variable
relationship: has_unit ECOSIM:uM ! uM
relationship: measurement_of ECOSIMCONCEPT:RubiscoOxygenaseActivity ! Rubisco oxygenase activity

[Term]
id: ECOSIM:XM1PBS
name: wet deposition of MgHPO4
def: "The process by which magnesium hydrogen phosphate (MgHPO4), a chemical compound often found in fertilizers and detergents, is deposited on the Earth's surface by rain or snow. 'Wet deposition' occurs when these chemical compounds are washed out of the atmosphere by precipitation, contributing to the nutrient content of the receiving ecosystem. Monitoring this process is important for understanding and predicting ecological change in response to atmospheric deposition." []
is_a: ECOSIM:CATEGORYDepositionFlux ! category - deposition flux
relationship: has_unit ECOSIM:gd-2h-1 ! g d-2 h-1
relationship: measurement_of ECOSIMCONCEPT:MgHPO4 ! Magnesium hydrogen phosphate

[Term]
id: ECOSIM:XMGBLS
name: wet deposition of Mg
def: "Wet deposition of Mg refers to the process where atmospheric magnesium (Mg) is carried to the Earth’s surface through precipitation events such as rain, hail, sleet, or snowfall. It contributes to transferring biologically significant elements, like magnesium, from the atmosphere to terrestrial and aquatic ecosystems, where it can affect nutrient availability and distribution, thus influencing various ecological processes." []
is_a: ECOSIM:CATEGORYDepositionFlux ! category - deposition flux
relationship: attribute ECOSIMCONCEPT:Deposition ! Deposition
relationship: has_unit ECOSIM:gd-2h-1 ! g d-2 h-1
relationship: measurement_of ECOSIMCONCEPT:Mg ! Magnesium

[Term]
id: ECOSIM:XMGCBS
name: wet deposition of MgCO3
def: "Wet deposition of MgCO3 refers to the process where Magnesium carbonate (MgCO3) particles in the atmosphere get absorbed by precipitation (rain, snow, etc.) and are deposited on the Earth’s surface. It's an important process in the Earth's carbon cycle as well as the geochemical cycle of magnesium." []
is_a: ECOSIM:CATEGORYDepositionFlux ! category - deposition flux
relationship: has_unit ECOSIM:gd-2h-1 ! g d-2 h-1
relationship: measurement_of ECOSIMCONCEPT:MgCO3 ! Magnesium carbonate

[Term]
id: ECOSIM:XMGHBS
name: wet deposition of MgHCO3
def: "Wet deposition of MgHCO3 refers to the process of magnesium bicarbonate (MgHCO3) being removed from the atmosphere during a precipitation event like rain or snowfall. This typically occurs when atmospheric MgHCO3 binds with water droplets and is brought down to the ground. Wet deposition of MgHCO3 is significant in earth system science as it affects the chemistry of atmospheric and terrestrial waters and plays a role in biogeochemical cycling." []
is_a: ECOSIM:CATEGORYDepositionFlux ! category - deposition flux
relationship: has_unit ECOSIM:gd-2h-1 ! g d-2 h-1
relationship: measurement_of ECOSIMCONCEPT:MgHCO3 ! Magnesium bicarbonate

[Term]
id: ECOSIM:XMGOBS
name: wet deposition of MgOH
def: "A process in which MgOH (magnesium hydroxide) from the atmosphere is dissolved into precipitation, such as rain or snow, then carried to the Earth's surface. This process affects the global distribution, fate and effects of MgOH." []
is_a: ECOSIM:CATEGORYDepositionFlux ! category - deposition flux
relationship: has_unit ECOSIM:gd-2h-1 ! g d-2 h-1
relationship: measurement_of ECOSIMCONCEPT:MgOH ! Magnesium hydroxide

[Term]
id: ECOSIM:XMGSBS
name: wet deposition of MgSO4
def: "Wet deposition of MgSO4 refers to the process where airborne magnesium sulfate (MgSO4) particles are absorbed by precipitation, such as rain, snow, or fog, and are then carried to the earth’s surface. The phenomenon plays an important part in the global distribution of nutrients and can impact soil chemistry, plant health, and water quality." []
is_a: ECOSIM:CATEGORYDepositionFlux ! category - deposition flux
relationship: has_unit ECOSIM:gd-2h-1 ! g d-2 h-1
relationship: measurement_of ECOSIMCONCEPT:MgSO4 ! Magnesium sulfate

[Term]
id: ECOSIM:XN2BLS
name: wet deposition of N2O
def: "The process in which nitrogen oxide (N2O) from the atmosphere dissolves into precipitation, such as rain or snow, and is carried to the Earth's surface. It is an important process in the nitrogen cycle." []
is_a: ECOSIM:CATEGORYDepositionFlux ! category - deposition flux
relationship: has_unit ECOSIM:gd-2h-1 ! g d-2 h-1
relationship: measurement_of ECOSIMCONCEPT:N2O ! Nitrous oxide

[Term]
id: ECOSIM:XN2DFG
name: soil N2O dissolution (+ve) - volatilization (-ve)
def: "This parameter represents the process of soil N2O (nitrous oxide) dissolution or volatilization in the environment. The term 'dissolution' refers to the absorption or resolution of N2O into the soil, while 'volatilization' indicates the conversion or evaporation of N2O from the soil to the atmosphere. The (+ve) indicates a positive value or increase in soil N2O due to dissolution, while the (-ve) indicates a negative value or decrease in soil N2O due to volatilization. This process can be influenced by various factors, such as soil type, temperature, moisture content, microbial activity, and the presence of other gases or nutrients in the soil." []
is_a: ECOSIM:CATEGORYNTransformation ! category - N transformation
is_a: ECOSIMCONCEPT:UnclassifiedVariable ! unclassified variable
relationship: attribute ECOSIMCONCEPT:Exchange ! Exchange
relationship: has_unit ECOSIM:gd-2h-1 ! g d-2 h-1
relationship: measured_in ECOSIMCONCEPT:Soil ! Soil
relationship: measurement_of ECOSIMCONCEPT:N2O ! Nitrous oxide

[Term]
id: ECOSIM:XN2DFS
name: surface - atmosphere N2O dissolution (+ve) - volatilization (-ve)
def: "The rate at which nitrous oxide (N2O) is dissolved into the surface water from the atmosphere or volatilized back to the atmosphere from the water surface can be represented by the flux term XN2DFS. This term is positive when there is dissolution of N2O from the atmosphere into surface waters and negative when N2O volatilizes from the water surface back to the atmosphere." []
is_a: ECOSIM:CATEGORYGasFlux ! category - Gas Flux
is_a: ECOSIMCONCEPT:UnclassifiedVariable ! unclassified variable
relationship: attribute ECOSIMCONCEPT:Flux ! Flux
relationship: context ECOSIMCONCEPT:Dissolution ! Dissolution
relationship: context ECOSIMCONCEPT:Volatilization ! Volatilization
relationship: has_unit ECOSIM:gd-2h-1 ! g d-2 h-1
relationship: measured_in ECOSIMCONCEPT:Atmosphere ! Atmosphere
relationship: measured_in ECOSIMCONCEPT:SurfaceWater ! Surface water
relationship: measurement_of ECOSIMCONCEPT:N2O ! Nitrous oxide

[Term]
id: ECOSIM:XN2GS
name: net microbial N2 exchange
is_a: ECOSIM:CATEGORYNTransformation ! category - N transformation
relationship: attribute ECOSIMCONCEPT:Exchange ! Exchange
relationship: has_unit ECOSIM:gd-2h-1 ! g d-2 h-1
relationship: measurement_of ECOSIMCONCEPT:N2 ! Dinitrogen

[Term]
id: ECOSIM:XN2QSS
name: snowpack runoff N2O flux
is_a: ECOSIM:CATEGORYNTransformation ! category - N transformation
is_a: ECOSIM:CATEGORYSnowpack ! category - Snowpack
relationship: attribute ECOSIMCONCEPT:Flux ! Flux
relationship: context ECOSIMCONCEPT:SnowpackRunoff ! Snowpack runoff
relationship: has_unit ECOSIM:gd-2h-1 ! g d-2 h-1
relationship: measurement_of ECOSIMCONCEPT:N2O ! Nitrous oxide

[Term]
id: ECOSIM:XN3BLW
name: wet deposition of NH3
def: "A process in which NH3 (ammonia) from the atmosphere is dissolved into precipitation, such as rain or snow, then carried to the Earth's surface. It plays a crucial role in nitrogen cycling within ecosystems." []
is_a: ECOSIM:CATEGORYDepositionFlux ! category - deposition flux
relationship: has_unit ECOSIM:gd-2h-1 ! g d-2 h-1
relationship: measurement_of ECOSIMCONCEPT:NH3 ! Ammonia

[Term]
id: ECOSIM:XN3DFG
name: soil NH3 dissolution (+ve) - volatilization (-ve) non-band
is_a: ECOSIM:CATEGORYGasFlux ! category - Gas Flux
relationship: has_unit ECOSIM:gd-2h-1 ! g d-2 h-1
relationship: measured_in ECOSIMCONCEPT:Soil ! Soil
relationship: measurement_of ECOSIMCONCEPT:NH3 ! Ammonia

[Term]
id: ECOSIM:XN3DFS
name: surface - atmosphere NH3 dissolution (+ve) - volatilization (-ve) non-band
def: "This represents the dissolution (positive) and volatilization (negative) of NH3 between the earth's surface and the atmosphere. It is a non-banded measurement, indicating it does not distinguish specific frequency bands." []
is_a: ECOSIM:CATEGORYGasFlux ! category - Gas Flux
is_a: ECOSIM:CATEGORYNTransformation ! category - N transformation
relationship: attribute ECOSIMCONCEPT:Exchange ! Exchange
relationship: has_unit ECOSIM:gd-2h-1 ! g d-2 h-1
relationship: measurement_of ECOSIMCONCEPT:NH3 ! Ammonia
relationship: qualifier ECOSIMCONCEPT:Dissolution ! Dissolution
relationship: qualifier ECOSIMCONCEPT:Volatilization ! Volatilization

[Term]
id: ECOSIM:XN3QSS
name: snowpack runoff NH3 flux
is_a: ECOSIM:CATEGORYSnowpack ! category - Snowpack
relationship: attribute ECOSIMCONCEPT:Flux ! Flux
relationship: context ECOSIMCONCEPT:Runoff ! Runoff
relationship: has_unit ECOSIM:gd-2h-1 ! g d-2 h-1
relationship: measured_in ECOSIMCONCEPT:Snowpack ! Snowpack
relationship: measurement_of ECOSIMCONCEPT:NH3 ! Ammonia

[Term]
id: ECOSIM:XN4BLW
name: wet deposition of NH4
is_a: ECOSIM:CATEGORYDepositionFlux ! category - deposition flux
relationship: attribute ECOSIMCONCEPT:Deposition ! Deposition
relationship: has_unit ECOSIM:gd-2h-1 ! g d-2 h-1
relationship: measurement_of ECOSIMCONCEPT:NH4 ! Ammonium

[Term]
id: ECOSIM:XN4QSS
name: snowpack runoff NH4 flux
is_a: ECOSIM:CATEGORYSnowpack ! category - Snowpack
relationship: attribute ECOSIMCONCEPT:Flux ! Flux
relationship: context ECOSIMCONCEPT:Runoff ! Runoff
relationship: has_unit ECOSIM:gd-2h-1 ! g d-2 h-1
relationship: measured_in ECOSIMCONCEPT:Snowpack ! Snowpack
relationship: measurement_of ECOSIMCONCEPT:NH4 ! Ammonium

[Term]
id: ECOSIM:XNABLS
name: wet deposition of Na
def: "Wet deposition of Na refers to the process by which sodium (Na) from the atmosphere dissolves into precipitation, such as rain or snow, then carried to the Earth's surface. It is an important process in biogeochemical cycles as it impacts soil and water chemistry." []
is_a: ECOSIM:CATEGORYDepositionFlux ! category - deposition flux
relationship: has_unit ECOSIM:gd-2h-1 ! g d-2 h-1
relationship: measurement_of ECOSIMCONCEPT:Na ! Na
relationship: measurement_of ECOSIMCONCEPT:Sodium ! Sodium

[Term]
id: ECOSIM:XNACBS
name: wet deposition of NaCO3
def: "A process in which NaCO3 (sodium carbonate) from the atmosphere is dissolved in precipitation, such as rain or snow, and transported to the Earth's surface. It is a key process in the Earth's sodium cycle." []
is_a: ECOSIM:CATEGORYDepositionFlux ! category - deposition flux
relationship: has_unit ECOSIM:gd-2h-1 ! g d-2 h-1
relationship: measurement_of ECOSIMCONCEPT:NaCO3 ! NaCO3

[Term]
id: ECOSIM:XNASBS
name: wet deposition of NaSO4
def: "Wet deposition of NaSO4 refers to the process by which sodium sulfate (NaSO4) particles in the atmosphere are removed by precipitation, such as rain, snow, or fog, and transported to the Earth's surface. This process plays an important role in the cycling and distribution of sodium and sulfur in the environment, affecting soil chemistry, plant health, water quality, and atmospheric dynamics." []
is_a: ECOSIM:CATEGORYDepositionFlux ! category - deposition flux
relationship: has_unit ECOSIM:gd-2h-1 ! g d-2 h-1
relationship: measurement_of ECOSIMCONCEPT:NaSO4 ! NaSO4

[Term]
id: ECOSIM:XNBDFG
name: soil NH3 dissolution (+ve) - volatilization (-ve) band
def: "The soil NH3 dissolution (+ve) - volatilization (-ve) band refers to the balance between the dissolution (positive sign) and volatilization (negative sign) of ammonia (NH3) in the soil. Dissolution and volatilization are two key processes that determine the availability of NH3 in soil for plant uptake and microbial activity, as well as its loss to the atmosphere. Therefore, the dissolution-volatilization band plays a significant role in the nitrogen (N) cycling within the soil ecosystem." []
is_a: ECOSIM:CATEGORYGasFlux ! category - Gas Flux
is_a: ECOSIMCONCEPT:Soil ! Soil
relationship: attribute ECOSIMCONCEPT:Dissolution ! Dissolution
relationship: attribute ECOSIMCONCEPT:Volatilization ! Volatilization
relationship: has_unit ECOSIM:gd-2h-1 ! g d-2 h-1
relationship: measurement_of ECOSIMCONCEPT:NH3 ! Ammonia

[Term]
id: ECOSIM:XNBDFS
name: surface - atmosphere NH3 dissolution (+ve) - volatilization (-ve) band
def: "Surface - atmosphere NH3 dissolution (+ve) - volatilization (-ve) band refers to the transition zone, or band, in which ammonia (NH3) can either dissolve into the surface (positive direction) or evaporate/volatilize into the atmosphere (negative direction). This band signals a changing environmental state where different variables and conditions might affect the movement and concentration of ammonia between the surface and the atmosphere." []
is_a: ECOSIMCONCEPT:UnclassifiedVariable ! unclassified variable
relationship: attribute ECOSIMCONCEPT:Dissolution ! Dissolution
relationship: attribute ECOSIMCONCEPT:Volatilization ! Volatilization
relationship: context ECOSIMCONCEPT:Surface ! Surface
relationship: has_unit ECOSIM:gd-2h-1 ! g d-2 h-1
relationship: measured_in ECOSIMCONCEPT:Atmosphere ! Atmosphere
relationship: measurement_of ECOSIMCONCEPT:NH3 ! Ammonia
relationship: qualifier ECOSIMCONCEPT:Band ! Band

[Term]
id: ECOSIM:XNGBLS
name: wet deposition of N2
is_a: ECOSIM:CATEGORYDepositionFlux ! category - deposition flux
relationship: has_unit ECOSIM:gd-2h-1 ! g d-2 h-1
relationship: measurement_of ECOSIMCONCEPT:N2 ! Dinitrogen

[Term]
id: ECOSIM:XNGDFG
name: soil N2 dissolution (+ve) - volatilization (-ve)
def: "Soil N2 dissolution (+ve) - volatilization (-ve) refers to the net flux of nitrogen gas (N2) from the soil due to the processes of dissolution and volatilization. Dissolution involves the conversion of nitrogen in the soil into a form that can be taken up by plants, while volatilization involves the release of nitrogen into the atmosphere. The sign convention indicates that a positive value represents a net influx of N2 into the soil system (dissolution), while a negative value represents a net efflux of N2 from the soil system (volatilization). This parameter is important in the cycling of nitrogen in ecosystems, influencing nutrient availability and productivity." []
is_a: ECOSIM:CATEGORYNTransformation ! category - N transformation
is_a: ECOSIMCONCEPT:UnclassifiedVariable ! unclassified variable
relationship: attribute ECOSIMCONCEPT:Flux ! Flux
relationship: has_unit ECOSIM:gd-2h-1 ! g d-2 h-1
relationship: measured_in ECOSIMCONCEPT:Soil ! Soil
relationship: measurement_of ECOSIMCONCEPT:N2 ! Dinitrogen

[Term]
id: ECOSIM:XNGDFS
name: surface - atmosphere N2 dissolution (+ve) - volatilization (-ve)
def: "Surface - atmosphere N2 dissolution/volatilization refers to the movement of nitrogen gas (N2) between the surface and the atmosphere, with dissolution (+ve) indicating the process of N2 being absorbed into the surface water from the atmosphere and volatilization (-ve) referring to the release of N2 from the surface water into the atmosphere. These processes play a crucial role in the nitrogen cycle, influencing the availability of nitrogen for biological processes and the composition of the atmosphere." []
is_a: ECOSIMCONCEPT:UnclassifiedVariable ! unclassified variable
relationship: attribute ECOSIMCONCEPT:Exchange ! Exchange
relationship: has_unit ECOSIM:gd-2h-1 ! g d-2 h-1
relationship: measured_in ECOSIMCONCEPT:Atmosphere ! Atmosphere
relationship: measured_in ECOSIMCONCEPT:Surface ! Surface
relationship: measurement_of ECOSIMCONCEPT:NitrogenGas ! NitrogenGas

[Term]
id: ECOSIM:XNGQSS
name: snowpack runoff N2 flux
is_a: ECOSIM:CATEGORYSnowpack ! category - Snowpack
relationship: attribute ECOSIMCONCEPT:Flux ! Flux
relationship: context ECOSIMCONCEPT:Runoff ! Runoff
relationship: has_unit ECOSIM:gd-2h-1 ! g d-2 h-1
relationship: measurement_of ECOSIMCONCEPT:N2 ! Dinitrogen

[Term]
id: ECOSIM:XNH3EB
name: total NH3 fertilizer erosion band
is_a: ECOSIMCONCEPT:UnclassifiedVariable ! unclassified variable
relationship: attribute ECOSIMCONCEPT:Fertilizer ! Fertilizer
relationship: context ECOSIMCONCEPT:ErosionBand ! ErosionBand
relationship: has_unit ECOSIM:gd-2h-1 ! g d-2 h-1
relationship: measurement_of ECOSIMCONCEPT:NH3 ! Ammonia

[Term]
id: ECOSIM:XNH3ER
name: total NH3 fertilizer erosion non-band
is_a: ECOSIMCONCEPT:UnclassifiedVariable ! unclassified variable
relationship: attribute ECOSIMCONCEPT:Erosion ! Erosion
relationship: context ECOSIMCONCEPT:NH3 ! Ammonia
relationship: has_unit ECOSIM:gd-2h-1 ! g d-2 h-1
relationship: measured_in ECOSIMCONCEPT:Fertilizer ! Fertilizer

[Term]
id: ECOSIM:XNH4B
name: net microbial NH4 exchange band
is_a: ECOSIM:CATEGORYNTransformation ! category - N transformation
relationship: attribute ECOSIMCONCEPT:Exchange ! Exchange
relationship: has_unit ECOSIM:gd-2h-1 ! g d-2 h-1
relationship: measurement_of ECOSIMCONCEPT:NH4 ! Ammonium
relationship: qualifier ECOSIMCONCEPT:Band ! Band

[Term]
id: ECOSIM:XNH4EB
name: total NH4 fertilizer erosion band
def: "Total NH4 fertilizer erosion band refers to the loss of ammonium (NH4) nutrient from the soil due to erosion. This generally occurs when the NH4 fertilizer has been applied in a banding method (a specific method of applying fertilizer in soil), and erosion happens due to factors such as heavy rain, wind, or other environmental conditions. The amount of erosion can affect the availability of NH4 for plants and can have a significant impact on crop productivity and environmental quality." []
is_a: ECOSIMCONCEPT:UnclassifiedVariable ! unclassified variable
relationship: context ECOSIMCONCEPT:Band ! Band
relationship: context ECOSIMCONCEPT:Erosion ! Erosion
relationship: context ECOSIMCONCEPT:Fertilizer ! Fertilizer
relationship: has_unit ECOSIM:gd-2h-1 ! g d-2 h-1
relationship: measurement_of ECOSIMCONCEPT:NH4 ! Ammonium

[Term]
id: ECOSIM:XNH4ER
name: total NH4 fertilizer erosion non-band
is_a: ECOSIMCONCEPT:UnclassifiedVariable ! unclassified variable
relationship: attribute ECOSIMCONCEPT:Erosion ! Erosion
relationship: has_unit ECOSIM:gd-2h-1 ! g d-2 h-1
relationship: measurement_of ECOSIMCONCEPT:FertilizerNH4 ! FertilizerNH4

[Term]
id: ECOSIM:XNH4S
name: net microbial NH4 exchange non-band
is_a: ECOSIM:CATEGORYNTransformation ! category - N transformation
relationship: attribute ECOSIMCONCEPT:Exchange ! Exchange
relationship: has_unit ECOSIM:gd-2h-1 ! g d-2 h-1
relationship: measurement_of ECOSIMCONCEPT:NH4 ! Ammonium

[Term]
id: ECOSIM:XNHUEB
name: total urea fertilizer erosion band
def: "Total urea fertilizer erosion band refers to the total amount of urea fertilizer that has been eroded from a specific area or 'band' as a result of various processes such as rainfall, wind, or human activity. This can be an important parameter in agricultural and environmental studies as it can provide information about the effectiveness of fertilizer application practices and the potential for nutrient losses and environmental contamination." []
is_a: ECOSIMCONCEPT:UnclassifiedVariable ! unclassified variable
relationship: context ECOSIMCONCEPT:Erosion ! Erosion
relationship: has_unit ECOSIM:gd-2h-1 ! g d-2 h-1
relationship: measured_in ECOSIMCONCEPT:Band ! Band
relationship: measurement_of ECOSIMCONCEPT:UreaFertilizer ! UreaFertilizer

[Term]
id: ECOSIM:XNHUER
name: total urea fertilizer erosion non-band
is_a: ECOSIM:CATEGORYNTransformation ! category - N transformation
is_a: ECOSIMCONCEPT:UnclassifiedVariable ! unclassified variable
relationship: attribute ECOSIMCONCEPT:Erosion ! Erosion
relationship: context ECOSIMCONCEPT:Fertilizer ! Fertilizer
relationship: has_unit ECOSIM:gd-2h-1 ! g d-2 h-1
relationship: measurement_of ECOSIMCONCEPT:Urea ! Urea

[Term]
id: ECOSIM:XNO2B
name: net microbial NO2 exchange band
is_a: ECOSIM:CATEGORYNTransformation ! category - N transformation
relationship: attribute ECOSIMCONCEPT:Exchange ! Exchange
relationship: has_unit ECOSIM:gd-2h-1 ! g d-2 h-1
relationship: measurement_of ECOSIMCONCEPT:NO2 ! Nitrogen dioxide
relationship: qualifier ECOSIMCONCEPT:Band ! Band

[Term]
id: ECOSIM:XNO2S
name: total NO2 exchange
def: "Total NO2 exchange refers to the total movement or transfer of Nitrogen dioxide (NO2), a key air pollutant, between different physical processes, chemical reactions or biological entities in the environment. It encompasses both uptake and emission of NO2 in the environment and is significant in atmospheric and environmental modeling, influencing various processes such as air quality, climate, and the nitrogen cycle." []
is_a: ECOSIM:CATEGORYNTransformation ! category - N transformation
relationship: attribute ECOSIMCONCEPT:Exchange ! Exchange
relationship: has_unit ECOSIM:gd-2h-1 ! g d-2 h-1
relationship: measurement_of ECOSIMCONCEPT:NO2 ! Nitrogen dioxide

[Term]
id: ECOSIM:XNO3B
name: net microbial NO3 exchange band
is_a: ECOSIM:CATEGORYNTransformation ! category - N transformation
relationship: attribute ECOSIMCONCEPT:Exchange ! Exchange
relationship: context ECOSIMCONCEPT:Band ! Band
relationship: has_unit ECOSIM:gd-2h-1 ! g d-2 h-1
relationship: measurement_of ECOSIMCONCEPT:NO3 ! Nitrate

[Term]
id: ECOSIM:XNO3EB
name: total NO3 fertilizer erosion band
is_a: ECOSIMCONCEPT:UnclassifiedVariable ! unclassified variable
relationship: has_unit ECOSIM:gd-2h-1 ! g d-2 h-1
relationship: measured_in ECOSIMCONCEPT:ErosionBand ! ErosionBand
relationship: measurement_of ECOSIMCONCEPT:NO3Fertilizer ! NO3Fertilizer

[Term]
id: ECOSIM:XNO3ER
name: total NO3 fertilizer erosion non-band
def: "Total NO3 fertilizer erosion non-band refers to the total amount of nitrate (NO3) from non-banded fertilizer applications that is lost due to erosion. Non-banded fertilizer applications are those in which the fertilizer is distributed across the soil surface, rather than being applied in a band or strip. Erosion, usually caused by rainfall and runoff, can carry away these surface-applied nutrients, potentially leading to decreased fertilizer efficiency, reduced plant growth and yield, and environmental pollution due to nutrient runoff." []
is_a: ECOSIM:CATEGORYNTransformation ! category - N transformation
is_a: ECOSIMCONCEPT:UnclassifiedVariable ! unclassified variable
relationship: context ECOSIMCONCEPT:Erosion ! Erosion
relationship: context ECOSIMCONCEPT:Fertilizer ! Fertilizer
relationship: has_unit ECOSIM:gd-2h-1 ! g d-2 h-1
relationship: measured_in ECOSIMCONCEPT:TopSoil ! TopSoil
relationship: measurement_of ECOSIMCONCEPT:NO3 ! Nitrate

[Term]
id: ECOSIM:XNO3S
name: net microbial NO3 exchange non-band
is_a: ECOSIM:CATEGORYNTransformation ! category - N transformation
relationship: attribute ECOSIMCONCEPT:Exchange ! Exchange
relationship: has_unit ECOSIM:gd-2h-1 ! g d-2 h-1
relationship: measurement_of ECOSIMCONCEPT:NO3 ! Nitrate

[Term]
id: ECOSIM:XNOBLW
name: wet deposition of NO3
def: "Wet deposition of NO3 refers to the process in which nitrogen oxide (NO3) in the atmosphere is absorbed into precipitation (like rain or snow) and then transported to the surface of the Earth. This process plays a vital role in the nitrogen cycle and impacts terrestrial and aquatic ecosystems." []
is_a: ECOSIM:CATEGORYDepositionFlux ! category - deposition flux
relationship: has_unit ECOSIM:gd-2h-1 ! g d-2 h-1
relationship: measurement_of ECOSIMCONCEPT:NO3 ! Nitrate

[Term]
id: ECOSIM:XNOQSS
name: snowpack runoff NO3 flux
is_a: ECOSIM:CATEGORYDepositionFlux ! category - deposition flux
is_a: ECOSIM:CATEGORYSnowpack ! category - Snowpack
relationship: attribute ECOSIMCONCEPT:Flux ! Flux
relationship: context ECOSIMCONCEPT:Runoff ! Runoff
relationship: context ECOSIMCONCEPT:Snowpack ! Snowpack
relationship: has_unit ECOSIM:gd-2h-1 ! g d-2 h-1
relationship: measurement_of ECOSIMCONCEPT:NO3 ! Nitrate

[Term]
id: ECOSIM:XOAFHS
name: acetate flux macropore
def: "Acetate flux in macropores refers to the movement of acetate, a short-chain fatty acid, in and out of large pores (macropores) in the soil matrix. Acetate flux in macropores provides vital insights into the transportation of organic matter within the soil structure and can reveal key aspects about soil biology, chemistry, and hydrodynamics." []
is_a: ECOSIMCONCEPT:UnclassifiedVariable ! unclassified variable
relationship: attribute ECOSIMCONCEPT:Flux ! Flux
relationship: has_unit ECOSIM:gd-2h-1 ! g d-2 h-1
relationship: measured_in ECOSIMCONCEPT:Macropore ! Macropore
relationship: measurement_of ECOSIMCONCEPT:Acetate ! Acetate

[Term]
id: ECOSIM:XOAFLS
name: aqueous acetate flux
def: "Aqueous acetate flux refers to the rate at which acetate, a form of organic carbon, is transported through an aqueous medium. This is an important parameter in earth systems modeling related to carbon cycling, microbial activity, and water quality." []
is_a: ECOSIMCONCEPT:UnclassifiedVariable ! unclassified variable
relationship: attribute ECOSIMCONCEPT:Flux ! Flux
relationship: context ECOSIMCONCEPT:Aqueous ! Aqueous
relationship: has_unit ECOSIM:gd-2h-1 ! g d-2 h-1
relationship: measurement_of ECOSIMCONCEPT:Acetate ! Acetate

[Term]
id: ECOSIM:XOAFXS
name: total acetate micropore-macropore transfer
def: "Total acetate micropore-macropore transfer refers to the process by which acetate ions (CH3COO-) are transferred from micropores (small soil pores typically less than 0.05mm in diameter) to macropores (larger soil pores usually greater than 0.05mm in diameter) in the soil. It is an essential process in soil chemistry that influences several aspects of soil functionality, including nutrient cycling and soil structure." []
is_a: ECOSIM:CATEGORYElementFlux ! category - C and nutrient flux
relationship: has_unit ECOSIM:gd-2h-1 ! g d-2 h-1
relationship: measured_in ECOSIMCONCEPT:Macropore ! Macropore
relationship: measured_in ECOSIMCONCEPT:Micropore ! Micropore
relationship: measurement_of ECOSIMCONCEPT:Acetate ! Acetate

[Term]
id: ECOSIM:XOAQRS
name: surface runoff acetate flux
def: "Surface runoff acetate flux refers to the movement of acetate from land to water bodies via surface runoff. Acetate is a key intermediate in microbial metabolic processes and its transport via runoff can affect microbial communities in aquatic systems. Changes in the acetate flux can thus impact biological productivity and nutrient cycling in both terrestrial and aquatic ecosystems." []
is_a: ECOSIM:CATEGORYHydrology ! category - Hydrology
is_a: ECOSIMCONCEPT:UnclassifiedVariable ! unclassified variable
relationship: attribute ECOSIMCONCEPT:Flux ! Flux
relationship: has_unit ECOSIM:gd-2h-1 ! g d-2 h-1
relationship: measured_in ECOSIMCONCEPT:SurfaceRunoff ! Surface runoff
relationship: measurement_of ECOSIMCONCEPT:Acetate ! Acetate

[Term]
id: ECOSIM:XOCFHS
name: DOC flux macropore
def: "DOC flux macropore refers to the amount of dissolved organic carbon (DOC) that is transported through the large pores present in the soil structure. It is an important indicator of carbon cycling within the soil ecosystem, playing a key role in nutrient cycling, soil fertility, and climate regulation." []
is_a: ECOSIM:CATEGORYSoilBiogeochemistry ! category - Soil Biogeochemistry
is_a: ECOSIMCONCEPT:UnclassifiedVariable ! unclassified variable
relationship: attribute ECOSIMCONCEPT:Flux ! Flux
relationship: has_unit ECOSIM:gd-2h-1 ! g d-2 h-1
relationship: measured_in ECOSIMCONCEPT:SoilMacropore ! SoilMacropore
relationship: measurement_of ECOSIMCONCEPT:DOC ! DOC

[Term]
id: ECOSIM:XOCFLS
name: DOC flux micropore
def: "DOC flux micropore refers to the amount of dissolved organic carbon (DOC) flowing through soil micropores. DOC is a component of the soil organic matter and represents a substantial pool of terrestrial carbon. It contributes to various soil functions and processes, and its dynamics are important in understanding carbon cycling in the environment. Micropores, the smallest pores in soil (< 0.05 mm), allow the transport of water and DOC. Thus, the flux of DOC in these micropores is an important aspect of carbon distribution and movement within the soil." []
is_a: ECOSIM:CATEGORYHydrology ! category - Hydrology
is_a: ECOSIMCONCEPT:UnclassifiedVariable ! unclassified variable
relationship: attribute ECOSIMCONCEPT:Flux ! Flux
relationship: has_unit ECOSIM:gd-2h-1 ! g d-2 h-1
relationship: measured_in ECOSIMCONCEPT:SoilMicropore ! Soil micropore
relationship: measurement_of ECOSIMCONCEPT:DOC ! DOC

[Term]
id: ECOSIM:XOCFXS
name: total DOC micropore-macropore transfer
def: "Total DOC micropore-macropore transfer refers to the total amount of dissolved organic carbon (DOC) that is transferred from the micropores to the macropores in the soil. This process plays a crucial role in soil carbon cycling and turnover, influencing soil fertility and ecosystem productivity. The amount of DOC transferred can be influenced by factors such as soil texture, organic matter content, and microbial activity." []
is_a: ECOSIM:CATEGORYElementFlux ! category - C and nutrient flux
relationship: has_unit ECOSIM:gd-2h-1 ! g d-2 h-1
relationship: measured_in ECOSIMCONCEPT:Macropore ! Macropore
relationship: measured_in ECOSIMCONCEPT:Micropore ! Micropore
relationship: measurement_of ECOSIMCONCEPT:DOC ! DOC

[Term]
id: ECOSIM:XOCQRS
name: surface runoff DOC flux
def: "Surface runoff DOC flux refers to the movement or transfer of Dissolved Organic Carbon (DOC) in the form of surface runoff across a given area over a specific period of time. DOC represents a significant proportion of the total organic carbon in many surface waters and plays a vital role in many biogeochemical processes. Its movement can affect the nutrient cycling, microbial activity, and water quality in the affected ecosystems." []
is_a: ECOSIMCONCEPT:UnclassifiedVariable ! unclassified variable
relationship: attribute ECOSIMCONCEPT:Flux ! Flux
relationship: has_unit ECOSIM:gd-2h-1 ! g d-2 h-1
relationship: measured_in ECOSIMCONCEPT:SurfaceRunoff ! Surface runoff
relationship: measurement_of ECOSIMCONCEPT:DissolvedOrganicCarbon ! Dissolved organic carbon

[Term]
id: ECOSIM:XOHBLS
name: wet deposition of OH
def: "Wet deposition of OH refers to the process whereby hydroxyl radicals (OH-) in the atmosphere are dissolved into precipitation, such as rain or snow, and then transported to the Earth's surface. This can affect the concentration of OH- radicals in the atmosphere, and plays a role in the cleaning of the atmosphere as these radicals react with pollutants." []
is_a: ECOSIM:CATEGORYDepositionFlux ! category - deposition flux
relationship: has_unit ECOSIM:gd-2h-1 ! g d-2 h-1
relationship: measurement_of ECOSIMCONCEPT:OH ! OH

[Term]
id: ECOSIM:XONFHS
name: DON flux macropore
def: "The flux of Dissolved Organic Nitrogen (DON) through macropores in the soil. Macropores, such as wormholes, root channels and cracks, are pathways for the rapid vertical transport of water and solutes, like DON, through the soil profile." []
is_a: ECOSIMCONCEPT:UnclassifiedVariable ! unclassified variable
relationship: attribute ECOSIMCONCEPT:Flux ! Flux
relationship: context ECOSIMCONCEPT:Macropore ! Macropore
relationship: has_unit ECOSIM:gd-2h-1 ! g d-2 h-1
relationship: measurement_of ECOSIMCONCEPT:DON ! DON

[Term]
id: ECOSIM:XONFLS
name: DON flux micropore
def: "The amount of dissolved organic nitrogen (DON) that moves through the soil via micropores. This flux can have significant implications for nutrient cycling and soil fertility." []
is_a: ECOSIMCONCEPT:UnclassifiedVariable ! unclassified variable
relationship: attribute ECOSIMCONCEPT:Flux ! Flux
relationship: has_unit ECOSIM:gd-2h-1 ! g d-2 h-1
relationship: measured_in ECOSIMCONCEPT:SoilMicropore ! Soil micropore
relationship: measurement_of ECOSIMCONCEPT:DON ! DON

[Term]
id: ECOSIM:XONFXS
name: total DON micropore-macropore transfer
def: "Total DON micropore-macropore transfer refers to the total transfer of Dissolved Organic Nitrogen (DON) between micropores and macropores in the soil. This transfer is a key part of the nutrient cycle in ecosystems and can influence a variety of biological and ecological processes." []
is_a: ECOSIM:CATEGORYElementFlux ! category - C and nutrient flux
relationship: has_unit ECOSIM:gd-2h-1 ! g d-2 h-1
relationship: measured_in ECOSIMCONCEPT:Macropore ! Macropore
relationship: measured_in ECOSIMCONCEPT:Micropore ! Micropore
relationship: measurement_of ECOSIMCONCEPT:DissolvedOrganicNitrogen ! Dissolved organic nitrogen

[Term]
id: ECOSIM:XONQRS
name: surface runoff DON flux
is_a: ECOSIM:CATEGORYHydrology ! category - Hydrology
is_a: ECOSIMCONCEPT:UnclassifiedVariable ! unclassified variable
relationship: attribute ECOSIMCONCEPT:Flux ! Flux
relationship: has_unit ECOSIM:gd-2h-1 ! g d-2 h-1
relationship: measured_in ECOSIMCONCEPT:SurfaceRunoff ! Surface runoff
relationship: measurement_of ECOSIMCONCEPT:DON ! DON

[Term]
id: ECOSIM:XOPFHS
name: DOP flux macropore
def: "DOP flux macropore refers to the of movement of Dissolved Organic Phosphorus (DOP) in the macropore spaces in the soil. It plays a significant role in the cycling of phosphorous in soils and can influence the availability of phosphorous to plants and microbes." []
is_a: ECOSIMCONCEPT:UnclassifiedVariable ! unclassified variable
relationship: attribute ECOSIMCONCEPT:Flux ! Flux
relationship: has_unit ECOSIM:gd-2h-1 ! g d-2 h-1
relationship: measured_in ECOSIMCONCEPT:SoilMacropore ! SoilMacropore
relationship: measurement_of ECOSIMCONCEPT:DOP ! Dissolved organic phosphorus

[Term]
id: ECOSIM:XOPFLS
name: DOP flux micropore
def: "Dissolved organic phosphorus (DOP) flux in micropores refers to the movement of DOP within the small pores within the soil structure. These micropores, which are generally less than 0.05mm in diameter, can influence the movement of water and nutrients including DOP in the soil. Understanding DOP flux in micropores can provide valuable insights into nutrient cycling and availability in soil ecosystems." []
is_a: ECOSIMCONCEPT:UnclassifiedVariable ! unclassified variable
relationship: attribute ECOSIMCONCEPT:Flux ! Flux
relationship: has_unit ECOSIM:gd-2h-1 ! g d-2 h-1
relationship: measured_in ECOSIMCONCEPT:Micropore ! Micropore
relationship: measurement_of ECOSIMCONCEPT:DOP ! Dissolved organic phosphorus

[Term]
id: ECOSIM:XOPFXS
name: total DOP micropore-macropore transfer
def: "Total DOP micropore-macropore transfer refers to the overall movement or transfer of Dissolved Organic Phosphorus (DOP) from the smaller pores (micropores) to the larger pores (macropores) in soil. This is an important factor in nutrient cycling in soil, influencing the availability and leaching of phosphorus." []
is_a: ECOSIM:CATEGORYElementFlux ! category - C and nutrient flux
relationship: context ECOSIMCONCEPT:SoilMacropore ! SoilMacropore
relationship: has_unit ECOSIM:gd-2h-1 ! g d-2 h-1
relationship: measured_in ECOSIMCONCEPT:MicroporeMacropore ! MicroporeMacropore
relationship: measured_in ECOSIMCONCEPT:SoilMicropore ! Soil micropore
relationship: measurement_of ECOSIMCONCEPT:DissolvedOrganicPhosphoros ! DissolvedOrganicPhosphoros
relationship: measurement_of ECOSIMCONCEPT:DOP ! Dissolved organic phosphorus

[Term]
id: ECOSIM:XOPQRS
name: surface runoff DOP flux
def: "Surface runoff DOP flux refers to the quantity or rate at which dissolved organic phosphorus (DOP) is transported from the land surface into aquatic systems due to runoff. This can be influenced by factors such as rainfall intensity, soil type, land cover, and human activities. DOP is a form of phosphorus that is dissolved in water and includes organic compounds like nucleic acids and phospholipids. Excessive DOP fluxes can lead to eutrophication in water bodies, causing harmful algal blooms and decreased water quality." []
is_a: ECOSIMCONCEPT:Runoff ! Runoff
is_a: ECOSIMCONCEPT:UnclassifiedVariable ! unclassified variable
relationship: attribute ECOSIMCONCEPT:Flux ! Flux
relationship: has_unit ECOSIM:gd-2h-1 ! g d-2 h-1
relationship: measured_in ECOSIMCONCEPT:RunoffSurface ! RunoffSurface
relationship: measurement_of ECOSIMCONCEPT:DOP ! Dissolved organic phosphorus

[Term]
id: ECOSIM:XOQAS
name: net microbial acetate flux
def: "Net microbial acetate flux refers to the net change in the amount of acetate, a key intermediate in many biological processes, due to microbial activity. This is an important measure in microbial ecology and biogeochemistry, as acetate fluxes can have significant impacts on various environmental processes and nutrient cycling." []
is_a: ECOSIM:CATEGORYNTransformation ! category - N transformation
relationship: attribute ECOSIMCONCEPT:Flux ! Flux
relationship: has_unit ECOSIM:gd-2h-1 ! g d-2 h-1
relationship: measurement_of ECOSIMCONCEPT:Acetate ! Acetate

[Term]
id: ECOSIM:XOQCS
name: net microbial DOC flux
def: "Net Microbial DOC flux refers to the net movement or transfer of Dissolved Organic Carbon (DOC) mediated by microbes across a certain area over a specified period of time. This plays a vital role in the carbon cycle as DOC represents a significant fraction of total organic carbon in most ecosystems." []
is_a: ECOSIM:CATEGORYElementFlux ! category - C and nutrient flux
is_a: ECOSIM:CATEGORYNTransformation ! category - N transformation
relationship: attribute ECOSIMCONCEPT:Flux ! Flux
relationship: has_unit ECOSIM:gd-2h-1 ! g d-2 h-1
relationship: measurement_of ECOSIMCONCEPT:DissolvedOrganicCarbon ! Dissolved organic carbon

[Term]
id: ECOSIM:XOQNS
name: net microbial DON flux
is_a: ECOSIM:CATEGORYNTransformation ! category - N transformation
relationship: attribute ECOSIMCONCEPT:Flux ! Flux
relationship: has_unit ECOSIM:gd-2h-1 ! g d-2 h-1
relationship: measurement_of ECOSIMCONCEPT:DON ! DON

[Term]
id: ECOSIM:XOQPS
name: net microbial DOP flux
def: "Net microbial DOP flux refers to the net movement or transfer of Dissolved Organic Phosphorus (DOP) caused by microbial activity in a system over a certain period of time. This parameter is important for understanding nutrient cycling and microbial dynamics in various ecosystems." []
is_a: ECOSIM:CATEGORYNTransformation ! category - N transformation
relationship: attribute ECOSIMCONCEPT:Flux ! Flux
relationship: has_unit ECOSIM:gd-2h-1 ! g d-2 h-1
relationship: measurement_of ECOSIMCONCEPT:DissolvedOrganicPhosphorus ! DissolvedOrganicPhosphorus

[Term]
id: ECOSIM:XOXBLS
name: wet deposition of O2
def: "A process in which O2 (oxygen) from the atmosphere is dissolved into precipitation, such as rain or snow, then carried to the Earth's surface. It is an important process in the Earth's oxygen cycle." []
is_a: ECOSIM:CATEGORYDepositionFlux ! category - deposition flux
relationship: has_unit ECOSIM:gd-2h-1 ! g d-2 h-1
relationship: measurement_of ECOSIMCONCEPT:O2 ! Dioxygen

[Term]
id: ECOSIM:XOXDFG
name: soil O2 dissolution (+ve) - volatilization (-ve)
is_a: ECOSIM:CATEGORYGasFlux ! category - Gas Flux
is_a: ECOSIM:CATEGORYSoilBiogeochemistry ! category - Soil Biogeochemistry
relationship: attribute ECOSIMCONCEPT:Dissolution ! Dissolution
relationship: attribute ECOSIMCONCEPT:Volatilization ! Volatilization
relationship: has_unit ECOSIM:gd-2h-1 ! g d-2 h-1
relationship: measured_in ECOSIMCONCEPT:Soil ! Soil
relationship: measurement_of ECOSIMCONCEPT:O2 ! Dioxygen

[Term]
id: ECOSIM:XOXDFS
name: surface - atmosphere O2 dissolution (+ve) - volatilization (-ve)
def: "Surface-atmosphere O2 dissolution (+ve) - volatilization (-ve) refers to the net flux of O2 between the surface of the water (e.g., a lake or ocean) and the atmosphere due to the processes of dissolution and volatilization. Dissolution is the process by which a gas like O2 dissolves in a liquid medium (positive direction), while volatilization is the process by which a substance is released from a liquid into the atmosphere (negative direction). This flux is an important parameter influencing the oxygen levels in both the atmosphere and the water body, and thus, it impacts the lifecycle of aquatic organisms as well as atmospheric chemistry." []
is_a: ECOSIM:CATEGORYGasFlux ! category - Gas Flux
is_a: ECOSIM:CATEGORYHydrology ! category - Hydrology
relationship: attribute ECOSIMCONCEPT:Flux ! Flux
relationship: context ECOSIMCONCEPT:SurfaceAtmosphere ! Surface atmosphere
relationship: has_unit ECOSIM:gd-2h-1 ! g d-2 h-1
relationship: measurement_of ECOSIMCONCEPT:O2 ! Dioxygen

[Term]
id: ECOSIM:XOXQSS
name: snowpack runoff O2 flux
is_a: ECOSIM:CATEGORYSnowpack ! category - Snowpack
relationship: attribute ECOSIMCONCEPT:Flux ! Flux
relationship: context ECOSIMCONCEPT:Runoff ! Runoff
relationship: has_unit ECOSIM:gd-2h-1 ! g d-2 h-1
relationship: measured_in ECOSIMCONCEPT:Snowpack ! Snowpack
relationship: measurement_of ECOSIMCONCEPT:O2 ! Dioxygen

[Term]
id: ECOSIM:XP1QSS
name: snowpack runoff HPO4 flux
def: "Snowpack runoff HPO4 flux refers to the amount of phosphate (HPO4) that is transported through runoff from snowpack. This parameter is important as it provides an estimate of the quantity of this nutrient that is being released into the environment from snow melt, which can influence nutrient cycling in downstream ecosystems." []
is_a: ECOSIM:CATEGORYSnowpack ! category - Snowpack
relationship: attribute ECOSIMCONCEPT:Flux ! Flux
relationship: context ECOSIMCONCEPT:SnowpackRunoff ! Snowpack runoff
relationship: has_unit ECOSIM:gd-2h-1 ! g d-2 h-1
relationship: measurement_of ECOSIMCONCEPT:HPO4 ! Hydrogen phosphate

[Term]
id: ECOSIM:XP4QSS
name: snowpack runoff PO4 flux
def: "Snowpack runoff PO4 flux refers to the movement rate of phosphate ions (PO4) contained within the runoff from snowpack. Snowpack, the total accumulated snow and ice on the ground, gradually melts and often carries with it various ions and particles, including phosphates, as it flows into rivers and other bodies of water. This flux of PO4 from snowpack runoff can contribute to the nutrients available in downstream aquatic ecosystems, but can also cause problems such as eutrophication if the levels are too high." []
is_a: ECOSIM:CATEGORYSnowpack ! category - Snowpack
relationship: attribute ECOSIMCONCEPT:Flux ! Flux
relationship: context ECOSIMCONCEPT:Runoff ! Runoff
relationship: has_unit ECOSIM:gd-2h-1 ! g d-2 h-1
relationship: measurement_of ECOSIMCONCEPT:PO4 ! Phosphate

[Term]
id: ECOSIM:XPPD
name: difference between current and critical daylengths used to calculate phenological progress
def: "Difference between the current and critical daylengths used to calculate phenological progress." []
is_a: ECOSIM:CATEGORYCanopyStructure ! category - canopy structure
relationship: context ECOSIMCONCEPT:PhenologicalProgress ! PhenologicalProgress
relationship: has_unit ECOSIM:h ! h
relationship: qualifier ECOSIMCONCEPT:Critical ! Critical

[Term]
id: ECOSIM:XRLA
name: rate of leaf initiation
is_a: ECOSIM:CATEGORYCanopyPhysiology ! category - Canopy Physiology
is_a: ECOSIM:CATEGORYCanopyStructure ! category - canopy structure
is_a: ECOSIM:CATEGORYPlantPhysiology ! category - plant physiology
relationship: attribute ECOSIMCONCEPT:Rate ! Rate
relationship: has_unit ECOSIM:h-1at25oC ! h-1 at 25 oC
relationship: measured_in ECOSIMCONCEPT:Plant ! Plant
relationship: measurement_of ECOSIMCONCEPT:Leaf ! Leaf

[Term]
id: ECOSIM:XRNI
name: rate of node initiation
def: "Rate of node initiation is the speed at which new nodes (joints from which leaves or branches originate) form on plants. This rate can influence plant growth and development as well as their yield potential." []
is_a: ECOSIM:CATEGORYCanopyStructure ! category - canopy structure
relationship: attribute ECOSIMCONCEPT:Rate ! Rate
relationship: has_unit ECOSIM:h-1at25oC ! h-1 at 25 oC
relationship: measurement_of ECOSIMCONCEPT:NodeInitiation ! NodeInitiation

[Term]
id: ECOSIM:XSANER
name: total sand erosion
def: "Total sand erosion refers to the aggregate amount of sand or sandy soil that has been displaced from its original location, due to forces such as wind or water. This concept is critical in understanding geologic formations, soil fertility, and ecosystem health." []
is_a: ECOSIMCONCEPT:UnclassifiedVariable ! unclassified variable
relationship: attribute ECOSIMCONCEPT:Erosion ! Erosion
relationship: has_unit ECOSIM:Mgd-2h-1 ! Mg d-2 h-1
relationship: measured_in ECOSIMCONCEPT:Sand ! Sand

[Term]
id: ECOSIM:XSILER
name: total silt erosion
def: "Total silt erosion refers to the total amount of silt that is eroded, typically as a result of water flow over a defined area or landscape. Silt, a sedimentary material composed of fine granules, is easily transported by water currents. Erosion of silt can impact soil fertility, water quality, and landscape stability. Total silt erosion is an important parameter in earth system modeling, particularly in understanding the effects of land use and climate change on soil loss and degradation." []
is_a: ECOSIMCONCEPT:UnclassifiedVariable ! unclassified variable
relationship: has_unit ECOSIM:Mgd-2h-1 ! Mg d-2 h-1
relationship: measured_in ECOSIMCONCEPT:Silt ! Silt
relationship: measurement_of ECOSIMCONCEPT:Erosion ! Erosion

[Term]
id: ECOSIM:XSOBLS
name: wet deposition of SO4
def: "Wet deposition of SO4 (sulfate) refers to the process in which sulfate from the atmosphere is dissolved in precipitation, such as rain or snow, then carried to the Earth's surface. This process plays an important role in Earth's sulfur cycle. Sulfate in the atmosphere can originate from natural sources, such as volcanic eruptions, as well as human activities, such as burning of fossil fuels. Once deposited on the Earth's surface, sulfate can affect soil and water chemistry, and influence the health of terrestrial and aquatic ecosystems." []
is_a: ECOSIM:CATEGORYDepositionFlux ! category - deposition flux
relationship: has_unit ECOSIM:gd-2h-1 ! g d-2 h-1
relationship: measurement_of ECOSIMCONCEPT:SO4 ! SO4

[Term]
id: ECOSIM:XTLI
name: number of nodes in seed
def: "Number of nodes in a seed refers to the number of nodal points present in the embryonic structure of a seed. These nodes are crucial as they generally give rise to shoots or roots as the seed germinates and begins to grow." []
is_a: ECOSIM:CATEGORYCanopyStructure ! category - canopy structure
is_a: ECOSIM:CATEGORYPlantPhysiology ! category - plant physiology
relationship: measured_in ECOSIMCONCEPT:Seed ! Seed
relationship: measurement_of ECOSIMCONCEPT:Node ! Node

[Term]
id: ECOSIM:Z2GE
name: atmospheric N2 concentration
is_a: ECOSIM:CATEGORYAtmosphericConditions ! category - Atmospheric Conditions
is_a: ECOSIMCONCEPT:UnclassifiedVariable ! unclassified variable
relationship: attribute ECOSIMCONCEPT:Concentration ! Concentration
relationship: context ECOSIMCONCEPT:Atmosphere ! Atmosphere
relationship: has_unit ECOSIM:umolmol-1 ! umol mol-1
relationship: measurement_of ECOSIMCONCEPT:N2 ! Dinitrogen

[Term]
id: ECOSIM:Z2OE
name: atmospheric N2O concentration
def: "Atmospheric N2O concentration refers to the quantity of nitrous oxide (N2O) present in each unit volume of air in the atmosphere. Also known as laughing gas, N2O is a powerful greenhouse gas that is released into the atmosphere through soil cultivation practices, especially the use of commercial and organic fertilizers, fossil fuel combustion, nitric acid production, and biomass burning. Monitoring the atmospheric N2O concentration is important for climate modeling and understanding global warming potential." []
is_a: ECOSIMCONCEPT:UnclassifiedVariable ! unclassified variable
relationship: attribute ECOSIMCONCEPT:Concentration ! Concentration
relationship: context ECOSIMCONCEPT:Atmosphere ! Atmosphere
relationship: has_unit ECOSIM:umolmol-1 ! umol mol-1
relationship: measurement_of ECOSIMCONCEPT:N2O ! Nitrous oxide

[Term]
id: ECOSIM:Z2SGL
name: gaseous N2O diffusivity
def: "Gaseous N2O diffusivity refers to the measure of the rate at which nitrous oxide (N2O) gas spreads or migrates. This is an important parameter in understanding green house gas emissions and nutrient cycling in ecosystems." []
is_a: ECOSIM:CATEGORYGasFlux ! category - Gas Flux
is_a: ECOSIMCONCEPT:UnclassifiedVariable ! unclassified variable
relationship: attribute ECOSIMCONCEPT:Diffusivity ! Diffusivity
relationship: has_unit ECOSIM:m2h-1 ! m2 h-1
relationship: measured_in ECOSIMCONCEPT:Atmosphere ! Atmosphere
relationship: measurement_of ECOSIMCONCEPT:GaseousN2O ! GaseousN2O

[Term]
id: ECOSIM:ZDRAIN
name: total N drainage below root zone
def: "Total N drainage below root zone represents the amount of nitrogen that has leached out from the root zone and entered the deeper layers of soil. This leaching process can result in a significant loss of nutrients from the soil, potentially impacting plant growth and productivity. Additionally, nitrogen leaching can contribute to groundwater pollution, as it can result in elevated levels of nitrate in groundwater." []
is_a: ECOSIM:CATEGORYTraceGasFlux ! category - trace gas flux
relationship: attribute ECOSIMCONCEPT:Drainage ! Drainage
relationship: has_unit ECOSIM:gd-2 ! g d-2
relationship: measured_in ECOSIMCONCEPT:RootZone ! Root zone
relationship: measurement_of ECOSIMCONCEPT:Nitrogen ! Nitrogen

[Term]
id: ECOSIM:ZESNC
name: total litterfall element
is_a: ECOSIMCONCEPT:UnclassifiedVariable ! unclassified variable
relationship: attribute ECOSIMCONCEPT:Element ! Element
relationship: has_unit ECOSIM:gd-2h-1 ! g d-2 h-1
relationship: measured_in ECOSIMCONCEPT:Litterfall ! Litterfall

[Term]
id: ECOSIM:ZHSGL
name: aqueous NH4 diffusivity
def: "Aqueous NH4 diffusivity refers to the measure of the rate at which ammonium (NH4) ions migrate or spread through water or an aqueous medium. It represents the ability of NH4 ions to move and mix within a water system. Aqueous NH4 diffusivity is an important parameter in earth systems modeling as it plays a crucial role in understanding nutrient cycling, plant nutrition, and the movement of pollutants in aquatic environments." []
is_a: ECOSIM:CATEGORYHydrology ! category - Hydrology
is_a: ECOSIMCONCEPT:UnclassifiedVariable ! unclassified variable
relationship: attribute ECOSIMCONCEPT:Diffusivity ! Diffusivity
relationship: has_unit ECOSIM:m2h-1 ! m2 h-1
relationship: measured_in ECOSIMCONCEPT:Water ! Water
relationship: measurement_of ECOSIMCONCEPT:Ammonium ! Ammonium
relationship: qualifier ECOSIMCONCEPT:Aqueous ! Aqueous

[Term]
id: ECOSIM:ZLSGL
name: aqueous N2 diffusivity
def: "Aqueous N2 diffusivity refers to the measure of the rate at which Nitrogen (N2) ions migrate or spread through water. It influences how effectively elements can move and mix in the water. Aqueous N2 diffusivity is an important parameter in hydrological modelling and in understanding pollutant dispersal in water bodies." []
is_a: ECOSIM:CATEGORYHydrology ! category - Hydrology
is_a: ECOSIMCONCEPT:UnclassifiedVariable ! unclassified variable
relationship: attribute ECOSIMCONCEPT:Diffusivity ! Diffusivity
relationship: has_unit ECOSIM:m2h-1 ! m2 h-1
relationship: measured_in ECOSIMCONCEPT:Water ! Water
relationship: measurement_of ECOSIMCONCEPT:Nitrogen ! Nitrogen
relationship: qualifier ECOSIMCONCEPT:Aqueous ! Aqueous

[Term]
id: ECOSIM:ZNH3E
name: atmospheric NH3 concentration
is_a: ECOSIMCONCEPT:UnclassifiedVariable ! unclassified variable
relationship: attribute ECOSIMCONCEPT:Concentration ! Concentration
relationship: has_unit ECOSIM:umolmol-1 ! umol mol-1
relationship: measured_in ECOSIMCONCEPT:Atmosphere ! Atmosphere
relationship: measurement_of ECOSIMCONCEPT:NH3 ! Ammonia

[Term]
id: ECOSIM:ZNOON
name: time of solar noon
def: "Solar noon is the moment when the sun appears to contact or pass over an observer's meridian, reaching its highest point in the sky on that day, and it is the midpoint of daylight hours." []
is_a: ECOSIMCONCEPT:UnclassifiedVariable ! unclassified variable
relationship: has_unit ECOSIM:h ! h
relationship: measurement_of ECOSIMCONCEPT:Sun ! Sun

[Term]
id: ECOSIM:ZNPP
name: total net primary productivity
def: "Total net primary productivity (ZNPP) is the total amount of energy that the primary producers in an ecosystem capture through photosynthesis minus the amount of energy used for respiration. It represents the total energy available for consumption by herbivores and subsequent trophic levels. ZNPP is a key measure of ecosystem productivity and health." []
is_a: ECOSIMCONCEPT:UnclassifiedVariable ! unclassified variable
relationship: has_unit ECOSIM:gd-2 ! g d-2
relationship: measured_in ECOSIMCONCEPT:Ecosystem ! Ecosystem
relationship: measurement_of ECOSIMCONCEPT:Energy ! Energy

[Term]
id: ECOSIM:ZNSGL
name: aqueous NH3 diffusivity
def: "Aqueous NH3 diffusivity refers to the measure of the rate at which ammonia (NH3) ions migrate or spread through water or an aqueous medium. It represents the ability of NH3 ions to move and mix within a water system. Aqueous NH3 diffusivity is an important parameter in earth systems modeling as it plays a role in understanding nutrient cycling and the movement of pollutants in aquatic environments." []
is_a: ECOSIM:CATEGORYHydrology ! category - Hydrology
is_a: ECOSIMCONCEPT:UnclassifiedVariable ! unclassified variable
relationship: attribute ECOSIMCONCEPT:Diffusivity ! Diffusivity
relationship: has_unit ECOSIM:m2h-1 ! m2 h-1
relationship: measured_in ECOSIMCONCEPT:Water ! Water
relationship: measurement_of ECOSIMCONCEPT:Ammonia ! Ammonia
relationship: qualifier ECOSIMCONCEPT:Aqueous ! Aqueous

[Term]
id: ECOSIM:ZOSGL
name: aqueous NO3 diffusivity
def: "Aqueous NO3 diffusivity refers to the measure of the rate at which nitrate (NO3) ions migrate or spread through water or an aqueous medium. It represents the ability of NO3 ions to move and mix within a water system. Aqueous NO3 diffusivity is an important parameter in earth systems modeling as it plays a crucial role in understanding nutrient cycling, pollution transformation, and the movement of pollutants in aquatic environments." []
is_a: ECOSIM:CATEGORYHydrology ! category - Hydrology
is_a: ECOSIMCONCEPT:UnclassifiedVariable ! unclassified variable
relationship: attribute ECOSIMCONCEPT:Diffusivity ! Diffusivity
relationship: has_unit ECOSIM:m2h-1 ! m2 h-1
relationship: measured_in ECOSIMCONCEPT:Water ! Water
relationship: measurement_of ECOSIMCONCEPT:Nitrate ! Nitrate
relationship: qualifier ECOSIMCONCEPT:Aqueous ! Aqueous

[Term]
id: ECOSIM:ZTYP
name: plant thermal adaptation zone
def: "Thermal adaptation zones are defined geographic areas characterized by specific average temperature ranges that determine which plant species can survive and thrive there. Such zones influence the distribution and diversity of plants, reflecting the adaptability of different species to various thermal environments." []
is_a: ECOSIM:CATEGORYCanopyPhysiology ! category - Canopy Physiology
is_a: ECOSIM:CATEGORYCanopyStructure ! category - canopy structure
relationship: context ECOSIMCONCEPT:ThermalAdaptation ! ThermalAdaptation
relationship: measured_in ECOSIMCONCEPT:Zone ! Zone

[Term]
id: ECOSIM:ZTYPI
name: initial plant thermal adaptation zone
def: "Initial plant thermal adaptation zone refers to the initial zone of temperature adaptation for a plant or plant species. It indicates the range of temperatures that a plant species is adapted to withstand and grow healthily upon first introduction to a new environment or at the beginning of a growth cycle. This parameter is an important consideration in plant ecology and in the modeling of plant distribution and potential adaptation under climate change scenarios." []
is_a: ECOSIM:CATEGORYCanopyStructure ! category - canopy structure
is_a: ECOSIM:CATEGORYPlantPhysiology ! category - plant physiology
relationship: measured_in ECOSIMCONCEPT:Plant ! Plant
relationship: measured_in ECOSIMCONCEPT:Zone ! Zone
relationship: measurement_of ECOSIMCONCEPT:ThermalAdaptation ! ThermalAdaptation

[Term]
id: ECOSIM:ZVSGL
name: aqueous N2O diffusivity
def: "Aqueous N2O diffusivity refers to the measure of the rate at which nitrous oxide (N2O) molecules move or spread through water or an aqueous medium. It is an important parameter in environmental and earth system modeling, as it can impact a range of processes, including greenhouse gas emissions, soil fertility, and water quality." []
is_a: ECOSIM:CATEGORYHydrology ! category - Hydrology
is_a: ECOSIMCONCEPT:UnclassifiedVariable ! unclassified variable
relationship: attribute ECOSIMCONCEPT:Diffusivity ! Diffusivity
relationship: has_unit ECOSIM:m2h-1 ! m2 h-1
relationship: measured_in ECOSIMCONCEPT:Water ! Water
relationship: measurement_of ECOSIMCONCEPT:NitrousOxide ! NitrousOxide

[Term]
id: ECOSIM:ZeroPlanDisp
name: zero plane displacement height
is_a: ECOSIMCONCEPT:UnclassifiedVariable ! unclassified variable
relationship: has_unit ECOSIM:m ! m

[Term]
id: ECOSIM:cumSedErosion
name: sediment erosion
def: "Cumulative sediment erosion refers to the total amount of sediment that has been eroded over a given time period. This can be caused by factors such as water flow, wind, or human activity. The measurement of cumulative sediment erosion is important for understanding the rate and scale of land degradation, as well as the impact of erosion on landscape formation and nutrient cycling." []
is_a: ECOSIMCONCEPT:Erosion ! Erosion
is_a: ECOSIMCONCEPT:UnclassifiedVariable ! unclassified variable
relationship: has_unit ECOSIM:Mgd-2h-1 ! Mg d-2 h-1
relationship: measurement_of ECOSIMCONCEPT:Sediment ! Sediment

[Term]
id: ECOSIM:d-2
name: d-2
is_a: ECOSIMCONCEPT:Unit ! unit

[Term]
id: ECOSIM:dSm-1
name: dS m-1
is_a: ECOSIMCONCEPT:Unit ! unit

[Term]
id: ECOSIM:degreefromhorizontal
name: degree from horizontal
is_a: ECOSIMCONCEPT:Unit ! unit

[Term]
id: ECOSIM:fTgrowCanP
name: canopy temperature growth function
def: "Canopy temperature growth function (fTgrowCanP) is a function that describes the effect of temperature on the growth of the plant canopy. It takes into account the optimum temperature for growth, the maximum and minimum temperatures at which growth can occur, and the actual temperature. This function is used in earth systems modeling to simulate plant growth and development under various temperature conditions." []
is_a: ECOSIM:CATEGORYCanopyStructure ! category - canopy structure
is_a: ECOSIM:CATEGORYPlantPhysiology ! category - plant physiology
is_a: ECOSIM:CATEGORYPlantPopulation ! category - Plant Population
relationship: context ECOSIMCONCEPT:Temperature ! temperature
relationship: measured_in ECOSIMCONCEPT:Canopy ! Canopy

[Term]
id: ECOSIM:fTgrowRootP
name: root layer temperature growth function
def: "Root layer temperature growth function represents how the growth of roots in plants can be affected by the temperature of the root layers. This parameter in earth systems modeling helps to understand root development under different temperature conditions. It also aids in understanding soil-plant interactions, nutrient uptake, and the effect of climate change on plant growth." []
is_a: ECOSIM:CATEGORYRootPhysiology ! category - root physiology
relationship: measured_in ECOSIMCONCEPT:RootLayer ! Root layer
relationship: measurement_of ECOSIMCONCEPT:Temperature ! temperature

[Term]
id: ECOSIM:g
name: g
is_a: ECOSIMCONCEPT:Unit ! unit

[Term]
id: ECOSIM:gCd-2
name: gC d-2
is_a: ECOSIMCONCEPT:Unit ! unit

[Term]
id: ECOSIM:gCm-2
name: g C m-2
is_a: ECOSIMCONCEPT:Unit ! unit

[Term]
id: ECOSIM:gCm-3
name: gC m-3
is_a: ECOSIMCONCEPT:Unit ! unit

[Term]
id: ECOSIM:gd-2
name: g d-2
is_a: ECOSIMCONCEPT:Unit ! unit

[Term]
id: ECOSIM:gd-2h-1
name: g d-2 h-1
is_a: ECOSIMCONCEPT:Unit ! unit

[Term]
id: ECOSIM:gd-2t-1
name: g d-2 t-1
is_a: ECOSIMCONCEPT:Unit ! unit

[Term]
id: ECOSIM:gg-1
name: g g-1
is_a: ECOSIMCONCEPT:Unit ! unit

[Term]
id: ECOSIM:gh-1
name: g h-1
is_a: ECOSIMCONCEPT:Unit ! unit

[Term]
id: ECOSIM:gm-2
name: g m-2
is_a: ECOSIMCONCEPT:Unit ! unit

[Term]
id: ECOSIM:gm-2h-1
name: g m-2 h-1
is_a: ECOSIMCONCEPT:Unit ! unit

[Term]
id: ECOSIM:gm-3
name: g m-3
is_a: ECOSIMCONCEPT:Unit ! unit

[Term]
id: ECOSIM:gp-1
name: g p-1
is_a: ECOSIMCONCEPT:Unit ! unit

[Term]
id: ECOSIM:h
name: h
is_a: ECOSIMCONCEPT:Unit ! unit

[Term]
id: ECOSIM:h-1
name: h-1
is_a: ECOSIMCONCEPT:Unit ! unit

[Term]
id: ECOSIM:h-1at25oC
name: h-1 at 25 oC
is_a: ECOSIMCONCEPT:Unit ! unit

[Term]
id: ECOSIM:hm-1
name: h m-1
is_a: ECOSIMCONCEPT:Unit ! unit

[Term]
id: ECOSIM:kPa
name: kPa
is_a: ECOSIMCONCEPT:Unit ! unit

[Term]
id: ECOSIM:m
name: m
is_a: ECOSIMCONCEPT:Unit ! unit

[Term]
id: ECOSIM:m-1
name: m-1
is_a: ECOSIMCONCEPT:Unit ! unit

[Term]
id: ECOSIM:m-2
name: m-2
is_a: ECOSIMCONCEPT:Unit ! unit

[Term]
id: ECOSIM:m2
name: m2
is_a: ECOSIMCONCEPT:Unit ! unit

[Term]
id: ECOSIM:m2d-2
name: m2 d-2
is_a: ECOSIMCONCEPT:Unit ! unit

[Term]
id: ECOSIM:m2d-2h-1
name: m2 d-2 h-1
is_a: ECOSIMCONCEPT:Unit ! unit

[Term]
id: ECOSIM:m2g-1
name: m2 g-1
is_a: ECOSIMCONCEPT:Unit ! unit

[Term]
id: ECOSIM:m2h-1
name: m2 h-1
is_a: ECOSIMCONCEPT:Unit ! unit

[Term]
id: ECOSIM:m3
name: m3
is_a: ECOSIMCONCEPT:Unit ! unit

[Term]
id: ECOSIM:m3d-2
name: m3 d-2
is_a: ECOSIMCONCEPT:Unit ! unit

[Term]
id: ECOSIM:m3d-2h-1
name: m3 d-2 h-1
is_a: ECOSIMCONCEPT:Unit ! unit

[Term]
id: ECOSIM:m3d-2t-1
name: m3 d-2 t-1
is_a: ECOSIMCONCEPT:Unit ! unit

[Term]
id: ECOSIM:m3g-1
name: m3 g-1
is_a: ECOSIMCONCEPT:Unit ! unit

[Term]
id: ECOSIM:m3m-3
name: m3 m-3
is_a: ECOSIMCONCEPT:Unit ! unit

[Term]
id: ECOSIM:mMPa-1h-1
name: m MPa-1 h-1
is_a: ECOSIMCONCEPT:Unit ! unit

[Term]
id: ECOSIM:md-1
name: m d-1
is_a: ECOSIMCONCEPT:Unit ! unit

[Term]
id: ECOSIM:md-2
name: m d-2
is_a: ECOSIMCONCEPT:Unit ! unit

[Term]
id: ECOSIM:mg-1
name: m g-1
is_a: ECOSIMCONCEPT:Unit ! unit

[Term]
id: ECOSIM:mgkg-1
name: mg kg-1
is_a: ECOSIMCONCEPT:Unit ! unit

[Term]
id: ECOSIM:mh-1
name: m h-1
is_a: ECOSIMCONCEPT:Unit ! unit

[Term]
id: ECOSIM:mm-3
name: m m-3
is_a: ECOSIMCONCEPT:Unit ! unit

[Term]
id: ECOSIM:mmh-1
name: mm h-1
is_a: ECOSIMCONCEPT:Unit ! unit

[Term]
id: ECOSIM:mold-2
name: mol d-2
is_a: ECOSIMCONCEPT:Unit ! unit

[Term]
id: ECOSIM:mold-2h-1
name: mol d-2 h-1
is_a: ECOSIMCONCEPT:Unit ! unit

[Term]
id: ECOSIM:molm-3
name: mol m-3
is_a: ECOSIMCONCEPT:Unit ! unit

[Term]
id: ECOSIM:mor-
name: m or -
is_a: ECOSIMCONCEPT:Unit ! unit

[Term]
id: ECOSIM:mp-1
name: m p-1
is_a: ECOSIMCONCEPT:Unit ! unit

[Term]
id: ECOSIM:mt-1
name: m t-1
is_a: ECOSIMCONCEPT:Unit ! unit

[Term]
id: ECOSIM:o
name: o
is_a: ECOSIMCONCEPT:Unit ! unit

[Term]
id: ECOSIM:oC
name: oC
is_a: ECOSIMCONCEPT:Unit ! unit

[Term]
id: ECOSIM:pftPlantPopulation
name: plant population
is_a: ECOSIM:CATEGORYCanopyStructure ! category - canopy structure
relationship: has_unit ECOSIM:d-2 ! d-2

[Term]
id: ECOSIM:sh-1
name: s h-1
is_a: ECOSIMCONCEPT:Unit ! unit

[Term]
id: ECOSIM:sm-1
name: s m-1
is_a: ECOSIMCONCEPT:Unit ! unit

[Term]
id: ECOSIM:trcSalt_RFLU
name: aqueous PO4 in underground irrigation non-band
def: "Aqueous PO4 in underground irrigation non-band refers to the concentration of dissolved phosphate (PO4) in water used for irrigation that is applied underground and not in a specific band pattern. This parameter is typically used in earth system models to simulate nutrient dynamics and their impact on ecosystem functioning in agricultural systems. It represents the amount of phosphate available for plants in the irrigation water that is not concentrated in a specific area but distributed evenly underground." []
is_a: ECOSIMCONCEPT:UnclassifiedVariable ! unclassified variable
relationship: has_unit ECOSIM:gd-2h-1 ! g d-2 h-1

[Term]
id: ECOSIM:trcSalt_TR
name: total salt solute transformation non-band
def: "Total salt solute transformation non-band refers to the process of converting soluble salts in a non-band environment. This transformation occurs through chemical reactions, such as dissolution, precipitation, adsorption, and desorption, that occur outside of specific bands or zones. It accounts for the overall change in the concentration of dissolved salts in the system, excluding any changes that occur within distinct bands or localized areas." []
is_a: ECOSIM:CATEGORYElementFlux ! category - C and nutrient flux
is_a: ECOSIMCONCEPT:Variable ! variable
relationship: has_unit ECOSIM:mold-2h-1 ! mol d-2 h-1
relationship: measurement_of ECOSIMCONCEPT:Salt ! Salt

[Term]
id: ECOSIM:trcSalt_XFXS
name: total salt micropore-macropore transfer non-band
def: "Total salt micropore-macropore transfer refers to the movement or exchange of salt between the micropores and macropores in a system, excluding any specific band or direction of transfer. Micropores refer to very small-sized pores or channels within the system, while macropores indicate larger-sized pores or channels. The transfer of salt between these two types of pores influences the overall salt distribution and transport within the system being modeled." []
is_a: ECOSIM:CATEGORYElementFlux ! category - C and nutrient flux
relationship: has_unit ECOSIM:gd-2h-1 ! g d-2 h-1

[Term]
id: ECOSIM:trcSalt_XQR
name: total Al in runoff
def: "Total Al in runoff refers to the concentration or amount of aluminum (Al) that is present in the water runoff from a specific area of land. Aluminum can be released into runoff from natural sources, such as weathering of rocks and soils, as well as from anthropogenic activities, including mining, industrial processes, and agriculture. This parameter is important to monitor as it can have significant impacts on water quality, ecosystem health, and the overall functioning of aquatic systems." []
is_a: ECOSIMCONCEPT:UnclassifiedVariable ! unclassified variable
relationship: has_unit ECOSIM:mold-2h-1 ! mol d-2 h-1

[Term]
id: ECOSIM:trcSalt_XQS
name: total salt in snow drift
def: "The term 'total salt in snow drift' refers to the amount of salt contained in a snow drift. It specifically represents the sum of all types of salts present, such as sodium chloride (NaCl), magnesium chloride (MgCl2), calcium chloride (CaCl2), and others. This parameter is essential for understanding the impact of salt on snowpack properties, such as its density, melting rate, and water content. It is commonly used in Earth system models to simulate the effects of salting on snow accumulation and the subsequent release of salt into the environment during snowmelt." []
is_a: ECOSIMCONCEPT:UnclassifiedVariable ! unclassified variable
relationship: has_unit ECOSIM:mold-2h-1 ! mol d-2 h-1

[Term]
id: ECOSIM:trcSalt_solml
name: soil aqueous salt content micropre
def: "Soil aqueous salt content microre is a parameter that refers to the concentration of dissolved salts in the soil water. It represents the amount of salts present in the water content of the soil." []
is_a: ECOSIM:CATEGORYSoilSolution ! category - soil solution
relationship: has_unit ECOSIM:mold-2 ! mol d-2

[Term]
id: ECOSIM:trcg_RDFA
name: dissolution (+ve) - volatilization (-ve) gas flux in roots
def: "Dissolution (+ve) - volatilization (-ve) gas flux in roots refers to the process of gas exchange occurring in the root system of plants, where gases dissolved in the soil water are taken up by roots (positive flux) or gases are released from the roots into the surrounding soil atmosphere (negative flux). These fluxes are influenced by factors such as soil composition, root morphology, and environmental conditions, and play a role in the overall cycling of gases within the earth system." []
is_a: ECOSIMCONCEPT:UnclassifiedVariable ! unclassified variable
relationship: has_unit ECOSIM:gd-2h-1 ! g d-2 h-1

[Term]
id: ECOSIM:trcg_RFLA
name: gaseous tracer flux through roots
def: "Gaseous tracer flux through roots refers to the movement of gases, such as carbon dioxide or nitrogen dioxide, through the roots of plants. It represents the transport of these gases from the atmosphere into the soil or from the soil into the atmosphere, mediated by the root system. This parameter is important for understanding the exchange of greenhouse gases between the soil and the atmosphere and how vegetation influences carbon and nitrogen cycling in terrestrial ecosystems." []
is_a: ECOSIMCONCEPT:UnclassifiedVariable ! unclassified variable
relationship: has_unit ECOSIM:gd-2h-1 ! g d-2 h-1

[Term]
id: ECOSIM:trcg_TFLA
name: total internal root gas flux
def: "Total internal root gas flux refers to the movement of gases, such as oxygen (O2), carbon dioxide (CO2), and methane (CH4), within plant roots. It represents the sum of all gases exchanged between the plant roots and the surrounding soil or water. This parameter is important in Earth systems modeling as it helps to quantify the exchange of gases between the terrestrial biosphere and the atmosphere, impacting processes such as plant respiration, photosynthesis, and greenhouse gas emissions." []
is_a: ECOSIMCONCEPT:UnclassifiedVariable ! unclassified variable
is_a: ECOSIMCONCEPT:Variable ! variable
relationship: attribute ECOSIMCONCEPT:Flux ! Flux
relationship: has_unit ECOSIM:gd-2h-1 ! g d-2 h-1
relationship: measured_in ECOSIMCONCEPT:Root ! Root

[Term]
id: ECOSIM:trcg_TLP
name: total root internal gas flux
def: "Total root internal gas flux refers to the overall movement of gases within the root system of plants. It represents the collective exchange of gases, such as oxygen and carbon dioxide, between the roots and the surrounding soil. This parameter is important for understanding the transport of gases and their impact on root respiration, nutrient uptake, and soil gas composition in Earth system models." []
is_a: ECOSIM:CATEGORYRootPhysiology ! category - root physiology
is_a: ECOSIMCONCEPT:UnclassifiedVariable ! unclassified variable
relationship: attribute ECOSIMCONCEPT:Flux ! Flux
relationship: has_unit ECOSIM:gd-2h-1 ! g d-2 h-1
relationship: measured_in ECOSIMCONCEPT:Root ! Root
relationship: measurement_of ECOSIMCONCEPT:Gas ! Gas

[Term]
id: ECOSIM:trcg_XBLL
name: CO2 bubbling
def: "CO2 bubbling refers to the process of releasing carbon dioxide gas (CO2) trapped in a liquid medium, such as water or a solution, in the form of bubbles. This usually occurs when there is a higher concentration of dissolved CO2 in the liquid, and the gas is being released due to a decrease in pressure or an increase in temperature. In the context of Earth systems modeling, CO2 bubbling can be an important parameter to consider when simulating carbon cycles and the exchange of CO2 between different reservoirs, such as the atmosphere and oceans." []
is_a: ECOSIMCONCEPT:UnclassifiedVariable ! unclassified variable
relationship: has_unit ECOSIM:gd-2h-1 ! g d-2 h-1

[Term]
id: ECOSIM:trcg_XDFR
name: soil surface gas dissolution (+ve) - volatilization (-ve)
def: "Soil surface gas dissolution-volatilization refers to the process in which gases exchange between the soil surface and the atmosphere. This parameter describes the net movement of gases, with positive values indicating the dissolution of gases into the soil and negative values indicating the volatilization or release of gases from the soil surface into the atmosphere." []
is_a: ECOSIMCONCEPT:UnclassifiedVariable ! unclassified variable
relationship: has_unit ECOSIM:gd-2h-1 ! g d-2 h-1

[Term]
id: ECOSIM:trcg_XRS
name: surface runoff gas flux
def: "Surface runoff gas flux refers to the exchange of gases between the Earth's surface and water bodies due to the movement of water runoff over the land. It represents the release or absorption of gases such as carbon dioxide (CO2), methane (CH4), or nitrogen oxides (NOx) into or from the water bodies during the process of surface runoff. This parameter plays a crucial role in understanding and predicting the biogeochemical cycles of greenhouse gases and their impact on climate change." []
is_a: ECOSIMCONCEPT:Flux ! Flux
is_a: ECOSIMCONCEPT:UnclassifiedVariable ! unclassified variable
relationship: has_unit ECOSIM:gd-2h-1 ! g d-2 h-1
relationship: measured_in ECOSIMCONCEPT:SurfaceRunoff ! Surface runoff
relationship: measurement_of ECOSIMCONCEPT:Gas ! Gas

[Term]
id: ECOSIM:trcn_XRS
name: surface runoff nutrient flux
def: "Surface runoff nutrient flux refers to the movement of nutrients, such as nitrogen and phosphorus, from the land surface to water bodies through runoff water. It represents the amount of nutrients that are transported from the terrestrial ecosystem to aquatic systems, contributing to nutrient loading and potentially causing eutrophication. Surface runoff nutrient flux is influenced by various factors, including land use, soil properties, rainfall, and nutrient management practices." []
is_a: ECOSIMCONCEPT:UnclassifiedVariable ! unclassified variable
relationship: attribute ECOSIMCONCEPT:Flux ! Flux
relationship: has_unit ECOSIM:gd-2h-1 ! g d-2 h-1
relationship: measured_in ECOSIMCONCEPT:SurfaceRunoff ! Surface runoff
relationship: measurement_of ECOSIMCONCEPT:Nutrient ! Nutrient

[Term]
id: ECOSIM:trcn_irrig
name: subsurface irrigation nutrient concentration
def: "Subsurface irrigation nutrient concentration refers to the measurement or estimate of the amount of nutrients present in the water used for subsurface irrigation. It represents the concentration of essential nutrients, such as nitrogen, phosphorus, and potassium, in the irrigation water that is delivered directly to the plant root zone through underground pipes or tubes. This parameter is important in earth systems modeling as it affects plant growth and nutrient cycling in agricultural systems, and can have implications for water quality and environmental sustainability." []
is_a: ECOSIMCONCEPT:UnclassifiedVariable ! unclassified variable
relationship: attribute ECOSIMCONCEPT:Concentration ! Concentration
relationship: context ECOSIMCONCEPT:Irrigation ! Irrigation
relationship: has_unit ECOSIM:gm-3 ! g m-3
relationship: measured_in ECOSIMCONCEPT:Subsurface ! Subsurface
relationship: measurement_of ECOSIMCONCEPT:Nutrient ! Nutrient

[Term]
id: ECOSIM:trcp_ER
name: total adsorbed ALOH3 erosion
def: "Total adsorbed ALOH3 erosion refers to the amount of aluminum hydroxide (ALOH3) that is detached from the Earth's surface due to erosion processes and becomes adsorbed onto other materials or particles. This parameter quantifies the overall erosion of ALOH3 and provides insight into the transport and redistribution of this compound within the Earth system." []
is_a: ECOSIMCONCEPT:UnclassifiedVariable ! unclassified variable
relationship: has_unit ECOSIM:gd-2h-1 ! g d-2 h-1

[Term]
id: ECOSIM:trcp_TR
name: total precipitated P containing transformation non-band
def: "The term 'total precipitated P containing transformation non-band' refers to the amount of phosphorous (P) that is transformed and then deposited onto the Earth's surface in forms other than bands within a specified time period. This parameter is a component of earth system models and is used to quantify and simulate the cycling and distribution of phosphorous in terrestrial and aquatic ecosystems. It provides valuable information for understanding nutrient dynamics and their impact on ecosystem health and functioning." []
is_a: ECOSIMCONCEPT:UnclassifiedVariable ! unclassified variable
relationship: has_unit ECOSIM:mold-2h-1 ! mol d-2 h-1

[Term]
id: ECOSIM:trcs_RFLU
name: aqueous non-salt solutes in underground irrigation
def: "Aqueous non-salt solutes in underground irrigation refers to the presence of dissolved substances in groundwater used for irrigation purposes, excluding any salts. These solutes can include organic compounds, such as pesticides or fertilizers, as well as inorganic compounds such as heavy metals or trace elements. The presence of these solutes can affect the quality of the water and subsequently impact the soil, plants, and overall ecosystem dynamics in the irrigated area." []
is_a: ECOSIMCONCEPT:UnclassifiedVariable ! unclassified variable
relationship: has_unit ECOSIM:gd-2h-1 ! g d-2 h-1

[Term]
id: ECOSIM:trcs_XFXS
name: total non-salt solute micropore-macropore transfer
def: "Total non-salt solute micropore-macropore transfer refers to the movement or transfer of solute substances, excluding salt or non-saline components, between micropores and macropores within a system. Micropores are small-scale pores within the soil matrix, while macropores are larger-scale conduits such as root channels or preferential flow paths. This parameter quantifies the amount of solute transferred between these different pore types, which is important for understanding solute transport and distribution within the soil profile." []
is_a: ECOSIM:CATEGORYElementFlux ! category - C and nutrient flux
relationship: context ECOSIMCONCEPT:Macropore ! Macropore
relationship: context ECOSIMCONCEPT:Micropore ! Micropore
relationship: has_unit ECOSIM:gd-2h-1 ! g d-2 h-1
relationship: measurement_of ECOSIMCONCEPT:Solute ! Solute

[Term]
id: ECOSIM:trcx_TR
name: total adsorbed OH- transformation non-band
def: "Total adsorbed OH- transformation non-band refers to the overall quantity of hydroxide ions (OH-) that undergo transformation through adsorption (attachment to the surface) in a non-band region in a given Earth system. This parameter represents the cumulative amount of OH- transformations occurring outside specific band regions, such as oceanic areas with specific temperature, salinity, or other physical characteristics. It is a measure of the chemical reactions and exchanges involving OH- that take place within the Earth system, which can have implications for various biogeochemical processes." []
is_a: ECOSIMCONCEPT:UnclassifiedVariable ! unclassified variable
relationship: has_unit ECOSIM:mold-2h-1 ! mol d-2 h-1

[Term]
id: ECOSIM:trcx_XER
name: total adsorbed sediment erosion non-band
def: "Total adsorbed sediment erosion non-band refers to the amount of sediment that is eroded and transported by water, wind, or ice without forming distinct bands or channels. This parameter accounts for the erosion of sediment particles that have been adsorbed onto the surfaces of other particles or are not part of a well-defined sediment transport pathway. It quantifies the total volume or mass of sediment eroded from a given area or system, which includes both the suspended sediments and the sediments that are in contact with the bed or substrate." []
is_a: ECOSIMCONCEPT:UnclassifiedVariable ! unclassified variable
relationship: attribute ECOSIMCONCEPT:Erosion ! Erosion
relationship: has_unit ECOSIM:gd-2h-1 ! g d-2 h-1
relationship: measured_in ECOSIMCONCEPT:Sediment ! Sediment

[Term]
id: ECOSIM:uM
name: uM
is_a: ECOSIMCONCEPT:Unit ! unit

[Term]
id: ECOSIM:uM/umolmol-1
name: uM /umol mol-1
is_a: ECOSIMCONCEPT:Unit ! unit

[Term]
id: ECOSIM:umolg-1h-1at25oC
name: umol g-1 h-1 at 25 oC
is_a: ECOSIMCONCEPT:Unit ! unit

[Term]
id: ECOSIM:umolm-2s-1
name: umol m-2 s-1
is_a: ECOSIMCONCEPT:Unit ! unit

[Term]
id: ECOSIM:umolm-3
name: umol m-3
is_a: ECOSIMCONCEPT:Unit ! unit

[Term]
id: ECOSIM:umolmol-1
name: umol mol-1
is_a: ECOSIMCONCEPT:Unit ! unit

[Term]
id: ECOSIM:umolumol-1
name: umol umol-1
is_a: ECOSIMCONCEPT:Unit ! unit

[Term]
id: ECOSIMCONCEPT:ALOH3
name: ALOH3
is_a: ECOSIMCONCEPT:ChemicalEntity ! chemical entity

[Term]
id: ECOSIMCONCEPT:Acetate
name: Acetate
is_a: ECOSIMCONCEPT:ChemicalEntity ! chemical entity

[Term]
id: ECOSIMCONCEPT:Activity
name: Activity
def: "The rate of a process or action" []
is_a: ECOSIMCONCEPT:Attribute ! attribute

[Term]
id: ECOSIMCONCEPT:Air
name: Air
def: "The mixture of gases comprising the Earth's atmosphere," []
is_a: ECOSIMCONCEPT:PhysicalEntity ! physical entity

[Term]
id: ECOSIMCONCEPT:Al
name: Aluminum
def: "A metallic chemical element with symbol Al and atomic number 13," []
is_a: ECOSIMCONCEPT:ChemicalEntity ! chemical entity

[Term]
id: ECOSIMCONCEPT:AlOH
name: Aluminum hydroxide
def: "An inorganic compound with the formula Al(OH)3," []
is_a: ECOSIMCONCEPT:ChemicalEntity ! chemical entity

[Term]
id: ECOSIMCONCEPT:AlOH2
name: Aluminum dihydroxide
def: "A chemical compound with formula Al(OH)2, " []
is_a: ECOSIMCONCEPT:MaterialEntity ! material entity

[Term]
id: ECOSIMCONCEPT:AlOH3
name: Aluminum trihydroxide
def: "A chemical compound with formula Al(OH)3," []
is_a: ECOSIMCONCEPT:ChemicalEntity ! chemical entity

[Term]
id: ECOSIMCONCEPT:AlOH4
name: Aluminum tetrahydroxide
def: "A chemical compound with formula Al(OH)4," []
is_a: ECOSIMCONCEPT:ChemicalEntity ! chemical entity

[Term]
id: ECOSIMCONCEPT:AlPO4
name: AlPO4
is_a: ECOSIMCONCEPT:ChemicalEntity ! chemical entity

[Term]
id: ECOSIMCONCEPT:AlSO4
name: Aluminum sulfate
def: "A chemical compound with the formula Al2(SO4)3," []
is_a: ECOSIMCONCEPT:ChemicalEntity ! chemical entity

[Term]
id: ECOSIMCONCEPT:Altitude
name: Altitude
is_a: ECOSIMCONCEPT:Attribute ! attribute

[Term]
id: ECOSIMCONCEPT:Aluminium
name: Aluminium
is_a: ECOSIMCONCEPT:ChemicalEntity ! chemical entity

[Term]
id: ECOSIMCONCEPT:Aluminum
name: Aluminum
is_a: ECOSIMCONCEPT:ChemicalEntity ! chemical entity

[Term]
id: ECOSIMCONCEPT:Ammonia
name: Ammonia
is_a: ECOSIMCONCEPT:ChemicalEntity ! chemical entity

[Term]
id: ECOSIMCONCEPT:Ammonium
name: Ammonium
def: "A positively charged polyatomic ion with the chemical formula NH4+," []
is_a: ECOSIMCONCEPT:ChemicalEntity ! chemical entity

[Term]
id: ECOSIMCONCEPT:AmmoniumUptake
name: Ammonium uptake
def: "The process by which ammonium ions are absorbed from the soil by plant roots," []
is_a: ECOSIMCONCEPT:Process ! process

[Term]
id: ECOSIMCONCEPT:AmmoniumUptakeRate
name: Ammonium uptake rate
def: "The rate at which ammonium ions are absorbed from the soil by plant roots," []
is_a: ECOSIMCONCEPT:Process ! process

[Term]
id: ECOSIMCONCEPT:Apatite
name: Apatite
is_a: ECOSIMCONCEPT:ChemicalEntity ! chemical entity

[Term]
id: ECOSIMCONCEPT:Aqueous
name: Aqueous
def: "Of, relating to, or resembling water," []
is_a: ECOSIMCONCEPT:PhysicalEntity ! physical entity

[Term]
id: ECOSIMCONCEPT:Area
name: Area
is_a: ECOSIMCONCEPT:Attribute ! attribute

[Term]
id: ECOSIMCONCEPT:Atmosphere
name: Atmosphere
def: "The envelope of gases surrounding the earth or another planet," []
is_a: ECOSIMCONCEPT:PhysicalEntity ! physical entity

[Term]
id: ECOSIMCONCEPT:AtmosphericPrecipitation
name: AtmosphericPrecipitation
is_a: ECOSIMCONCEPT:PhysicalEntity ! physical entity

[Term]
id: ECOSIMCONCEPT:Attribute
name: attribute
subset: upper_level

[Term]
id: ECOSIMCONCEPT:Bacteria
name: Bacteria
def: "Microscopic unicellular organisms, typically having cell walls but lacking organelles and an organized nucleus," []
is_a: ECOSIMCONCEPT:Organismal ! organismal

[Term]
id: ECOSIMCONCEPT:Band
name: Band
is_a: ECOSIMCONCEPT:PhysicalEntity ! physical entity

[Term]
id: ECOSIMCONCEPT:Bicarbonate
name: Bicarbonate
is_a: ECOSIMCONCEPT:ChemicalEntity ! chemical entity

[Term]
id: ECOSIMCONCEPT:BoundaryLayer
name: BoundaryLayer
is_a: ECOSIMCONCEPT:PhysicalEntity ! physical entity

[Term]
id: ECOSIMCONCEPT:BoundaryLayerOfCanopy
name: BoundaryLayerOfCanopy
is_a: ECOSIMCONCEPT:PhysicalEntity ! physical entity

[Term]
id: ECOSIMCONCEPT:Branch
name: Branch
def: "A woody part of a tree arising from the trunk and dividing into limbs and smaller branches," []
is_a: ECOSIMCONCEPT:Organismal ! organismal

[Term]
id: ECOSIMCONCEPT:BranchElement
name: Branch element
def: "A modeled branch component in a plant or tree," []
is_a: ECOSIMCONCEPT:Organismal ! organismal

[Term]
id: ECOSIMCONCEPT:BranchHusk
name: Branch husk
def: "The outer protective layer of a branch," []
is_a: ECOSIMCONCEPT:Organismal ! organismal

[Term]
id: ECOSIMCONCEPT:BranchLeaf
name: BranchLeaf
is_a: ECOSIMCONCEPT:PlantPart ! plant part

[Term]
id: ECOSIMCONCEPT:BranchLeafElement
name: Branch leaf element
def: "The modeled leaf component attached to a branch element," []
is_a: ECOSIMCONCEPT:Organismal ! organismal

[Term]
id: ECOSIMCONCEPT:BranchPlusStalk
name: Branch plus stalk
def: "The modeled branch and stalk biomass in crops," []
is_a: ECOSIMCONCEPT:Organismal ! organismal

[Term]
id: ECOSIMCONCEPT:BranchSheath
name: BranchSheath
is_a: ECOSIMCONCEPT:MaterialEntity ! material entity

[Term]
id: ECOSIMCONCEPT:BranchShoot
name: Branch shoot
def: "The above-ground woody portion of a branch with leaves and reproductive structures," []
is_a: ECOSIMCONCEPT:Organismal ! organismal

[Term]
id: ECOSIMCONCEPT:BranchStalk
name: BranchStalk
is_a: ECOSIMCONCEPT:PlantPart ! plant part

[Term]
id: ECOSIMCONCEPT:BundleSheathCell
name: BundleSheathCell
is_a: ECOSIMCONCEPT:PlantPart ! plant part

[Term]
id: ECOSIMCONCEPT:C3Compound
name: C3Compound
is_a: ECOSIMCONCEPT:MaterialEntity ! material entity

[Term]
id: ECOSIMCONCEPT:C4
name: C4
is_a: ECOSIMCONCEPT:MaterialEntity ! material entity

[Term]
id: ECOSIMCONCEPT:C4Carboxylation
name: C4 carboxylation
def: "The enzymatic addition of carbon dioxide to a C4 organic compound," []
is_a: ECOSIMCONCEPT:Process ! process

[Term]
id: ECOSIMCONCEPT:C4CarboxylationRate
name: C4 carboxylation rate
def: "The rate at which carbon dioxide is enzymatically added to C4 organic compounds," []
is_a: ECOSIMCONCEPT:Process ! process

[Term]
id: ECOSIMCONCEPT:C4Photosynthesis
name: C4Photosynthesis
is_a: ECOSIMCONCEPT:Process ! process

[Term]
id: ECOSIMCONCEPT:CH4
name: Methane
def: "A colorless, odorless gas with chemical formula CH4, the main component of natural gas," []
is_a: ECOSIMCONCEPT:ChemicalEntity ! chemical entity

[Term]
id: ECOSIMCONCEPT:CHPO4
name: Calcium hydrogen phosphate
def: "A calcium phosphate mineral with formula CaHPO4," []
is_a: ECOSIMCONCEPT:ChemicalEntity ! chemical entity

[Term]
id: ECOSIMCONCEPT:CNRatio
name: CNRatio
is_a: ECOSIMCONCEPT:PhysicalEntity ! physical entity

[Term]
id: ECOSIMCONCEPT:CO2
name: Carbon dioxide
def: "A colorless, odorless gas with chemical formula CO2," []
is_a: ECOSIMCONCEPT:ChemicalEntity ! chemical entity

[Term]
id: ECOSIMCONCEPT:CO2CarboxylationRate
name: Carbon dioxide carboxylation rate
def: "The rate at which carbon dioxide is enzymatically added to organic compounds by rubisco," []
is_a: ECOSIMCONCEPT:Process ! process

[Term]
id: ECOSIMCONCEPT:CO2Concentration
name: CO2Concentration
is_a: ECOSIMCONCEPT:Attribute ! attribute

[Term]
id: ECOSIMCONCEPT:CO2Fixation
name: CO2Fixation
is_a: ECOSIMCONCEPT:Process ! process

[Term]
id: ECOSIMCONCEPT:CO3
name: Carbonate
def: "A carbon oxoanion with chemical formula CO3(2-)," []
is_a: ECOSIMCONCEPT:ChemicalEntity ! chemical entity

[Term]
id: ECOSIMCONCEPT:Ca
name: Calcium
def: "A chemical element with symbol Ca and atomic number 20," []
is_a: ECOSIMCONCEPT:ChemicalEntity ! chemical entity

[Term]
id: ECOSIMCONCEPT:Ca-NaSelection
name: Ca-NaSelection
is_a: ECOSIMCONCEPT:Process ! process

[Term]
id: ECOSIMCONCEPT:CaCO3
name: Calcium carbonate
def: "A chemical compound with formula CaCO3," []
is_a: ECOSIMCONCEPT:ChemicalEntity ! chemical entity

[Term]
id: ECOSIMCONCEPT:CaH2PO4
name: Calcium dihydrogen phosphate
def: "An inorganic compound with the formula Ca(H2PO4)2, " []
is_a: ECOSIMCONCEPT:ChemicalEntity ! chemical entity

[Term]
id: ECOSIMCONCEPT:CaHCO3
name: Calcium bicarbonate
def: "A chemical compound with formula Ca(HCO3)2," []
is_a: ECOSIMCONCEPT:MaterialEntity ! material entity

[Term]
id: ECOSIMCONCEPT:CaHPO4
name: CaHPO4
is_a: ECOSIMCONCEPT:ChemicalEntity ! chemical entity

[Term]
id: ECOSIMCONCEPT:CaOH
name: Calcium hydroxide
def: "An inorganic compound with the chemical formula Ca(OH)2," []
is_a: ECOSIMCONCEPT:ChemicalEntity ! chemical entity

[Term]
id: ECOSIMCONCEPT:CaPO4
name: Calcium phosphate
def: "An umbrella term for a group of minerals containing calcium and phosphate," []
is_a: ECOSIMCONCEPT:ChemicalEntity ! chemical entity

[Term]
id: ECOSIMCONCEPT:CaSO4
name: Calcium sulfate
def: "A chemical compound with the formula CaSO4," []
is_a: ECOSIMCONCEPT:ChemicalEntity ! chemical entity

[Term]
id: ECOSIMCONCEPT:Calcium
name: Calcium
is_a: ECOSIMCONCEPT:MaterialEntity ! material entity

[Term]
id: ECOSIMCONCEPT:Canopy
name: Canopy
def: "The uppermost layer of vegetation in a forest or crop," []
is_a: ECOSIMCONCEPT:Organismal ! organismal

[Term]
id: ECOSIMCONCEPT:CanopyBranch
name: CanopyBranch
is_a: ECOSIMCONCEPT:PlantPart ! plant part

[Term]
id: ECOSIMCONCEPT:CanopyLayer
name: CanopyLayer
is_a: ECOSIMCONCEPT:PhysicalEntity ! physical entity

[Term]
id: ECOSIMCONCEPT:CanopyNodule
name: CanopyNodule
is_a: ECOSIMCONCEPT:Organismal ! organismal

[Term]
id: ECOSIMCONCEPT:CanopyPlant
name: CanopyPlant
is_a: ECOSIMCONCEPT:Organismal ! organismal

[Term]
id: ECOSIMCONCEPT:CanopyShoot
name: CanopyShoot
is_a: ECOSIMCONCEPT:Organismal ! organismal

[Term]
id: ECOSIMCONCEPT:CanopyShootCarbon
name: Canopy shoot carbon
def: "The carbon in the above-ground portion of the plant canopy," []
is_a: ECOSIMCONCEPT:PhysicalEntity ! physical entity

[Term]
id: ECOSIMCONCEPT:Carbon
name: Carbon
def: "A chemical element with symbol C and atomic number 6," []
is_a: ECOSIMCONCEPT:Attribute ! attribute
is_a: ECOSIMCONCEPT:ChemicalEntity ! chemical entity

[Term]
id: ECOSIMCONCEPT:CarbonDioxide
name: CarbonDioxide
is_a: ECOSIMCONCEPT:ChemicalEntity ! chemical entity

[Term]
id: ECOSIMCONCEPT:CarbonDioxideConcentrationInAir
name: CarbonDioxideConcentrationInAir
is_a: ECOSIMCONCEPT:Attribute ! attribute

[Term]
id: ECOSIMCONCEPT:CarbonDioxideConcentrationInInterCellularAir
name: CarbonDioxideConcentrationInInterCellularAir
is_a: ECOSIMCONCEPT:Attribute ! attribute

[Term]
id: ECOSIMCONCEPT:CarbonNitrogenRatio
name: CarbonNitrogenRatio
is_a: ECOSIMCONCEPT:PhysicalEntity ! physical entity

[Term]
id: ECOSIMCONCEPT:CarbonPhosphorusRatio
name: CarbonPhosphorusRatio
is_a: ECOSIMCONCEPT:PhysicalEntity ! physical entity

[Term]
id: ECOSIMCONCEPT:CarboxylaseActivity
name: Carboxylase activity
def: "The catalytic activity of enzymes that add carbon dioxide to organic substrates," []
is_a: ECOSIMCONCEPT:Process ! process

[Term]
id: ECOSIMCONCEPT:Carboxylation
name: Carboxylation
is_a: ECOSIMCONCEPT:Process ! process

[Term]
id: ECOSIMCONCEPT:Ch4Emission
name: Methane emission
def: "The release of methane gas into the atmosphere," []
is_a: ECOSIMCONCEPT:Process ! process

[Term]
id: ECOSIMCONCEPT:ChemicalEntity
name: chemical entity
subset: upper_level
is_a: ECOSIMCONCEPT:MaterialEntity ! material entity

[Term]
id: ECOSIMCONCEPT:Chloride
name: Chloride
is_a: ECOSIMCONCEPT:ChemicalEntity ! chemical entity

[Term]
id: ECOSIMCONCEPT:Chlorophyll
name: Chlorophyll
is_a: ECOSIMCONCEPT:ChemicalEntity ! chemical entity

[Term]
id: ECOSIMCONCEPT:Cl
name: Chlorine
def: "A chemical element with symbol Cl and atomic number 17, " []
is_a: ECOSIMCONCEPT:ChemicalEntity ! chemical entity

[Term]
id: ECOSIMCONCEPT:Clay
name: Clay
def: "A stiff, sticky fine-grained earth," []
is_a: ECOSIMCONCEPT:PhysicalEntity ! physical entity

[Term]
id: ECOSIMCONCEPT:Clumping
name: Clumping
is_a: ECOSIMCONCEPT:Attribute ! attribute

[Term]
id: ECOSIMCONCEPT:Coefficient
name: Coefficient
is_a: ECOSIMCONCEPT:Attribute ! attribute

[Term]
id: ECOSIMCONCEPT:ColdRequirement
name: Cold requirement
def: "The amount of cold temperature exposure needed for a plant process" []
is_a: ECOSIMCONCEPT:Attribute ! attribute

[Term]
id: ECOSIMCONCEPT:Concentration
name: Concentration
def: "The relative amount of a substance mixed with another substance" []
is_a: ECOSIMCONCEPT:Attribute ! attribute

[Term]
id: ECOSIMCONCEPT:Constraint
name: Constraint
def: "A limitation or restriction" []
is_a: ECOSIMCONCEPT:Attribute ! attribute

[Term]
id: ECOSIMCONCEPT:Content
name: Content
def: "The amount contained" []
is_a: ECOSIMCONCEPT:Attribute ! attribute

[Term]
id: ECOSIMCONCEPT:Context
name: context
subset: upper_level

[Term]
id: ECOSIMCONCEPT:ConvectiveHeat
name: ConvectiveHeat
is_a: ECOSIMCONCEPT:PhysicalEntity ! physical entity

[Term]
id: ECOSIMCONCEPT:Cotyledon
name: Cotyledon
is_a: ECOSIMCONCEPT:PlantPart ! plant part

[Term]
id: ECOSIMCONCEPT:Critical
name: Critical
def: "Of the highest importance" []
is_a: ECOSIMCONCEPT:Attribute ! attribute

[Term]
id: ECOSIMCONCEPT:DIC
name: Dissolved inorganic carbon
def: "Carbon dioxide and bicarbonate and carbonate ions dissolved in water," []
is_a: ECOSIMCONCEPT:PhysicalEntity ! physical entity

[Term]
id: ECOSIMCONCEPT:DIP
name: Dissolved inorganic phosphorus
def: "Orthophosphate ions dissolved in water," []
is_a: ECOSIMCONCEPT:PhysicalEntity ! physical entity

[Term]
id: ECOSIMCONCEPT:DOC
name: DOC
is_a: ECOSIMCONCEPT:PhysicalEntity ! physical entity

[Term]
id: ECOSIMCONCEPT:DON
name: DON
is_a: ECOSIMCONCEPT:PhysicalEntity ! physical entity

[Term]
id: ECOSIMCONCEPT:DOP
name: Dissolved organic phosphorus
def: "Phosphorus bound in dissolved organic matter in water," []
is_a: ECOSIMCONCEPT:PhysicalEntity ! physical entity

[Term]
id: ECOSIMCONCEPT:Day
name: Day
is_a: ECOSIMCONCEPT:Process ! process

[Term]
id: ECOSIMCONCEPT:DeadStandingTree
name: DeadStandingTree
is_a: ECOSIMCONCEPT:Plant ! Plant

[Term]
id: ECOSIMCONCEPT:DeadTree
name: Dead tree
def: "A non-living tree," []
is_a: ECOSIMCONCEPT:Organismal ! organismal

[Term]
id: ECOSIMCONCEPT:Dehardening
name: Dehardening
is_a: ECOSIMCONCEPT:Process ! process

[Term]
id: ECOSIMCONCEPT:Deposition
name: Deposition
def: "The accumulation of material on a surface" []
is_a: ECOSIMCONCEPT:Attribute ! attribute

[Term]
id: ECOSIMCONCEPT:Depth
name: Depth
def: "Vertical distance below a surface" []
is_a: ECOSIMCONCEPT:Attribute ! attribute

[Term]
id: ECOSIMCONCEPT:Diffusivity
name: Diffusivity
def: "The rate at which particles spread through a medium" []
is_a: ECOSIMCONCEPT:Attribute ! attribute

[Term]
id: ECOSIMCONCEPT:Dissolution
name: Dissolution
def: "The process of dissolving a solid into a liquid" []
is_a: ECOSIMCONCEPT:Attribute ! attribute

[Term]
id: ECOSIMCONCEPT:DissolutionVolatilization
name: Dissolution volatilization
def: "The dissolution and volatilization transfer processes\" " []
is_a: ECOSIMCONCEPT:Attribute ! attribute

[Term]
id: ECOSIMCONCEPT:DissolvedInorganicNitrogen
name: Dissolved inorganic nitrogen
def: "Nitrogen species such as nitrate, nitrite and ammonium ions dissolved in water," []
is_a: ECOSIMCONCEPT:PhysicalEntity ! physical entity

[Term]
id: ECOSIMCONCEPT:DissolvedOrganicCarbon
name: Dissolved organic carbon
def: "Organic carbon dissolved in water, " []
is_a: ECOSIMCONCEPT:PhysicalEntity ! physical entity

[Term]
id: ECOSIMCONCEPT:DissolvedOrganicNitrogen
name: Dissolved organic nitrogen
def: "Organically bound nitrogen dissolved in water," []
is_a: ECOSIMCONCEPT:PhysicalEntity ! physical entity

[Term]
id: ECOSIMCONCEPT:DissolvedOrganicPhosphoros
name: DissolvedOrganicPhosphoros
is_a: ECOSIMCONCEPT:PhysicalEntity ! physical entity

[Term]
id: ECOSIMCONCEPT:DissolvedOrganicPhosphorus
name: DissolvedOrganicPhosphorus
is_a: ECOSIMCONCEPT:PhysicalEntity ! physical entity

[Term]
id: ECOSIMCONCEPT:Drainage
name: Drainage
def: "The outflow of water from an area" []
is_a: ECOSIMCONCEPT:Attribute ! attribute

[Term]
id: ECOSIMCONCEPT:Duration
name: Duration
def: "The time period over which something continues" []
is_a: ECOSIMCONCEPT:Attribute ! attribute

[Term]
id: ECOSIMCONCEPT:Ear
name: Ear
def: "The seed-bearing spike of a cereal plant," []
is_a: ECOSIMCONCEPT:Organismal ! organismal

[Term]
id: ECOSIMCONCEPT:EarthSurface
name: EarthSurface
is_a: ECOSIMCONCEPT:PhysicalEntity ! physical entity

[Term]
id: ECOSIMCONCEPT:Ecosystem
name: Ecosystem
def: "A biological community of interacting living organisms and their physical environment," []
is_a: ECOSIMCONCEPT:MaterialEntity ! material entity

[Term]
id: ECOSIMCONCEPT:Element
name: Element
def: "A component or constituent of a whole" []
is_a: ECOSIMCONCEPT:Attribute ! attribute
is_a: ECOSIMCONCEPT:PhysicalEntity ! physical entity

[Term]
id: ECOSIMCONCEPT:Emission
name: Emission
def: "The release of something, such as gas or radiation" []
is_a: ECOSIMCONCEPT:Attribute ! attribute

[Term]
id: ECOSIMCONCEPT:Energy
name: Energy
is_a: ECOSIMCONCEPT:PhysicalEntity ! physical entity

[Term]
id: ECOSIMCONCEPT:EnvironmentalEntity
name: environmental entity
subset: upper_level
is_a: ECOSIMCONCEPT:MaterialEntity ! material entity

[Term]
id: ECOSIMCONCEPT:Enzyme
name: Enzyme
def: "A protein that catalyzes chemical reactions," []
is_a: ECOSIMCONCEPT:ChemicalEntity ! chemical entity

[Term]
id: ECOSIMCONCEPT:Erosion
name: Erosion
is_a: ECOSIMCONCEPT:Process ! process

[Term]
id: ECOSIMCONCEPT:ErosionBand
name: ErosionBand
is_a: ECOSIMCONCEPT:PhysicalEntity ! physical entity

[Term]
id: ECOSIMCONCEPT:ErosionRate
name: Erosion rate
def: "The speed at which erosion is occurring" []
is_a: ECOSIMCONCEPT:Attribute ! attribute

[Term]
id: ECOSIMCONCEPT:Evaporation
name: Evaporation
def: "The conversion of liquid water to water vapor" []
is_a: ECOSIMCONCEPT:Attribute ! attribute
is_a: ECOSIMCONCEPT:Process ! process

[Term]
id: ECOSIMCONCEPT:Evapotranspiration
name: Evapotranspiration
is_a: ECOSIMCONCEPT:Process ! process

[Term]
id: ECOSIMCONCEPT:Exchange
name: Exchange
def: "The act of giving or taking one thing in return for another" []
is_a: ECOSIMCONCEPT:Attribute ! attribute

[Term]
id: ECOSIMCONCEPT:F1PR
name: F1PR
is_a: ECOSIMCONCEPT:ChemicalEntity ! chemical entity

[Term]
id: ECOSIMCONCEPT:Fe
name: Iron
def: "A metallic chemical element with symbol Fe and atomic number 26," []
is_a: ECOSIMCONCEPT:ChemicalEntity ! chemical entity

[Term]
id: ECOSIMCONCEPT:FeH2PO4
name: Iron dihydrogen phosphate
def: "An inorganic compound with the formula Fe(H2PO4)2," []
is_a: ECOSIMCONCEPT:ChemicalEntity ! chemical entity

[Term]
id: ECOSIMCONCEPT:FeHPO4
name: Iron hydrogen phosphate
def: "An inorganic compound with the formula FeHPO4," []
is_a: ECOSIMCONCEPT:MaterialEntity ! material entity

[Term]
id: ECOSIMCONCEPT:FeOH
name: Iron hydroxide
def: "An inorganic compound with the formula FeOH," []
is_a: ECOSIMCONCEPT:ChemicalEntity ! chemical entity

[Term]
id: ECOSIMCONCEPT:FeOH2
name: Iron dihydroxide
def: "An inorganic compound with the formula Fe(OH)2,  " []
is_a: ECOSIMCONCEPT:ChemicalEntity ! chemical entity

[Term]
id: ECOSIMCONCEPT:FeOH3
name: Iron trihydroxide
def: "An inorganic compound with the formula Fe(OH)3," []
is_a: ECOSIMCONCEPT:ChemicalEntity ! chemical entity

[Term]
id: ECOSIMCONCEPT:FeOH4
name: Iron tetrahydroxide
def: "An inorganic compound with the formula Fe(OH)4," []
is_a: ECOSIMCONCEPT:ChemicalEntity ! chemical entity

[Term]
id: ECOSIMCONCEPT:FePO4
name: FePO4
is_a: ECOSIMCONCEPT:ChemicalEntity ! chemical entity

[Term]
id: ECOSIMCONCEPT:FeSO4
name: Iron sulfate
def: "A chemical compound with formula FeSO4," []
is_a: ECOSIMCONCEPT:ChemicalEntity ! chemical entity

[Term]
id: ECOSIMCONCEPT:Fertilizer
name: Fertilizer
is_a: ECOSIMCONCEPT:PhysicalEntity ! physical entity

[Term]
id: ECOSIMCONCEPT:FertilizerApplication
name: FertilizerApplication
is_a: ECOSIMCONCEPT:Process ! process

[Term]
id: ECOSIMCONCEPT:FertilizerNH4
name: FertilizerNH4
is_a: ECOSIMCONCEPT:PhysicalEntity ! physical entity

[Term]
id: ECOSIMCONCEPT:Field
name: Field
is_a: ECOSIMCONCEPT:PhysicalEntity ! physical entity

[Term]
id: ECOSIMCONCEPT:FieldCapacityWiltingPoint
name: FieldCapacityWiltingPoint
is_a: ECOSIMCONCEPT:Attribute ! attribute

[Term]
id: ECOSIMCONCEPT:Fire
name: Fire
def: "The rapid oxidation of combustible material releasing heat, light and various reaction products," []
is_a: ECOSIMCONCEPT:Process ! process

[Term]
id: ECOSIMCONCEPT:Flux
name: Flux
def: "The rate of flow of a quantity" []
is_a: ECOSIMCONCEPT:Attribute ! attribute
is_a: ECOSIMCONCEPT:PhysicalEntity ! physical entity

[Term]
id: ECOSIMCONCEPT:Fraction
name: Fraction
is_a: ECOSIMCONCEPT:Attribute ! attribute

[Term]
id: ECOSIMCONCEPT:Gas
name: Gas
is_a: ECOSIMCONCEPT:PhysicalEntity ! physical entity

[Term]
id: ECOSIMCONCEPT:GasFlux
name: GasFlux
is_a: ECOSIMCONCEPT:PhysicalEntity ! physical entity

[Term]
id: ECOSIMCONCEPT:GaseousN2O
name: GaseousN2O
is_a: ECOSIMCONCEPT:ChemicalEntity ! chemical entity

[Term]
id: ECOSIMCONCEPT:Genome
name: Genome
is_a: ECOSIMCONCEPT:PhysicalEntity ! physical entity

[Term]
id: ECOSIMCONCEPT:Geometry
name: Geometry
is_a: ECOSIMCONCEPT:Attribute ! attribute

[Term]
id: ECOSIMCONCEPT:Grain
name: Grain
def: "The edible seed of a cereal grass," []
is_a: ECOSIMCONCEPT:Organismal ! organismal

[Term]
id: ECOSIMCONCEPT:GrainElement
name: GrainElement
is_a: ECOSIMCONCEPT:PlantPart ! plant part

[Term]
id: ECOSIMCONCEPT:GrainGrowth
name: GrainGrowth
is_a: ECOSIMCONCEPT:Process ! process

[Term]
id: ECOSIMCONCEPT:GrainNumber
name: GrainNumber
is_a: ECOSIMCONCEPT:Attribute ! attribute

[Term]
id: ECOSIMCONCEPT:Grid
name: Grid
is_a: ECOSIMCONCEPT:PhysicalEntity ! physical entity

[Term]
id: ECOSIMCONCEPT:GridCell
name: GridCell
is_a: ECOSIMCONCEPT:PhysicalEntity ! physical entity

[Term]
id: ECOSIMCONCEPT:GridLayer
name: GridLayer
is_a: ECOSIMCONCEPT:PhysicalEntity ! physical entity

[Term]
id: ECOSIMCONCEPT:GroundSurface
name: Ground surface
def: "The uppermost layer of the land surface," []
is_a: ECOSIMCONCEPT:PhysicalEntity ! physical entity

[Term]
id: ECOSIMCONCEPT:Growth
name: Growth
is_a: ECOSIMCONCEPT:Process ! process

[Term]
id: ECOSIMCONCEPT:H
name: Hydrogen
def: "A chemical element with symbol H and atomic number 1," []
is_a: ECOSIMCONCEPT:ChemicalEntity ! chemical entity

[Term]
id: ECOSIMCONCEPT:H2
name: Dihydrogen
def: "A gas with the formula H2," []
is_a: ECOSIMCONCEPT:ChemicalEntity ! chemical entity

[Term]
id: ECOSIMCONCEPT:H2O
name: H2O
is_a: ECOSIMCONCEPT:ChemicalEntity ! chemical entity

[Term]
id: ECOSIMCONCEPT:H2PO4
name: Dihydrogen phosphate
def: "An oxoanion with the chemical formula H2PO4-," []
is_a: ECOSIMCONCEPT:ChemicalEntity ! chemical entity

[Term]
id: ECOSIMCONCEPT:H3PO4
name: Phosphoric acid
def: "An inorganic compound with the chemical formula H3PO4," []
is_a: ECOSIMCONCEPT:ChemicalEntity ! chemical entity

[Term]
id: ECOSIMCONCEPT:HCO3
name: Bicarbonate
def: "An oxoanion with the chemical formula HCO3-," []
is_a: ECOSIMCONCEPT:ChemicalEntity ! chemical entity

[Term]
id: ECOSIMCONCEPT:HPO4
name: Hydrogen phosphate
def: "An oxoanion with the chemical formula HPO42-," []
is_a: ECOSIMCONCEPT:ChemicalEntity ! chemical entity

[Term]
id: ECOSIMCONCEPT:HalfSaturationConstant
name: Half saturation constant
def: "The concentration at which a reaction rate is half its maximum" []
is_a: ECOSIMCONCEPT:Attribute ! attribute

[Term]
id: ECOSIMCONCEPT:Harvest
name: Harvest
def: "The process of gathering a crop\" " []
is_a: ECOSIMCONCEPT:Attribute ! attribute
is_a: ECOSIMCONCEPT:Process ! process

[Term]
id: ECOSIMCONCEPT:Heat
name: Heat
is_a: ECOSIMCONCEPT:PhysicalEntity ! physical entity

[Term]
id: ECOSIMCONCEPT:HeatCapacity
name: Heat capacity
def: "The amount of heat energy required to change the temperature of an object" []
is_a: ECOSIMCONCEPT:Attribute ! attribute

[Term]
id: ECOSIMCONCEPT:HeatRequirement
name: HeatRequirement
is_a: ECOSIMCONCEPT:Attribute ! attribute

[Term]
id: ECOSIMCONCEPT:HeatTransfer
name: HeatTransfer
is_a: ECOSIMCONCEPT:Process ! process

[Term]
id: ECOSIMCONCEPT:Height
name: Height
def: "Vertical distance from bottom to top" []
is_a: ECOSIMCONCEPT:Attribute ! attribute

[Term]
id: ECOSIMCONCEPT:Humus
name: Humus
def: "The organic component of soil, formed by the decomposition of leaves and other plant material by soil microorganisms," []
is_a: ECOSIMCONCEPT:PhysicalEntity ! physical entity

[Term]
id: ECOSIMCONCEPT:Husk
name: Husk
def: "The dry external covering of certain fruits or seeds," []
is_a: ECOSIMCONCEPT:Organismal ! organismal

[Term]
id: ECOSIMCONCEPT:HuskElement
name: HuskElement
is_a: ECOSIMCONCEPT:PlantPart ! plant part

[Term]
id: ECOSIMCONCEPT:Hydrogen
name: Hydrogen
is_a: ECOSIMCONCEPT:ChemicalEntity ! chemical entity

[Term]
id: ECOSIMCONCEPT:HydrogenGas
name: HydrogenGas
is_a: ECOSIMCONCEPT:ChemicalEntity ! chemical entity

[Term]
id: ECOSIMCONCEPT:Hydroxide
name: Hydroxide
is_a: ECOSIMCONCEPT:ChemicalEntity ! chemical entity

[Term]
id: ECOSIMCONCEPT:Ice
name: Ice
def: "Frozen water," []
is_a: ECOSIMCONCEPT:PhysicalEntity ! physical entity

[Term]
id: ECOSIMCONCEPT:Internode
name: Internode
is_a: ECOSIMCONCEPT:PlantPart ! plant part

[Term]
id: ECOSIMCONCEPT:Ion
name: Ion
def: "An atom or molecule with a net electric charge," []
is_a: ECOSIMCONCEPT:PhysicalEntity ! physical entity

[Term]
id: ECOSIMCONCEPT:IonSelectivity
name: IonSelectivity
is_a: ECOSIMCONCEPT:MaterialEntity ! material entity

[Term]
id: ECOSIMCONCEPT:Ions
name: Ions
is_a: ECOSIMCONCEPT:PhysicalEntity ! physical entity

[Term]
id: ECOSIMCONCEPT:Iron
name: Iron
is_a: ECOSIMCONCEPT:ChemicalEntity ! chemical entity

[Term]
id: ECOSIMCONCEPT:Irrigation
name: Irrigation
is_a: ECOSIMCONCEPT:Process ! process

[Term]
id: ECOSIMCONCEPT:IrrigationWater
name: IrrigationWater
is_a: ECOSIMCONCEPT:PhysicalEntity ! physical entity

[Term]
id: ECOSIMCONCEPT:K
name: Potassium
def: "A chemical element with symbol K and atomic number 19," []
is_a: ECOSIMCONCEPT:ChemicalEntity ! chemical entity

[Term]
id: ECOSIMCONCEPT:KMValue
name: Km value
def: "The half saturation constant in Michaelis-Menten enzyme kinetics" []
is_a: ECOSIMCONCEPT:Attribute ! attribute

[Term]
id: ECOSIMCONCEPT:KSO4
name: Potassium sulfate
def: "An inorganic compound with formula K2SO4," []
is_a: ECOSIMCONCEPT:ChemicalEntity ! chemical entity

[Term]
id: ECOSIMCONCEPT:LAI
name: LAI
is_a: ECOSIMCONCEPT:Attribute ! attribute

[Term]
id: ECOSIMCONCEPT:LWRad
name: LWRad
is_a: ECOSIMCONCEPT:PhysicalEntity ! physical entity

[Term]
id: ECOSIMCONCEPT:LandSurface
name: LandSurface
is_a: ECOSIMCONCEPT:PhysicalEntity ! physical entity

[Term]
id: ECOSIMCONCEPT:Landscape
name: Landscape
is_a: ECOSIMCONCEPT:PhysicalEntity ! physical entity

[Term]
id: ECOSIMCONCEPT:LatentHeat
name: LatentHeat
is_a: ECOSIMCONCEPT:PhysicalEntity ! physical entity

[Term]
id: ECOSIMCONCEPT:Layer
name: Layer
is_a: ECOSIMCONCEPT:PhysicalEntity ! physical entity

[Term]
id: ECOSIMCONCEPT:Leaf
name: Leaf
def: "The flattened blade of a plant leaf," []
is_a: ECOSIMCONCEPT:Organismal ! organismal

[Term]
id: ECOSIMCONCEPT:LeafArea
name: LeafArea
is_a: ECOSIMCONCEPT:MaterialEntity ! material entity

[Term]
id: ECOSIMCONCEPT:LeafElement
name: Leaf element
def: "A modeled leaf component in a plant," []
is_a: ECOSIMCONCEPT:Organismal ! organismal

[Term]
id: ECOSIMCONCEPT:LeafNumber
name: LeafNumber
is_a: ECOSIMCONCEPT:Attribute ! attribute

[Term]
id: ECOSIMCONCEPT:LeafPlusSheath
name: LeafPlusSheath
is_a: ECOSIMCONCEPT:PlantPart ! plant part

[Term]
id: ECOSIMCONCEPT:LeafStructuralElement
name: LeafStructuralElement
is_a: ECOSIMCONCEPT:PlantPart ! plant part

[Term]
id: ECOSIMCONCEPT:Leafout
name: Leaf out
def: "The emergence and expansion of new leaves on plants in spring," []
is_a: ECOSIMCONCEPT:Process ! process

[Term]
id: ECOSIMCONCEPT:Litter
name: Litter
def: "Dead plant material such as leaves on the ground in a forest or woodland," []
is_a: ECOSIMCONCEPT:PhysicalEntity ! physical entity

[Term]
id: ECOSIMCONCEPT:Litterfall
name: Litterfall
def: "The falling of dead plant material such as leaves from trees to the forest floor," []
is_a: ECOSIMCONCEPT:Process ! process

[Term]
id: ECOSIMCONCEPT:LongwaveRadiation
name: LongwaveRadiation
is_a: ECOSIMCONCEPT:PhysicalEntity ! physical entity

[Term]
id: ECOSIMCONCEPT:Macropore
name: Macropore
def: "A large pore space between soil particles that facilitates water drainage and aeration," []
is_a: ECOSIMCONCEPT:PhysicalEntity ! physical entity

[Term]
id: ECOSIMCONCEPT:Magnesium
name: Magnesium
is_a: ECOSIMCONCEPT:ChemicalEntity ! chemical entity

[Term]
id: ECOSIMCONCEPT:Mass
name: Mass
def: "A measure of the amount of matter in an object" []
is_a: ECOSIMCONCEPT:Attribute ! attribute

[Term]
id: ECOSIMCONCEPT:MaterialEntity
name: material entity
subset: upper_level

[Term]
id: ECOSIMCONCEPT:MeltWater
name: MeltWater
is_a: ECOSIMCONCEPT:PhysicalEntity ! physical entity

[Term]
id: ECOSIMCONCEPT:Meltwater
name: Meltwater
def: "Water from melting snow or ice," []
is_a: ECOSIMCONCEPT:PhysicalEntity ! physical entity

[Term]
id: ECOSIMCONCEPT:MetabolicActivity
name: MetabolicActivity
is_a: ECOSIMCONCEPT:Process ! process

[Term]
id: ECOSIMCONCEPT:MetabolicRate
name: Metabolic rate
def: "The rate of energy conversion and use in an organism's cells\" " []
is_a: ECOSIMCONCEPT:Attribute ! attribute

[Term]
id: ECOSIMCONCEPT:Mg
name: Magnesium
def: "A chemical element with symbol Mg and atomic number 12," []
is_a: ECOSIMCONCEPT:MaterialEntity ! material entity

[Term]
id: ECOSIMCONCEPT:MgCO3
name: Magnesium carbonate
def: "A chemical compound with the formula MgCO3," []
is_a: ECOSIMCONCEPT:ChemicalEntity ! chemical entity

[Term]
id: ECOSIMCONCEPT:MgHCO3
name: Magnesium bicarbonate
def: "A chemical compound with the formula Mg(HCO3)2," []
is_a: ECOSIMCONCEPT:ChemicalEntity ! chemical entity

[Term]
id: ECOSIMCONCEPT:MgHPO4
name: Magnesium hydrogen phosphate
def: "A magnesium phosphate mineral with the formula MgHPO4," []
is_a: ECOSIMCONCEPT:ChemicalEntity ! chemical entity

[Term]
id: ECOSIMCONCEPT:MgOH
name: Magnesium hydroxide
def: "An inorganic compound with the formula Mg(OH)2," []
is_a: ECOSIMCONCEPT:ChemicalEntity ! chemical entity

[Term]
id: ECOSIMCONCEPT:MgSO4
name: Magnesium sulfate
def: "An inorganic compound with formula MgSO4, " []
is_a: ECOSIMCONCEPT:ChemicalEntity ! chemical entity

[Term]
id: ECOSIMCONCEPT:MichaelisConstant
name: Michaelis constant
def: "The substrate concentration at which enzyme reaction rate is half its maximum" []
is_a: ECOSIMCONCEPT:Attribute ! attribute

[Term]
id: ECOSIMCONCEPT:MicrobialBiomass
name: MicrobialBiomass
is_a: ECOSIMCONCEPT:PhysicalEntity ! physical entity

[Term]
id: ECOSIMCONCEPT:Micropore
name: Micropore
def: "A small pore space between soil particles that holds water by capillary forces," []
is_a: ECOSIMCONCEPT:Attribute ! attribute
is_a: ECOSIMCONCEPT:PhysicalEntity ! physical entity

[Term]
id: ECOSIMCONCEPT:MicroporeMacropore
name: MicroporeMacropore
is_a: ECOSIMCONCEPT:PhysicalEntity ! physical entity

[Term]
id: ECOSIMCONCEPT:Moisture
name: Moisture
is_a: ECOSIMCONCEPT:Attribute ! attribute

[Term]
id: ECOSIMCONCEPT:N2
name: Dinitrogen
def: "A colorless, odorless diatomic gas with the formula N2,  " []
is_a: ECOSIMCONCEPT:ChemicalEntity ! chemical entity

[Term]
id: ECOSIMCONCEPT:N2O
name: Nitrous oxide
def: "A potent greenhouse gas with formula N2O," []
is_a: ECOSIMCONCEPT:ChemicalEntity ! chemical entity

[Term]
id: ECOSIMCONCEPT:NH3
name: Ammonia
def: "A colorless gas with a characteristic pungent smell and formula NH3," []
is_a: ECOSIMCONCEPT:ChemicalEntity ! chemical entity

[Term]
id: ECOSIMCONCEPT:NH4
name: Ammonium
def: "A positively charged polyatomic ion with the chemical formula NH4+, " []
is_a: ECOSIMCONCEPT:ChemicalEntity ! chemical entity

[Term]
id: ECOSIMCONCEPT:NH4NH3
name: Ammonium/Ammonia
def: "The chemical species pair of ammonium (NH4+) and ammonia (NH3)," []
is_a: ECOSIMCONCEPT:ChemicalEntity ! chemical entity

[Term]
id: ECOSIMCONCEPT:NO2
name: Nitrogen dioxide
def: "A reddish-brown gas with formula NO2 that is a byproduct of combustion," []
is_a: ECOSIMCONCEPT:ChemicalEntity ! chemical entity

[Term]
id: ECOSIMCONCEPT:NO3
name: Nitrate
def: "An oxoanion with the chemical formula NO3-," []
is_a: ECOSIMCONCEPT:ChemicalEntity ! chemical entity

[Term]
id: ECOSIMCONCEPT:NO3Fertilizer
name: NO3Fertilizer
is_a: ECOSIMCONCEPT:PhysicalEntity ! physical entity

[Term]
id: ECOSIMCONCEPT:Na
name: Na
is_a: ECOSIMCONCEPT:ChemicalEntity ! chemical entity

[Term]
id: ECOSIMCONCEPT:NaCO3
name: NaCO3
is_a: ECOSIMCONCEPT:ChemicalEntity ! chemical entity

[Term]
id: ECOSIMCONCEPT:NaSO4
name: NaSO4
is_a: ECOSIMCONCEPT:ChemicalEntity ! chemical entity

[Term]
id: ECOSIMCONCEPT:NetExchange
name: Net exchange
def: "The total exchange between two regions accounting for transfers in both directions" []
is_a: ECOSIMCONCEPT:Attribute ! attribute

[Term]
id: ECOSIMCONCEPT:Nitrate
name: Nitrate
is_a: ECOSIMCONCEPT:ChemicalEntity ! chemical entity

[Term]
id: ECOSIMCONCEPT:Nitrogen
name: Nitrogen
def: "A colorless, odorless gaseous element constituting about four-fifths of the volume of the atmosphere" []
is_a: ECOSIMCONCEPT:Attribute ! attribute
is_a: ECOSIMCONCEPT:ChemicalEntity ! chemical entity

[Term]
id: ECOSIMCONCEPT:NitrogenCarbonRatio
name: NitrogenCarbonRatio
is_a: ECOSIMCONCEPT:PhysicalEntity ! physical entity

[Term]
id: ECOSIMCONCEPT:NitrogenFixation
name: Nitrogen fixation
def: "The conversion of molecular nitrogen (N2) to ammonia by soil bacteria," []
is_a: ECOSIMCONCEPT:Process ! process

[Term]
id: ECOSIMCONCEPT:NitrogenGas
name: NitrogenGas
is_a: ECOSIMCONCEPT:ChemicalEntity ! chemical entity

[Term]
id: ECOSIMCONCEPT:NitrousOxide
name: NitrousOxide
is_a: ECOSIMCONCEPT:ChemicalEntity ! chemical entity

[Term]
id: ECOSIMCONCEPT:Node
name: Node
is_a: ECOSIMCONCEPT:PlantPart ! plant part

[Term]
id: ECOSIMCONCEPT:NodeElement
name: Node element
def: "A modeled internode section on a plant stem," []
is_a: ECOSIMCONCEPT:Organismal ! organismal

[Term]
id: ECOSIMCONCEPT:NodeInitiation
name: NodeInitiation
is_a: ECOSIMCONCEPT:Process ! process

[Term]
id: ECOSIMCONCEPT:NodeNumber
name: NodeNumber
is_a: ECOSIMCONCEPT:Attribute ! attribute

[Term]
id: ECOSIMCONCEPT:Nodes
name: Nodes
is_a: ECOSIMCONCEPT:PlantPart ! plant part

[Term]
id: ECOSIMCONCEPT:Nodule
name: Nodule
is_a: ECOSIMCONCEPT:PlantPart ! plant part

[Term]
id: ECOSIMCONCEPT:NoduleElement
name: Nodule element
def: "Specialized structures on the roots of some plants that house nitrogen-fixing bacteria," []
is_a: ECOSIMCONCEPT:Organismal ! organismal

[Term]
id: ECOSIMCONCEPT:NonBandRegion
name: NonBandRegion
is_a: ECOSIMCONCEPT:PhysicalEntity ! physical entity

[Term]
id: ECOSIMCONCEPT:NonSaltSolute
name: NonSaltSolute
is_a: ECOSIMCONCEPT:PhysicalEntity ! physical entity

[Term]
id: ECOSIMCONCEPT:NonStructuralC
name: Non-structural carbohydrate
def: "Carbohydrates produced by plants that are not part of supporting structures," []
is_a: ECOSIMCONCEPT:PhysicalEntity ! physical entity

[Term]
id: ECOSIMCONCEPT:NonStructuralElement
name: Non-structural element
def: "A modeled pool of non-structural carbohydrate in a plant," []
is_a: ECOSIMCONCEPT:PhysicalEntity ! physical entity

[Term]
id: ECOSIMCONCEPT:NonstructuralC3Content
name: NonstructuralC3Content
is_a: ECOSIMCONCEPT:PhysicalEntity ! physical entity

[Term]
id: ECOSIMCONCEPT:NonstructuralCarbonTransfer
name: NonstructuralCarbonTransfer
is_a: ECOSIMCONCEPT:Process ! process

[Term]
id: ECOSIMCONCEPT:NonstructuralOrganicCompounds
name: NonstructuralOrganicCompounds
is_a: ECOSIMCONCEPT:PhysicalEntity ! physical entity

[Term]
id: ECOSIMCONCEPT:Number
name: Number
def: "An arithmetical value" []
is_a: ECOSIMCONCEPT:Attribute ! attribute

[Term]
id: ECOSIMCONCEPT:NumericType
name: Numeric type
def: "A data type representing numbers" []
is_a: ECOSIMCONCEPT:Attribute ! attribute

[Term]
id: ECOSIMCONCEPT:Nutrient
name: Nutrient
is_a: ECOSIMCONCEPT:PhysicalEntity ! physical entity

[Term]
id: ECOSIMCONCEPT:O2
name: Dioxygen
def: "A colorless, odorless gas with formula O2 that makes up about 20% of the earth's atmosphere," []
is_a: ECOSIMCONCEPT:ChemicalEntity ! chemical entity

[Term]
id: ECOSIMCONCEPT:OH
name: OH
is_a: ECOSIMCONCEPT:ChemicalEntity ! chemical entity

[Term]
id: ECOSIMCONCEPT:OrganicCarbon
name: OrganicCarbon
is_a: ECOSIMCONCEPT:PhysicalEntity ! physical entity

[Term]
id: ECOSIMCONCEPT:Organismal
name: organismal
subset: upper_level
is_a: ECOSIMCONCEPT:MaterialEntity ! material entity

[Term]
id: ECOSIMCONCEPT:OverlandFlow
name: OverlandFlow
is_a: ECOSIMCONCEPT:PhysicalEntity ! physical entity

[Term]
id: ECOSIMCONCEPT:Oxygen
name: Oxygen
def: "A colorless, odorless reactive gaseous element constituting about one-fifth of the volume of the atmosphere and present in a combined state in nature," []
is_a: ECOSIMCONCEPT:ChemicalEntity ! chemical entity

[Term]
id: ECOSIMCONCEPT:P
name: Phosphorus
def: "A highly reactive, non-metallic chemical element with symbol P and atomic number 15," []
is_a: ECOSIMCONCEPT:ChemicalEntity ! chemical entity

[Term]
id: ECOSIMCONCEPT:PCRatio
name: PCRatio
is_a: ECOSIMCONCEPT:PhysicalEntity ! physical entity

[Term]
id: ECOSIMCONCEPT:PEPCarboxylase
name: Phosphoenolpyruvate carboxylase
def: "An enzyme that catalyzes the addition of carbon dioxide to phosphoenolpyruvate," []
is_a: ECOSIMCONCEPT:ChemicalEntity ! chemical entity

[Term]
id: ECOSIMCONCEPT:PEPCarboxylaseActivity
name: Phosphoenolpyruvate carboxylase activity
def: "The catalytic activity of phosphoenolpyruvate carboxylase," []
is_a: ECOSIMCONCEPT:Process ! process

[Term]
id: ECOSIMCONCEPT:PO4
name: Phosphate
def: "An oxoanion formed of one phosphorus and four oxygen atoms, PO43-," []
is_a: ECOSIMCONCEPT:ChemicalEntity ! chemical entity

[Term]
id: ECOSIMCONCEPT:PO4Band
name: Phosphate band
def: "A layer of phosphate bound to soil particles," []
is_a: ECOSIMCONCEPT:PhysicalEntity ! physical entity

[Term]
id: ECOSIMCONCEPT:PO4band
name: Phosphate band
def: "A layer of phosphate bound to soil particles," []
is_a: ECOSIMCONCEPT:PhysicalEntity ! physical entity

[Term]
id: ECOSIMCONCEPT:Partitioning
name: Partitioning
is_a: ECOSIMCONCEPT:Process ! process

[Term]
id: ECOSIMCONCEPT:Percipitation
name: Percipitation
is_a: ECOSIMCONCEPT:Process ! process

[Term]
id: ECOSIMCONCEPT:Permafrost
name: Permafrost
is_a: ECOSIMCONCEPT:PhysicalEntity ! physical entity

[Term]
id: ECOSIMCONCEPT:Permeability
name: Permeability
def: "The degree to which a material allows fluids to pass through it\" " []
is_a: ECOSIMCONCEPT:Attribute ! attribute

[Term]
id: ECOSIMCONCEPT:PhenologicalProgress
name: PhenologicalProgress
is_a: ECOSIMCONCEPT:Attribute ! attribute

[Term]
id: ECOSIMCONCEPT:Phosphate
name: Phosphate
def: "An oxoanion formed of one phosphorus and four oxygen atoms, PO43-," []
is_a: ECOSIMCONCEPT:ChemicalEntity ! chemical entity

[Term]
id: ECOSIMCONCEPT:Phosphates
name: Phosphates
def: "Salts or esters of phosphoric acid," []
is_a: ECOSIMCONCEPT:PhysicalEntity ! physical entity

[Term]
id: ECOSIMCONCEPT:PhosphorosCarbonRatio
name: PhosphorosCarbonRatio
is_a: ECOSIMCONCEPT:PhysicalEntity ! physical entity

[Term]
id: ECOSIMCONCEPT:PhosphorousCarbonRatio
name: PhosphorousCarbonRatio
is_a: ECOSIMCONCEPT:PhysicalEntity ! physical entity

[Term]
id: ECOSIMCONCEPT:Phosphorus
name: Phosphorus
def: "A highly reactive, non-metallic chemical element with symbol P and atomic number 15," []
is_a: ECOSIMCONCEPT:ChemicalEntity ! chemical entity

[Term]
id: ECOSIMCONCEPT:PhotosyntheticallyActiveRadiation
name: PhotosyntheticallyActiveRadiation
is_a: ECOSIMCONCEPT:PhysicalEntity ! physical entity

[Term]
id: ECOSIMCONCEPT:PhysicalEntity
name: physical entity
subset: upper_level
is_a: ECOSIMCONCEPT:MaterialEntity ! material entity

[Term]
id: ECOSIMCONCEPT:PhysiologicalMaturity
name: PhysiologicalMaturity
is_a: ECOSIMCONCEPT:Attribute ! attribute

[Term]
id: ECOSIMCONCEPT:Plant
name: Plant
def: "A living organism of the kind exemplified by trees, shrubs, herbs, grasses, ferns, and mosses, typically growing in a permanent site, absorbing water and inorganic substances through its roots, and synthesizing nutrients in its leaves by photosynthesis," []
is_a: ECOSIMCONCEPT:Organismal ! organismal

[Term]
id: ECOSIMCONCEPT:PlantBranch
name: PlantBranch
is_a: ECOSIMCONCEPT:Organismal ! organismal

[Term]
id: ECOSIMCONCEPT:PlantElement
name: PlantElement
is_a: ECOSIMCONCEPT:PhysicalEntity ! physical entity

[Term]
id: ECOSIMCONCEPT:PlantLitterfall
name: PlantLitterfall
is_a: ECOSIMCONCEPT:Process ! process

[Term]
id: ECOSIMCONCEPT:PlantMaturity
name: PlantMaturity
is_a: ECOSIMCONCEPT:Attribute ! attribute

[Term]
id: ECOSIMCONCEPT:PlantPart
name: plant part
subset: upper_level
is_a: ECOSIMCONCEPT:Organismal ! organismal

[Term]
id: ECOSIMCONCEPT:PlantWaterStress
name: PlantWaterStress
is_a: ECOSIMCONCEPT:MaterialEntity ! material entity

[Term]
id: ECOSIMCONCEPT:Plants
name: Plants
is_a: ECOSIMCONCEPT:MaterialEntity ! material entity

[Term]
id: ECOSIMCONCEPT:Potassium
name: Potassium
is_a: ECOSIMCONCEPT:MaterialEntity ! material entity

[Term]
id: ECOSIMCONCEPT:PowerFluxDensity
name: Power flux density
def: "The rate of flow of radiant energy per unit area" []
is_a: ECOSIMCONCEPT:Attribute ! attribute

[Term]
id: ECOSIMCONCEPT:Precipitation
name: Precipitation
def: "Rain, snow, sleet, or hail that falls to the ground," []
is_a: ECOSIMCONCEPT:Process ! process

[Term]
id: ECOSIMCONCEPT:Pressure
name: Pressure
def: "Force per unit area applied to an object" []
is_a: ECOSIMCONCEPT:Attribute ! attribute

[Term]
id: ECOSIMCONCEPT:Process
name: process
subset: upper_level

[Term]
id: ECOSIMCONCEPT:ProteinCarbon
name: ProteinCarbon
is_a: ECOSIMCONCEPT:MaterialEntity ! material entity

[Term]
id: ECOSIMCONCEPT:Qualifier
name: qualifier
subset: upper_level

[Term]
id: ECOSIMCONCEPT:Radiation
name: Radiation
is_a: ECOSIMCONCEPT:MaterialEntity ! material entity

[Term]
id: ECOSIMCONCEPT:Rate
name: Rate
def: "A measure of change over time\" " []
is_a: ECOSIMCONCEPT:Attribute ! attribute

[Term]
id: ECOSIMCONCEPT:Reserve
name: Reserve
def: "Something kept back or set aside for future use" []
is_a: ECOSIMCONCEPT:Attribute ! attribute

[Term]
id: ECOSIMCONCEPT:ReserveElement
name: Reserve element
def: "A modeled pool of non-structural carbohydrate reserve in a plant," []
is_a: ECOSIMCONCEPT:PhysicalEntity ! physical entity

[Term]
id: ECOSIMCONCEPT:Root
name: Root
def: "The underground base part of a plant that absorbs water and nutrients," []
is_a: ECOSIMCONCEPT:Organismal ! organismal

[Term]
id: ECOSIMCONCEPT:RootCarbon
name: Root carbon
def: "The carbon in plant root biomass," []
is_a: ECOSIMCONCEPT:PhysicalEntity ! physical entity

[Term]
id: ECOSIMCONCEPT:RootGrowthYield
name: RootGrowthYield
is_a: ECOSIMCONCEPT:MaterialEntity ! material entity

[Term]
id: ECOSIMCONCEPT:RootLayer
name: Root layer
def: "A modeled soil layer containing plant roots," []
is_a: ECOSIMCONCEPT:PhysicalEntity ! physical entity

[Term]
id: ECOSIMCONCEPT:RootNodule
name: Root nodule
def: "A nodular swelling on the root of a legume containing nitrogen-fixing bacteria," []
is_a: ECOSIMCONCEPT:Organismal ! organismal

[Term]
id: ECOSIMCONCEPT:RootZone
name: Root zone
def: "The region of soil explored and influenced by plant roots," []
is_a: ECOSIMCONCEPT:PhysicalEntity ! physical entity

[Term]
id: ECOSIMCONCEPT:RubiscoActivity
name: Rubisco activity
def: "The catalytic activity of the enzyme rubisco in fixing carbon dioxide," []
is_a: ECOSIMCONCEPT:Process ! process

[Term]
id: ECOSIMCONCEPT:RubiscoCarboxylaseActivity
name: RubiscoCarboxylaseActivity
is_a: ECOSIMCONCEPT:MaterialEntity ! material entity

[Term]
id: ECOSIMCONCEPT:RubiscoOxygenase
name: Rubisco oxygenase
def: "The oxygenase function of rubisco that catalyzes photorespiration," []
is_a: ECOSIMCONCEPT:ChemicalEntity ! chemical entity

[Term]
id: ECOSIMCONCEPT:RubiscoOxygenaseActivity
name: Rubisco oxygenase activity
def: "The rate of the oxygenase reaction catalyzed by rubisco that leads to photorespiration," []
is_a: ECOSIMCONCEPT:Process ! process

[Term]
id: ECOSIMCONCEPT:Runoff
name: Runoff
def: "The draining away of water from the surface of an area of land" []
is_a: ECOSIMCONCEPT:Attribute ! attribute
is_a: ECOSIMCONCEPT:PhysicalEntity ! physical entity

[Term]
id: ECOSIMCONCEPT:RunoffSurface
name: RunoffSurface
is_a: ECOSIMCONCEPT:MaterialEntity ! material entity

[Term]
id: ECOSIMCONCEPT:RunoffWater
name: Runoff water
def: "Water draining away from the land surface," []
is_a: ECOSIMCONCEPT:PhysicalEntity ! physical entity

[Term]
id: ECOSIMCONCEPT:SO4
name: SO4
is_a: ECOSIMCONCEPT:MaterialEntity ! material entity

[Term]
id: ECOSIMCONCEPT:Salt
name: Salt
is_a: ECOSIMCONCEPT:MaterialEntity ! material entity

[Term]
id: ECOSIMCONCEPT:Sand
name: Sand
is_a: ECOSIMCONCEPT:MaterialEntity ! material entity

[Term]
id: ECOSIMCONCEPT:SecondaryAxes
name: Secondary axes
def: "Additional axes in a multidimensional array besides the primary axis" []
is_a: ECOSIMCONCEPT:Attribute ! attribute
is_a: ECOSIMCONCEPT:MaterialEntity ! material entity

[Term]
id: ECOSIMCONCEPT:Sediment
name: Sediment
def: "Solid fragments of inorganic or organic material that come from the weathering of rock and are carried and deposited by wind, water, or ice," []
is_a: ECOSIMCONCEPT:PhysicalEntity ! physical entity

[Term]
id: ECOSIMCONCEPT:Seed
name: Seed
is_a: ECOSIMCONCEPT:MaterialEntity ! material entity

[Term]
id: ECOSIMCONCEPT:SeedSet
name: SeedSet
is_a: ECOSIMCONCEPT:MaterialEntity ! material entity

[Term]
id: ECOSIMCONCEPT:SelfShading
name: SelfShading
is_a: ECOSIMCONCEPT:MaterialEntity ! material entity

[Term]
id: ECOSIMCONCEPT:Sheath
name: Sheath
def: "A protective covering such as the lower part of a leaf clasping the stem," []
is_a: ECOSIMCONCEPT:Organismal ! organismal

[Term]
id: ECOSIMCONCEPT:SheathProteinC
name: Sheath protein carbon
def: "The carbon in proteins contained in the sheath structure of cereal crops," []
is_a: ECOSIMCONCEPT:PhysicalEntity ! physical entity

[Term]
id: ECOSIMCONCEPT:Shoot
name: Shoot
is_a: ECOSIMCONCEPT:MaterialEntity ! material entity

[Term]
id: ECOSIMCONCEPT:ShortwaveRadiation
name: ShortwaveRadiation
is_a: ECOSIMCONCEPT:MaterialEntity ! material entity

[Term]
id: ECOSIMCONCEPT:Silt
name: Silt
is_a: ECOSIMCONCEPT:MaterialEntity ! material entity

[Term]
id: ECOSIMCONCEPT:Slope
name: Slope
is_a: ECOSIMCONCEPT:MaterialEntity ! material entity

[Term]
id: ECOSIMCONCEPT:Snow
name: Snow
def: "Atmospheric water vapor frozen into ice crystals and falling in light white flakes or lying on the ground as a white layer," []
is_a: ECOSIMCONCEPT:PhysicalEntity ! physical entity

[Term]
id: ECOSIMCONCEPT:SnowPack
name: SnowPack
is_a: ECOSIMCONCEPT:MaterialEntity ! material entity

[Term]
id: ECOSIMCONCEPT:Snowpack
name: Snowpack
def: "A seasonal accumulation of slow-melting snow," []
is_a: ECOSIMCONCEPT:PhysicalEntity ! physical entity

[Term]
id: ECOSIMCONCEPT:SnowpackRunoff
name: Snowpack runoff
def: "Runoff from melting of the snowpack," []
is_a: ECOSIMCONCEPT:PhysicalEntity ! physical entity

[Term]
id: ECOSIMCONCEPT:Sodium
name: Sodium
is_a: ECOSIMCONCEPT:MaterialEntity ! material entity

[Term]
id: ECOSIMCONCEPT:Soil
name: Soil
def: "The upper layer of earth in which plants grow," []
is_a: ECOSIMCONCEPT:PhysicalEntity ! physical entity

[Term]
id: ECOSIMCONCEPT:SoilBand
name: SoilBand
is_a: ECOSIMCONCEPT:MaterialEntity ! material entity

[Term]
id: ECOSIMCONCEPT:SoilDetachment
name: Soil detachment
def: "The removal of soil particles from the land surface by rainfall, runoff and erosion," []
is_a: ECOSIMCONCEPT:Process ! process

[Term]
id: ECOSIMCONCEPT:SoilHumus
name: Soil humus
def: "The organic component of soil formed by decomposition of plant and animal residues," []
is_a: ECOSIMCONCEPT:PhysicalEntity ! physical entity

[Term]
id: ECOSIMCONCEPT:SoilMacropore
name: SoilMacropore
is_a: ECOSIMCONCEPT:MaterialEntity ! material entity

[Term]
id: ECOSIMCONCEPT:SoilMicropore
name: Soil micropore
def: "A small pore space between soil particles that holds water by capillary forces," []
is_a: ECOSIMCONCEPT:PhysicalEntity ! physical entity

[Term]
id: ECOSIMCONCEPT:SoilSurface
name: Soil surface
def: "The uppermost layer of the land surface" []
is_a: ECOSIMCONCEPT:PhysicalEntity ! physical entity

[Term]
id: ECOSIMCONCEPT:SoilWater
name: Soil water
def: "Water held in the spaces between soil particles" []
is_a: ECOSIMCONCEPT:PhysicalEntity ! physical entity

[Term]
id: ECOSIMCONCEPT:Solute
name: Solute
is_a: ECOSIMCONCEPT:MaterialEntity ! material entity

[Term]
id: ECOSIMCONCEPT:Solution
name: Solution
is_a: ECOSIMCONCEPT:MaterialEntity ! material entity

[Term]
id: ECOSIMCONCEPT:SpecificChemicalElement
name: SpecificChemicalElement
is_a: ECOSIMCONCEPT:MaterialEntity ! material entity

[Term]
id: ECOSIMCONCEPT:Speed
name: Speed
def: "Rate of motion" []
is_a: ECOSIMCONCEPT:Attribute ! attribute

[Term]
id: ECOSIMCONCEPT:SpringLeafout
name: Spring leaf out
def: "The emergence and expansion of new leaves on plants in spring" []
is_a: ECOSIMCONCEPT:Process ! process

[Term]
id: ECOSIMCONCEPT:Stalk
name: Stalk
def: "The stem or main axis of a plant" []
is_a: ECOSIMCONCEPT:Organismal ! organismal

[Term]
id: ECOSIMCONCEPT:StandingDead
name: Standing dead
def: "Dead vegetation remaining upright" []
is_a: ECOSIMCONCEPT:Attribute ! attribute
is_a: ECOSIMCONCEPT:MaterialEntity ! material entity

[Term]
id: ECOSIMCONCEPT:Stem
name: Stem
is_a: ECOSIMCONCEPT:MaterialEntity ! material entity

[Term]
id: ECOSIMCONCEPT:Stoma
name: Stoma
is_a: ECOSIMCONCEPT:MaterialEntity ! material entity

[Term]
id: ECOSIMCONCEPT:StorageCapacity
name: Storage capacity
def: "The maximum amount that can be contained\"  " []
is_a: ECOSIMCONCEPT:Attribute ! attribute

[Term]
id: ECOSIMCONCEPT:Stored
name: Stored
def: "Kept in a location for later use\" " []
is_a: ECOSIMCONCEPT:Attribute ! attribute

[Term]
id: ECOSIMCONCEPT:StressIndicator
name: Stress indicator
def: "A variable indicating the level of stress" []
is_a: ECOSIMCONCEPT:Attribute ! attribute

[Term]
id: ECOSIMCONCEPT:StructuralCarbon
name: StructuralCarbon
is_a: ECOSIMCONCEPT:MaterialEntity ! material entity

[Term]
id: ECOSIMCONCEPT:Structure
name: Structure
def: "Something made up of interconnected elements" []
is_a: ECOSIMCONCEPT:Attribute ! attribute

[Term]
id: ECOSIMCONCEPT:Subsurface
name: Subsurface
def: "Below the surface of the ground" []
is_a: ECOSIMCONCEPT:PhysicalEntity ! physical entity

[Term]
id: ECOSIMCONCEPT:SubsurfaceIrrigation
name: SubsurfaceIrrigation
is_a: ECOSIMCONCEPT:MaterialEntity ! material entity

[Term]
id: ECOSIMCONCEPT:Sun
name: Sun
is_a: ECOSIMCONCEPT:MaterialEntity ! material entity

[Term]
id: ECOSIMCONCEPT:Surface
name: Surface
def: "The outer or topmost layer or area of something" []
is_a: ECOSIMCONCEPT:PhysicalEntity ! physical entity

[Term]
id: ECOSIMCONCEPT:SurfaceAtmosphere
name: Surface atmosphere
def: "The atmospheric layer immediately above the land or water surface" []
is_a: ECOSIMCONCEPT:PhysicalEntity ! physical entity

[Term]
id: ECOSIMCONCEPT:SurfaceIrrigation
name: SurfaceIrrigation
is_a: ECOSIMCONCEPT:MaterialEntity ! material entity

[Term]
id: ECOSIMCONCEPT:SurfaceLitter
name: Surface litter
def: "Dead plant material such as leaves on the ground surface" []
is_a: ECOSIMCONCEPT:PhysicalEntity ! physical entity

[Term]
id: ECOSIMCONCEPT:SurfaceRunoff
name: Surface runoff
def: "Water flowing over land from excess rainfall, snowmelt, or irrigation" []
is_a: ECOSIMCONCEPT:PhysicalEntity ! physical entity

[Term]
id: ECOSIMCONCEPT:SurfaceWater
name: Surface water
def: "Water on the surface of the land, including lakes, rivers, streams, ponds, flooding and runoff" []
is_a: ECOSIMCONCEPT:PhysicalEntity ! physical entity

[Term]
id: ECOSIMCONCEPT:SurfaceWaterBody
name: Surface water body
def: "A natural or artificial lake, pond, reservoir, or other body of water on the land surface" []
is_a: ECOSIMCONCEPT:PhysicalEntity ! physical entity

[Term]
id: ECOSIMCONCEPT:Temperature
name: Temperature
def: "thermal energy in a system" []
is_a: ECOSIMCONCEPT:Attribute ! attribute
is_a: ECOSIMCONCEPT:MaterialEntity ! material entity

[Term]
id: ECOSIMCONCEPT:ThermalAdaptation
name: ThermalAdaptation
is_a: ECOSIMCONCEPT:MaterialEntity ! material entity

[Term]
id: ECOSIMCONCEPT:TopSoil
name: TopSoil
is_a: ECOSIMCONCEPT:MaterialEntity ! material entity

[Term]
id: ECOSIMCONCEPT:TotalEvaporation
name: TotalEvaporation
is_a: ECOSIMCONCEPT:MaterialEntity ! material entity

[Term]
id: ECOSIMCONCEPT:Tracers
name: Tracers
is_a: ECOSIMCONCEPT:MaterialEntity ! material entity

[Term]
id: ECOSIMCONCEPT:UnclassifiedVariable
name: unclassified variable
is_a: ECOSIMCONCEPT:Variable ! variable

[Term]
id: ECOSIMCONCEPT:UndergroundIrrigation
name: UndergroundIrrigation
is_a: ECOSIMCONCEPT:MaterialEntity ! material entity

[Term]
id: ECOSIMCONCEPT:UndergroundIrrigationSystem
name: UndergroundIrrigationSystem
is_a: ECOSIMCONCEPT:MaterialEntity ! material entity

[Term]
id: ECOSIMCONCEPT:Unit
name: unit
subset: upper_level

[Term]
id: ECOSIMCONCEPT:UnitArea
name: UnitArea
is_a: ECOSIMCONCEPT:MaterialEntity ! material entity

[Term]
id: ECOSIMCONCEPT:Uptake
name: Uptake
def: "The absorption or intake of a substance" []
is_a: ECOSIMCONCEPT:Attribute ! attribute

[Term]
id: ECOSIMCONCEPT:UptakeExudation
name: Uptake exudation
def: "The combined processes of uptake and exudation" []
is_a: ECOSIMCONCEPT:Attribute ! attribute

[Term]
id: ECOSIMCONCEPT:UptakeKinetics
name: Uptake kinetics
def: "The dynamics of how a substance is absorbed" []
is_a: ECOSIMCONCEPT:Attribute ! attribute

[Term]
id: ECOSIMCONCEPT:UptakeRate
name: Uptake rate
def: "The rate at which a substance is absorbed" []
is_a: ECOSIMCONCEPT:Attribute ! attribute
is_a: ECOSIMCONCEPT:MaterialEntity ! material entity

[Term]
id: ECOSIMCONCEPT:UptakeVelocity
name: Uptake velocity
def: "The speed at which a substance is absorbed" []
is_a: ECOSIMCONCEPT:Attribute ! attribute

[Term]
id: ECOSIMCONCEPT:Urea
name: Urea
is_a: ECOSIMCONCEPT:MaterialEntity ! material entity

[Term]
id: ECOSIMCONCEPT:UreaFertilizer
name: UreaFertilizer
is_a: ECOSIMCONCEPT:MaterialEntity ! material entity

[Term]
id: ECOSIMCONCEPT:VHeatCap
name: VHeatCap
is_a: ECOSIMCONCEPT:MaterialEntity ! material entity

[Term]
id: ECOSIMCONCEPT:Vapor
name: Vapor
def: "A substance in the gas phase at a temperature lower than its critical temperature" []
is_a: ECOSIMCONCEPT:PhysicalEntity ! physical entity

[Term]
id: ECOSIMCONCEPT:Variable
name: variable
subset: upper_level

[Term]
id: ECOSIMCONCEPT:Volatilization
name: Volatilization
def: "Transition of a substance from liquid to gas" []
is_a: ECOSIMCONCEPT:Attribute ! attribute

[Term]
id: ECOSIMCONCEPT:Volume
name: Volume
def: "Amount of space occupied in three dimensions" []
is_a: ECOSIMCONCEPT:Attribute ! attribute
is_a: ECOSIMCONCEPT:MaterialEntity ! material entity

[Term]
id: ECOSIMCONCEPT:VolumeFraction
name: Volume fraction
def: "Fraction of the total volume occupied\" " []
is_a: ECOSIMCONCEPT:Attribute ! attribute

[Term]
id: ECOSIMCONCEPT:WDPTHD
name: WDPTHD
is_a: ECOSIMCONCEPT:MaterialEntity ! material entity

[Term]
id: ECOSIMCONCEPT:Water
name: Water
def: "A clear, colorless, odorless liquid made up of hydrogen and oxygen that freezes into ice and boils into steam" []
is_a: ECOSIMCONCEPT:PhysicalEntity ! physical entity

[Term]
id: ECOSIMCONCEPT:WaterContent
name: Water content
def: "Amount of water present\" " []
is_a: ECOSIMCONCEPT:Attribute ! attribute

[Term]
id: ECOSIMCONCEPT:WaterDistribution
name: Water distribution
def: "The way water is spread over an area" []
is_a: ECOSIMCONCEPT:Attribute ! attribute

[Term]
id: ECOSIMCONCEPT:WaterFlow
name: WaterFlow
is_a: ECOSIMCONCEPT:MaterialEntity ! material entity

[Term]
id: ECOSIMCONCEPT:WaterFlux
name: Water flux
def: "The rate of flow of water" []
is_a: ECOSIMCONCEPT:Attribute ! attribute
is_a: ECOSIMCONCEPT:MaterialEntity ! material entity

[Term]
id: ECOSIMCONCEPT:WaterHoldingCapacity
name: Water holding capacity
def: "The maximum amount of water that can be held" []
is_a: ECOSIMCONCEPT:Attribute ! attribute

[Term]
id: ECOSIMCONCEPT:WaterTable
name: WaterTable
is_a: ECOSIMCONCEPT:MaterialEntity ! material entity

[Term]
id: ECOSIMCONCEPT:WaterTransfer
name: Water transfer
def: "The movement of water from one place to another" []
is_a: ECOSIMCONCEPT:Attribute ! attribute

[Term]
id: ECOSIMCONCEPT:WaterVapor
name: Water vapor
def: "Water in its gas phase" []
is_a: ECOSIMCONCEPT:PhysicalEntity ! physical entity

[Term]
id: ECOSIMCONCEPT:Width
name: Width
def: "The measurement or extent from side to side" []
is_a: ECOSIMCONCEPT:Attribute ! attribute

[Term]
id: ECOSIMCONCEPT:Wind
name: Wind
def: "The natural movement of air at the Earth's surface" []
is_a: ECOSIMCONCEPT:PhysicalEntity ! physical entity

[Term]
id: ECOSIMCONCEPT:WindSpeed
name: WindSpeed
is_a: ECOSIMCONCEPT:MaterialEntity ! material entity

[Term]
id: ECOSIMCONCEPT:Zone
name: Zone
is_a: ECOSIMCONCEPT:MaterialEntity ! material entity

[Term]
id: http://purl.obolibrary.org/obo/ECOSIMCONCEPT_Ca-NH4_Exchange
name: Ca-NH4_Exchange
is_a: ECOSIMCONCEPT:Process ! process

[Term]
id: http://purl.obolibrary.org/obo/ECOSIMCONCEPT_Ca_Al_Exchange
name: Ca_Al_Exchange
is_a: ECOSIMCONCEPT:MaterialEntity ! material entity

[Term]
id: http://purl.obolibrary.org/obo/ECOSIMCONCEPT_LeafLength_WidthRatio
name: LeafLength_WidthRatio
is_a: ECOSIMCONCEPT:Attribute ! attribute

[Term]
id: http://purl.obolibrary.org/obo/ECOSIMCONCEPT_NO3_Band
name: NO3_Band
is_a: ECOSIMCONCEPT:PhysicalEntity ! physical entity

[Term]
id: http://purl.obolibrary.org/obo/ECOSIMCONCEPT_OH_Minus
name: OH_Minus
is_a: ECOSIMCONCEPT:ChemicalEntity ! chemical entity

[Typedef]
id: attribute
name: attribute
xref: ECOSIM:attribute
range: ECOSIMCONCEPT:Attribute ! attribute

[Typedef]
id: context
name: context
xref: ECOSIM:context
range: ECOSIMCONCEPT:Context ! context

[Typedef]
id: has_unit
name: has unit
xref: ECOSIM:has_unit
domain: ECOSIMCONCEPT:Variable ! variable

[Typedef]
id: measured_in
name: measured in
xref: ECOSIM:measured_in
range: ECOSIMCONCEPT:MaterialEntity ! material entity

[Typedef]
id: measurement_of
name: measurement_of
xref: ECOSIM:measurement_of
range: ECOSIMCONCEPT:MaterialEntity ! material entity

[Typedef]
id: qualifier
name: qualifier
xref: ECOSIM:qualifier
range: ECOSIMCONCEPT:Qualifier ! qualifier

